<?xml version="1.0" encoding="UTF-8"?>
<rdf:RDF xmlns="http://data.europa.eu/a4g/ontology#"
         xmlns:adms="http://www.w3.org/ns/adms#"
         xmlns:at-voc="http://publications.europa.eu/resource/authority/"
         xmlns:at-voc-new="http://publications.europa.eu/resource/authority/new/"
         xmlns:cccev="http://data.europa.eu/m8g/"
         xmlns:core="http://data.europa.eu/m8g/"
         xmlns:cpov="http://data.europa.eu/m8g/"
         xmlns:cpsv="http://data.europa.eu/m8g/"
         xmlns:cpv="http://data.europa.eu/m8g/"
         xmlns:cv="http://data.europa.eu/m8g/"
         xmlns:dc="http://purl.org/dc/elements/1.1/"
         xmlns:dct="http://purl.org/dc/terms/"
         xmlns:dul="http://www.ontologydesignpatterns.org/ont/dul/DUL.owl#"
         xmlns:eli="http://data.europa.eu/eli/ontology#"
         xmlns:epo="http://data.europa.eu/a4g/ontology#"
         xmlns:epo-acc="http://data.europa.eu/a4g/ontology#"
         xmlns:epo-cat="http://data.europa.eu/a4g/ontology#"
         xmlns:epo-con="http://data.europa.eu/a4g/ontology#"
         xmlns:epo-ful="http://data.europa.eu/a4g/ontology#"
         xmlns:epo-inv="http://data.europa.eu/a4g/ontology#"
         xmlns:epo-not="http://data.europa.eu/a4g/ontology#"
         xmlns:epo-ord="http://data.europa.eu/a4g/ontology#"
         xmlns:epo-sub="http://data.europa.eu/a4g/ontology#"
         xmlns:espd="https://github.com/ESPD/ESPD-EDM/"
         xmlns:foaf="http://xmlns.com/foaf/0.1/"
         xmlns:frbroo="http://iflastandards.info/ns/fr/frbr/frbroo/"
         xmlns:geosparql="http://www.opengis.net/ont/geosparql#"
         xmlns:locn="http://www.w3.org/ns/locn#"
         xmlns:nuts="http://data.europa.eu/nuts/"
         xmlns:org="http://www.w3.org/ns/org#"
         xmlns:owl="http://www.w3.org/2002/07/owl#"
         xmlns:person="http://www.w3.org/ns/person#"
         xmlns:rdf="http://www.w3.org/1999/02/22-rdf-syntax-ns#"
         xmlns:rdfs="http://www.w3.org/2000/01/rdf-schema#"
         xmlns:skos="http://www.w3.org/2004/02/skos/core#"
         xmlns:time="http://www.w3.org/2006/time#"
         xmlns:vann="http://purl.org/vocab/vann/"
         xmlns:xsd="http://www.w3.org/2001/XMLSchema#">
   <owl:Ontology rdf:about="http://data.europa.eu/a4g/ontology#acc">
      <owl:imports rdf:resource="http://xmlns.com/foaf/0.1/"/>
      <owl:imports rdf:resource="http://purl.org/dc/terms/"/>
      <owl:imports rdf:resource="http://www.w3.org/ns/org#"/>
      <owl:imports rdf:resource="http://www.w3.org/2004/02/skos/core"/>
      <owl:imports rdf:resource="http://data.europa.eu/a4g/ontology#core"/>
      <owl:imports rdf:resource="http://data.europa.eu/a4g/ontology#sub"/>
      <owl:imports rdf:resource="http://www.w3.org/2006/time"/>
      <owl:imports rdf:resource="http://www.w3.org/ns/locn"/>
      <owl:imports rdf:resource="http://data.europa.eu/m8g/"/>
      <owl:imports rdf:resource="http://data.europa.eu/m8g/"/>
      <owl:imports rdf:resource="http://data.europa.eu/m8g/"/>
      <owl:imports rdf:resource="http://data.europa.eu/m8g/"/>
      <owl:imports rdf:resource="http://data.europa.eu/m8g/"/>
      <owl:imports rdf:resource="http://data.europa.eu/m8g/"/>
      <owl:imports rdf:resource="http://www.w3.org/ns/person"/>
      <owl:imports rdf:resource="http://www.w3.org/ns/adms"/>
      <owl:imports rdf:resource="http://purl.org/vocab/vann/"/>
      <owl:imports rdf:resource="http://data.europa.eu/eli/ontology#"/>
      <owl:imports rdf:resource="http://iflastandards.info/ns/fr/frbr/frbroo/"/>
      <dct:title xml:lang="en">eProcurement Ontology Access - core</dct:title>
      <rdfs:label xml:lang="en">eProcurement Ontology Access - core</rdfs:label>
      <dct:description xml:lang="en">The eProcurement Ontology Access core describes the concepts and properties representing the European Public Procurement Access domain. The provision of these semantics offers the basis for a common understanding of the domain for all stakeholders ensuring the quality of data exchange and transparency. The ontology restrictions are published in a separate artefact.</dct:description>
      <dct:publisher>http://publications.europa.eu/resource/authority/corporate-body/PUBL</dct:publisher>
      <rdfs:comment>This version is automatically generated from eAccess.xml on 2024-07-23</rdfs:comment>
      <rdfs:seeAlso rdf:resource="https://github.com/OP-TED/ePO/releases"/>
      <rdfs:seeAlso rdf:resource="https://joinup.ec.europa.eu/collection/eprocurement/solution/eprocurement-ontology/about"/>
      <rdfs:seeAlso rdf:resource="https://op.europa.eu/en/web/eu-vocabularies/e-procurement"/>
      <rdfs:seeAlso rdf:resource="https://docs.ted.europa.eu/home/index.html"/>
      <dct:issued rdf:datatype="http://www.w3.org/2001/XMLSchema#date">2024-07-23</dct:issued>
      <dct:created rdf:datatype="http://www.w3.org/2001/XMLSchema#date">2021-06-01</dct:created>
      <owl:versionInfo>4.2.0</owl:versionInfo>
      <owl:incompatibleWith>3.1.0</owl:incompatibleWith>
      <owl:versionIRI rdf:resource="http://data.europa.eu/a4g/ontology#acc-4.2.0"/>
      <owl:priorVersion>http://data.europa.eu/a4g/ontology#acc-4.1.0</owl:priorVersion>
      <vann:preferredNamespaceUri>http://data.europa.eu/a4g/ontology#</vann:preferredNamespaceUri>
      <vann:preferredNamespacePrefix>epo</vann:preferredNamespacePrefix>
      <dct:license>Â© European Union, 2014. Unless otherwise noted, the reuse of the Ontology is authorised under the European Union Public Licence v1.2 (https://eupl.eu/).</dct:license>
   </owl:Ontology>
   <owl:Class rdf:about="http://data.europa.eu/m8g/EvidenceType"/>
   <rdf:Description rdf:about="http://data.europa.eu/m8g/EvidenceType">
      <skos:prefLabel xml:lang="en">Evidence type</skos:prefLabel>
   </rdf:Description>
   <rdf:Description rdf:about="http://data.europa.eu/m8g/EvidenceType">
      <skos:definition xml:lang="en">Information about the characteristics of an Evidence. Additional Information: The Evidence Type and the characteristics it describes are not concrete individual responses to a Requirement (i.e. Evidence), but descriptions about the desired form, content, source and/or other characteristics that an actual response should have and provide (e.g. membership of a class of Evidences).</skos:definition>
   </rdf:Description>
   <owl:Class rdf:about="http://data.europa.eu/m8g/EvidenceTypeList"/>
   <rdf:Description rdf:about="http://data.europa.eu/m8g/EvidenceTypeList">
      <skos:prefLabel xml:lang="en">Evidence type list</skos:prefLabel>
   </rdf:Description>
   <rdf:Description rdf:about="http://data.europa.eu/m8g/EvidenceTypeList">
      <skos:definition xml:lang="en">Group of Evidence Types for conforming to a Requirement. Additional Information: An Evidence Type List is satisfied, if and only if, for all included Evidence Types in this List, corresponding conformant Evidence(s) are supporting the Requirement having this List. The Evidence Type List describes thus an AND condition on the different Evidence Types within the list and an OR condition between two or more Evidence Type Lists. Combinations of alternative Lists can be provided for a respondent of a Requirement to choose amongst them.</skos:definition>
   </rdf:Description>
   <owl:Class rdf:about="http://data.europa.eu/eli/ontology#LegalExpression"/>
   <rdf:Description rdf:about="http://data.europa.eu/eli/ontology#LegalExpression">
      <skos:prefLabel xml:lang="en">Legal expression</skos:prefLabel>
   </rdf:Description>
   <rdf:Description rdf:about="http://data.europa.eu/eli/ontology#LegalExpression">
      <skos:definition xml:lang="en">The intellectual realisation of a legal resource in the form of a "sequence of signs" (typically alpha-numeric characters in a legal context). For example, any version of the legal resource whose content is specified and different from others for any reason: language, versions, etc.; Note that ELI ontology accommodates different point of view on what should be considered a new legal resource, or a new legal expression of the same resource. Typically, a consolidated version can be viewed, in the context of ELI, either as separate legal resource (linked to original version and previous consolidated version using corresponding ELI relations), or as a different legal expression of the same legal resource.</skos:definition>
   </rdf:Description>
   <owl:Class rdf:about="http://data.europa.eu/eli/ontology#LegalResource"/>
   <rdf:Description rdf:about="http://data.europa.eu/eli/ontology#LegalResource">
      <skos:prefLabel xml:lang="en">Legal resource</skos:prefLabel>
   </rdf:Description>
   <rdf:Description rdf:about="http://data.europa.eu/eli/ontology#LegalResource">
      <skos:definition xml:lang="en">A work in a legislative corpus. This applies to acts that have been legally enacted (whether or not they are still in force). For example, the abstract concept of the legal resource; e.g. "act 3 of 2005" (adapted from Akoma Ntoso) A legal resource can represent a legal act or any component of a legal act, like an article. Legal resources can be linked together using properties defined in the model. Note that ELI ontology accommodates different point of view on what should be considered a new legal resource, or a new legal expression of the same resource. Typically, a consolidated version can be viewed, in the context of ELI, either as separate legal resource (linked to original version and previous consolidated version using corresponding ELI relations), or as a different legal expression of the same legal resource.</skos:definition>
   </rdf:Description>
   <owl:Class rdf:about="http://data.europa.eu/eli/ontology#LegalResourceSubdivision"/>
   <rdf:Description rdf:about="http://data.europa.eu/eli/ontology#LegalResourceSubdivision">
      <skos:prefLabel xml:lang="en">Legal resource subdivision</skos:prefLabel>
   </rdf:Description>
   <rdf:Description rdf:about="http://data.europa.eu/eli/ontology#LegalResourceSubdivision">
      <skos:definition xml:lang="en">A component of a legal act, at an arbitrary level of precision, like a chapter, an article, an alinea, a paragraph or an list item.</skos:definition>
   </rdf:Description>
   <owl:Class rdf:about="http://data.europa.eu/eli/ontology#Work"/>
   <rdf:Description rdf:about="http://data.europa.eu/eli/ontology#Work">
      <skos:prefLabel xml:lang="en">Work</skos:prefLabel>
   </rdf:Description>
   <rdf:Description rdf:about="http://data.europa.eu/eli/ontology#Work">
      <skos:definition xml:lang="en">Any distinct intellectual creation (i.e., the intellectual content), in the context of ELI. The substance of Work is ideas.</skos:definition>
   </rdf:Description>
   <owl:Class rdf:about="http://data.europa.eu/a4g/ontology#ESPDRequest"/>
   <rdf:Description rdf:about="http://data.europa.eu/a4g/ontology#ESPDRequest">
      <skos:prefLabel xml:lang="en">E s p d request</skos:prefLabel>
   </rdf:Description>
   <rdf:Description rdf:about="http://data.europa.eu/a4g/ontology#ESPDRequest">
      <skos:definition xml:lang="en">An updated self-declaration used by the economic operator as a preliminary evidence in replacement of certificates issued by public authorities or third parties confirming that the economic operator fulfils the Exclusion Grounds and the Selection Criteria set out by the Buyer for a specific Procurement. WG Approval 05/03/2024</skos:definition>
   </rdf:Description>
   <rdf:Description rdf:about="http://data.europa.eu/a4g/ontology#ESPDRequest">
      <rdfs:isDefinedBy rdf:resource="http://data.europa.eu/a4g/ontology#acc"/>
   </rdf:Description>
   <rdfs:Datatype rdf:about="http://www.w3.org/1999/02/22-rdf-syntax-ns#PlainLiteral"/>
   <rdf:Description rdf:about="http://www.w3.org/1999/02/22-rdf-syntax-ns#PlainLiteral">
      <skos:prefLabel xml:lang="en">Plain literal</skos:prefLabel>
   </rdf:Description>
   <rdfs:Datatype rdf:about="http://www.w3.org/2001/XMLSchema#anyURI"/>
   <rdf:Description rdf:about="http://www.w3.org/2001/XMLSchema#anyURI">
      <skos:prefLabel xml:lang="en">Any u r i</skos:prefLabel>
   </rdf:Description>
   <rdfs:Datatype rdf:about="http://www.w3.org/2001/XMLSchema#boolean"/>
   <rdf:Description rdf:about="http://www.w3.org/2001/XMLSchema#boolean">
      <skos:prefLabel xml:lang="en">Boolean</skos:prefLabel>
   </rdf:Description>
   <rdfs:Datatype rdf:about="http://www.w3.org/2001/XMLSchema#date"/>
   <rdf:Description rdf:about="http://www.w3.org/2001/XMLSchema#date">
      <skos:prefLabel xml:lang="en">Date</skos:prefLabel>
   </rdf:Description>
   <rdfs:Datatype rdf:about="http://www.w3.org/2001/XMLSchema#dateTime"/>
   <rdf:Description rdf:about="http://www.w3.org/2001/XMLSchema#dateTime">
      <skos:prefLabel xml:lang="en">Date time</skos:prefLabel>
   </rdf:Description>
   <rdfs:Datatype rdf:about="http://www.w3.org/2001/XMLSchema#decimal"/>
   <rdf:Description rdf:about="http://www.w3.org/2001/XMLSchema#decimal">
      <skos:prefLabel xml:lang="en">Decimal</skos:prefLabel>
   </rdf:Description>
   <rdfs:Datatype rdf:about="http://www.w3.org/2001/XMLSchema#integer"/>
   <rdf:Description rdf:about="http://www.w3.org/2001/XMLSchema#integer">
      <skos:prefLabel xml:lang="en">Integer</skos:prefLabel>
   </rdf:Description>
   <rdf:Description rdf:about="http://data.europa.eu/a4g/ontology#concernsProcedure">
      <skos:editorialNote xml:lang="en">The relations epo-acc:concernsProcedure and epo:refersToProcedure have to refer to the same Procedure.</skos:editorialNote>
   </rdf:Description>
   <owl:Class rdf:about="http://data.europa.eu/eli/ontology#LegalResource">
      <rdfs:subClassOf rdf:resource="http://data.europa.eu/eli/ontology#Work"/>
   </owl:Class>
   <owl:Class rdf:about="http://data.europa.eu/eli/ontology#LegalResourceSubdivision">
      <rdfs:subClassOf rdf:resource="http://data.europa.eu/eli/ontology#LegalResource"/>
   </owl:Class>
   <owl:Class rdf:about="http://data.europa.eu/a4g/ontology#ESPDRequest">
      <rdfs:subClassOf rdf:resource="http://data.europa.eu/a4g/ontology#ProcurementDocument"/>
   </owl:Class>
   <owl:ObjectProperty rdf:about="http://www.w3.org/ns/adms#identifier"/>
   <rdf:Description rdf:about="http://www.w3.org/ns/adms#identifier">
      <skos:prefLabel xml:lang="en">Identifier</skos:prefLabel>
   </rdf:Description>
   <rdf:Description rdf:about="http://www.w3.org/ns/adms#identifier">
      <skos:definition xml:lang="en">Links a resource to an adms:Identifier class. (cccev:EvidenceType -&gt; adms:Identifier (+adms:identifier)) Links a resource to an adms:Identifier class. (cccev:EvidenceTypeList -&gt; adms:Identifier (+adms:identifier))</skos:definition>
   </rdf:Description>
   <owl:ObjectProperty rdf:about="http://data.europa.eu/m8g/validityPeriodConstraint"/>
   <rdf:Description rdf:about="http://data.europa.eu/m8g/validityPeriodConstraint">
      <skos:prefLabel xml:lang="en">Validity period constraint</skos:prefLabel>
   </rdf:Description>
   <rdf:Description rdf:about="http://data.europa.eu/m8g/validityPeriodConstraint">
      <skos:definition xml:lang="en">Temporal condition on the validity period of the Evidence Type. Additional Information: E.g. A Belgian birth evidence is valid for X months after emission. To express constraints on the validity period that must hold when assessing the evidence (e.g. the certificate of good conduct cannot be issued more than 3 months ago), we refer to the Constraint class. (cccev:EvidenceType -&gt; epo:Period (+cccev:validityPeriodConstraint))</skos:definition>
   </rdf:Description>
   <owl:ObjectProperty rdf:about="http://data.europa.eu/m8g/specifiesEvidenceType"/>
   <rdf:Description rdf:about="http://data.europa.eu/m8g/specifiesEvidenceType">
      <skos:prefLabel xml:lang="en">Specifies evidence type</skos:prefLabel>
   </rdf:Description>
   <rdf:Description rdf:about="http://data.europa.eu/m8g/specifiesEvidenceType">
      <skos:definition xml:lang="en">Evidence Type included in this Evidence Type List. (cccev:EvidenceTypeList -&gt; cccev:EvidenceType (+cccev:specifiesEvidenceType))</skos:definition>
   </rdf:Description>
   <owl:ObjectProperty rdf:about="http://purl.org/dc/terms/conformsTo"/>
   <rdf:Description rdf:about="http://purl.org/dc/terms/conformsTo">
      <skos:prefLabel xml:lang="en">Conforms to</skos:prefLabel>
   </rdf:Description>
   <rdf:Description rdf:about="http://purl.org/dc/terms/conformsTo">
      <skos:definition xml:lang="en">An established standard to which the described resource conforms. Additional Information: Examples of characteristics could be the layout or the configuration of the Evidence. (cccev:Evidence -&gt; cccev:EvidenceType (+dct:conformsTo))</skos:definition>
   </rdf:Description>
   <owl:ObjectProperty rdf:about="http://data.europa.eu/m8g/hasEvidenceTypeList"/>
   <rdf:Description rdf:about="http://data.europa.eu/m8g/hasEvidenceTypeList">
      <skos:prefLabel xml:lang="en">Has evidence type list</skos:prefLabel>
   </rdf:Description>
   <rdf:Description rdf:about="http://data.europa.eu/m8g/hasEvidenceTypeList">
      <skos:definition xml:lang="en">Evidence Type List that specifies the Evidence Types that are needed to meet the Requirement. Additional Information: One or several Lists of Evidence Types can support a Requirement. At least one of them must be satisfied by the response to the Requirement. (cccev:Requirement -&gt; cccev:EvidenceTypeList (+cccev:hasEvidenceTypeList))</skos:definition>
   </rdf:Description>
   <owl:ObjectProperty rdf:about="http://data.europa.eu/eli/ontology#jurisdiction"/>
   <rdf:Description rdf:about="http://data.europa.eu/eli/ontology#jurisdiction">
      <skos:prefLabel xml:lang="en">Jurisdiction</skos:prefLabel>
   </rdf:Description>
   <rdf:Description rdf:about="http://data.europa.eu/eli/ontology#jurisdiction">
      <skos:definition xml:lang="en">The jurisdiction from which the legal resource originates. The place identifier can be taken from the Administrative Territorial Unit table published of the EU Publications Office at https://op.europa.eu/en/web/eu-vocabularies/at-dataset/-/resource/dataset/atu. Member States don't have to recreate their own list of values. (eli:LegalExpression -&gt; at-voc:atu (+eli:jurisdiction)) The jurisdiction from which the legal resource originates. The place identifier can be taken from the Administrative Territorial Unit table published of the EU Publications Office at https://op.europa.eu/en/web/eu-vocabularies/at-dataset/-/resource/dataset/atu. Member States don't have to recreate their own list of values. (eli:LegalResource -&gt; at-voc:atu (+eli:jurisdiction))</skos:definition>
   </rdf:Description>
   <owl:ObjectProperty rdf:about="http://data.europa.eu/eli/ontology#is_realized_by"/>
   <rdf:Description rdf:about="http://data.europa.eu/eli/ontology#is_realized_by">
      <skos:prefLabel xml:lang="en">Is_realized_by</skos:prefLabel>
   </rdf:Description>
   <rdf:Description rdf:about="http://data.europa.eu/eli/ontology#is_realized_by">
      <skos:definition xml:lang="en">Relates a work to an expression of this work in the form of a "sequence of signs" (typically alpha-numeric characters in a legal context). Inverse of "realizes". (eli:LegalExpression -&gt; eli:Work (+eli:is_realized_by))</skos:definition>
   </rdf:Description>
   <owl:ObjectProperty rdf:about="http://data.europa.eu/eli/ontology#uri_schema"/>
   <rdf:Description rdf:about="http://data.europa.eu/eli/ontology#uri_schema">
      <skos:prefLabel xml:lang="en">Uri_schema</skos:prefLabel>
   </rdf:Description>
   <rdf:Description rdf:about="http://data.europa.eu/eli/ontology#uri_schema">
      <skos:definition xml:lang="en">Schema describing the URI of an ELI instance. ELI uses URI template specifications (IETF RFC 6570). Schemes should be associated with member states and will be published in a registry. (eli:LegalExpression -&gt; adms:Identifier (+eli:uri_schema)) Schema describing the URI of an ELI instance. ELI uses URI template specifications (IETF RFC 6570). Schemes should be associated with member states and will be published in a registry. (eli:LegalResourceSubdivision -&gt; adms:Identifier (+eli:uri_schema))</skos:definition>
   </rdf:Description>
   <owl:ObjectProperty rdf:about="http://purl.org/dc/terms/language"/>
   <rdf:Description rdf:about="http://purl.org/dc/terms/language">
      <skos:prefLabel xml:lang="en">Language</skos:prefLabel>
   </rdf:Description>
   <rdf:Description rdf:about="http://purl.org/dc/terms/language">
      <skos:definition xml:lang="en">A language of the resource. (eli:LegalExpression -&gt; at-voc:language (+dct:language))</skos:definition>
   </rdf:Description>
   <owl:ObjectProperty rdf:about="http://data.europa.eu/a4g/ontology#hasResourceType"/>
   <rdf:Description rdf:about="http://data.europa.eu/a4g/ontology#hasResourceType">
      <skos:prefLabel xml:lang="en">Has resource type</skos:prefLabel>
   </rdf:Description>
   <rdf:Description rdf:about="http://data.europa.eu/a4g/ontology#hasResourceType">
      <rdfs:isDefinedBy rdf:resource="http://data.europa.eu/a4g/ontology#acc"/>
   </rdf:Description>
   <owl:ObjectProperty rdf:about="http://data.europa.eu/m8g/isDerivedFrom"/>
   <rdf:Description rdf:about="http://data.europa.eu/m8g/isDerivedFrom">
      <skos:prefLabel xml:lang="en">Is derived from</skos:prefLabel>
   </rdf:Description>
   <rdf:Description rdf:about="http://data.europa.eu/m8g/isDerivedFrom">
      <skos:definition xml:lang="en">Reference Framework on which the Requirement is based, such as a law or regulation. Additional Information: The relation between a parent Requirement and a sub-Requirement can be complex. Therefore, qualified relations (see hasQualifiedRelation) can be used to represent this relationship on its own and qualify it with additional information such as a date, a place. This is left to implementers. In the case where the purpose is to link the two Requirements without additional information, the simple relationship as proposed here can be directly used. (cccev:Requirement -&gt; eli:LegalResource (+cccev:isDerivedFrom))</skos:definition>
   </rdf:Description>
   <owl:ObjectProperty rdf:about="http://data.europa.eu/a4g/ontology#hasSubdivision"/>
   <rdf:Description rdf:about="http://data.europa.eu/a4g/ontology#hasSubdivision">
      <skos:prefLabel xml:lang="en">Has subdivision</skos:prefLabel>
   </rdf:Description>
   <rdf:Description rdf:about="http://data.europa.eu/a4g/ontology#hasSubdivision">
      <rdfs:isDefinedBy rdf:resource="http://data.europa.eu/a4g/ontology#acc"/>
   </rdf:Description>
   <owl:ObjectProperty rdf:about="http://purl.org/dc/terms/isPartOf"/>
   <rdf:Description rdf:about="http://purl.org/dc/terms/isPartOf">
      <skos:prefLabel xml:lang="en">Is part of</skos:prefLabel>
   </rdf:Description>
   <rdf:Description rdf:about="http://purl.org/dc/terms/isPartOf">
      <skos:definition xml:lang="en">A related resource in which the described resource is physically or logically included. (eli:Work -&gt; eli:Work (+dct:isPartOf))</skos:definition>
   </rdf:Description>
   <owl:ObjectProperty rdf:about="http://data.europa.eu/a4g/ontology#specifiesProcurementCriterion"/>
   <rdf:Description rdf:about="http://data.europa.eu/a4g/ontology#specifiesProcurementCriterion">
      <skos:prefLabel xml:lang="en">Specifies procurement criterion</skos:prefLabel>
   </rdf:Description>
   <rdf:Description rdf:about="http://data.europa.eu/a4g/ontology#specifiesProcurementCriterion">
      <rdfs:isDefinedBy rdf:resource="http://data.europa.eu/a4g/ontology#acc"/>
   </rdf:Description>
   <owl:ObjectProperty rdf:about="http://data.europa.eu/a4g/ontology#refersToNotice"/>
   <rdf:Description rdf:about="http://data.europa.eu/a4g/ontology#refersToNotice">
      <skos:prefLabel xml:lang="en">Refers to notice</skos:prefLabel>
   </rdf:Description>
   <rdf:Description rdf:about="http://data.europa.eu/a4g/ontology#refersToNotice">
      <skos:definition xml:lang="en">Reference to a Notice. WG approval 12/03/2024 (epo-acc:ESPDRequest -&gt; epo:Notice (+epo-acc:refersToNotice))</skos:definition>
   </rdf:Description>
   <rdf:Description rdf:about="http://data.europa.eu/a4g/ontology#refersToNotice">
      <rdfs:isDefinedBy rdf:resource="http://data.europa.eu/a4g/ontology#acc"/>
   </rdf:Description>
   <owl:ObjectProperty rdf:about="http://data.europa.eu/a4g/ontology#concernsProcedure"/>
   <rdf:Description rdf:about="http://data.europa.eu/a4g/ontology#concernsProcedure">
      <skos:prefLabel xml:lang="en">Concerns procedure</skos:prefLabel>
   </rdf:Description>
   <rdf:Description rdf:about="http://data.europa.eu/a4g/ontology#concernsProcedure">
      <skos:definition xml:lang="en">Relates to Procedure. WG approval 05/03/2024 (epo-acc:ESPDRequest -&gt; epo:Procedure (+epo:concernsProcedure))</skos:definition>
   </rdf:Description>
   <rdf:Description rdf:about="http://data.europa.eu/a4g/ontology#concernsProcedure">
      <rdfs:isDefinedBy rdf:resource="http://data.europa.eu/a4g/ontology#acc"/>
   </rdf:Description>
   <owl:ObjectProperty rdf:about="http://data.europa.eu/a4g/ontology#relatesToESPDRequest"/>
   <rdf:Description rdf:about="http://data.europa.eu/a4g/ontology#relatesToESPDRequest">
      <skos:prefLabel xml:lang="en">Relates to e s p d request</skos:prefLabel>
   </rdf:Description>
   <rdf:Description rdf:about="http://data.europa.eu/a4g/ontology#relatesToESPDRequest">
      <skos:definition xml:lang="en">Is about an European Single Procurement Document (ESPD) Request. WG approval 05/03/2024 (epo-sub:ESPD -&gt; epo-acc:ESPDRequest (+epo-sub:relatesToESPDRequest))</skos:definition>
   </rdf:Description>
   <rdf:Description rdf:about="http://data.europa.eu/a4g/ontology#relatesToESPDRequest">
      <rdfs:isDefinedBy rdf:resource="http://data.europa.eu/a4g/ontology#acc"/>
   </rdf:Description>
   <owl:DatatypeProperty rdf:about="http://www.w3.org/2004/02/skos/core#prefLabel"/>
   <rdf:Description rdf:about="http://www.w3.org/2004/02/skos/core#prefLabel">
      <skos:prefLabel xml:lang="en">Pref label</skos:prefLabel>
   </rdf:Description>
   <rdf:Description rdf:about="http://www.w3.org/2004/02/skos/core#prefLabel">
      <skos:definition xml:lang="en">The preferred lexical label for a resource, in a given language. WG approval 30/05/2023 (cccev:EvidenceTypeList)</skos:definition>
   </rdf:Description>
   <owl:DatatypeProperty rdf:about="http://purl.org/dc/terms/description"/>
   <rdf:Description rdf:about="http://purl.org/dc/terms/description">
      <skos:prefLabel xml:lang="en">Description</skos:prefLabel>
   </rdf:Description>
   <rdf:Description rdf:about="http://purl.org/dc/terms/description">
      <skos:definition xml:lang="en">An account of the resource. Additional Information: Description may include but is not limited to: an abstract, a table of contents, a graphical representation, or a free-text account of the resource. WG Approval 30/05/2023 (cccev:EvidenceTypeList) An account of the resource. Additional Information: Description may include but is not limited to: an abstract, a table of contents, a graphical representation, or a free-text account of the resource. WG Approval 30/05/2023 (eli:LegalExpression) An account of the resource. Additional Information: Description may include but is not limited to: an abstract, a table of contents, a graphical representation, or a free-text account of the resource. WG Approval 30/05/2023 (eli:LegalResource)</skos:definition>
   </rdf:Description>
   <owl:DatatypeProperty rdf:about="http://data.europa.eu/eli/ontology#number"/>
   <rdf:Description rdf:about="http://data.europa.eu/eli/ontology#number">
      <skos:prefLabel xml:lang="en">Number</skos:prefLabel>
   </rdf:Description>
   <rdf:Description rdf:about="http://data.europa.eu/eli/ontology#number">
      <skos:definition xml:lang="en">An identifier or other disambiguating feature for a legal resource or legal expression. This can be the number of a legislation, the number of an article, or the issue number of an official journal. (eli:LegalExpression) An identifier or other disambiguating feature for a legal resource or legal expression. This can be the number of a legislation, the number of an article, or the issue number of an official journal. (eli:LegalResource)</skos:definition>
   </rdf:Description>
   <owl:DatatypeProperty rdf:about="http://purl.org/dc/terms/identifier"/>
   <rdf:Description rdf:about="http://purl.org/dc/terms/identifier">
      <skos:prefLabel xml:lang="en">Identifier</skos:prefLabel>
   </rdf:Description>
   <rdf:Description rdf:about="http://purl.org/dc/terms/identifier">
      <skos:definition xml:lang="en">An unambiguous reference to the resource within a given context. (eli:LegalExpression) An unambiguous reference to the resource within a given context. (eli:LegalResource)</skos:definition>
   </rdf:Description>
   <owl:ObjectProperty rdf:about="http://purl.org/dc/terms/title"/>
   <rdf:Description rdf:about="http://purl.org/dc/terms/title">
      <skos:prefLabel xml:lang="en">Title</skos:prefLabel>
   </rdf:Description>
   <rdf:Description rdf:about="http://purl.org/dc/terms/title">
      <skos:definition xml:lang="en">A name given to the resource. (eli:LegalExpression)</skos:definition>
   </rdf:Description>
</rdf:RDF>
