@prefix : <http://data.europa.eu/a4g/ontology#> .
@prefix adms: <http://www.w3.org/ns/adms#> .
@prefix cccev: <http://data.europa.eu/m8g/> .
@prefix dcterms: <http://purl.org/dc/terms/> .
@prefix eli: <http://data.europa.eu/eli/ontology#> .
@prefix foaf: <http://xmlns.com/foaf/0.1/> .
@prefix frbroo: <http://iflastandards.info/ns/fr/frbr/frbroo/> .
@prefix locn: <http://www.w3.org/ns/locn#> .
@prefix org: <http://www.w3.org/ns/org#> .
@prefix owl: <http://www.w3.org/2002/07/owl#> .
@prefix person: <http://www.w3.org/ns/person#> .
@prefix rdf: <http://www.w3.org/1999/02/22-rdf-syntax-ns#> .
@prefix rdfs: <http://www.w3.org/2000/01/rdf-schema#> .
@prefix skos: <http://www.w3.org/2004/02/skos/core#> .
@prefix time: <http://www.w3.org/2006/time#> .
@prefix vann: <http://purl.org/vocab/vann/> .
@prefix xsd: <http://www.w3.org/2001/XMLSchema#> .

:AccessTerm a owl:Class ;
    rdfs:isDefinedBy :core ;
    rdfs:subClassOf :LotSpecificTerm,
        :ProcedureSpecificTerm ;
    skos:definition "Conditions and stipulations about where and how to access the Procurement Documents. WG Approval 09/03/2021"@en ;
    skos:prefLabel "Access term"@en .

:AcquiringCentralPurchasingBody a owl:Class ;
    rdfs:isDefinedBy :core ;
    rdfs:subClassOf :CentralPurchasingBody ;
    skos:definition "Role of an Agent procuring activities conducted on a permanent basis in the form of the acquisition of supplies and/or services intended for other Buyers. Additional Information: In Public Procurement the Role of Acquiring Central Purchasing Body is carried out by a Central Purchasing Body for other Contracting Authorities. WG approval 05/08/2021"@en ;
    skos:prefLabel "Acquiring central purchasing body"@en .

:AdHocChannel a owl:Class ;
    rdfs:isDefinedBy :core ;
    rdfs:subClassOf cccev:Channel ;
    skos:definition "Web page where tools and devices for electronic communication that are not generally available can be downloaded free of charge. Additional Information: This corresponds in eForms to BT-724 Tool Atypical. WG Acceptance 10/01/2023"@en ;
    skos:prefLabel "Ad hoc channel"@en .

:AuxiliaryParty a owl:Class ;
    rdfs:isDefinedBy :core ;
    rdfs:subClassOf :AgentInRole ;
    skos:definition "Role of an Agent who may be mentioned in the information exchanged during the Procurement Process but who does not play an active part in it."@en ;
    skos:prefLabel "Auxiliary party"@en .

:AwardCriteriaSummary a owl:Class ;
    rdfs:isDefinedBy :core ;
    rdfs:subClassOf :ProcurementCriteriaSummary ;
    skos:definition "Overview of the Award Criteria. WG approval 19/03/2024"@en ;
    skos:prefLabel "Award criteria summary"@en .

:AwardCriterion a owl:Class ;
    rdfs:isDefinedBy :core ;
    rdfs:subClassOf :ProcurementCriterion ;
    skos:definition "Criterion that describes a Requirement that the Tender needs to resolve and on which the Tender is evaluated and ranked. WG approval 05/11/2018"@en ;
    skos:prefLabel "Award criterion"@en .

:AwardDecision a owl:Class ;
    rdfs:isDefinedBy :core ;
    rdfs:subClassOf :Document ;
    skos:definition "Resolution of the Buyer as to the result of the Procurement Procedure. WG approval 14/11/2018"@en ;
    skos:prefLabel "Award decision"@en .

:AwardEvaluationTerm a owl:Class ;
    rdfs:isDefinedBy :core ;
    rdfs:subClassOf :EvaluationTerm ;
    skos:definition "Conditions and stipulations defining particularities of the evaluation of Award Criteria."@en ;
    skos:prefLabel "Award evaluation term"@en .

:Awarder a owl:Class ;
    rdfs:isDefinedBy :core ;
    rdfs:subClassOf :AcquiringParty ;
    skos:definition "A Role of an Agent that signs the Award Decision. Additional information: BT-08 can be Awarding CBP; BG-03 is the Buyer. But Awarding CPB is not the same as the Buyer; the organisations may differ for these roles. Having the Awarder Role allows us to specify which Organisation is involved in the Award Decision."@en ;
    skos:prefLabel "Awarder"@en .

:AwardingCentralPurchasingBody a owl:Class ;
    rdfs:isDefinedBy :core ;
    rdfs:subClassOf :CentralPurchasingBody ;
    skos:definition "Role of an Agent procuring activities conducted on a permanent basis in the form of the award of Public Contracts or the conclusion of Framework Agreements for works, supplies or services intended for other Buyers. Additional Information: In Public Procurement the Role of Awarding Central purchasing Body is carried out by a Central Purchasing Body for other Contracting Authorities. WG approval 05/08/2021"@en ;
    skos:prefLabel "Awarding central purchasing body"@en .

:BudgetProvider a owl:Class ;
    rdfs:isDefinedBy :core ;
    rdfs:subClassOf :AcquiringParty ;
    skos:definition "A role of an agent whose Budget is used to pay for the Contract."@en ;
    skos:prefLabel "Budget provider"@en .

:Business a owl:Class ;
    rdfs:isDefinedBy :core ;
    rdfs:subClassOf org:Organization ;
    skos:definition "A private law company registered in a national registry. WG Approval 28/04/2020"@en ;
    skos:prefLabel "Business"@en .

:Candidate a owl:Class ;
    rdfs:isDefinedBy :core ;
    rdfs:subClassOf :OfferingParty ;
    skos:definition "The Role of an Agent that has sought an invitation or has been invited to take part in a restricted Procedure, in a competitive Procedure with negotiation, in a negotiated Procedure without prior publication, in a competitive dialogue or in an innovation partnership. WG approval 30/05/2023"@en ;
    skos:prefLabel "Candidate"@en .

:CatalogueProvider a owl:Class ;
    rdfs:isDefinedBy :core ;
    rdfs:subClassOf :OfferingParty ;
    skos:definition "A Role of an Agent compiling and supplying a Catalogue. Additional Information: The Catalogue Provider Role is usually played by the Agent that acts as a Seller, or by another Agent that acts on behalf of the Seller. WG Approval 28/01/2021"@en ;
    skos:prefLabel "Catalogue provider"@en .

:CatalogueReceiver a owl:Class ;
    rdfs:isDefinedBy :core ;
    rdfs:subClassOf :AcquiringParty ;
    skos:definition "A Role of an Agent processing a Catalogue. Additional Information: The Catalogue Receiver may not only receive it but also validate it, process it, etc. The Catalogue Receiver role is usually played by the agent that acts as a Buyer, or by another Agent that acts on behalf of the Buyer. WG Approval 28/01/2021"@en ;
    skos:prefLabel "Catalogue receiver"@en .

:Certificate a owl:Class ;
    rdfs:isDefinedBy :core ;
    rdfs:subClassOf cccev:Evidence ;
    skos:definition "Proof of conformance of the instance of the concept to a defined set of criteria. Additional Information: Certificates provide assurance of credibility, trust, and transparency in the procurement process. WG approval 16/05/2023"@en ;
    skos:prefLabel "Certificate"@en .

:CertificationLabel a owl:Class ;
    rdfs:isDefinedBy :core ;
    rdfs:subClassOf cccev:InformationConcept ;
    skos:definition "Concept that stands for a set of norms, expectations, standards and policies. Additional Information: Such standards may relate to social, ethical and quality etc. WG approval 26/07/2022"@en ;
    skos:prefLabel "Certification label"@en .

:Certifier a owl:Class ;
    rdfs:isDefinedBy :core ;
    skos:definition "The role of an agent who issues a certificate. Additional Information: The certifier is responsible for verifying and confirming the conformance of the instance of the concept to a defined set of criteria. WG approval 16/05/2023"@en ;
    skos:prefLabel "Certifier"@en .

:ChangeInformation a owl:Class ;
    rdfs:isDefinedBy :core ;
    rdfs:subClassOf :ContextDescription ;
    skos:definition "Alteration to previously provided details."@en ;
    skos:editorialNote "Added hasAdditionalInformation to cover for section VII.2 in F14, since we do not have the Corrigendum notice type anymore in eForms."@en ;
    skos:prefLabel "Change information"@en .

:ConcessionContract a owl:Class ;
    rdfs:isDefinedBy :core ;
    rdfs:subClassOf :Contract ;
    skos:definition "A Contract between one or more Buyers and one or more Economic Operators giving the right to the Economic Operators to exploit the rights foreseen in the Contract which may include the receipt of Payments. WG Approval 24/05/2022"@en ;
    skos:prefLabel "Concession contract"@en .

:ConcessionEstimate a owl:Class ;
    rdfs:isDefinedBy :core ;
    rdfs:subClassOf :Estimate ;
    skos:definition "Approximation concerning the foreseen Concession Contract. WG approval 19/03/2024"@en ;
    skos:prefLabel "Concession estimate"@en .

:ContractLotCompletionInformation a owl:Class ;
    rdfs:isDefinedBy :core ;
    rdfs:subClassOf :ContextDescription ;
    skos:definition "Information related to a given Lot at the end of the procurement."@en ;
    skos:prefLabel "Contract lot completion information"@en .

:ContractTerm a owl:Class ;
    rdfs:isDefinedBy :core ;
    rdfs:subClassOf :ContractSpecificTerm ;
    skos:definition "Conditions and stipulations defining particularities of the Post Award Phase. (WG approval 23/11/2018)"@en ;
    skos:prefLabel "Contract term"@en .

:Contractor a owl:Class ;
    rdfs:isDefinedBy :core ;
    rdfs:subClassOf :OfferingParty ;
    skos:definition "The Role of an Agent that has signed a Contract with a Buyer. WG approval 08/11/2022"@en ;
    skos:prefLabel "Contractor"@en .

:DesignContestRegimeTerm a owl:Class ;
    rdfs:isDefinedBy :core ;
    rdfs:subClassOf :LotSpecificTerm,
        :ProcedureSpecificTerm ;
    skos:definition "Conditions and stipulations defining particularities of a Design Contest. WG approval: 04-02-2021"@en ;
    skos:prefLabel "Design contest regime term"@en .

:DirectAwardTerm a owl:Class ;
    rdfs:isDefinedBy :core ;
    rdfs:subClassOf :ProcedureSpecificTerm ;
    skos:definition "Conditions and stipulations defining particularities of the award of a Contract without prior publication. Addtional Information: Direct award may refer to a previous Procedure and/or specific Lot(s). It may also refer to other justified situations whereby there is no previous Procedure. See Directive 2014/24/EU Article 32. WG Approval 22/11/2019"@en ;
    skos:prefLabel "Direct award term"@en .

:DirectContract a owl:Class ;
    rdfs:isDefinedBy :core ;
    rdfs:subClassOf :Contract ;
    skos:definition "A Contract resulting from Lot Award Outcome. Additional information: A Framework Agreement is not a Direct Contract. WG approval 19/03/2024"@en ;
    skos:prefLabel "Direct contract"@en .

:DynamicPurchaseSystemTechnique a owl:Class ;
    rdfs:isDefinedBy :core ;
    rdfs:subClassOf :Technique ;
    skos:definition "A Technique that allows the selection of Candidates throughout the Procedure via the Qualification Criteria, followed by individual Mini-Competitions for the Award of Purchase Contracts. WG approval 23/05/2023"@en ;
    skos:prefLabel "Dynamic purchase system technique"@en .

:EAuctionTechnique a owl:Class ;
    rdfs:isDefinedBy :core ;
    rdfs:subClassOf :Technique ;
    skos:definition "A repetitive Technique in which new Prices, revised downwards, and/or new values concerning certain elements of Tenders are bid on-line. Additional Information: This corresponds in eForms to BT-767 Electronic Auction . WG approval 20/07/2018"@en ;
    skos:prefLabel "E auction technique"@en .

:EconomicStandingSummary a owl:Class ;
    rdfs:isDefinedBy :core ;
    rdfs:subClassOf :SelectionCriteriaSummary ;
    skos:definition "Overview of the financial viability of the economic operator. WG approval 19/03/2024"@en ;
    skos:prefLabel "Economic standing summary"@en .

:ElectronicSignature a owl:Class ;
    rdfs:isDefinedBy :core ;
    skos:definition "Data in electronic form which is attached to or logically associated with other data in electronic form and which is used by the signatory to sign. Additional information: The definition comes from REGULATION (EU) No 910/2014. WG approval 19/03/2024"@en ;
    skos:prefLabel "Electronic signature"@en .

:EmploymentInformationProvider a owl:Class ;
    rdfs:isDefinedBy :core ;
    skos:definition "A Role of an Agent responsible for providing information concerning the general regulatory framework for employment protection and working conditions."@en ;
    skos:prefLabel "Employment information provider"@en .

:EnvironmentalProtectionInformationProvider a owl:Class ;
    rdfs:isDefinedBy :core ;
    skos:definition "A Role of an Agent responsible for providing information concerning the general regulatory framework for Environmental Protection."@en ;
    skos:prefLabel "Environmental protection information provider"@en .

:ExclusionGround a owl:Class ;
    rdfs:isDefinedBy :core ;
    rdfs:subClassOf :QualificationCriterion ;
    skos:definition "Criterion that describes a legal Requirement to be met by the Economic Operator to be a Candidate in the Procurement. Additional Information: This corresponds in eForms to BG-701 Exclusion Grounds. WG approval 31/10/2018"@en ;
    skos:prefLabel "Exclusion ground"@en .

:ExclusionGroundsSummary a owl:Class ;
    rdfs:isDefinedBy :core ;
    rdfs:subClassOf :QualificationCriteriaSummary ;
    skos:definition "Overview of the Exclusion Grounds. WG approval 19/03/2024"@en ;
    skos:prefLabel "Exclusion grounds summary"@en .

:ExpressionOfInterest a owl:Class ;
    rdfs:isDefinedBy :core ;
    rdfs:subClassOf :Document ;
    skos:definition "Document presenting an Economic Operator's Request to be considered for Procedures covering a specific domain. WG approval 13/04/2021"@en ;
    skos:prefLabel "Expression of interest"@en .

:FrameworkAgreement a owl:Class ;
    rdfs:isDefinedBy :core ;
    rdfs:subClassOf :Contract ;
    skos:definition "An agreement between one or more Contracting Authorities and one or more Economic Operators. Additional Information: When a Framework Agreement is concerned, the FA will result from LotAwardOutcome which describes a Lot which specifies the both the Qualification and Award Criteria. WG approval 18/05/2021"@en ;
    skos:prefLabel "Framework agreement"@en .

:FrameworkAgreementTechnique a owl:Class ;
    rdfs:isDefinedBy :core ;
    rdfs:subClassOf :Technique ;
    skos:definition "Technique that establishes the terms governing Contracts to be awarded during a given Period, in particular with regard to Price and, where appropriate, the Quantity envisaged. WG approval 18/05/2021"@en ;
    skos:prefLabel "Framework agreement technique"@en .

:FrameworkAgreementTerm a owl:Class ;
    rdfs:isDefinedBy :core ;
    rdfs:subClassOf :ContractSpecificTerm,
        :LotSpecificTerm,
        :ProcedureSpecificTerm ;
    skos:definition "Conditions and stipulations defining particularities in a Framework Agreement."@en ;
    skos:prefLabel "Framework agreement term"@en .

:Fund a owl:Class ;
    rdfs:isDefinedBy :core ;
    skos:definition "A financial resource used to support the Procurement. Additional Information: In the context of EU, Funds can be divided into programmes, actions and projects. Examples of EU funds are: the European Structural and Investment Funds, European Social Fund (ESF), the Connecting Europe Facility (CEF) programme, or the ISA2 programme and its actions (e.g. Action 2016.05 European Public Procurement Initiative, which supports the eProcurement Ontology under sub-action 3). Funds may change between the lot and the contract, for example in the case of an emergency crisis, a contract may be financed by a budget that was not foreseen in the call. WG Approved 14/05/2019"@en ;
    skos:prefLabel "Fund"@en .

:GreenProcurement a owl:Class ;
    rdfs:isDefinedBy :core ;
    rdfs:subClassOf :StrategicProcurement ;
    skos:definition "Approach whereby Buyers seek to procure with a reduced Environmental Impact. Additional Information: The approach may apply to the complete life cycle. The reduced Environmental Impact is in comparison to goods, services and works with the same primary function that would otherwise be procured. Tightly related are article 68 - Life-cycle costing and article 67 - most economically advantageous Tender (see GPP handbook) https://ec.europa.eu/environment/gpp/pdf/Buying-Green-Handbook-3rd-Edition.pdf An instance of the class GreenProcurement is represented in eForms with the code \"env-imp\" defined in the codelist Strategic-Procurement.Paragraphs) https://ec.europa.eu/environment/gpp/pdf/Buying-Green-Handbook-3rd-Edition.pdf"@en ;
    skos:prefLabel "Green procurement"@en .

:IndefiniteDuration a owl:Class ;
    rdfs:isDefinedBy :core ;
    rdfs:subClassOf :Duration ;
    skos:definition "A Duration without a fixed end date. WG approval 19/03/2024"@en ;
    skos:editorialNote "it cannot be a specialization of the Duration. proposal to be deprecated in 5.0.0; needs further investigation."@en ;
    skos:prefLabel "Indefinite duration"@en .

:InnovativeProcurement a owl:Class ;
    rdfs:isDefinedBy :core ;
    rdfs:subClassOf :StrategicProcurement ;
    skos:definition "Approach whereby Buyers seek to procure an innovative work, supply or service. Additional Information: ‘innovation’ means the implementation of a new or significantly improved product, service or process, including but not limited to production, building or construction processes, a new marketing method, or a new organizational method in business practices, workplace Organisation or external relations inter alia with the purpose of helping to solve societal challenges or to support the Europe 2020 strategy for smart, sustainable and inclusive growth; See: Directive 2014/24 Articles: 2, 26 (3), 31, 67 (2.a)"@en ;
    skos:prefLabel "Innovative procurement"@en .

:JuryMember a owl:Class ;
    rdfs:isDefinedBy :core ;
    rdfs:subClassOf :AcquiringParty ;
    skos:definition "Role of an Agent who evaluates a design contest. WG approval 19/03/2024"@en ;
    skos:prefLabel "Jury member"@en .

:LeadBuyer a owl:Class ;
    rdfs:isDefinedBy :core ;
    rdfs:subClassOf :Buyer ;
    skos:definition "A Role of an Agent who is a Buyer and takes the administrative lead of the Procedure. WG agreement: 2022-11-22"@en ;
    skos:prefLabel "Lead buyer"@en .

:Lot a owl:Class ;
    rdfs:isDefinedBy :core ;
    rdfs:subClassOf :ProcurementObject ;
    skos:definition "A qualitative, quantitative or strategic subdivision of the goods, services or works to be procured, allowing the award of one or more Contracts. WG approval 12/09/2018"@en ;
    skos:prefLabel "Lot"@en .

:LotAwardOutcome a owl:Class ;
    rdfs:isDefinedBy :core ;
    rdfs:subClassOf :AwardOutcome ;
    skos:definition "Result concerning the Lot that was attributed by the Awarder. WG approval 19/03/2024"@en ;
    skos:prefLabel "Lot award outcome"@en .

:LotGroup a owl:Class ;
    rdfs:isDefinedBy :core ;
    skos:definition "Combination of several Lots to conduct comparative assessment of the Tenders. Additional Information: The comparative assessment may refer to the Selection Criteria, Award and Value that apply to several Lots. Pending of discussion with eForms Member States may provide that, where more than one lot may be awarded to the same tenderer, contracting authorities may award contracts combining several or all lots where they have specified in the contract notice or in the invitation to confirm interest that they reserve the possibility of doing so and indicate the lots or groups of lots that may be combined."@en ;
    skos:prefLabel "Lot group"@en .

:LotGroupAwardInformation a owl:Class ;
    rdfs:isDefinedBy :core ;
    rdfs:subClassOf :ContextDescription ;
    skos:definition "Award information related to a given Group of Lots."@en ;
    skos:prefLabel "Lot group award information"@en .

:Mediator a owl:Class ;
    rdfs:isDefinedBy :core ;
    rdfs:subClassOf :AcquiringParty ;
    skos:definition "A Role of an Agent that attempts to resolve a dispute between different Agents and come to an agreement. WG approval 20/04/2021"@en ;
    skos:prefLabel "Mediator"@en .

:MiniCompetitionAwardOutcome a owl:Class ;
    rdfs:isDefinedBy :core ;
    rdfs:subClassOf :AwardOutcome ;
    skos:definition "Result concerning the mini-competition that was attributed by the Awarder. Additional Information: The mini-competition is the process where multiple winners or candidates of previous stages of a procedure bid for a specific procurement. It is typically used in framework agreements where the suppliers have already been pre-selected, and the mini competition is used to determine which supplier is best suited for a particular project or contract. It is also used in a Dynamic Purchasing System where the suppliers come from a list of Candidates. WG approval 19/03/2024"@en ;
    skos:prefLabel "Mini competition award outcome"@en .

:MonetaryValue a owl:Class ;
    rdfs:isDefinedBy :core ;
    skos:definition "A number of monetary units specified using a given unit of currency. Additional information: In the pre-award phase of the procurement, all monetary values are considered to exclude VAT based on the Directive 2014/24/EU. WG approval 13/04/2021"@en ;
    skos:prefLabel "Monetary value"@en .

:MultipleStageProcedureTerm a owl:Class ;
    rdfs:isDefinedBy :core ;
    rdfs:subClassOf :LotSpecificTerm ;
    skos:definition "Conditions and stipulations defining particularities of Procedures carried out in several steps Additional Information: Generally this refers to Procedures where selection is carried out to qualify Tenderers who are then requested to submit the rest of their Tender for evaluation is Restricted Procedure. WG Approval 15/04/2021"@en ;
    skos:prefLabel "Multiple stage procedure term"@en .

:NonDisclosureAgreementTerm a owl:Class ;
    rdfs:isDefinedBy :core ;
    rdfs:subClassOf :LotSpecificTerm ;
    skos:definition "Conditions and stipulations about a non-disclosure agreement. Additional information: A non-disclosure agreement is a Contract between different parties which ensures information is not shared with other parties. WG approval 26/03/2024"@en ;
    skos:prefLabel "Non disclosure agreement term"@en .

:NonPublishedInformation a owl:Class ;
    rdfs:isDefinedBy :core ;
    rdfs:subClassOf :ContextDescription ;
    skos:definition "Information about fields not published in this Notice. Additional Information: The non-published information may become available at a later date and may differ from one element to another within a given Document. Examples of fields that may not be immediately published are Winner, Tender and Procedure Lot Result, etc., e.g. for security reasons."@en ;
    skos:prefLabel "Non published information"@en .

:Notice a owl:Class ;
    rdfs:isDefinedBy :core ;
    rdfs:subClassOf :Document ;
    skos:definition "Document published by the Buyer about market opportunities and results. WG Approval 23/05/2019"@en ;
    skos:prefLabel "Notice"@en .

:NoticeAwardInformation a owl:Class ;
    rdfs:isDefinedBy :core ;
    rdfs:subClassOf :ContextDescription ;
    skos:definition "Information about an Award Notice."@en ;
    skos:prefLabel "Notice award information"@en .

:Offer a owl:Class ;
    rdfs:isDefinedBy :core ;
    rdfs:subClassOf :Document ;
    skos:definition "Document providing the Monetary Value and the details to fulfill the Requirements set out in the Procurement Documents or Request for Offer. Additional information: A quotation is considered to be an Offer in the eProcurement Ontology. WG approval 09/02/2023"@en ;
    skos:prefLabel "Offer"@en .

:OfferIssuer a owl:Class ;
    rdfs:isDefinedBy :core ;
    rdfs:subClassOf :OfferingParty ;
    skos:definition "The Role of an Agent that distributes an Offer. WG approval 09/02/2023"@en ;
    skos:prefLabel "Offer issuer"@en .

:OfflineAccessProvider a owl:Class ;
    rdfs:isDefinedBy :core ;
    rdfs:subClassOf :AcquiringParty ;
    skos:definition "A Role of an Agent responsible for providing offline access to the Procurement Documents."@en ;
    skos:prefLabel "Offline access provider"@en .

:OpeningTerm a owl:Class ;
    rdfs:isDefinedBy :core ;
    rdfs:subClassOf :LotSpecificTerm,
        :ProcedureSpecificTerm ;
    skos:definition "Conditions and stipulations defining particularities of the opening of Tenders. Additional Information: The opening of Tenders is the event when Tenders are made accessible for evaluation, it is generally the same date and time for all Tenders. WG Approval 15/04/2021"@en ;
    skos:prefLabel "Opening term"@en .

:OrganisationGroup a owl:Class ;
    rdfs:isDefinedBy :core ;
    rdfs:subClassOf org:Organization ;
    skos:definition "Agreed collaboration of several Organisations. Additional Information: This concept has been created to fulfill the need to represent a grouping of Organisations that is not necessarily registered i.e, consortia. WG approval 15/04/2021"@en ;
    skos:prefLabel "Organisation group"@en .

:OriginatorRequest a owl:Class ;
    rdfs:isDefinedBy :core ;
    rdfs:subClassOf :Document ;
    skos:definition "Document in which the Originator describes his needs. WG approval 09/02/2023"@en ;
    skos:prefLabel "Originator request"@en .

:OtherEntity a owl:Class ;
    rdfs:isDefinedBy :core ;
    rdfs:subClassOf :OfferingParty ;
    skos:definition "Economic Operator (who is not a Subcontractor) on which the Tenderer relies upon, to meet Selection Criteria."@en ;
    skos:prefLabel "Other entity"@en .

:ParticipationCondition a owl:Class ;
    rdfs:isDefinedBy :core ;
    rdfs:subClassOf :ProcurementCriterion ;
    skos:definition "Criterion that describes a Requirement to take part in a procurement. WG approval 30/05/2023"@en ;
    skos:prefLabel "Participation condition"@en .

:ParticipationConditionsSummary a owl:Class ;
    rdfs:isDefinedBy :core ;
    rdfs:subClassOf :ProcurementCriteriaSummary ;
    skos:definition "Overview of the Participation Conditions. WG approval 19/03/2024"@en ;
    skos:prefLabel "Participation conditions summary"@en .

:ParticipationRequestProcessor a owl:Class ;
    rdfs:isDefinedBy :core ;
    rdfs:subClassOf :AcquiringParty ;
    skos:definition "A Role of an Agent responsible for processing Requests To Participate."@en ;
    skos:prefLabel "Participation request processor"@en .

:ParticipationRequestReceiver a owl:Class ;
    rdfs:isDefinedBy :core ;
    rdfs:subClassOf :AcquiringParty ;
    skos:definition "A Role of an Agent responsible for receiving Requests To Participate."@en ;
    skos:prefLabel "Participation request receiver"@en .

:ParticipationRequestTerm a owl:Class ;
    rdfs:isDefinedBy :core ;
    rdfs:subClassOf :LotSpecificTerm ;
    skos:definition "Conditions and stipulations defining particularities of requesting participation in a Procedure."@en ;
    skos:prefLabel "Participation request term"@en .

:PaymentExecutor a owl:Class ;
    rdfs:isDefinedBy :core ;
    rdfs:subClassOf :AcquiringParty ;
    skos:definition "A Role of an Agent responsible for executing the Payment."@en ;
    skos:prefLabel "Payment executor"@en .

:Period a owl:Class ;
    rdfs:isDefinedBy :core ;
    skos:definition "A time interval or a Duration. WG approval 28/04/2020"@en ;
    skos:prefLabel "Period"@en .

:PlannedProcurementPart a owl:Class ;
    rdfs:isDefinedBy :core ;
    rdfs:subClassOf :ProcurementElement ;
    skos:definition "A subdivision of a Planned Procurement that may later become one or more Lots or a self-standing Procedure. A Lot or a Procedure can also cover one or more parts of the Planned Procurement. WG Approval 20/06/2019"@en ;
    skos:prefLabel "Planned procurement part"@en .

:Prize a owl:Class ;
    rdfs:isDefinedBy :core ;
    skos:definition "A reward given in a Contest. WG approval: 15/04/2021"@en ;
    skos:prefLabel "Prize"@en .

:Procedure a owl:Class ;
    rdfs:isDefinedBy :core ;
    rdfs:subClassOf :ProcurementObject ;
    skos:definition "A legally defined set of administrative activities conducted to conclude one or more Contracts. Additional Information The Procedure is categorised in the law according to different rules determining whether the Procedure is Open, Restricted, Negotiated with or without publicity, etc. (see Procedure Type). WG Approval 20/08/2019"@en ;
    skos:prefLabel "Procedure"@en .

:ProcedureTerm a owl:Class ;
    rdfs:isDefinedBy :core ;
    rdfs:subClassOf :ProcedureSpecificTerm ;
    skos:definition "Conditions and stipulations defining particularities of the Procedure. (WG approval 23/11/2018)"@en ;
    skos:prefLabel "Procedure term"@en .

:ProcessPlanningTerm a owl:Class ;
    rdfs:isDefinedBy :core ;
    rdfs:subClassOf :Term ;
    skos:definition "Conditions and stipulations defining particularities of the unfolding of the Procurement Process."@en ;
    skos:prefLabel "Process planning term"@en .

:ProcurementDocument a owl:Class ;
    rdfs:isDefinedBy :core ;
    rdfs:subClassOf :Document ;
    skos:definition "Document produced or referred to by the Buyer to describe or determine elements of the Procurement. Additional information: Procurement Documents are to be accessible since the date of publication of the Contract Notice or the prior information Notice when used as a call for competition. Examples of Procurement Documents are Technical Specifications, the Descriptive Document, proposed conditions of Contract, formats for the presentation of Documents by Candidates and Tenderers, information on generally applicable obligations. Other Documents related to the Procedure such as Notices are not considered to be Procurement Documents. WG Approval 23/05/2019 17:08:30"@en ;
    skos:prefLabel "Procurement document"@en .

:ProcurementProcedureInformationProvider a owl:Class ;
    rdfs:isDefinedBy :core ;
    rdfs:subClassOf :AcquiringParty ;
    skos:definition "A Role of an Agent responsible for providing additional information about the Procurement Procedure."@en ;
    skos:prefLabel "Procurement procedure information provider"@en .

:ProcurementProcessInformation a owl:Class ;
    rdfs:isDefinedBy :core ;
    rdfs:subClassOf :ContextDescription ;
    skos:definition "Information about the temporal unfolding or succession of Procurement Objects."@en ;
    skos:prefLabel "Procurement process information"@en .

:ProcurementServiceProvider a owl:Class ;
    rdfs:isDefinedBy :core ;
    rdfs:subClassOf :AcquiringParty ;
    skos:definition "Role of a public or private body which offers ancillary purchasing activities on the market. Additional information \"Ancillary Purchasing Activities\" means activities consisting in the provision of support to purchasing activities, in particular in the following forms: (a) technical infrastructure enabling Contracting Authorities to award Public Contracts or to conclude Framework Agreements for works, supplies or services; (b) advice on the conduct or design of public Procurement Procedures; (c) preparation and management of Procurement Procedures on behalf and for the account of the Contracting Authority concerned; Source: Directive 2014/24/EU, Article 2, paragraphs 17 and 15. This would be equivalent to the concept of 'ProcuringEntity' in OCDS: 'The Entity managing the Procurement, which may be different from the Buyer who is paying / using the items being procured'. WG Approval 24/03/2020"@en ;
    skos:prefLabel "Procurement service provider"@en .

:ProfessionalSuitabilitySummary a owl:Class ;
    rdfs:isDefinedBy :core ;
    rdfs:subClassOf :SelectionCriteriaSummary ;
    skos:definition "Overview of the professional ability required for the economic operator to execute the contract. WG approval 19/03/2024"@en ;
    skos:prefLabel "Professional suitability summary"@en .

:Project a owl:Class ;
    rdfs:isDefinedBy :core ;
    skos:definition "A collaborative enterprise that is carefully planned to achieve a particular aim."@en ;
    skos:prefLabel "Project"@en .

:PurchaseContract a owl:Class ;
    rdfs:isDefinedBy :core ;
    rdfs:subClassOf :Contract ;
    skos:definition "A Contract resulting from using a Dynamic Purchasing System Technique or Framework Agreement Technique."@en ;
    skos:prefLabel "Purchase contract"@en .

:Purpose a owl:Class ;
    rdfs:isDefinedBy :core ;
    skos:definition "The description of the objectives related to a Procurement. Additional information: The description of the objectives includes the Subject Matter and Quantities. The quantification of the objectives related to a procurement. To be re-reviewed by the WG the soonest. (WG to be discussed, this was pointed out on the 09/04/2019 14:38:25 WG Meeting) The old definition read as follows: The description of the objectives related to a procurement. (WG approval 05/12/2018)"@en ;
    skos:prefLabel "Purpose"@en .

:Quantity a owl:Class ;
    rdfs:isDefinedBy :core ;
    skos:definition "A counted number of non-monetary units possibly including fractions."@en ;
    skos:prefLabel "Quantity"@en .

:RequestForClarification a owl:Class ;
    rdfs:isDefinedBy :core ;
    rdfs:subClassOf :Document ;
    skos:definition "A demand for elucidation of received information. Additional Information: Requests for clarification are usually used by Buyers during the process of award or evaluation to understand specific aspects of the Tender without altering the Tender. WG approval 20/04/2021"@en ;
    skos:prefLabel "Request for clarification"@en .

:RequestForParticipation a owl:Class ;
    rdfs:isDefinedBy :core ;
    rdfs:subClassOf :Document ;
    skos:definition "Application of an Economic Operator to be included in a Procurement Procedure. WG approval: 20/04/2021"@en ;
    skos:prefLabel "Request for participation"@en .

:ReviewDecision a owl:Class ;
    rdfs:isDefinedBy :core ;
    rdfs:subClassOf :ReviewObject ;
    skos:definition "Information about Review Decisions."@en ;
    skos:prefLabel "Review decision"@en .

:ReviewIrregularitySummary a owl:Class ;
    rdfs:isDefinedBy :core ;
    rdfs:subClassOf :StatisticalInformation ;
    skos:definition "Overview of the number and type of requests the Buyer received to review any of its decisions (e.g. the Technical Specifications, Award Decision). WG approval 19/03/2024"@en ;
    skos:prefLabel "Review irregularity summary"@en .

:ReviewProcedureInformationProvider a owl:Class ;
    rdfs:isDefinedBy :core ;
    rdfs:subClassOf :AcquiringParty ;
    skos:definition "A Role of an Agent who is providing more information on the time limits for review Procedures."@en ;
    skos:prefLabel "Review procedure information provider"@en .

:ReviewRequest a owl:Class ;
    rdfs:isDefinedBy :core ;
    rdfs:subClassOf :ReviewObject ;
    skos:definition "Information about requests to review procedures."@en ;
    skos:prefLabel "Review request"@en .

:ReviewRequestSummary a owl:Class ;
    rdfs:isDefinedBy :core ;
    rdfs:subClassOf :StatisticalInformation ;
    skos:definition "Overview of the requests received by the Buyer to review any of its decisions (e.g. the technical specifications, award decision), as set out in Art. 1(5) of Directive 89/665/EEC and Directive 92/13/EEC, and about the complainants that submitted the requests. WG approval 19/03/2024"@en ;
    skos:prefLabel "Review request summary"@en .

:ReviewRequester a owl:Class ;
    rdfs:isDefinedBy :core ;
    rdfs:subClassOf :OfferingParty ;
    skos:definition "Role of an Agent who requests the review of a (Procurement) Procedure. WG Approval 23/10/2021"@en ;
    skos:prefLabel "Review requester"@en .

:ReviewTerm a owl:Class ;
    rdfs:isDefinedBy :core ;
    rdfs:subClassOf :LotSpecificTerm,
        :ProcedureSpecificTerm ;
    skos:definition "Conditions and stipulations defining particularities of the review. WG approval 23/11/2018"@en ;
    skos:prefLabel "Review term"@en .

:Reviewer a owl:Class ;
    rdfs:isDefinedBy :core ;
    rdfs:subClassOf :AcquiringParty ;
    skos:definition "Role of an Agent who investigates the overall correctness of a Procurement Procedure, producing a related report. Additional Information: Any Organisation or Person may request a review of a Procurement Procedure. WG approval: 20/04/2021"@en ;
    skos:prefLabel "Reviewer"@en .

:SecurityClearanceTerm a owl:Class ;
    rdfs:isDefinedBy :core ;
    rdfs:subClassOf :LotSpecificTerm ;
    skos:definition "Conditions and stipulations about the status requested of individuals allowing them access to classified information (state or organisational secrets) or to restricted areas, after completion of a thorough background check. Additional information: This corresponds in eForms to BT-578, BT-78, BT-732 . WG approval 20/06/2023"@en ;
    skos:prefLabel "Security clearance term"@en .

:SelectedCandidateList a owl:Class ;
    rdfs:isDefinedBy :core ;
    skos:definition "Record of Candidates admitted to take part in award phases of procurements. WG approval 30/05/2023"@en ;
    skos:prefLabel "Selected candidate list"@en .

:SelectionCriterion a owl:Class ;
    rdfs:isDefinedBy :core ;
    rdfs:subClassOf :QualificationCriterion ;
    skos:definition "Criterion that describes a capacity Requirement that the Economic Operator needs to fulfill to participate in the procurement. Additional Information: Selection criteria may relate to: (a) suitability to pursue the professional activity; (b) economic and financial standing; (c) technical and professional ability WG approval 31/10/2018"@en ;
    skos:prefLabel "Selection criterion"@en .

:SelectionEvaluationTerm a owl:Class ;
    rdfs:isDefinedBy :core ;
    rdfs:subClassOf :EvaluationTerm ;
    skos:definition "Conditions and stipulations defining particularities of the evaluation of Selection Criteria."@en ;
    skos:prefLabel "Selection evaluation term"@en .

:SocialProcurement a owl:Class ;
    rdfs:isDefinedBy :core ;
    rdfs:subClassOf :StrategicProcurement ;
    skos:definition "Approach whereby Buyers seek to procure by fulfilling social objectives. Additional Information: Socially Responsible Public Procurement (SRPP) - ‘SRPP’ means Procurement Operations that take into account one or more of the following social considerations: employment opportunities, decent work, compliance with social and labour rights, social inclusion (including persons with disabilities), equal opportunities, accessibility design for all, taking account of sustainability criteria, including ethical trade issues and wider voluntary compliance with corporate social responsibility (CSR), while observing the principles enshrined in the Treaty for the European Union (TFEU) and the Procurement Directives. Source: Buying Social - A Guide to Taking Account of Social Considerations in Public Procurement (Publications Office of the European Union, 2011) https://op.europa.eu/en/publication-detail/-/publication/cb70c481-0e29-4040-9be2-c408cddf081f/language-en See Article 18 and Annex X Directive 2014/24."@en ;
    skos:prefLabel "Social procurement"@en .

:SpecificDuration a owl:Class ;
    rdfs:isDefinedBy :core ;
    rdfs:subClassOf :Duration ;
    skos:definition "The exact Duration. WG approval 19/03/2024"@en ;
    skos:prefLabel "Specific duration"@en .

:SubcontractTerm a owl:Class ;
    rdfs:isDefinedBy :core ;
    rdfs:subClassOf :ContractSpecificTerm ;
    skos:definition "A concept to describe the main information regarding the share of parts of the Contract to third parties."@en ;
    skos:prefLabel "Subcontract term"@en .

:SubcontractingEstimate a owl:Class ;
    rdfs:isDefinedBy :core ;
    rdfs:subClassOf :Estimate ;
    skos:definition "Approximation concerning the foreseen Subcontracting. WG approval 19/03/2024"@en ;
    skos:prefLabel "Subcontracting estimate"@en .

:Subcontractor a owl:Class ;
    rdfs:isDefinedBy :core ;
    rdfs:subClassOf :OfferingParty ;
    skos:definition "A Role of an Agent that has an agreement to perform part or all of the obligations of another Agents's Contract. Additional information For some Procedures, the Subcontractor signs as well the Contract between the Buyer and the Contractor. At tendering time, entities relied upon by the Economic Operators can be Subcontractors or not. When modelling ESPD we will analyze whether we need or not a Role named \"relied upon\". WG approval 05/08/2021"@en ;
    skos:prefLabel "Subcontractor"@en .

:SubmissionStatisticalInformation a owl:Class ;
    rdfs:isDefinedBy :core ;
    rdfs:subClassOf :StatisticalInformation ;
    skos:definition "Statistical information about submissions on a given competition, either at Lot level or Mini-Competition level. WG approval 30/05/2023"@en ;
    skos:prefLabel "Submission statistical information"@en .

:SubmissionTerm a owl:Class ;
    rdfs:isDefinedBy :core ;
    rdfs:subClassOf :LotSpecificTerm,
        :ProcedureSpecificTerm ;
    skos:definition "Conditions and stipulations defining particularities of submitting Documents to the Buyer. Additional Information: These Documents can be Tenders, Request To Participate and expressions of interest. WG Approval 14/07/2020"@en ;
    skos:prefLabel "Submission term"@en .

:System a owl:Class ;
    rdfs:isDefinedBy :core ;
    rdfs:subClassOf foaf:Agent ;
    skos:definition "Software application used for performing Procurement activities. WG Approval 28/04/2020"@en ;
    skos:prefLabel "System"@en .

:TaxInformationProvider a owl:Class ;
    rdfs:isDefinedBy :core ;
    skos:definition "A Role of an Agent responsible for providing information concerning the general regulatory framework for taxes."@en ;
    skos:prefLabel "Tax information provider"@en .

:TechnicalAbilitySummary a owl:Class ;
    rdfs:isDefinedBy :core ;
    rdfs:subClassOf :SelectionCriteriaSummary ;
    skos:definition "Overview of the expertise required for the economic operator to execute the contract. WG approval 19/03/2024"@en ;
    skos:prefLabel "Technical ability summary"@en .

:TechnicalSpecification a owl:Class ;
    rdfs:isDefinedBy :core ;
    skos:definition "A set of documented Requirements applicable to the object of the Procurement. Additional Information: A specification often includes technical standards. WG approval: 20/04/2021"@en ;
    skos:prefLabel "Technical specification"@en .

:Tender a owl:Class ;
    rdfs:isDefinedBy :core ;
    rdfs:subClassOf :Document ;
    skos:definition "Information submitted by the Economic Operator to specify its Offer regarding a specific Lot, in response to the call for Tender. (WG approval 03/05/2022)"@en ;
    skos:prefLabel "Tender"@en .

:TenderAwardOutcome a owl:Class ;
    rdfs:isDefinedBy :core ;
    rdfs:subClassOf :ContextualProjection ;
    skos:definition "Result concerning the Tender attributed by the Awarder."@en ;
    skos:prefLabel "Tender award outcome"@en .

:TenderGroup a owl:Class ;
    rdfs:isDefinedBy :core ;
    skos:definition "Specific Offer in response to a Lot Group. Additional Information: This class is generally used to provide the Monetary Value in response to a Lot Group."@en ;
    skos:prefLabel "Tender group"@en .

:TenderProcessor a owl:Class ;
    rdfs:isDefinedBy :core ;
    rdfs:subClassOf :AcquiringParty ;
    skos:definition "A Role of an Agent responsible for processing Tenders."@en ;
    skos:prefLabel "Tender processor"@en .

:TenderReceiver a owl:Class ;
    rdfs:isDefinedBy :core ;
    rdfs:subClassOf :AcquiringParty ;
    skos:definition "A Role of an Agent responsible for receiving Tenders."@en ;
    skos:prefLabel "Tender receiver"@en .

:Tenderer a owl:Class ;
    rdfs:isDefinedBy :core ;
    rdfs:subClassOf :OfferingParty ;
    skos:definition "A Role of an Agent that has submitted a Tender. Additional Information: A Tenderer is an Economic Operator or group of Economic Operators that has submitted a Tender. WG approval 05/08/2021"@en ;
    skos:prefLabel "Tenderer"@en .

:VehicleInformation a owl:Class ;
    rdfs:isDefinedBy :core ;
    skos:definition "Information related to clean vehicles legislation. Additional information: In the European Union, the legislation concerned is the European Parliament and Council 2009/33/EC (Clean Vehicles Directive – CVD). WG approval 07/05/2024"@en ;
    skos:prefLabel "Vehicle information"@en .

:Winner a owl:Class ;
    rdfs:isDefinedBy :core ;
    rdfs:subClassOf :OfferingParty ;
    skos:definition "A Role of an Agent to whom a Lot is awarded. WG approval 05/08/2021 (revised 26/10/2021)"@en ;
    skos:prefLabel "Winner"@en .

:actsOnBehalfOf a owl:ObjectProperty ;
    rdfs:isDefinedBy :core ;
    skos:definition "Represents. (epo:ProcurementServiceProvider -> epo:Buyer (+epo:actsOnBehalfOf))"@en ;
    skos:prefLabel "Acts on behalf of"@en .

:agreedByBuyer a owl:ObjectProperty ;
    rdfs:isDefinedBy :core ;
    skos:definition "Accepted by Buyer. WG approval 10/06/2024 (epo-ful:ShipmentAgreement -> epo:Buyer (+epo-ful:agreedByBuyer))"@en ;
    skos:prefLabel "Agreed by buyer"@en .

:amendsContract a owl:ObjectProperty ;
    rdfs:isDefinedBy :core ;
    skos:prefLabel "Amends contract"@en .

:announcesAwardDecision a owl:ObjectProperty ;
    rdfs:isDefinedBy :core ;
    skos:prefLabel "Announces award decision"@en .

:announcesCompletionOfContract a owl:ObjectProperty ;
    rdfs:isDefinedBy :core ;
    skos:prefLabel "Announces completion of contract"@en .

:announcesContract a owl:ObjectProperty ;
    rdfs:isDefinedBy :core ;
    skos:prefLabel "Announces contract"@en .

:announcesLot a owl:ObjectProperty ;
    rdfs:isDefinedBy :core ;
    skos:prefLabel "Announces lot"@en .

:announcesLotGroup a owl:ObjectProperty ;
    rdfs:isDefinedBy :core ;
    skos:prefLabel "Announces lot group"@en .

:announcesLotGroupAwardInformation a owl:ObjectProperty ;
    rdfs:isDefinedBy :core ;
    skos:prefLabel "Announces lot group award information"@en .

:announcesNoticeAwardInformation a owl:ObjectProperty ;
    rdfs:isDefinedBy :core ;
    skos:prefLabel "Announces notice award information"@en .

:announcesPlannedProcurementPart a owl:ObjectProperty ;
    rdfs:isDefinedBy :core ;
    skos:prefLabel "Announces planned procurement part"@en .

:announcesProcedure a owl:ObjectProperty ;
    rdfs:isDefinedBy :core ;
    skos:prefLabel "Announces procedure"@en .

:announcesReviewObject a owl:ObjectProperty ;
    rdfs:isDefinedBy :core ;
    skos:prefLabel "Announces review object"@en .

:announcesRole a owl:ObjectProperty ;
    rdfs:isDefinedBy :core ;
    skos:prefLabel "Announces role"@en .

:answersQuestion a owl:ObjectProperty ;
    rdfs:isDefinedBy :core ;
    skos:definition "Relation indicating that the Response replies to a question. WG approval 12/03/2024 (epo-sub:Response -> cccev:InformationRequirement (+epo-sub:answersQuestion))"@en ;
    skos:prefLabel "Answers question"@en .

:associatedWith a owl:ObjectProperty ;
    rdfs:isDefinedBy :core ;
    skos:definition "The document to which a document is associated. WGM 01/03/2022 (epo:Document -> epo:Document (+epo:associatedWith))"@en ;
    skos:prefLabel "Associated with"@en .

:attestedByLabel a owl:ObjectProperty ;
    rdfs:isDefinedBy :core ;
    skos:definition "Relation indicating which label the certificate is about. WG approval 28/07/2022 (epo:Certificate -> epo:CertificationLabel (+epo:attestedByLabel))"@en ;
    skos:prefLabel "Attested by label"@en .

:bindsBuyer a owl:ObjectProperty ;
    rdfs:isDefinedBy :core ;
    skos:definition "Provides legal constraint on the Buyer. (epo:Contract -> epo:Buyer (+epo:bindsBuyer))"@en ;
    skos:prefLabel "Binds buyer"@en .

:bindsContractor a owl:ObjectProperty ;
    rdfs:isDefinedBy :core ;
    skos:definition "Provides legal constraint on the Contractor. (epo:Contract -> epo:Contractor (+epo:bindsContractor))"@en ;
    skos:prefLabel "Binds contractor"@en .

:canProvideNonDiscriminatoryEvidence a owl:ObjectProperty ;
    rdfs:isDefinedBy :core ;
    skos:definition "Relation showing that an Organization can supply an Evidence with regard to the fulfilment of non-discriminatory criteria or the rules applied in order to reduce the number of participants. WG approval 12/03/2024 (org:Organization -> cccev:Evidence (+epo:canProvideNonDiscriminatoryEvidence))"@en ;
    skos:prefLabel "Can provide non discriminatory evidence"@en .

:canProvideTaxAndSocialSecuritiesEvidence a owl:ObjectProperty ;
    rdfs:isDefinedBy :core ;
    skos:definition "Relation showing that an Organization can supply an Evidence with regard to the payment of social security contributions and taxes. WG approval 12/03/2024 (org:Organization -> cccev:Evidence (+epo:canProvideTaxAndSocialSecuritiesEvidence))"@en ;
    skos:prefLabel "Can provide tax and social securities evidence"@en .

:comprisesAwardOutcome a owl:ObjectProperty ;
    rdfs:isDefinedBy :core ;
    skos:definition "Incorporates AwardOutcome. (epo:AwardDecision -> epo:AwardOutcome (+epo:comprisesAwardOutcome))"@en ;
    skos:prefLabel "Comprises award outcome"@en .

:comprisesTender a owl:ObjectProperty ;
    rdfs:isDefinedBy :core ;
    skos:definition "Incorporates Tender. (epo:TenderGroup -> epo:Tender (+epo:comprisesTender))"@en ;
    skos:prefLabel "Comprises tender"@en .

:comprisesTenderAwardOutcome a owl:ObjectProperty ;
    rdfs:isDefinedBy :core ;
    skos:definition "Incorporates TenderAwardOutcome. (epo:AwardOutcome -> epo:TenderAwardOutcome (+epo:comprisesTenderAwardOutcome))"@en ;
    skos:prefLabel "Comprises tender award outcome"@en .

:concernsContract a owl:ObjectProperty ;
    rdfs:isDefinedBy :core ;
    skos:prefLabel "Concerns contract"@en .

:concernsGreenProcurement a owl:ObjectProperty ;
    rdfs:isDefinedBy :core ;
    skos:definition "Relates to Green Procurement. WG approval 07/05/2024 (epo:VehicleInformation -> epo:GreenProcurement (+epo:concernsGreenProcurement))"@en ;
    skos:prefLabel "Concerns green procurement"@en .

:concernsLot a owl:ObjectProperty ;
    rdfs:isDefinedBy :core ;
    skos:definition "Relates to Lot. (epo:LotAwardOutcome -> epo:Lot (+epo:concernsLot)) Relates to Lot. (epo:ProcurementProcessInformation -> epo:Lot (+epo:concernsLot))"@en ;
    skos:prefLabel "Concerns lot"@en .

:concernsLotGroup a owl:ObjectProperty ;
    rdfs:isDefinedBy :core ;
    skos:prefLabel "Concerns lot group"@en .

:concernsNotice a owl:ObjectProperty ;
    rdfs:isDefinedBy :core ;
    skos:definition "Relates to Notice. WG approval 14/05/2024 (epo:ChangeInformation -> epo:Notice (+epo:concernsNotice)) Relates to Notice. WG approval 14/05/2024 (epo:NonPublishedInformation -> epo:Notice (+epo:concernsNotice))"@en ;
    skos:prefLabel "Concerns notice"@en .

:concernsOrganisation a owl:ObjectProperty ;
    rdfs:isDefinedBy :core ;
    skos:definition "Relates to Organization. WG approval 05/03/2024 (epo-sub:NationalPreQualificationData -> org:Organization (+epo-sub:concernsOrganisation))"@en ;
    skos:prefLabel "Concerns organisation"@en .

:concernsOriginatorRequest a owl:ObjectProperty ;
    rdfs:isDefinedBy :core ;
    skos:prefLabel "Concerns originator request"@en .

:concernsProcedure a owl:ObjectProperty ;
    rdfs:isDefinedBy :core ;
    skos:definition "Relates to Procedure. (epo:ProcurementProcessInformation -> epo:Procedure (+epo:concernsProcedure)) Relates to Procedure. WG approval 05/03/2024 (epo-acc:ESPDRequest -> epo:Procedure (+epo:concernsProcedure))"@en ;
    skos:prefLabel "Concerns procedure"@en .

:concernsReviewSummaryForLot a owl:ObjectProperty ;
    rdfs:isDefinedBy :core ;
    skos:definition "Relates to Lot review summary. Additional information: This relation corresponds in eForms to BT-13722 Buyer Review Lot Identifier. (epo:ReviewRequestSummary -> epo:Lot (+epo:concernsReviewSummaryForLot))"@en ;
    skos:prefLabel "Concerns review summary for lot"@en .

:concernsTender a owl:ObjectProperty ;
    rdfs:isDefinedBy :core ;
    skos:definition "Relates to Tender. WG approval 14/05/2024 (epo:TenderAwardOutcome -> epo:Tender (+epo:concernsTender))"@en ;
    skos:prefLabel "Concerns tender"@en .

:conformsToLegalBasis a owl:ObjectProperty ;
    rdfs:isDefinedBy :core ;
    skos:definition "The Notice was designed in accordance with the given legal basis. Additional Information: This Notice can be used for Procedures which do not have the same legal basis. This holds for standard forms. (epo:Notice -> at-voc:legal-basis (+epo:conformsToLegalBasis))"@en ;
    skos:prefLabel "Conforms to legal basis"@en .

:containsCandidate a owl:ObjectProperty ;
    rdfs:isDefinedBy :core ;
    skos:definition "Includes Candidate. WG approval 14/05/2024 (epo:SelectedCandidateList -> epo:Candidate (+epo:containsCandidate))"@en ;
    skos:prefLabel "Contains candidate"@en .

:contextualisedBy a owl:ObjectProperty ;
    rdfs:isDefinedBy :core ;
    skos:definition "The place of the AgentInRole in the procurement is expressed by a ProcurementObject. (epo:AgentInRole -> epo:ProcurementObject (+epo:contextualisedBy))"@en ;
    skos:prefLabel "Contextualised by"@en .

:definesBudgetProvider a owl:ObjectProperty ;
    rdfs:isDefinedBy :core ;
    skos:definition "Relation indicating a ProcedureTerm has a BudgetProvider. (epo:ProcedureTerm -> epo:BudgetProvider (+epo:definesBudgetProvider))"@en ;
    skos:prefLabel "Defines budget provider"@en .

:definesCatalogueProvider a owl:ObjectProperty ;
    rdfs:isDefinedBy :core ;
    skos:definition "Relation indicating an AccessTerm has a CatalogueProvider. (epo:AccessTerm -> epo:CatalogueProvider (+epo:definesCatalogueProvider))"@en ;
    skos:prefLabel "Defines catalogue provider"@en .

:definesCatalogueReceiver a owl:ObjectProperty ;
    rdfs:isDefinedBy :core ;
    skos:definition "Relation indicating an AccessTerm has a CatalogueReceiver. (epo:AccessTerm -> epo:CatalogueReceiver (+epo:definesCatalogueReceiver))"@en ;
    skos:prefLabel "Defines catalogue receiver"@en .

:definesContractDuration a owl:ObjectProperty ;
    rdfs:isDefinedBy :core ;
    skos:definition "Relation indicating a ContractTerm has a Duration. (epo:ContractTerm -> epo:Duration (+epo:definesContractDuration))"@en ;
    skos:prefLabel "Defines contract duration"@en .

:definesContractPeriod a owl:ObjectProperty ;
    rdfs:isDefinedBy :core ;
    skos:definition "Relation indicating a ContractTerm has a Period. (epo:ContractTerm -> epo:Period (+epo:definesContractPeriod))"@en ;
    skos:prefLabel "Defines contract period"@en .

:definesInformationProvider a owl:ObjectProperty ;
    rdfs:isDefinedBy :core ;
    skos:definition "Relation indicating a ProcedureTerm has an information provider. (epo:ProcedureTerm -> epo:AuxiliaryParty (+epo:definesInformationProvider))"@en ;
    skos:prefLabel "Defines information provider"@en .

:definesLotGroup a owl:ObjectProperty ;
    rdfs:isDefinedBy :core ;
    skos:definition "Relation indicating a ProcedureTerm has a LotGroup. (epo:ProcedureTerm -> epo:LotGroup (+epo:definesLotGroup))"@en ;
    skos:prefLabel "Defines lot group"@en .

:definesMediator a owl:ObjectProperty ;
    rdfs:isDefinedBy :core ;
    skos:definition "Relation indicating a ProcedureTerm has a Mediator. (epo:ProcedureTerm -> epo:Mediator (+epo:definesMediator))"@en ;
    skos:prefLabel "Defines mediator"@en .

:definesOfflineAccessProvider a owl:ObjectProperty ;
    rdfs:isDefinedBy :core ;
    skos:definition "Relation indicating an AccessTerm has an OfflineAccessProvider. (epo:AccessTerm -> epo:OfflineAccessProvider (+epo:definesOfflineAccessProvider))"@en ;
    skos:prefLabel "Defines offline access provider"@en .

:definesOpeningPlace a owl:ObjectProperty ;
    rdfs:isDefinedBy :core ;
    skos:definition "The place where the tenders will be publicly opened. WG Approval 10-10-2019 (epo:OpeningTerm -> locn:Address (+epo:definesOpeningPlace))"@en ;
    skos:prefLabel "Defines opening place"@en .

:definesParticipationRequestProcessor a owl:ObjectProperty ;
    rdfs:isDefinedBy :core ;
    skos:definition "Relation indicating a ParticipationRequestTerm has a ParticipationRequestProcessor. (epo:ParticipationRequestTerm -> epo:ParticipationRequestProcessor (+epo:definesParticipationRequestProcessor))"@en ;
    skos:prefLabel "Defines participation request processor"@en .

:definesParticipationRequestReceiver a owl:ObjectProperty ;
    rdfs:isDefinedBy :core ;
    skos:definition "Relation indicating a ParticipationRequestTerm has a ParticipationRequestReceiver. (epo:ParticipationRequestTerm -> epo:ParticipationRequestReceiver (+epo:definesParticipationRequestReceiver))"@en ;
    skos:prefLabel "Defines participation request receiver"@en .

:definesPaymentExecutor a owl:ObjectProperty ;
    rdfs:isDefinedBy :core ;
    skos:definition "Relation indicating a ContractTerm has a PaymentExecutor. (epo:ContractTerm -> epo:PaymentExecutor (+epo:definesPaymentExecutor))"@en ;
    skos:prefLabel "Defines payment executor"@en .

:definesPrize a owl:ObjectProperty ;
    rdfs:isDefinedBy :core ;
    skos:definition "Relation indicating a DesignContestRegimeTerm has a Prize. (epo:DesignContestRegimeTerm -> epo:Prize (+epo:definesPrize))"@en ;
    skos:prefLabel "Defines prize"@en .

:definesProcurementProcedureInformationProvider a owl:ObjectProperty ;
    rdfs:isDefinedBy :core ;
    skos:definition "Relation indicating an AccessTerm has a ProcurementProcedureInformationProvider. (epo:AccessTerm -> epo:ProcurementProcedureInformationProvider (+epo:definesProcurementProcedureInformationProvider))"@en ;
    skos:prefLabel "Defines procurement procedure information provider"@en .

:definesReviewProcedureInformationProvider a owl:ObjectProperty ;
    rdfs:isDefinedBy :core ;
    skos:definition "Relation indicating a ReviewTerm has a ReviewProcedureInformationProvider. (epo:ReviewTerm -> epo:ReviewProcedureInformationProvider (+epo:definesReviewProcedureInformationProvider))"@en ;
    skos:prefLabel "Defines review procedure information provider"@en .

:definesReviewer a owl:ObjectProperty ;
    rdfs:isDefinedBy :core ;
    skos:definition "Relation indicating a ReviewTerm has a Reviewer. (epo:ReviewTerm -> epo:Reviewer (+epo:definesReviewer))"@en ;
    skos:prefLabel "Defines reviewer"@en .

:definesSpecificPlaceOfPerformance a owl:ObjectProperty ;
    rdfs:isDefinedBy :core ;
    skos:definition "Relation indicating a ContractTerm has a specific place of performance. (epo:ContractTerm -> dct:Location (+epo:definesSpecificPlaceOfPerformance))"@en ;
    skos:prefLabel "Defines specific place of performance"@en .

:definesSubcontractingTerm a owl:ObjectProperty ;
    rdfs:isDefinedBy :core ;
    skos:definition "Relation indicating a ContractTerm has a SubcontractingTerm. (epo:ContractTerm -> epo:SubcontractTerm (+epo:definesSubcontractingTerm))"@en ;
    skos:prefLabel "Defines subcontracting term"@en .

:definesTenderProcessor a owl:ObjectProperty ;
    rdfs:isDefinedBy :core ;
    skos:definition "Relation indicating a SubmissionTerm has a TenderProcessor. (epo:SubmissionTerm -> epo:TenderProcessor (+epo:definesTenderProcessor))"@en ;
    skos:prefLabel "Defines tender processor"@en .

:definesTenderReceiver a owl:ObjectProperty ;
    rdfs:isDefinedBy :core ;
    skos:definition "Relation indicating a SubmissionTerm has a TenderReceiver. (epo:SubmissionTerm -> epo:TenderReceiver (+epo:definesTenderReceiver))"@en ;
    skos:prefLabel "Defines tender receiver"@en .

:delegatesAncillaryActivitiesTo a owl:ObjectProperty ;
    rdfs:isDefinedBy :core ;
    skos:definition "Entrusts ancillary purchasing activities to ProcurementServiceProvider. Additional Information: Directive 2014/24/EU describes ancillary purchasing activities as activities consisting in the provision of support to purchasing activities, in particular in the following forms: (a) technical infrastructure enabling contracting authorities to award public contracts or to conclude framework agreements for works, supplies or services; (b) advice on the conduct or design of public procurement procedures; (c) preparation and management of procurement procedures on behalf and for the account of the contracting authority concerned; (epo:Buyer -> epo:ProcurementServiceProvider (+epo:delegatesAncillaryActivitiesTo))"@en ;
    skos:prefLabel "Delegates ancillary activities to"@en .

:describesDirectAwardPrenotificationNotice a owl:ObjectProperty ;
    rdfs:isDefinedBy :core ;
    skos:prefLabel "Describes direct award prenotification notice"@en .

:describesLotCompletion a owl:ObjectProperty ;
    rdfs:isDefinedBy :core ;
    skos:prefLabel "Describes lot completion"@en .

:describesLotGroup a owl:ObjectProperty ;
    rdfs:isDefinedBy :core ;
    skos:prefLabel "Describes lot group"@en .

:describesMinimumLevelOfStandards a owl:DatatypeProperty ;
    rdfs:isDefinedBy :core ;
    skos:definition "Explanatory text regarding the minimum level of standards required. WG approval 02/05/2024 (epo:SelectionCriteriaSummary)"@en ;
    skos:prefLabel "Describes minimum level of standards"@en .

:describesObjectiveParticipationRules a owl:DatatypeProperty ;
    rdfs:isDefinedBy :core ;
    skos:definition "General explanatory text on the rules and criteria to be fulfilled by the Tender. WG approval 02/05/2024 (epo:ParticipationConditionsSummary)"@en ;
    skos:prefLabel "Describes objective participation rules"@en .

:describesProfession a owl:DatatypeProperty ;
    rdfs:isDefinedBy :core ;
    skos:definition "Explanatory text about the profession. WG approval 02/05/2024 (epo:ProfessionalSuitabilitySummary)"@en ;
    skos:prefLabel "Describes profession"@en .

:describesProfessionRelevantLaw a owl:DatatypeProperty ;
    rdfs:isDefinedBy :core ;
    skos:definition "Explanatory text about the law concerning the profession. WG approval 02/05/2024 (epo:ProfessionalSuitabilitySummary)"@en ;
    skos:prefLabel "Describes profession relevant law"@en .

:describesResultNotice a owl:ObjectProperty ;
    rdfs:isDefinedBy :core ;
    skos:prefLabel "Describes result notice"@en .

:describesVerificationMethod a owl:DatatypeProperty ;
    rdfs:isDefinedBy :core ;
    skos:definition "General explanatory text on the means used to validate the Participation Conditions. WG approval 02/05/2024 (epo:ParticipationConditionsSummary)"@en ;
    skos:prefLabel "Describes verification method"@en .

:distributesOffer a owl:ObjectProperty ;
    rdfs:isDefinedBy :core ;
    skos:prefLabel "Distributes offer"@en .

:exposesChannel a owl:ObjectProperty ;
    rdfs:isDefinedBy :core ;
    skos:prefLabel "Exposes channel"@en .

:exposesInvoiceeChannel a owl:ObjectProperty ;
    rdfs:isDefinedBy :core ;
    skos:prefLabel "Exposes invoicee channel"@en .

:followsRulesSetBy a owl:ObjectProperty ;
    rdfs:isDefinedBy :core ;
    skos:prefLabel "Follows rules set by"@en .

:foreseesConcession a owl:ObjectProperty ;
    rdfs:isDefinedBy :core ;
    skos:prefLabel "Foresees concession"@en .

:foreseesContractSpecificTerm a owl:ObjectProperty ;
    rdfs:isDefinedBy :core ;
    skos:prefLabel "Foresees contract specific term"@en .

:foreseesProcurementObject a owl:ObjectProperty ;
    rdfs:isDefinedBy :core ;
    skos:definition "Relation indicating the instance of a Procurement Object that is planned. Additional Information: The properties of the Procurement Object that is foreseen should be read as foreseen properties. For example, Procedure isSMESuitable should be read as Procedure foreseesToBeSMESuitable. For example, Procedure isFundedBy should be read as Procedure foreseesToBeFundedBy. (epo:PlannedProcurementPart -> epo:ProcurementObject (+epo:foreseesProcurementObject))"@en ;
    skos:prefLabel "Foresees procurement object"@en .

:foreseesSubcontracting a owl:ObjectProperty ;
    rdfs:isDefinedBy :core ;
    skos:prefLabel "Foresees subcontracting"@en .

:foreseesSubcontractor a owl:ObjectProperty ;
    rdfs:isDefinedBy :core ;
    skos:prefLabel "Foresees subcontractor"@en .

:foreseesTechnique a owl:ObjectProperty ;
    rdfs:isDefinedBy :core ;
    skos:prefLabel "Foresees technique"@en .

:fulfillsRequirement a owl:ObjectProperty ;
    rdfs:isDefinedBy :core ;
    skos:definition "The requirement to which the concept meets. WG Approval 09/11/2021 (epo:GreenProcurement -> at-voc:green-public-procurement-criteria (+epo:fulfillsRequirement)) The requirement to which the concept meets. WG Approval 09/11/2021 (epo:GreenProcurement -> at-voc:environmental-impact (+epo:fulfillsRequirement)) The requirement to which the concept meets. WG Approval 09/11/2021 (epo:InnovativeProcurement -> at-voc:innovative-acquisition (+epo:fulfillsRequirement)) The requirement to which the concept meets. WG Approval 09/11/2021 (epo:SocialProcurement -> at-voc:social-objective (+epo:fulfillsRequirement))"@en ;
    skos:prefLabel "Fulfills requirement"@en .

:fulfillsStrategicProcurement a owl:ObjectProperty ;
    rdfs:isDefinedBy :core ;
    skos:prefLabel "Fulfills strategic procurement"@en .

:hasAbnormallyLowTenders a owl:DatatypeProperty ;
    rdfs:isDefinedBy :core ;
    skos:definition "Tenders received that were found irregular and non-acceptable due to an abnormally low price or cost. Additional Information The definition implies that abnormally Low Tender Lots are Inadmissible Tender Lots. WG Approval 28/07/2020 (epo:SubmissionStatisticalInformation)"@en ;
    skos:prefLabel "Has abnormally low tenders"@en .

:hasAcceleratedProcedureJustification a owl:DatatypeProperty ;
    rdfs:isDefinedBy :core ;
    skos:definition "The reasons why the procedure is accelerated. Additional Information: A procedure is accelerated to cover needs of extraordinary circumstances ie earthquake relief. WG Approval 09/06/2020 (epo:Procedure)"@en ;
    skos:prefLabel "Has accelerated procedure justification"@en .

:hasAccessURL a owl:DatatypeProperty ;
    rdfs:isDefinedBy :core ;
    skos:definition "Location where the resource can be accessed. WG approval 07/04/2022 (epo:Document)"@en ;
    skos:prefLabel "Has access u r l"@en .

:hasAccessibilityDate a owl:DatatypeProperty ;
    rdfs:isDefinedBy :core ;
    skos:definition "The date at which unpublished data shall be published. WG Approval 11/06/2020 (epo:NonPublishedInformation)"@en ;
    skos:prefLabel "Has accessibility date"@en .

:hasActivityDescription a owl:DatatypeProperty ;
    rdfs:isDefinedBy :core ;
    skos:definition "In the ePO ontology a taxonomy with all activities, based on different classifications (COFOG, UTILITIES, NACE), will be provided. In ePO this field is to be used exclusively to complement the definition attached to the MainActivityCode. However, in eForms there is the code \"other\" to cover undefined activities. For mapping to this eForms feature one could also use this property. (epo:Buyer)"@en ;
    skos:prefLabel "Has activity description"@en .

:hasAdditionalClassification a owl:ObjectProperty ;
    rdfs:isDefinedBy :core ;
    skos:prefLabel "Has additional classification"@en .

:hasAdditionalContractNature a owl:ObjectProperty ;
    rdfs:isDefinedBy :core ;
    skos:definition "Additional type of acquisition taken into consideration in the contract. WG Approval 11/06/2020 (epo:ContractTerm -> at-voc:contract-nature (+epo:hasAdditionalContractNature))"@en ;
    skos:prefLabel "Has additional contract nature"@en .

:hasAdditionalInformation a owl:DatatypeProperty ;
    rdfs:isDefinedBy :core ;
    skos:definition "Supplementary data about the instance of the concept. WG Approval 15/10/2019 (epo:ChangeInformation) Supplementary data about the instance of the concept. WG Approval 15/10/2019 (epo:Notice) Supplementary data about the instance of the concept. WG Approval 15/10/2019 (epo:ProcurementCriterion) Supplementary data about the instance of the concept. WG Approval 15/10/2019 (epo:ProcurementObject)"@en ;
    skos:prefLabel "Has additional information"@en .

:hasAdditionalInformationDeadline a owl:DatatypeProperty ;
    rdfs:isDefinedBy :core ;
    skos:definition "The time limit for requesting further information. Additional information: This is generally used to indicate the deadline for Economic Operators to request further information of the procedure before the submission deadline. This corresponds in eForms to BT-13 Additional Information Deadline. WG Approval 09/06/2020 (epo:AccessTerm)"@en ;
    skos:prefLabel "Has additional information deadline"@en .

:hasAdditionalNonAwardJustification a owl:DatatypeProperty ;
    rdfs:isDefinedBy :core ;
    skos:definition "Further justification for the non award . Additional information: This is generally used when the non award reason code is set to \"Other\". WG: 18/01/2022 (epo:AwardDecision)"@en ;
    skos:prefLabel "Has additional non award justification"@en .

:hasAddressURL a owl:DatatypeProperty ;
    rdfs:isDefinedBy :core ;
    skos:definition "The resource identifier for a Channel. WG approval 26/03/2024 (cv:Channel)"@en ;
    skos:prefLabel "Has address u r l"@en .

:hasAlias a owl:DatatypeProperty ;
    rdfs:isDefinedBy :core ;
    skos:definition "Acronym or alternative name of the Agent. WG Approval 25/03/2021 (foaf:Agent)"@en ;
    skos:prefLabel "Has alias"@en .

:hasAllegedIrregularityType a owl:ObjectProperty ;
    rdfs:isDefinedBy :core ;
    skos:definition "Additional information: This relation corresponds in eForms to BT-791 Review Irregularity Type (epo:ReviewRequest -> at-voc:irregularity-type (+epo:hasAllegedIrregularityType))"@en ;
    skos:prefLabel "Has alleged irregularity type"@en .

:hasAmount a owl:ObjectProperty ;
    rdfs:isDefinedBy :core ;
    skos:definition "The predetermined monetary value charged in addition to the price. WG approval 26/07/2022 (epo-ord:AllowanceChargeInformation -> epo:MonetaryValue (+epo-cat:hasAmount)) The predetermined monetary value charged in addition to the price. WG approval 26/07/2022 (epo-ord:TaxInformation -> epo:MonetaryValue (+epo-cat:hasAmount))"@en ;
    skos:prefLabel "Has amount"@en .

:hasAmountDueForPayment a owl:ObjectProperty ;
    rdfs:isDefinedBy :core ;
    skos:prefLabel "Has amount due for payment"@en .

:hasAmountValue a owl:DatatypeProperty ;
    rdfs:isDefinedBy :core ;
    skos:definition "The numeric value of the amount, including decimals. (epo:MonetaryValue)"@en ;
    skos:prefLabel "Has amount value"@en .

:hasApproximateFrameworkAgreementValue a owl:ObjectProperty ;
    rdfs:isDefinedBy :core ;
    skos:definition "The estimated value to be spent within the Framework Agreement(s). Additional information: In the case of an Award Decision for a Lot, this relation represents the estimated value for the awarded Framework Agreement. In the case of a Notice, this relation represents the estimated value for all Framework Agreements covered by the Notice. (epo:LotAwardOutcome -> epo:MonetaryValue (+epo:hasApproximateFrameworkAgreementValue)) The estimated value to be spent within the Framework Agreement(s). Additional information: In the case of an Award Decision for a Lot, this relation represents the estimated value for the awarded Framework Agreement. In the case of a Notice, this relation represents the estimated value for all Framework Agreements covered by the Notice. (epo:NoticeAwardInformation -> epo:MonetaryValue (+epo:hasApproximateFrameworkAgreementValue))"@en ;
    skos:prefLabel "Has approximate framework agreement value"@en .

:hasApproximateGroupFrameworkAgreementValue a owl:ObjectProperty ;
    rdfs:isDefinedBy :core ;
    skos:prefLabel "Has approximate group framework agreement value"@en .

:hasAssociatedDocument a owl:ObjectProperty ;
    rdfs:isDefinedBy :core ;
    skos:definition "Is related to a Document. WG approval 06/10/2024 (epo-ful:DespatchAdvice -> epo:Document (+epo-ful:hasAssociatedDocument)) Is related to a Document. WG approval 06/10/2024 (epo-ful:DespatchLine -> epo:Document (+epo-ful:hasAssociatedDocument))"@en ;
    skos:prefLabel "Has associated document"@en .

:hasAwardCriteriaEvaluationFormula a owl:DatatypeProperty ;
    rdfs:isDefinedBy :core ;
    skos:definition "The mathematical equation or any other description used for complicated weighing of criteria (e.g. non-linear weighing, the analytic hierarchy process) when a weighing cannot be expressed per criterion. Additional Information: This corresponds in eForms to BT-543 Award Criteria Complicated. (epo:AwardEvaluationTerm)"@en ;
    skos:prefLabel "Has award criteria evaluation formula"@en .

:hasAwardCriteriaOrderJustification a owl:DatatypeProperty ;
    rdfs:isDefinedBy :core ;
    skos:definition "The justification for only indicating the award criteria's order of importance, not their weighing. Additional Information: This corresponds in eForms to BT-733 Award Criteria Order Justification. (epo:AwardEvaluationTerm)"@en ;
    skos:prefLabel "Has award criteria order justification"@en .

:hasAwardCriteriaStatedInProcurementDocuments a owl:DatatypeProperty ;
    rdfs:isDefinedBy :core ;
    skos:definition "The Award Criteria are provided in the Procurement Documents. WG approval 26/03/2024 (epo:AwardCriterion)"@en ;
    skos:prefLabel "Has award criteria stated in procurement documents"@en .

:hasAwardCriterionType a owl:ObjectProperty ;
    rdfs:isDefinedBy :core ;
    skos:definition "Category of award criterion. (epo:AwardCriterion -> at-voc:award-criterion-type (+epo:hasAwardCriterionType))"@en ;
    skos:prefLabel "Has award criterion type"@en .

:hasAwardDateScheduled a owl:DatatypeProperty ;
    rdfs:isDefinedBy :core ;
    skos:definition "Planned date for the award decision. WG Approval 09/11/2021 (epo:ProcessPlanningTerm)"@en ;
    skos:prefLabel "Has award date scheduled"@en .

:hasAwardDecisionDate a owl:DatatypeProperty ;
    rdfs:isDefinedBy :core ;
    skos:definition "The official date of the award decision. Additional Information: This corresponds in eForms to BT-1451 Winner Decision Date. WG Approval 09/01/2020 (epo:AwardDecision)"@en ;
    skos:prefLabel "Has award decision date"@en .

:hasAwardRank a owl:DatatypeProperty ;
    rdfs:isDefinedBy :core ;
    skos:definition "The position of the tender (i.e. whether the tender ended up first, second, third, etc.) in a design contest, some framework agreements with multiple winners (e.g. cascades) or an innovation partnership. Additional Information: This corresponds in eForms to BT-171 Tender Rank. (epo:TenderAwardOutcome)"@en ;
    skos:prefLabel "Has award rank"@en .

:hasAwardStatus a owl:ObjectProperty ;
    rdfs:isDefinedBy :core ;
    skos:definition "Indicates whether the lot is awarded, not awarded or still open. WG Approval 03/12/2019 (epo:AwardOutcome -> at-voc:winner-selection-status (+epo:hasAwardStatus))"@en ;
    skos:prefLabel "Has award status"@en .

:hasAwardedValue a owl:ObjectProperty ;
    rdfs:isDefinedBy :core ;
    skos:definition "The value of the procurement provided by the Award Decision. Additional Information: Different cases of awarded values may refer to a lot, the global value of the procedure, or of a combinatorial value of a group of lots. In the case of framework agreements and dynamic purchasing systems this refers to the maximum awarded value. WG Approval 10/12/2019 (epo:AwardOutcome -> epo:MonetaryValue (+epo:hasAwardedValue))"@en ;
    skos:editorialNote "Used in F18 and other standard forms."@en ;
    skos:prefLabel "Has awarded value"@en .

:hasBankingIdentifier a owl:ObjectProperty ;
    rdfs:isDefinedBy :core ;
    skos:definition "An unique banking reference identifier of the Payee or Seller, assigned by the Payee or Seller bank. WG approval 11/07/2024 (epo-inv:PaymentInstructionsInformation -> adms:Identifier (+epo-inv:hasBankingIdentifier))"@en ;
    skos:prefLabel "Has banking identifier"@en .

:hasBargainPrice a owl:ObjectProperty ;
    rdfs:isDefinedBy :core ;
    skos:definition "The value of procured supplies that have used a particularly advantageous opportunity available for a very short time at a value considerably lower than normal market prices. WG approval 23/05/2023 (epo:AwardOutcome -> epo:MonetaryValue (+epo:hasBargainPrice))"@en ;
    skos:prefLabel "Has bargain price"@en .

:hasBaseQuantity a owl:ObjectProperty ;
    rdfs:isDefinedBy :core ;
    skos:definition "The quantity at which the net monetary value applies. (epo-cat:Price -> epo:Quantity (+epo-cat:hasBaseQuantity))"@en ;
    skos:prefLabel "Has base quantity"@en .

:hasBatchID a owl:ObjectProperty ;
    rdfs:isDefinedBy :core ;
    skos:definition "The identifier assigned to a specific batch of the produced Item. WG Approval 16/05/2023 (epo-cat:Batch -> adms:Identifier (+epo:hasBatchID))"@en ;
    skos:prefLabel "Has batch i d"@en .

:hasBeginning a owl:DatatypeProperty ;
    rdfs:isDefinedBy :core ;
    skos:definition "The date and time on which this period begins. (epo:Period)"@en ;
    skos:prefLabel "Has beginning"@en .

:hasBeneficialOwner a owl:ObjectProperty ;
    rdfs:isDefinedBy :core ;
    skos:definition "A role of any natural person(s) who ultimately owns or controls the organisation or on whose behalf a transaction or activity is being conducted. Additional Information: This role is defined in the directive EU 2015/849 and it's beyond the scope for public eProcurement domain. WG approval 14/09/2021 (epo:Business <-> person:Person (+epo:hasBeneficialOwner +epo:isBeneficialOwnerOf))"@en ;
    skos:prefLabel "Has beneficial owner"@en .

:hasBroadPlaceOfPerformance a owl:ObjectProperty ;
    rdfs:isDefinedBy :core ;
    skos:definition "Geopolitical zone where the contract can be executed. Additional Information Used for setting restrictions that cannot be established with one country code or a geographical zone identifier (like NUTS), because they have a broader scope (geographical, economic, political, other). (epo:ContractTerm -> at-voc:other-place-service (+epo:hasBroadPlaceOfPerformance))"@en ;
    skos:prefLabel "Has broad place of performance"@en .

:hasBusinessSize a owl:ObjectProperty ;
    rdfs:isDefinedBy :core ;
    skos:definition "The category of the business depending on number of employees and turnover. Additional information: See Commission Recommendation of 6 May 2003 concerning the definition of micro, small and medium-sized enterprises. WG Approval 28/05/2020 (epo:Business -> at-voc:economic-operator-size (+epo:hasBusinessSize))"@en ;
    skos:prefLabel "Has business size"@en .

:hasBuyerCategoryDescription a owl:DatatypeProperty ;
    rdfs:isDefinedBy :core ;
    skos:definition "A classification of buyers participating in a framework agreement. Additional Information: Buyers that can use the Framework Agreement not mentioned by name. For example, the classification \"all hospitals in the Tuscany region\" is used instead of naming each individual buyer. This corresponds in eForms to BT-111 Framework Buyer Categories. WG Approval 2019-05-06 (epo:FrameworkAgreementTerm)"@en ;
    skos:prefLabel "Has buyer category description"@en .

:hasBuyerItemID a owl:ObjectProperty ;
    rdfs:isDefinedBy :core ;
    skos:definition "The general identifier assigned to the concept as defined by the Buyer.​ WG approval 16/05/2023 (epo-cat:Item -> adms:Identifier (+epo:hasBuyerItemID))"@en ;
    skos:prefLabel "Has buyer item i d"@en .

:hasBuyerLegalType a owl:ObjectProperty ;
    rdfs:isDefinedBy :core ;
    skos:definition "A category that indicates the right of an Organisation to play the role of a buyer. Additional Information: The category also effects the rules that the buyer has to abide to within the public procurement procedure. WG 07/09/2021 (org:Organization -> at-voc:buyer-legal-type (+epo:hasBuyerLegalType))"@en ;
    skos:prefLabel "Has buyer legal type"@en .

:hasBuyerLegalTypeDescription a owl:DatatypeProperty ;
    rdfs:isDefinedBy :core ;
    skos:definition "Self-explanatory text about the Buyer Legal Type. Additional information: This field is used when the Buyer Legal Type is not available in the controlled list at-voc:buyer-legal-type . This is necessary in to cover data provided in the TED Standard Forms. It shall be deprecated in the future. WG Approval 06/09/2022 (org:Organization)"@en ;
    skos:prefLabel "Has buyer legal type description"@en .

:hasBuyerProfile a owl:DatatypeProperty ;
    rdfs:isDefinedBy :core ;
    skos:definition "Website address where the buyer publishes information on its procurement procedures and general information. Additional information: This corresponds in the eForms to BT-508 Buyer Profile URL. WG approval 04/05/2018 (epo:Buyer)"@en ;
    skos:prefLabel "Has buyer profile"@en .

:hasCalculationMethod a owl:DatatypeProperty ;
    rdfs:isDefinedBy :core ;
    skos:definition "Formula for obtaining values. Additional Information: The possible values are monetary values, ranking scores, criterion weighting. WG Approval 25/05/2018 (epo:ConcessionEstimate)"@en ;
    skos:prefLabel "Has calculation method"@en .

:hasCarrierConsignmentID a owl:ObjectProperty ;
    rdfs:isDefinedBy :core ;
    skos:definition "The identifier of the the Consignment given by the Carrier. WG approval 10/06/2024 (epo-ful:Consignment -> adms:Identifier (+epo-ful:hasCarrierConsignmentID))"@en ;
    skos:prefLabel "Has carrier consignment i d"@en .

:hasCatalogueLineValidity a owl:ObjectProperty ;
    rdfs:isDefinedBy :core ;
    skos:definition "The relation indicating until when a Catalogue Line instance is applicable. WG approval 21/09/2023 (epo-cat:CatalogueLine -> epo:Period (+epo-cat:hasCatalogueLineValidity))"@en ;
    skos:prefLabel "Has catalogue line validity"@en .

:hasCertification a owl:ObjectProperty ;
    rdfs:isDefinedBy :core ;
    skos:definition "Relation to the proof of conformance. WG approval 30/05/2023 (foaf:Person -> epo:Certificate (+epo:hasCertification)) Relation to the proof of conformance. WG approval 30/05/2023 (org:Organization -> epo:Certificate (+epo:hasCertification)) Relation to the proof of conformance. WG approval 30/05/2023 (epo-cat:Item -> epo:Certificate (+epo:hasCertification))"@en ;
    skos:prefLabel "Has certification"@en .

:hasCertificationNumber a owl:DatatypeProperty ;
    rdfs:isDefinedBy :core ;
    skos:definition "The unique identifier of the certificate. WG approval 26/07/2022 (epo:Certificate)"@en ;
    skos:prefLabel "Has certification number"@en .

:hasChangeDescription a owl:DatatypeProperty ;
    rdfs:isDefinedBy :core ;
    skos:definition "Explanatory text about the instance of the concept. WG Approval 30/09/2019 (epo:ChangeInformation)"@en ;
    skos:prefLabel "Has change description"@en .

:hasChangeJustification a owl:ObjectProperty ;
    rdfs:isDefinedBy :core ;
    skos:definition "Code explaining the change. WG Approval 5/11/2019 (epo:ChangeInformation -> at-voc:change-corrig-justification (+epo:hasChangeJustification))"@en ;
    skos:prefLabel "Has change justification"@en .

:hasChangeReasonDescription a owl:DatatypeProperty ;
    rdfs:isDefinedBy :core ;
    skos:definition "Explanatory text about why the element is altered. Additional information: This corresponds in eForms to BT-762 Change Reason Description. (epo:ChangeInformation)"@en ;
    skos:prefLabel "Has change reason description"@en .

:hasChargeableWeight a owl:ObjectProperty ;
    rdfs:isDefinedBy :core ;
    skos:definition "The (epo-ful:Consignment -> epo:Quantity (+epo-ful:hasChargeableWeight))"@en ;
    skos:prefLabel "Has chargeable weight"@en .

:hasCleanVehicles a owl:DatatypeProperty ;
    rdfs:isDefinedBy :core ;
    skos:definition "The number of all clean vehicles that have either been purchased, leased, rented, hired-purchased or their use has been contractually committed to for the provision of a purchased service. Additional Information: In the European Union, the legal requirements and scope for the provision of these vehicles or services are covered by Directive 2009/33/EC. WG Approval 28/07/2020 (epo:VehicleInformation)"@en ;
    skos:prefLabel "Has clean vehicles"@en .

:hasConcessionEstimatedValue a owl:ObjectProperty ;
    rdfs:isDefinedBy :core ;
    skos:prefLabel "Has concession estimated value"@en .

:hasConditionVerificationMethod a owl:DatatypeProperty ;
    rdfs:isDefinedBy :core ;
    skos:definition "Means used to validate the qualification requirements. WG approval 02/05/2024 (epo:QualificationCriteriaSummary)"@en ;
    skos:prefLabel "Has condition verification method"@en .

:hasConfidentialityJustification a owl:DatatypeProperty ;
    rdfs:isDefinedBy :core ;
    skos:definition "A narrative explanation of why data is not published. Additional Information: This element is generally used when the non-publication-justification code chosen is \"other\". WG Approval 09/11/2021 (epo:NonPublishedInformation)"@en ;
    skos:prefLabel "Has confidentiality justification"@en .

:hasConfirmedIrregularityType a owl:ObjectProperty ;
    rdfs:isDefinedBy :core ;
    skos:definition "Additional information: This relation corresponds in eForms to BT-791 Review Irregularity Type (epo:ReviewDecision -> at-voc:irregularity-type (+epo:hasConfirmedIrregularityType))"@en ;
    skos:prefLabel "Has confirmed irregularity type"@en .

:hasConsigneeConsignmentID a owl:ObjectProperty ;
    rdfs:isDefinedBy :core ;
    skos:definition "The identifier of the the Consignment given by the Consignee. WG approval 10/06/2024 (epo-ful:Consignment -> adms:Identifier (+epo-ful:hasConsigneeConsignmentID))"@en ;
    skos:prefLabel "Has consignee consignment i d"@en .

:hasConsignmentDeclaredStatisticsValue a owl:ObjectProperty ;
    rdfs:isDefinedBy :core ;
    skos:prefLabel "Has consignment declared statistics value"@en .

:hasConsignmentFreeOnBoardValue a owl:ObjectProperty ;
    rdfs:isDefinedBy :core ;
    skos:definition "The Monetary Value of the Consignment when there is a transfer of liability for goods, damaged or destroyed, during shipping. at the exporter's customs frontier. (epo-ful:Consignment -> epo:MonetaryValue (+epo-ful:hasConsignmentFreeOnBoardValue))"@en ;
    skos:prefLabel "Has consignment free on board value"@en .

:hasConsignmentInvoiceValue a owl:ObjectProperty ;
    rdfs:isDefinedBy :core ;
    skos:definition "Declared amount of the Consignment. Additional Information: This is a logistics information needed for logistics, security measures, customs check, etc. WG approval 18/06/2024 (epo-ful:Consignment -> epo:MonetaryValue (+epo-ful:hasConsignmentInvoiceValue))"@en ;
    skos:prefLabel "Has consignment invoice value"@en .

:hasConstraint a owl:ObjectProperty ;
    rdfs:isDefinedBy :core ;
    skos:prefLabel "Has constraint"@en .

:hasContactName a owl:DatatypeProperty ;
    rdfs:isDefinedBy :core ;
    skos:definition "A short text by which a contact is known or referred to. WG Approval: 27/01/2022 (cpov:ContactPoint)"@en ;
    skos:prefLabel "Has contact name"@en .

:hasContactPointInRole a owl:ObjectProperty ;
    rdfs:isDefinedBy :core ;
    skos:prefLabel "Has contact point in role"@en .

:hasContractConclusionDate a owl:DatatypeProperty ;
    rdfs:isDefinedBy :core ;
    skos:definition "The date the contract was signed by the last signatory party. <u>Additional Information:</u> In exceptional cases contracts may be concluded without signature and therefore another date may be used. The date of contract conclusion is always later than the end of any standstill period. This concept is not to be confused with the date of completion/end of the contract. This corresponds in eForms to BT-145 Contract Conclusion Date. WG Approval 09/01/2020 (epo:Contract)"@en ;
    skos:prefLabel "Has contract conclusion date"@en .

:hasContractNatureType a owl:ObjectProperty ;
    rdfs:isDefinedBy :core ;
    skos:definition "Subject of the acquisition. WG Approval 11/06/2020 (epo:ContractTerm -> at-voc:contract-nature (+epo:hasContractNatureType))"@en ;
    skos:prefLabel "Has contract nature type"@en .

:hasContractValue a owl:ObjectProperty ;
    rdfs:isDefinedBy :core ;
    skos:prefLabel "Has contract value"@en .

:hasCountryCode a owl:ObjectProperty ;
    rdfs:isDefinedBy :core ;
    skos:definition "(locn:Address -> at-voc:country (+epo:hasCountryCode))"@en ;
    skos:prefLabel "Has country code"@en .

:hasCountryOfBirth a owl:ObjectProperty ;
    rdfs:isDefinedBy :core ;
    skos:definition "The country in which the Person was born. (person:Person -> at-voc:country (+epo:hasCountryOfBirth))"@en ;
    skos:prefLabel "Has country of birth"@en .

:hasCountryOfOrigin a owl:ObjectProperty ;
    rdfs:isDefinedBy :core ;
    skos:definition "The source country of the product or service. Additional Information: The country of origin can be provided by the buyer as a requirement or by the tenderer information of the item to be provided. WG Approval 07/01/2020 (epo-cat:Item -> at-voc:country (+epo-cat:hasCountryOfOrigin))"@en ;
    skos:prefLabel "Has country of origin"@en .

:hasCrossBorderLaw a owl:DatatypeProperty ;
    rdfs:isDefinedBy :core ;
    skos:definition "The applicable law when buyers from different countries procure together within one procurement procedure. Additional Information: This corresponds in eForms to BT-09 Cross Border Law. (epo:ProcedureTerm)"@en ;
    skos:prefLabel "Has cross border law"@en .

:hasCurrency a owl:ObjectProperty ;
    rdfs:isDefinedBy :core ;
    skos:definition "The identifier of the currency as in the standard code list used. (epo:MonetaryValue -> at-voc:currency (+epo:hasCurrency))"@en ;
    skos:prefLabel "Has currency"@en .

:hasCurrencyCodeListAgencyID a owl:DatatypeProperty ;
    rdfs:isDefinedBy :core ;
    skos:definition "Identifier of the agency that maintains the currency code list used. WG approval 13/04/2021 (epo:MonetaryValue)"@en ;
    skos:prefLabel "Has currency code list agency i d"@en .

:hasCurrencyCodeListAgencyName a owl:DatatypeProperty ;
    rdfs:isDefinedBy :core ;
    skos:definition "Name of the agency that maintains the currency code list used. WG approval 13/04/2021 (epo:MonetaryValue)"@en ;
    skos:prefLabel "Has currency code list agency name"@en .

:hasCurrencyCodeListID a owl:DatatypeProperty ;
    rdfs:isDefinedBy :core ;
    skos:definition "Concept scheme URI used for the currency code list. WG approval 13/04/2021 (epo:MonetaryValue)"@en ;
    skos:prefLabel "Has currency code list i d"@en .

:hasDPSScope a owl:ObjectProperty ;
    rdfs:isDefinedBy :core ;
    skos:definition "Explanation as to whether a dps is used and by whom. Additional Information: This corresponds in eForms to BT-766 Dynamic Purchasing System. WG Approval 09/11/2021 (epo:DynamicPurchaseSystemTechnique -> at-voc:dps-usage (+epo:hasDPSScope))"@en ;
    skos:prefLabel "Has d p s scope"@en .

:hasDeadline a owl:DatatypeProperty ;
    rdfs:isDefinedBy :core ;
    skos:definition "The time limit by which the security clearance must be submitted to the buyer. WG Approval 02/05/2024 (epo:SecurityClearanceTerm)"@en ;
    skos:prefLabel "Has deadline"@en .

:hasDebitedAccountIdentifier a owl:ObjectProperty ;
    rdfs:isDefinedBy :core ;
    skos:definition "An identifier for the account to be debited by the direct debit. WG approval 11/07/2024 (epo-inv:PaymentInstructionsInformation -> adms:Identifier (+epo-inv:hasDebitedAccountIdentifier))"@en ;
    skos:prefLabel "Has debited account identifier"@en .

:hasDecisionDate a owl:DatatypeProperty ;
    rdfs:isDefinedBy :core ;
    skos:definition "The date of the review decision. Additional information: This attribute corresponds to the BT-787 Review Date in eForms. (epo:ReviewDecision)"@en ;
    skos:prefLabel "Has decision date"@en .

:hasDeclaredStatisticalValue a owl:ObjectProperty ;
    rdfs:isDefinedBy :core ;
    skos:definition "The Monetary Value declared for statistical purposes. WG approval 10/06/2024 (epo-ful:Consignment -> epo:MonetaryValue (+epo-ful:hasDeclaredStatisticalValue))"@en ;
    skos:prefLabel "Has declared statistical value"@en .

:hasDeliveryLocation a owl:ObjectProperty ;
    rdfs:isDefinedBy :core ;
    skos:definition "Location delivery area where the Item can be ordered to the given price. (epo-cat:Price -> dct:Location (+epo-cat:hasDeliveryLocation))"@en ;
    skos:prefLabel "Has delivery location"@en .

:hasDeliveryPeriod a owl:ObjectProperty ;
    rdfs:isDefinedBy :core ;
    skos:prefLabel "Has delivery period"@en .

:hasDescriptionOfPrizes a owl:DatatypeProperty ;
    rdfs:isDefinedBy :core ;
    skos:definition "Explanatory text about Prizes. WG approval 26/03/2024 (epo:DesignContestRegimeTerm)"@en ;
    skos:prefLabel "Has description of prizes"@en .

:hasDespatchPeriod a owl:ObjectProperty ;
    rdfs:isDefinedBy :core ;
    skos:definition "The time period when the Despatcher picks-up the Goods Items to be delivered. WG approval 16/07/2024 (epo-ful:ShipmentInformation -> epo:Period (+epo-ful:hasDespatchPeriod))"@en ;
    skos:prefLabel "Has despatch period"@en .

:hasDespatchedQuantity a owl:ObjectProperty ;
    rdfs:isDefinedBy :core ;
    skos:definition "The Quantity that has been sent. WG approval 18/06/2024 (epo-ful:DespatchLine -> epo:Quantity (+epo-ful:hasDespatchedQuantity))"@en ;
    skos:prefLabel "Has despatched quantity"@en .

:hasDespatcherConsignmentID a owl:ObjectProperty ;
    rdfs:isDefinedBy :core ;
    skos:definition "The identifier of the the Consignment given by the Despatcher. WG approval 10/06/2024 (epo-ful:Consignment -> adms:Identifier (+epo-ful:hasDespatcherConsignmentID))"@en ;
    skos:prefLabel "Has despatcher consignment i d"@en .

:hasDirectAwardJustification a owl:ObjectProperty ;
    rdfs:isDefinedBy :core ;
    skos:definition "List of reasons for using a procedure which allows awarding contracts directly without publishing a notice. WG Approval 28/05/2020 (epo:DirectAwardTerm -> at-voc:direct-award-justification (+epo:hasDirectAwardJustification))"@en ;
    skos:prefLabel "Has direct award justification"@en .

:hasDispatchDate a owl:DatatypeProperty ;
    rdfs:isDefinedBy :core ;
    skos:definition "Date and time of transmission of a record to an Organization. WG Approval 31/08/2023 (epo:Document)"@en ;
    skos:prefLabel "Has dispatch date"@en .

:hasDocumentRestrictionJustification a owl:ObjectProperty ;
    rdfs:isDefinedBy :core ;
    skos:definition "An explanation about the reasons why some procurement documents are restricted. Additional Information: This corresponds in eForms to BT-707 Documents Restricted Justification. WG Approval 09/03/2021 (epo:AccessTerm -> at-voc:communication-justification (+epo:hasDocumentRestrictionJustification))"@en ;
    skos:prefLabel "Has document restriction justification"@en .

:hasDurationExtensionJustification a owl:DatatypeProperty ;
    rdfs:isDefinedBy :core ;
    skos:definition "The explanation of the reason why the framework agreement has an extended duration. Additional Information: This corresponds in eForms to BT-109 Framework Duration Justification. The justification for exceptional cases when the duration of the framework agreement exceeds the legal limits. Four years in the case of the general procurement Directive, seven years in the case of the defence Directive, and eight years in the case of the sectoral Directive. WG Approval 26/09/2019 (epo:FrameworkAgreementTerm)"@en ;
    skos:prefLabel "Has duration extension justification"@en .

:hasEAuctionURL a owl:DatatypeProperty ;
    rdfs:isDefinedBy :core ;
    skos:definition "The internet address of the electronic auction. Additional Information: This corresponds in eForms to BT-123 Electronic Auction URL. (epo:SubmissionTerm)"@en ;
    skos:prefLabel "Has e auction u r l"@en .

:hasECataloguePermission a owl:ObjectProperty ;
    rdfs:isDefinedBy :core ;
    skos:definition "The extent to which electronic catalogues may be used in tenders. WG Approval 03/10/2019 (epo:SubmissionTerm -> at-voc:permission (+epo:hasECataloguePermission))"@en ;
    skos:prefLabel "Has e catalogue permission"@en .

:hasEEAReceivedTenders a owl:DatatypeProperty ;
    rdfs:isDefinedBy :core ;
    skos:definition "The amount of tenders received from economic operators in other EEA countries other than the country of the buyer. WG Approval 12/12/2019 (epo:SubmissionStatisticalInformation)"@en ;
    skos:prefLabel "Has e e a received tenders"@en .

:hasEFormsSubtype a owl:DatatypeProperty ;
    rdfs:isDefinedBy :core ;
    skos:prefLabel "Has e forms subtype"@en .

:hasEInvoicing a owl:DatatypeProperty ;
    rdfs:isDefinedBy :core ;
    skos:definition "Electronic means will be used for invoicing in the post-award process. Additional Information: This attribute is used for standard form mappings. WG Approval 12/09/2019 (epo:ContractTerm)"@en ;
    skos:prefLabel "Has e invoicing"@en .

:hasEInvoicingPermission a owl:ObjectProperty ;
    rdfs:isDefinedBy :core ;
    skos:prefLabel "Has e invoicing permission"@en .

:hasEOrdering a owl:DatatypeProperty ;
    rdfs:isDefinedBy :core ;
    skos:definition "Electronic means will be used for requesting and purchasing in the post-award process. WG Approval 12/09/2019 (epo:ContractTerm)"@en ;
    skos:prefLabel "Has e ordering"@en .

:hasEPayment a owl:DatatypeProperty ;
    rdfs:isDefinedBy :core ;
    skos:definition "Electronic means must be used for paying. WG Approval 09/11/2021 (epo:ContractTerm)"@en ;
    skos:prefLabel "Has e payment"@en .

:hasESenderDispatchDate a owl:DatatypeProperty ;
    rdfs:isDefinedBy :core ;
    skos:definition "The date and time the notice was transmitted electronically by the eSender to the Publications Office of the European Union. Additional Information: Typically, eSenders include national Official Journals, Buyers sending a large number of electronic Notices, public or private bodies acting on behalf of Buyers and eProcurement software developers. WG approval 20/06/2023 (epo:Notice)"@en ;
    skos:prefLabel "Has e sender dispatch date"@en .

:hasESubmissionPermission a owl:ObjectProperty ;
    rdfs:isDefinedBy :core ;
    skos:definition "The requirements as to what extent electronic submission is allowed. WG Approval 03/10/2019 (epo:SubmissionTerm -> at-voc:permission (+epo:hasESubmissionPermission))"@en ;
    skos:prefLabel "Has e submission permission"@en .

:hasEUReceivedTenders a owl:DatatypeProperty ;
    rdfs:isDefinedBy :core ;
    skos:definition "The amount of tenders received from economic operators in other EU countries other than the country of the buyer. (epo:SubmissionStatisticalInformation)"@en ;
    skos:prefLabel "Has e u received tenders"@en .

:hasElectronicDigest a owl:ObjectProperty ;
    rdfs:isDefinedBy :core ;
    skos:prefLabel "Has electronic digest"@en .

:hasElectronicSignature a owl:ObjectProperty ;
    rdfs:isDefinedBy :core ;
    skos:prefLabel "Has electronic signature"@en .

:hasElectronicSubmission a owl:DatatypeProperty ;
    rdfs:isDefinedBy :core ;
    skos:definition "Transmission of tenders is possible by electronic means of communication. (epo:Tender)"@en ;
    skos:prefLabel "Has electronic submission"@en .

:hasElectronicTenders a owl:DatatypeProperty ;
    rdfs:isDefinedBy :core ;
    skos:definition "Electronic Tender Lots received. WG Approval 28/07/2020 (epo:SubmissionStatisticalInformation)"@en ;
    skos:prefLabel "Has electronic tenders"@en .

:hasElementReference a owl:DatatypeProperty ;
    rdfs:isDefinedBy :core ;
    skos:definition "Reference to the class instance in the current notice. Additional information: This corresponds in eForms to BT-13716 Change Previous Notice Section Identifier, BT-786 Review Notice Section Identifier and BT-1501 Modification Previous Notice Section Identifier. (epo:ReviewObject)"@en ;
    skos:prefLabel "Has element reference"@en .

:hasEnd a owl:DatatypeProperty ;
    rdfs:isDefinedBy :core ;
    skos:definition "The date and time at which this period ends. (epo:Period)"@en ;
    skos:prefLabel "Has end"@en .

:hasEndpointIdentifier a owl:ObjectProperty ;
    rdfs:isDefinedBy :core ;
    skos:prefLabel "Has endpoint identifier"@en .

:hasEntryIntoForceDate a owl:DatatypeProperty ;
    rdfs:isDefinedBy :core ;
    skos:definition "The date on which the contract enters into force. Additional information: This is generally the date on which the fulfillment of the contract begins. This corresponds in eForms to WG approval 05/11/2019 (epo:Contract)"@en ;
    skos:prefLabel "Has entry into force date"@en .

:hasEstimatedBuyerConcessionRevenue a owl:ObjectProperty ;
    rdfs:isDefinedBy :core ;
    skos:definition "The expected payments made by the buyer to the economic operator awarded the concession that are not directly related to the use of the concession. <u>Additional Information:</u> For example the public buyer pays a yearly fee to provide a ticketing solution to the public. The fee the public pays for every ticket sold through the solution is not included in this estimation but in the estimation of the user concession revenue. This corresponds to BT-160 in eForms. WG Approval 07/01/2020 (epo:ConcessionEstimate -> epo:MonetaryValue (+epo:hasEstimatedBuyerConcessionRevenue))"@en ;
    skos:prefLabel "Has estimated buyer concession revenue"@en .

:hasEstimatedContractNoticePublicationDate a owl:DatatypeProperty ;
    rdfs:isDefinedBy :core ;
    skos:definition "Foreseen date for publication of Contract Notice. Additional information: This corresponds in eForms BT-127 Future Notice. (epo:ProcessPlanningTerm)"@en ;
    skos:prefLabel "Has estimated contract notice publication date"@en .

:hasEstimatedDeliveryPeriod a owl:ObjectProperty ;
    rdfs:isDefinedBy :core ;
    skos:definition "The forecasted time period given by the Despatcher to provide the goods and services. WG approval 18/06/2024 (epo-ful:ShipmentInformation -> epo:Period (+epo-ful:hasEstimatedDeliveryPeriod))"@en ;
    skos:prefLabel "Has estimated delivery period"@en .

:hasEstimatedDuration a owl:ObjectProperty ;
    rdfs:isDefinedBy :core ;
    skos:definition "Relation indicating a Contract has an estimated Duration. Additional Information When the Lot uses a Technique the contract estimated duration applies to the Technique. (epo:Contract -> epo:Duration (+epo:hasEstimatedDuration))"@en ;
    skos:prefLabel "Has estimated duration"@en .

:hasEstimatedInvitationToExpressInterestDate a owl:DatatypeProperty ;
    rdfs:isDefinedBy :core ;
    skos:definition "The estimated date of dispatch of the invitations to confirm interest. Additional Information: This corresponds in eForms to BT-631 Dispatch Invitation Interest. (epo:MultipleStageProcedureTerm)"@en ;
    skos:prefLabel "Has estimated invitation to express interest date"@en .

:hasEstimatedInvitationToTenderDate a owl:DatatypeProperty ;
    rdfs:isDefinedBy :core ;
    skos:definition "The estimated date of dispatch of the invitations to submit tenders in two (or more) stage procedures. Additional Information: This corresponds in eForms to BT-130 Dispatch Invitation Tender. WG Approval 01/10/2019 (epo:MultipleStageProcedureTerm)"@en ;
    skos:prefLabel "Has estimated invitation to tender date"@en .

:hasEstimatedPercentage a owl:DatatypeProperty ;
    rdfs:isDefinedBy :core ;
    skos:definition "The estimated proportion foreseen to be subcontracted. WG Approval 07/01/2020 (epo:SubcontractingEstimate)"@en ;
    skos:prefLabel "Has estimated percentage"@en .

:hasEstimatedTenderInvitationDate a owl:DatatypeProperty ;
    rdfs:isDefinedBy :core ;
    skos:definition "The planned date for the dispatch of the invitations to submit tenders. WG Approval 09/11/2021 (epo:ProcessPlanningTerm)"@en ;
    skos:prefLabel "Has estimated tender invitation date"@en .

:hasEstimatedTotalSubcontracts a owl:DatatypeProperty ;
    rdfs:isDefinedBy :core ;
    skos:definition "The estimated amount of work to be subcontracted in the contract resulting from the lot. WG Approval 09/11/2021 (epo:SubmissionStatisticalInformation)"@en ;
    skos:prefLabel "Has estimated total subcontracts"@en .

:hasEstimatedUserConcessionRevenue a owl:ObjectProperty ;
    rdfs:isDefinedBy :core ;
    skos:definition "The estimated revenue coming from the use of the concession. Additional Information: Revenues are for example fees and fines. For example, the fees and fines coming from the cars using a motorway. This corresponds to BT-162 in eForms. (epo:ConcessionEstimate -> epo:MonetaryValue (+epo:hasEstimatedUserConcessionRevenue))"@en ;
    skos:prefLabel "Has estimated user concession revenue"@en .

:hasEstimatedValue a owl:ObjectProperty ;
    rdfs:isDefinedBy :core ;
    skos:definition "A forecast of the value of the procurement before competition. Additional Information: Different cases of estimated values may refer to a lot, the global value of the procedure, or of a combinatorial value of a group of lots. The forecast is calculated by the buyer and covers all revenues whether coming from the buyer or third parties. See for example recital (19), Article 5 of Directive 2014/24/EU and other articles from the rest of Directives about procurement. In the case of framework agreements and dynamic purchasing systems this refers to the maximum estimated value. This property corresponds to BT-27 in eForms (for Lot and Procedure) and can be used for BT-157 (for LotGroup). <b> </b>WG Approval 05/12/2019 (epo:LotGroup -> epo:MonetaryValue (+epo:hasEstimatedValue)) A forecast of the value of the procurement before competition. Additional Information: Different cases of estimated values may refer to a lot, the global value of the procedure, or of a combinatorial value of a group of lots. The forecast is calculated by the buyer and covers all revenues whether coming from the buyer or third parties. See for example recital (19), Article 5 of Directive 2014/24/EU and other articles from the rest of Directives about procurement. In the case of framework agreements and dynamic purchasing systems this refers to the maximum estimated value. This property corresponds to BT-27 in eForms (for Lot and Procedure) and can be used for BT-157 (for LotGroup). <b> </b><b>WG Approval 05/12/2019</b> (epo:ProcurementElement -> epo:MonetaryValue (+epo:hasEstimatedValue))"@en ;
    skos:prefLabel "Has estimated value"@en .

:hasExpectedDeliveryTime a owl:ObjectProperty ;
    rdfs:isDefinedBy :core ;
    skos:definition "The expected amount of time between the order and delivery of an item. WG approval 26/07/2022 (epo-cat:Price -> epo:Duration (+epo-cat:hasExpectedDeliveryTime))"@en ;
    skos:prefLabel "Has expected delivery time"@en .

:hasExternalSpecification a owl:ObjectProperty ;
    rdfs:isDefinedBy :core ;
    skos:definition "URI reference to external item information or specifications, e.g. web address. (epo-cat:Item -> epo:Document (+epo-cat:hasExternalSpecification))"@en ;
    skos:prefLabel "Has external specification"@en .

:hasFax a owl:DatatypeProperty ;
    rdfs:isDefinedBy :core ;
    skos:definition "The fax number used to reach a person or an organisation. (cpov:ContactPoint)"@en ;
    skos:prefLabel "Has fax"@en .

:hasFinancialOfferValue a owl:ObjectProperty ;
    rdfs:isDefinedBy :core ;
    skos:definition "The value offered by the Tenderer for a Lot. Additional Information: This value is normally the one awarded for a winning Tender Lot. In case of negotiated procedures the original financial value may be reviewed and the offer updated. This corresponds to BT-720 in eForms. (epo:Tender -> epo:MonetaryValue (+epo:hasFinancialOfferValue))"@en ;
    skos:prefLabel "Has financial offer value"@en .

:hasFixedValue a owl:DatatypeProperty ;
    rdfs:isDefinedBy :core ;
    skos:definition "This corresponds in the eForms to BT-541 Award Criterion Number in association with BT-5422 Award Criterion Number Fixed. (epo:AwardCriterion)"@en ;
    skos:prefLabel "Has fixed value"@en .

:hasFixedValueType a owl:ObjectProperty ;
    rdfs:isDefinedBy :core ;
    skos:definition "The method to interpret the fixed value as pertaining to a total or unit. WG Approval 17/09/2019 (epo:AwardCriterion -> at-voc:number-fixed (+epo:hasFixedValueType))"@en ;
    skos:prefLabel "Has fixed value type"@en .

:hasFollowupContract a owl:DatatypeProperty ;
    rdfs:isDefinedBy :core ;
    skos:definition "Any subsequent service contract will be awarded to the winner or, in the case of a design contest, winners. WG Approval 29/08/2019 (epo:DesignContestRegimeTerm)"@en ;
    skos:prefLabel "Has followup contract"@en .

:hasFollowupContractInformation a owl:DatatypeProperty ;
    rdfs:isDefinedBy :core ;
    skos:definition "Further information about follow-up contracts, prizes and payments (for example non-monetary prizes, payments given for participation). WG Approval 03/09/2019 (epo:DesignContestRegimeTerm)"@en ;
    skos:prefLabel "Has followup contract information"@en .

:hasFormNumber a owl:DatatypeProperty ;
    rdfs:isDefinedBy :core ;
    skos:definition "The number of the form used to create the Standard Form Notice and not an eForms Notice. WG approval 26/03/2024 (epo:Notice)"@en ;
    skos:prefLabel "Has form number"@en .

:hasFormType a owl:ObjectProperty ;
    rdfs:isDefinedBy :core ;
    skos:definition "A categorisation of the steps in which the Notice is used. WG Approval 12/05/2020 (epo:Notice -> at-voc:form-type (+epo:hasFormType))"@en ;
    skos:prefLabel "Has form type"@en .

:hasFormula a owl:DatatypeProperty ;
    rdfs:isDefinedBy :core ;
    skos:definition "The mathematical equation or any other description used for complicated weighing of criteria (e.g. non-linear weighing, the analytic hierarchy process) when a weighing cannot be expressed per criterion. Additional Information: This corresponds in eForms to BT-543. (epo:ProcurementCriterion)"@en ;
    skos:prefLabel "Has formula"@en .

:hasFrameworkAgreementMaximumValue a owl:ObjectProperty ;
    rdfs:isDefinedBy :core ;
    skos:prefLabel "Has framework agreement maximum value"@en .

:hasFrameworkAgreementType a owl:ObjectProperty ;
    rdfs:isDefinedBy :core ;
    skos:definition "The form of framework agreement used in a procurement procedure. Addition information: A concept to distinguish the different types of framework agreement, which are: 1. Framework agreement without reopening of competition, 2. Framework agreement with reopening of competition, or 3. Framework agreement partly without reopening of competition. WG Approval 19/09/2019 (epo:FrameworkAgreementTerm -> at-voc:framework-agreement (+epo:hasFrameworkAgreementType))"@en ;
    skos:prefLabel "Has framework agreement type"@en .

:hasFreightForwarderConsignmentID a owl:ObjectProperty ;
    rdfs:isDefinedBy :core ;
    skos:definition "The identifier of the the Consignment given by the Freight Forwarder. WG approval 10/06/2024 (epo-ful:Consignment -> adms:Identifier (+epo-ful:hasFreightForwarderConsignmentID))"@en ;
    skos:prefLabel "Has freight forwarder consignment i d"@en .

:hasFundProgramme a owl:ObjectProperty ;
    rdfs:isDefinedBy :core ;
    skos:prefLabel "Has fund programme"@en .

:hasGrossMonetaryValue a owl:ObjectProperty ;
    rdfs:isDefinedBy :core ;
    skos:prefLabel "Has gross monetary value"@en .

:hasGrossVolume a owl:ObjectProperty ;
    rdfs:isDefinedBy :core ;
    skos:definition "The amount of space that is required including the packaging. WG approval 18/06/2024 (epo-ful:AbstractContainer -> epo:Quantity (+epo-ful:hasGrossVolume)) The amount of space that is required including the packaging. WG approval 18/06/2024 (epo-ful:Consignment -> epo:Quantity (+epo-ful:hasGrossVolume))"@en ;
    skos:prefLabel "Has gross volume"@en .

:hasGrossWeight a owl:ObjectProperty ;
    rdfs:isDefinedBy :core ;
    skos:definition "The total mass of goods including the packaging. WG approval 18/06/2024 (epo-ful:AbstractContainer -> epo:Quantity (+epo-ful:hasGrossWeight)) The total mass of goods including the packaging. WG approval 18/06/2024 (epo-ful:Consignment -> epo:Quantity (+epo-ful:hasGrossWeight))"@en ;
    skos:prefLabel "Has gross weight"@en .

:hasGroupFrameworkAgreementMaximumValue a owl:ObjectProperty ;
    rdfs:isDefinedBy :core ;
    skos:definition "This corresponds to BT-156 in the eForms. (epo:LotGroupAwardInformation -> epo:MonetaryValue (+epo:hasGroupFrameworkAgreementMaximumValue))"@en ;
    skos:prefLabel "Has group framework agreement maximum value"@en .

:hasGroupLotEvaluationMethod a owl:DatatypeProperty ;
    rdfs:isDefinedBy :core ;
    skos:definition "Description of how lots and groups of lots are evaluated against one another in the procedure. (epo:ProcedureTerm)"@en ;
    skos:prefLabel "Has group lot evaluation method"@en .

:hasGroupType a owl:DatatypeProperty ;
    rdfs:isDefinedBy :core ;
    skos:definition "Form of collaboration agreement between organisations. Additional Information: This is not a legal type; not to be mistaken with epo:hasLegalFormType which may also be used for Organisation Groups. WG Approval 09/11/2021 (epo:OrganisationGroup)"@en ;
    skos:prefLabel "Has group type"@en .

:hasGuaranteeDescription a owl:DatatypeProperty ;
    rdfs:isDefinedBy :core ;
    skos:definition "Information on the financial commitment required from the economic operator. Additional Information: 1. This information may include the amount and the way of delivering of the guarantee 2. The financial commitment may be retained by the buyer in the case the tenderer withdraws the submitted information (i.e. tender, expression of interest and request for participation, but not request for clarifications) before the award of the contract or does not sign the contract. 3. Usual modalities are bonds, cheques, loans, other. WG Approval 21/07/20 (epo:SubmissionTerm)"@en ;
    skos:prefLabel "Has guarantee description"@en .

:hasHeight a owl:ObjectProperty ;
    rdfs:isDefinedBy :core ;
    skos:definition "The vertical measurement. WG approval 18/06/2024 (epo-ful:AbstractContainer -> epo:Quantity (+epo-ful:hasHeight))"@en ;
    skos:prefLabel "Has height"@en .

:hasHighestReceivedTenderValue a owl:ObjectProperty ;
    rdfs:isDefinedBy :core ;
    skos:definition "Amount of the Tender with the highest value. Additional Information The value must correspond to an admissible tender. For example, tenders compliant with the procurement document requirements, not having an abnormally low price or cost, etc. WG Approval 12/12/2019 (epo:SubmissionStatisticalInformation -> epo:MonetaryValue (+epo:hasHighestReceivedTenderValue))"@en ;
    skos:prefLabel "Has highest received tender value"@en .

:hasInadmissibleTenders a owl:DatatypeProperty ;
    rdfs:isDefinedBy :core ;
    skos:definition "Tenders received that cannot be awarded due to non-compliance to procurement document requirements or having an abnormally low price or cost. <u>Additional Information: </u> Non-compliance with a Procurement Document requirements include exclusion grounds, selection criteria and submission deadline, etc. WG Approval 12/12/2019 (epo:SubmissionStatisticalInformation)"@en ;
    skos:prefLabel "Has inadmissible tenders"@en .

:hasInternalIdentifier a owl:ObjectProperty ;
    rdfs:isDefinedBy :core ;
    skos:prefLabel "Has internal identifier"@en .

:hasInternetAddress a owl:DatatypeProperty ;
    rdfs:isDefinedBy :core ;
    skos:definition "The main web page used by the instance of the concept. WG Approval 01/06/2023 (cpov:ContactPoint) The main web page used by the instance of the concept. WG Approval 01/06/2023 (org:Organization)"@en ;
    skos:prefLabel "Has internet address"@en .

:hasInvoiceLineObjectIdentifier a owl:ObjectProperty ;
    rdfs:isDefinedBy :core ;
    skos:definition "An identifier for an object on which the invoice line is based, given by the Seller. Additional Information: It may be a subscription number, telephone number, meter point etc., as applicable. WG approval 26/06/2024 (epo-inv:InvoiceLine -> adms:Identifier (+epo-inv:hasInvoiceLineObjectIdentifier))"@en ;
    skos:prefLabel "Has invoice line object identifier"@en .

:hasInvoiceLinePeriod a owl:ObjectProperty ;
    rdfs:isDefinedBy :core ;
    skos:prefLabel "Has invoice line period"@en .

:hasInvoicedObjectIdentifier a owl:ObjectProperty ;
    rdfs:isDefinedBy :core ;
    skos:definition "An identifier for an object on which the invoice is based, given by the Seller. (epo-inv:Invoice -> adms:Identifier (+epo-inv:hasInvoicedObjectIdentifier))"@en ;
    skos:prefLabel "Has invoiced object identifier"@en .

:hasInvoicingPeriod a owl:ObjectProperty ;
    rdfs:isDefinedBy :core ;
    skos:prefLabel "Has invoicing period"@en .

:hasIrregularityType a owl:ObjectProperty ;
    rdfs:isDefinedBy :core ;
    skos:definition "Additional information: This relation corresponds in eForms to BT-636 Buyer Review Requests Irregularity Type (epo:ReviewIrregularitySummary -> at-voc:irregularity-type (+epo:hasIrregularityType))"@en ;
    skos:prefLabel "Has irregularity type"@en .

:hasItemClassificationIdentifier a owl:ObjectProperty ;
    rdfs:isDefinedBy :core ;
    skos:prefLabel "Has item classification identifier"@en .

:hasItemCountryOfOrigin a owl:ObjectProperty ;
    rdfs:isDefinedBy :core ;
    skos:definition "The source country of the product or service. Additional Information: The country of origin can be provided by the buyer as a requirement or by the tenderer information of the item to be provided. WG Approval 07/01/2020 The codelist to be used is at-voc:country which is available at http://publications.europa.eu/resource/dataset/country (epo:Tender -> at-voc:country (+epo:hasItemCountryOfOrigin))"@en ;
    skos:prefLabel "Has item country of origin"@en .

:hasItemStandardID a owl:ObjectProperty ;
    rdfs:isDefinedBy :core ;
    skos:definition "The general identifier assigned to the concept based on a standard scheme.​ Additional information: For example the GTIN scheme (Global Trade Item Number). WG approval 16/05/2023 (epo-cat:Item -> adms:Identifier (+epo:hasItemStandardID))"@en ;
    skos:prefLabel "Has item standard i d"@en .

:hasJustification a owl:DatatypeProperty ;
    rdfs:isDefinedBy :core ;
    skos:definition "An explanation about the reasons for using the concept. WG Approval 5/11/2019 (epo:DirectAwardTerm)"@en ;
    skos:prefLabel "Has justification"@en .

:hasLabelType a owl:ObjectProperty ;
    rdfs:isDefinedBy :core ;
    skos:definition "The label type such environmental, quality, social etc. (epo:CertificationLabel -> at-voc-new:certification-label-type (+epo:hasLabelType))"@en ;
    skos:prefLabel "Has label type"@en .

:hasLanguage a owl:ObjectProperty ;
    rdfs:isDefinedBy :core ;
    skos:definition "Language in which the submitted information is to be expressed. WG Approval 21/07/2020 (epo:SubmissionTerm -> at-voc:language (+epo:hasLanguage))"@en ;
    skos:prefLabel "Has language"@en .

:hasLateSubmissionInformationDescription a owl:DatatypeProperty ;
    rdfs:isDefinedBy :core ;
    skos:definition "A narrative text explaining the content of the economic operator information that can be submitted late. Additional Information This does not apply to requests for clarifications. (epo:SubmissionTerm)"@en ;
    skos:prefLabel "Has late submission information description"@en .

:hasLateSubmissionPermission a owl:ObjectProperty ;
    rdfs:isDefinedBy :core ;
    skos:definition "Whether economic operator-related information can be supplemented even after the submission deadline. Additional Information This is specific to the information on the economic operator and not the actual offer. This does not apply to the requests for clarification. WG Approval 21/07/2020 (epo:SubmissionTerm -> at-voc:missing-info-submission (+epo:hasLateSubmissionPermission))"@en ;
    skos:prefLabel "Has late submission permission"@en .

:hasLaunchFrameworkAgreementMaximumValue a owl:ObjectProperty ;
    rdfs:isDefinedBy :core ;
    skos:prefLabel "Has launch framework agreement maximum value"@en .

:hasLegalBasis a owl:ObjectProperty ;
    rdfs:isDefinedBy :core ;
    skos:definition "The legal basis under which the procurement procedure takes place. Additional Information: For example European Directives or Regulations, national laws etc. The recommended code list is the example for the legal basis at the European level. WG 04/04/2023 (epo:ProcurementObject -> at-voc:legal-basis (+epo:hasLegalBasis))"@en ;
    skos:prefLabel "Has legal basis"@en .

:hasLegalBasisDescription a owl:DatatypeProperty ;
    rdfs:isDefinedBy :core ;
    skos:definition "Explanatory text about the legal basis. WG approval 02/05/2024 (epo:ProcurementObject)"@en ;
    skos:prefLabel "Has legal basis description"@en .

:hasLegalFormRequirement a owl:DatatypeProperty ;
    rdfs:isDefinedBy :core ;
    skos:definition "The legal form to be taken by a Contractor. Additional Information: Generally, this is defined to cover the case where an Organisation Group is involved. Note that the codelist provided at national level should be used. (epo:ContractTerm)"@en ;
    skos:prefLabel "Has legal form requirement"@en .

:hasLegalFormType a owl:DatatypeProperty ;
    rdfs:isDefinedBy :core ;
    skos:definition "The classification of an Organisation according to legislation. Additional Information: Generally, this is defined for Tenderers who want to submit as an Organisation Group. Note that the codelist provided at national level should be used. (org:Organization)"@en ;
    skos:prefLabel "Has legal form type"@en .

:hasLegalIdentifier a owl:ObjectProperty ;
    rdfs:isDefinedBy :core ;
    skos:prefLabel "Has legal identifier"@en .

:hasLegalName a owl:DatatypeProperty ;
    rdfs:isDefinedBy :core ;
    skos:definition "The officially registered name of an organisation. WG Approval 10/01/2023 (org:Organization)"@en ;
    skos:prefLabel "Has legal name"@en .

:hasLength a owl:ObjectProperty ;
    rdfs:isDefinedBy :core ;
    skos:definition "The horizontal measurement. Additional Information: The length is the longer side between the length and the width. WG approval 18/06/2024 (epo-ful:AbstractContainer -> epo:Quantity (+epo-ful:hasLength))"@en ;
    skos:prefLabel "Has length"@en .

:hasLoadingLength a owl:ObjectProperty ;
    rdfs:isDefinedBy :core ;
    skos:definition "The length (epo-ful:Consignment -> epo:Quantity (+epo-ful:hasLoadingLength))"@en ;
    skos:prefLabel "Has loading length"@en .

:hasLoadingMeter a owl:ObjectProperty ;
    rdfs:isDefinedBy :core ;
    skos:definition "The area of the Consignment in meters divided by the width of the truck, which is considered to be 2.4 meters. WG approval 18/06/2024 (epo-ful:Consignment -> epo:Quantity (+epo-ful:hasLoadingMeter))"@en ;
    skos:prefLabel "Has loading meter"@en .

:hasLotAwardCombination a owl:DatatypeProperty ;
    rdfs:isDefinedBy :core ;
    skos:definition "The contracting authority reserves the right to award contracts combining lots or groups of lots. Additional Information: This property contains information about the Lots concerned. This property is required by the regulation (EU)-2015-1986 (modeled in the TED Standard Forms). WG approval 23/08/2022 (epo:ProcedureTerm)"@en ;
    skos:prefLabel "Has lot award combination"@en .

:hasLotReference a owl:ObjectProperty ;
    rdfs:isDefinedBy :core ;
    skos:prefLabel "Has lot reference"@en .

:hasLowestReceivedTenderValue a owl:ObjectProperty ;
    rdfs:isDefinedBy :core ;
    skos:definition "Amount of the Tender with the lowest value. Additional Information The value must correspond to an admissible tender. For example, tenders compliant with the procurement document requirements, not having an abnormally low price or cost, etc. WG Approval 12/12/2019 (epo:SubmissionStatisticalInformation -> epo:MonetaryValue (+epo:hasLowestReceivedTenderValue))"@en ;
    skos:prefLabel "Has lowest received tender value"@en .

:hasMainActivity a owl:ObjectProperty ;
    rdfs:isDefinedBy :core ;
    skos:definition "The principal sectoral area in which an organisation operates. Additional information: The activities associated with buyers are derived from the top level of the Classification of the functions of the government (COFOG) from the United Nations Statistics Division. The activities associated with buyer are derived from sectors explicitly falling within the sectoral directive (2014/25/EU Art. 8 - Art. 14). WG Approval 05/05/2020 (org:Organization -> at-voc:main-activity (+epo:hasMainActivity))"@en ;
    skos:prefLabel "Has main activity"@en .

:hasMainActivityDescription a owl:DatatypeProperty ;
    rdfs:isDefinedBy :core ;
    skos:definition "Self-explanatory text about the Main Activity . Additional information: This field is used when the Main Activity is not available in the controlled list at-voc:main-activity-type . This is necessary in to cover data provided in the TED Standard Forms. It shall be deprecated in the future. WG Approval 06/09/2022 (org:Organization)"@en ;
    skos:prefLabel "Has main activity description"@en .

:hasMainClassification a owl:ObjectProperty ;
    rdfs:isDefinedBy :core ;
    skos:prefLabel "Has main classification"@en .

:hasMainFeature a owl:DatatypeProperty ;
    rdfs:isDefinedBy :core ;
    skos:definition "Main features of the procedure and information about where the full rules for the procedure can be found. Additional Information: This information should be given when the procedure is not one of those mentioned in the procurement directives. This can be the case for example for concessions, for social and other specific services, and in case of voluntary publication of procurement procedures below the EU procurement thresholds. (epo:Procedure)"@en ;
    skos:prefLabel "Has main feature"@en .

:hasMandateIdentifier a owl:ObjectProperty ;
    rdfs:isDefinedBy :core ;
    skos:definition "An unique identifier for referencing the direct debit mandate, assigned by the Payee. WG approval 11/07/2024 (epo-inv:PaymentInstructionsInformation -> adms:Identifier (+epo-inv:hasMandateIdentifier))"@en ;
    skos:prefLabel "Has mandate identifier"@en .

:hasManufacturerID a owl:ObjectProperty ;
    rdfs:isDefinedBy :core ;
    skos:definition "The manufacturer's identifier for the item. (epo-cat:Manufacturer -> adms:Identifier (+epo:hasManufacturerID))"@en ;
    skos:prefLabel "Has manufacturer i d"@en .

:hasManufacturerItemID a owl:ObjectProperty ;
    rdfs:isDefinedBy :core ;
    skos:definition "The general identifier assigned to the concept as defined by the Manufacturer. ​ WG approval 16/05/2023 (epo-cat:Item -> adms:Identifier (+epo:hasManufacturerItemID))"@en ;
    skos:prefLabel "Has manufacturer item i d"@en .

:hasMaximumFrameworkAgreementAwardedValue a owl:ObjectProperty ;
    rdfs:isDefinedBy :core ;
    skos:definition "The maximum value which can be spent through all the framework agreements announced in this notice, including options and renewals of contracts. Additional information: The value provided is a threshold value that implicity means that it cannot be exceeded however it may not be reached during the execution of a contract. The Framework Agreements in a CAN are to be traced back and added to provide this value. This corresponds to the BT-118 in eForms. WG Approval 03/12/2019 (epo:NoticeAwardInformation -> epo:MonetaryValue (+epo:hasMaximumFrameworkAgreementAwardedValue))"@en ;
    skos:prefLabel "Has maximum framework agreement awarded value"@en .

:hasMaximumLotSubmissionAllowed a owl:DatatypeProperty ;
    rdfs:isDefinedBy :core ;
    skos:definition "The total number of lots for which one Tenderer can submit Tenders. Additional information: This field is used to complement the SubmissionTerms (which are at the Lot level) for the Procedure level which is covered by the regulation (EU)-2015-1986 (modeled in the TED Standard Forms). WG approval 12/12/2018 (epo:ProcedureTerm)"@en ;
    skos:prefLabel "Has maximum lot submission allowed"@en .

:hasMaximumNumberOfCandidates a owl:DatatypeProperty ;
    rdfs:isDefinedBy :core ;
    skos:definition "Maximum number of candidates to be invited for the second stage of the procedure. WG Approval 22/08/2019 (epo:MultipleStageProcedureTerm)"@en ;
    skos:prefLabel "Has maximum number of candidates"@en .

:hasMaximumNumberOfLotsToBeAwarded a owl:DatatypeProperty ;
    rdfs:isDefinedBy :core ;
    skos:definition "The maximum number of lots for which contract(s) can be awarded to one tenderer. Additional information: This field is used to complement the SubmissionTerms (which are at the Lot level) for the Procedure level which is covered by the regulation (EU)-2015-1986 (modeled in the TED Standard Forms). WG Approval 22/08/2019 (epo:ProcedureTerm)"@en ;
    skos:prefLabel "Has maximum number of lots to be awarded"@en .

:hasMaximumNumberOfRenewals a owl:DatatypeProperty ;
    rdfs:isDefinedBy :core ;
    skos:definition "The maximum number of times the contract can be renewed. Additional Information By renewing, the buyer reserves the right (i.e. not an obligation) to renew the contract (i.e. extend its duration) without a new procurement procedure. For example, a contract may be valid for one year and the buyer may keep a possibility to renew it (e.g. once, twice) for another three months, if he is content with the services he received. PLEASE REVIEW THIS DEFINITION AGAIN WITH THE WORKING GROUP. It was originally taken from eForms. (epo:ContractTerm)"@en ;
    skos:prefLabel "Has maximum number of renewals"@en .

:hasMaximumOrderQuantity a owl:ObjectProperty ;
    rdfs:isDefinedBy :core ;
    skos:definition "The maximum number of orderable units that can be ordered according to details provided in the catalogue line, such as price. (epo-cat:CatalogueLine -> epo:Quantity (+epo-cat:hasMaximumOrderQuantity))"@en ;
    skos:prefLabel "Has maximum order quantity"@en .

:hasMaximumParticipantsNumber a owl:DatatypeProperty ;
    rdfs:isDefinedBy :core ;
    skos:definition "The maximum number of participants in the framework agreement. Additional Information: Maximum number of tenderers who may be awarded a contract within the framework agreement. The number is a positive integer. This corresponds in eForms to BT-113 Framework Maximum Participants Number. WG Approval 2019-02-05 (epo:FrameworkAgreementTerm)"@en ;
    skos:prefLabel "Has maximum participants number"@en .

:hasMaximumShare a owl:DatatypeProperty ;
    rdfs:isDefinedBy :core ;
    skos:definition "The maximum proportion of something to be distributed. Additional Information: In the case of subcontracting the share may refer to the proportion of works, services or supplies being subcontracted. WG Approval 17/09/2019 (epo:SubcontractTerm)"@en ;
    skos:prefLabel "Has maximum share"@en .

:hasMaximumTemperature a owl:ObjectProperty ;
    rdfs:isDefinedBy :core ;
    skos:definition "The highest tolerated temperature. WG approval 18/06/2024 (epo-ful:TemperatureSpecification -> epo:Quantity (+epo-ful:hasMaximumTemperature))"@en ;
    skos:prefLabel "Has maximum temperature"@en .

:hasMediumTenderPerLots a owl:DatatypeProperty ;
    rdfs:isDefinedBy :core ;
    skos:definition "Tenders from medium-sized enterprise. <u>Additional Information:</u> See Commission Recommendation 2003/361/EC. (epo:SubmissionStatisticalInformation)"@en ;
    skos:prefLabel "Has medium tender per lots"@en .

:hasMember a owl:ObjectProperty ;
    rdfs:isDefinedBy :core ;
    skos:prefLabel "Has member"@en .

:hasMinimumNumberOfCandidates a owl:DatatypeProperty ;
    rdfs:isDefinedBy :core ;
    skos:definition "Minimum number of candidates to be invited for the second stage of the procedure. WG Approval 22/08/2019 (epo:MultipleStageProcedureTerm)"@en ;
    skos:prefLabel "Has minimum number of candidates"@en .

:hasMinimumQuantityGuaranteedForDelivery a owl:ObjectProperty ;
    rdfs:isDefinedBy :core ;
    skos:definition "The minimum quantity of an item that is guaranteed by the seller to be delivered. (epo-cat:CatalogueLine -> epo:Quantity (+epo-cat:hasMinimumQuantityGuaranteedForDelivery))"@en ;
    skos:prefLabel "Has minimum quantity guaranteed for delivery"@en .

:hasMinimumShare a owl:DatatypeProperty ;
    rdfs:isDefinedBy :core ;
    skos:definition "The minimum proportion of something to be distributed. Additional Information: In the case of subcontracting the share may refer to the proportion of works, services or supplies being subcontracted. WG Approval 17/09/2019 (epo:SubcontractTerm)"@en ;
    skos:prefLabel "Has minimum share"@en .

:hasMinimumSubcontractorsProposedObligation a owl:DatatypeProperty ;
    rdfs:isDefinedBy :core ;
    skos:definition "The minimum percentage of the contract value that the contractor must subcontract. Additional information: This is used for the competitive procedure described in Title III of Directive 2009/81/EC. WG Approval 09/11/2021 (epo:SubcontractTerm)"@en ;
    skos:prefLabel "Has minimum subcontractors proposed obligation"@en .

:hasMinimumTemperature a owl:ObjectProperty ;
    rdfs:isDefinedBy :core ;
    skos:definition "The lowest tolerated temperature. WG approval 18/06/2024 (epo-ful:TemperatureSpecification -> epo:Quantity (+epo-ful:hasMinimumTemperature))"@en ;
    skos:prefLabel "Has minimum temperature"@en .

:hasModificationJustification a owl:ObjectProperty ;
    rdfs:isDefinedBy :core ;
    skos:definition "Explanation of why a contract was modified. WG Approval 09/11/2021 The codelist to be used is at-voc:modification-justification which is available at http://publications.europa.eu/resource/dataset/modification-justification Additional Information This corresponds in Standard forms to Field VII.2.2.1 and VII.2.2.3 in F20 . This corresponds in eForms to BT-200. (epo-con:ContractModificationInformation -> at-voc:modification-justification (+epo:hasModificationJustification))"@en ;
    skos:prefLabel "Has modification justification"@en .

:hasNationalProcedureRules a owl:DatatypeProperty ;
    rdfs:isDefinedBy :core ;
    skos:definition "The resource identifier where the information about the national rules applicable to the procedure can be found. WG approval 02/05/2024 (epo:ProcedureTerm)"@en ;
    skos:prefLabel "Has national procedure rules"@en .

:hasNationality a owl:ObjectProperty ;
    rdfs:isDefinedBy :core ;
    skos:definition "(person:Person -> at-voc:country (+epo:hasNationality))"@en ;
    skos:prefLabel "Has nationality"@en .

:hasNetAmount a owl:ObjectProperty ;
    rdfs:isDefinedBy :core ;
    skos:prefLabel "Has net amount"@en .

:hasNetMonetaryValue a owl:ObjectProperty ;
    rdfs:isDefinedBy :core ;
    skos:prefLabel "Has net monetary value"@en .

:hasNetQuantity a owl:ObjectProperty ;
    rdfs:isDefinedBy :core ;
    skos:definition "The net quantity of the item that is contained in each consumable unit, excluding any packaging materials. (epo-cat:Item -> epo:Quantity (+epo-cat:hasNetQuantity))"@en ;
    skos:prefLabel "Has net quantity"@en .

:hasNetVolume a owl:ObjectProperty ;
    rdfs:isDefinedBy :core ;
    skos:definition "The amount of space that is required without the packaging. WG approval 18/06/2024 (epo-ful:AbstractContainer -> epo:Quantity (+epo-ful:hasNetVolume))"@en ;
    skos:prefLabel "Has net volume"@en .

:hasNetWeight a owl:ObjectProperty ;
    rdfs:isDefinedBy :core ;
    skos:definition "The total mass of goods without the packaging. WG approval 18/06/2024 (epo-ful:AbstractContainer -> epo:Quantity (+epo-ful:hasNetWeight)) The total mass of goods without the packaging. WG approval 18/06/2024 (epo-ful:Consignment -> epo:Quantity (+epo-ful:hasNetWeight))"@en ;
    skos:prefLabel "Has net weight"@en .

:hasNoNegotiationNecessary a owl:DatatypeProperty ;
    rdfs:isDefinedBy :core ;
    skos:definition "The buyer reserves the right to award the contract on the basis of the initial tenders without any further negotiations. Additional information: See Article 29(4) of Directive 2014/24/EU. (epo:MultipleStageProcedureTerm)"@en ;
    skos:prefLabel "Has no negotiation necessary"@en .

:hasNonAccessibilityCriterionJustification a owl:DatatypeProperty ;
    rdfs:isDefinedBy :core ;
    skos:definition "Reason for not applying accessibility criteria. Additional information: This corresponds in eForma to BT-755 Accessibility Justification. WG Approval 05/03/2019 (epo:StrategicProcurement)"@en ;
    skos:prefLabel "Has non accessibility criterion justification"@en .

:hasNonAwardJustification a owl:ObjectProperty ;
    rdfs:isDefinedBy :core ;
    skos:definition "On hold; Enumeration. (epo:AwardOutcome -> at-voc:non-award-justification (+epo:hasNonAwardJustification))"@en ;
    skos:prefLabel "Has non award justification"@en .

:hasNonAwardedContractNumber a owl:DatatypeProperty ;
    rdfs:isDefinedBy :core ;
    skos:definition "The number the contract would have had if it had been awarded. Additional information: This field is provided to support the data provided in the TED Standard Forms, and it should be discontinued in the future. WG agreement: 06/09/2022 (epo:LotAwardOutcome)"@en ;
    skos:prefLabel "Has non awarded contract number"@en .

:hasNonAwardedContractTitle a owl:DatatypeProperty ;
    rdfs:isDefinedBy :core ;
    skos:definition "The title the contract would have had if it had been awarded. Additional information: This field is provided to support the data provided in the TED Standard Forms, and it should be discontinued in the future. WG agreement: 06/09/2022 (epo:LotAwardOutcome)"@en ;
    skos:prefLabel "Has non awarded contract title"@en .

:hasNonEEAReceivedTenders a owl:DatatypeProperty ;
    rdfs:isDefinedBy :core ;
    skos:definition "The amount of tenders received from economic operators in non-EEA countries. WG Approval 12/12/2019 15:20:36 (epo:SubmissionStatisticalInformation)"@en ;
    skos:prefLabel "Has non e e a received tenders"@en .

:hasNonEUReceivedTenders a owl:DatatypeProperty ;
    rdfs:isDefinedBy :core ;
    skos:definition "The amount of tenders received from economic operators in non-EU countries. (epo:SubmissionStatisticalInformation)"@en ;
    skos:prefLabel "Has non e u received tenders"@en .

:hasNonElectronicSubmissionDescription a owl:DatatypeProperty ;
    rdfs:isDefinedBy :core ;
    skos:definition "Textual explanation of how non-electronic information is to be presented. WG Approval 21/07/2020 (epo:SubmissionTerm)"@en ;
    skos:prefLabel "Has non electronic submission description"@en .

:hasNonElectronicSubmissionJustification a owl:ObjectProperty ;
    rdfs:isDefinedBy :core ;
    skos:definition "Reason for not accepting electronic information. WG Approval 21/07/2020 (epo:SubmissionTerm -> at-voc:communication-justification (+epo:hasNonElectronicSubmissionJustification))"@en ;
    skos:prefLabel "Has non electronic submission justification"@en .

:hasNonPublicationJustification a owl:ObjectProperty ;
    rdfs:isDefinedBy :core ;
    skos:definition "The reason why data is not published. WG Approval 11/06/2020 (epo:NonPublishedInformation -> at-voc:non-publication-justification (+epo:hasNonPublicationJustification))"@en ;
    skos:prefLabel "Has non publication justification"@en .

:hasNoticePublicationNumber a owl:DatatypeProperty ;
    rdfs:isDefinedBy :core ;
    skos:definition "The identifier of the published Notice. Additional information: The format of this identifier is XXXXXXXX-YYYY. WG approval 26/03/2024 (epo:Notice)"@en ;
    skos:prefLabel "Has notice publication number"@en .

:hasNoticeType a owl:ObjectProperty ;
    rdfs:isDefinedBy :core ;
    skos:prefLabel "Has notice type"@en .

:hasNumberOfReviewRequests a owl:DatatypeProperty ;
    rdfs:isDefinedBy :core ;
    skos:definition "The number of requests the buyer received to review any of its decisions. (epo:ReviewRequest)"@en ;
    skos:prefLabel "Has number of review requests"@en .

:hasNumberOfTenderersInvited a owl:DatatypeProperty ;
    rdfs:isDefinedBy :core ;
    skos:definition "Number of economic operators invited to tender. Additional Information This may be used for single-stage procedures or to indicate the number of candidates invited to tender in multi-stage procedures. WG Approval 01/12/2020 (epo:SubmissionStatisticalInformation)"@en ;
    skos:prefLabel "Has number of tenderers invited"@en .

:hasNutsCode a owl:ObjectProperty ;
    rdfs:isDefinedBy :core ;
    skos:prefLabel "Has nuts code"@en .

:hasOJSIssueNumber a owl:DatatypeProperty ;
    rdfs:isDefinedBy :core ;
    skos:definition "The issue identifier of the Supplement to the EU Official Journal. Additional information: The format of this identifier is XX-YYYY. WG approval 26/03/2024 (epo:Notice)"@en ;
    skos:prefLabel "Has o j s issue number"@en .

:hasOJSType a owl:DatatypeProperty ;
    rdfs:isDefinedBy :core ;
    skos:prefLabel "Has o j s type"@en .

:hasOfficialLanguage a owl:ObjectProperty ;
    rdfs:isDefinedBy :core ;
    skos:definition "The language(s) in which the instances of the given concepts are officially available. These linguistic versions are equally legally valid. WG Approval 03/10/2019 (epo:Document -> at-voc:language (+epo:hasOfficialLanguage))"@en ;
    skos:prefLabel "Has official language"@en .

:hasOpeningDateTime a owl:DatatypeProperty ;
    rdfs:isDefinedBy :core ;
    skos:definition "Date and time for the opening of tenders. WG Approval 12/03/2019 (epo:OpeningTerm)"@en ;
    skos:prefLabel "Has opening date time"@en .

:hasOpeningDescription a owl:DatatypeProperty ;
    rdfs:isDefinedBy :core ;
    skos:definition "Further information about the opening of tenders. Additional Information For example, who may participate in the opening and whether any authorization is needed. WG Approval 12/03/2019 (epo:OpeningTerm)"@en ;
    skos:prefLabel "Has opening description"@en .

:hasOpeningURL a owl:DatatypeProperty ;
    rdfs:isDefinedBy :core ;
    skos:definition "The identifier of the address of the Opening of Tenders. WG Approval 09/11/2021 (epo:OpeningTerm)"@en ;
    skos:prefLabel "Has opening u r l"@en .

:hasOptions a owl:DatatypeProperty ;
    rdfs:isDefinedBy :core ;
    skos:definition "The buyer reserves the right (not an obligation) for additional purchases from the contractor (while the contract is valid). (epo:ContractTerm)"@en ;
    skos:prefLabel "Has options"@en .

:hasOptionsDescription a owl:DatatypeProperty ;
    rdfs:isDefinedBy :core ;
    skos:definition "The motivation and details about additional purchases that the buyer may undertake while the contract is valid. WG Approval 09/04/2019 (epo:ContractTerm)"@en ;
    skos:prefLabel "Has options description"@en .

:hasOrderabableUnitFactorRate a owl:ObjectProperty ;
    rdfs:isDefinedBy :core ;
    skos:prefLabel "Has orderabable unit factor rate"@en .

:hasOtherCountriesReceivedTenders a owl:DatatypeProperty ;
    rdfs:isDefinedBy :core ;
    skos:definition "The amount of Tenders received from countries other than that of the Buyer. WG approval 02/05/2024 (epo:SubmissionStatisticalInformation)"@en ;
    skos:prefLabel "Has other countries received tenders"@en .

:hasOutstandingQuantity a owl:ObjectProperty ;
    rdfs:isDefinedBy :core ;
    skos:definition "The Quantity of non-despatched Goods Items. WG approval 05/06/2024 (epo-ful:DespatchLine -> epo:Quantity (+epo-ful:hasOutstandingQuantity))"@en ;
    skos:prefLabel "Has outstanding quantity"@en .

:hasOverallCostAwardCriteriaPonderation a owl:DatatypeProperty ;
    rdfs:isDefinedBy :core ;
    skos:definition "The weighting given to cost. Additional Information: This weighting covers usually all cost criteria against price or quality criteria. (epo:AwardEvaluationTerm)"@en ;
    skos:prefLabel "Has overall cost award criteria ponderation"@en .

:hasOverallPriceAwardCriteriaPonderation a owl:DatatypeProperty ;
    rdfs:isDefinedBy :core ;
    skos:definition "The weighting given to price. Additional Information: This weighting covers usually all price criteria against cost or quality criteria. (epo:AwardEvaluationTerm)"@en ;
    skos:prefLabel "Has overall price award criteria ponderation"@en .

:hasOverallQualityAwardCriteriaPonderation a owl:DatatypeProperty ;
    rdfs:isDefinedBy :core ;
    skos:definition "The weighting given to quality. Additional Information: This weighting covers usually all quality criteria against price or cost criteria. (epo:AwardEvaluationTerm)"@en ;
    skos:prefLabel "Has overall quality award criteria ponderation"@en .

:hasOversupplyQuantity a owl:ObjectProperty ;
    rdfs:isDefinedBy :core ;
    skos:prefLabel "Has oversupply quantity"@en .

:hasParticipationPayment a owl:DatatypeProperty ;
    rdfs:isDefinedBy :core ;
    skos:definition "Details on payments to participants WG Approval 09/11/2021 (epo:DesignContestRegimeTerm)"@en ;
    skos:prefLabel "Has participation payment"@en .

:hasPaymentAccountIdentifier a owl:ObjectProperty ;
    rdfs:isDefinedBy :core ;
    skos:definition "A unique identifier of the financial payment account, at a payment service provider, to which payment should be made. WG approval 11/07/2024 (epo-inv:CreditTransferInformation -> adms:Identifier (+epo-inv:hasPaymentAccountIdentifier))"@en ;
    skos:prefLabel "Has payment account identifier"@en .

:hasPaymentArrangement a owl:DatatypeProperty ;
    rdfs:isDefinedBy :core ;
    skos:definition "Information about financial clauses that will govern some economic aspects of the execution of the contract. Additional Information: These clauses usually refer to financial and payment provisions. This type of information should be structured instead of a free text in order to reuse it an ideal world. Unfortunately this is an information that in the real life no one is willing to provide pro-actively. WG Pending of discussion with eForms (epo:ContractTerm)"@en ;
    skos:prefLabel "Has payment arrangement"@en .

:hasPaymentServiceProviderIdentifier a owl:ObjectProperty ;
    rdfs:isDefinedBy :core ;
    skos:definition "An identifier for the payment service provider where a payment account is located. WG approval 11/07/2024 (epo-inv:CreditTransferInformation -> adms:Identifier (+epo-inv:hasPaymentServiceProviderIdentifier))"@en ;
    skos:prefLabel "Has payment service provider identifier"@en .

:hasPaymentValueDiscrepancyJustification a owl:DatatypeProperty ;
    rdfs:isDefinedBy :core ;
    skos:definition "Justification for the actual value being different to the value in the initial Contract. WG approval 26/03/2024 (epo:ContractLotCompletionInformation)"@en ;
    skos:prefLabel "Has payment value discrepancy justification"@en .

:hasPerformanceConditions a owl:DatatypeProperty ;
    rdfs:isDefinedBy :core ;
    skos:definition "The particular conditions and additional information related to the execution of the contract. Additional Information: For example, specific information about the place of performance, intermediary deliverables, compensation for damages, intellectual property rights. WG approval 15-01-2019 (epo:ContractTerm)"@en ;
    skos:prefLabel "Has performance conditions"@en .

:hasPerformingStaffQualificationInformation a owl:ObjectProperty ;
    rdfs:isDefinedBy :core ;
    skos:definition "Additional information: This relation corresponds in eForms to BT-79. (epo:ProcurementCriterion -> at-voc:requirement-stage (+epo:hasPerformingStaffQualificationInformation))"@en ;
    skos:prefLabel "Has performing staff qualification information"@en .

:hasPlaceOfPerformanceAdditionalInformation a owl:DatatypeProperty ;
    rdfs:isDefinedBy :core ;
    skos:definition "Further details on the location of the execution of the contract. WG Approval 30/07/2019 (epo:ContractTerm)"@en ;
    skos:prefLabel "Has place of performance additional information"@en .

:hasPlannedDuration a owl:ObjectProperty ;
    rdfs:isDefinedBy :core ;
    skos:prefLabel "Has planned duration"@en .

:hasPlannedPeriod a owl:ObjectProperty ;
    rdfs:isDefinedBy :core ;
    skos:prefLabel "Has planned period"@en .

:hasPreferredLanguageForProcurementDocument a owl:ObjectProperty ;
    rdfs:isDefinedBy :core ;
    skos:prefLabel "Has preferred language for procurement document"@en .

:hasPrepaidAmount a owl:ObjectProperty ;
    rdfs:isDefinedBy :core ;
    skos:prefLabel "Has prepaid amount"@en .

:hasPriceValidity a owl:ObjectProperty ;
    rdfs:isDefinedBy :core ;
    skos:prefLabel "Has price validity"@en .

:hasPrimaryContactPoint a owl:ObjectProperty ;
    rdfs:isDefinedBy :core ;
    skos:prefLabel "Has primary contact point"@en .

:hasPrizeRank a owl:DatatypeProperty ;
    rdfs:isDefinedBy :core ;
    skos:definition "The position of the prize (e.g. first place, second place) in a design contest list of prizes. WG Approval 29/08/2019 (epo:Prize)"@en ;
    skos:prefLabel "Has prize rank"@en .

:hasPrizeValue a owl:ObjectProperty ;
    rdfs:isDefinedBy :core ;
    skos:definition "The monetary value of a prize, if any, for the winner (or runners-up) of the design contest. Additional Information: This corresponds to BT-644 in eForms. WG Approval 29/08/2019 (epo:Prize -> epo:MonetaryValue (+epo:hasPrizeValue))"@en ;
    skos:prefLabel "Has prize value"@en .

:hasProcedureType a owl:ObjectProperty ;
    rdfs:isDefinedBy :core ;
    skos:definition "Identification of the Procedure used. WG Approval 09/06/2020 (epo:Procedure -> at-voc:procurement-procedure-type (+epo:hasProcedureType))"@en ;
    skos:prefLabel "Has procedure type"@en .

:hasProcurementDocumentChangeDate a owl:DatatypeProperty ;
    rdfs:isDefinedBy :core ;
    skos:definition "The date and time of the change. Additional information: This corresponds in eForms to BT-719 Change Procurement Documents Date WG Approval 5/11/2019 (epo:ChangeInformation)"@en ;
    skos:prefLabel "Has procurement document change date"@en .

:hasProcurementHighestReceivedTenderValue a owl:ObjectProperty ;
    rdfs:isDefinedBy :core ;
    skos:definition "The highest received tender value for the procurement. Additional Information: This corresponds to section II.1.7.3. according to Regulation (EU) 2015/1986. (epo:NoticeAwardInformation -> epo:MonetaryValue (+epo:hasProcurementHighestReceivedTenderValue))"@en ;
    skos:prefLabel "Has procurement highest received tender value"@en .

:hasProcurementLowestReceivedTenderValue a owl:ObjectProperty ;
    rdfs:isDefinedBy :core ;
    skos:definition "The lowest received tender value for the procurement. Additional Information: This corresponds to section II.1.7.2. according to Regulation (EU) 2015/1986. (epo:NoticeAwardInformation -> epo:MonetaryValue (+epo:hasProcurementLowestReceivedTenderValue))"@en ;
    skos:prefLabel "Has procurement lowest received tender value"@en .

:hasProcurementScopeDividedIntoLot a owl:ObjectProperty ;
    rdfs:isDefinedBy :core ;
    skos:prefLabel "Has procurement scope divided into lot"@en .

:hasPublicAccessURL a owl:DatatypeProperty ;
    rdfs:isDefinedBy :core ;
    skos:definition "Web page where the procurement documents can be downloaded. Additional Information: This corresponds in the eForms to BT-15 Documents URL. WG Approval 09/03/2021 (epo:AccessTerm)"@en ;
    skos:prefLabel "Has public access u r l"@en .

:hasPublicationDate a owl:DatatypeProperty ;
    rdfs:isDefinedBy :core ;
    skos:definition "Date of formal public issuance of the document. WG approval 20/06/2023 (epo:Document)"@en ;
    skos:prefLabel "Has publication date"@en .

:hasPurpose a owl:ObjectProperty ;
    rdfs:isDefinedBy :core ;
    skos:definition "Relation indicating the Purpose of a concept. (epo:ProcurementObject -> epo:Purpose (+epo:hasPurpose))"@en ;
    skos:prefLabel "Has purpose"@en .

:hasQualificationCondition a owl:DatatypeProperty ;
    rdfs:isDefinedBy :core ;
    skos:definition "Requirements to be fulfilled by tenders in view of their qualification. WG approval 02/05/2024 (epo:QualificationCriteriaSummary)"@en ;
    skos:prefLabel "Has qualification condition"@en .

:hasQualificationSystemDuration a owl:ObjectProperty ;
    rdfs:isDefinedBy :core ;
    skos:prefLabel "Has qualification system duration"@en .

:hasQualificationSystemRenewalDescription a owl:DatatypeProperty ;
    rdfs:isDefinedBy :core ;
    skos:definition "Explanation of how a Qualification System is re-established. Additional information: A Qualification System qualifies an economic operator to take part in a tendering process. Usually, in such cases the economic operator passes the Exclusion Grounds and Selection Criteria. WG approval 26/03/2024 (epo:MultipleStageProcedureTerm)"@en ;
    skos:prefLabel "Has qualification system renewal description"@en .

:hasQualifiedValue a owl:ObjectProperty ;
    rdfs:isDefinedBy :core ;
    skos:definition "Qualified value of the property, which is defined in a classification scheme. Additional Information: For example, the (0173-1#02-AAA026#007) drilling diameter of an item has value of 12 inches. WG approval 28/07/2022 (epo-cat:ItemProperty -> epo:Quantity (+epo-cat:hasQualifiedValue))"@en ;
    skos:prefLabel "Has qualified value"@en .

:hasQuantity a owl:ObjectProperty ;
    rdfs:isDefinedBy :core ;
    skos:prefLabel "Has quantity"@en .

:hasQuantityThreshold a owl:ObjectProperty ;
    rdfs:isDefinedBy :core ;
    skos:prefLabel "Has quantity threshold"@en .

:hasQuantityValue a owl:DatatypeProperty ;
    rdfs:isDefinedBy :core ;
    skos:definition "The numeric value of the quantity, including decimals. (epo:Quantity)"@en ;
    skos:prefLabel "Has quantity value"@en .

:hasReceiptDeadline a owl:DatatypeProperty ;
    rdfs:isDefinedBy :core ;
    skos:definition "The time limit for receiving submissions. Additional Information This is the deadline by which the buyer must receive submissions (e.g. tenders, requests to participate, clarifications, etc.) and is not the time at which the information is submitted by the economic operator. This attribute should be used for standard forms mappings. WG Approval 21/07/2020 (epo:SubmissionTerm)"@en ;
    skos:prefLabel "Has receipt deadline"@en .

:hasReceiptExpressionDeadline a owl:DatatypeProperty ;
    rdfs:isDefinedBy :core ;
    skos:definition "Time limit for receipt of expressions of interest. Pending of review by the WG (epo:SubmissionTerm)"@en ;
    skos:prefLabel "Has receipt expression deadline"@en .

:hasReceiptParticipationRequestDeadline a owl:DatatypeProperty ;
    rdfs:isDefinedBy :core ;
    skos:definition "The time limit until which requests to participate can be received. WG approval 02/05/2024 (epo:SubmissionTerm)"@en ;
    skos:prefLabel "Has receipt participation request deadline"@en .

:hasReceiptPreliminaryMarketConsultationDeadline a owl:DatatypeProperty ;
    rdfs:isDefinedBy :core ;
    skos:definition "The time limit until which answers to the Preliminary Market Consultation can be received. WG approval 02/05/2024 (epo:SubmissionTerm)"@en ;
    skos:prefLabel "Has receipt preliminary market consultation deadline"@en .

:hasReceiptTenderDeadline a owl:DatatypeProperty ;
    rdfs:isDefinedBy :core ;
    skos:definition "The time limit until which the Tenders can be received. WG approval 02/05/2024 (epo:SubmissionTerm)"@en ;
    skos:prefLabel "Has receipt tender deadline"@en .

:hasReceivedMicroTenders a owl:DatatypeProperty ;
    rdfs:isDefinedBy :core ;
    skos:definition "The amount of tenders received from a micro enterprise. <u>Additional Information:</u> See Commission Recommendation 2003/361/EC. (epo:SubmissionStatisticalInformation)"@en ;
    skos:prefLabel "Has received micro tenders"@en .

:hasReceivedParticipationRequests a owl:DatatypeProperty ;
    rdfs:isDefinedBy :core ;
    skos:definition "The amount of applications to participate from economic operators. WG Approval 12/12/2019 (epo:SubmissionStatisticalInformation)"@en ;
    skos:prefLabel "Has received participation requests"@en .

:hasReceivedQuantity a owl:ObjectProperty ;
    rdfs:isDefinedBy :core ;
    skos:prefLabel "Has received quantity"@en .

:hasReceivedSmallTenders a owl:DatatypeProperty ;
    rdfs:isDefinedBy :core ;
    skos:definition "Tenders from small enterprise. <u>Additional Information:</u> See Commission Recommendation 2003/361/EC. (epo:SubmissionStatisticalInformation)"@en ;
    skos:prefLabel "Has received small tenders"@en .

:hasReceivedSubmissionType a owl:ObjectProperty ;
    rdfs:isDefinedBy :core ;
    skos:prefLabel "Has received submission type"@en .

:hasReceivedTenders a owl:DatatypeProperty ;
    rdfs:isDefinedBy :core ;
    skos:definition "The total amount of tenders received. WG Approval 12/12/2019 (epo:SubmissionStatisticalInformation)"@en ;
    skos:prefLabel "Has received tenders"@en .

:hasReceptionDate a owl:DatatypeProperty ;
    rdfs:isDefinedBy :core ;
    skos:definition "Notes: Date when a record is acknowledged by an organisation. WG Approval 12/05/2020 (epo:Document)"@en ;
    skos:prefLabel "Has reception date"@en .

:hasRecurrenceDescription a owl:DatatypeProperty ;
    rdfs:isDefinedBy :core ;
    skos:definition "Any additional information about the recurrence of the Procurement. Additional Information: For example estimated timing of the Procedure. This corresponds in eForms to BT-95 Recurrence Description. (WG approval 2019-01-16) (epo:ProcurementObject)"@en ;
    skos:prefLabel "Has recurrence description"@en .

:hasReferenceURI a owl:DatatypeProperty ;
    rdfs:isDefinedBy :core ;
    skos:definition "A reference to where the label specification (norms, expectations, standards and policies) can be found. WG approval 26/07/2022 (epo:CertificationLabel)"@en ;
    skos:prefLabel "Has reference u r i"@en .

:hasRegistrationCountry a owl:ObjectProperty ;
    rdfs:isDefinedBy :core ;
    skos:prefLabel "Has registration country"@en .

:hasRejectedQuantity a owl:ObjectProperty ;
    rdfs:isDefinedBy :core ;
    skos:prefLabel "Has rejected quantity"@en .

:hasRemedyValue a owl:ObjectProperty ;
    rdfs:isDefinedBy :core ;
    skos:definition "Additional information: This relation corresponds in eForms to BT-793 Review Remedy Value. (epo:ReviewDecision -> epo:MonetaryValue (+epo:hasRemedyValue))"@en ;
    skos:prefLabel "Has remedy value"@en .

:hasRenewalDescription a owl:DatatypeProperty ;
    rdfs:isDefinedBy :core ;
    skos:definition "Any other information about the renewal(s). WG approval 16/04/2019 (epo:ContractTerm)"@en ;
    skos:prefLabel "Has renewal description"@en .

:hasRequestDate a owl:DatatypeProperty ;
    rdfs:isDefinedBy :core ;
    skos:definition "The date when the review request was submitted. Additional information: This attribute corresponds to the BT-787 Review Date in eForms. (epo:ReviewRequest)"@en ;
    skos:prefLabel "Has request date"@en .

:hasReservedExecution a owl:ObjectProperty ;
    rdfs:isDefinedBy :core ;
    skos:prefLabel "Has reserved execution"@en .

:hasReservedProcurement a owl:ObjectProperty ;
    rdfs:isDefinedBy :core ;
    skos:definition "Explanation as to whether a procurement may be reserved for the participation of certain types of organisation. Additional information: This property corresponds in eForms to the BT-71 WG Approval 09/11/2021 (epo:ParticipationCondition -> at-voc:reserved-procurement (+epo:hasReservedProcurement)) Explanation as to whether a procurement may be reserved for the participation of certain types of organisation. Additional information: This property corresponds in eForms to the BT-71 WG Approval 09/11/2021 (epo:ParticipationConditionsSummary -> at-voc:reserved-procurement (+epo:hasReservedProcurement))"@en ;
    skos:prefLabel "Has reserved procurement"@en .

:hasRestrictedAccessURL a owl:DatatypeProperty ;
    rdfs:isDefinedBy :core ;
    skos:definition "The internet address with information on accessing the restricted (part of the) procurement document. Additional Information: This corresponds in eForms to BT-615 Documents Restricted URL. (epo:AccessTerm)"@en ;
    skos:prefLabel "Has restricted access u r l"@en .

:hasReviewBodyType a owl:ObjectProperty ;
    rdfs:isDefinedBy :core ;
    skos:prefLabel "Has review body type"@en .

:hasReviewDeadline a owl:DatatypeProperty ;
    rdfs:isDefinedBy :core ;
    skos:definition "The time limit for review procedures. WG Approval 09/11/2021 (epo:ReviewTerm)"@en ;
    skos:prefLabel "Has review deadline"@en .

:hasReviewDeadlineInformation a owl:DatatypeProperty ;
    rdfs:isDefinedBy :core ;
    skos:definition "The description of the time limits for review procedures. WG Approval 01/10/2019 (epo:ReviewTerm)"@en ;
    skos:prefLabel "Has review deadline information"@en .

:hasReviewDecisionType a owl:ObjectProperty ;
    rdfs:isDefinedBy :core ;
    skos:definition "Additional information: This relation corresponds in eForms to BT-790 Review Decision Type. (epo:ReviewDecision -> at-voc:review-decision-type (+epo:hasReviewDecisionType))"@en ;
    skos:prefLabel "Has review decision type"@en .

:hasReviewIrregularityCount a owl:DatatypeProperty ;
    rdfs:isDefinedBy :core ;
    skos:definition "The number of requests for a given irregularity. Additional information: This attribute corresponds in eForms to BT-635 Buyer Review Requests Count. (epo:ReviewIrregularitySummary)"@en ;
    skos:prefLabel "Has review irregularity count"@en .

:hasReviewIrregularitySummary a owl:ObjectProperty ;
    rdfs:isDefinedBy :core ;
    skos:definition "Additional information: This relation corresponds in eForms to BG-613 Buyer Review Requests (epo:ReviewRequestSummary -> epo:ReviewIrregularitySummary (+epo:hasReviewIrregularitySummary))"@en ;
    skos:prefLabel "Has review irregularity summary"@en .

:hasReviewProcedure a owl:DatatypeProperty ;
    rdfs:isDefinedBy :core ;
    skos:definition "The description of the method used to request the verification that the procedure has been carried out correctly. WG Approval 09/11/2021 (epo:ReviewTerm)"@en ;
    skos:prefLabel "Has review procedure"@en .

:hasReviewRequestFee a owl:ObjectProperty ;
    rdfs:isDefinedBy :core ;
    skos:definition "Additional information: This relation corresponds in eForms to BT-795 Review Request Fee. (epo:ReviewRequest -> epo:MonetaryValue (+epo:hasReviewRequestFee))"@en ;
    skos:prefLabel "Has review request fee"@en .

:hasReviewURL a owl:DatatypeProperty ;
    rdfs:isDefinedBy :core ;
    skos:definition "The internet address of the documents concerning the review instance. Additional information: This attribute corresponds in eForms to BT-794 Review URL. (epo:ReviewObject)"@en ;
    skos:prefLabel "Has review u r l"@en .

:hasRoundingAmount a owl:ObjectProperty ;
    rdfs:isDefinedBy :core ;
    skos:prefLabel "Has rounding amount"@en .

:hasSMEReceivedTenders a owl:DatatypeProperty ;
    rdfs:isDefinedBy :core ;
    skos:definition "The amount of tenders received from micro, small and medium-sized enterprises. <u>Additional Information:</u> See Commission Recommendation 2003/361/EC. The ReceivedSMETenderLots is used when the size of the company is not exactly knokn. WG Approval 05/03/2020 (epo:SubmissionStatisticalInformation)"@en ;
    skos:prefLabel "Has s m e received tenders"@en .

:hasSMEReceivedTendersExcludingSubcontractors a owl:DatatypeProperty ;
    rdfs:isDefinedBy :core ;
    skos:prefLabel "Has s m e received tenders excluding subcontractors"@en .

:hasScheme a owl:DatatypeProperty ;
    rdfs:isDefinedBy :core ;
    skos:definition "The name of the identification scheme. (adms:Identifier)"@en ;
    skos:prefLabel "Has scheme"@en .

:hasSchemeVersion a owl:DatatypeProperty ;
    rdfs:isDefinedBy :core ;
    skos:definition "The version of the identification scheme. (adms:Identifier)"@en ;
    skos:prefLabel "Has scheme version"@en .

:hasSelectionCriteriaStatedInProcurementDocuments a owl:DatatypeProperty ;
    rdfs:isDefinedBy :core ;
    skos:definition "The Selection Criteria are present in the Procurement Documents. WG approval 02/05/2024 (epo:SelectionCriteriaSummary)"@en ;
    skos:prefLabel "Has selection criteria stated in procurement documents"@en .

:hasSelectionCriteriaUsage a owl:ObjectProperty ;
    rdfs:isDefinedBy :core ;
    skos:definition "Additional Information: This corresponds in eForms to BT-748 Selection Criteria Used. (epo:SelectionCriterion -> at-voc:usage (+epo:hasSelectionCriteriaUsage))"@en ;
    skos:prefLabel "Has selection criteria usage"@en .

:hasSelectionCriterionType a owl:ObjectProperty ;
    rdfs:isDefinedBy :core ;
    skos:definition "The classification of the selection criteria. Additional Information: This corresponds in eForms to BT-747 Selection Criteria Type. WG Approval 09/11/2021 (epo:SelectionCriterion -> at-voc:selection-criterion (+epo:hasSelectionCriterionType))"@en ;
    skos:prefLabel "Has selection criterion type"@en .

:hasSellerItemID a owl:ObjectProperty ;
    rdfs:isDefinedBy :core ;
    skos:definition "The general identifier assigned to the concept as defined by the Seller.​ WG approval 16/05/2023 (epo-cat:Item -> adms:Identifier (+epo:hasSellerItemID))"@en ;
    skos:prefLabel "Has seller item i d"@en .

:hasSellerOrderID a owl:ObjectProperty ;
    rdfs:isDefinedBy :core ;
    skos:definition "The identifier of the Order given by the Seller. Additional Information: This identifier is different than the identifier of the Order given by the Buyer and it is useful for internal purposes. WG approval 12/10/2023 (epo-ord:Order -> adms:Identifier (+epo-ord:hasSellerOrderID))"@en ;
    skos:prefLabel "Has seller order i d"@en .

:hasSerialID a owl:ObjectProperty ;
    rdfs:isDefinedBy :core ;
    skos:definition "The identifier assigned to the specific instance of the produced concept. WG Approval 16/05/2023 (epo-cat:Item -> adms:Identifier (+epo:hasSerialID))"@en ;
    skos:prefLabel "Has serial i d"@en .

:hasServiceReservedToParticularProfession a owl:DatatypeProperty ;
    rdfs:isDefinedBy :core ;
    skos:definition "Execution of the contract is limited to a particular profession. WG approval 02/05/2024 (epo:ProfessionalSuitabilitySummary)"@en ;
    skos:prefLabel "Has service reserved to particular profession"@en .

:hasShortQuantity a owl:ObjectProperty ;
    rdfs:isDefinedBy :core ;
    skos:prefLabel "Has short quantity"@en .

:hasStartDate a owl:ObjectProperty ;
    rdfs:isDefinedBy :core ;
    skos:prefLabel "Has start date"@en .

:hasStrategicProcurementDescription a owl:DatatypeProperty ;
    rdfs:isDefinedBy :core ;
    skos:definition "Self-explanatory text about a concept. (epo:StrategicProcurement)"@en ;
    skos:prefLabel "Has strategic procurement description"@en .

:hasSubcontracting a owl:ObjectProperty ;
    rdfs:isDefinedBy :core ;
    skos:prefLabel "Has subcontracting"@en .

:hasSubcontractingEstimatedValue a owl:ObjectProperty ;
    rdfs:isDefinedBy :core ;
    skos:definition "The estimated value of a single subcontract. This relates to BT-553 in eForms. WG Approval 01/09/2020 (epo:SubcontractingEstimate -> epo:MonetaryValue (+epo:hasSubcontractingEstimatedValue))"@en ;
    skos:prefLabel "Has subcontracting estimated value"@en .

:hasSubcontractingInvolved a owl:DatatypeProperty ;
    rdfs:isDefinedBy :core ;
    skos:definition "List of Subcontractors and the subject matter they cover are required. Additional Information: The tenderer will ned to supply this information in the tender. WG Approval 28/02/2019 (epo:SubcontractTerm)"@en ;
    skos:prefLabel "Has subcontracting involved"@en .

:hasSubcontractingObligation a owl:ObjectProperty ;
    rdfs:isDefinedBy :core ;
    skos:definition "The requirement the tender must meet with regard to subcontracting parts of the contract. WG Approval 09/11/2021 (epo:SubcontractTerm -> at-voc:subcontracting-obligation (+epo:hasSubcontractingObligation))"@en ;
    skos:prefLabel "Has subcontracting obligation"@en .

:hasSubcontractor a owl:ObjectProperty ;
    rdfs:isDefinedBy :core ;
    skos:prefLabel "Has subcontractor"@en .

:hasSubcontractorsProposedAboveObligation a owl:DatatypeProperty ;
    rdfs:isDefinedBy :core ;
    skos:definition "The maximum percentage of the contract value that the contractor must subcontract. Additional information: This is used for the competitive procedure described in Title III of Directive 2009/81/EC. WG Approval 09/11/2021 (epo:SubcontractTerm)"@en ;
    skos:prefLabel "Has subcontractors proposed above obligation"@en .

:hasSubjectMatter a owl:DatatypeProperty ;
    rdfs:isDefinedBy :core ;
    skos:definition "Description of the share of the contract that is to be subcontracted. Additional infromation: This can be an aggregate of several subcontracts. WG Approval 09/11/2021 (epo:SubcontractingEstimate)"@en ;
    skos:prefLabel "Has subject matter"@en .

:hasSubmissionURL a owl:DatatypeProperty ;
    rdfs:isDefinedBy :core ;
    skos:definition "Additional Information: This corresponds to the eForms BT-18 Submission URL. This corresponds in eForms to BT-509 Organisation eDelivery Gateway. (epo:SubmissionTerm)"@en ;
    skos:prefLabel "Has submission u r l"@en .

:hasSuccessiveReduction a owl:DatatypeProperty ;
    rdfs:isDefinedBy :core ;
    skos:definition "The number of solutions or tenders will be reduced in iterative evaluations for multiple staged procedures. Additional information: This refers to multiple-stage procedures (included two-stage procedures, at least). Open Procedures can be seen as one-stage procedures. WG Approval 22/08/2019 (epo:MultipleStageProcedureTerm)"@en ;
    skos:prefLabel "Has successive reduction"@en .

:hasTaxIdentifier a owl:ObjectProperty ;
    rdfs:isDefinedBy :core ;
    skos:prefLabel "Has tax identifier"@en .

:hasTaxInformation a owl:ObjectProperty ;
    rdfs:isDefinedBy :core ;
    skos:prefLabel "Has tax information"@en .

:hasTenderSubcontractingInformation a owl:ObjectProperty ;
    rdfs:isDefinedBy :core ;
    skos:definition "The information about subcontracting that must be indicated in the tender. WG Approval 10/10/2019 (epo:SubmissionTerm -> at-voc:subcontracting-indication (+epo:hasTenderSubcontractingInformation))"@en ;
    skos:prefLabel "Has tender subcontracting information"@en .

:hasTenderValidityDuration a owl:ObjectProperty ;
    rdfs:isDefinedBy :core ;
    skos:prefLabel "Has tender validity duration"@en .

:hasTenderValidityPeriod a owl:ObjectProperty ;
    rdfs:isDefinedBy :core ;
    skos:definition "The relation indicating until when a tender instance is applicable. (epo:SubmissionTerm -> epo:Period (+epo:hasTenderValidityPeriod))"@en ;
    skos:prefLabel "Has tender validity period"@en .

:hasThresholdType a owl:ObjectProperty ;
    rdfs:isDefinedBy :core ;
    skos:definition "The method to interpret the threshold value as minimum or a maximum. WG Approval 17/09/2019 (cccev:Constraint -> at-voc:number-threshold (+epo:hasThresholdType))"@en ;
    skos:prefLabel "Has threshold type"@en .

:hasThresholdValue a owl:DatatypeProperty ;
    rdfs:isDefinedBy :core ;
    skos:definition "The cut-off level for a given concept. Additional Information: This value is given as e.g. a minimum score, a maximum number of tenders with the highest score passing (see codelist at-voc:number-threshold). (cccev:Constraint)"@en ;
    skos:prefLabel "Has threshold value"@en .

:hasTimePeriod a owl:ObjectProperty ;
    rdfs:isDefinedBy :core ;
    skos:definition "(epo:Period -> at-voc:timeperiod (+epo:hasTimePeriod))"@en ;
    skos:prefLabel "Has time period"@en .

:hasTotalAccountingCurrencyTaxAmount a owl:ObjectProperty ;
    rdfs:isDefinedBy :core ;
    skos:prefLabel "Has total accounting currency tax amount"@en .

:hasTotalAllowanceAmount a owl:ObjectProperty ;
    rdfs:isDefinedBy :core ;
    skos:prefLabel "Has total allowance amount"@en .

:hasTotalAwardedValue a owl:ObjectProperty ;
    rdfs:isDefinedBy :core ;
    skos:definition "The awarded value of all lots announced in this notice, including options and renewals. Additional information: The values of the individual Lots awarded under a framework agreement and mentioned in this notice are included. The values of the individual lots announced in a CAN are to be traced back and added to provide this value. This corresponds to the BT-161 in eForms. WG Approval 03/12/2019 (epo:NoticeAwardInformation -> epo:MonetaryValue (+epo:hasTotalAwardedValue))"@en ;
    skos:prefLabel "Has total awarded value"@en .

:hasTotalChargeAmount a owl:ObjectProperty ;
    rdfs:isDefinedBy :core ;
    skos:prefLabel "Has total charge amount"@en .

:hasTotalGoodsItemQuantity a owl:ObjectProperty ;
    rdfs:isDefinedBy :core ;
    skos:definition "Relation indicating the number of the Goods Items. WG approval 25/06/2024 (epo-ful:AbstractContainer -> epo:Quantity (+epo-ful:hasTotalGoodsItemQuantity)) Relation indicating the number of the Goods Items. WG approval 25/06/2024 (epo-ful:Consignment -> epo:Quantity (+epo-ful:hasTotalGoodsItemQuantity))"@en ;
    skos:prefLabel "Has total goods item quantity"@en .

:hasTotalLineAmount a owl:ObjectProperty ;
    rdfs:isDefinedBy :core ;
    skos:prefLabel "Has total line amount"@en .

:hasTotalNumberOfComplainants a owl:DatatypeProperty ;
    rdfs:isDefinedBy :core ;
    skos:definition "The number of economic operators that requested the buyer to review any of its decisions (e.g. the technical specifications, award decision), as set out in Art. 1(5) of Directive 89/665/EEC and Directive 92/13/EEC. Additional information: This attribute corresponds in eForms to BT-712 Buyer Review Complainants WG Approval 11/04/2019 (epo:ReviewRequestSummary)"@en ;
    skos:prefLabel "Has total number of complainants"@en .

:hasTotalQuantity a owl:ObjectProperty ;
    rdfs:isDefinedBy :core ;
    skos:definition "The number of units required. Additional Information: The quantity needs to go along with the unit. (epo:Purpose -> epo:Quantity (+epo:hasTotalQuantity))"@en ;
    skos:prefLabel "Has total quantity"@en .

:hasTotalTaxAmount a owl:ObjectProperty ;
    rdfs:isDefinedBy :core ;
    skos:prefLabel "Has total tax amount"@en .

:hasTotalTaxExclusiveAmount a owl:ObjectProperty ;
    rdfs:isDefinedBy :core ;
    skos:prefLabel "Has total tax exclusive amount"@en .

:hasTotalTaxInclusiveAmount a owl:ObjectProperty ;
    rdfs:isDefinedBy :core ;
    skos:prefLabel "Has total tax inclusive amount"@en .

:hasTotalValue a owl:ObjectProperty ;
    rdfs:isDefinedBy :core ;
    skos:prefLabel "Has total value"@en .

:hasTotalVehicles a owl:DatatypeProperty ;
    rdfs:isDefinedBy :core ;
    skos:definition "The number of all vehicles (regardless of whether clean or not) that have either been purchased, leased, rented, hired-purchased or their use has been contractually committed to for the provision of a purchased service. Additional Information: In the European Union, the legal requirements and scope for the provision of these vehicles or services are covered by Directive 2009/33/EC. WG Approval 28/07/2020 (epo:VehicleInformation)"@en ;
    skos:prefLabel "Has total vehicles"@en .

:hasTraceID a owl:ObjectProperty ;
    rdfs:isDefinedBy :core ;
    skos:definition "The identifier used for tracking the Goods Item. Additional information: An example is the EPC number used in RFID. WG approval 21/09/2023 (epo-ful:GoodsItem -> adms:Identifier (+epo-ful:hasTraceID))"@en ;
    skos:prefLabel "Has trace i d"@en .

:hasTrackingID a owl:ObjectProperty ;
    rdfs:isDefinedBy :core ;
    skos:prefLabel "Has tracking i d"@en .

:hasTransportHandlingUnitQuantity a owl:ObjectProperty ;
    rdfs:isDefinedBy :core ;
    skos:definition "Relation indicating the number of the Transport Handling Unit. WG approval 25/06/2024 (epo-ful:Consignment -> epo:Quantity (+epo-ful:hasTransportHandlingUnitQuantity))"@en ;
    skos:prefLabel "Has transport handling unit quantity"@en .

:hasURL a owl:DatatypeProperty ;
    rdfs:isDefinedBy :core ;
    skos:definition "The identifier of a resource. Additional Information For example: 1. The URL of the system from where to access the procurement documents; 2. The URL of the system for the submission of tender documents; 3. The URL of the system from where to download a tool to communicate with the Buyer; 4. The URL of the system used by a Technique to allow Economic Operators to exchange information with the Buyer (e.g. eAuction and DPS Systems) 5. The URL of the system used to exchange information between Buyer and EO for questions and clarifications; WG Approval 30/09/2019 (cccev:Evidence) The identifier of a resource. Additional Information For example: 1. The URL of the system from where to access the procurement documents; 2. The URL of the system for the submission of tender documents; 3. The URL of the system from where to download a tool to communicate with the Buyer; 4. The URL of the system used by a Technique to allow Economic Operators to exchange information with the Buyer (e.g. eAuction and DPS Systems) 5. The URL of the system used to exchange information between Buyer and EO for questions and clarifications; WG Approval 30/09/2019 (epo:Fund)"@en ;
    skos:prefLabel "Has u r l"@en .

:hasUUID a owl:ObjectProperty ;
    rdfs:isDefinedBy :core ;
    skos:definition "A universally unique identifier for an instance of this document. WG Approval 12/05/2020 (epo-cat:CatalogueResponseLine -> adms:Identifier (+epo:hasUUID)) A universally unique identifier for an instance of this document. WG Approval 12/05/2020 (epo:Document -> adms:Identifier (+epo:hasUUID))"@en ;
    skos:prefLabel "Has u u i d"@en .

:hasUnitCode a owl:ObjectProperty ;
    rdfs:isDefinedBy :core ;
    skos:prefLabel "Has unit code"@en .

:hasUnitDescription a owl:DatatypeProperty ;
    rdfs:isDefinedBy :core ;
    skos:definition "A narrative explanation defining the units of items being counted Additional information: This could be for example individual items or pack or two. WG Approval 09/11/2021 (epo:Quantity)"@en ;
    skos:prefLabel "Has unit description"@en .

:hasUnofficialLanguage a owl:ObjectProperty ;
    rdfs:isDefinedBy :core ;
    skos:definition "The language translation(s) in which the instances of the given concepts are available. These linguistic versions are not an official translation, they are provided only for information. WG Approval 03/10/2019 (epo:Document -> at-voc:language (+epo:hasUnofficialLanguage))"@en ;
    skos:prefLabel "Has unofficial language"@en .

:hasUnverifiedTenders a owl:DatatypeProperty ;
    rdfs:isDefinedBy :core ;
    skos:definition "Offers received for which it has not been verified if they are admissible or inadmissible (e.g. because award criteria have been evaluated for all tenders and admissibility is checked only for the winning tender). WG Approval 28/07/2020 (epo:SubmissionStatisticalInformation)"@en ;
    skos:prefLabel "Has unverified tenders"@en .

:hasUsage a owl:ObjectProperty ;
    rdfs:isDefinedBy :core ;
    skos:definition "The codelist to be used is at-voc:usage which is available at http://publications.europa.eu/resource/dataset/usage (epo:Technique -> at-voc:usage (+epo:hasUsage))"@en ;
    skos:prefLabel "Has usage"@en .

:hasValidityPeriod a owl:ObjectProperty ;
    rdfs:isDefinedBy :core ;
    skos:definition "The relation indicating until when a given instance of a concept is applicable. WG approval 30/05/2023 (cccev:Evidence -> epo:Period (+epo:hasValidityPeriod)) The relation indicating until when a given instance of a concept is applicable. WG approval 30/05/2023 (epo-cat:Catalogue -> epo:Period (+epo:hasValidityPeriod)) The relation indicating until when a given instance of a concept is applicable. WG approval 30/05/2023 (epo:Technique -> epo:Period (+epo:hasValidityPeriod))"@en ;
    skos:prefLabel "Has validity period"@en .

:hasVariantPermission a owl:ObjectProperty ;
    rdfs:isDefinedBy :core ;
    skos:definition "The obligation or possibility for tenderers to submit variants or not. Additional Information: Variants are alternative ways to fulfil the buyer's needs as opposed to solutions indicated in the procurement documents. eForms: Whether tenderers are required, allowed or forbidden to submit tenders which fulfil the buyer's needs differently than as proposed in the procurement documents. Additional Information: Further conditions for submitting variant tenders are in the procurement documents. (epo:SubmissionTerm -> at-voc:permission (+epo:hasVariantPermission))"@en ;
    skos:prefLabel "Has variant permission"@en .

:hasVehicleID a owl:ObjectProperty ;
    rdfs:isDefinedBy :core ;
    skos:definition "The identifier of the Transport Means. WG approval 25/06/2024 (epo-ful:TransportMeans -> adms:Identifier (+epo-ful:hasVehicleID))"@en ;
    skos:prefLabel "Has vehicle i d"@en .

:hasVehicleSegmentID a owl:ObjectProperty ;
    rdfs:isDefinedBy :core ;
    skos:definition "The identifier of a part of the Transport Means. WG approval 25/06/2024 (epo-ful:TransportMeans -> adms:Identifier (+epo-ful:hasVehicleSegmentID))"@en ;
    skos:prefLabel "Has vehicle segment i d"@en .

:hasVersion a owl:DatatypeProperty ;
    rdfs:isDefinedBy :core ;
    skos:definition "A number that identifies a specific state of a document. WG approval: 18/11/2021 (epo:Document)"@en ;
    skos:prefLabel "Has version"@en .

:hasWeightValueType a owl:ObjectProperty ;
    rdfs:isDefinedBy :core ;
    skos:definition "No definition. Waiting on CCCEV alignment. (epo:ProcurementCriterion -> at-voc:number-weight (+epo:hasWeightValueType))"@en ;
    skos:prefLabel "Has weight value type"@en .

:hasWidth a owl:ObjectProperty ;
    rdfs:isDefinedBy :core ;
    skos:definition "The measurement of the depth. Additional Information: The width is the shorter side between the length and the width. WG approval 18/06/2024 (epo-ful:AbstractContainer -> epo:Quantity (+epo-ful:hasWidth))"@en ;
    skos:prefLabel "Has width"@en .

:hasWithdrawalDate a owl:DatatypeProperty ;
    rdfs:isDefinedBy :core ;
    skos:definition "The date and time when the request for review was withdrawn. Additional information: This attribute corresponds in eForms to BT-797 Review Request Withdrawn Date. (epo:ReviewRequest)"@en ;
    skos:prefLabel "Has withdrawal date"@en .

:hasWithdrawalReason a owl:DatatypeProperty ;
    rdfs:isDefinedBy :core ;
    skos:definition "The explanation for withdrawing the request for review. Additional information: This attribute corresponds in eForms to BT-798 Review Request Withdrawn Reasons (epo:ReviewRequest)"@en ;
    skos:prefLabel "Has withdrawal reason"@en .

:hasZeroEmissionVehicles a owl:DatatypeProperty ;
    rdfs:isDefinedBy :core ;
    skos:definition "The number of all zero-emission heavy-duty vehicles that have either been purchased, leased, rented, hired-purchased or their use has been contractually committed to for the provision of a purchased service. Additional Information: In the European Union, the legal requirements and scope for the provision of these vehicles or services are covered by Directive 2009/33/EC. WG Approval 28/07/2020 (epo:VehicleInformation)"@en ;
    skos:prefLabel "Has zero emission vehicles"@en .

:implementsContract a owl:ObjectProperty ;
    rdfs:isDefinedBy :core ;
    skos:prefLabel "Implements contract"@en .

:includesAccessibilityCriterion a owl:ObjectProperty ;
    rdfs:isDefinedBy :core ;
    skos:definition "Explanation as to whether accessibility Criterion are used or not. WG Approval 09/11/2021 (epo:StrategicProcurement -> at-voc:accessibility (+epo:includesAccessibilityCriterion))"@en ;
    skos:prefLabel "Includes accessibility criterion"@en .

:includesNationalCriterion a owl:ObjectProperty ;
    rdfs:isDefinedBy :core ;
    skos:definition "Relation indicating that a Criterion contains a Criterion that is specific to a given Member State. Additional Information: In the ESPD, a Subcriterion is used to define national sub-criteria; maps to a UBL-2.3 cac:SubTenderingCriterion class. It is currently used only for purely national criteria, to be able to establish the mapping from eCertis. WG approval 07/11/2023 (epo:QualificationCriterion -> epo:QualificationCriterion (+epo:includesNationalCriterion))"@en ;
    skos:prefLabel "Includes national criterion"@en .

:includesTender a owl:ObjectProperty ;
    rdfs:isDefinedBy :core ;
    skos:definition "Additional information: This corresponds in eForms to BT-3202 Contract Tender Identifier. (epo:Contract -> epo:Tender (+epo:includesTender))"@en ;
    skos:prefLabel "Includes tender"@en .

:indicatesAwardToWinner a owl:ObjectProperty ;
    rdfs:isDefinedBy :core ;
    skos:definition "Reveals the winner to whom the tender award outcome is attributed. (epo:TenderAwardOutcome -> epo:Winner (+epo:indicatesAwardToWinner))"@en ;
    skos:prefLabel "Indicates award to winner"@en .

:indicatesInvoiceeContactPoint a owl:ObjectProperty ;
    rdfs:isDefinedBy :core ;
    skos:prefLabel "Indicates invoicee contact point"@en .

:indicatesPerformingStaffInformationRequirement a owl:DatatypeProperty ;
    rdfs:isDefinedBy :core ;
    skos:definition "Obligation to indicate the names and professional qualifications of the staff assigned to performing the contract. WG approval 02/05/2024 (epo:ProcurementCriteriaSummary)"@en ;
    skos:prefLabel "Indicates performing staff information requirement"@en .

:involvesBuyer a owl:ObjectProperty ;
    rdfs:isDefinedBy :core ;
    skos:prefLabel "Involves buyer"@en .

:involvesProcurementDocument a owl:ObjectProperty ;
    rdfs:isDefinedBy :core ;
    skos:prefLabel "Involves procurement document"@en .

:isAccelerated a owl:DatatypeProperty ;
    rdfs:isDefinedBy :core ;
    skos:definition "Statement about the fact that the procedure will be reduced due to a state of urgency. Additional Information This modifies the time limit for the receipt of requests to participate or the receipt of tenders. WG Approval 20/08/2019 (epo:Procedure)"@en ;
    skos:prefLabel "Is accelerated"@en .

:isAdvancedElectronicSignatureRequired a owl:DatatypeProperty ;
    rdfs:isDefinedBy :core ;
    skos:definition "Advanced or qualified electronic signature or seal (as defined in Regulation (EU) No 910/2014) is required. The submitted information is required to be signed electronically. Additional Information: Signature can be defined as \"data in electronic form which is attached to or logically associated with other data in electronic form and which is used by the signatory to sign. For more details on the meaning and uses of electronic signature you may consult different authoritative sources, a relevant one being for instance the Regulation (EU) 910/2014 on electronic identification and trust services for electronic transactions in the internal market. WG Approval 21/07/2020 (epo:SubmissionTerm)"@en ;
    skos:prefLabel "Is advanced electronic signature required"@en .

:isAwardedByCPB a owl:DatatypeProperty ;
    rdfs:isDefinedBy :core ;
    skos:definition "Procedure is awarded by a Central Purchasing Body. (epo:ProcedureTerm)"@en ;
    skos:prefLabel "Is awarded by c p b"@en .

:isBasedOnImplementingRegulation a owl:ObjectProperty ;
    rdfs:isDefinedBy :core ;
    skos:definition "Indicates under which regulation a notice is created. WG Acceptance 06/09/2022 (epo:Notice -> at-voc:legal-basis (+epo:isBasedOnImplementingRegulation))"@en ;
    skos:prefLabel "Is based on implementing regulation"@en .

:isBeneficialOwnerOf a owl:ObjectProperty ;
    rdfs:isDefinedBy :core ;
    skos:definition "A role of any natural person(s) who ultimately owns or controls the organisation or on whose behalf a transaction or activity is being conducted. Additional Information: This role is defined in the directive EU 2015/849 and it's beyond the scope for public eProcurement domain. WG approval 14/09/2021 (epo:Business <-> person:Person (+epo:hasBeneficialOwner +epo:isBeneficialOwnerOf))"@en ;
    skos:prefLabel "Is beneficial owner of"@en .

:isCalculatedOn a owl:ObjectProperty ;
    rdfs:isDefinedBy :core ;
    skos:definition "The monetary amount to which the multiplier factor is applied in calculating the amount of this allowance or charge. (epo-ord:AllowanceChargeInformation -> epo:MonetaryValue (+epo:isCalculatedOn)) The monetary amount to which the multiplier factor is applied in calculating the amount of this allowance or charge. (epo-ord:TaxInformation -> epo:MonetaryValue (+epo:isCalculatedOn))"@en ;
    skos:prefLabel "Is calculated on"@en .

:isCompetitionTerminated a owl:DatatypeProperty ;
    rdfs:isDefinedBy :core ;
    skos:definition "No further contracts will be awarded in this procedure. Additional Information: This can be instantiated in the post award phase. PIN for Competition needs to be signaled. This field can be used even if no contracts are awarded in the contract award notice. This corresponds in eForms to BT-756 PIN Competition Termination. (epo:ProcurementProcessInformation)"@en ;
    skos:prefLabel "Is competition terminated"@en .

:isContractingEntity a owl:DatatypeProperty ;
    rdfs:isDefinedBy :core ;
    skos:definition "Role of entities, which: (a) are contracting authorities or public undertakings and which pursue one of the activities referred to in Articles 8 to 14 of the Directive 2014/25/EU. (b) when they are not contracting authorities or public undertakings, have as one of their activities any of the activities referred to in Articles 8 to 14, or any combination thereof and operate on the basis of special or exclusive rights granted by a competent authority of a Member State. Additional Information The indicator is needed in order to discriminate between those contracts where the Contracting Entity acts as a Contracting Authority undergoing the limits and the rules of Directive 24 and those where it acts as a Contracting Entity, with certain relaxed constraints. For example, the Contracting Entities have different thresholds for the application of Directive 24 if compared with Contracting Authorities. WG Approval 28/04/2020 (epo:Buyer)"@en ;
    skos:prefLabel "Is contracting entity"@en .

:isCoveredByGPA a owl:DatatypeProperty ;
    rdfs:isDefinedBy :core ;
    skos:definition "Specifies whether the Agreement on Government Procurement (GPA) applies. Additional information: The GPA aims to establish a multilateral framework of balanced rights and obligations relating to public contracts with a view to achieving the liberalization and expansion of world trade. This corresponds in the e Forms to BT-115 GPA Coverage. WG Approval 15/10/2019 (epo:ProcurementObject)"@en ;
    skos:prefLabel "Is covered by g p a"@en .

:isDPSTerminated a owl:DatatypeProperty ;
    rdfs:isDefinedBy :core ;
    skos:definition "End of the Dynamic Purchase System (DPS). Additional Information: This property can be used in the contract award notice even if no contracts are awarded. WG Approval 22/11/2019 (epo:ProcurementProcessInformation)"@en ;
    skos:prefLabel "Is d p s terminated"@en .

:isDesignContest a owl:DatatypeProperty ;
    rdfs:isDefinedBy :core ;
    skos:definition "A competition which enables the buyer to acquire a plan or design via a jury. Additional information: Design contests have traditionally mostly been used in the fields of town and country planning, architecture and engineering or data processing, other purposes, such as to obtain plans for financial engineering The contest may include or not the award of prizes; WG approval 04-02-2021 (epo:Procedure)"@en ;
    skos:prefLabel "Is design contest"@en .

:isExecutedByProcurementServiceProvider a owl:ObjectProperty ;
    rdfs:isDefinedBy :core ;
    skos:prefLabel "Is executed by procurement service provider"@en .

:isFundedBy a owl:ObjectProperty ;
    rdfs:isDefinedBy :core ;
    skos:definition "Funding is provided either completely or partially by a Fund. Additional information: This corresponds in eForms to BG - 61 EU Funds (specified per Lot) and to BG - 611 Contract EU Funds (applied per Contract lot) Funds may change between the lot and the contract, for example in the case of an emergency crisis, a contract may be financed by a budget that was not foreseen in the call. (epo:Contract -> epo:Fund (+epo:isFundedBy)) Funding is provided either completely or partially by a Fund. Additional information: This corresponds in eForms to BG - 61 EU Funds (specified per Lot) and to BG - 611 Contract EU Funds (applied per Contract lot) Funds may change between the lot and the contract, for example in the case of an emergency crisis, a contract may be financed by a budget that was not foreseen in the call. (epo:ProcurementObject -> epo:Fund (+epo:isFundedBy))"@en ;
    skos:prefLabel "Is funded by"@en .

:isGuaranteeRequired a owl:DatatypeProperty ;
    rdfs:isDefinedBy :core ;
    skos:definition "The submitted information must include a financial commitment to be used in case of default. Additional Information: See the additional information provided in the definition of the 'Guarantee Description' element. WG Approval 21/07/20 (epo:SubmissionTerm)"@en ;
    skos:prefLabel "Is guarantee required"@en .

:isJointProcurement a owl:DatatypeProperty ;
    rdfs:isDefinedBy :core ;
    skos:definition "Multiple buyers procure together within the same procedure. Addition Information: In case the joint procurement involves buyers from different countries, the national law is specified by the epo:hasCrossBorderLaw in the ProcedureTerm . (epo:Procedure)"@en ;
    skos:prefLabel "Is joint procurement"@en .

:isJuryDecisionBinding a owl:DatatypeProperty ;
    rdfs:isDefinedBy :core ;
    skos:definition "Indicates whether the procuring entity is bound to apply the decision of the jury. (epo:DesignContestRegimeTerm)"@en ;
    skos:prefLabel "Is jury decision binding"@en .

:isListedCompany a owl:DatatypeProperty ;
    rdfs:isDefinedBy :core ;
    skos:definition "Public companies listed on a stock exchange and subject to disclosure requirements (either by stock exchange rules or through law or enforceable means), which impose requirements to ensure adequate transparency of beneficial ownership. <u>Additional Information:</u> In eForms this indicator is used when the nationality of beneficial owner is not provided because the Economic Operator is registered in a regulated market that is subject to disclosure requirements consistent with Union law or subject to equivalent international standards which ensure adequate transparency of ownership information. WG Approval 21/11/2019 (epo:Business)"@en ;
    skos:prefLabel "Is listed company"@en .

:isMultipleTenderSubmissionAllowed a owl:DatatypeProperty ;
    rdfs:isDefinedBy :core ;
    skos:definition "Tenderers may submit more than one competing tenders. WG Approval 10/10/2019 (epo:SubmissionTerm)"@en ;
    skos:prefLabel "Is multiple tender submission allowed"@en .

:isNonDisclosureAgreementRequired a owl:DatatypeProperty ;
    rdfs:isDefinedBy :core ;
    skos:definition "A non-disclosure agreement is needed. Additional information: A non-disclosure agreement is a Contract between different parties which ensures information is not shared with other parties. WG approval 26/03/2024 (epo:NonDisclosureAgreementTerm)"@en ;
    skos:prefLabel "Is non disclosure agreement required"@en .

:isOneLotOnlyAllowed a owl:DatatypeProperty ;
    rdfs:isDefinedBy :core ;
    skos:definition "Indicates whether tenders may be submitted for only one Lot. Additional information: This field is used to complement the SubmissionTerms (which are at the Lot level) for the Procedure level which is covered by the regulation (EU)-2015-1986 (modeled in the TED Standard Forms). WG approval 23/08/2022 (epo:ProcedureTerm)"@en ;
    skos:prefLabel "Is one lot only allowed"@en .

:isOwnedByAgent a owl:ObjectProperty ;
    rdfs:isDefinedBy :core ;
    skos:prefLabel "Is owned by agent"@en .

:isProcurementDocumentChanged a owl:DatatypeProperty ;
    rdfs:isDefinedBy :core ;
    skos:definition "One or more procurement documents have been changed. Additional information: This corresponds in eForms to BT-718 Change Procurement Documents WG Approval 05/11/2019 (epo:ChangeInformation)"@en ;
    skos:prefLabel "Is procurement document changed"@en .

:isProcurementDocumentRestricted a owl:DatatypeProperty ;
    rdfs:isDefinedBy :core ;
    skos:definition "The access to certain procurement documents is restricted. Additional Information: This corresponds in eForms to BT-14 Documents Restricted. WG Approval 10/10/2019 (epo:AccessTerm)"@en ;
    skos:prefLabel "Is procurement document restricted"@en .

:isRecurrent a owl:DatatypeProperty ;
    rdfs:isDefinedBy :core ;
    skos:definition "The Procurement being notified is likely to be included in another procedure in the foreseeable future. Additional Information: For example, a regularly re-tendered municipal service. This does not include awarding multiple contracts within a single qualification system, framework agreement, or a dynamic purchasing system. This corresponds in eForms to BT-94 Recurrence. WG Approval 12/05/2020 (epo:ProcurementObject)"@en ;
    skos:prefLabel "Is recurrent"@en .

:isReinforcedBy a owl:ObjectProperty ;
    rdfs:isDefinedBy :core ;
    skos:definition "Relation indicating an Evidence that supports the Response. WG approval 12/03/2024 (epo-sub:Response -> cccev:Evidence (+epo-sub:isReinforcedBy))"@en ;
    skos:prefLabel "Is reinforced by"@en .

:isRenewalIndicator a owl:DatatypeProperty ;
    rdfs:isDefinedBy :core ;
    skos:definition "Indicates whether the contract is subject to a renewal clause. WG Approval 09/11/2021 (epo:ContractTerm)"@en ;
    skos:prefLabel "Is renewal indicator"@en .

:isResponsibilityOfBuyer a owl:ObjectProperty ;
    rdfs:isDefinedBy :core ;
    skos:definition "The buyer in charge of the procedure. Additional Information: In case there are multiple buyers, it may be the case that one or more buyers are in charge of the procedure. (epo:Procedure -> epo:Buyer (+epo:isResponsibilityOfBuyer))"@en ;
    skos:prefLabel "Is responsibility of buyer"@en .

:isSMESuitable a owl:DatatypeProperty ;
    rdfs:isDefinedBy :core ;
    skos:definition "The Lot is suitable for small and medium enterprises (SMEs). Additional Information This allows the buyer to make emphasis on the fact that the procedure has been designed having SMEs in mind. This indicator is also to be reflected in the selection criteria. For example, number of employees and turnover are applicable to the definition of an SME. WG Approval 15/10/2019 (epo:ProcurementObject)"@en ;
    skos:prefLabel "Is s m e suitable"@en .

:isSecurityClearanceRequired a owl:DatatypeProperty ;
    rdfs:isDefinedBy :core ;
    skos:definition "Security Clearance is needed. WG approval 02/05/2024 (epo:SecurityClearanceTerm)"@en ;
    skos:prefLabel "Is security clearance required"@en .

:isSubcontractingPercentageKnown a owl:DatatypeProperty ;
    rdfs:isDefinedBy :core ;
    skos:prefLabel "Is subcontracting percentage known"@en .

:isSubcontractingValueKnown a owl:DatatypeProperty ;
    rdfs:isDefinedBy :core ;
    skos:prefLabel "Is subcontracting value known"@en .

:isSubjectToContractSpecificTerm a owl:ObjectProperty ;
    rdfs:isDefinedBy :core ;
    skos:prefLabel "Is subject to contract specific term"@en .

:isSubjectToGrouping a owl:ObjectProperty ;
    rdfs:isDefinedBy :core ;
    skos:prefLabel "Is subject to grouping"@en .

:isSubjectToLotSpecificTerm a owl:ObjectProperty ;
    rdfs:isDefinedBy :core ;
    rdfs:subPropertyOf :isSubjectToTerm ;
    skos:prefLabel "Is subject to lot specific term"@en .

:isSubjectToProcedureSpecificTerm a owl:ObjectProperty ;
    rdfs:isDefinedBy :core ;
    rdfs:subPropertyOf :isSubjectToTerm ;
    skos:prefLabel "Is subject to procedure specific term"@en .

:isSubmissionForAllLotsRequired a owl:DatatypeProperty ;
    rdfs:isDefinedBy :core ;
    skos:definition "Indicates whether tenders must be submitted for all Lots. (epo:ProcedureTerm)"@en ;
    skos:prefLabel "Is submission for all lots required"@en .

:isSubmitedBy a owl:ObjectProperty ;
    rdfs:isDefinedBy :core ;
    skos:definition "Relation indicating the submission of a tender by an economic operator. WG approval 18/05/2021 (epo:Tender -> epo:Tenderer (+epo:isSubmitedBy))"@en ;
    skos:prefLabel "Is submited by"@en .

:isSubmittedForLot a owl:ObjectProperty ;
    rdfs:isDefinedBy :core ;
    skos:prefLabel "Is submitted for lot"@en .

:isSubmittedForLotGroup a owl:ObjectProperty ;
    rdfs:isDefinedBy :core ;
    skos:prefLabel "Is submitted for lot group"@en .

:isSubordinatedToContract a owl:ObjectProperty ;
    rdfs:isDefinedBy :core ;
    skos:prefLabel "Is subordinated to contract"@en .

:isSupportedBy a owl:ObjectProperty ;
    rdfs:isDefinedBy :core ;
    skos:prefLabel "Is supported by"@en .

:isToBeRelaunched a owl:DatatypeProperty ;
    rdfs:isDefinedBy :core ;
    skos:definition "Indicator of whether the procurement object is to be relaunched. Additional information: This can be instantiated in the post award phase. This corresponds in eForms to BT-634 Procurement Relaunch. WG Approval: 18/01/2022 (epo:ProcurementProcessInformation)"@en ;
    skos:prefLabel "Is to be relaunched"@en .

:isUsedForCandidateRestriction a owl:DatatypeProperty ;
    rdfs:isDefinedBy :core ;
    skos:definition "The criterion will be used to select the candidates to be invited for the second stage of a multistage procedure. Additional Information: This property is only used if a maximum number of candidates was foreseen in the procedure. This corresponds in eForms to BT-40 Selection Criteria Second Stage Invite (epo:SelectionCriterion)"@en ;
    skos:prefLabel "Is used for candidate restriction"@en .

:isUsingEUFunds a owl:DatatypeProperty ;
    rdfs:isDefinedBy :core ;
    skos:definition "The procurement foresees funding by the Union. Additional Information: The funding may cover the whole procurement or part of the procurement. For example the European Structural and Investment Funds or grants awarded by the European Union. (epo:ProcurementObject)"@en ;
    skos:prefLabel "Is using e u funds"@en .

:isVariant a owl:DatatypeProperty ;
    rdfs:isDefinedBy :core ;
    skos:definition "Alternative solution to fulfil the buyer's needs as opposed to solutions indicated in the procurement documents. Additional Information: The permission to offer variants is only allowed if specified in a Contract Notice or a Prior Information Notice that used as a means for calling for a competition. The buyer lays out minimum requirements in the procurement documents that must be respected by tenderers submitting variants. WG Approval 29/05/2019 (epo:Tender)"@en ;
    skos:prefLabel "Is variant"@en .

:isWithdrawn a owl:DatatypeProperty ;
    rdfs:isDefinedBy :core ;
    skos:definition "The review request was withdrawn. Additional information: This attribute corresponds in eForms to BT-796 Review Request Withdrawn. (epo:ReviewRequest)"@en ;
    skos:prefLabel "Is withdrawn"@en .

:issuedByCertifier a owl:ObjectProperty ;
    rdfs:isDefinedBy :core ;
    skos:definition "Relation indicating the Certifier responsible for providing the ItemCertificate. Additional Information: Certifier is a role played by an organisation. WG approval 26/07/2022 (epo:Certificate -> epo:Certifier (+epo:issuedByCertifier))"@en ;
    skos:prefLabel "Issued by certifier"@en .

:leadBy a owl:ObjectProperty ;
    rdfs:isDefinedBy :core ;
    skos:definition "The epo:OrganisationGroup epo:leadBy org:Organization was implemented to be used in case of an Economic Operator Group. (epo:OrganisationGroup -> org:Organization (+epo:leadBy))"@en ;
    skos:prefLabel "Lead by"@en .

:needsToBeATenderer a owl:ObjectProperty ;
    rdfs:isDefinedBy :core ;
    skos:definition "The Winner must be a Tenderer. (epo:Winner -> epo:Tenderer (+epo:needsToBeATenderer))"@en ;
    skos:prefLabel "Needs to be a tenderer"@en .

:needsToBeAWinner a owl:ObjectProperty ;
    rdfs:isDefinedBy :core ;
    skos:definition "The Contractor must be a Winner. (epo:Contractor -> epo:Winner (+epo:needsToBeAWinner))"@en ;
    skos:prefLabel "Needs to be a winner"@en .

:ownsSystem a owl:ObjectProperty ;
    rdfs:isDefinedBy :core ;
    skos:prefLabel "Owns system"@en .

:playedBy a owl:ObjectProperty ;
    rdfs:isDefinedBy :core ;
    skos:prefLabel "Played by"@en .

:providesContractTotalPaymentValue a owl:ObjectProperty ;
    rdfs:isDefinedBy :core ;
    skos:definition "Additional Information: This corresponds to BT-779 in eForms. (epo:ContractLotCompletionInformation -> epo:MonetaryValue (+epo:providesContractTotalPaymentValue))"@en ;
    skos:prefLabel "Provides contract total payment value"@en .

:providesContractTotalPenaltyValue a owl:ObjectProperty ;
    rdfs:isDefinedBy :core ;
    skos:definition "Additional Information: This corresponds to BT-782 in eForms. (epo:ContractLotCompletionInformation -> epo:MonetaryValue (+epo:providesContractTotalPenaltyValue))"@en ;
    skos:prefLabel "Provides contract total penalty value"@en .

:providesInformationOn a owl:ObjectProperty ;
    rdfs:isDefinedBy :core ;
    skos:definition "Offers information about an instance of a concept. WG approval 05/03/2024 (epo-sub:ESPD -> org:Organization (+epo-sub:providesInformationOn))"@en ;
    skos:prefLabel "Provides information on"@en .

:providesOrganisationEmployeeQuantity a owl:ObjectProperty ;
    rdfs:isDefinedBy :core ;
    skos:definition "The number of people hired by the Organization. WG approval 05/03/2024 (epo-sub:NationalPreQualificationData -> epo:Quantity (+epo-sub:providesOrganisationEmployeeQuantity))"@en ;
    skos:prefLabel "Provides organisation employee quantity"@en .

:providesOrganisationFinancialCapability a owl:ObjectProperty ;
    rdfs:isDefinedBy :core ;
    skos:definition "A monetary amount representing the financial capability of the Organization. Additional information: Used to represent the general Turnover of the Organization (for statistical purposes). WG approval 05/03/2024 (epo-sub:NationalPreQualificationData -> epo:MonetaryValue (+epo-sub:providesOrganisationFinancialCapability))"@en ;
    skos:prefLabel "Provides organisation financial capability"@en .

:providesOrganisationPreQualificationListingIdentifier a owl:ObjectProperty ;
    rdfs:isDefinedBy :core ;
    skos:definition "The identifier assigned to an economic operator in a national pre-qualification system or official list. WG approval 05/03/2024 (epo-sub:NationalPreQualificationData -> adms:Identifier (+epo-sub:providesOrganisationPreQualificationListingIdentifier))"@en ;
    skos:prefLabel "Provides organisation pre qualification listing identifier"@en .

:providesRulingOnRemedy a owl:ObjectProperty ;
    rdfs:isDefinedBy :core ;
    skos:definition "States the measures to be taken after a review procedure. (epo:ReviewDecision -> at-voc:remedy-type (+epo:providesRulingOnRemedy))"@en ;
    skos:prefLabel "Provides ruling on remedy"@en .

:refersToApplicablePeriod a owl:ObjectProperty ;
    rdfs:isDefinedBy :core ;
    skos:definition "Relation indicating the period to which the Response shall apply. WG approval 12/03/2024 (epo-sub:Response -> epo:Period (+epo-sub:refersToApplicablePeriod))"@en ;
    skos:prefLabel "Refers to applicable period"@en .

:refersToAwardDecision a owl:ObjectProperty ;
    rdfs:isDefinedBy :core ;
    skos:prefLabel "Refers to award decision"@en .

:refersToContract a owl:ObjectProperty ;
    rdfs:isDefinedBy :core ;
    skos:prefLabel "Refers to contract"@en .

:refersToContractToBeModified a owl:ObjectProperty ;
    rdfs:isDefinedBy :core ;
    skos:prefLabel "Refers to contract to be modified"@en .

:refersToLot a owl:ObjectProperty ;
    rdfs:isDefinedBy :core ;
    skos:prefLabel "Refers to lot"@en .

:refersToLotGroup a owl:ObjectProperty ;
    rdfs:isDefinedBy :core ;
    skos:prefLabel "Refers to lot group"@en .

:refersToLotGroupAwardInformation a owl:ObjectProperty ;
    rdfs:isDefinedBy :core ;
    skos:prefLabel "Refers to lot group award information"@en .

:refersToNotice a owl:ObjectProperty ;
    rdfs:isDefinedBy :core ;
    skos:definition "Reference to a Notice. WG approval 12/03/2024 (epo-acc:ESPDRequest -> epo:Notice (+epo-acc:refersToNotice))"@en ;
    skos:prefLabel "Refers to notice"@en .

:refersToNoticeAwardInformation a owl:ObjectProperty ;
    rdfs:isDefinedBy :core ;
    skos:prefLabel "Refers to notice award information"@en .

:refersToPlannedPart a owl:ObjectProperty ;
    rdfs:isDefinedBy :core ;
    skos:prefLabel "Refers to planned part"@en .

:refersToPrevious a owl:ObjectProperty ;
    rdfs:isDefinedBy :core ;
    skos:prefLabel "Refers to previous"@en .

:refersToPreviousNotice a owl:ObjectProperty ;
    rdfs:isDefinedBy :core ;
    skos:definition "Additional information: This corresponds in eForms to BT-758 Change Notice Version Identifier. (epo:ChangeInformation -> epo:Notice (+epo:refersToPreviousNotice))"@en ;
    skos:prefLabel "Refers to previous notice"@en .

:refersToPreviousProcedure a owl:ObjectProperty ;
    rdfs:isDefinedBy :core ;
    skos:definition "Reference to a previous procedure. Additional Information: In the case of Direct Award Terms, this property points to a previous Procedure justifying the use of Direct Award without a prior publication. This corresponds in the eForms to BT-1252 Direct Award Justification Previous Procedure Identifier (epo:DirectAwardTerm -> epo:Procedure (+epo:refersToPreviousProcedure))"@en ;
    skos:prefLabel "Refers to previous procedure"@en .

:refersToPreviousProcedureLot a owl:ObjectProperty ;
    rdfs:isDefinedBy :core ;
    skos:definition "Reference to one or more Lots in a previous procedure. Additional Information: In the case of Direct Award Terms, this property points to a previous Procedure justifying the use of Direct Award without a prior publication. This corresponds in the eForms to BT-1252 Direct Award Justification Previous Procedure Identifier WG Approval 22/11/2019 14:33:55 (epo:DirectAwardTerm -> epo:Lot (+epo:refersToPreviousProcedureLot))"@en ;
    skos:prefLabel "Refers to previous procedure lot"@en .

:refersToPreviousReview a owl:ObjectProperty ;
    rdfs:isDefinedBy :core ;
    skos:definition "Additional information: This relation corresponds in eForms to BT-785 \"Review Previous Identifier\". (epo:ReviewObject -> epo:ReviewObject (+epo:refersToPreviousReview))"@en ;
    skos:prefLabel "Refers to previous review"@en .

:refersToProcedure a owl:ObjectProperty ;
    rdfs:isDefinedBy :core ;
    skos:prefLabel "Refers to procedure"@en .

:refersToProject a owl:ObjectProperty ;
    rdfs:isDefinedBy :core ;
    skos:prefLabel "Refers to project"@en .

:refersToRole a owl:ObjectProperty ;
    rdfs:isDefinedBy :core ;
    skos:prefLabel "Refers to role"@en .

:relatesToEFormSectionIdentifier a owl:ObjectProperty ;
    rdfs:isDefinedBy :core ;
    skos:prefLabel "Relates to e form section identifier"@en .

:requestsRemedyType a owl:ObjectProperty ;
    rdfs:isDefinedBy :core ;
    skos:definition "Additional information: This relation corresponds in eForms to BT-792 Review Remedy Type (epo:ReviewRequest -> at-voc:remedy-type (+epo:requestsRemedyType))"@en ;
    skos:prefLabel "Requests remedy type"@en .

:resolvesReviewRequest a owl:ObjectProperty ;
    rdfs:isDefinedBy :core ;
    skos:prefLabel "Resolves review request"@en .

:resultsFromLotAwardOutcome a owl:ObjectProperty ;
    rdfs:isDefinedBy :core ;
    skos:prefLabel "Results from lot award outcome"@en .

:resultsFromMiniCompetitionAwardOutcome a owl:ObjectProperty ;
    rdfs:isDefinedBy :core ;
    skos:prefLabel "Results from mini competition award outcome"@en .

:resultsFromUsingCandidateList a owl:ObjectProperty ;
    rdfs:isDefinedBy :core ;
    skos:prefLabel "Results from using candidate list"@en .

:setsGroupingContextForLot a owl:ObjectProperty ;
    rdfs:isDefinedBy :core ;
    skos:prefLabel "Sets grouping context for lot"@en .

:signedByBuyer a owl:ObjectProperty ;
    rdfs:isDefinedBy :core ;
    skos:prefLabel "Signed by buyer"@en .

:signedByContractor a owl:ObjectProperty ;
    rdfs:isDefinedBy :core ;
    skos:prefLabel "Signed by contractor"@en .

:signsAwardDecision a owl:ObjectProperty ;
    rdfs:isDefinedBy :core ;
    skos:prefLabel "Signs award decision"@en .

:specifiesBuyer a owl:ObjectProperty ;
    rdfs:isDefinedBy :core ;
    skos:prefLabel "Specifies buyer"@en .

:specifiesCatalogueProvider a owl:ObjectProperty ;
    rdfs:isDefinedBy :core ;
    skos:prefLabel "Specifies catalogue provider"@en .

:specifiesCatalogueReceiver a owl:ObjectProperty ;
    rdfs:isDefinedBy :core ;
    skos:prefLabel "Specifies catalogue receiver"@en .

:specifiesCleanVehicleDirectiveContractType a owl:ObjectProperty ;
    rdfs:isDefinedBy :core ;
    skos:prefLabel "Specifies clean vehicle directive contract type"@en .

:specifiesCleanVehicleDirectiveVehicleCategory a owl:ObjectProperty ;
    rdfs:isDefinedBy :core ;
    skos:prefLabel "Specifies clean vehicle directive vehicle category"@en .

:specifiesDeliverable a owl:ObjectProperty ;
    rdfs:isDefinedBy :core ;
    skos:prefLabel "Specifies deliverable"@en .

:specifiesDeliveryAgreementLocation a owl:ObjectProperty ;
    rdfs:isDefinedBy :core ;
    skos:prefLabel "Specifies delivery agreement location"@en .

:specifiesEconomicOperator a owl:ObjectProperty ;
    rdfs:isDefinedBy :core ;
    skos:prefLabel "Specifies economic operator"@en .

:specifiesPlaceOfDelivery a owl:ObjectProperty ;
    rdfs:isDefinedBy :core ;
    skos:prefLabel "Specifies place of delivery"@en .

:specifiesPlaceOfDespatch a owl:ObjectProperty ;
    rdfs:isDefinedBy :core ;
    skos:definition "Relation indicating the Location of the Despatch of the Goods Items to be delivered. WG approval 25/06/2024 (epo-ful:ShipmentInformation -> dct:Location (+epo-ful:specifiesPlaceOfDespatch))"@en ;
    skos:prefLabel "Specifies place of despatch"@en .

:specifiesProcurementCriteriaSummary a owl:ObjectProperty ;
    rdfs:isDefinedBy :core ;
    skos:prefLabel "Specifies procurement criteria summary"@en .

:specifiesProcurementCriterion a owl:ObjectProperty ;
    rdfs:isDefinedBy :core ;
    skos:prefLabel "Specifies procurement criterion"@en .

:specifiesSubcontractors a owl:ObjectProperty ;
    rdfs:isDefinedBy :core ;
    skos:prefLabel "Specifies subcontractors"@en .

:substantiatesExclusionGround a owl:ObjectProperty ;
    rdfs:isDefinedBy :core ;
    skos:prefLabel "Substantiates exclusion ground"@en .

:summarisesInformationAboutCertificate a owl:ObjectProperty ;
    rdfs:isDefinedBy :core ;
    skos:definition "Relation indicating the Certificate that the information refers to. WG approval 12/03/2024 (epo-sub:CertificateInformation -> epo:Certificate (+epo-sub:summarisesInformationAboutCertificate))"@en ;
    skos:prefLabel "Summarises information about certificate"@en .

:summarisesInformationForAwardOutcome a owl:ObjectProperty ;
    rdfs:isDefinedBy :core ;
    skos:definition "Relates to submission for the given competition, either at Lot level or Mini-Competition level. WG approval 30/05/2023 (epo:SubmissionStatisticalInformation -> epo:AwardOutcome (+epo:summarisesInformationForAwardOutcome))"@en ;
    skos:prefLabel "Summarises information for award outcome"@en .

:updatesContractValue a owl:ObjectProperty ;
    rdfs:isDefinedBy :core ;
    skos:prefLabel "Updates contract value"@en .

:usesChannel a owl:ObjectProperty ;
    rdfs:isDefinedBy :core ;
    skos:prefLabel "Uses channel"@en .

:usesCleanVehicleDirective a owl:DatatypeProperty ;
    rdfs:isDefinedBy :core ;
    skos:definition "The procurement falls within the scope of the European Parliament and Council 2009/33/EC (Clean Vehicles Directive – CVD). (epo:GreenProcurement)"@en ;
    skos:prefLabel "Uses clean vehicle directive"@en .

:usesTechnique a owl:ObjectProperty ;
    rdfs:isDefinedBy :core ;
    skos:prefLabel "Uses technique"@en .

eli:uri_schema a owl:ObjectProperty ;
    skos:definition "Schema describing the URI of an ELI instance. ELI uses URI template specifications (IETF RFC 6570). Schemes should be associated with member states and will be published in a registry. (eli:LegalResourceSubdivision -> adms:Identifier (+eli:uri_schema)) Schema describing the URI of an ELI instance. ELI uses URI template specifications (IETF RFC 6570). Schemes should be associated with member states and will be published in a registry. (eli:LegalExpression -> adms:Identifier (+eli:uri_schema))"@en ;
    skos:prefLabel "Uri_schema"@en .

cccev:Constraint a owl:Class ;
    rdfs:subClassOf cccev:Requirement ;
    skos:definition "Limitation applied to an Information Concept. Additional Information: Constraints are Requirements in themselves, since they impose prerequisites which influence the definition, use and/or Fulfilment of the Requirement. They represent hard conditions such as minimum or maximum expressions which can be used to evaluate pieces of information, the required age, income, involvement in activities, etc. An example from the eProcurement domain is a threshold as the minimum turnover required by the buying Organisation to select the Candidates. Note that CCCEV does not provide any specific guidance on when which kind of Requirement should be used. Users of this vocabulary should make decisions on this topic in their specific context."@en ;
    skos:prefLabel "Constraint"@en .

cccev:ContactPoint a owl:Class ;
    skos:definition "Information (e.g. e-mail address, telephone number) of a Person or department through which the user can get in touch with. Additional information: This class represents the contact information for a Public Service, Channel, Public Organisation, etc. The Contact Point could be a role, email address, telephone number, etc. WG approval 5/11/2019"@en ;
    skos:prefLabel "Contact point"@en .

cccev:InformationRequirement a owl:Class ;
    rdfs:subClassOf cccev:Requirement ;
    skos:definition "Requested data that is to be proven by Evidence. Additional Information: Information Requirements are the most neutral kind of Requirements. They aim to request information in any form, e.g. a person's date of birth or a company's turnover. They represent requests for data that prove one or more facts of the real world in a formal manner, or that leads to the source of such a proof. They can be understood as 'requests for Evidences'. The response to an Information Requirement is an Evidence when the issuer of the response is an authoritative source (e.g. a Civil Registry providing data about a natural person for the provision of public service through the Single Digital Gateway). In other cases, the responses might not be issued by an authoritative source, but the issuer supports the responses with Evidences (or commits to support them timely, e.g. a self-declaration or a declaration of oath). The Information Requirement can require structured data or documents of any form. For structured data, the Requirement can use 'Concepts' to specify the structure and type of the data expected in the response. For both structured and unstructured data, the Information Requirement can indicate the expected Type of Evidence, its format, source, and other properties related to the Evidence."@en ;
    skos:prefLabel "Information requirement"@en .

cccev:PublicOrganisation a owl:Class ;
    rdfs:subClassOf org:Organization ;
    skos:definition "An Organisation that is defined as being part of the public sector by a legal framework at any level. Additional information: A body governed by public law: - (a) established for the specific Purpose of meeting needs in the general interest - (b) having legal personality; - (c) financed, for the most part by the State, or regional or local authorities. Examples of Public Organisations are municipality, international public body, ministry, others. WG Approval 28/04/2020"@en ;
    skos:prefLabel "Public organisation"@en .

cccev:bias a owl:DatatypeProperty ;
    skos:definition "Parameter used to adjust the evaluation of the Criterion. Additional Information: The bias parameter tries to correct a systematic error. For example in procurement, a home bias corresponds to the \"presence of local preferences distorting international specialisation and resource allocation\". When quantified, this systematic error can be removed. (cccev:Criterion)"@en ;
    skos:prefLabel "Bias"@en .

cccev:birthDate a owl:DatatypeProperty ;
    skos:definition "The point in time on which the Person was born. (person:Person)"@en ;
    skos:prefLabel "Birth date"@en .

cccev:confidentialityLevelType a owl:ObjectProperty ;
    skos:definition "Security classification assigned to an Evidence e.g. classified, sensitive, public. Additional Information: Classifications should be defined by an organisation/country as an outcome of a security assessment. (cccev:Evidence -> at-voc:access-rights (+cccev:confidentialityLevelType)) Security classification assigned to an Evidence e.g. classified, sensitive, public. Additional Information: Classifications should be defined by an organisation/country as an outcome of a security assessment. (epo-sub:Response -> at-voc:access-rights (+cccev:confidentialityLevelType))"@en ;
    skos:prefLabel "Confidentiality level type"@en .

cccev:constrains a owl:ObjectProperty ;
    skos:definition "Information Concept about which a Constraint expresses a limitation. Additional Information: Information Concepts are tools to make Requirements more machine processable: they allow to provide more detail about a Requirement. This way, Constraints can be made very precise, namely the limit that must be achieved, is a limit on the value for the associated Information Concept. For example, the Information Concept would be the age of a person and the Constraint would be the required age in the context of a specific evaluation. (cccev:Constraint -> cccev:InformationConcept (+cccev:constrains))"@en ;
    skos:prefLabel "Constrains"@en .

cccev:coordinates a owl:DatatypeProperty ;
    skos:definition "The coordinate list. (locn:Geometry)"@en ;
    skos:prefLabel "Coordinates"@en .

cccev:email a owl:DatatypeProperty ;
    skos:definition "The email of the Organisation. (cpov:ContactPoint)"@en ;
    skos:prefLabel "Email"@en .

cccev:hasConcept a owl:ObjectProperty ;
    skos:definition "Information Concept for which a value is expected by the Requirement. Additional Information: Information Concepts defined for specific Requirements also represent the basis for specifying the Supported Value an Evidence should provide. (cccev:Requirement -> cccev:InformationConcept (+cccev:hasConcept))"@en ;
    skos:prefLabel "Has concept"@en .

cccev:hasEvidenceTypeList a owl:ObjectProperty ;
    skos:definition "Evidence Type List that specifies the Evidence Types that are needed to meet the Requirement. Additional Information: One or several Lists of Evidence Types can support a Requirement. At least one of them must be satisfied by the response to the Requirement. (cccev:Requirement -> cccev:EvidenceTypeList (+cccev:hasEvidenceTypeList))"@en ;
    skos:prefLabel "Has evidence type list"@en .

cccev:hasRequirement a owl:ObjectProperty ;
    skos:definition "A more specific Requirement that is part of the Requirement. (cccev:Requirement -> cccev:Requirement (+cccev:hasRequirement))"@en ;
    skos:prefLabel "Has requirement"@en .

cccev:isDerivedFrom a owl:ObjectProperty ;
    skos:definition "Reference Framework on which the Requirement is based, such as a law or regulation. Additional Information: The relation between a parent Requirement and a sub-Requirement can be complex. Therefore, qualified relations (see hasQualifiedRelation) can be used to represent this relationship on its own and qualify it with additional information such as a date, a place. This is left to implementers. In the case where the purpose is to link the two Requirements without additional information, the simple relationship as proposed here can be directly used. (cccev:Requirement -> eli:LegalResource (+cccev:isDerivedFrom))"@en ;
    skos:prefLabel "Is derived from"@en .

cccev:latitude a owl:DatatypeProperty ;
    skos:definition "The latitude. (locn:Geometry)"@en ;
    skos:prefLabel "Latitude"@en .

cccev:longitude a owl:DatatypeProperty ;
    skos:definition "The longitude. (locn:Geometry)"@en ;
    skos:prefLabel "Longitude"@en .

cccev:providesValueFor a owl:ObjectProperty ;
    skos:definition "Information Concept for which the Supported Value provides a value. (cccev:SupportedValue -> cccev:InformationConcept (+cccev:providesValueFor))"@en ;
    skos:prefLabel "Provides value for"@en .

cccev:registeredAddress a owl:ObjectProperty ;
    skos:definition "The registered address relationship links a Resource with the legally registered Address. Additional Information: It is the address to which formal communications can be sent, such as the postal address. (person:Person -> locn:Address (+cv:registeredAddress)) The registered address relationship links a Resource with the legally registered Address. Additional Information: It is the address to which formal communications can be sent, such as the postal address. (org:Organization -> locn:Address (+cv:registeredAddress))"@en ;
    skos:prefLabel "Registered address"@en .

cccev:supportsConcept a owl:ObjectProperty ;
    skos:definition "Information Concept providing facts found/inferred from the Evidence. Additional Information: Examples of Information Concepts are values found explicitly in the evidence such as a birth date or information derived from the Evidence such as \"I am older that 18 years\" or \"this is a Fair Trade product\". (cccev:Evidence -> cccev:InformationConcept (+cccev:supportsConcept))"@en ;
    skos:prefLabel "Supports concept"@en .

cccev:supportsRequirement a owl:ObjectProperty ;
    skos:definition "Requirement for which the Evidence provides proof. (cccev:Evidence -> cccev:Requirement (+cccev:supportsRequirement))"@en ;
    skos:prefLabel "Supports requirement"@en .

cccev:supportsValue a owl:ObjectProperty ;
    skos:definition "Supported Value that the Evidence contains. (cccev:Evidence -> cccev:SupportedValue (+cccev:supportsValue))"@en ;
    skos:prefLabel "Supports value"@en .

cccev:telephone a owl:DatatypeProperty ;
    skos:definition "A telephone number through which the Contact Point can be contacted. (cpov:ContactPoint)"@en ;
    skos:prefLabel "Telephone"@en .

cccev:validityPeriodConstraint a owl:ObjectProperty ;
    skos:definition "Temporal condition on the validity period of the Evidence Type. Additional Information: E.g. A Belgian birth evidence is valid for X months after emission. To express constraints on the validity period that must hold when assessing the evidence (e.g. the certificate of good conduct cannot be issued more than 3 months ago), we refer to the Constraint class. (cccev:EvidenceType -> epo:Period (+cccev:validityPeriodConstraint))"@en ;
    skos:prefLabel "Validity period constraint"@en .

cccev:weight a owl:DatatypeProperty ;
    skos:definition "Relative importance of the Criterion. Additional Information: The weight must be between 0 and 1. Usually, all Criteria can be integrated within a weighted sum equal to 1. (cccev:Criterion)"@en ;
    skos:prefLabel "Weight"@en .

cccev:weightingConsiderationDescription a owl:DatatypeProperty ;
    skos:definition "Explanation of how the weighting of a Criterion is to be used. Additional Information: This description gives the view of the creator of the Criterion weights on how to interpret and use them during the evaluation process. (cccev:Criterion)"@en ;
    skos:prefLabel "Weighting consideration description"@en .

dcterms:Location a owl:Class ;
    skos:definition "An identifiable geographic place or named place."@en ;
    skos:prefLabel "Location"@en .

dcterms:alternative a owl:DatatypeProperty ;
    skos:definition "Any name by which an individual is known other than their full name. WG 09/11/2021 (person:Person)"@en ;
    skos:prefLabel "Alternative"@en .

dcterms:conformsTo a owl:ObjectProperty ;
    skos:definition "An established standard to which the described resource conforms. Additional Information: Examples of characteristics could be the layout or the configuration of the Evidence. (cccev:Evidence -> cccev:EvidenceType (+dct:conformsTo))"@en ;
    skos:prefLabel "Conforms to"@en .

dcterms:description a owl:DatatypeProperty ;
    skos:definition "An account of the resource. Additional Information: Description may include but is not limited to: an abstract, a table of contents, a graphical representation, or a free-text account of the resource. WG Approval 30/05/2023 (cccev:Evidence) An account of the resource. Additional Information: Description may include but is not limited to: an abstract, a table of contents, a graphical representation, or a free-text account of the resource. WG Approval 30/05/2023 (cccev:InformationConcept) An account of the resource. Additional Information: Description may include but is not limited to: an abstract, a table of contents, a graphical representation, or a free-text account of the resource. WG Approval 30/05/2023 (cccev:Requirement) An account of the resource. Additional Information: Description may include but is not limited to: an abstract, a table of contents, a graphical representation, or a free-text account of the resource. WG Approval 30/05/2023 (cpov:ContactPoint) An account of the resource. Additional Information: Description may include but is not limited to: an abstract, a table of contents, a graphical representation, or a free-text account of the resource. WG Approval 30/05/2023 (cv:Channel) An account of the resource. Additional Information: Description may include but is not limited to: an abstract, a table of contents, a graphical representation, or a free-text account of the resource. WG Approval 30/05/2023 (epo:AgentInRole) An account of the resource. Additional Information: Description may include but is not limited to: an abstract, a table of contents, a graphical representation, or a free-text account of the resource. WG Approval 30/05/2023 (epo:Document) An account of the resource. Additional Information: Description may include but is not limited to: an abstract, a table of contents, a graphical representation, or a free-text account of the resource. WG Approval 30/05/2023 (epo:ElectronicSignature) An account of the resource. Additional Information: Description may include but is not limited to: an abstract, a table of contents, a graphical representation, or a free-text account of the resource. WG Approval 30/05/2023 (epo:Fund) An account of the resource. Additional Information: Description may include but is not limited to: an abstract, a table of contents, a graphical representation, or a free-text account of the resource. WG Approval 30/05/2023 (epo:NonDisclosureAgreementTerm) An account of the resource. Additional Information: Description may include but is not limited to: an abstract, a table of contents, a graphical representation, or a free-text account of the resource. WG Approval 30/05/2023 (epo:SecurityClearanceTerm) An account of the resource. Additional Information: Description may include but is not limited to: an abstract, a table of contents, a graphical representation, or a free-text account of the resource. WG Approval 30/05/2023 (epo:SubcontractingEstimate) An account of the resource. Additional Information: Description may include but is not limited to: an abstract, a table of contents, a graphical representation, or a free-text account of the resource. WG Approval 30/05/2023 (epo:SubcontractTerm) An account of the resource. Additional Information: Description may include but is not limited to: an abstract, a table of contents, a graphical representation, or a free-text account of the resource. WG Approval 30/05/2023 (epo:System) An account of the resource. Additional Information: Description may include but is not limited to: an abstract, a table of contents, a graphical representation, or a free-text account of the resource. WG Approval 30/05/2023 (epo:Technique) An account of the resource. Additional Information: Description may include but is not limited to: an abstract, a table of contents, a graphical representation, or a free-text account of the resource. WG Approval 30/05/2023 (epo:LotGroup) An account of the resource. Additional Information: Description may include but is not limited to: an abstract, a table of contents, a graphical representation, or a free-text account of the resource. WG Approval 30/05/2023 (epo:ProcurementElement) An account of the resource. Additional Information: Description may include but is not limited to: an abstract, a table of contents, a graphical representation, or a free-text account of the resource. WG Approval 30/05/2023 (epo:TenderGroup)"@en ;
    skos:prefLabel "Description"@en .

dcterms:issued a owl:DatatypeProperty ;
    skos:definition "Date of formal issuance of the resource. Additional information: This is generally used for modules other than eNotice. The xsd:dateTime here means that we can provide either xsd:date, xsd:dateTime, or xsd:timeStamp or any other variant of time expression. This extension needs to be encoded/automated in the ontology and in the application profile. Why is it like this? Because UML cannot handle such expressions of disjunctive property ranges. WG approval 26/01/2023 (epo:Document)"@en ;
    skos:prefLabel "Issued"@en .

dcterms:language a owl:ObjectProperty ;
    skos:definition "A language of the resource. (eli:LegalExpression -> at-voc:language (+dct:language))"@en ;
    skos:prefLabel "Language"@en .

dcterms:title a owl:DatatypeProperty ;
    skos:definition "A name given to the resource. WG approval 30/05/2023 (epo:AgentInRole) A name given to the resource. WG approval 30/05/2023 (epo:Document) A name given to the resource. WG approval 30/05/2023 (epo:Fund) A name given to the resource. WG approval 30/05/2023 (foaf:Agent) A name given to the resource. WG approval 30/05/2023 (epo:LotGroup) A name given to the resource. WG approval 30/05/2023 (epo:ProcurementElement) A name given to the resource. WG approval 30/05/2023 (epo:TenderGroup)"@en ;
    skos:prefLabel "Title"@en .

dcterms:type a owl:ObjectProperty ;
    skos:definition "Category to which the Requirement belongs. (cccev:Criterion -> at-voc:criterion (+dct:type))"@en ;
    skos:prefLabel "Type"@en .

rdf:PlainLiteral a rdfs:Datatype ;
    skos:prefLabel "Plain literal"@en .

xsd:anyURI a rdfs:Datatype ;
    skos:prefLabel "Any u r i"@en .

xsd:boolean a rdfs:Datatype ;
    skos:prefLabel "Boolean"@en .

xsd:date a rdfs:Datatype ;
    skos:prefLabel "Date"@en .

xsd:dateTime a rdfs:Datatype ;
    skos:prefLabel "Date time"@en .

xsd:decimal a rdfs:Datatype ;
    skos:prefLabel "Decimal"@en .

xsd:integer a rdfs:Datatype ;
    skos:prefLabel "Integer"@en .

skos:notation a owl:DatatypeProperty ;
    skos:definition "The literal identifying an entity, like a person or an object. (adms:Identifier)"@en ;
    skos:prefLabel "Notation"@en .

skos:prefLabel a owl:DatatypeProperty ;
    skos:definition "The preferred lexical label for a resource, in a given language. WG approval 30/05/2023 (cccev:InformationConcept) The preferred lexical label for a resource, in a given language. WG approval 30/05/2023 (cccev:Requirement)"@en ;
    skos:prefLabel "Pref label"@en .

time:numericDuration a owl:DatatypeProperty ;
    skos:definition "Value of a temporal extent expressed as a number. (epo:SpecificDuration)"@en ;
    skos:prefLabel "Numeric duration"@en .

time:unitType a owl:ObjectProperty ;
    skos:prefLabel "Unit type"@en .

adms:Identifier a owl:Class ;
    skos:definition "A character string to identify and distinguish uniquely, one instance of an object in an identification scheme from all other objects in the same scheme together with relevant supplementary information."@en ;
    skos:prefLabel "Identifier"@en .

adms:identifier a owl:ObjectProperty ;
    skos:definition "Links a resource to an adms:Identifier class. (cccev:EvidenceType -> adms:Identifier (+adms:identifier)) Links a resource to an adms:Identifier class. (epo-ful:Consignment -> adms:Identifier (+adms:identifier)) Links a resource to an adms:Identifier class. (foaf:Agent -> adms:Identifier (+adms:identifier)) Links a resource to an adms:Identifier class. (epo:Document -> adms:Identifier (+adms:identifier)) Links a resource to an adms:Identifier class. (dct:Location -> adms:Identifier (+adms:identifier)) Links a resource to an adms:Identifier class. (cccev:Requirement -> adms:Identifier (+adms:identifier)) A unique identifier of the instance of the concept. Additional Information For example, in the case of the Procurement Identifier, this could be the European Public Procurement Identifier, and/or any other identifier provided by the buyer, the service provider or any other stakeholder. WG Approval 12/11/2019 (epo:LotGroup -> adms:Identifier (+adms:identifier)) A unique identifier of the instance of the concept. Additional Information For example, in the case of the Procurement Identifier, this could be the European Public Procurement Identifier, and/or any other identifier provided by the buyer, the service provider or any other stakeholder. WG Approval 12/11/2019 (epo:TenderGroup -> adms:Identifier (+adms:identifier)) Links a resource to an adms:Identifier class. (cccev:Evidence -> adms:Identifier (+adms:identifier)) A unique identifier of the instance of the concept. Additional Information For example, in the case of the Procurement Identifier, this could be the European Public Procurement Identifier, and/or any other identifier provided by the buyer, the service provider or any other stakeholder. WG Approval 12/11/2019 (epo:ProcurementElement -> adms:Identifier (+adms:identifier)) Links a resource to an adms:Identifier class. (cccev:EvidenceTypeList -> adms:Identifier (+adms:identifier)) Links a resource to an adms:Identifier class. (epo-ful:ShipmentInformation -> adms:Identifier (+adms:identifier)) Links a resource to an adms:Identifier class. (epo-cat:Line -> adms:Identifier (+adms:identifier)) Links a resource to an adms:Identifier class. (cccev:InformationConcept -> adms:Identifier (+adms:identifier)) Links a resource to an adms:Identifier class. (epo-ful:AbstractContainer -> adms:Identifier (+adms:identifier)) A unique identifier of the instance of the concept. Additional Information For example, in the case of the Procurement Identifier, this could be the European Public Procurement Identifier, and/or any other identifier provided by the buyer, the service provider or any other stakeholder. WG Approval 12/11/2019 (epo:Project -> adms:Identifier (+adms:identifier)) Links a resource to an adms:Identifier class. (epo:Fund -> adms:Identifier (+adms:identifier))"@en ;
    skos:prefLabel "Identifier"@en .

adms:schemaAgency a owl:DatatypeProperty ;
    skos:definition "The name of the agency that issued the identifier. (adms:Identifier)"@en ;
    skos:prefLabel "Schema agency"@en .

locn:Address a owl:Class ;
    skos:definition "The particulars of the place where a Person or an Organisation is located. WG Approval 28/04/2020 Additional Information: An \"Address Representation\" as conceptually defined by the INSPIRE Address Representation data type: \"Representation of an address spatial object for use in external application schemas that need to include the basic, address information in a readable way.\". The representation of Addresses varies widely from one country's postal System to another. Even within countries, there are almost always examples of Addresses that do not conform to the stated national standard. At the time of publication, work is progressing on ISO 19160-1 that defines a method through which different Addresses can be converted from one conceptual model to another. This specification was heavily based on the INSPIRE Address Representation data type. It is noteworthy that if an Address is provided using the detailed breakdown suggested by the properties for this class, then it will be INSPIRE-conformant. To this very granular set of properties, we add two further properties: - full address (the complete address as a formatted string) - addressID (a unique identifier for the address) The first of these allows publishers to simply provide the complete Address as one string, with or without formatting. This is analogous to vCard's label property. The addressID is part of the INSPIRE guidelines and provides a hook that can be used to link the Address to an alternative representation, such as vCard or OASIS xAL."@en ;
    skos:prefLabel "Address"@en .

locn:Geometry a owl:Class ;
    skos:definition "The Geometry class provides the means to identify a Location as a point, line, polygon, etc. expressed using coordinates in some coordinate reference System. Additional Information: This class defines the notion of \"Geometry\" at the conceptual level, and it shall be encoded by using different formats (see usage note of the locn:geometry property). We also refer to the Examples section of this specification for a number of different Geometry examples expressed in different formats."@en ;
    skos:prefLabel "Geometry"@en .

locn:address a owl:ObjectProperty ;
    skos:definition "Associates any Resource with the corresponding Address. Additional Information: Asserting the address relationship implies that the Resource has an Address. (cpov:ContactPoint -> locn:Address (+locn:address)) Associates any Resource with the corresponding Address. Additional Information: Asserting the address relationship implies that the Resource has an Address. (org:Organization -> locn:Address (+locn:address))"@en ;
    skos:prefLabel "Address"@en .

locn:addressArea a owl:DatatypeProperty ;
    skos:definition "The name or names of a geographic area or locality that groups a number of addressable objects for addressing purposes, without being an administrative unit. Additional Information: This would typically be part of a city, a neighbourhood or village, e.g. Montmartre. (locn:Address)"@en ;
    skos:prefLabel "Address area"@en .

locn:addressID a owl:ObjectProperty ;
    skos:definition "A globally unique identifier for each instance of an Address. Additional Information: The concept of adding a globally unique identifier for each instance of an address is a crucial part of the INSPIRE data spec. A number of EU countries have already implemented an ID (a UUID) in their Address Register/gazetteer, among them Denmark. OASIS xAL also includes an address identifier. It is the address Identifier that allows an address to be represented in a format other than INSPIRE whilst remaining conformant to the Core Vocabulary. The INSPIRE method of representing addresses is very detailed, designed primarily for use in databases of addresses. Whilst data that is published in full conformance with the INSPIRE data structure can be made available using the Location Core Vocabulary the reverse is not true since the Core Vocabulary allows much greater flexibility. Many datasets that include address data as one piece of information about something else are likely to have that data in simpler formats. These might be tailored to the specific need of the dataset, follow a national norm, or make use of a standard like vCard. To provide maximum flexibility in the Core Vocabulary, whilst remaining interoperable with INSPIRE Address Guidelines (which EU Member States are obliged to use), the Location Core Vocabulary provides the extra property of full address and makes use of INSPIRE's addressID. (locn:Address -> adms:Identifier (+locn:addressID))"@en ;
    skos:prefLabel "Address i d"@en .

locn:adminUnitL1 a owl:DatatypeProperty ;
    skos:definition "The name or names of a unit of administration related to the exercise of jurisdictional rights, for local, regional and national governance. Level 1 refers to the uppermost administrative unit for the address, almost always a country. Additional Information: Best practice is to use the ISO 3166-1 code but if this is inappropriate for the context, country names should be provided in a consistent manner to reduce ambiguity. For example, either write 'France' or 'FRA' consistently throughout the dataset and avoid mixing the two. The Country controlled vocabulary from the Publications Office can be reused for this. (locn:Address)"@en ;
    skos:prefLabel "Admin unit l1"@en .

locn:adminUnitL2 a owl:DatatypeProperty ;
    skos:definition "The name or names of a unit of administration related to the exercise of jurisdictional rights, for local, regional and national governance. Level 2 refers to the region of the address, usually a county, state or other such area that typically encompasses several localities. Additional Information: Some recommended codelists from the EU Publications Office include: Administrative Territorial Units (ATU), NUTS and Local Administrative Units (LAU). The first arrondissement of Paris is for example expressed as \"http://publications.europa.eu/resource/authority/atu/FRA_AR_PAR01\" in the ATU controlled vocabulary. (locn:Address)"@en ;
    skos:prefLabel "Admin unit l2"@en .

locn:fullAddress a owl:DatatypeProperty ;
    skos:definition "The complete address written as a formatted string. Additional Information: Use of this property is recommended as it will not suffer any misunderstandings that might arise through the breaking up of an address into its component parts. This property is analogous to vCard's label property but with two important differences: (1) formatting is not assumed so that, unlike vCard label, it may not be suitable to print this on an address label, (2) vCard's label property has a domain of vCard Address; the fullAddress property has no such restriction. An example of a full address is \"Champ de Mars, 5 Avenue Anatole France, 75007 Paris, France\". (locn:Address)"@en ;
    skos:prefLabel "Full address"@en .

locn:geographicIdentifier a owl:ObjectProperty ;
    skos:definition "A URI that identifies the Location. Additional Information: GeoNames.org provides stable, widely recognised identifiers for more than 10 million geographical names that can be used as links to further information. For example, http://sws.geonames.org/593116/ identifies the Lithuanian capital Vilnius. Unfortunately these URIs cannot easily be automatically deduced since the URI scheme uses simple numeric codes. Finding a GeoNames identifier for a Location is almost always a manual process. Where such identifiers are known or can be found, however, it is recommended that they be used. Where the Location Class is used to identify a country, if the geonames URI is not known, the recommendation is to use DBpedia URIs of the form http://dbpedia.org/resource/ISO_3166-1:XX where XX is the ISO 3166 two character code for the country. The EU's Publication Office diverges from ISO 3166-1 and uses EL and UK for Greece and the United Kingdom respectively. DBpedia sticks to the ISO codes and so the correct URIs for these countries are: - http://dbpedia.org/resource/ISO_3166-1:GR - http://dbpedia.org/resource/ISO_3166-1:GB even when the geographic name is given as EL or UK. The use of a URIs has added advantages: - it can be used by automated systems to look up additional data (linked data); - a triple store may store only one copy of the URI, whereas if a string is used, a copy of that string is always stored for each and every person in the database. Thus, in large data sets, the saving on memory capacity and the improvement in transmission efficiency can be substantial. (dct:Location -> adms:Identifier (+locn:geographicIdentifier))"@en ;
    skos:prefLabel "Geographic identifier"@en .

locn:geographicName a owl:DatatypeProperty ;
    skos:definition "A textual description for a Location. Additional Information: The INSPIRE Data Specification on Geographical Names provides a detailed model for describing a 'named place', including methods for providing multiple names in multiple scripts. This is beyond what is necessary for the Core Location Vocabulary but, importantly, the concept of a geographic name used here is consistent. A geographic name is a proper noun applied to a spatial object. Taking the example used in the INSPIRE document (page 15), the following are all valid geographic names for the Greek capital: - \"Aθnνa\"@gr-Grek (the Greek endonym written in the Greek script) - \"Ath&#237;na\"@gr-Latn (the standard Romanisation of the endonym) - \"Athens\"@en (the English language exonym) INSPIRE has a detailed (XML-based) method of providing metadata about a geographic name and in XML-data sets that may be the most appropriate method to follow. When using the Core Location Vocabulary in data sets that are not focussed on environmental/geographical data (the use case for INSPIRE), the Code datatype or a simple language identifier may be used to provide such metadata. The country codes defined in ISO 3166 may be used as geographic names and these are generally preferred over either the long form or short form of a country's name (as they are less error prone). The Publications Office of the European Union recommends the use of ISO 3166-1 codes for countries in all cases except two: - use 'UK' in preference to the ISO 3166 code GB for the United Kingdom; - use 'EL' in preference to the ISO 3166 code GR for Greece. Where a country has changed its name or no longer exists (such as Czechoslovakia, Yugoslavia etc.) use the ISO 3166-3 code. (dct:Location)"@en ;
    skos:prefLabel "Geographic name"@en .

locn:geometry a owl:ObjectProperty ;
    skos:prefLabel "Geometry"@en .

locn:locatorDesignator a owl:DatatypeProperty ;
    skos:definition "A number or a sequence of characters which allows a user or an application to interpret, parse and format the locator within the relevant scope. A locator may include more locator designators. Additional Information: In simpler terms, this is the building number, apartment number, etc. For an address such as \"Flat 3, 17 Bridge Street\", the locator is \"flat 3, 17\". (locn:Address)"@en ;
    skos:prefLabel "Locator designator"@en .

locn:locatorName a owl:DatatypeProperty ;
    skos:definition "Proper noun(s) applied to the real world entity identified by the locator. Additional Information: The locator name could be the name of the property or complex, of the building or part of the building, or it could be the name of a room inside a building. The key difference between a locator and a locator name is that the latter is a proper name and is unlikely to include digits. For example, \"Shumann, Berlaymont\" is a meeting room within the European Commission headquarters for which locator name is more appropriate than locator. (locn:Address)"@en ;
    skos:prefLabel "Locator name"@en .

locn:postCode a owl:DatatypeProperty ;
    skos:definition "The post/zip code of an address. (INSPIRE's definition is \"A code created and maintained for postal purposes to identify a subdivision of addresses and postal delivery points.\") Additional Information: Post codes are common elements in many countries' postal address systems. One of the many post codes of Paris is for example \"75000\". (locn:Address)"@en ;
    skos:prefLabel "Post code"@en .

locn:postName a owl:DatatypeProperty ;
    skos:definition "The key postal division of the address, usually the city. (INSPIRE's definition is \"One or more names created and maintained for postal purposes to identify a subdivision of addresses and postal delivery points.) For example, \"Paris\". (locn:Address)"@en ;
    skos:prefLabel "Post name"@en .

locn:thoroughfare a owl:DatatypeProperty ;
    skos:definition "An address component that represents the name or names of a passage or way through from one location to another. A thoroughfare is not necessarily a road, it might be a waterway or some other feature. Additional Information: For example, \"Avenue des Champs-&#201;lys&#233;es\". (locn:Address)"@en ;
    skos:prefLabel "Thoroughfare"@en .

org:subOrganizationOf a owl:ObjectProperty ;
    skos:definition "Represents hierarchical containment of Organizations or OrganizationalUnits; indicates an Organization which contains this Organization. WG 31/08/2023 (org:Organization -> org:Organization (+org:subOrganizationOf))"@en ;
    skos:prefLabel "Sub organization of"@en .

person:Person a owl:Class ;
    rdfs:subClassOf foaf:Person ;
    skos:definition "A individual human being who may be dead or alive, but not imaginary."@en ;
    skos:prefLabel "Person"@en .

person:birthName a owl:DatatypeProperty ;
    skos:definition "Family name of the Person given upon their birth. WG Approval 09/11/2021 (person:Person)"@en ;
    skos:prefLabel "Birth name"@en .

person:patronymicName a owl:DatatypeProperty ;
    skos:definition "Name based on the given name of the Person's father. WG Approval 09/11/2021 (person:Person)"@en ;
    skos:prefLabel "Patronymic name"@en .

foaf:familyName a owl:DatatypeProperty ;
    skos:definition "The hereditary surname of a family. (person:Person)"@en ;
    skos:prefLabel "Family name"@en .

foaf:givenName a owl:DatatypeProperty ;
    skos:definition "The name(s) that identify the Person within a family with a common surname. (person:Person)"@en ;
    skos:prefLabel "Given name"@en .

foaf:name a owl:DatatypeProperty ;
    skos:definition "The complete name of the Person as one string. (person:Person)"@en ;
    skos:prefLabel "Name"@en .

cccev:Channel a owl:Class ;
    skos:definition "A medium through which Agents interact. Additional Information Typical examples include online services, email, endpoint on eDelivery infrastructure, phone, etc. Software solutions and electronic devices for communication and exchange of information between Buyers and economic Operators. Lots may use ad-hoc electronic means of communication that are not generally available such as specific solutions for secure and dedicated communication or non-standard eCatalogues. See also Directive recitals 53 to 56. WG approval 2023-02-14"@en ;
    skos:prefLabel "Channel"@en .

cccev:Criterion a owl:Class ;
    rdfs:subClassOf cccev:Requirement ;
    skos:definition "Condition for evaluation or assessment. Additional Information: In general, Criteria are used for comparison, filtering or Selection purposes. Criteria usually set minimum conditions (e.g. limits, intervals, thresholds, etc.) that need to be met in order to pass the Requirements or to fulfil them to a certain degree or quality. The concept of Criteria is broader than the concept of Constraint since it covers more usages. The evaluation of the fulfilment is usually supported by the provision of Evidence. For example in the eProcurement domain, the eProcurement Ontology defines different subclasses of Criterion such as Exclusion Grounds, Selection Criteria or Award Criteria. A concrete example of a Criterion is 'participation in a criminal organisation' which could also be considered as an Exclusion Ground Criterion in the procurement domain or for requiring a public service."@en ;
    skos:prefLabel "Criterion"@en .

cccev:Evidence a owl:Class ;
    skos:definition "Proof that a Requirement is met. Additional Information: The class Evidence provides the means to support responses to Criteria or to a concrete Information Requirement or to an Information Concept inside an Information Requirement. The proof described by an Evidence can [1] verify a claim (i.e. is it true that John is 25, yes/no), [2] prove a condition (i.e. is John 18+, yes/no), or [3] simply provide data (i.e. the age of a person, namely 25). The proof can be given through documents or extracts of base registries, independently from its structure, format or medium used to exchange it: a pdf document, a video, a recording, etc."@en ;
    skos:prefLabel "Evidence"@en .

cccev:InformationConcept a owl:Class ;
    skos:definition "Piece of information that the Evidence provides or the Requirement needs. Additional Information: The Information Concept class offers the ability to describe conceptually the Requirements and provided facts in Evidences. In complementarity with the Supported Value class, this is a (first) step towards facilitating the assessment of the requirements in an automated way based on the Evidence provided."@en ;
    skos:prefLabel "Information concept"@en .

time:Duration a owl:Class ;
    skos:definition "Duration of a temporal extent expressed as a number scaled by a temporal unit."@en ;
    skos:prefLabel "Duration"@en .

foaf:Person a owl:Class ;
    rdfs:subClassOf foaf:Agent ;
    skos:definition "The Person class represents people. Something is a Person if it is a Person. We don't nitpick about whether they're alive, dead, real, or imaginary. The Person class is a sub-class of the Agent class, since all people are considered 'Agents' in FOAF."@en ;
    skos:prefLabel "Person"@en .

:AwardOutcome a owl:Class ;
    rdfs:isDefinedBy :core ;
    rdfs:subClassOf :ContextualProjection ;
    skos:definition "Result concerning the competition that was attributed by the Awarder. WG approval 19/03/2024"@en ;
    skos:prefLabel "Award outcome"@en .

:Buyer a owl:Class ;
    rdfs:isDefinedBy :core ;
    rdfs:subClassOf :AcquiringParty ;
    skos:definition "A Role of an Agent that awards a Contract and/or purchases items. Additional information: In Public Procurement the Role of Buyer is carried out by the following types of Organisation: Contracting Authority, Contracting Entity, a defense Contractor, an international Organisation, or an organisation awarding a Contract subsidized by a Contracting Authority. In Pre-Award, the Buyer generally awards the Contract, however future purchasers may be foreseen. In Post-Award the buyer generally refers to the purchaser of items."@en ;
    skos:prefLabel "Buyer"@en .

:CentralPurchasingBody a owl:Class ;
    rdfs:isDefinedBy :core ;
    rdfs:subClassOf :Buyer ;
    skos:definition "Role of an Agent that provides centralised purchasing activities and, possibly, ancillary purchasing activities for other Buyers. Additional Information: In Public Procurement the Role of Central Purchasing Body is carried out by a Contracting Authority for other Contracting Authorities. Contracting Authority procuring activities conducted on a permanent basis, in one of the following forms:[...](b) the award of Public Contracts or the conclusion of Framework Agreements for works, supplies or services intended for Contracting Authorities; WG approval 05/08/2021"@en ;
    skos:prefLabel "Central purchasing body"@en .

:ContextualProjection a owl:Class ;
    rdfs:isDefinedBy :core ;
    skos:definition "Projection of an Entity and all of its properties that hold in a given Situation Context. Additional Information: The contextual projection does not have its own identity (-I), is dependent (+D) on the described Entity, and is anti-rigid (~R) We say that ContextualProjection *describes* an Entity. Adaptation of ContextSlices pattern encoding a 4D view. http://ontologydesignpatterns.org/wiki/Submissions:Context_Slices"@en ;
    skos:prefLabel "Contextual projection"@en .

:Duration a owl:Class ;
    rdfs:isDefinedBy :core ;
    rdfs:subClassOf time:Duration ;
    skos:definition "The length of time in which a concept occurs."@en ;
    skos:prefLabel "Duration"@en .

:Estimate a owl:Class ;
    rdfs:isDefinedBy :core ;
    rdfs:subClassOf :ContextDescription ;
    skos:definition "An approximate calculation or a judgement of the value, number, Quantity or extent of something."@en ;
    skos:prefLabel "Estimate"@en .

:EvaluationTerm a owl:Class ;
    rdfs:isDefinedBy :core ;
    rdfs:subClassOf :LotSpecificTerm ;
    skos:definition "Conditions and stipulations defining particularities of the Tender evaluation. (WG approval 23/11/2018)"@en ;
    skos:prefLabel "Evaluation term"@en .

:ProcurementElement a owl:Class ;
    rdfs:isDefinedBy :core ;
    skos:definition "Gathering class for critical/central elements in the Procurement Process. TODO: add definition Additional information: Alias: ProcurementComponent"@en ;
    skos:prefLabel "Procurement element"@en .

:ProcurementObject a owl:Class ;
    rdfs:isDefinedBy :core ;
    rdfs:subClassOf :ProcurementElement ;
    skos:definition "The whole or a division of goods, services or works to be procured. Additional Information: Anything that can specify the procurement content (i.e. goods, services, work) is a Procurement Object. In a sense, such an \"object\" can constitute the \"object of a Contract\". To test whether something is a Procedure Object check if it can have a Purpose and/or CPV classification (<i>The CPV establishes a single classification system for public procurement aimed at standardising the references used by Contracting Authorities and entities to describe the subject of Procurement Contracts.</i>). Note: Procedure, seems to be an exception from this rule. Because it is a conflated term: it carries process properties and \"purpose\" properties."@en ;
    skos:prefLabel "Procurement object"@en .

:QualificationCriteriaSummary a owl:Class ;
    rdfs:isDefinedBy :core ;
    rdfs:subClassOf :ProcurementCriteriaSummary ;
    skos:definition "Overview of the Qualification Criteria. WG approval 19/03/2024"@en ;
    skos:prefLabel "Qualification criteria summary"@en .

:QualificationCriterion a owl:Class ;
    rdfs:isDefinedBy :core ;
    rdfs:subClassOf :ProcurementCriterion ;
    skos:definition "Criterion used in the first stage of procurement. WG approval 30/05/2023"@en ;
    skos:prefLabel "Qualification criterion"@en .

:ReviewObject a owl:Class ;
    rdfs:isDefinedBy :core ;
    rdfs:subClassOf :Document ;
    skos:definition "Information about a Review Request or a Review Decision. Additional information: This class corresponds to the BG-714 Review in eForms."@en ;
    skos:prefLabel "Review object"@en .

:isSubjectToTerm a owl:ObjectProperty ;
    rdfs:isDefinedBy :core ;
    skos:prefLabel "Is subject to term"@en .

:AgentInRole a owl:Class ;
    rdfs:isDefinedBy :core ;
    skos:definition "Relative concept that ties an Agent to a part they play in a given Situational Context. Additional information: The classification of roles is based is based on the degree of involvement into the Procurement Process: - Primary (Procurement) Pole is directly involved in the Procurement Process; - Secondary (Procurement sub-) Role is secondary to the Procurement Process - Tertiary (Related) Role is not involved in the Procurement Process."@en ;
    skos:prefLabel "Agent in role"@en .

:ContractSpecificTerm a owl:Class ;
    rdfs:isDefinedBy :core ;
    rdfs:subClassOf :Term ;
    skos:definition "Gathering class for conditions and stipulations related to a contract in the Post-Award Phase."@en ;
    skos:prefLabel "Contract specific term"@en .

:ProcurementCriteriaSummary a owl:Class ;
    rdfs:isDefinedBy :core ;
    rdfs:subClassOf cccev:Requirement ;
    skos:definition "Overview of the Procurement Criteria. WG approval 19/03/2024"@en ;
    skos:prefLabel "Procurement criteria summary"@en .

:ProcurementCriterion a owl:Class ;
    rdfs:isDefinedBy :core ;
    rdfs:subClassOf cccev:Criterion ;
    skos:definition "A criterion specific to Procurement. Additional Information: This Procurement Criterion can be only Exclusion Ground, Selection Criterion or Award Criterion. Each of these Criteria can contain subcriteria (Criterion class). WG Approval 23/04/2020"@en ;
    skos:prefLabel "Procurement criterion"@en .

:SelectionCriteriaSummary a owl:Class ;
    rdfs:isDefinedBy :core ;
    rdfs:subClassOf :QualificationCriteriaSummary ;
    skos:definition "Overview of the Selection Criteria. WG approval 19/03/2024"@en ;
    skos:prefLabel "Selection criteria summary"@en .

:StatisticalInformation a owl:Class ;
    rdfs:isDefinedBy :core ;
    rdfs:subClassOf :ContextDescription ;
    skos:definition "Statistical data on the Procedure and the Lot. Additional Information At the present time Procurement Procedures are not fully electronic. At a later date, information on the Tenders received could be inferred by the data in the eProcurement System. Therefore this class is temporal and should cease to exist in fully electronic Procurement. The need for its presence responds also to the alignment with the Regulation (EU) 2019/1780 (eForms). Attention will have to be paid in the future to possible inconsistencies derived from data placed in other classes and data held in the Statistical Information class; e.g. the TenderEvaluation class (see eEvaluation diagram) has the attribute admissibileTender indicator, which in case of being false, may enter in contradiction with the highest or lowest Tender value for that very same inadmissible Tender. WG Approval 12/12/2019"@en ;
    skos:prefLabel "Statistical information"@en .

:StrategicProcurement a owl:Class ;
    rdfs:isDefinedBy :core ;
    skos:definition "Public Procurement that contributes to achieving pressing policy goals. Additional Information: Specific strategic goals could be, for example, Environmental Protection, innovation, job creation and the development of small and medium enterprises. This corresponds in eForms to BG-713 Strategic Procurement. The subclasses are given by the choices in BT-06 Strategic Procurement. Based on https://legalinstruments.oecd.org/en/instruments/OECD-LEGAL-0411 (see paragraph on \"background information\". WG Approval 10/03/2020"@en ;
    skos:prefLabel "Strategic procurement"@en .

:Technique a owl:Class ;
    rdfs:isDefinedBy :core ;
    skos:definition "Method used for conducting Procurement Procedures. Addtional information: This corresponds in eForms to BG-706 Techniques. Several Techniques can be combined in one single Procurement Procedure (e.g. eAuction can be carried out in a Framework Agreement or DPS). WG Approval 19/09/2019"@en ;
    skos:prefLabel "Technique"@en .

org:Organization a owl:Class ;
    rdfs:subClassOf foaf:Agent ;
    skos:definition "A collection of people organized together into a community or other social, commercial or political structure. The group has some common purpose or reason for existence which goes beyond the set of people belonging to it and can act as an Agent. Organisations are often decomposable into hierarchical structures. (WG approval 23/11/2018)."@en ;
    skos:prefLabel "Organization"@en .

foaf:Agent a owl:Class ;
    skos:definition "A Person, an Organisation, or a System that acts in Procurement or have the power to act in Procurement. WG Approval 28/04/2020"@en ;
    skos:prefLabel "Agent"@en .

:Contract a owl:Class ;
    rdfs:isDefinedBy :core ;
    rdfs:subClassOf :Document ;
    skos:definition "A voluntary, deliberate, and legally binding agreement between two or more competent parties. WG approval 19/03/2024"@en ;
    skos:prefLabel "Contract"@en .

:Term a owl:Class ;
    rdfs:isDefinedBy :core ;
    skos:definition "A governing condition or stipulation."@en ;
    skos:prefLabel "Term"@en .

cccev:Requirement a owl:Class ;
    skos:definition "Condition or prerequisite that is to be proven by Evidence. Additional Information: Requirement is a generic class representing any type of prerequisite that may be desired, needed or imposed as an obligation. CCCEV recommends to not use the Requirement class directly, but rather a more semantically-enriched subclass such as Criterion, Information Requirement or Constraint. Also note that the Requirement class is specified at a more abstract level and is not to be used as the instantiation of a Requirement for a specific Agent. To illustrate the notion: the European Directive on services in the internal market defines requirement as any obligation, prohibition, condition or limit provided for in the laws, regulations or administrative provisions of the Member States or in consequence of case-law, administrative practice, the rules of professional bodies, or the collective rules of professional associations or other professional Organisations, adopted in the exercise of their legal autonomy. To stay consistent to how identification is realised in the eProcurement ontology, we switch to using `adms:identifier` instead of `dct:identifier` as per CCCEV specification."@en ;
    skos:prefLabel "Requirement"@en .

:ContextDescription a owl:Class ;
    rdfs:isDefinedBy :core ;
    skos:definition "A description concerning a Procurement Object or a Notice in a specific Situation Context. Additional Information: The description has its own identity (+I) but is dependent (+D) on the concerned Entity. We say that ContextDescription *concerns* an Entity."@en ;
    skos:prefLabel "Context description"@en .

:ProcedureSpecificTerm a owl:Class ;
    rdfs:isDefinedBy :core ;
    rdfs:subClassOf :Term ;
    skos:definition "Gathering class for conditions and stipulations related to a Procedure."@en ;
    skos:prefLabel "Procedure specific term"@en .

:OfferingParty a owl:Class ;
    rdfs:isDefinedBy :core ;
    rdfs:subClassOf :AgentInRole ;
    skos:definition "The Role of an Agent that acts on the Economic Operator side during a Procurement Process. Additional information: As per the European Procurement Directives the notion of ‘Economic Operators’ should be interpreted in a broad manner so as to include any Persons and/or Entities which offer the execution of works, the supply of products or the provision of services on the market, irrespective of the legal form under which they have chosen to operate. Thus, firms, branches, subsidiaries, partnerships, cooperative societies, limited companies, universities, public or private, and other forms of entities than natural Persons should all fall within the notion of Economic Operator, whether or not they are ‘Legal Persons’ in all circumstances."@en ;
    skos:prefLabel "Offering party"@en .

:Document a owl:Class ;
    rdfs:isDefinedBy :core ;
    skos:definition "A set of interrelated Business Information representing the Business facts and associated metadata. The information may be conveyed in any language, medium or form, including textual, numerical, graphic, cartographic, audio-visual forms, etc. WG Approval 23/05/2019"@en ;
    skos:prefLabel "Document"@en .

:LotSpecificTerm a owl:Class ;
    rdfs:isDefinedBy :core ;
    rdfs:subClassOf :Term ;
    skos:definition "Gathering class for conditions and stipulations related to a Lot."@en ;
    skos:prefLabel "Lot specific term"@en .

:AcquiringParty a owl:Class ;
    rdfs:isDefinedBy :core ;
    rdfs:subClassOf :AgentInRole ;
    skos:definition "The Role of an Agent that acts on the buying side of a Procurement Process."@en ;
    skos:prefLabel "Acquiring party"@en .

:core a owl:Ontology ;
    rdfs:label "eProcurement Ontology - core"@en ;
    dcterms:created "2021-06-01"^^xsd:date ;
    dcterms:description "The eProcurement Ontology core describes the concepts and properties representing the European Public Procurement domain. The provision of these semantics offers the basis for a common understanding of the domain for all stakeholders ensuring the quality of data exchange and transparency. The ontology restrictions are published in a separate artefact."@en ;
    dcterms:issued "2024-07-23"^^xsd:date ;
    dcterms:license "© European Union, 2014. Unless otherwise noted, the reuse of the Ontology is authorised under the European Union Public Licence v1.2 (https://eupl.eu/)." ;
    dcterms:publisher "http://publications.europa.eu/resource/authority/corporate-body/PUBL" ;
    dcterms:title "eProcurement Ontology - core"@en ;
    vann:preferredNamespacePrefix "epo" ;
    vann:preferredNamespaceUri "http://data.europa.eu/a4g/ontology#" ;
    rdfs:comment "This version is automatically generated from ePO_core.xml on 2024-07-23" ;
    rdfs:seeAlso <https://docs.ted.europa.eu/home/index.html>,
        <https://github.com/OP-TED/ePO/releases>,
        <https://joinup.ec.europa.eu/collection/eprocurement/solution/eprocurement-ontology/about>,
        <https://op.europa.eu/en/web/eu-vocabularies/e-procurement> ;
    owl:imports eli:,
        cccev:,
        frbroo:,
        dcterms:,
        vann:,
        <http://www.w3.org/2004/02/skos/core>,
        <http://www.w3.org/2006/time>,
        <http://www.w3.org/ns/adms>,
        <http://www.w3.org/ns/locn>,
        org:,
        <http://www.w3.org/ns/person>,
        foaf: ;
    owl:incompatibleWith "3.1.0" ;
    owl:priorVersion "http://data.europa.eu/a4g/ontology#core-4.1.0" ;
    owl:versionIRI :core-4.2.0 ;
    owl:versionInfo "4.2.0" .

