<?xml version="1.0" encoding="UTF-8"?>
<rdf:RDF xmlns="http://data.europa.eu/a4g/ontology#"
         xmlns:cc="http://creativecommons.org/ns#"
         xmlns:dc="http://www.omg.org/spec/UML/20131001/UMLDC"
         xmlns:dct="http://purl.org/dc/terms/"
         xmlns:epo="http://data.europa.eu/a4g/ontology#"
         xmlns:epor="http://data.europa.eu/a4g/rule#"
         xmlns:epos="http://data.europa.eu/a4g/shape#"
         xmlns:foaf="http://xmlns.com/foaf/0.1/"
         xmlns:org="http://www.w3.org/ns/org#"
         xmlns:owl="http://www.w3.org/2002/07/owl#"
         xmlns:rdf="http://www.w3.org/1999/02/22-rdf-syntax-ns#"
         xmlns:rdfs="http://www.w3.org/2000/01/rdf-schema#"
         xmlns:skos="http://www.w3.org/2004/02/skos/core#"
         xmlns:vann="http://purl.org/vocab/vann/"
         xml:base="http://data.europa.eu/a4g/ontology">
   <owl:Ontology rdf:about="http://data.europa.eu/a4g/ontology">
      <owl:imports rdf:resource="http://purl.org/dc/terms/"/>
      <owl:imports rdf:resource="http://www.w3.org/2004/02/skos/core"/>
      <dct:description xml:lang="en">
        This module provides the definitions for the core eProcurement ontology.
        
        Procurement data has been identified as data with a
        high-reuse potential. Given the increasing importance of data standards for
        eProcurement, a number of initiatives driven by the public sector, the industry and
        academia have been kick-started in recent years. Some have grown organically, while
        others are the result of standardisation work. The vocabularies and the semantics that
        they are introducing, the phases of public procurement that they are covering, and the
        technologies that they are using all differ. These differences hamper data
        interoperability and thus its reuse by them or by the wider public. This creates the
        need for a common data standard for publishing procurement data, hence allowing data
        from different sources to be easily accessed and linked, and consequently
        reused.</dct:description>
      <vann:preferredNamespacePrefix>epo</vann:preferredNamespacePrefix>
      <vann:preferredNamespaceUri>http://data.europa.eu/a4g/ontology#</vann:preferredNamespaceUri>
      <dct:license rdf:resource="http://creativecommons.org/licenses/by-sa/4.0/"/>
      <rdfs:label xml:lang="en">eProcurement core ontology</rdfs:label>
      <dct:title xml:lang="en">eProcurement core ontology</dct:title>
      <owl:versionIRI rdf:resource="http://data.europa.eu/a4g/ontology#ePO_CM.xml-2022-01-03"/>
      <owl:versionInfo>eProcurement core ontology version generated automatically from 
                ePO_CM.xml on 03/01/2022</owl:versionInfo>
      <rdfs:seeAlso rdf:resource="https://op.europa.eu/en/web/eu-vocabularies/e-procurement"/>
      <rdfs:seeAlso rdf:resource="https://joinup.ec.europa.eu/solution/eprocurement-ontology/about"/>
      <rdfs:seeAlso rdf:resource="https://github.com/eprocurementontology/eprocurementontology"/>
      <cc:attributionName>PublicationsOffice of the European Union</cc:attributionName>
      <cc:attributionURL rdf:resource="http://publications.europa.eu/resource/authority/corporate-body/PUBL"/>
      <dct:date rdf:datatype="http://www.w3.org/2001/XMLSchema#date">2022-01-03Z</dct:date>
   </owl:Ontology>
   <owl:Class rdf:about="http://purl.org/dc/terms/Location">
      <rdfs:label xml:lang="en">Location</rdfs:label>
      <skos:prefLabel xml:lang="en">Location</skos:prefLabel>
      <rdfs:comment xml:lang="en">An identifiable geographic place or named place.</rdfs:comment>
      <skos:definition xml:lang="en">An identifiable geographic place or named place.</skos:definition>
   </owl:Class>
   <owl:Class rdf:about="http://data.europa.eu/a4g/ontology#AccessTerm">
      <rdfs:label xml:lang="en">Access term</rdfs:label>
      <skos:prefLabel xml:lang="en">Access term</skos:prefLabel>
      <rdfs:comment xml:lang="en">Conditions and stipulations about where and how to access the procurement documents.

WG Approval 09/03/2021

</rdfs:comment>
      <skos:definition xml:lang="en">Conditions and stipulations about where and how to access the procurement documents.

WG Approval 09/03/2021

</skos:definition>
      <rdfs:isDefinedBy rdf:resource="http://data.europa.eu/a4g/ontology"/>
   </owl:Class>
   <owl:Class rdf:about="http://data.europa.eu/a4g/ontology#AcquiringCentralPurchasingBody">
      <rdfs:label xml:lang="en">Acquiring central purchasing body</rdfs:label>
      <skos:prefLabel xml:lang="en">Acquiring central purchasing body</skos:prefLabel>
      <rdfs:comment xml:lang="en">Role of an agent procuring activities conducted on a permanent basis in the form of the acquisition of supplies and/or services intended for other buyers.
Additional Information:
In public procurement the role of Acquiring Central purchasing body is carried out by a Central Purchasing Body for other Contracting Authorities.

WG approval 05/08/2021
</rdfs:comment>
      <skos:definition xml:lang="en">Role of an agent procuring activities conducted on a permanent basis in the form of the acquisition of supplies and/or services intended for other buyers.
Additional Information:
In public procurement the role of Acquiring Central purchasing body is carried out by a Central Purchasing Body for other Contracting Authorities.

WG approval 05/08/2021
</skos:definition>
      <rdfs:isDefinedBy rdf:resource="http://data.europa.eu/a4g/ontology"/>
   </owl:Class>
   <owl:Class rdf:about="http://data.europa.eu/a4g/ontology#Agent">
      <rdfs:label xml:lang="en">Agent</rdfs:label>
      <skos:prefLabel xml:lang="en">Agent</skos:prefLabel>
      <rdfs:comment xml:lang="en">A  person, an organization, or a system that act in procurement or have the power to act in procurement.

WG Approval 28/04/2020</rdfs:comment>
      <skos:definition xml:lang="en">A  person, an organization, or a system that act in procurement or have the power to act in procurement.

WG Approval 28/04/2020</skos:definition>
      <rdfs:isDefinedBy rdf:resource="http://data.europa.eu/a4g/ontology"/>
   </owl:Class>
   <owl:Class rdf:about="http://data.europa.eu/a4g/ontology#AwardCriterion">
      <rdfs:label xml:lang="en">Award criterion</rdfs:label>
      <skos:prefLabel xml:lang="en">Award criterion</skos:prefLabel>
      <rdfs:comment xml:lang="en">Describes a requirement that the tender needs to resolve and on which the tender is evaluated and ranked.

(WG approval 05/11/2018)</rdfs:comment>
      <skos:definition xml:lang="en">Describes a requirement that the tender needs to resolve and on which the tender is evaluated and ranked.

(WG approval 05/11/2018)</skos:definition>
      <rdfs:isDefinedBy rdf:resource="http://data.europa.eu/a4g/ontology"/>
   </owl:Class>
   <owl:Class rdf:about="http://data.europa.eu/a4g/ontology#AwardDecision">
      <rdfs:label xml:lang="en">Award decision</rdfs:label>
      <skos:prefLabel xml:lang="en">Award decision</skos:prefLabel>
      <rdfs:comment xml:lang="en">Resolution of the buyer as to the result of the procurement procedure.

(WG approval 14/11/2018)</rdfs:comment>
      <skos:definition xml:lang="en">Resolution of the buyer as to the result of the procurement procedure.

(WG approval 14/11/2018)</skos:definition>
      <rdfs:isDefinedBy rdf:resource="http://data.europa.eu/a4g/ontology"/>
   </owl:Class>
   <owl:Class rdf:about="http://data.europa.eu/a4g/ontology#AwardingCentralPurchasingBody">
      <rdfs:label xml:lang="en">Awarding central purchasing body</rdfs:label>
      <skos:prefLabel xml:lang="en">Awarding central purchasing body</skos:prefLabel>
      <rdfs:comment xml:lang="en">Role of an agent procuring activities conducted on a permanent basis in the form of the award of public contracts or the conclusion of framework agreements for works, supplies or services intended for other buyers.
Additional Information:
In public procurement the role of Awarding Central purchasing body is carried out by a Central Purchasing Body for other Contracting Authorities.

WG approval 05/08/2021
</rdfs:comment>
      <skos:definition xml:lang="en">Role of an agent procuring activities conducted on a permanent basis in the form of the award of public contracts or the conclusion of framework agreements for works, supplies or services intended for other buyers.
Additional Information:
In public procurement the role of Awarding Central purchasing body is carried out by a Central Purchasing Body for other Contracting Authorities.

WG approval 05/08/2021
</skos:definition>
      <rdfs:isDefinedBy rdf:resource="http://data.europa.eu/a4g/ontology"/>
   </owl:Class>
   <owl:Class rdf:about="http://data.europa.eu/a4g/ontology#Business">
      <rdfs:label xml:lang="en">Business</rdfs:label>
      <skos:prefLabel xml:lang="en">Business</skos:prefLabel>
      <rdfs:comment xml:lang="en">A private law company registered in a national registry.

WG Approval 28/04/2020

</rdfs:comment>
      <skos:definition xml:lang="en">A private law company registered in a national registry.

WG Approval 28/04/2020

</skos:definition>
      <rdfs:isDefinedBy rdf:resource="http://data.europa.eu/a4g/ontology"/>
   </owl:Class>
   <owl:Class rdf:about="http://data.europa.eu/a4g/ontology#Buyer">
      <rdfs:label xml:lang="en">Buyer</rdfs:label>
      <skos:prefLabel xml:lang="en">Buyer</skos:prefLabel>
      <rdfs:comment xml:lang="en">A role of an agent that awards a contract and/or purchases items.

Additional information:
In public procurement the role of buyer is carried out by the following types of organisation contracting authority, contracting entity, a defence contractor, an international organisation, or an organisation awarding a contract subsidized by a contracting authority.
In pre-award, the buyer generally awards the contract, however future purchasers may be foreseen.
In post-award the buyer generally refers to the purchaser of items.</rdfs:comment>
      <skos:definition xml:lang="en">A role of an agent that awards a contract and/or purchases items.

Additional information:
In public procurement the role of buyer is carried out by the following types of organisation contracting authority, contracting entity, a defence contractor, an international organisation, or an organisation awarding a contract subsidized by a contracting authority.
In pre-award, the buyer generally awards the contract, however future purchasers may be foreseen.
In post-award the buyer generally refers to the purchaser of items.</skos:definition>
      <rdfs:isDefinedBy rdf:resource="http://data.europa.eu/a4g/ontology"/>
   </owl:Class>
   <owl:Class rdf:about="http://data.europa.eu/a4g/ontology#BuyerProfile">
      <rdfs:label xml:lang="en">Buyer profile</rdfs:label>
      <skos:prefLabel xml:lang="en">Buyer profile</skos:prefLabel>
      <rdfs:comment xml:lang="en">Website address where the buyer publishes information on its procurement procedures and general information.

WG approval 04/05/2018
</rdfs:comment>
      <skos:definition xml:lang="en">Website address where the buyer publishes information on its procurement procedures and general information.

WG approval 04/05/2018
</skos:definition>
      <rdfs:isDefinedBy rdf:resource="http://data.europa.eu/a4g/ontology"/>
   </owl:Class>
   <owl:Class rdf:about="http://data.europa.eu/a4g/ontology#BuyerProfileNotice">
      <rdfs:label xml:lang="en">Buyer profile notice</rdfs:label>
      <skos:prefLabel xml:lang="en">Buyer profile notice</skos:prefLabel>
      <rdfs:comment xml:lang="en">Notice of the existence of a buyer profile.
WG approval 13/04/2021</rdfs:comment>
      <skos:definition xml:lang="en">Notice of the existence of a buyer profile.
WG approval 13/04/2021</skos:definition>
      <rdfs:isDefinedBy rdf:resource="http://data.europa.eu/a4g/ontology"/>
   </owl:Class>
   <owl:Class rdf:about="http://data.europa.eu/a4g/ontology#CallForCompetition">
      <rdfs:label xml:lang="en">Call for competition</rdfs:label>
      <skos:prefLabel xml:lang="en">Call for competition</skos:prefLabel>
      <rdfs:comment xml:lang="en">A public announcement of the launch of a procurement procedure.

(WG approval 14/05/2017)</rdfs:comment>
      <skos:definition xml:lang="en">A public announcement of the launch of a procurement procedure.

(WG approval 14/05/2017)</skos:definition>
      <rdfs:isDefinedBy rdf:resource="http://data.europa.eu/a4g/ontology"/>
   </owl:Class>
   <owl:Class rdf:about="http://data.europa.eu/a4g/ontology#CallForExpressionOfInterest">
      <rdfs:label xml:lang="en">Call for expression of interest</rdfs:label>
      <skos:prefLabel xml:lang="en">Call for expression of interest</skos:prefLabel>
      <rdfs:comment xml:lang="en">A call to potential providers of goods and/or services to register interest in supplying them. It is a document that describes a set of requirements or specifications and that service providers have to demonstrate their ability to meet those requirements. 
</rdfs:comment>
      <skos:definition xml:lang="en">A call to potential providers of goods and/or services to register interest in supplying them. It is a document that describes a set of requirements or specifications and that service providers have to demonstrate their ability to meet those requirements. 
</skos:definition>
      <rdfs:isDefinedBy rdf:resource="http://data.europa.eu/a4g/ontology"/>
   </owl:Class>
   <owl:Class rdf:about="http://data.europa.eu/a4g/ontology#CatalogueProvider">
      <rdfs:label xml:lang="en">Catalogue provider</rdfs:label>
      <skos:prefLabel xml:lang="en">Catalogue provider</skos:prefLabel>
      <rdfs:comment xml:lang="en">A role of an agent compiling and supplying a catalogue.

Additional Information:

The catalogue provider role is usually played by the agent that acts as a seller, or by another agent that acts on behalf of the seller.

WG Approval 28/01/2021
</rdfs:comment>
      <skos:definition xml:lang="en">A role of an agent compiling and supplying a catalogue.

Additional Information:

The catalogue provider role is usually played by the agent that acts as a seller, or by another agent that acts on behalf of the seller.

WG Approval 28/01/2021
</skos:definition>
      <rdfs:isDefinedBy rdf:resource="http://data.europa.eu/a4g/ontology"/>
   </owl:Class>
   <owl:Class rdf:about="http://data.europa.eu/a4g/ontology#CatalogueReceiver">
      <rdfs:label xml:lang="en">Catalogue receiver</rdfs:label>
      <skos:prefLabel xml:lang="en">Catalogue receiver</skos:prefLabel>
      <rdfs:comment xml:lang="en">A role of an agent processing a catalogue.

Additional Information:
The catalogue receiver may not only receive it but also validate it, process it, etc.

The catalogue receiver role is usually played by the agent that acts as a buyer, or by another agent that acts on behalf of the buyer.

WG Approval 28/01/2021</rdfs:comment>
      <skos:definition xml:lang="en">A role of an agent processing a catalogue.

Additional Information:
The catalogue receiver may not only receive it but also validate it, process it, etc.

The catalogue receiver role is usually played by the agent that acts as a buyer, or by another agent that acts on behalf of the buyer.

WG Approval 28/01/2021</skos:definition>
      <rdfs:isDefinedBy rdf:resource="http://data.europa.eu/a4g/ontology"/>
   </owl:Class>
   <owl:Class rdf:about="http://data.europa.eu/a4g/ontology#CentralPurchasingBody">
      <rdfs:label xml:lang="en">Central purchasing body</rdfs:label>
      <skos:prefLabel xml:lang="en">Central purchasing body</skos:prefLabel>
      <rdfs:comment xml:lang="en">Role of an agent that provides centralised purchasing activities and, possibly, ancillary purchasing activities for other buyers.
WG approval 05/08/2021
Additional Information:
In public procurement the role of Central purchasing body is carried out by a Contracting Authority for other Contracting Authorities.
Contracting authority procuring activities conducted on a permanent basis, in one of the following forms:[...](b) the award of public contracts or the conclusion of framework agreements for works, supplies or services intended for contracting authorities;
</rdfs:comment>
      <skos:definition xml:lang="en">Role of an agent that provides centralised purchasing activities and, possibly, ancillary purchasing activities for other buyers.
WG approval 05/08/2021
Additional Information:
In public procurement the role of Central purchasing body is carried out by a Contracting Authority for other Contracting Authorities.
Contracting authority procuring activities conducted on a permanent basis, in one of the following forms:[...](b) the award of public contracts or the conclusion of framework agreements for works, supplies or services intended for contracting authorities;
</skos:definition>
      <rdfs:isDefinedBy rdf:resource="http://data.europa.eu/a4g/ontology"/>
   </owl:Class>
   <owl:Class rdf:about="http://data.europa.eu/a4g/ontology#Change">
      <rdfs:label xml:lang="en">Change</rdfs:label>
      <skos:prefLabel xml:lang="en">Change</skos:prefLabel>
      <rdfs:comment xml:lang="en">Update of information.

WG Approval 5/11/2019</rdfs:comment>
      <skos:definition xml:lang="en">Update of information.

WG Approval 5/11/2019</skos:definition>
      <rdfs:isDefinedBy rdf:resource="http://data.europa.eu/a4g/ontology"/>
   </owl:Class>
   <owl:Class rdf:about="http://data.europa.eu/a4g/ontology#Channel">
      <rdfs:label xml:lang="en">Channel</rdfs:label>
      <skos:prefLabel xml:lang="en">Channel</skos:prefLabel>
      <rdfs:comment xml:lang="en">Software solutions and electronic devices for communication and exchange of information between buyers and economic operators.

Additional Information

Lots may use ad-hoc electronic means of communication that are not generally available such as specific solutions for secure and dedicated communication or non-standard eCatalogues. 

See also Directive recitals 53 to 56.

WG Suggestion to eForms 30/09/2019


</rdfs:comment>
      <skos:definition xml:lang="en">Software solutions and electronic devices for communication and exchange of information between buyers and economic operators.

Additional Information

Lots may use ad-hoc electronic means of communication that are not generally available such as specific solutions for secure and dedicated communication or non-standard eCatalogues. 

See also Directive recitals 53 to 56.

WG Suggestion to eForms 30/09/2019


</skos:definition>
      <rdfs:isDefinedBy rdf:resource="http://data.europa.eu/a4g/ontology"/>
   </owl:Class>
   <owl:Class rdf:about="http://data.europa.eu/a4g/ontology#ContactPoint">
      <rdfs:label xml:lang="en">Contact point</rdfs:label>
      <skos:prefLabel xml:lang="en">Contact point</skos:prefLabel>
      <rdfs:comment xml:lang="en">Details used to reach an organisation.

Additional information: 

The contact point could be a role, email address, telephone number, etc.

WG approval 5/11/2019</rdfs:comment>
      <skos:definition xml:lang="en">Details used to reach an organisation.

Additional information: 

The contact point could be a role, email address, telephone number, etc.

WG approval 5/11/2019</skos:definition>
      <rdfs:isDefinedBy rdf:resource="http://data.europa.eu/a4g/ontology"/>
   </owl:Class>
   <owl:Class rdf:about="http://data.europa.eu/a4g/ontology#Contract">
      <rdfs:label xml:lang="en">Contract</rdfs:label>
      <skos:prefLabel xml:lang="en">Contract</skos:prefLabel>
      <rdfs:comment xml:lang="en">A voluntary, deliberate, and legally binding agreement between two or more competent parties.

Additional information:

This includes concession contracts.

(WG approval 01/06/2018)</rdfs:comment>
      <skos:definition xml:lang="en">A voluntary, deliberate, and legally binding agreement between two or more competent parties.

Additional information:

This includes concession contracts.

(WG approval 01/06/2018)</skos:definition>
      <rdfs:isDefinedBy rdf:resource="http://data.europa.eu/a4g/ontology"/>
   </owl:Class>
   <owl:Class rdf:about="http://data.europa.eu/a4g/ontology#ContractAwardNotice">
      <rdfs:label xml:lang="en">Contract award notice</rdfs:label>
      <skos:prefLabel xml:lang="en">Contract award notice</skos:prefLabel>
      <rdfs:comment xml:lang="en">An announcement of the award or non-award of a contract by a procuring entity.

(WG approval 27/03/2019 9:41:42)</rdfs:comment>
      <skos:definition xml:lang="en">An announcement of the award or non-award of a contract by a procuring entity.

(WG approval 27/03/2019 9:41:42)</skos:definition>
      <rdfs:isDefinedBy rdf:resource="http://data.europa.eu/a4g/ontology"/>
   </owl:Class>
   <owl:Class rdf:about="http://data.europa.eu/a4g/ontology#ContractModificationNotice">
      <rdfs:label xml:lang="en">Contract modification notice</rdfs:label>
      <skos:prefLabel xml:lang="en">Contract modification notice</skos:prefLabel>
      <rdfs:comment xml:lang="en">An announcement of the modification of a contract/concession during during its term by a procuring entity.

</rdfs:comment>
      <skos:definition xml:lang="en">An announcement of the modification of a contract/concession during during its term by a procuring entity.

</skos:definition>
      <rdfs:isDefinedBy rdf:resource="http://data.europa.eu/a4g/ontology"/>
   </owl:Class>
   <owl:Class rdf:about="http://data.europa.eu/a4g/ontology#ContractNotice">
      <rdfs:label xml:lang="en">Contract notice</rdfs:label>
      <skos:prefLabel xml:lang="en">Contract notice</skos:prefLabel>
      <rdfs:comment xml:lang="en">An announcement of the launch of a procurement procedure by a procuring entity.

(WG approval 18/05/2018)</rdfs:comment>
      <skos:definition xml:lang="en">An announcement of the launch of a procurement procedure by a procuring entity.

(WG approval 18/05/2018)</skos:definition>
      <rdfs:isDefinedBy rdf:resource="http://data.europa.eu/a4g/ontology"/>
   </owl:Class>
   <owl:Class rdf:about="http://data.europa.eu/a4g/ontology#Contractor">
      <rdfs:label xml:lang="en">Contractor</rdfs:label>
      <skos:prefLabel xml:lang="en">Contractor</skos:prefLabel>
      <rdfs:comment xml:lang="en">An economic operator that has signed a contract with a purchaser.
WG approval 13/04/2021</rdfs:comment>
      <skos:definition xml:lang="en">An economic operator that has signed a contract with a purchaser.
WG approval 13/04/2021</skos:definition>
      <rdfs:isDefinedBy rdf:resource="http://data.europa.eu/a4g/ontology"/>
   </owl:Class>
   <owl:Class rdf:about="http://data.europa.eu/a4g/ontology#ContractTerm">
      <rdfs:label xml:lang="en">Contract term</rdfs:label>
      <skos:prefLabel xml:lang="en">Contract term</skos:prefLabel>
      <rdfs:comment xml:lang="en">Conditions and stipulations defining particularities of the post award phase.

(WG approval 23/11/2018)
</rdfs:comment>
      <skos:definition xml:lang="en">Conditions and stipulations defining particularities of the post award phase.

(WG approval 23/11/2018)
</skos:definition>
      <rdfs:isDefinedBy rdf:resource="http://data.europa.eu/a4g/ontology"/>
   </owl:Class>
   <owl:Class rdf:about="http://data.europa.eu/a4g/ontology#DesignContestRegimeTerm">
      <rdfs:label xml:lang="en">Design contest regime term</rdfs:label>
      <skos:prefLabel xml:lang="en">Design contest regime term</skos:prefLabel>
      <rdfs:comment xml:lang="en">Conditions and stipulations defining particularities of a Design Contest.

WG approval: 04-02-2021</rdfs:comment>
      <skos:definition xml:lang="en">Conditions and stipulations defining particularities of a Design Contest.

WG approval: 04-02-2021</skos:definition>
      <rdfs:isDefinedBy rdf:resource="http://data.europa.eu/a4g/ontology"/>
   </owl:Class>
   <owl:Class rdf:about="http://data.europa.eu/a4g/ontology#DirectAwardTerm">
      <rdfs:label xml:lang="en">Direct award term</rdfs:label>
      <skos:prefLabel xml:lang="en">Direct award term</skos:prefLabel>
      <rdfs:comment xml:lang="en">Conditions and stipulations defining particularities of the award of a contract without prior publication.

Addtional Information:

Direct award may refer to a previous procedure and/or specific Lot(s).

It may also refer to other justified situations whereby there is no previous procedure.

See Directive 2014/24/EU Article 32.

WG Approval 22/11/2019


</rdfs:comment>
      <skos:definition xml:lang="en">Conditions and stipulations defining particularities of the award of a contract without prior publication.

Addtional Information:

Direct award may refer to a previous procedure and/or specific Lot(s).

It may also refer to other justified situations whereby there is no previous procedure.

See Directive 2014/24/EU Article 32.

WG Approval 22/11/2019


</skos:definition>
      <rdfs:isDefinedBy rdf:resource="http://data.europa.eu/a4g/ontology"/>
   </owl:Class>
   <owl:Class rdf:about="http://data.europa.eu/a4g/ontology#Document">
      <rdfs:label xml:lang="en">Document</rdfs:label>
      <skos:prefLabel xml:lang="en">Document</skos:prefLabel>
      <rdfs:comment xml:lang="en">A set of interrelated Business Information representing the business facts.

Additional Information:
Documents may convey information in any language, medium or form, including textual, numerical, graphic, cartographic, audio-visual forms, etc.

WG Approval 23/05/2019
</rdfs:comment>
      <skos:definition xml:lang="en">A set of interrelated Business Information representing the business facts.

Additional Information:
Documents may convey information in any language, medium or form, including textual, numerical, graphic, cartographic, audio-visual forms, etc.

WG Approval 23/05/2019
</skos:definition>
      <rdfs:isDefinedBy rdf:resource="http://data.europa.eu/a4g/ontology"/>
   </owl:Class>
   <owl:Class rdf:about="http://data.europa.eu/a4g/ontology#DynamicPurchaseSystemTechnique">
      <rdfs:label xml:lang="en">Dynamic purchase system technique</rdfs:label>
      <skos:prefLabel xml:lang="en">Dynamic purchase system technique</skos:prefLabel>
      <rdfs:comment xml:lang="en">An electronic system that is set up by a procuring entity which lists the economic operators that satisfy the selection and exclusion criteria.   This technique then allows the purchase via consultation of the listed tenderers using award criteria.

(WG approval 13/07/2018)</rdfs:comment>
      <skos:definition xml:lang="en">An electronic system that is set up by a procuring entity which lists the economic operators that satisfy the selection and exclusion criteria.   This technique then allows the purchase via consultation of the listed tenderers using award criteria.

(WG approval 13/07/2018)</skos:definition>
      <rdfs:isDefinedBy rdf:resource="http://data.europa.eu/a4g/ontology"/>
   </owl:Class>
   <owl:Class rdf:about="http://data.europa.eu/a4g/ontology#EAuctionTechnique">
      <rdfs:label xml:lang="en">E auction technique</rdfs:label>
      <skos:prefLabel xml:lang="en">E auction technique</skos:prefLabel>
      <rdfs:comment xml:lang="en">A repetitive technique in which new prices, revised downwards, and/or new values concerning certain elements of tenders are bid on-line.

(WG approval 20/07/2018)</rdfs:comment>
      <skos:definition xml:lang="en">A repetitive technique in which new prices, revised downwards, and/or new values concerning certain elements of tenders are bid on-line.

(WG approval 20/07/2018)</skos:definition>
      <rdfs:isDefinedBy rdf:resource="http://data.europa.eu/a4g/ontology"/>
   </owl:Class>
   <owl:Class rdf:about="http://data.europa.eu/a4g/ontology#EconomicOperator">
      <rdfs:label xml:lang="en">Economic operator</rdfs:label>
      <skos:prefLabel xml:lang="en">Economic operator</skos:prefLabel>
      <rdfs:comment xml:lang="en">A role of an agent which offers the execution of works, services or supplies on the market.
WG Approval 05/08/2021</rdfs:comment>
      <skos:definition xml:lang="en">A role of an agent which offers the execution of works, services or supplies on the market.
WG Approval 05/08/2021</skos:definition>
      <rdfs:isDefinedBy rdf:resource="http://data.europa.eu/a4g/ontology"/>
   </owl:Class>
   <owl:Class rdf:about="http://data.europa.eu/a4g/ontology#EvaluationBoard">
      <rdfs:label xml:lang="en">Evaluation board</rdfs:label>
      <skos:prefLabel xml:lang="en">Evaluation board</skos:prefLabel>
      <rdfs:comment xml:lang="en">Committee set up to evaluate the tenders submitted.
Additional Information: 
The committee may be a regular board or a jury.
WG approval 13/04/2021</rdfs:comment>
      <skos:definition xml:lang="en">Committee set up to evaluate the tenders submitted.
Additional Information: 
The committee may be a regular board or a jury.
WG approval 13/04/2021</skos:definition>
      <rdfs:isDefinedBy rdf:resource="http://data.europa.eu/a4g/ontology"/>
   </owl:Class>
   <owl:Class rdf:about="http://data.europa.eu/a4g/ontology#EvaluationTerm">
      <rdfs:label xml:lang="en">Evaluation term</rdfs:label>
      <skos:prefLabel xml:lang="en">Evaluation term</skos:prefLabel>
      <rdfs:comment xml:lang="en">Conditions and stipulations defining particularities of the tender evaluation.

(WG approval 23/11/2018)


</rdfs:comment>
      <skos:definition xml:lang="en">Conditions and stipulations defining particularities of the tender evaluation.

(WG approval 23/11/2018)


</skos:definition>
      <rdfs:isDefinedBy rdf:resource="http://data.europa.eu/a4g/ontology"/>
   </owl:Class>
   <owl:Class rdf:about="http://data.europa.eu/a4g/ontology#ExclusionGround">
      <rdfs:label xml:lang="en">Exclusion ground</rdfs:label>
      <skos:prefLabel xml:lang="en">Exclusion ground</skos:prefLabel>
      <rdfs:comment xml:lang="en">Describes a legal requirement to be met by the economic operator to be a candidate in the procurement procedure.

WG approval 31/10/2018</rdfs:comment>
      <skos:definition xml:lang="en">Describes a legal requirement to be met by the economic operator to be a candidate in the procurement procedure.

WG approval 31/10/2018</skos:definition>
      <rdfs:isDefinedBy rdf:resource="http://data.europa.eu/a4g/ontology"/>
   </owl:Class>
   <owl:Class rdf:about="http://data.europa.eu/a4g/ontology#ExpressionOfInterest">
      <rdfs:label xml:lang="en">Expression of interest</rdfs:label>
      <skos:prefLabel xml:lang="en">Expression of interest</skos:prefLabel>
      <rdfs:comment xml:lang="en">Document presenting an economic operator's request to be considered for procedures covering a specific domain.
WG approval 13/04/2021</rdfs:comment>
      <skos:definition xml:lang="en">Document presenting an economic operator's request to be considered for procedures covering a specific domain.
WG approval 13/04/2021</skos:definition>
      <rdfs:isDefinedBy rdf:resource="http://data.europa.eu/a4g/ontology"/>
   </owl:Class>
   <owl:Class rdf:about="http://data.europa.eu/a4g/ontology#FrameworkAgreement">
      <rdfs:label xml:lang="en">Framework agreement</rdfs:label>
      <skos:prefLabel xml:lang="en">Framework agreement</skos:prefLabel>
      <rdfs:comment xml:lang="en">An agreement between one or more contracting authorities and one or more economic operators.

WG approval 18/05/2021</rdfs:comment>
      <skos:definition xml:lang="en">An agreement between one or more contracting authorities and one or more economic operators.

WG approval 18/05/2021</skos:definition>
      <rdfs:isDefinedBy rdf:resource="http://data.europa.eu/a4g/ontology"/>
   </owl:Class>
   <owl:Class rdf:about="http://data.europa.eu/a4g/ontology#FrameworkAgreementTechnique">
      <rdfs:label xml:lang="en">Framework agreement technique</rdfs:label>
      <skos:prefLabel xml:lang="en">Framework agreement technique</skos:prefLabel>
      <rdfs:comment xml:lang="en">Technique that establishes the terms governing contracts to be awarded during a given period, in particular with regard to price and, where appropriate, the quantity envisaged.

WG approval 18/05/2021</rdfs:comment>
      <skos:definition xml:lang="en">Technique that establishes the terms governing contracts to be awarded during a given period, in particular with regard to price and, where appropriate, the quantity envisaged.

WG approval 18/05/2021</skos:definition>
      <rdfs:isDefinedBy rdf:resource="http://data.europa.eu/a4g/ontology"/>
   </owl:Class>
   <owl:Class rdf:about="http://data.europa.eu/a4g/ontology#FrameworkAgreementTerm">
      <rdfs:label xml:lang="en">Framework agreement term</rdfs:label>
      <skos:prefLabel xml:lang="en">Framework agreement term</skos:prefLabel>
      <rdfs:comment xml:lang="en">Reason for extending time limits.

Additional Information: in exceptional cases related, for example, to framework agreements that exceed the legal limits, these limits need to be justified.. (Four years in the case of the general procurement directive, seven years in the case of the defence directive, and eight years in the case of the sectoral directive.).

WG Approval 2019-19-02
</rdfs:comment>
      <skos:definition xml:lang="en">Reason for extending time limits.

Additional Information: in exceptional cases related, for example, to framework agreements that exceed the legal limits, these limits need to be justified.. (Four years in the case of the general procurement directive, seven years in the case of the defence directive, and eight years in the case of the sectoral directive.).

WG Approval 2019-19-02
</skos:definition>
      <rdfs:isDefinedBy rdf:resource="http://data.europa.eu/a4g/ontology"/>
   </owl:Class>
   <owl:Class rdf:about="http://data.europa.eu/a4g/ontology#Fund">
      <rdfs:label xml:lang="en">Fund</rdfs:label>
      <skos:prefLabel xml:lang="en">Fund</skos:prefLabel>
      <rdfs:comment xml:lang="en">A financial resource used to support the procurement.

Additional Information:

In the context of EU, funds can be divided into programmes, actions and projects.

Examples of EU funds are: the European Structural and Investment Funds, European Social Fund (ESF), the Connecting Europe Facility (CEF) programme, or the ISA2 programme and its actions (e.g. Action 2016.05 European Public Procurement Initiative, which supports the eProcurement Ontology under sub-action 3).

Funds may change between the lot and the contract, for example in the case of an emergency crisis, a contract may be financed by a budget that was not foreseen in the call.

WG Approved 14/05/2019




</rdfs:comment>
      <skos:definition xml:lang="en">A financial resource used to support the procurement.

Additional Information:

In the context of EU, funds can be divided into programmes, actions and projects.

Examples of EU funds are: the European Structural and Investment Funds, European Social Fund (ESF), the Connecting Europe Facility (CEF) programme, or the ISA2 programme and its actions (e.g. Action 2016.05 European Public Procurement Initiative, which supports the eProcurement Ontology under sub-action 3).

Funds may change between the lot and the contract, for example in the case of an emergency crisis, a contract may be financed by a budget that was not foreseen in the call.

WG Approved 14/05/2019




</skos:definition>
      <rdfs:isDefinedBy rdf:resource="http://data.europa.eu/a4g/ontology"/>
   </owl:Class>
   <owl:Class rdf:about="http://data.europa.eu/a4g/ontology#GreenProcurement">
      <rdfs:label xml:lang="en">Green procurement</rdfs:label>
      <skos:prefLabel xml:lang="en">Green procurement</skos:prefLabel>
      <rdfs:comment xml:lang="en">Approach whereby buyers seek to procure with a reduced environmental impact.

Additional Information:

The approach may apply to the complete life cycle. The reduced environmental impact is in comparison to goods, services and works with the same primary function that would otherwise be procured. 

Tightly related are article 68 - Life-cycle costing and article 67 - most economically advantageous tender (see GPP handbook) https://ec.europa.eu/environment/gpp/pdf/Buying-Green-Handbook-3rd-Edition.pdf
An instance of the class GreenProcurement is represented in eForms with the code "env-imp" defined in the codelist strategic-procurement.paragraphs) https://ec.europa.eu/environment/gpp/pdf/Buying-Green-Handbook-3rd-Edition.pdf</rdfs:comment>
      <skos:definition xml:lang="en">Approach whereby buyers seek to procure with a reduced environmental impact.

Additional Information:

The approach may apply to the complete life cycle. The reduced environmental impact is in comparison to goods, services and works with the same primary function that would otherwise be procured. 

Tightly related are article 68 - Life-cycle costing and article 67 - most economically advantageous tender (see GPP handbook) https://ec.europa.eu/environment/gpp/pdf/Buying-Green-Handbook-3rd-Edition.pdf
An instance of the class GreenProcurement is represented in eForms with the code "env-imp" defined in the codelist strategic-procurement.paragraphs) https://ec.europa.eu/environment/gpp/pdf/Buying-Green-Handbook-3rd-Edition.pdf</skos:definition>
      <rdfs:isDefinedBy rdf:resource="http://data.europa.eu/a4g/ontology"/>
   </owl:Class>
   <owl:Class rdf:about="http://data.europa.eu/a4g/ontology#InnovativeProcurement">
      <rdfs:label xml:lang="en">Innovative procurement</rdfs:label>
      <skos:prefLabel xml:lang="en">Innovative procurement</skos:prefLabel>
      <rdfs:comment xml:lang="en">An instance of the class InnovativeProcurement is represented in eForms with the code "inn-pur" defined in the codelist strategic-procurement.

Research (21/01/2020):

Purchasing and early adoption of solutions which are not yet available on large scale commercial basis. 

Source: Adapted from the Digital Single Market's Policy on Public Procurement of Innovative Solutions. https://ec.europa.eu/digital-single-market/en/public-procurement-innovative-solutions

Additional Information: 
‘innovation’ means the implementation of a new or significantly improved product, service or process, including but not limited to production, building or construction processes, a new marketing method, or a new organisational method in business practices, workplace organisation or external relations inter alia with the purpose of helping to solve societal challenges or to support the Europe 2020 strategy for smart, sustainable and inclusive growth;
See: Directive 2014/24
Articles: 2, 26 (3), 31, 67 (2.a)

Question: 
Is  Pre-Commercial Procurement (PCP) another type of Strategic Procurement?</rdfs:comment>
      <skos:definition xml:lang="en">An instance of the class InnovativeProcurement is represented in eForms with the code "inn-pur" defined in the codelist strategic-procurement.

Research (21/01/2020):

Purchasing and early adoption of solutions which are not yet available on large scale commercial basis. 

Source: Adapted from the Digital Single Market's Policy on Public Procurement of Innovative Solutions. https://ec.europa.eu/digital-single-market/en/public-procurement-innovative-solutions

Additional Information: 
‘innovation’ means the implementation of a new or significantly improved product, service or process, including but not limited to production, building or construction processes, a new marketing method, or a new organisational method in business practices, workplace organisation or external relations inter alia with the purpose of helping to solve societal challenges or to support the Europe 2020 strategy for smart, sustainable and inclusive growth;
See: Directive 2014/24
Articles: 2, 26 (3), 31, 67 (2.a)

Question: 
Is  Pre-Commercial Procurement (PCP) another type of Strategic Procurement?</skos:definition>
      <rdfs:isDefinedBy rdf:resource="http://data.europa.eu/a4g/ontology"/>
   </owl:Class>
   <owl:Class rdf:about="http://data.europa.eu/a4g/ontology#Item">
      <rdfs:label xml:lang="en">Item</rdfs:label>
      <skos:prefLabel xml:lang="en">Item</skos:prefLabel>
      <rdfs:comment xml:lang="en">A singular product or service.
Additional Information:
An item can be an atomic thing or a composition of things that together are seen as a unit, e.g. a tetrabrik of milk or an indivisible package of six tetrabriks.
WG approval 04/03/2021</rdfs:comment>
      <skos:definition xml:lang="en">A singular product or service.
Additional Information:
An item can be an atomic thing or a composition of things that together are seen as a unit, e.g. a tetrabrik of milk or an indivisible package of six tetrabriks.
WG approval 04/03/2021</skos:definition>
      <rdfs:isDefinedBy rdf:resource="http://data.europa.eu/a4g/ontology"/>
   </owl:Class>
   <owl:Class rdf:about="http://data.europa.eu/a4g/ontology#Lot">
      <rdfs:label xml:lang="en">Lot</rdfs:label>
      <skos:prefLabel xml:lang="en">Lot</skos:prefLabel>
      <rdfs:comment xml:lang="en">A qualitative, quantitative or strategic subdivision of the goods, services or works to be procured, allowing the award of one or more contracts.

WG approval 12/09/2018</rdfs:comment>
      <skos:definition xml:lang="en">A qualitative, quantitative or strategic subdivision of the goods, services or works to be procured, allowing the award of one or more contracts.

WG approval 12/09/2018</skos:definition>
      <rdfs:isDefinedBy rdf:resource="http://data.europa.eu/a4g/ontology"/>
   </owl:Class>
   <owl:Class rdf:about="http://data.europa.eu/a4g/ontology#LotGroup">
      <rdfs:label xml:lang="en">Lot group</rdfs:label>
      <skos:prefLabel xml:lang="en">Lot group</skos:prefLabel>
      <rdfs:comment xml:lang="en">Combination of several lots to conduct comparative assessment of the tenders.

Additional Information:

The comparative assessment may refer to the selection criteria, award and value that apply to several lots.

Pending of discussion with eForms



Member States may provide that, where more than one lot may be awarded to the same tenderer, contracting authorities may award contracts combining several or all lots where they have specified in the contract notice or in the invitation to confirm interest that they reserve the possibility of doing so and indicate the lots or groups of lots that may be combined.</rdfs:comment>
      <skos:definition xml:lang="en">Combination of several lots to conduct comparative assessment of the tenders.

Additional Information:

The comparative assessment may refer to the selection criteria, award and value that apply to several lots.

Pending of discussion with eForms



Member States may provide that, where more than one lot may be awarded to the same tenderer, contracting authorities may award contracts combining several or all lots where they have specified in the contract notice or in the invitation to confirm interest that they reserve the possibility of doing so and indicate the lots or groups of lots that may be combined.</skos:definition>
      <rdfs:isDefinedBy rdf:resource="http://data.europa.eu/a4g/ontology"/>
   </owl:Class>
   <owl:Class rdf:about="http://data.europa.eu/a4g/ontology#Mediator">
      <rdfs:label xml:lang="en">Mediator</rdfs:label>
      <skos:prefLabel xml:lang="en">Mediator</skos:prefLabel>
      <rdfs:comment xml:lang="en">A role of an agent  that  attempts to resolve a dispute between different agents and come to an agreement.
WG approval 20/04/2021</rdfs:comment>
      <skos:definition xml:lang="en">A role of an agent  that  attempts to resolve a dispute between different agents and come to an agreement.
WG approval 20/04/2021</skos:definition>
      <rdfs:isDefinedBy rdf:resource="http://data.europa.eu/a4g/ontology"/>
   </owl:Class>
   <owl:Class rdf:about="http://data.europa.eu/a4g/ontology#MultipleStageProcedureTerm">
      <rdfs:label xml:lang="en">Multiple stage procedure term</rdfs:label>
      <skos:prefLabel xml:lang="en">Multiple stage procedure term</skos:prefLabel>
      <rdfs:comment xml:lang="en">Conditions and stipulations defining particularities of procedures carried out in several steps
Additional Information: 
Generally this refers to procedures where selection is carried out to qualify tenderers who are then requested to submit the rest of their tender for evaluation  ie Restricted procedure
WG Approval 15/04/2021</rdfs:comment>
      <skos:definition xml:lang="en">Conditions and stipulations defining particularities of procedures carried out in several steps
Additional Information: 
Generally this refers to procedures where selection is carried out to qualify tenderers who are then requested to submit the rest of their tender for evaluation  ie Restricted procedure
WG Approval 15/04/2021</skos:definition>
      <rdfs:isDefinedBy rdf:resource="http://data.europa.eu/a4g/ontology"/>
   </owl:Class>
   <owl:Class rdf:about="http://data.europa.eu/a4g/ontology#Notice">
      <rdfs:label xml:lang="en">Notice</rdfs:label>
      <skos:prefLabel xml:lang="en">Notice</skos:prefLabel>
      <rdfs:comment xml:lang="en">Document published by the buyer about market opportunities and results.

WG Approval 23/05/2019
</rdfs:comment>
      <skos:definition xml:lang="en">Document published by the buyer about market opportunities and results.

WG Approval 23/05/2019
</skos:definition>
      <rdfs:isDefinedBy rdf:resource="http://data.europa.eu/a4g/ontology"/>
   </owl:Class>
   <owl:Class rdf:about="http://data.europa.eu/a4g/ontology#OpeningTerm">
      <rdfs:label xml:lang="en">Opening term</rdfs:label>
      <skos:prefLabel xml:lang="en">Opening term</skos:prefLabel>
      <rdfs:comment xml:lang="en">Conditions and stipulations defining particularities of the opening of tenders.
Additional Information:
The opening of tenders is the event when tenders are made accessible for evaluation, it is generally the same date and time for all tenders.
WG Approval 15/04/2021</rdfs:comment>
      <skos:definition xml:lang="en">Conditions and stipulations defining particularities of the opening of tenders.
Additional Information:
The opening of tenders is the event when tenders are made accessible for evaluation, it is generally the same date and time for all tenders.
WG Approval 15/04/2021</skos:definition>
      <rdfs:isDefinedBy rdf:resource="http://data.europa.eu/a4g/ontology"/>
   </owl:Class>
   <owl:Class rdf:about="http://data.europa.eu/a4g/ontology#Organisation">
      <rdfs:label xml:lang="en">Organisation</rdfs:label>
      <skos:prefLabel xml:lang="en">Organisation</skos:prefLabel>
      <rdfs:comment xml:lang="en">A collection of people organized together into a community or other social, commercial or political structure. The group has some common purpose or reason for existence which goes beyond the set of people belonging to it and can act as an Agent. Organisations are often decomposable into hierarchical structures.

(WG approval 23/11/2018).
</rdfs:comment>
      <skos:definition xml:lang="en">A collection of people organized together into a community or other social, commercial or political structure. The group has some common purpose or reason for existence which goes beyond the set of people belonging to it and can act as an Agent. Organisations are often decomposable into hierarchical structures.

(WG approval 23/11/2018).
</skos:definition>
      <rdfs:isDefinedBy rdf:resource="http://data.europa.eu/a4g/ontology"/>
   </owl:Class>
   <owl:Class rdf:about="http://data.europa.eu/a4g/ontology#OrganisationGroup">
      <rdfs:label xml:lang="en">Organisation group</rdfs:label>
      <skos:prefLabel xml:lang="en">Organisation group</skos:prefLabel>
      <rdfs:comment xml:lang="en">Agreed collaboration of several organisations.
Additional Information:
This concept has been created to fulfill the need to represent a grouping of organisations that is not necessarily registered ie consortia.
WG approval 15/04/2021</rdfs:comment>
      <skos:definition xml:lang="en">Agreed collaboration of several organisations.
Additional Information:
This concept has been created to fulfill the need to represent a grouping of organisations that is not necessarily registered ie consortia.
WG approval 15/04/2021</skos:definition>
      <rdfs:isDefinedBy rdf:resource="http://data.europa.eu/a4g/ontology"/>
   </owl:Class>
   <owl:Class rdf:about="http://data.europa.eu/a4g/ontology#Period">
      <rdfs:label xml:lang="en">Period</rdfs:label>
      <skos:prefLabel xml:lang="en">Period</skos:prefLabel>
      <rdfs:comment xml:lang="en">A time interval or a duration.

(WG approval 28/04/2020)
</rdfs:comment>
      <skos:definition xml:lang="en">A time interval or a duration.

(WG approval 28/04/2020)
</skos:definition>
      <rdfs:isDefinedBy rdf:resource="http://data.europa.eu/a4g/ontology"/>
   </owl:Class>
   <owl:Class rdf:about="http://data.europa.eu/a4g/ontology#Person">
      <rdfs:label xml:lang="en">Person</rdfs:label>
      <skos:prefLabel xml:lang="en">Person</skos:prefLabel>
      <rdfs:comment xml:lang="en">Individual who is able to carry out actions. 

WG Approval 28/04/2020
</rdfs:comment>
      <skos:definition xml:lang="en">Individual who is able to carry out actions. 

WG Approval 28/04/2020
</skos:definition>
      <rdfs:isDefinedBy rdf:resource="http://data.europa.eu/a4g/ontology"/>
   </owl:Class>
   <owl:Class rdf:about="http://data.europa.eu/a4g/ontology#PlannedProcurementPart">
      <rdfs:label xml:lang="en">Planned procurement part</rdfs:label>
      <skos:prefLabel xml:lang="en">Planned procurement part</skos:prefLabel>
      <rdfs:comment xml:lang="en">A subdivision of a planned procurement that may later become one or more lots or a self-standing procedure. A lot or a procedure can also cover one or more parts of the planned procurement.

WG Approval 20/06/2019</rdfs:comment>
      <skos:definition xml:lang="en">A subdivision of a planned procurement that may later become one or more lots or a self-standing procedure. A lot or a procedure can also cover one or more parts of the planned procurement.

WG Approval 20/06/2019</skos:definition>
      <rdfs:isDefinedBy rdf:resource="http://data.europa.eu/a4g/ontology"/>
   </owl:Class>
   <owl:Class rdf:about="http://data.europa.eu/a4g/ontology#PriorInformationNotice">
      <rdfs:label xml:lang="en">Prior information notice</rdfs:label>
      <skos:prefLabel xml:lang="en">Prior information notice</skos:prefLabel>
      <rdfs:comment xml:lang="en">Notice which sets out the contracting authority's purchasing intentions. It is used by contracting authorities to provide suppliers with information about a procurement process. </rdfs:comment>
      <skos:definition xml:lang="en">Notice which sets out the contracting authority's purchasing intentions. It is used by contracting authorities to provide suppliers with information about a procurement process. </skos:definition>
      <rdfs:isDefinedBy rdf:resource="http://data.europa.eu/a4g/ontology"/>
   </owl:Class>
   <owl:Class rdf:about="http://data.europa.eu/a4g/ontology#Prize">
      <rdfs:label xml:lang="en">Prize</rdfs:label>
      <skos:prefLabel xml:lang="en">Prize</skos:prefLabel>
      <rdfs:comment xml:lang="en">A reward given  in a contest.
WG approval: 15/04/2021</rdfs:comment>
      <skos:definition xml:lang="en">A reward given  in a contest.
WG approval: 15/04/2021</skos:definition>
      <rdfs:isDefinedBy rdf:resource="http://data.europa.eu/a4g/ontology"/>
   </owl:Class>
   <owl:Class rdf:about="http://data.europa.eu/a4g/ontology#Procedure">
      <rdfs:label xml:lang="en">Procedure</rdfs:label>
      <skos:prefLabel xml:lang="en">Procedure</skos:prefLabel>
      <rdfs:comment xml:lang="en">A legally defined set of administrative activities conducted  to conclude one or more contracts.

Additional Information
The procedure is categorised in the law according to different rules determining whether the procedure is open, restricted, negotiated with or without  publicity, etc. (see Procedure Type).

WG Approval 20/08/2019
</rdfs:comment>
      <skos:definition xml:lang="en">A legally defined set of administrative activities conducted  to conclude one or more contracts.

Additional Information
The procedure is categorised in the law according to different rules determining whether the procedure is open, restricted, negotiated with or without  publicity, etc. (see Procedure Type).

WG Approval 20/08/2019
</skos:definition>
      <rdfs:isDefinedBy rdf:resource="http://data.europa.eu/a4g/ontology"/>
   </owl:Class>
   <owl:Class rdf:about="http://data.europa.eu/a4g/ontology#ProcedureTerm">
      <rdfs:label xml:lang="en">Procedure term</rdfs:label>
      <skos:prefLabel xml:lang="en">Procedure term</skos:prefLabel>
      <rdfs:comment xml:lang="en">Conditions and stipulations defining particularities of the procedure.

(WG approval 23/11/2018)</rdfs:comment>
      <skos:definition xml:lang="en">Conditions and stipulations defining particularities of the procedure.

(WG approval 23/11/2018)</skos:definition>
      <rdfs:isDefinedBy rdf:resource="http://data.europa.eu/a4g/ontology"/>
   </owl:Class>
   <owl:Class rdf:about="http://data.europa.eu/a4g/ontology#ProcurementCriterion">
      <rdfs:label xml:lang="en">Procurement criterion</rdfs:label>
      <skos:prefLabel xml:lang="en">Procurement criterion</skos:prefLabel>
      <rdfs:comment xml:lang="en">A criterion specific to Procurement.

Additional Information:

This Procurement Criterion can be only Exclusion Ground, Selection Criterion or Award Criterion. Each of these criteria can contain subcriteria (Criterion class).

WG Approval 23/04/2020</rdfs:comment>
      <skos:definition xml:lang="en">A criterion specific to Procurement.

Additional Information:

This Procurement Criterion can be only Exclusion Ground, Selection Criterion or Award Criterion. Each of these criteria can contain subcriteria (Criterion class).

WG Approval 23/04/2020</skos:definition>
      <rdfs:isDefinedBy rdf:resource="http://data.europa.eu/a4g/ontology"/>
   </owl:Class>
   <owl:Class rdf:about="http://data.europa.eu/a4g/ontology#ProcurementDocument">
      <rdfs:label xml:lang="en">Procurement document</rdfs:label>
      <skos:prefLabel xml:lang="en">Procurement document</skos:prefLabel>
      <rdfs:comment xml:lang="en">Document produced or referred to by the buyer to describe or determine elements of the procurement.

Additional information:

Procurement documents are to be accessible since the date of publication of the contract notice or the prior information notice when used as a call for competition.

Examples of procurement documents are technical specifications, the descriptive document, proposed conditions of contract, formats for the presentation of documents by candidates and tenderers, information on generally applicable obligations.

Other documents related to the procedure such as notices are not considered to be procurement documents.

WG Approval 23/05/2019 17:08:30</rdfs:comment>
      <skos:definition xml:lang="en">Document produced or referred to by the buyer to describe or determine elements of the procurement.

Additional information:

Procurement documents are to be accessible since the date of publication of the contract notice or the prior information notice when used as a call for competition.

Examples of procurement documents are technical specifications, the descriptive document, proposed conditions of contract, formats for the presentation of documents by candidates and tenderers, information on generally applicable obligations.

Other documents related to the procedure such as notices are not considered to be procurement documents.

WG Approval 23/05/2019 17:08:30</skos:definition>
      <rdfs:isDefinedBy rdf:resource="http://data.europa.eu/a4g/ontology"/>
   </owl:Class>
   <owl:Class rdf:about="http://data.europa.eu/a4g/ontology#ProcurementRole">
      <rdfs:label xml:lang="en">Procurement role</rdfs:label>
      <skos:prefLabel xml:lang="en">Procurement role</skos:prefLabel>
      <rdfs:comment xml:lang="en">A part played by an agent in a particular procurement process.
In ePO, the 'procurement processes' related to procurement can be 'purchasing', 'tendering', 'evaluating', 'awarding', 'ordering', 'invoicing', etc. 
WG approval 9/09/2021</rdfs:comment>
      <skos:definition xml:lang="en">A part played by an agent in a particular procurement process.
In ePO, the 'procurement processes' related to procurement can be 'purchasing', 'tendering', 'evaluating', 'awarding', 'ordering', 'invoicing', etc. 
WG approval 9/09/2021</skos:definition>
      <rdfs:isDefinedBy rdf:resource="http://data.europa.eu/a4g/ontology"/>
   </owl:Class>
   <owl:Class rdf:about="http://data.europa.eu/a4g/ontology#ProcurementServiceProvider">
      <rdfs:label xml:lang="en">Procurement service provider</rdfs:label>
      <skos:prefLabel xml:lang="en">Procurement service provider</skos:prefLabel>
      <rdfs:comment xml:lang="en">Role of a public or private body which offers ancillary purchasing activities on the market.

Additional information

"Ancillary purchasing activities" means activities consisting in the provision of support to purchasing activities, in particular in the following forms:
(a) technical infrastructure enabling contracting authorities to award public contracts or to conclude framework agreements for works, supplies or services;
(b) advice on the conduct or design of public procurement procedures;
(c) preparation and management of procurement procedures on behalf and for the account of the contracting authority concerned;

Source: Directive 2014/24/EU, Article 2, paragraphs 17 and 15.

This would be equivalent to the concept of 'procuringEntity' in OCDS: 'The entity managing the procurement, which may be different from the buyer who is paying / using the items being procured'.

WG Approval 24/03/2020
</rdfs:comment>
      <skos:definition xml:lang="en">Role of a public or private body which offers ancillary purchasing activities on the market.

Additional information

"Ancillary purchasing activities" means activities consisting in the provision of support to purchasing activities, in particular in the following forms:
(a) technical infrastructure enabling contracting authorities to award public contracts or to conclude framework agreements for works, supplies or services;
(b) advice on the conduct or design of public procurement procedures;
(c) preparation and management of procurement procedures on behalf and for the account of the contracting authority concerned;

Source: Directive 2014/24/EU, Article 2, paragraphs 17 and 15.

This would be equivalent to the concept of 'procuringEntity' in OCDS: 'The entity managing the procurement, which may be different from the buyer who is paying / using the items being procured'.

WG Approval 24/03/2020
</skos:definition>
      <rdfs:isDefinedBy rdf:resource="http://data.europa.eu/a4g/ontology"/>
   </owl:Class>
   <owl:Class rdf:about="http://data.europa.eu/a4g/ontology#ProjectProcurement">
      <rdfs:label xml:lang="en">Project procurement</rdfs:label>
      <skos:prefLabel xml:lang="en">Project procurement</skos:prefLabel>
      <rdfs:comment xml:lang="en">A set of linked procurement activities.

Additional Information:
Project Procurement can be explained as the grouping of several procurements. For example, when planning the construction of an airport several procurements can be foreseen, which may end up in different lots in one or more procedures: one aimed at the purchasing of tarmac for the runways, another for the contracting of catering services, another for the construction of the buildings, etc.. These procurements may be launched in different times (different years, for example).

WG 12/09/2018</rdfs:comment>
      <skos:definition xml:lang="en">A set of linked procurement activities.

Additional Information:
Project Procurement can be explained as the grouping of several procurements. For example, when planning the construction of an airport several procurements can be foreseen, which may end up in different lots in one or more procedures: one aimed at the purchasing of tarmac for the runways, another for the contracting of catering services, another for the construction of the buildings, etc.. These procurements may be launched in different times (different years, for example).

WG 12/09/2018</skos:definition>
      <rdfs:isDefinedBy rdf:resource="http://data.europa.eu/a4g/ontology"/>
   </owl:Class>
   <owl:Class rdf:about="http://data.europa.eu/a4g/ontology#PublicationProvision">
      <rdfs:label xml:lang="en">Publication provision</rdfs:label>
      <skos:prefLabel xml:lang="en">Publication provision</skos:prefLabel>
      <rdfs:comment xml:lang="en">Information about fields not intended for publication. 


Additional Information:
The non-published information may become available at a later date and may differ from one element to another within a given document.

Examples of fields that may not be immediately published are Winner, Tender and Procedure Lot Result, etc., e.g. for security reasons.

WG Approval 16/05/2019




</rdfs:comment>
      <skos:definition xml:lang="en">Information about fields not intended for publication. 


Additional Information:
The non-published information may become available at a later date and may differ from one element to another within a given document.

Examples of fields that may not be immediately published are Winner, Tender and Procedure Lot Result, etc., e.g. for security reasons.

WG Approval 16/05/2019




</skos:definition>
      <rdfs:isDefinedBy rdf:resource="http://data.europa.eu/a4g/ontology"/>
   </owl:Class>
   <owl:Class rdf:about="http://data.europa.eu/a4g/ontology#PublicOrganisation">
      <rdfs:label xml:lang="en">Public organisation</rdfs:label>
      <skos:prefLabel xml:lang="en">Public organisation</skos:prefLabel>
      <rdfs:comment xml:lang="en">A body governed by public law:
- (a) established for the specific purpose of meeting needs in the general interest
- (b) having legal personality; 
- (c) financed, for the most part by the State, or regional or local authorities. 

Additional information: 
Examples of Public Organisations are municipality, international public body, ministry, others.

WG Approval 28/04/2020</rdfs:comment>
      <skos:definition xml:lang="en">A body governed by public law:
- (a) established for the specific purpose of meeting needs in the general interest
- (b) having legal personality; 
- (c) financed, for the most part by the State, or regional or local authorities. 

Additional information: 
Examples of Public Organisations are municipality, international public body, ministry, others.

WG Approval 28/04/2020</skos:definition>
      <rdfs:isDefinedBy rdf:resource="http://data.europa.eu/a4g/ontology"/>
   </owl:Class>
   <owl:Class rdf:about="http://data.europa.eu/a4g/ontology#PurchaseContract">
      <rdfs:label xml:lang="en">Purchase contract</rdfs:label>
      <skos:prefLabel xml:lang="en">Purchase contract</skos:prefLabel>
      <rdfs:comment xml:lang="en">A contract resulting from a Dynamic Purchasing System or Framework Agreement Contract.</rdfs:comment>
      <skos:definition xml:lang="en">A contract resulting from a Dynamic Purchasing System or Framework Agreement Contract.</skos:definition>
      <rdfs:isDefinedBy rdf:resource="http://data.europa.eu/a4g/ontology"/>
   </owl:Class>
   <owl:Class rdf:about="http://data.europa.eu/a4g/ontology#Purpose">
      <rdfs:label xml:lang="en">Purpose</rdfs:label>
      <skos:prefLabel xml:lang="en">Purpose</skos:prefLabel>
      <rdfs:comment xml:lang="en">The description of the objectives related to a procurement. 

Additional information:

The description of the objectives includes the subject matter and quantities.


The quantification of the objectives related to a procurement.

To be re-reviewed by the WG the soonest.

(WG to be discussed, this was pointed out on the 09/04/2019 14:38:25 WG Meeting)

The old definition read as follows:

The description of the objectives related to a procurement.

(WG approval 05/12/2018)
</rdfs:comment>
      <skos:definition xml:lang="en">The description of the objectives related to a procurement. 

Additional information:

The description of the objectives includes the subject matter and quantities.


The quantification of the objectives related to a procurement.

To be re-reviewed by the WG the soonest.

(WG to be discussed, this was pointed out on the 09/04/2019 14:38:25 WG Meeting)

The old definition read as follows:

The description of the objectives related to a procurement.

(WG approval 05/12/2018)
</skos:definition>
      <rdfs:isDefinedBy rdf:resource="http://data.europa.eu/a4g/ontology"/>
   </owl:Class>
   <owl:Class rdf:about="http://data.europa.eu/a4g/ontology#RegulatoryFrameworkInformation">
      <rdfs:label xml:lang="en">Regulatory framework information</rdfs:label>
      <skos:prefLabel xml:lang="en">Regulatory framework information</skos:prefLabel>
      <rdfs:comment xml:lang="en">Legal information that governs specific aspects of the procedure.
Additional Information:
The legal information can concern tax regimes in a given country for example.
WG approval: 15/04/2021</rdfs:comment>
      <skos:definition xml:lang="en">Legal information that governs specific aspects of the procedure.
Additional Information:
The legal information can concern tax regimes in a given country for example.
WG approval: 15/04/2021</skos:definition>
      <rdfs:isDefinedBy rdf:resource="http://data.europa.eu/a4g/ontology"/>
   </owl:Class>
   <owl:Class rdf:about="http://data.europa.eu/a4g/ontology#RequestForParticipation">
      <rdfs:label xml:lang="en">Request for participation</rdfs:label>
      <skos:prefLabel xml:lang="en">Request for participation</skos:prefLabel>
      <rdfs:comment xml:lang="en">Application of an economic operator to be included in a procurement procedure.
WG approval: 20/04/2021</rdfs:comment>
      <skos:definition xml:lang="en">Application of an economic operator to be included in a procurement procedure.
WG approval: 20/04/2021</skos:definition>
      <rdfs:isDefinedBy rdf:resource="http://data.europa.eu/a4g/ontology"/>
   </owl:Class>
   <owl:Class rdf:about="http://data.europa.eu/a4g/ontology#ResourceElement">
      <rdfs:label xml:lang="en">Resource element</rdfs:label>
      <skos:prefLabel xml:lang="en">Resource element</skos:prefLabel>
      <rdfs:comment xml:lang="en">Reference to a semantic building block necessary to describe a specific concept. 

Addtional Information:

A building block may be a basic core component (e.g. Receipt Deadline, a property of type DateTime, in the class Submission Terms) or an aggregate component (e.g. Submission Terms, a class in the ontology).

WG Approval 23/05/2019</rdfs:comment>
      <skos:definition xml:lang="en">Reference to a semantic building block necessary to describe a specific concept. 

Addtional Information:

A building block may be a basic core component (e.g. Receipt Deadline, a property of type DateTime, in the class Submission Terms) or an aggregate component (e.g. Submission Terms, a class in the ontology).

WG Approval 23/05/2019</skos:definition>
      <rdfs:isDefinedBy rdf:resource="http://data.europa.eu/a4g/ontology"/>
   </owl:Class>
   <owl:Class rdf:about="http://data.europa.eu/a4g/ontology#Reviewer">
      <rdfs:label xml:lang="en">Reviewer</rdfs:label>
      <skos:prefLabel xml:lang="en">Reviewer</skos:prefLabel>
      <rdfs:comment xml:lang="en">Role of an agent who investigates the overall correctness of a procurement procedure, producing a related report.
Additional Information:
Any organisation or person may request a review of a procurement procedure.
WG approval: 20/04/2021</rdfs:comment>
      <skos:definition xml:lang="en">Role of an agent who investigates the overall correctness of a procurement procedure, producing a related report.
Additional Information:
Any organisation or person may request a review of a procurement procedure.
WG approval: 20/04/2021</skos:definition>
      <rdfs:isDefinedBy rdf:resource="http://data.europa.eu/a4g/ontology"/>
   </owl:Class>
   <owl:Class rdf:about="http://data.europa.eu/a4g/ontology#ReviewRequester">
      <rdfs:label xml:lang="en">Review requester</rdfs:label>
      <skos:prefLabel xml:lang="en">Review requester</skos:prefLabel>
      <rdfs:comment xml:lang="en">Role of an agent who requests the review of a (procurement) procedure.

WG Approval 23/10/2021</rdfs:comment>
      <skos:definition xml:lang="en">Role of an agent who requests the review of a (procurement) procedure.

WG Approval 23/10/2021</skos:definition>
      <rdfs:isDefinedBy rdf:resource="http://data.europa.eu/a4g/ontology"/>
   </owl:Class>
   <owl:Class rdf:about="http://data.europa.eu/a4g/ontology#ReviewTerm">
      <rdfs:label xml:lang="en">Review term</rdfs:label>
      <skos:prefLabel xml:lang="en">Review term</skos:prefLabel>
      <rdfs:comment xml:lang="en">Conditions and stipulations defining particularities of the review.

(WG approval 23/11/2018)
</rdfs:comment>
      <skos:definition xml:lang="en">Conditions and stipulations defining particularities of the review.

(WG approval 23/11/2018)
</skos:definition>
      <rdfs:isDefinedBy rdf:resource="http://data.europa.eu/a4g/ontology"/>
   </owl:Class>
   <owl:Class rdf:about="http://data.europa.eu/a4g/ontology#SecurityClearanceTerm">
      <rdfs:label xml:lang="en">Security clearance term</rdfs:label>
      <skos:prefLabel xml:lang="en">Security clearance term</skos:prefLabel>
      <rdfs:comment xml:lang="en">Status requested to individuals allowing them access to classified information (state or organisational secrets) or to restricted areas, after completion of a thorough background check.

WG Approval 2015-02-26
</rdfs:comment>
      <skos:definition xml:lang="en">Status requested to individuals allowing them access to classified information (state or organisational secrets) or to restricted areas, after completion of a thorough background check.

WG Approval 2015-02-26
</skos:definition>
      <rdfs:isDefinedBy rdf:resource="http://data.europa.eu/a4g/ontology"/>
   </owl:Class>
   <owl:Class rdf:about="http://data.europa.eu/a4g/ontology#SelectionCriterion">
      <rdfs:label xml:lang="en">Selection criterion</rdfs:label>
      <skos:prefLabel xml:lang="en">Selection criterion</skos:prefLabel>
      <rdfs:comment xml:lang="en">Describes a capacity requirement that the economic operator needs to fulfill to participate in the procedure.

WG approval 31/10/2018</rdfs:comment>
      <skos:definition xml:lang="en">Describes a capacity requirement that the economic operator needs to fulfill to participate in the procedure.

WG approval 31/10/2018</skos:definition>
      <rdfs:isDefinedBy rdf:resource="http://data.europa.eu/a4g/ontology"/>
   </owl:Class>
   <owl:Class rdf:about="http://data.europa.eu/a4g/ontology#SocialProcurement">
      <rdfs:label xml:lang="en">Social procurement</rdfs:label>
      <skos:prefLabel xml:lang="en">Social procurement</skos:prefLabel>
      <rdfs:comment xml:lang="en">An instance of the class SocialProcurement  is represented in eForms with the code "soc-obj" defined in the codelist strategic-procurement.


Research (21/01/2020): 
Socially responsible public procurement (SRPP):

‘SRPP’ means procurement operations that take into account one or more of the following social considerations: employment opportunities, decent work, compliance with social and labour rights, social inclusion (including persons with disabilities), equal opportunities, accessibility design for all, taking account of sustainability criteria, including ethical trade issues and wider voluntary compliance with corporate social responsibility (CSR), while observing the principles enshrined in the Treaty for the European Union (TFEU) and the Procurement Directives. 
Source: Buying Social - A Guide to Taking Account of Social Considerations in Public Procurement (Publications Office of the European Union, 2011) https://op.europa.eu/en/publication-detail/-/publication/cb70c481-0e29-4040-9be2-c408cddf081f/language-en
See Article 18 and Annex X Directive 2014/24.</rdfs:comment>
      <skos:definition xml:lang="en">An instance of the class SocialProcurement  is represented in eForms with the code "soc-obj" defined in the codelist strategic-procurement.


Research (21/01/2020): 
Socially responsible public procurement (SRPP):

‘SRPP’ means procurement operations that take into account one or more of the following social considerations: employment opportunities, decent work, compliance with social and labour rights, social inclusion (including persons with disabilities), equal opportunities, accessibility design for all, taking account of sustainability criteria, including ethical trade issues and wider voluntary compliance with corporate social responsibility (CSR), while observing the principles enshrined in the Treaty for the European Union (TFEU) and the Procurement Directives. 
Source: Buying Social - A Guide to Taking Account of Social Considerations in Public Procurement (Publications Office of the European Union, 2011) https://op.europa.eu/en/publication-detail/-/publication/cb70c481-0e29-4040-9be2-c408cddf081f/language-en
See Article 18 and Annex X Directive 2014/24.</skos:definition>
      <rdfs:isDefinedBy rdf:resource="http://data.europa.eu/a4g/ontology"/>
   </owl:Class>
   <owl:Class rdf:about="http://data.europa.eu/a4g/ontology#StatisticalInformation">
      <rdfs:label xml:lang="en">Statistical information</rdfs:label>
      <skos:prefLabel xml:lang="en">Statistical information</skos:prefLabel>
      <rdfs:comment xml:lang="en">Statistical data on the procedure and the lot. 

Additional Information

At the present time Procurement Procedures are not fully electronic. At a later date, information on the tenders received could be inferred by the data in the eProcurement system.
Therefore this class is temporal and should cease to exist in fully electronic procurement.
The need for its presence responds also to the alignment with the Regulation (EU) 2019/1780 (eForms).

Attention will have to be paid in the future to possible inconsistencies derived from data placed in other classes and data held in the Statistical Information class; e.g. the TenderEvaluation class (see eEvaluation diagram) has the attribute admissibileTender indicator, which in case of being false, may enter in contradiction with the highest or lowest tender value for that very same inadmissible tender.

WG Approval 12/12/2019
</rdfs:comment>
      <skos:definition xml:lang="en">Statistical data on the procedure and the lot. 

Additional Information

At the present time Procurement Procedures are not fully electronic. At a later date, information on the tenders received could be inferred by the data in the eProcurement system.
Therefore this class is temporal and should cease to exist in fully electronic procurement.
The need for its presence responds also to the alignment with the Regulation (EU) 2019/1780 (eForms).

Attention will have to be paid in the future to possible inconsistencies derived from data placed in other classes and data held in the Statistical Information class; e.g. the TenderEvaluation class (see eEvaluation diagram) has the attribute admissibileTender indicator, which in case of being false, may enter in contradiction with the highest or lowest tender value for that very same inadmissible tender.

WG Approval 12/12/2019
</skos:definition>
      <rdfs:isDefinedBy rdf:resource="http://data.europa.eu/a4g/ontology"/>
   </owl:Class>
   <owl:Class rdf:about="http://data.europa.eu/a4g/ontology#RequestForClarification">
      <rdfs:label xml:lang="en">Request for clarification</rdfs:label>
      <skos:prefLabel xml:lang="en">Request for clarification</skos:prefLabel>
      <rdfs:comment xml:lang="en">A demand for elucidation of received information.
Additional Information:  
Requests for clarification are usually used by buyers during the process of award or evaluation to understand specific aspects of the tender without altering the tender.
WG approval 20/04/2021</rdfs:comment>
      <skos:definition xml:lang="en">A demand for elucidation of received information.
Additional Information:  
Requests for clarification are usually used by buyers during the process of award or evaluation to understand specific aspects of the tender without altering the tender.
WG approval 20/04/2021</skos:definition>
      <rdfs:isDefinedBy rdf:resource="http://data.europa.eu/a4g/ontology"/>
   </owl:Class>
   <owl:Class rdf:about="http://data.europa.eu/a4g/ontology#StrategicProcurement">
      <rdfs:label xml:lang="en">Strategic procurement</rdfs:label>
      <skos:prefLabel xml:lang="en">Strategic procurement</skos:prefLabel>
      <rdfs:comment xml:lang="en">Public procurement that contributes to achieving pressing policy goals.

Additional Information:
Specific strategic goals could be, for example, environmental protection, innovation, job creation and the development of small and medium enterprises.

Based on https://legalinstruments.oecd.org/en/instruments/OECD-LEGAL-0411 (see paragraph on "background information".

WG Approval 10/03/2020</rdfs:comment>
      <skos:definition xml:lang="en">Public procurement that contributes to achieving pressing policy goals.

Additional Information:
Specific strategic goals could be, for example, environmental protection, innovation, job creation and the development of small and medium enterprises.

Based on https://legalinstruments.oecd.org/en/instruments/OECD-LEGAL-0411 (see paragraph on "background information".

WG Approval 10/03/2020</skos:definition>
      <rdfs:isDefinedBy rdf:resource="http://data.europa.eu/a4g/ontology"/>
   </owl:Class>
   <owl:Class rdf:about="http://data.europa.eu/a4g/ontology#Subcontract">
      <rdfs:label xml:lang="en">Subcontract</rdfs:label>
      <skos:prefLabel xml:lang="en">Subcontract</skos:prefLabel>
      <rdfs:comment xml:lang="en">A contract between a contractor of an original contract and another economic operator to fulfil the original contract.

WG Approval 07/05/2019</rdfs:comment>
      <skos:definition xml:lang="en">A contract between a contractor of an original contract and another economic operator to fulfil the original contract.

WG Approval 07/05/2019</skos:definition>
      <rdfs:isDefinedBy rdf:resource="http://data.europa.eu/a4g/ontology"/>
   </owl:Class>
   <owl:Class rdf:about="http://data.europa.eu/a4g/ontology#Subcontractor">
      <rdfs:label xml:lang="en">Subcontractor</rdfs:label>
      <skos:prefLabel xml:lang="en">Subcontractor</skos:prefLabel>
      <rdfs:comment xml:lang="en">A role of an agent that has an agreement to perform part or all of the obligations of another agents's contract. 
Additional information
For some procedures, the subcontractor signs as well the contract between the buyer and the contractor.

At tendering time, entities relied upon by the economic operators can be subcontractors or not. 

When modelling ESPD we well analyse whether we need or not a role named "relied upon".

WG approval 05/08/2021
</rdfs:comment>
      <skos:definition xml:lang="en">A role of an agent that has an agreement to perform part or all of the obligations of another agents's contract. 
Additional information
For some procedures, the subcontractor signs as well the contract between the buyer and the contractor.

At tendering time, entities relied upon by the economic operators can be subcontractors or not. 

When modelling ESPD we well analyse whether we need or not a role named "relied upon".

WG approval 05/08/2021
</skos:definition>
      <rdfs:isDefinedBy rdf:resource="http://data.europa.eu/a4g/ontology"/>
   </owl:Class>
   <owl:Class rdf:about="http://data.europa.eu/a4g/ontology#SubcontractTerm">
      <rdfs:label xml:lang="en">Subcontract term</rdfs:label>
      <skos:prefLabel xml:lang="en">Subcontract term</skos:prefLabel>
      <rdfs:comment xml:lang="en">A concept to describe the main information regarding the share of parts of the contract to third parties.</rdfs:comment>
      <skos:definition xml:lang="en">A concept to describe the main information regarding the share of parts of the contract to third parties.</skos:definition>
      <rdfs:isDefinedBy rdf:resource="http://data.europa.eu/a4g/ontology"/>
   </owl:Class>
   <owl:Class rdf:about="http://data.europa.eu/a4g/ontology#SubmissionTerm">
      <rdfs:label xml:lang="en">Submission term</rdfs:label>
      <skos:prefLabel xml:lang="en">Submission term</skos:prefLabel>
      <rdfs:comment xml:lang="en">Conditions and stipulations defining particularities of submitting documents to the buyer

Additional Information: 

These documents can be tenders, request to participate and expressions of interest.

WG Approval 14/07/2020</rdfs:comment>
      <skos:definition xml:lang="en">Conditions and stipulations defining particularities of submitting documents to the buyer

Additional Information: 

These documents can be tenders, request to participate and expressions of interest.

WG Approval 14/07/2020</skos:definition>
      <rdfs:isDefinedBy rdf:resource="http://data.europa.eu/a4g/ontology"/>
   </owl:Class>
   <owl:Class rdf:about="http://data.europa.eu/a4g/ontology#System">
      <rdfs:label xml:lang="en">System</rdfs:label>
      <skos:prefLabel xml:lang="en">System</skos:prefLabel>
      <rdfs:comment xml:lang="en">Software application used for performing procurement activities. 

WG Approval 28/04/2020

</rdfs:comment>
      <skos:definition xml:lang="en">Software application used for performing procurement activities. 

WG Approval 28/04/2020

</skos:definition>
      <rdfs:isDefinedBy rdf:resource="http://data.europa.eu/a4g/ontology"/>
   </owl:Class>
   <owl:Class rdf:about="http://data.europa.eu/a4g/ontology#TechnicalSpecification">
      <rdfs:label xml:lang="en">Technical specification</rdfs:label>
      <skos:prefLabel xml:lang="en">Technical specification</skos:prefLabel>
      <rdfs:comment xml:lang="en">A set of documented requirements applicable to the object of the procurement.
Additional Information: 
A specification often includes technical standards.
WG approval: 20/04/2021</rdfs:comment>
      <skos:definition xml:lang="en">A set of documented requirements applicable to the object of the procurement.
Additional Information: 
A specification often includes technical standards.
WG approval: 20/04/2021</skos:definition>
      <rdfs:isDefinedBy rdf:resource="http://data.europa.eu/a4g/ontology"/>
   </owl:Class>
   <owl:Class rdf:about="http://data.europa.eu/a4g/ontology#Technique">
      <rdfs:label xml:lang="en">Technique</rdfs:label>
      <skos:prefLabel xml:lang="en">Technique</skos:prefLabel>
      <rdfs:comment xml:lang="en">Methods used for conducting procurement procedure.

Addtional information:

Several techniques can be combined in one single procurement procedure (e.g. eAuction can be carried out in a Framework Agreement or DPS).

WG Approval 19/09/2019 
</rdfs:comment>
      <skos:definition xml:lang="en">Methods used for conducting procurement procedure.

Addtional information:

Several techniques can be combined in one single procurement procedure (e.g. eAuction can be carried out in a Framework Agreement or DPS).

WG Approval 19/09/2019 
</skos:definition>
      <rdfs:isDefinedBy rdf:resource="http://data.europa.eu/a4g/ontology"/>
   </owl:Class>
   <owl:Class rdf:about="http://data.europa.eu/a4g/ontology#Tender">
      <rdfs:label xml:lang="en">Tender</rdfs:label>
      <skos:prefLabel xml:lang="en">Tender</skos:prefLabel>
      <rdfs:comment xml:lang="en">A unique identifier of the instance of the concept.

Additional Information

For example, in the case of the Procurement Identifier, this could be the European Public Procurement Identifier, and/or any other identifier provided by the buyer, the service provider or any other stakeholder.

WG Approval 12/11/2019
</rdfs:comment>
      <skos:definition xml:lang="en">A unique identifier of the instance of the concept.

Additional Information

For example, in the case of the Procurement Identifier, this could be the European Public Procurement Identifier, and/or any other identifier provided by the buyer, the service provider or any other stakeholder.

WG Approval 12/11/2019
</skos:definition>
      <rdfs:isDefinedBy rdf:resource="http://data.europa.eu/a4g/ontology"/>
   </owl:Class>
   <owl:Class rdf:about="http://data.europa.eu/a4g/ontology#TenderDocument">
      <rdfs:label xml:lang="en">Tender document</rdfs:label>
      <skos:prefLabel xml:lang="en">Tender document</skos:prefLabel>
      <rdfs:comment xml:lang="en">Document that is part of the tender.
WG approval 22/04/2021</rdfs:comment>
      <skos:definition xml:lang="en">Document that is part of the tender.
WG approval 22/04/2021</skos:definition>
      <rdfs:isDefinedBy rdf:resource="http://data.europa.eu/a4g/ontology"/>
   </owl:Class>
   <owl:Class rdf:about="http://data.europa.eu/a4g/ontology#Tenderer">
      <rdfs:label xml:lang="en">Tenderer</rdfs:label>
      <skos:prefLabel xml:lang="en">Tenderer</skos:prefLabel>
      <rdfs:comment xml:lang="en">A role of an agent that has submitted a tender.

Additional Information:
A tenderer is an economic operator or group of economic operators that has submitted a tender.
WG approval 05/08/2021</rdfs:comment>
      <skos:definition xml:lang="en">A role of an agent that has submitted a tender.

Additional Information:
A tenderer is an economic operator or group of economic operators that has submitted a tender.
WG approval 05/08/2021</skos:definition>
      <rdfs:isDefinedBy rdf:resource="http://data.europa.eu/a4g/ontology"/>
   </owl:Class>
   <owl:Class rdf:about="http://data.europa.eu/a4g/ontology#TenderLot">
      <rdfs:label xml:lang="en">Tender lot</rdfs:label>
      <skos:prefLabel xml:lang="en">Tender lot</skos:prefLabel>
      <rdfs:comment xml:lang="en">Information submitted by the economic operator to specify its offer regarding one or more lots or the whole procedure, in response to the call for tender.

(WG approval 07/11/2018)



</rdfs:comment>
      <skos:definition xml:lang="en">Information submitted by the economic operator to specify its offer regarding one or more lots or the whole procedure, in response to the call for tender.

(WG approval 07/11/2018)



</skos:definition>
      <rdfs:isDefinedBy rdf:resource="http://data.europa.eu/a4g/ontology"/>
   </owl:Class>
   <owl:Class rdf:about="http://data.europa.eu/a4g/ontology#TenderLotEvaluationRank">
      <rdfs:label xml:lang="en">Tender lot evaluation rank</rdfs:label>
      <skos:prefLabel xml:lang="en">Tender lot evaluation rank</skos:prefLabel>
      <rdfs:comment xml:lang="en">The position of the Tender Lot in relation to other Tender Lots (i.e. first, second, third, etc.).

Additional information: This is specially the case of design contests, some framework agreements with multiple winners (e.g. cascades) or innovation partnerships.

In multi-staged procedures this may be used for ranking the Tender Lots to be evaluated for further stages.

WG Approval 19/12/2019

</rdfs:comment>
      <skos:definition xml:lang="en">The position of the Tender Lot in relation to other Tender Lots (i.e. first, second, third, etc.).

Additional information: This is specially the case of design contests, some framework agreements with multiple winners (e.g. cascades) or innovation partnerships.

In multi-staged procedures this may be used for ranking the Tender Lots to be evaluated for further stages.

WG Approval 19/12/2019

</skos:definition>
      <rdfs:isDefinedBy rdf:resource="http://data.europa.eu/a4g/ontology"/>
   </owl:Class>
   <owl:Class rdf:about="http://data.europa.eu/a4g/ontology#Value">
      <rdfs:label xml:lang="en">Value</rdfs:label>
      <skos:prefLabel xml:lang="en">Value</skos:prefLabel>
      <rdfs:comment xml:lang="en">Post-poned until  discussion on lots values and amounts.
WG approval 22/04/2021</rdfs:comment>
      <skos:definition xml:lang="en">Post-poned until  discussion on lots values and amounts.
WG approval 22/04/2021</skos:definition>
      <rdfs:isDefinedBy rdf:resource="http://data.europa.eu/a4g/ontology"/>
   </owl:Class>
   <owl:Class rdf:about="http://data.europa.eu/a4g/ontology#VoluntaryEx-anteTransparencyNotice">
      <rdfs:label xml:lang="en">Voluntary ex-ante transparency notice</rdfs:label>
      <skos:prefLabel xml:lang="en">Voluntary ex-ante transparency notice</skos:prefLabel>
      <rdfs:comment xml:lang="en">A notice informing of the intention to award  a contract without prior publication of a contract notice.
 
Additional Information:
 
For European notices above the threshold
 
"A means of advertising the intention to award the contract without opening it up to formal competition. A contracting authority may decide that a contract does not require prior publication through a contract notice in the O.J.E.U. A reason for this decision may be that the contract meets the exceptional conditions described in Article 31 of Directive 2004/18/EC. In a recent V.E.A.T notice the reason was listed as “extreme urgency brought about by events unforeseeable by the contracting entity and in accordance with the strict conditions stated in the Directive” .
"Voluntary Ex-Ante Transparency Notice" (VEAT) where a contracting authority deems that a contract does not require prior publication of a contract notice in the European Journal (OJEU). This may apply, for example, if the contract meets the exceptional conditions justifying direct award of contracts.
 
&lt;b&gt;This definition is still to be worked on.&lt;/b&gt;</rdfs:comment>
      <skos:definition xml:lang="en">A notice informing of the intention to award  a contract without prior publication of a contract notice.
 
Additional Information:
 
For European notices above the threshold
 
"A means of advertising the intention to award the contract without opening it up to formal competition. A contracting authority may decide that a contract does not require prior publication through a contract notice in the O.J.E.U. A reason for this decision may be that the contract meets the exceptional conditions described in Article 31 of Directive 2004/18/EC. In a recent V.E.A.T notice the reason was listed as “extreme urgency brought about by events unforeseeable by the contracting entity and in accordance with the strict conditions stated in the Directive” .
"Voluntary Ex-Ante Transparency Notice" (VEAT) where a contracting authority deems that a contract does not require prior publication of a contract notice in the European Journal (OJEU). This may apply, for example, if the contract meets the exceptional conditions justifying direct award of contracts.
 
&lt;b&gt;This definition is still to be worked on.&lt;/b&gt;</skos:definition>
      <rdfs:isDefinedBy rdf:resource="http://data.europa.eu/a4g/ontology"/>
   </owl:Class>
   <owl:Class rdf:about="http://data.europa.eu/a4g/ontology#Winner">
      <rdfs:label xml:lang="en">Winner</rdfs:label>
      <skos:prefLabel xml:lang="en">Winner</skos:prefLabel>
      <rdfs:comment xml:lang="en">A role of an agent to whom a lot is awarded.
WG approval 05/08/2021 (revised 26/10/2021)</rdfs:comment>
      <skos:definition xml:lang="en">A role of an agent to whom a lot is awarded.
WG approval 05/08/2021 (revised 26/10/2021)</skos:definition>
      <rdfs:isDefinedBy rdf:resource="http://data.europa.eu/a4g/ontology"/>
   </owl:Class>
   <owl:Class rdf:about="http://unknown.domain/for/prefix#Address">
      <rdfs:label xml:lang="en">Address</rdfs:label>
      <skos:prefLabel xml:lang="en">Address</skos:prefLabel>
      <rdfs:comment xml:lang="en">The particulars of the place where a person or an organisation is located.

WG Approval 28/04/2020

Additional Information:
An "address representation" as conceptually defined by the INSPIRE Address Representation data type: "Representation of an address spatial object for use in external application schemas that need to include the basic, address information in a readable way.".


The representation of Addresses varies widely from one country's postal system to another. Even within countries, there are almost always examples of Addresses that do not conform to the stated national standard. At the time of publication, work is progressing on ISO 19160-1 that defines a method through which different Addresses can be converted from one conceptual model to another.


This specification was heavily based on the INSPIRE Address Representation data type. It is noteworthy that if an Address is provided using the detailed breakdown suggested by the properties for this class, then it will be INSPIRE-conformant. To this very granular set of properties, we add two further properties:

- full address (the complete address as a formatted string)
- addressID (a unique identifier for the address)
The first of these allows publishers to simply provide the complete Address as one string, with or without formatting. This is analogous to vCard's label property.

The addressID is part of the INSPIRE guidelines and provides a hook that can be used to link the Address to an alternative representation, such as vCard or OASIS xAL.</rdfs:comment>
      <skos:definition xml:lang="en">The particulars of the place where a person or an organisation is located.

WG Approval 28/04/2020

Additional Information:
An "address representation" as conceptually defined by the INSPIRE Address Representation data type: "Representation of an address spatial object for use in external application schemas that need to include the basic, address information in a readable way.".


The representation of Addresses varies widely from one country's postal system to another. Even within countries, there are almost always examples of Addresses that do not conform to the stated national standard. At the time of publication, work is progressing on ISO 19160-1 that defines a method through which different Addresses can be converted from one conceptual model to another.


This specification was heavily based on the INSPIRE Address Representation data type. It is noteworthy that if an Address is provided using the detailed breakdown suggested by the properties for this class, then it will be INSPIRE-conformant. To this very granular set of properties, we add two further properties:

- full address (the complete address as a formatted string)
- addressID (a unique identifier for the address)
The first of these allows publishers to simply provide the complete Address as one string, with or without formatting. This is analogous to vCard's label property.

The addressID is part of the INSPIRE guidelines and provides a hook that can be used to link the Address to an alternative representation, such as vCard or OASIS xAL.</skos:definition>
   </owl:Class>
   <owl:Class rdf:about="http://unknown.domain/for/prefix#Geometry">
      <rdfs:label xml:lang="en">Geometry</rdfs:label>
      <skos:prefLabel xml:lang="en">Geometry</skos:prefLabel>
      <rdfs:comment xml:lang="en">The Geometry class provides the means to identify a Location as a point, line, polygon, etc. expressed using coordinates in some coordinate reference system.

Additional Information:
This class defines the notion of "geometry" at the conceptual level, and it shall be encoded by using different formats (see usage note of the locn:geometry property). We also refer to the Examples section of this specification for a number of different geometry examples expressed in different formats.</rdfs:comment>
      <skos:definition xml:lang="en">The Geometry class provides the means to identify a Location as a point, line, polygon, etc. expressed using coordinates in some coordinate reference system.

Additional Information:
This class defines the notion of "geometry" at the conceptual level, and it shall be encoded by using different formats (see usage note of the locn:geometry property). We also refer to the Examples section of this specification for a number of different geometry examples expressed in different formats.</skos:definition>
   </owl:Class>
   <owl:Class rdf:about="http://data.europa.eu/a4g/ontology#Amount">
      <rdfs:label xml:lang="en">Amount</rdfs:label>
      <skos:prefLabel xml:lang="en">Amount</skos:prefLabel>
      <rdfs:comment xml:lang="en">A number of monetary units specified using a given unit of currency.
WG approval 13/04/2021</rdfs:comment>
      <skos:definition xml:lang="en">A number of monetary units specified using a given unit of currency.
WG approval 13/04/2021</skos:definition>
      <rdfs:isDefinedBy rdf:resource="http://data.europa.eu/a4g/ontology"/>
   </owl:Class>
   <owl:Class rdf:about="http://data.europa.eu/a4g/ontology#Identifier">
      <rdfs:label xml:lang="en">Identifier</rdfs:label>
      <skos:prefLabel xml:lang="en">Identifier</skos:prefLabel>
      <rdfs:comment xml:lang="en">A character string to identify and distinguish uniquely, one instance of an object in an identification scheme from all other objects in the same scheme together with relevant supplementary information.
</rdfs:comment>
      <skos:definition xml:lang="en">A character string to identify and distinguish uniquely, one instance of an object in an identification scheme from all other objects in the same scheme together with relevant supplementary information.
</skos:definition>
      <rdfs:isDefinedBy rdf:resource="http://data.europa.eu/a4g/ontology"/>
   </owl:Class>
   <owl:Class rdf:about="http://data.europa.eu/a4g/ontology#Measure">
      <rdfs:label xml:lang="en">Measure</rdfs:label>
      <skos:prefLabel xml:lang="en">Measure</skos:prefLabel>
      <rdfs:comment xml:lang="en">A numeric value determined by measuring an object along with the specified unit of measure.
</rdfs:comment>
      <skos:definition xml:lang="en">A numeric value determined by measuring an object along with the specified unit of measure.
</skos:definition>
      <rdfs:isDefinedBy rdf:resource="http://data.europa.eu/a4g/ontology"/>
   </owl:Class>
   <owl:Class rdf:about="http://data.europa.eu/a4g/ontology#Quantity">
      <rdfs:label xml:lang="en">Quantity</rdfs:label>
      <skos:prefLabel xml:lang="en">Quantity</skos:prefLabel>
      <rdfs:comment xml:lang="en">A counted number of non-monetary units possibly including fractions.
</rdfs:comment>
      <skos:definition xml:lang="en">A counted number of non-monetary units possibly including fractions.
</skos:definition>
      <rdfs:isDefinedBy rdf:resource="http://data.europa.eu/a4g/ontology"/>
   </owl:Class>
   <owl:ObjectProperty rdf:about="http://data.europa.eu/a4g/ontology#leadOf">
      <rdfs:subPropertyOf rdf:resource="http://data.europa.eu/a4g/ontology#isMemberOf"/>
   </owl:ObjectProperty>
   <owl:ObjectProperty rdf:about="http://data.europa.eu/a4g/ontology#notifies">
      <rdfs:subPropertyOf rdf:resource="http://data.europa.eu/a4g/ontology#relatesTo"/>
   </owl:ObjectProperty>
   <owl:Class rdf:about="http://data.europa.eu/a4g/ontology#AcquiringCentralPurchasingBody">
      <rdfs:subClassOf rdf:resource="http://data.europa.eu/a4g/ontology#CentralPurchasingBody"/>
   </owl:Class>
   <rdf:Description rdf:about="http://data.europa.eu/a4g/ontology#AcquiringCentralPurchasingBody">
      <owl:disjointWith rdf:resource="http://data.europa.eu/a4g/ontology#AwardingCentralPurchasingBody"/>
   </rdf:Description>
   <owl:Class rdf:about="http://data.europa.eu/a4g/ontology#Organisation">
      <rdfs:subClassOf rdf:resource="http://data.europa.eu/a4g/ontology#Agent"/>
   </owl:Class>
   <rdf:Description rdf:about="http://data.europa.eu/a4g/ontology#Organisation">
      <owl:disjointWith rdf:resource="http://data.europa.eu/a4g/ontology#System"/>
   </rdf:Description>
   <rdf:Description rdf:about="http://data.europa.eu/a4g/ontology#Organisation">
      <owl:disjointWith rdf:resource="http://data.europa.eu/a4g/ontology#Person"/>
   </rdf:Description>
   <owl:Class rdf:about="http://data.europa.eu/a4g/ontology#System">
      <rdfs:subClassOf rdf:resource="http://data.europa.eu/a4g/ontology#Agent"/>
   </owl:Class>
   <rdf:Description rdf:about="http://data.europa.eu/a4g/ontology#System">
      <owl:disjointWith rdf:resource="http://data.europa.eu/a4g/ontology#Organisation"/>
   </rdf:Description>
   <rdf:Description rdf:about="http://data.europa.eu/a4g/ontology#System">
      <owl:disjointWith rdf:resource="http://data.europa.eu/a4g/ontology#Person"/>
   </rdf:Description>
   <owl:Class rdf:about="http://data.europa.eu/a4g/ontology#Person">
      <rdfs:subClassOf rdf:resource="http://data.europa.eu/a4g/ontology#Agent"/>
   </owl:Class>
   <rdf:Description rdf:about="http://data.europa.eu/a4g/ontology#Person">
      <owl:disjointWith rdf:resource="http://data.europa.eu/a4g/ontology#Organisation"/>
   </rdf:Description>
   <rdf:Description rdf:about="http://data.europa.eu/a4g/ontology#Person">
      <owl:disjointWith rdf:resource="http://data.europa.eu/a4g/ontology#System"/>
   </rdf:Description>
   <owl:Class rdf:about="http://data.europa.eu/a4g/ontology#AwardCriterion">
      <rdfs:subClassOf rdf:resource="http://data.europa.eu/a4g/ontology#ProcurementCriterion"/>
   </owl:Class>
   <rdf:Description rdf:about="http://data.europa.eu/a4g/ontology#AwardCriterion">
      <owl:disjointWith rdf:resource="http://data.europa.eu/a4g/ontology#ExclusionGround"/>
   </rdf:Description>
   <rdf:Description rdf:about="http://data.europa.eu/a4g/ontology#AwardCriterion">
      <owl:disjointWith rdf:resource="http://data.europa.eu/a4g/ontology#SelectionCriterion"/>
   </rdf:Description>
   <owl:Class rdf:about="http://data.europa.eu/a4g/ontology#AwardingCentralPurchasingBody">
      <rdfs:subClassOf rdf:resource="http://data.europa.eu/a4g/ontology#CentralPurchasingBody"/>
   </owl:Class>
   <rdf:Description rdf:about="http://data.europa.eu/a4g/ontology#AwardingCentralPurchasingBody">
      <owl:disjointWith rdf:resource="http://data.europa.eu/a4g/ontology#AcquiringCentralPurchasingBody"/>
   </rdf:Description>
   <owl:Class rdf:about="http://data.europa.eu/a4g/ontology#Business">
      <rdfs:subClassOf rdf:resource="http://data.europa.eu/a4g/ontology#Organisation"/>
   </owl:Class>
   <rdf:Description rdf:about="http://data.europa.eu/a4g/ontology#Business">
      <owl:disjointWith rdf:resource="http://data.europa.eu/a4g/ontology#OrganisationGroup"/>
   </rdf:Description>
   <rdf:Description rdf:about="http://data.europa.eu/a4g/ontology#Business">
      <owl:disjointWith rdf:resource="http://data.europa.eu/a4g/ontology#PublicOrganisation"/>
   </rdf:Description>
   <owl:Class rdf:about="http://data.europa.eu/a4g/ontology#Buyer">
      <rdfs:subClassOf rdf:resource="http://data.europa.eu/a4g/ontology#ProcurementRole"/>
   </owl:Class>
   <rdf:Description rdf:about="http://data.europa.eu/a4g/ontology#Buyer">
      <owl:disjointWith rdf:resource="http://data.europa.eu/a4g/ontology#CatalogueProvider"/>
   </rdf:Description>
   <rdf:Description rdf:about="http://data.europa.eu/a4g/ontology#Buyer">
      <owl:disjointWith rdf:resource="http://data.europa.eu/a4g/ontology#CatalogueReceiver"/>
   </rdf:Description>
   <rdf:Description rdf:about="http://data.europa.eu/a4g/ontology#Buyer">
      <owl:disjointWith rdf:resource="http://data.europa.eu/a4g/ontology#EconomicOperator"/>
   </rdf:Description>
   <rdf:Description rdf:about="http://data.europa.eu/a4g/ontology#Buyer">
      <owl:disjointWith rdf:resource="http://data.europa.eu/a4g/ontology#Mediator"/>
   </rdf:Description>
   <rdf:Description rdf:about="http://data.europa.eu/a4g/ontology#Buyer">
      <owl:disjointWith rdf:resource="http://data.europa.eu/a4g/ontology#ProcurementServiceProvider"/>
   </rdf:Description>
   <rdf:Description rdf:about="http://data.europa.eu/a4g/ontology#Buyer">
      <owl:disjointWith rdf:resource="http://data.europa.eu/a4g/ontology#Reviewer"/>
   </rdf:Description>
   <rdf:Description rdf:about="http://data.europa.eu/a4g/ontology#Buyer">
      <owl:disjointWith rdf:resource="http://data.europa.eu/a4g/ontology#ReviewRequester"/>
   </rdf:Description>
   <owl:Class rdf:about="http://data.europa.eu/a4g/ontology#CentralPurchasingBody">
      <rdfs:subClassOf rdf:resource="http://data.europa.eu/a4g/ontology#Buyer"/>
   </owl:Class>
   <owl:Class rdf:about="http://data.europa.eu/a4g/ontology#BuyerProfileNotice">
      <rdfs:subClassOf rdf:resource="http://data.europa.eu/a4g/ontology#Notice"/>
   </owl:Class>
   <rdf:Description rdf:about="http://data.europa.eu/a4g/ontology#BuyerProfileNotice">
      <owl:disjointWith rdf:resource="http://data.europa.eu/a4g/ontology#CallForExpressionOfInterest"/>
   </rdf:Description>
   <rdf:Description rdf:about="http://data.europa.eu/a4g/ontology#BuyerProfileNotice">
      <owl:disjointWith rdf:resource="http://data.europa.eu/a4g/ontology#ContractAwardNotice"/>
   </rdf:Description>
   <rdf:Description rdf:about="http://data.europa.eu/a4g/ontology#BuyerProfileNotice">
      <owl:disjointWith rdf:resource="http://data.europa.eu/a4g/ontology#ContractModificationNotice"/>
   </rdf:Description>
   <rdf:Description rdf:about="http://data.europa.eu/a4g/ontology#BuyerProfileNotice">
      <owl:disjointWith rdf:resource="http://data.europa.eu/a4g/ontology#ContractNotice"/>
   </rdf:Description>
   <rdf:Description rdf:about="http://data.europa.eu/a4g/ontology#BuyerProfileNotice">
      <owl:disjointWith rdf:resource="http://data.europa.eu/a4g/ontology#PriorInformationNotice"/>
   </rdf:Description>
   <rdf:Description rdf:about="http://data.europa.eu/a4g/ontology#BuyerProfileNotice">
      <owl:disjointWith rdf:resource="http://data.europa.eu/a4g/ontology#VoluntaryEx-anteTransparencyNotice"/>
   </rdf:Description>
   <owl:Class rdf:about="http://data.europa.eu/a4g/ontology#CallForCompetition">
      <rdfs:subClassOf rdf:resource="http://data.europa.eu/a4g/ontology#ProcurementDocument"/>
   </owl:Class>
   <rdf:Description rdf:about="http://data.europa.eu/a4g/ontology#CallForCompetition">
      <owl:disjointWith rdf:resource="http://data.europa.eu/a4g/ontology#TechnicalSpecification"/>
   </rdf:Description>
   <owl:Class rdf:about="http://data.europa.eu/a4g/ontology#CallForExpressionOfInterest">
      <rdfs:subClassOf rdf:resource="http://data.europa.eu/a4g/ontology#Notice"/>
   </owl:Class>
   <rdf:Description rdf:about="http://data.europa.eu/a4g/ontology#CallForExpressionOfInterest">
      <owl:disjointWith rdf:resource="http://data.europa.eu/a4g/ontology#BuyerProfileNotice"/>
   </rdf:Description>
   <rdf:Description rdf:about="http://data.europa.eu/a4g/ontology#CallForExpressionOfInterest">
      <owl:disjointWith rdf:resource="http://data.europa.eu/a4g/ontology#ContractAwardNotice"/>
   </rdf:Description>
   <rdf:Description rdf:about="http://data.europa.eu/a4g/ontology#CallForExpressionOfInterest">
      <owl:disjointWith rdf:resource="http://data.europa.eu/a4g/ontology#ContractModificationNotice"/>
   </rdf:Description>
   <rdf:Description rdf:about="http://data.europa.eu/a4g/ontology#CallForExpressionOfInterest">
      <owl:disjointWith rdf:resource="http://data.europa.eu/a4g/ontology#ContractNotice"/>
   </rdf:Description>
   <rdf:Description rdf:about="http://data.europa.eu/a4g/ontology#CallForExpressionOfInterest">
      <owl:disjointWith rdf:resource="http://data.europa.eu/a4g/ontology#PriorInformationNotice"/>
   </rdf:Description>
   <rdf:Description rdf:about="http://data.europa.eu/a4g/ontology#CallForExpressionOfInterest">
      <owl:disjointWith rdf:resource="http://data.europa.eu/a4g/ontology#VoluntaryEx-anteTransparencyNotice"/>
   </rdf:Description>
   <owl:Class rdf:about="http://data.europa.eu/a4g/ontology#CatalogueProvider">
      <rdfs:subClassOf rdf:resource="http://data.europa.eu/a4g/ontology#ProcurementRole"/>
   </owl:Class>
   <rdf:Description rdf:about="http://data.europa.eu/a4g/ontology#CatalogueProvider">
      <owl:disjointWith rdf:resource="http://data.europa.eu/a4g/ontology#Buyer"/>
   </rdf:Description>
   <rdf:Description rdf:about="http://data.europa.eu/a4g/ontology#CatalogueProvider">
      <owl:disjointWith rdf:resource="http://data.europa.eu/a4g/ontology#CatalogueReceiver"/>
   </rdf:Description>
   <rdf:Description rdf:about="http://data.europa.eu/a4g/ontology#CatalogueProvider">
      <owl:disjointWith rdf:resource="http://data.europa.eu/a4g/ontology#EconomicOperator"/>
   </rdf:Description>
   <rdf:Description rdf:about="http://data.europa.eu/a4g/ontology#CatalogueProvider">
      <owl:disjointWith rdf:resource="http://data.europa.eu/a4g/ontology#Mediator"/>
   </rdf:Description>
   <rdf:Description rdf:about="http://data.europa.eu/a4g/ontology#CatalogueProvider">
      <owl:disjointWith rdf:resource="http://data.europa.eu/a4g/ontology#ProcurementServiceProvider"/>
   </rdf:Description>
   <rdf:Description rdf:about="http://data.europa.eu/a4g/ontology#CatalogueProvider">
      <owl:disjointWith rdf:resource="http://data.europa.eu/a4g/ontology#Reviewer"/>
   </rdf:Description>
   <rdf:Description rdf:about="http://data.europa.eu/a4g/ontology#CatalogueProvider">
      <owl:disjointWith rdf:resource="http://data.europa.eu/a4g/ontology#ReviewRequester"/>
   </rdf:Description>
   <owl:Class rdf:about="http://data.europa.eu/a4g/ontology#CatalogueReceiver">
      <rdfs:subClassOf rdf:resource="http://data.europa.eu/a4g/ontology#ProcurementRole"/>
   </owl:Class>
   <rdf:Description rdf:about="http://data.europa.eu/a4g/ontology#CatalogueReceiver">
      <owl:disjointWith rdf:resource="http://data.europa.eu/a4g/ontology#Buyer"/>
   </rdf:Description>
   <rdf:Description rdf:about="http://data.europa.eu/a4g/ontology#CatalogueReceiver">
      <owl:disjointWith rdf:resource="http://data.europa.eu/a4g/ontology#CatalogueProvider"/>
   </rdf:Description>
   <rdf:Description rdf:about="http://data.europa.eu/a4g/ontology#CatalogueReceiver">
      <owl:disjointWith rdf:resource="http://data.europa.eu/a4g/ontology#EconomicOperator"/>
   </rdf:Description>
   <rdf:Description rdf:about="http://data.europa.eu/a4g/ontology#CatalogueReceiver">
      <owl:disjointWith rdf:resource="http://data.europa.eu/a4g/ontology#Mediator"/>
   </rdf:Description>
   <rdf:Description rdf:about="http://data.europa.eu/a4g/ontology#CatalogueReceiver">
      <owl:disjointWith rdf:resource="http://data.europa.eu/a4g/ontology#ProcurementServiceProvider"/>
   </rdf:Description>
   <rdf:Description rdf:about="http://data.europa.eu/a4g/ontology#CatalogueReceiver">
      <owl:disjointWith rdf:resource="http://data.europa.eu/a4g/ontology#Reviewer"/>
   </rdf:Description>
   <rdf:Description rdf:about="http://data.europa.eu/a4g/ontology#CatalogueReceiver">
      <owl:disjointWith rdf:resource="http://data.europa.eu/a4g/ontology#ReviewRequester"/>
   </rdf:Description>
   <owl:Class rdf:about="http://data.europa.eu/a4g/ontology#Contract">
      <rdfs:subClassOf rdf:resource="http://data.europa.eu/a4g/ontology#Document"/>
   </owl:Class>
   <rdf:Description rdf:about="http://data.europa.eu/a4g/ontology#Contract">
      <owl:disjointWith rdf:resource="http://data.europa.eu/a4g/ontology#ProcurementDocument"/>
   </rdf:Description>
   <rdf:Description rdf:about="http://data.europa.eu/a4g/ontology#Contract">
      <owl:disjointWith rdf:resource="http://data.europa.eu/a4g/ontology#Notice"/>
   </rdf:Description>
   <rdf:Description rdf:about="http://data.europa.eu/a4g/ontology#Contract">
      <owl:disjointWith rdf:resource="http://data.europa.eu/a4g/ontology#TenderDocument"/>
   </rdf:Description>
   <owl:Class rdf:about="http://data.europa.eu/a4g/ontology#PurchaseContract">
      <rdfs:subClassOf rdf:resource="http://data.europa.eu/a4g/ontology#Contract"/>
   </owl:Class>
   <rdf:Description rdf:about="http://data.europa.eu/a4g/ontology#PurchaseContract">
      <owl:disjointWith rdf:resource="http://data.europa.eu/a4g/ontology#FrameworkAgreement"/>
   </rdf:Description>
   <owl:Class rdf:about="http://data.europa.eu/a4g/ontology#FrameworkAgreement">
      <rdfs:subClassOf rdf:resource="http://data.europa.eu/a4g/ontology#Contract"/>
   </owl:Class>
   <rdf:Description rdf:about="http://data.europa.eu/a4g/ontology#FrameworkAgreement">
      <owl:disjointWith rdf:resource="http://data.europa.eu/a4g/ontology#PurchaseContract"/>
   </rdf:Description>
   <owl:Class rdf:about="http://data.europa.eu/a4g/ontology#ContractAwardNotice">
      <rdfs:subClassOf rdf:resource="http://data.europa.eu/a4g/ontology#Notice"/>
   </owl:Class>
   <rdf:Description rdf:about="http://data.europa.eu/a4g/ontology#ContractAwardNotice">
      <owl:disjointWith rdf:resource="http://data.europa.eu/a4g/ontology#BuyerProfileNotice"/>
   </rdf:Description>
   <rdf:Description rdf:about="http://data.europa.eu/a4g/ontology#ContractAwardNotice">
      <owl:disjointWith rdf:resource="http://data.europa.eu/a4g/ontology#CallForExpressionOfInterest"/>
   </rdf:Description>
   <rdf:Description rdf:about="http://data.europa.eu/a4g/ontology#ContractAwardNotice">
      <owl:disjointWith rdf:resource="http://data.europa.eu/a4g/ontology#ContractModificationNotice"/>
   </rdf:Description>
   <rdf:Description rdf:about="http://data.europa.eu/a4g/ontology#ContractAwardNotice">
      <owl:disjointWith rdf:resource="http://data.europa.eu/a4g/ontology#ContractNotice"/>
   </rdf:Description>
   <rdf:Description rdf:about="http://data.europa.eu/a4g/ontology#ContractAwardNotice">
      <owl:disjointWith rdf:resource="http://data.europa.eu/a4g/ontology#PriorInformationNotice"/>
   </rdf:Description>
   <rdf:Description rdf:about="http://data.europa.eu/a4g/ontology#ContractAwardNotice">
      <owl:disjointWith rdf:resource="http://data.europa.eu/a4g/ontology#VoluntaryEx-anteTransparencyNotice"/>
   </rdf:Description>
   <owl:Class rdf:about="http://data.europa.eu/a4g/ontology#ContractModificationNotice">
      <rdfs:subClassOf rdf:resource="http://data.europa.eu/a4g/ontology#Notice"/>
   </owl:Class>
   <rdf:Description rdf:about="http://data.europa.eu/a4g/ontology#ContractModificationNotice">
      <owl:disjointWith rdf:resource="http://data.europa.eu/a4g/ontology#BuyerProfileNotice"/>
   </rdf:Description>
   <rdf:Description rdf:about="http://data.europa.eu/a4g/ontology#ContractModificationNotice">
      <owl:disjointWith rdf:resource="http://data.europa.eu/a4g/ontology#CallForExpressionOfInterest"/>
   </rdf:Description>
   <rdf:Description rdf:about="http://data.europa.eu/a4g/ontology#ContractModificationNotice">
      <owl:disjointWith rdf:resource="http://data.europa.eu/a4g/ontology#ContractAwardNotice"/>
   </rdf:Description>
   <rdf:Description rdf:about="http://data.europa.eu/a4g/ontology#ContractModificationNotice">
      <owl:disjointWith rdf:resource="http://data.europa.eu/a4g/ontology#ContractNotice"/>
   </rdf:Description>
   <rdf:Description rdf:about="http://data.europa.eu/a4g/ontology#ContractModificationNotice">
      <owl:disjointWith rdf:resource="http://data.europa.eu/a4g/ontology#PriorInformationNotice"/>
   </rdf:Description>
   <rdf:Description rdf:about="http://data.europa.eu/a4g/ontology#ContractModificationNotice">
      <owl:disjointWith rdf:resource="http://data.europa.eu/a4g/ontology#VoluntaryEx-anteTransparencyNotice"/>
   </rdf:Description>
   <owl:Class rdf:about="http://data.europa.eu/a4g/ontology#ContractNotice">
      <rdfs:subClassOf rdf:resource="http://data.europa.eu/a4g/ontology#Notice"/>
   </owl:Class>
   <rdf:Description rdf:about="http://data.europa.eu/a4g/ontology#ContractNotice">
      <owl:disjointWith rdf:resource="http://data.europa.eu/a4g/ontology#BuyerProfileNotice"/>
   </rdf:Description>
   <rdf:Description rdf:about="http://data.europa.eu/a4g/ontology#ContractNotice">
      <owl:disjointWith rdf:resource="http://data.europa.eu/a4g/ontology#CallForExpressionOfInterest"/>
   </rdf:Description>
   <rdf:Description rdf:about="http://data.europa.eu/a4g/ontology#ContractNotice">
      <owl:disjointWith rdf:resource="http://data.europa.eu/a4g/ontology#ContractAwardNotice"/>
   </rdf:Description>
   <rdf:Description rdf:about="http://data.europa.eu/a4g/ontology#ContractNotice">
      <owl:disjointWith rdf:resource="http://data.europa.eu/a4g/ontology#ContractModificationNotice"/>
   </rdf:Description>
   <rdf:Description rdf:about="http://data.europa.eu/a4g/ontology#ContractNotice">
      <owl:disjointWith rdf:resource="http://data.europa.eu/a4g/ontology#PriorInformationNotice"/>
   </rdf:Description>
   <rdf:Description rdf:about="http://data.europa.eu/a4g/ontology#ContractNotice">
      <owl:disjointWith rdf:resource="http://data.europa.eu/a4g/ontology#VoluntaryEx-anteTransparencyNotice"/>
   </rdf:Description>
   <owl:Class rdf:about="http://data.europa.eu/a4g/ontology#Contractor">
      <rdfs:subClassOf rdf:resource="http://data.europa.eu/a4g/ontology#Winner"/>
   </owl:Class>
   <owl:Class rdf:about="http://data.europa.eu/a4g/ontology#ProcurementDocument">
      <rdfs:subClassOf rdf:resource="http://data.europa.eu/a4g/ontology#Document"/>
   </owl:Class>
   <rdf:Description rdf:about="http://data.europa.eu/a4g/ontology#ProcurementDocument">
      <owl:disjointWith rdf:resource="http://data.europa.eu/a4g/ontology#Contract"/>
   </rdf:Description>
   <rdf:Description rdf:about="http://data.europa.eu/a4g/ontology#ProcurementDocument">
      <owl:disjointWith rdf:resource="http://data.europa.eu/a4g/ontology#Notice"/>
   </rdf:Description>
   <rdf:Description rdf:about="http://data.europa.eu/a4g/ontology#ProcurementDocument">
      <owl:disjointWith rdf:resource="http://data.europa.eu/a4g/ontology#TenderDocument"/>
   </rdf:Description>
   <owl:Class rdf:about="http://data.europa.eu/a4g/ontology#Notice">
      <rdfs:subClassOf rdf:resource="http://data.europa.eu/a4g/ontology#Document"/>
   </owl:Class>
   <rdf:Description rdf:about="http://data.europa.eu/a4g/ontology#Notice">
      <owl:disjointWith rdf:resource="http://data.europa.eu/a4g/ontology#Contract"/>
   </rdf:Description>
   <rdf:Description rdf:about="http://data.europa.eu/a4g/ontology#Notice">
      <owl:disjointWith rdf:resource="http://data.europa.eu/a4g/ontology#ProcurementDocument"/>
   </rdf:Description>
   <rdf:Description rdf:about="http://data.europa.eu/a4g/ontology#Notice">
      <owl:disjointWith rdf:resource="http://data.europa.eu/a4g/ontology#TenderDocument"/>
   </rdf:Description>
   <owl:Class rdf:about="http://data.europa.eu/a4g/ontology#TenderDocument">
      <rdfs:subClassOf rdf:resource="http://data.europa.eu/a4g/ontology#Document"/>
   </owl:Class>
   <rdf:Description rdf:about="http://data.europa.eu/a4g/ontology#TenderDocument">
      <owl:disjointWith rdf:resource="http://data.europa.eu/a4g/ontology#Contract"/>
   </rdf:Description>
   <rdf:Description rdf:about="http://data.europa.eu/a4g/ontology#TenderDocument">
      <owl:disjointWith rdf:resource="http://data.europa.eu/a4g/ontology#ProcurementDocument"/>
   </rdf:Description>
   <rdf:Description rdf:about="http://data.europa.eu/a4g/ontology#TenderDocument">
      <owl:disjointWith rdf:resource="http://data.europa.eu/a4g/ontology#Notice"/>
   </rdf:Description>
   <owl:Class rdf:about="http://data.europa.eu/a4g/ontology#DynamicPurchaseSystemTechnique">
      <rdfs:subClassOf rdf:resource="http://data.europa.eu/a4g/ontology#Technique"/>
   </owl:Class>
   <rdf:Description rdf:about="http://data.europa.eu/a4g/ontology#DynamicPurchaseSystemTechnique">
      <owl:disjointWith rdf:resource="http://data.europa.eu/a4g/ontology#EAuctionTechnique"/>
   </rdf:Description>
   <rdf:Description rdf:about="http://data.europa.eu/a4g/ontology#DynamicPurchaseSystemTechnique">
      <owl:disjointWith rdf:resource="http://data.europa.eu/a4g/ontology#FrameworkAgreementTechnique"/>
   </rdf:Description>
   <owl:Class rdf:about="http://data.europa.eu/a4g/ontology#EAuctionTechnique">
      <rdfs:subClassOf rdf:resource="http://data.europa.eu/a4g/ontology#Technique"/>
   </owl:Class>
   <rdf:Description rdf:about="http://data.europa.eu/a4g/ontology#EAuctionTechnique">
      <owl:disjointWith rdf:resource="http://data.europa.eu/a4g/ontology#DynamicPurchaseSystemTechnique"/>
   </rdf:Description>
   <rdf:Description rdf:about="http://data.europa.eu/a4g/ontology#EAuctionTechnique">
      <owl:disjointWith rdf:resource="http://data.europa.eu/a4g/ontology#FrameworkAgreementTechnique"/>
   </rdf:Description>
   <owl:Class rdf:about="http://data.europa.eu/a4g/ontology#EconomicOperator">
      <rdfs:subClassOf rdf:resource="http://data.europa.eu/a4g/ontology#ProcurementRole"/>
   </owl:Class>
   <rdf:Description rdf:about="http://data.europa.eu/a4g/ontology#EconomicOperator">
      <owl:disjointWith rdf:resource="http://data.europa.eu/a4g/ontology#Buyer"/>
   </rdf:Description>
   <rdf:Description rdf:about="http://data.europa.eu/a4g/ontology#EconomicOperator">
      <owl:disjointWith rdf:resource="http://data.europa.eu/a4g/ontology#CatalogueProvider"/>
   </rdf:Description>
   <rdf:Description rdf:about="http://data.europa.eu/a4g/ontology#EconomicOperator">
      <owl:disjointWith rdf:resource="http://data.europa.eu/a4g/ontology#CatalogueReceiver"/>
   </rdf:Description>
   <rdf:Description rdf:about="http://data.europa.eu/a4g/ontology#EconomicOperator">
      <owl:disjointWith rdf:resource="http://data.europa.eu/a4g/ontology#Mediator"/>
   </rdf:Description>
   <rdf:Description rdf:about="http://data.europa.eu/a4g/ontology#EconomicOperator">
      <owl:disjointWith rdf:resource="http://data.europa.eu/a4g/ontology#ProcurementServiceProvider"/>
   </rdf:Description>
   <rdf:Description rdf:about="http://data.europa.eu/a4g/ontology#EconomicOperator">
      <owl:disjointWith rdf:resource="http://data.europa.eu/a4g/ontology#Reviewer"/>
   </rdf:Description>
   <rdf:Description rdf:about="http://data.europa.eu/a4g/ontology#EconomicOperator">
      <owl:disjointWith rdf:resource="http://data.europa.eu/a4g/ontology#ReviewRequester"/>
   </rdf:Description>
   <owl:Class rdf:about="http://data.europa.eu/a4g/ontology#Tenderer">
      <rdfs:subClassOf rdf:resource="http://data.europa.eu/a4g/ontology#EconomicOperator"/>
   </owl:Class>
   <rdf:Description rdf:about="http://data.europa.eu/a4g/ontology#Tenderer">
      <owl:disjointWith rdf:resource="http://data.europa.eu/a4g/ontology#Subcontractor"/>
   </rdf:Description>
   <owl:Class rdf:about="http://data.europa.eu/a4g/ontology#Subcontractor">
      <rdfs:subClassOf rdf:resource="http://data.europa.eu/a4g/ontology#EconomicOperator"/>
   </owl:Class>
   <rdf:Description rdf:about="http://data.europa.eu/a4g/ontology#Subcontractor">
      <owl:disjointWith rdf:resource="http://data.europa.eu/a4g/ontology#Tenderer"/>
   </rdf:Description>
   <owl:Class rdf:about="http://data.europa.eu/a4g/ontology#ExclusionGround">
      <rdfs:subClassOf rdf:resource="http://data.europa.eu/a4g/ontology#ProcurementCriterion"/>
   </owl:Class>
   <rdf:Description rdf:about="http://data.europa.eu/a4g/ontology#ExclusionGround">
      <owl:disjointWith rdf:resource="http://data.europa.eu/a4g/ontology#AwardCriterion"/>
   </rdf:Description>
   <rdf:Description rdf:about="http://data.europa.eu/a4g/ontology#ExclusionGround">
      <owl:disjointWith rdf:resource="http://data.europa.eu/a4g/ontology#SelectionCriterion"/>
   </rdf:Description>
   <owl:Class rdf:about="http://data.europa.eu/a4g/ontology#ExpressionOfInterest">
      <rdfs:subClassOf rdf:resource="http://data.europa.eu/a4g/ontology#TenderDocument"/>
   </owl:Class>
   <rdf:Description rdf:about="http://data.europa.eu/a4g/ontology#ExpressionOfInterest">
      <owl:disjointWith rdf:resource="http://data.europa.eu/a4g/ontology#RequestForParticipation"/>
   </rdf:Description>
   <rdf:Description rdf:about="http://data.europa.eu/a4g/ontology#ExpressionOfInterest">
      <owl:disjointWith rdf:resource="http://data.europa.eu/a4g/ontology#RequestForClarification"/>
   </rdf:Description>
   <owl:Class rdf:about="http://data.europa.eu/a4g/ontology#FrameworkAgreementTechnique">
      <rdfs:subClassOf rdf:resource="http://data.europa.eu/a4g/ontology#Technique"/>
   </owl:Class>
   <rdf:Description rdf:about="http://data.europa.eu/a4g/ontology#FrameworkAgreementTechnique">
      <owl:disjointWith rdf:resource="http://data.europa.eu/a4g/ontology#DynamicPurchaseSystemTechnique"/>
   </rdf:Description>
   <rdf:Description rdf:about="http://data.europa.eu/a4g/ontology#FrameworkAgreementTechnique">
      <owl:disjointWith rdf:resource="http://data.europa.eu/a4g/ontology#EAuctionTechnique"/>
   </rdf:Description>
   <owl:Class rdf:about="http://data.europa.eu/a4g/ontology#GreenProcurement">
      <rdfs:subClassOf rdf:resource="http://data.europa.eu/a4g/ontology#StrategicProcurement"/>
   </owl:Class>
   <rdf:Description rdf:about="http://data.europa.eu/a4g/ontology#GreenProcurement">
      <owl:disjointWith rdf:resource="http://data.europa.eu/a4g/ontology#InnovativeProcurement"/>
   </rdf:Description>
   <rdf:Description rdf:about="http://data.europa.eu/a4g/ontology#GreenProcurement">
      <owl:disjointWith rdf:resource="http://data.europa.eu/a4g/ontology#SocialProcurement"/>
   </rdf:Description>
   <owl:Class rdf:about="http://data.europa.eu/a4g/ontology#InnovativeProcurement">
      <rdfs:subClassOf rdf:resource="http://data.europa.eu/a4g/ontology#StrategicProcurement"/>
   </owl:Class>
   <rdf:Description rdf:about="http://data.europa.eu/a4g/ontology#InnovativeProcurement">
      <owl:disjointWith rdf:resource="http://data.europa.eu/a4g/ontology#GreenProcurement"/>
   </rdf:Description>
   <rdf:Description rdf:about="http://data.europa.eu/a4g/ontology#InnovativeProcurement">
      <owl:disjointWith rdf:resource="http://data.europa.eu/a4g/ontology#SocialProcurement"/>
   </rdf:Description>
   <owl:Class rdf:about="http://data.europa.eu/a4g/ontology#Mediator">
      <rdfs:subClassOf rdf:resource="http://data.europa.eu/a4g/ontology#ProcurementRole"/>
   </owl:Class>
   <rdf:Description rdf:about="http://data.europa.eu/a4g/ontology#Mediator">
      <owl:disjointWith rdf:resource="http://data.europa.eu/a4g/ontology#Buyer"/>
   </rdf:Description>
   <rdf:Description rdf:about="http://data.europa.eu/a4g/ontology#Mediator">
      <owl:disjointWith rdf:resource="http://data.europa.eu/a4g/ontology#CatalogueProvider"/>
   </rdf:Description>
   <rdf:Description rdf:about="http://data.europa.eu/a4g/ontology#Mediator">
      <owl:disjointWith rdf:resource="http://data.europa.eu/a4g/ontology#CatalogueReceiver"/>
   </rdf:Description>
   <rdf:Description rdf:about="http://data.europa.eu/a4g/ontology#Mediator">
      <owl:disjointWith rdf:resource="http://data.europa.eu/a4g/ontology#EconomicOperator"/>
   </rdf:Description>
   <rdf:Description rdf:about="http://data.europa.eu/a4g/ontology#Mediator">
      <owl:disjointWith rdf:resource="http://data.europa.eu/a4g/ontology#ProcurementServiceProvider"/>
   </rdf:Description>
   <rdf:Description rdf:about="http://data.europa.eu/a4g/ontology#Mediator">
      <owl:disjointWith rdf:resource="http://data.europa.eu/a4g/ontology#Reviewer"/>
   </rdf:Description>
   <rdf:Description rdf:about="http://data.europa.eu/a4g/ontology#Mediator">
      <owl:disjointWith rdf:resource="http://data.europa.eu/a4g/ontology#ReviewRequester"/>
   </rdf:Description>
   <owl:Class rdf:about="http://data.europa.eu/a4g/ontology#PriorInformationNotice">
      <rdfs:subClassOf rdf:resource="http://data.europa.eu/a4g/ontology#Notice"/>
   </owl:Class>
   <rdf:Description rdf:about="http://data.europa.eu/a4g/ontology#PriorInformationNotice">
      <owl:disjointWith rdf:resource="http://data.europa.eu/a4g/ontology#BuyerProfileNotice"/>
   </rdf:Description>
   <rdf:Description rdf:about="http://data.europa.eu/a4g/ontology#PriorInformationNotice">
      <owl:disjointWith rdf:resource="http://data.europa.eu/a4g/ontology#CallForExpressionOfInterest"/>
   </rdf:Description>
   <rdf:Description rdf:about="http://data.europa.eu/a4g/ontology#PriorInformationNotice">
      <owl:disjointWith rdf:resource="http://data.europa.eu/a4g/ontology#ContractAwardNotice"/>
   </rdf:Description>
   <rdf:Description rdf:about="http://data.europa.eu/a4g/ontology#PriorInformationNotice">
      <owl:disjointWith rdf:resource="http://data.europa.eu/a4g/ontology#ContractModificationNotice"/>
   </rdf:Description>
   <rdf:Description rdf:about="http://data.europa.eu/a4g/ontology#PriorInformationNotice">
      <owl:disjointWith rdf:resource="http://data.europa.eu/a4g/ontology#ContractNotice"/>
   </rdf:Description>
   <rdf:Description rdf:about="http://data.europa.eu/a4g/ontology#PriorInformationNotice">
      <owl:disjointWith rdf:resource="http://data.europa.eu/a4g/ontology#VoluntaryEx-anteTransparencyNotice"/>
   </rdf:Description>
   <owl:Class rdf:about="http://data.europa.eu/a4g/ontology#VoluntaryEx-anteTransparencyNotice">
      <rdfs:subClassOf rdf:resource="http://data.europa.eu/a4g/ontology#Notice"/>
   </owl:Class>
   <rdf:Description rdf:about="http://data.europa.eu/a4g/ontology#VoluntaryEx-anteTransparencyNotice">
      <owl:disjointWith rdf:resource="http://data.europa.eu/a4g/ontology#BuyerProfileNotice"/>
   </rdf:Description>
   <rdf:Description rdf:about="http://data.europa.eu/a4g/ontology#VoluntaryEx-anteTransparencyNotice">
      <owl:disjointWith rdf:resource="http://data.europa.eu/a4g/ontology#CallForExpressionOfInterest"/>
   </rdf:Description>
   <rdf:Description rdf:about="http://data.europa.eu/a4g/ontology#VoluntaryEx-anteTransparencyNotice">
      <owl:disjointWith rdf:resource="http://data.europa.eu/a4g/ontology#ContractAwardNotice"/>
   </rdf:Description>
   <rdf:Description rdf:about="http://data.europa.eu/a4g/ontology#VoluntaryEx-anteTransparencyNotice">
      <owl:disjointWith rdf:resource="http://data.europa.eu/a4g/ontology#ContractModificationNotice"/>
   </rdf:Description>
   <rdf:Description rdf:about="http://data.europa.eu/a4g/ontology#VoluntaryEx-anteTransparencyNotice">
      <owl:disjointWith rdf:resource="http://data.europa.eu/a4g/ontology#ContractNotice"/>
   </rdf:Description>
   <rdf:Description rdf:about="http://data.europa.eu/a4g/ontology#VoluntaryEx-anteTransparencyNotice">
      <owl:disjointWith rdf:resource="http://data.europa.eu/a4g/ontology#PriorInformationNotice"/>
   </rdf:Description>
   <owl:Class rdf:about="http://data.europa.eu/a4g/ontology#OrganisationGroup">
      <rdfs:subClassOf rdf:resource="http://data.europa.eu/a4g/ontology#Organisation"/>
   </owl:Class>
   <rdf:Description rdf:about="http://data.europa.eu/a4g/ontology#OrganisationGroup">
      <owl:disjointWith rdf:resource="http://data.europa.eu/a4g/ontology#Business"/>
   </rdf:Description>
   <rdf:Description rdf:about="http://data.europa.eu/a4g/ontology#OrganisationGroup">
      <owl:disjointWith rdf:resource="http://data.europa.eu/a4g/ontology#PublicOrganisation"/>
   </rdf:Description>
   <owl:Class rdf:about="http://data.europa.eu/a4g/ontology#PublicOrganisation">
      <rdfs:subClassOf rdf:resource="http://data.europa.eu/a4g/ontology#Organisation"/>
   </owl:Class>
   <rdf:Description rdf:about="http://data.europa.eu/a4g/ontology#PublicOrganisation">
      <owl:disjointWith rdf:resource="http://data.europa.eu/a4g/ontology#Business"/>
   </rdf:Description>
   <rdf:Description rdf:about="http://data.europa.eu/a4g/ontology#PublicOrganisation">
      <owl:disjointWith rdf:resource="http://data.europa.eu/a4g/ontology#OrganisationGroup"/>
   </rdf:Description>
   <owl:Class rdf:about="http://data.europa.eu/a4g/ontology#SelectionCriterion">
      <rdfs:subClassOf rdf:resource="http://data.europa.eu/a4g/ontology#ProcurementCriterion"/>
   </owl:Class>
   <rdf:Description rdf:about="http://data.europa.eu/a4g/ontology#SelectionCriterion">
      <owl:disjointWith rdf:resource="http://data.europa.eu/a4g/ontology#AwardCriterion"/>
   </rdf:Description>
   <rdf:Description rdf:about="http://data.europa.eu/a4g/ontology#SelectionCriterion">
      <owl:disjointWith rdf:resource="http://data.europa.eu/a4g/ontology#ExclusionGround"/>
   </rdf:Description>
   <owl:Class rdf:about="http://data.europa.eu/a4g/ontology#TechnicalSpecification">
      <rdfs:subClassOf rdf:resource="http://data.europa.eu/a4g/ontology#ProcurementDocument"/>
   </owl:Class>
   <rdf:Description rdf:about="http://data.europa.eu/a4g/ontology#TechnicalSpecification">
      <owl:disjointWith rdf:resource="http://data.europa.eu/a4g/ontology#CallForCompetition"/>
   </rdf:Description>
   <owl:Class rdf:about="http://data.europa.eu/a4g/ontology#ProcurementServiceProvider">
      <rdfs:subClassOf rdf:resource="http://data.europa.eu/a4g/ontology#ProcurementRole"/>
   </owl:Class>
   <rdf:Description rdf:about="http://data.europa.eu/a4g/ontology#ProcurementServiceProvider">
      <owl:disjointWith rdf:resource="http://data.europa.eu/a4g/ontology#Buyer"/>
   </rdf:Description>
   <rdf:Description rdf:about="http://data.europa.eu/a4g/ontology#ProcurementServiceProvider">
      <owl:disjointWith rdf:resource="http://data.europa.eu/a4g/ontology#CatalogueProvider"/>
   </rdf:Description>
   <rdf:Description rdf:about="http://data.europa.eu/a4g/ontology#ProcurementServiceProvider">
      <owl:disjointWith rdf:resource="http://data.europa.eu/a4g/ontology#CatalogueReceiver"/>
   </rdf:Description>
   <rdf:Description rdf:about="http://data.europa.eu/a4g/ontology#ProcurementServiceProvider">
      <owl:disjointWith rdf:resource="http://data.europa.eu/a4g/ontology#EconomicOperator"/>
   </rdf:Description>
   <rdf:Description rdf:about="http://data.europa.eu/a4g/ontology#ProcurementServiceProvider">
      <owl:disjointWith rdf:resource="http://data.europa.eu/a4g/ontology#Mediator"/>
   </rdf:Description>
   <rdf:Description rdf:about="http://data.europa.eu/a4g/ontology#ProcurementServiceProvider">
      <owl:disjointWith rdf:resource="http://data.europa.eu/a4g/ontology#Reviewer"/>
   </rdf:Description>
   <rdf:Description rdf:about="http://data.europa.eu/a4g/ontology#ProcurementServiceProvider">
      <owl:disjointWith rdf:resource="http://data.europa.eu/a4g/ontology#ReviewRequester"/>
   </rdf:Description>
   <owl:Class rdf:about="http://data.europa.eu/a4g/ontology#Reviewer">
      <rdfs:subClassOf rdf:resource="http://data.europa.eu/a4g/ontology#ProcurementRole"/>
   </owl:Class>
   <rdf:Description rdf:about="http://data.europa.eu/a4g/ontology#Reviewer">
      <owl:disjointWith rdf:resource="http://data.europa.eu/a4g/ontology#Buyer"/>
   </rdf:Description>
   <rdf:Description rdf:about="http://data.europa.eu/a4g/ontology#Reviewer">
      <owl:disjointWith rdf:resource="http://data.europa.eu/a4g/ontology#CatalogueProvider"/>
   </rdf:Description>
   <rdf:Description rdf:about="http://data.europa.eu/a4g/ontology#Reviewer">
      <owl:disjointWith rdf:resource="http://data.europa.eu/a4g/ontology#CatalogueReceiver"/>
   </rdf:Description>
   <rdf:Description rdf:about="http://data.europa.eu/a4g/ontology#Reviewer">
      <owl:disjointWith rdf:resource="http://data.europa.eu/a4g/ontology#EconomicOperator"/>
   </rdf:Description>
   <rdf:Description rdf:about="http://data.europa.eu/a4g/ontology#Reviewer">
      <owl:disjointWith rdf:resource="http://data.europa.eu/a4g/ontology#Mediator"/>
   </rdf:Description>
   <rdf:Description rdf:about="http://data.europa.eu/a4g/ontology#Reviewer">
      <owl:disjointWith rdf:resource="http://data.europa.eu/a4g/ontology#ProcurementServiceProvider"/>
   </rdf:Description>
   <rdf:Description rdf:about="http://data.europa.eu/a4g/ontology#Reviewer">
      <owl:disjointWith rdf:resource="http://data.europa.eu/a4g/ontology#ReviewRequester"/>
   </rdf:Description>
   <owl:Class rdf:about="http://data.europa.eu/a4g/ontology#ReviewRequester">
      <rdfs:subClassOf rdf:resource="http://data.europa.eu/a4g/ontology#ProcurementRole"/>
   </owl:Class>
   <rdf:Description rdf:about="http://data.europa.eu/a4g/ontology#ReviewRequester">
      <owl:disjointWith rdf:resource="http://data.europa.eu/a4g/ontology#Buyer"/>
   </rdf:Description>
   <rdf:Description rdf:about="http://data.europa.eu/a4g/ontology#ReviewRequester">
      <owl:disjointWith rdf:resource="http://data.europa.eu/a4g/ontology#CatalogueProvider"/>
   </rdf:Description>
   <rdf:Description rdf:about="http://data.europa.eu/a4g/ontology#ReviewRequester">
      <owl:disjointWith rdf:resource="http://data.europa.eu/a4g/ontology#CatalogueReceiver"/>
   </rdf:Description>
   <rdf:Description rdf:about="http://data.europa.eu/a4g/ontology#ReviewRequester">
      <owl:disjointWith rdf:resource="http://data.europa.eu/a4g/ontology#EconomicOperator"/>
   </rdf:Description>
   <rdf:Description rdf:about="http://data.europa.eu/a4g/ontology#ReviewRequester">
      <owl:disjointWith rdf:resource="http://data.europa.eu/a4g/ontology#Mediator"/>
   </rdf:Description>
   <rdf:Description rdf:about="http://data.europa.eu/a4g/ontology#ReviewRequester">
      <owl:disjointWith rdf:resource="http://data.europa.eu/a4g/ontology#ProcurementServiceProvider"/>
   </rdf:Description>
   <rdf:Description rdf:about="http://data.europa.eu/a4g/ontology#ReviewRequester">
      <owl:disjointWith rdf:resource="http://data.europa.eu/a4g/ontology#Reviewer"/>
   </rdf:Description>
   <owl:Class rdf:about="http://data.europa.eu/a4g/ontology#RequestForParticipation">
      <rdfs:subClassOf rdf:resource="http://data.europa.eu/a4g/ontology#TenderDocument"/>
   </owl:Class>
   <rdf:Description rdf:about="http://data.europa.eu/a4g/ontology#RequestForParticipation">
      <owl:disjointWith rdf:resource="http://data.europa.eu/a4g/ontology#ExpressionOfInterest"/>
   </rdf:Description>
   <rdf:Description rdf:about="http://data.europa.eu/a4g/ontology#RequestForParticipation">
      <owl:disjointWith rdf:resource="http://data.europa.eu/a4g/ontology#RequestForClarification"/>
   </rdf:Description>
   <owl:Class rdf:about="http://data.europa.eu/a4g/ontology#SocialProcurement">
      <rdfs:subClassOf rdf:resource="http://data.europa.eu/a4g/ontology#StrategicProcurement"/>
   </owl:Class>
   <rdf:Description rdf:about="http://data.europa.eu/a4g/ontology#SocialProcurement">
      <owl:disjointWith rdf:resource="http://data.europa.eu/a4g/ontology#GreenProcurement"/>
   </rdf:Description>
   <rdf:Description rdf:about="http://data.europa.eu/a4g/ontology#SocialProcurement">
      <owl:disjointWith rdf:resource="http://data.europa.eu/a4g/ontology#InnovativeProcurement"/>
   </rdf:Description>
   <owl:Class rdf:about="http://data.europa.eu/a4g/ontology#RequestForClarification">
      <rdfs:subClassOf rdf:resource="http://data.europa.eu/a4g/ontology#TenderDocument"/>
   </owl:Class>
   <rdf:Description rdf:about="http://data.europa.eu/a4g/ontology#RequestForClarification">
      <owl:disjointWith rdf:resource="http://data.europa.eu/a4g/ontology#ExpressionOfInterest"/>
   </rdf:Description>
   <rdf:Description rdf:about="http://data.europa.eu/a4g/ontology#RequestForClarification">
      <owl:disjointWith rdf:resource="http://data.europa.eu/a4g/ontology#RequestForParticipation"/>
   </rdf:Description>
   <owl:Class rdf:about="http://data.europa.eu/a4g/ontology#Winner">
      <rdfs:subClassOf rdf:resource="http://data.europa.eu/a4g/ontology#Tenderer"/>
   </owl:Class>
   <owl:ObjectProperty rdf:about="http://data.europa.eu/a4g/ontology#adminUnitL1">
      <rdfs:label xml:lang="en">Admin unit l1</rdfs:label>
      <skos:prefLabel xml:lang="en">Admin unit l1</skos:prefLabel>
      <skos:definition xml:lang="en">
 (locn:Address -&gt; at-voc:nuts (+locn:adminUnitL1)) </skos:definition>
      <rdfs:comment xml:lang="en">
 (locn:Address -&gt; at-voc:nuts (+locn:adminUnitL1)) </rdfs:comment>
      <skos:scopeNote xml:lang="en">The name or names of a unit of administration related to the exercise of jurisdictional rights, for local, regional and national governance. Level 1 refers to the uppermost administrative unit for the address, almost always a country.

Additional Information:
The codelist to be used is at-voc:nuts which is available at https://op.europa.eu/en/web/eu-vocabularies/at-dataset/-/resource/dataset/nuts

Best practice is to use the ISO 3166-1 code but if this is inappropriate for the context, country names should be provided in a consistent manner to reduce ambiguity. For example, either write 'France' or 'FRA' consistently throughout the dataset and avoid mixing the two. The Country controlled vocabulary from the Publications Office can be reused for this. (dct:Location -&gt; at-voc:nuts (+locn:adminUnitL1)) The name or names of a unit of administration related to the exercise of jurisdictional rights, for local, regional and national governance. Level 1 refers to the uppermost administrative unit for the address, almost always a country.

Additional Information:
The codelist to be used is at-voc:nuts which is available at https://op.europa.eu/en/web/eu-vocabularies/at-dataset/-/resource/dataset/nuts

Best practice is to use the ISO 3166-1 code but if this is inappropriate for the context, country names should be provided in a consistent manner to reduce ambiguity. For example, either write 'France' or 'FRA' consistently throughout the dataset and avoid mixing the two. The Country controlled vocabulary from the Publications Office can be reused for this. (locn:Address -&gt; at-voc:nuts (+locn:adminUnitL1)) </skos:scopeNote>
      <rdfs:comment xml:lang="en">The name or names of a unit of administration related to the exercise of jurisdictional rights, for local, regional and national governance. Level 1 refers to the uppermost administrative unit for the address, almost always a country.

Additional Information:
The codelist to be used is at-voc:nuts which is available at https://op.europa.eu/en/web/eu-vocabularies/at-dataset/-/resource/dataset/nuts

Best practice is to use the ISO 3166-1 code but if this is inappropriate for the context, country names should be provided in a consistent manner to reduce ambiguity. For example, either write 'France' or 'FRA' consistently throughout the dataset and avoid mixing the two. The Country controlled vocabulary from the Publications Office can be reused for this. (dct:Location -&gt; at-voc:nuts (+locn:adminUnitL1)) The name or names of a unit of administration related to the exercise of jurisdictional rights, for local, regional and national governance. Level 1 refers to the uppermost administrative unit for the address, almost always a country.

Additional Information:
The codelist to be used is at-voc:nuts which is available at https://op.europa.eu/en/web/eu-vocabularies/at-dataset/-/resource/dataset/nuts

Best practice is to use the ISO 3166-1 code but if this is inappropriate for the context, country names should be provided in a consistent manner to reduce ambiguity. For example, either write 'France' or 'FRA' consistently throughout the dataset and avoid mixing the two. The Country controlled vocabulary from the Publications Office can be reused for this. (locn:Address -&gt; at-voc:nuts (+locn:adminUnitL1)) </rdfs:comment>
      <rdfs:isDefinedBy rdf:resource="http://data.europa.eu/a4g/ontology"/>
   </owl:ObjectProperty>
   <owl:ObjectProperty rdf:about="http://data.europa.eu/a4g/ontology#hasCountryCode">
      <rdfs:label xml:lang="en">Has country code</rdfs:label>
      <skos:prefLabel xml:lang="en">Has country code</skos:prefLabel>
      <skos:definition xml:lang="en">
 (locn:Address -&gt; at-voc:country (+epo:hasCountryCode)) </skos:definition>
      <rdfs:comment xml:lang="en">
 (locn:Address -&gt; at-voc:country (+epo:hasCountryCode)) </rdfs:comment>
      <skos:scopeNote xml:lang="en">The codelist to be used is at-voc:country which is available at https://op.europa.eu/web/eu-vocabularies/at-dataset/-/resource/dataset/country
 (locn:Address -&gt; at-voc:country (+epo:hasCountryCode)) </skos:scopeNote>
      <rdfs:comment xml:lang="en">The codelist to be used is at-voc:country which is available at https://op.europa.eu/web/eu-vocabularies/at-dataset/-/resource/dataset/country
 (locn:Address -&gt; at-voc:country (+epo:hasCountryCode)) </rdfs:comment>
      <rdfs:isDefinedBy rdf:resource="http://data.europa.eu/a4g/ontology"/>
   </owl:ObjectProperty>
   <owl:ObjectProperty rdf:about="http://data.europa.eu/a4g/ontology#adminUnitL2">
      <rdfs:label xml:lang="en">Admin unit l2</rdfs:label>
      <skos:prefLabel xml:lang="en">Admin unit l2</skos:prefLabel>
      <skos:scopeNote xml:lang="en">The name or names of a unit of administration related to the exercise of jurisdictional rights, for local, regional and national governance. Level 2 referst to the region of the address, usually a county, state or other such area that typically encompasses several localities.

Additional Information:
Some recommended codelists from the EU Publications Office include: Administrative Territorial Units (ATU), NUTS and Local Administrative Units (LAU). The first arrondissement of Paris is for example expressed as "http://publications.europa.eu/resource/authority/atu/FRA_AR_PAR01" in the ATU controlled vocabulary.
 (dct:Location -&gt; at-voc:nuts (+locn:adminUnitL2)) The name or names of a unit of administration related to the exercise of jurisdictional rights, for local, regional and national governance. Level 2 referst to the region of the address, usually a county, state or other such area that typically encompasses several localities.

Additional Information:
Some recommended codelists from the EU Publications Office include: Administrative Territorial Units (ATU), NUTS and Local Administrative Units (LAU). The first arrondissement of Paris is for example expressed as "http://publications.europa.eu/resource/authority/atu/FRA_AR_PAR01" in the ATU controlled vocabulary.
 (locn:Address -&gt; at-voc:nuts (+locn:adminUnitL2)) </skos:scopeNote>
      <rdfs:comment xml:lang="en">The name or names of a unit of administration related to the exercise of jurisdictional rights, for local, regional and national governance. Level 2 referst to the region of the address, usually a county, state or other such area that typically encompasses several localities.

Additional Information:
Some recommended codelists from the EU Publications Office include: Administrative Territorial Units (ATU), NUTS and Local Administrative Units (LAU). The first arrondissement of Paris is for example expressed as "http://publications.europa.eu/resource/authority/atu/FRA_AR_PAR01" in the ATU controlled vocabulary.
 (dct:Location -&gt; at-voc:nuts (+locn:adminUnitL2)) The name or names of a unit of administration related to the exercise of jurisdictional rights, for local, regional and national governance. Level 2 referst to the region of the address, usually a county, state or other such area that typically encompasses several localities.

Additional Information:
Some recommended codelists from the EU Publications Office include: Administrative Territorial Units (ATU), NUTS and Local Administrative Units (LAU). The first arrondissement of Paris is for example expressed as "http://publications.europa.eu/resource/authority/atu/FRA_AR_PAR01" in the ATU controlled vocabulary.
 (locn:Address -&gt; at-voc:nuts (+locn:adminUnitL2)) </rdfs:comment>
      <rdfs:isDefinedBy rdf:resource="http://data.europa.eu/a4g/ontology"/>
   </owl:ObjectProperty>
   <owl:ObjectProperty rdf:about="http://data.europa.eu/a4g/ontology#geometry">
      <rdfs:label xml:lang="en">Geometry</rdfs:label>
      <skos:prefLabel xml:lang="en">Geometry</skos:prefLabel>
      <rdfs:isDefinedBy rdf:resource="http://data.europa.eu/a4g/ontology"/>
   </owl:ObjectProperty>
   <owl:ObjectProperty rdf:about="http://data.europa.eu/a4g/ontology#address">
      <rdfs:label xml:lang="en">Address</rdfs:label>
      <skos:prefLabel xml:lang="en">Address</skos:prefLabel>
      <rdfs:isDefinedBy rdf:resource="http://data.europa.eu/a4g/ontology"/>
   </owl:ObjectProperty>
   <owl:ObjectProperty rdf:about="http://data.europa.eu/a4g/ontology#hasSpecificPlaceOfPerformance">
      <rdfs:label xml:lang="en">Has specific place of performance</rdfs:label>
      <skos:prefLabel xml:lang="en">Has specific place of performance</skos:prefLabel>
      <rdfs:isDefinedBy rdf:resource="http://data.europa.eu/a4g/ontology"/>
   </owl:ObjectProperty>
   <owl:ObjectProperty rdf:about="http://data.europa.eu/a4g/ontology#hasRestrictedAccessAddress">
      <rdfs:label xml:lang="en">Has restricted access address</rdfs:label>
      <skos:prefLabel xml:lang="en">Has restricted access address</skos:prefLabel>
      <rdfs:isDefinedBy rdf:resource="http://data.europa.eu/a4g/ontology"/>
   </owl:ObjectProperty>
   <owl:ObjectProperty rdf:about="http://data.europa.eu/a4g/ontology#isSubjectTo">
      <rdfs:label xml:lang="en">Is subject to</rdfs:label>
      <skos:prefLabel xml:lang="en">Is subject to</skos:prefLabel>
      <skos:scopeNote xml:lang="en">Relation that specifies rules that are applicable to the lot. (epo:PlannedProcurementPart -&gt; epo:AccessTerm (+epo:isSubjectTo)) Relation that specifies rules that are applicable to the lot. (epo:PlannedProcurementPart -&gt; epo:ContractTerm (+epo:isSubjectTo)) Relation that specifies rules that are applicable to the lot. (epo:Procedure -&gt; epo:DirectAwardTerm (+epo:isSubjectTo)) Relation that specifies rules that are applicable to the lot. (epo:Lot -&gt; epo:OpeningTerm (+epo:isSubjectTo)) Relation that specifies rules that are applicable to the lot. (epo:Procedure -&gt; epo:ProcedureTerm (+epo:isSubjectTo)) </skos:scopeNote>
      <rdfs:comment xml:lang="en">Relation that specifies rules that are applicable to the lot. (epo:PlannedProcurementPart -&gt; epo:AccessTerm (+epo:isSubjectTo)) Relation that specifies rules that are applicable to the lot. (epo:PlannedProcurementPart -&gt; epo:ContractTerm (+epo:isSubjectTo)) Relation that specifies rules that are applicable to the lot. (epo:Procedure -&gt; epo:DirectAwardTerm (+epo:isSubjectTo)) Relation that specifies rules that are applicable to the lot. (epo:Lot -&gt; epo:OpeningTerm (+epo:isSubjectTo)) Relation that specifies rules that are applicable to the lot. (epo:Procedure -&gt; epo:ProcedureTerm (+epo:isSubjectTo)) </rdfs:comment>
      <rdfs:isDefinedBy rdf:resource="http://data.europa.eu/a4g/ontology"/>
   </owl:ObjectProperty>
   <owl:ObjectProperty rdf:about="http://data.europa.eu/a4g/ontology#uses">
      <rdfs:label xml:lang="en">Uses</rdfs:label>
      <skos:prefLabel xml:lang="en">Uses</skos:prefLabel>
      <skos:definition xml:lang="en">

Additional Information
This property allows to obtain the estimated value of both a group of lots used in a Framework Agreement and the estimated value of each individual lot; which helps to compare the difference between the estimated value of the group against the addition of each lot estimated value.

 (epo:FrameworkAgreementTechnique &lt;-&gt; epo:LotGroup (+epo:isOrganisedIn +epo:uses)) </skos:definition>
      <rdfs:comment xml:lang="en">

Additional Information
This property allows to obtain the estimated value of both a group of lots used in a Framework Agreement and the estimated value of each individual lot; which helps to compare the difference between the estimated value of the group against the addition of each lot estimated value.

 (epo:FrameworkAgreementTechnique &lt;-&gt; epo:LotGroup (+epo:isOrganisedIn +epo:uses)) </rdfs:comment>
      <rdfs:isDefinedBy rdf:resource="http://data.europa.eu/a4g/ontology"/>
   </owl:ObjectProperty>
   <owl:ObjectProperty rdf:about="http://data.europa.eu/a4g/ontology#isProvidedBy">
      <rdfs:label xml:lang="en">Is provided by</rdfs:label>
      <skos:prefLabel xml:lang="en">Is provided by</skos:prefLabel>
      <rdfs:isDefinedBy rdf:resource="http://data.europa.eu/a4g/ontology"/>
   </owl:ObjectProperty>
   <owl:ObjectProperty rdf:about="http://data.europa.eu/a4g/ontology#provides">
      <rdfs:label xml:lang="en">Provides</rdfs:label>
      <skos:prefLabel xml:lang="en">Provides</skos:prefLabel>
      <rdfs:isDefinedBy rdf:resource="http://data.europa.eu/a4g/ontology"/>
   </owl:ObjectProperty>
   <owl:ObjectProperty rdf:about="http://data.europa.eu/a4g/ontology#isCreatedBy">
      <rdfs:label xml:lang="en">Is created by</rdfs:label>
      <skos:prefLabel xml:lang="en">Is created by</skos:prefLabel>
      <rdfs:isDefinedBy rdf:resource="http://data.europa.eu/a4g/ontology"/>
   </owl:ObjectProperty>
   <owl:ObjectProperty rdf:about="http://data.europa.eu/a4g/ontology#isCreatorOf">
      <rdfs:label xml:lang="en">Is creator of</rdfs:label>
      <skos:prefLabel xml:lang="en">Is creator of</skos:prefLabel>
      <rdfs:isDefinedBy rdf:resource="http://data.europa.eu/a4g/ontology"/>
   </owl:ObjectProperty>
   <owl:ObjectProperty rdf:about="http://data.europa.eu/a4g/ontology#submitsDocument">
      <rdfs:label xml:lang="en">Submits document</rdfs:label>
      <skos:prefLabel xml:lang="en">Submits document</skos:prefLabel>
      <skos:definition xml:lang="en">The transmitter of documents. 

Additional Information

An example of transmitters are TeD eSenders, which are usually either the Buyer or a Service Provider acting on behalf of the Buyer, qualified by the Publication Office of the European Union.

 (epo:Agent -&gt; epo:Document (+epo:submitsDocument)) </skos:definition>
      <rdfs:comment xml:lang="en">The transmitter of documents. 

Additional Information

An example of transmitters are TeD eSenders, which are usually either the Buyer or a Service Provider acting on behalf of the Buyer, qualified by the Publication Office of the European Union.

 (epo:Agent -&gt; epo:Document (+epo:submitsDocument)) </rdfs:comment>
      <rdfs:isDefinedBy rdf:resource="http://data.europa.eu/a4g/ontology"/>
   </owl:ObjectProperty>
   <owl:ObjectProperty rdf:about="http://data.europa.eu/a4g/ontology#actsOnBehalfOf">
      <rdfs:label xml:lang="en">Acts on behalf of</rdfs:label>
      <skos:prefLabel xml:lang="en">Acts on behalf of</skos:prefLabel>
      <rdfs:isDefinedBy rdf:resource="http://data.europa.eu/a4g/ontology"/>
   </owl:ObjectProperty>
   <owl:ObjectProperty rdf:about="http://data.europa.eu/a4g/ontology#delegatesAncillaryActivitiesOn">
      <rdfs:label xml:lang="en">Delegates ancillary activities on</rdfs:label>
      <skos:prefLabel xml:lang="en">Delegates ancillary activities on</skos:prefLabel>
      <rdfs:isDefinedBy rdf:resource="http://data.europa.eu/a4g/ontology"/>
   </owl:ObjectProperty>
   <owl:ObjectProperty rdf:about="http://data.europa.eu/a4g/ontology#isRoleOf">
      <rdfs:label xml:lang="en">Is role of</rdfs:label>
      <skos:prefLabel xml:lang="en">Is role of</skos:prefLabel>
      <skos:definition xml:lang="en">
 (epo:Agent &lt;-&gt; epo:ProcurementRole (+epo:hasRole +epo:isRoleOf)) </skos:definition>
      <rdfs:comment xml:lang="en">
 (epo:Agent &lt;-&gt; epo:ProcurementRole (+epo:hasRole +epo:isRoleOf)) </rdfs:comment>
      <rdfs:isDefinedBy rdf:resource="http://data.europa.eu/a4g/ontology"/>
   </owl:ObjectProperty>
   <owl:ObjectProperty rdf:about="http://data.europa.eu/a4g/ontology#hasRole">
      <rdfs:label xml:lang="en">Has role</rdfs:label>
      <skos:prefLabel xml:lang="en">Has role</skos:prefLabel>
      <skos:definition xml:lang="en">
 (epo:Agent &lt;-&gt; epo:ProcurementRole (+epo:hasRole +epo:isRoleOf)) </skos:definition>
      <rdfs:comment xml:lang="en">
 (epo:Agent &lt;-&gt; epo:ProcurementRole (+epo:hasRole +epo:isRoleOf)) </rdfs:comment>
      <skos:scopeNote xml:lang="en">The role in the context of procurement that is played by an agent in a specific procurement situation.
WG approval 09/09/2021 (epo:Agent &lt;-&gt; epo:ProcurementRole (+epo:hasRole +epo:isRoleOf)) </skos:scopeNote>
      <rdfs:comment xml:lang="en">The role in the context of procurement that is played by an agent in a specific procurement situation.
WG approval 09/09/2021 (epo:Agent &lt;-&gt; epo:ProcurementRole (+epo:hasRole +epo:isRoleOf)) </rdfs:comment>
      <rdfs:isDefinedBy rdf:resource="http://data.europa.eu/a4g/ontology"/>
   </owl:ObjectProperty>
   <owl:ObjectProperty rdf:about="http://data.europa.eu/a4g/ontology#isSignatoryPartyOf">
      <rdfs:label xml:lang="en">Is signatory party of</rdfs:label>
      <skos:prefLabel xml:lang="en">Is signatory party of</skos:prefLabel>
      <rdfs:isDefinedBy rdf:resource="http://data.europa.eu/a4g/ontology"/>
   </owl:ObjectProperty>
   <owl:ObjectProperty rdf:about="http://data.europa.eu/a4g/ontology#isSignedBy">
      <rdfs:label xml:lang="en">Is signed by</rdfs:label>
      <skos:prefLabel xml:lang="en">Is signed by</skos:prefLabel>
      <rdfs:isDefinedBy rdf:resource="http://data.europa.eu/a4g/ontology"/>
   </owl:ObjectProperty>
   <owl:ObjectProperty rdf:about="http://data.europa.eu/a4g/ontology#owns">
      <rdfs:label xml:lang="en">Owns</rdfs:label>
      <skos:prefLabel xml:lang="en">Owns</skos:prefLabel>
      <rdfs:isDefinedBy rdf:resource="http://data.europa.eu/a4g/ontology"/>
   </owl:ObjectProperty>
   <owl:ObjectProperty rdf:about="http://data.europa.eu/a4g/ontology#isOwnedBy">
      <rdfs:label xml:lang="en">Is owned by</rdfs:label>
      <skos:prefLabel xml:lang="en">Is owned by</skos:prefLabel>
      <rdfs:isDefinedBy rdf:resource="http://data.europa.eu/a4g/ontology"/>
   </owl:ObjectProperty>
   <owl:ObjectProperty rdf:about="http://data.europa.eu/a4g/ontology#hasEvaluationMember">
      <rdfs:label xml:lang="en">Has evaluation member</rdfs:label>
      <skos:prefLabel xml:lang="en">Has evaluation member</skos:prefLabel>
      <skos:scopeNote xml:lang="en">An agent involved in an evaluation board.
WG approval 14/09/2021 (epo:EvaluationBoard -&gt; epo:Agent (+epo:hasEvaluationMember)) </skos:scopeNote>
      <rdfs:comment xml:lang="en">An agent involved in an evaluation board.
WG approval 14/09/2021 (epo:EvaluationBoard -&gt; epo:Agent (+epo:hasEvaluationMember)) </rdfs:comment>
      <rdfs:isDefinedBy rdf:resource="http://data.europa.eu/a4g/ontology"/>
   </owl:ObjectProperty>
   <owl:ObjectProperty rdf:about="http://data.europa.eu/a4g/ontology#hasWeightValueType">
      <rdfs:label xml:lang="en">Has weight value type</rdfs:label>
      <skos:prefLabel xml:lang="en">Has weight value type</skos:prefLabel>
      <skos:definition xml:lang="en">The codelist to be used is at-voc:number-threshold which is available at https://op.europa.eu/en/web/eu-vocabularies/at-dataset/-/resource/dataset/number-weight
 (epo:AwardCriterion -&gt; at-voc:number-weight (+epo:hasWeightValueType)) The codelist to be used is at-voc:number-threshold which is available at https://op.europa.eu/en/web/eu-vocabularies/at-dataset/-/resource/dataset/number-weight
 (epo:SelectionCriterion -&gt; at-voc:number-weight (+epo:hasWeightValueType)) </skos:definition>
      <rdfs:comment xml:lang="en">The codelist to be used is at-voc:number-threshold which is available at https://op.europa.eu/en/web/eu-vocabularies/at-dataset/-/resource/dataset/number-weight
 (epo:AwardCriterion -&gt; at-voc:number-weight (+epo:hasWeightValueType)) The codelist to be used is at-voc:number-threshold which is available at https://op.europa.eu/en/web/eu-vocabularies/at-dataset/-/resource/dataset/number-weight
 (epo:SelectionCriterion -&gt; at-voc:number-weight (+epo:hasWeightValueType)) </rdfs:comment>
      <rdfs:isDefinedBy rdf:resource="http://data.europa.eu/a4g/ontology"/>
   </owl:ObjectProperty>
   <owl:ObjectProperty rdf:about="http://data.europa.eu/a4g/ontology#hasThresholdType">
      <rdfs:label xml:lang="en">Has threshold type</rdfs:label>
      <skos:prefLabel xml:lang="en">Has threshold type</skos:prefLabel>
      <skos:definition xml:lang="en">The codelist to be used is at-voc:number-threshold which is available at https://op.europa.eu/en/web/eu-vocabularies/at-dataset/-/resource/dataset/number-threshold
 (epo:AwardCriterion -&gt; at-voc:number-threshold (+epo:hasThresholdType)) The codelist to be used is at-voc:number-threshold which is available at https://op.europa.eu/en/web/eu-vocabularies/at-dataset/-/resource/dataset/number-threshold
 (epo:SelectionCriterion -&gt; at-voc:number-threshold (+epo:hasThresholdType)) </skos:definition>
      <rdfs:comment xml:lang="en">The codelist to be used is at-voc:number-threshold which is available at https://op.europa.eu/en/web/eu-vocabularies/at-dataset/-/resource/dataset/number-threshold
 (epo:AwardCriterion -&gt; at-voc:number-threshold (+epo:hasThresholdType)) The codelist to be used is at-voc:number-threshold which is available at https://op.europa.eu/en/web/eu-vocabularies/at-dataset/-/resource/dataset/number-threshold
 (epo:SelectionCriterion -&gt; at-voc:number-threshold (+epo:hasThresholdType)) </rdfs:comment>
      <rdfs:isDefinedBy rdf:resource="http://data.europa.eu/a4g/ontology"/>
   </owl:ObjectProperty>
   <owl:ObjectProperty rdf:about="http://data.europa.eu/a4g/ontology#isUsedToAward">
      <rdfs:label xml:lang="en">Is used to award</rdfs:label>
      <skos:prefLabel xml:lang="en">Is used to award</skos:prefLabel>
      <rdfs:isDefinedBy rdf:resource="http://data.europa.eu/a4g/ontology"/>
   </owl:ObjectProperty>
   <owl:ObjectProperty rdf:about="http://data.europa.eu/a4g/ontology#hasAwardCriterionType">
      <rdfs:label xml:lang="en">Has award criterion type</rdfs:label>
      <skos:prefLabel xml:lang="en">Has award criterion type</skos:prefLabel>
      <skos:definition xml:lang="en">The codelist to be used is at-voc:award-criterion-type which is available at https://op.europa.eu/web/eu-vocabularies/at-dataset/-/resource/dataset/award-criterion-type (epo:AwardCriterion -&gt; at-voc:award-criterion-type (+epo:hasAwardCriterionType)) </skos:definition>
      <rdfs:comment xml:lang="en">The codelist to be used is at-voc:award-criterion-type which is available at https://op.europa.eu/web/eu-vocabularies/at-dataset/-/resource/dataset/award-criterion-type (epo:AwardCriterion -&gt; at-voc:award-criterion-type (+epo:hasAwardCriterionType)) </rdfs:comment>
      <rdfs:isDefinedBy rdf:resource="http://data.europa.eu/a4g/ontology"/>
   </owl:ObjectProperty>
   <owl:ObjectProperty rdf:about="http://data.europa.eu/a4g/ontology#hasFixedValueType">
      <rdfs:label xml:lang="en">Has fixed value type</rdfs:label>
      <skos:prefLabel xml:lang="en">Has fixed value type</skos:prefLabel>
      <skos:definition xml:lang="en">The codelist to be used is at-voc:number-fixed which is available at https://op.europa.eu/en/web/eu-vocabularies/at-dataset/-/resource/dataset/number-fixed
 (epo:AwardCriterion -&gt; at-voc:number-fixed (+epo:hasFixedValueType)) </skos:definition>
      <rdfs:comment xml:lang="en">The codelist to be used is at-voc:number-fixed which is available at https://op.europa.eu/en/web/eu-vocabularies/at-dataset/-/resource/dataset/number-fixed
 (epo:AwardCriterion -&gt; at-voc:number-fixed (+epo:hasFixedValueType)) </rdfs:comment>
      <rdfs:isDefinedBy rdf:resource="http://data.europa.eu/a4g/ontology"/>
   </owl:ObjectProperty>
   <owl:ObjectProperty rdf:about="http://data.europa.eu/a4g/ontology#hasWinning">
      <rdfs:label xml:lang="en">Has winning</rdfs:label>
      <skos:prefLabel xml:lang="en">Has winning</skos:prefLabel>
      <rdfs:isDefinedBy rdf:resource="http://data.europa.eu/a4g/ontology"/>
   </owl:ObjectProperty>
   <owl:ObjectProperty rdf:about="http://data.europa.eu/a4g/ontology#hasAwardStatus">
      <rdfs:label xml:lang="en">Has award status</rdfs:label>
      <skos:prefLabel xml:lang="en">Has award status</skos:prefLabel>
      <skos:definition xml:lang="en">The codelist to be used is at-voc:winner-selection-status which is available at https://op.europa.eu/en/web/eu-vocabularies/at-dataset/-/resource/dataset/winner-selection-status
 (epo:AwardDecision -&gt; at-voc:winner-selection-status (+epo:hasAwardStatus)) </skos:definition>
      <rdfs:comment xml:lang="en">The codelist to be used is at-voc:winner-selection-status which is available at https://op.europa.eu/en/web/eu-vocabularies/at-dataset/-/resource/dataset/winner-selection-status
 (epo:AwardDecision -&gt; at-voc:winner-selection-status (+epo:hasAwardStatus)) </rdfs:comment>
      <rdfs:isDefinedBy rdf:resource="http://data.europa.eu/a4g/ontology"/>
   </owl:ObjectProperty>
   <owl:ObjectProperty rdf:about="http://data.europa.eu/a4g/ontology#isReferredByA">
      <rdfs:label xml:lang="en">Is referred by a</rdfs:label>
      <skos:prefLabel xml:lang="en">Is referred by a</skos:prefLabel>
      <rdfs:isDefinedBy rdf:resource="http://data.europa.eu/a4g/ontology"/>
   </owl:ObjectProperty>
   <owl:ObjectProperty rdf:about="http://data.europa.eu/a4g/ontology#isWinnerDefinedIn">
      <rdfs:label xml:lang="en">Is winner defined in</rdfs:label>
      <skos:prefLabel xml:lang="en">Is winner defined in</skos:prefLabel>
      <skos:scopeNote xml:lang="en">Relation indicating that a winner is defined in an award decision. (epo:AwardDecision &lt;-&gt; epo:Winner (+epo:specifiesWinner +epo:isWinnerDefinedIn)) </skos:scopeNote>
      <rdfs:comment xml:lang="en">Relation indicating that a winner is defined in an award decision. (epo:AwardDecision &lt;-&gt; epo:Winner (+epo:specifiesWinner +epo:isWinnerDefinedIn)) </rdfs:comment>
      <rdfs:isDefinedBy rdf:resource="http://data.europa.eu/a4g/ontology"/>
   </owl:ObjectProperty>
   <owl:ObjectProperty rdf:about="http://data.europa.eu/a4g/ontology#specifiesWinner">
      <rdfs:label xml:lang="en">Specifies winner</rdfs:label>
      <skos:prefLabel xml:lang="en">Specifies winner</skos:prefLabel>
      <skos:scopeNote xml:lang="en">Relation indicating that the AwardDecision defines a winner. (epo:AwardDecision &lt;-&gt; epo:Winner (+epo:specifiesWinner +epo:isWinnerDefinedIn)) </skos:scopeNote>
      <rdfs:comment xml:lang="en">Relation indicating that the AwardDecision defines a winner. (epo:AwardDecision &lt;-&gt; epo:Winner (+epo:specifiesWinner +epo:isWinnerDefinedIn)) </rdfs:comment>
      <rdfs:isDefinedBy rdf:resource="http://data.europa.eu/a4g/ontology"/>
   </owl:ObjectProperty>
   <owl:ObjectProperty rdf:about="http://data.europa.eu/a4g/ontology#refersTo">
      <rdfs:label xml:lang="en">Refers to</rdfs:label>
      <skos:prefLabel xml:lang="en">Refers to</skos:prefLabel>
      <rdfs:isDefinedBy rdf:resource="http://data.europa.eu/a4g/ontology"/>
   </owl:ObjectProperty>
   <owl:ObjectProperty rdf:about="http://data.europa.eu/a4g/ontology#hasNonAwardJustification">
      <rdfs:label xml:lang="en">Has non award justification</rdfs:label>
      <skos:prefLabel xml:lang="en">Has non award justification</skos:prefLabel>
      <skos:definition xml:lang="en">The codelist to be used is at-voc:non-award-justification which is available at https://op.europa.eu/en/web/eu-vocabularies/at-dataset/-/resource/dataset/non-award-justification
 (epo:AwardDecision -&gt; at-voc:non-award-justification (+epo:hasNonAwardJustification)) </skos:definition>
      <rdfs:comment xml:lang="en">The codelist to be used is at-voc:non-award-justification which is available at https://op.europa.eu/en/web/eu-vocabularies/at-dataset/-/resource/dataset/non-award-justification
 (epo:AwardDecision -&gt; at-voc:non-award-justification (+epo:hasNonAwardJustification)) </rdfs:comment>
      <rdfs:isDefinedBy rdf:resource="http://data.europa.eu/a4g/ontology"/>
   </owl:ObjectProperty>
   <owl:ObjectProperty rdf:about="http://data.europa.eu/a4g/ontology#hasSubcontract">
      <rdfs:label xml:lang="en">Has subcontract</rdfs:label>
      <skos:prefLabel xml:lang="en">Has subcontract</skos:prefLabel>
      <rdfs:isDefinedBy rdf:resource="http://data.europa.eu/a4g/ontology"/>
   </owl:ObjectProperty>
   <owl:ObjectProperty rdf:about="http://data.europa.eu/a4g/ontology#refersToAwardResult">
      <rdfs:label xml:lang="en">Refers to award result</rdfs:label>
      <skos:prefLabel xml:lang="en">Refers to award result</skos:prefLabel>
      <rdfs:isDefinedBy rdf:resource="http://data.europa.eu/a4g/ontology"/>
   </owl:ObjectProperty>
   <owl:ObjectProperty rdf:about="http://data.europa.eu/a4g/ontology#makesDecsion">
      <rdfs:label xml:lang="en">Makes decsion</rdfs:label>
      <skos:prefLabel xml:lang="en">Makes decsion</skos:prefLabel>
      <skos:scopeNote xml:lang="en">This decision may be made based on the evaluation results issued by the evaluation board. (epo:Buyer -&gt; epo:AwardDecision (+epo:makesDecsion)) </skos:scopeNote>
      <rdfs:comment xml:lang="en">This decision may be made based on the evaluation results issued by the evaluation board. (epo:Buyer -&gt; epo:AwardDecision (+epo:makesDecsion)) </rdfs:comment>
      <rdfs:isDefinedBy rdf:resource="http://data.europa.eu/a4g/ontology"/>
   </owl:ObjectProperty>
   <owl:ObjectProperty rdf:about="http://data.europa.eu/a4g/ontology#isNotifiedIn">
      <rdfs:label xml:lang="en">Is notified in</rdfs:label>
      <skos:prefLabel xml:lang="en">Is notified in</skos:prefLabel>
      <rdfs:isDefinedBy rdf:resource="http://data.europa.eu/a4g/ontology"/>
   </owl:ObjectProperty>
   <owl:ObjectProperty rdf:about="http://data.europa.eu/a4g/ontology#notifiesAwardResult">
      <rdfs:label xml:lang="en">Notifies award result</rdfs:label>
      <skos:prefLabel xml:lang="en">Notifies award result</skos:prefLabel>
      <rdfs:isDefinedBy rdf:resource="http://data.europa.eu/a4g/ontology"/>
   </owl:ObjectProperty>
   <owl:ObjectProperty rdf:about="http://data.europa.eu/a4g/ontology#acceptsProposalOf">
      <rdfs:label xml:lang="en">Accepts proposal of</rdfs:label>
      <skos:prefLabel xml:lang="en">Accepts proposal of</skos:prefLabel>
      <rdfs:isDefinedBy rdf:resource="http://data.europa.eu/a4g/ontology"/>
   </owl:ObjectProperty>
   <owl:ObjectProperty rdf:about="http://data.europa.eu/a4g/ontology#hasSize">
      <rdfs:label xml:lang="en">Has size</rdfs:label>
      <skos:prefLabel xml:lang="en">Has size</skos:prefLabel>
      <skos:definition xml:lang="en">The codelist to be used is at-voc:economic-operator-size which is available at https://op.europa.eu/en/web/eu-vocabularies/at-dataset/-/resource/dataset/economic-operator-size
 (epo:Business -&gt; at-voc:economic-operator-size (+epo:hasSize)) </skos:definition>
      <rdfs:comment xml:lang="en">The codelist to be used is at-voc:economic-operator-size which is available at https://op.europa.eu/en/web/eu-vocabularies/at-dataset/-/resource/dataset/economic-operator-size
 (epo:Business -&gt; at-voc:economic-operator-size (+epo:hasSize)) </rdfs:comment>
      <rdfs:isDefinedBy rdf:resource="http://data.europa.eu/a4g/ontology"/>
   </owl:ObjectProperty>
   <owl:ObjectProperty rdf:about="http://data.europa.eu/a4g/ontology#isBeneficialOwnerOf">
      <rdfs:label xml:lang="en">Is beneficial owner of</rdfs:label>
      <skos:prefLabel xml:lang="en">Is beneficial owner of</skos:prefLabel>
      <rdfs:isDefinedBy rdf:resource="http://data.europa.eu/a4g/ontology"/>
   </owl:ObjectProperty>
   <owl:ObjectProperty rdf:about="http://data.europa.eu/a4g/ontology#hasBeneficialOwner">
      <rdfs:label xml:lang="en">Has beneficial owner</rdfs:label>
      <skos:prefLabel xml:lang="en">Has beneficial owner</skos:prefLabel>
      <skos:scopeNote xml:lang="en">A role of any natural person(s) who ultimately owns or controls the organisation or on whose behalf a transaction or activity is being conducted.
Additional Information:
This role is defined in the directive EU 2015/849 and it's beyond the scope for public eProcurement domain.
WG approval 14/09/2021 (epo:Business &lt;-&gt; epo:Person (+epo:hasBeneficialOwner +epo:isBeneficialOwnerOf)) </skos:scopeNote>
      <rdfs:comment xml:lang="en">A role of any natural person(s) who ultimately owns or controls the organisation or on whose behalf a transaction or activity is being conducted.
Additional Information:
This role is defined in the directive EU 2015/849 and it's beyond the scope for public eProcurement domain.
WG approval 14/09/2021 (epo:Business &lt;-&gt; epo:Person (+epo:hasBeneficialOwner +epo:isBeneficialOwnerOf)) </rdfs:comment>
      <rdfs:isDefinedBy rdf:resource="http://data.europa.eu/a4g/ontology"/>
   </owl:ObjectProperty>
   <owl:ObjectProperty rdf:about="http://data.europa.eu/a4g/ontology#isRoleOfBusiness">
      <rdfs:label xml:lang="en">Is role of business</rdfs:label>
      <skos:prefLabel xml:lang="en">Is role of business</skos:prefLabel>
      <rdfs:isDefinedBy rdf:resource="http://data.europa.eu/a4g/ontology"/>
   </owl:ObjectProperty>
   <owl:ObjectProperty rdf:about="http://data.europa.eu/a4g/ontology#hasMainActivityType">
      <rdfs:label xml:lang="en">Has main activity type</rdfs:label>
      <skos:prefLabel xml:lang="en">Has main activity type</skos:prefLabel>
      <skos:definition xml:lang="en">The codelist to be used is at-voc:main-activity which is available at https://op.europa.eu/en/web/eu-vocabularies/at-dataset/-/resource/dataset/main-activity
 (epo:Buyer -&gt; at-voc:main-activity (+epo:hasMainActivityType)) </skos:definition>
      <rdfs:comment xml:lang="en">The codelist to be used is at-voc:main-activity which is available at https://op.europa.eu/en/web/eu-vocabularies/at-dataset/-/resource/dataset/main-activity
 (epo:Buyer -&gt; at-voc:main-activity (+epo:hasMainActivityType)) </rdfs:comment>
      <rdfs:isDefinedBy rdf:resource="http://data.europa.eu/a4g/ontology"/>
   </owl:ObjectProperty>
   <owl:ObjectProperty rdf:about="http://data.europa.eu/a4g/ontology#executesPayment">
      <rdfs:label xml:lang="en">Executes payment</rdfs:label>
      <skos:prefLabel xml:lang="en">Executes payment</skos:prefLabel>
      <rdfs:isDefinedBy rdf:resource="http://data.europa.eu/a4g/ontology"/>
   </owl:ObjectProperty>
   <owl:ObjectProperty rdf:about="http://data.europa.eu/a4g/ontology#processesTenders">
      <rdfs:label xml:lang="en">Processes tenders</rdfs:label>
      <skos:prefLabel xml:lang="en">Processes tenders</skos:prefLabel>
      <rdfs:isDefinedBy rdf:resource="http://data.europa.eu/a4g/ontology"/>
   </owl:ObjectProperty>
   <owl:ObjectProperty rdf:about="http://data.europa.eu/a4g/ontology#hasBuyerWebsite">
      <rdfs:label xml:lang="en">Has buyer website</rdfs:label>
      <skos:prefLabel xml:lang="en">Has buyer website</skos:prefLabel>
      <skos:scopeNote xml:lang="en">Relation indicating the website of the buyer. (epo:Buyer -&gt; epo:BuyerProfile (+epo:hasBuyerWebsite)) </skos:scopeNote>
      <rdfs:comment xml:lang="en">Relation indicating the website of the buyer. (epo:Buyer -&gt; epo:BuyerProfile (+epo:hasBuyerWebsite)) </rdfs:comment>
      <rdfs:isDefinedBy rdf:resource="http://data.europa.eu/a4g/ontology"/>
   </owl:ObjectProperty>
   <owl:ObjectProperty rdf:about="http://data.europa.eu/a4g/ontology#processesRequestsToParticipate">
      <rdfs:label xml:lang="en">Processes requests to participate</rdfs:label>
      <skos:prefLabel xml:lang="en">Processes requests to participate</skos:prefLabel>
      <rdfs:isDefinedBy rdf:resource="http://data.europa.eu/a4g/ontology"/>
   </owl:ObjectProperty>
   <owl:ObjectProperty rdf:about="http://data.europa.eu/a4g/ontology#providiesMoreInformationOnTimeLimitsForReviewProcedures">
      <rdfs:label xml:lang="en">Providies more information on time limits for review procedures</rdfs:label>
      <skos:prefLabel xml:lang="en">Providies more information on time limits for review procedures</skos:prefLabel>
      <rdfs:isDefinedBy rdf:resource="http://data.europa.eu/a4g/ontology"/>
   </owl:ObjectProperty>
   <owl:ObjectProperty rdf:about="http://data.europa.eu/a4g/ontology#receivesRequestsToParticipate">
      <rdfs:label xml:lang="en">Receives requests to participate</rdfs:label>
      <skos:prefLabel xml:lang="en">Receives requests to participate</skos:prefLabel>
      <rdfs:isDefinedBy rdf:resource="http://data.europa.eu/a4g/ontology"/>
   </owl:ObjectProperty>
   <owl:ObjectProperty rdf:about="http://data.europa.eu/a4g/ontology#isGroupLeader">
      <rdfs:label xml:lang="en">Is group leader</rdfs:label>
      <skos:prefLabel xml:lang="en">Is group leader</skos:prefLabel>
      <rdfs:isDefinedBy rdf:resource="http://data.europa.eu/a4g/ontology"/>
   </owl:ObjectProperty>
   <owl:ObjectProperty rdf:about="http://data.europa.eu/a4g/ontology#appointedBy">
      <rdfs:label xml:lang="en">Appointed by</rdfs:label>
      <skos:prefLabel xml:lang="en">Appointed by</skos:prefLabel>
      <rdfs:isDefinedBy rdf:resource="http://data.europa.eu/a4g/ontology"/>
   </owl:ObjectProperty>
   <owl:ObjectProperty rdf:about="http://data.europa.eu/a4g/ontology#appoints">
      <rdfs:label xml:lang="en">Appoints</rdfs:label>
      <skos:prefLabel xml:lang="en">Appoints</skos:prefLabel>
      <rdfs:isDefinedBy rdf:resource="http://data.europa.eu/a4g/ontology"/>
   </owl:ObjectProperty>
   <owl:ObjectProperty rdf:about="http://data.europa.eu/a4g/ontology#providesAdditionalInformationAboutProcurementProcedure">
      <rdfs:label xml:lang="en">Provides additional information about procurement procedure</rdfs:label>
      <skos:prefLabel xml:lang="en">Provides additional information about procurement procedure</skos:prefLabel>
      <rdfs:isDefinedBy rdf:resource="http://data.europa.eu/a4g/ontology"/>
   </owl:ObjectProperty>
   <owl:ObjectProperty rdf:about="http://data.europa.eu/a4g/ontology#usesBudgetToPayContract">
      <rdfs:label xml:lang="en">Uses budget to pay contract</rdfs:label>
      <skos:prefLabel xml:lang="en">Uses budget to pay contract</skos:prefLabel>
      <rdfs:isDefinedBy rdf:resource="http://data.europa.eu/a4g/ontology"/>
   </owl:ObjectProperty>
   <owl:ObjectProperty rdf:about="http://data.europa.eu/a4g/ontology#receivesTenders">
      <rdfs:label xml:lang="en">Receives tenders</rdfs:label>
      <skos:prefLabel xml:lang="en">Receives tenders</skos:prefLabel>
      <rdfs:isDefinedBy rdf:resource="http://data.europa.eu/a4g/ontology"/>
   </owl:ObjectProperty>
   <owl:ObjectProperty rdf:about="http://data.europa.eu/a4g/ontology#hasBuyerType">
      <rdfs:label xml:lang="en">Has buyer type</rdfs:label>
      <skos:prefLabel xml:lang="en">Has buyer type</skos:prefLabel>
      <skos:definition xml:lang="en">The codelist to be used is at-voc:buyer-legal-type which is available at https://op.europa.eu/web/eu-vocabularies/at-dataset/-/resource/dataset/buyer-legal-type (epo:Buyer -&gt; at-voc:buyer-legal-type (+epo:hasBuyerType)) </skos:definition>
      <rdfs:comment xml:lang="en">The codelist to be used is at-voc:buyer-legal-type which is available at https://op.europa.eu/web/eu-vocabularies/at-dataset/-/resource/dataset/buyer-legal-type (epo:Buyer -&gt; at-voc:buyer-legal-type (+epo:hasBuyerType)) </rdfs:comment>
      <rdfs:isDefinedBy rdf:resource="http://data.europa.eu/a4g/ontology"/>
   </owl:ObjectProperty>
   <owl:ObjectProperty rdf:about="http://data.europa.eu/a4g/ontology#providesOfflineAccessToProcurementDocuments">
      <rdfs:label xml:lang="en">Provides offline access to procurement documents</rdfs:label>
      <skos:prefLabel xml:lang="en">Provides offline access to procurement documents</skos:prefLabel>
      <rdfs:isDefinedBy rdf:resource="http://data.europa.eu/a4g/ontology"/>
   </owl:ObjectProperty>
   <owl:ObjectProperty rdf:about="http://data.europa.eu/a4g/ontology#isPlannedBy">
      <rdfs:label xml:lang="en">Is planned by</rdfs:label>
      <skos:prefLabel xml:lang="en">Is planned by</skos:prefLabel>
      <rdfs:isDefinedBy rdf:resource="http://data.europa.eu/a4g/ontology"/>
   </owl:ObjectProperty>
   <owl:ObjectProperty rdf:about="http://data.europa.eu/a4g/ontology#plans">
      <rdfs:label xml:lang="en">Plans</rdfs:label>
      <skos:prefLabel xml:lang="en">Plans</skos:prefLabel>
      <rdfs:isDefinedBy rdf:resource="http://data.europa.eu/a4g/ontology"/>
   </owl:ObjectProperty>
   <owl:ObjectProperty rdf:about="http://data.europa.eu/a4g/ontology#signsContract">
      <rdfs:label xml:lang="en">Signs contract</rdfs:label>
      <skos:prefLabel xml:lang="en">Signs contract</skos:prefLabel>
      <rdfs:isDefinedBy rdf:resource="http://data.europa.eu/a4g/ontology"/>
   </owl:ObjectProperty>
   <owl:ObjectProperty rdf:about="http://data.europa.eu/a4g/ontology#isResponsibleFor">
      <rdfs:label xml:lang="en">Is responsible for</rdfs:label>
      <skos:prefLabel xml:lang="en">Is responsible for</skos:prefLabel>
      <rdfs:isDefinedBy rdf:resource="http://data.europa.eu/a4g/ontology"/>
   </owl:ObjectProperty>
   <owl:ObjectProperty rdf:about="http://data.europa.eu/a4g/ontology#isResponsiblityOf">
      <rdfs:label xml:lang="en">Is responsiblity of</rdfs:label>
      <skos:prefLabel xml:lang="en">Is responsiblity of</skos:prefLabel>
      <rdfs:isDefinedBy rdf:resource="http://data.europa.eu/a4g/ontology"/>
   </owl:ObjectProperty>
   <owl:ObjectProperty rdf:about="http://data.europa.eu/a4g/ontology#manages">
      <rdfs:label xml:lang="en">Manages</rdfs:label>
      <skos:prefLabel xml:lang="en">Manages</skos:prefLabel>
      <rdfs:isDefinedBy rdf:resource="http://data.europa.eu/a4g/ontology"/>
   </owl:ObjectProperty>
   <owl:ObjectProperty rdf:about="http://data.europa.eu/a4g/ontology#notifies">
      <rdfs:label xml:lang="en">Notifies</rdfs:label>
      <skos:prefLabel xml:lang="en">Notifies</skos:prefLabel>
      <rdfs:isDefinedBy rdf:resource="http://data.europa.eu/a4g/ontology"/>
   </owl:ObjectProperty>
   <owl:ObjectProperty rdf:about="http://data.europa.eu/a4g/ontology#isNotifiedThrough">
      <rdfs:label xml:lang="en">Is notified through</rdfs:label>
      <skos:prefLabel xml:lang="en">Is notified through</skos:prefLabel>
      <skos:scopeNote xml:lang="en">[only CN or PIN] (epo:CallForCompetition &lt;-&gt; epo:Notice (+epo:isNotifiedThrough +epo:notifies)) </skos:scopeNote>
      <rdfs:comment xml:lang="en">[only CN or PIN] (epo:CallForCompetition &lt;-&gt; epo:Notice (+epo:isNotifiedThrough +epo:notifies)) </rdfs:comment>
      <rdfs:isDefinedBy rdf:resource="http://data.europa.eu/a4g/ontology"/>
   </owl:ObjectProperty>
   <owl:ObjectProperty rdf:about="http://data.europa.eu/a4g/ontology#refersToADifferent">
      <rdfs:label xml:lang="en">Refers to a different</rdfs:label>
      <skos:prefLabel xml:lang="en">Refers to a different</skos:prefLabel>
      <rdfs:isDefinedBy rdf:resource="http://data.europa.eu/a4g/ontology"/>
   </owl:ObjectProperty>
   <owl:ObjectProperty rdf:about="http://data.europa.eu/a4g/ontology#hasChangeElement">
      <rdfs:label xml:lang="en">Has change element</rdfs:label>
      <skos:prefLabel xml:lang="en">Has change element</skos:prefLabel>
      <rdfs:isDefinedBy rdf:resource="http://data.europa.eu/a4g/ontology"/>
   </owl:ObjectProperty>
   <owl:ObjectProperty rdf:about="http://data.europa.eu/a4g/ontology#hasChangeReason">
      <rdfs:label xml:lang="en">Has change reason</rdfs:label>
      <skos:prefLabel xml:lang="en">Has change reason</skos:prefLabel>
      <skos:definition xml:lang="en">The codelist to be used is at-voc:change-corrig-justification which is available at https://op.europa.eu/en/web/eu-vocabularies/at-dataset/-/resource/dataset/change-corrig-justification
 (epo:Change -&gt; at-voc:change-corrig-justification (+epo:hasChangeReason)) </skos:definition>
      <rdfs:comment xml:lang="en">The codelist to be used is at-voc:change-corrig-justification which is available at https://op.europa.eu/en/web/eu-vocabularies/at-dataset/-/resource/dataset/change-corrig-justification
 (epo:Change -&gt; at-voc:change-corrig-justification (+epo:hasChangeReason)) </rdfs:comment>
      <rdfs:isDefinedBy rdf:resource="http://data.europa.eu/a4g/ontology"/>
   </owl:ObjectProperty>
   <owl:ObjectProperty rdf:about="http://data.europa.eu/a4g/ontology#hasChange">
      <rdfs:label xml:lang="en">Has change</rdfs:label>
      <skos:prefLabel xml:lang="en">Has change</skos:prefLabel>
      <rdfs:isDefinedBy rdf:resource="http://data.europa.eu/a4g/ontology"/>
   </owl:ObjectProperty>
   <owl:ObjectProperty rdf:about="http://data.europa.eu/a4g/ontology#hasSubmissionCommunicationMeans">
      <rdfs:label xml:lang="en">Has submission communication means</rdfs:label>
      <skos:prefLabel xml:lang="en">Has submission communication means</skos:prefLabel>
      <rdfs:isDefinedBy rdf:resource="http://data.europa.eu/a4g/ontology"/>
   </owl:ObjectProperty>
   <owl:ObjectProperty rdf:about="http://data.europa.eu/a4g/ontology#hasChannel">
      <rdfs:label xml:lang="en">Has channel</rdfs:label>
      <skos:prefLabel xml:lang="en">Has channel</skos:prefLabel>
      <rdfs:isDefinedBy rdf:resource="http://data.europa.eu/a4g/ontology"/>
   </owl:ObjectProperty>
   <owl:ObjectProperty rdf:about="http://data.europa.eu/a4g/ontology#isMadeAvailableVia">
      <rdfs:label xml:lang="en">Is made available via</rdfs:label>
      <skos:prefLabel xml:lang="en">Is made available via</skos:prefLabel>
      <rdfs:isDefinedBy rdf:resource="http://data.europa.eu/a4g/ontology"/>
   </owl:ObjectProperty>
   <owl:ObjectProperty rdf:about="http://data.europa.eu/a4g/ontology#hasClarificationsAvailableVia">
      <rdfs:label xml:lang="en">Has clarifications available via</rdfs:label>
      <skos:prefLabel xml:lang="en">Has clarifications available via</skos:prefLabel>
      <rdfs:isDefinedBy rdf:resource="http://data.europa.eu/a4g/ontology"/>
   </owl:ObjectProperty>
   <owl:ObjectProperty rdf:about="http://data.europa.eu/a4g/ontology#isAvailableVia">
      <rdfs:label xml:lang="en">Is available via</rdfs:label>
      <skos:prefLabel xml:lang="en">Is available via</skos:prefLabel>
      <rdfs:isDefinedBy rdf:resource="http://data.europa.eu/a4g/ontology"/>
   </owl:ObjectProperty>
   <owl:ObjectProperty rdf:about="http://data.europa.eu/a4g/ontology#usesAdhoc">
      <rdfs:label xml:lang="en">Uses adhoc</rdfs:label>
      <skos:prefLabel xml:lang="en">Uses adhoc</skos:prefLabel>
      <rdfs:isDefinedBy rdf:resource="http://data.europa.eu/a4g/ontology"/>
   </owl:ObjectProperty>
   <owl:ObjectProperty rdf:about="http://data.europa.eu/a4g/ontology#hasQuestionsMadeAvailableVia">
      <rdfs:label xml:lang="en">Has questions made available via</rdfs:label>
      <skos:prefLabel xml:lang="en">Has questions made available via</skos:prefLabel>
      <rdfs:isDefinedBy rdf:resource="http://data.europa.eu/a4g/ontology"/>
   </owl:ObjectProperty>
   <owl:ObjectProperty rdf:about="http://data.europa.eu/a4g/ontology#hasVirtualTenderOpeningAddress">
      <rdfs:label xml:lang="en">Has virtual tender opening address</rdfs:label>
      <skos:prefLabel xml:lang="en">Has virtual tender opening address</skos:prefLabel>
      <rdfs:isDefinedBy rdf:resource="http://data.europa.eu/a4g/ontology"/>
   </owl:ObjectProperty>
   <owl:ObjectProperty rdf:about="http://data.europa.eu/a4g/ontology#isPersonOfContact">
      <rdfs:label xml:lang="en">Is person of contact</rdfs:label>
      <skos:prefLabel xml:lang="en">Is person of contact</skos:prefLabel>
      <rdfs:isDefinedBy rdf:resource="http://data.europa.eu/a4g/ontology"/>
   </owl:ObjectProperty>
   <owl:ObjectProperty rdf:about="http://data.europa.eu/a4g/ontology#hasContactPersonRole">
      <rdfs:label xml:lang="en">Has contact person role</rdfs:label>
      <skos:prefLabel xml:lang="en">Has contact person role</skos:prefLabel>
      <rdfs:isDefinedBy rdf:resource="http://data.europa.eu/a4g/ontology"/>
   </owl:ObjectProperty>
   <owl:ObjectProperty rdf:about="http://data.europa.eu/a4g/ontology#hasContactPoint">
      <rdfs:label xml:lang="en">Has contact point</rdfs:label>
      <skos:prefLabel xml:lang="en">Has contact point</skos:prefLabel>
      <rdfs:isDefinedBy rdf:resource="http://data.europa.eu/a4g/ontology"/>
   </owl:ObjectProperty>
   <owl:ObjectProperty rdf:about="http://data.europa.eu/a4g/ontology#hasDefaultContactPoint">
      <rdfs:label xml:lang="en">Has default contact point</rdfs:label>
      <skos:prefLabel xml:lang="en">Has default contact point</skos:prefLabel>
      <skos:definition xml:lang="en">To be discussed 30/04/2020 (epo:Organisation -&gt; epo:ContactPoint (+epo:hasDefaultContactPoint)) </skos:definition>
      <rdfs:comment xml:lang="en">To be discussed 30/04/2020 (epo:Organisation -&gt; epo:ContactPoint (+epo:hasDefaultContactPoint)) </rdfs:comment>
      <rdfs:isDefinedBy rdf:resource="http://data.europa.eu/a4g/ontology"/>
   </owl:ObjectProperty>
   <owl:ObjectProperty rdf:about="http://data.europa.eu/a4g/ontology#funds">
      <rdfs:label xml:lang="en">Funds</rdfs:label>
      <skos:prefLabel xml:lang="en">Funds</skos:prefLabel>
      <skos:definition xml:lang="en">Funds may change between the lot and the contract, for example in the case of an emergency crisis, a contract may be financed by a budget that was not foreseen in the call.
 (epo:Contract &lt;-&gt; epo:Fund (+epo:isFundedBy +epo:funds)) </skos:definition>
      <rdfs:comment xml:lang="en">Funds may change between the lot and the contract, for example in the case of an emergency crisis, a contract may be financed by a budget that was not foreseen in the call.
 (epo:Contract &lt;-&gt; epo:Fund (+epo:isFundedBy +epo:funds)) </rdfs:comment>
      <rdfs:isDefinedBy rdf:resource="http://data.europa.eu/a4g/ontology"/>
   </owl:ObjectProperty>
   <owl:ObjectProperty rdf:about="http://data.europa.eu/a4g/ontology#isFundedBy">
      <rdfs:label xml:lang="en">Is funded by</rdfs:label>
      <skos:prefLabel xml:lang="en">Is funded by</skos:prefLabel>
      <skos:definition xml:lang="en">Funds may change between the lot and the contract, for example in the case of an emergency crisis, a contract may be financed by a budget that was not foreseen in the call.
 (epo:Contract &lt;-&gt; epo:Fund (+epo:isFundedBy +epo:funds)) Funds may change between the lot and the contract, for example in the case of an emergency crisis, a contract may be financed by a budget that was not foreseen in the call. (epo:Lot -&gt; epo:Fund (+epo:isFundedBy)) </skos:definition>
      <rdfs:comment xml:lang="en">Funds may change between the lot and the contract, for example in the case of an emergency crisis, a contract may be financed by a budget that was not foreseen in the call.
 (epo:Contract &lt;-&gt; epo:Fund (+epo:isFundedBy +epo:funds)) Funds may change between the lot and the contract, for example in the case of an emergency crisis, a contract may be financed by a budget that was not foreseen in the call. (epo:Lot -&gt; epo:Fund (+epo:isFundedBy)) </rdfs:comment>
      <rdfs:isDefinedBy rdf:resource="http://data.europa.eu/a4g/ontology"/>
   </owl:ObjectProperty>
   <owl:ObjectProperty rdf:about="http://data.europa.eu/a4g/ontology#isAttachedIn">
      <rdfs:label xml:lang="en">Is attached in</rdfs:label>
      <skos:prefLabel xml:lang="en">Is attached in</skos:prefLabel>
      <skos:scopeNote xml:lang="en">Relation indicating a document is included in a Thing. (epo:Contract &lt;-&gt; epo:Document (+epo:attaches +epo:isAttachedIn)) Relation indicating a document is included in a Thing. (epo:Tender &lt;-&gt; epo:TenderDocument (+epo:attaches +epo:isAttachedIn)) </skos:scopeNote>
      <rdfs:comment xml:lang="en">Relation indicating a document is included in a Thing. (epo:Contract &lt;-&gt; epo:Document (+epo:attaches +epo:isAttachedIn)) Relation indicating a document is included in a Thing. (epo:Tender &lt;-&gt; epo:TenderDocument (+epo:attaches +epo:isAttachedIn)) </rdfs:comment>
      <rdfs:isDefinedBy rdf:resource="http://data.europa.eu/a4g/ontology"/>
   </owl:ObjectProperty>
   <owl:ObjectProperty rdf:about="http://data.europa.eu/a4g/ontology#attaches">
      <rdfs:label xml:lang="en">Attaches</rdfs:label>
      <skos:prefLabel xml:lang="en">Attaches</skos:prefLabel>
      <skos:scopeNote xml:lang="en">Relation indicating that a Thing includes a Document. (epo:Contract &lt;-&gt; epo:Document (+epo:attaches +epo:isAttachedIn)) Relation indicating that a Thing includes a Document. (epo:Tender &lt;-&gt; epo:TenderDocument (+epo:attaches +epo:isAttachedIn)) </skos:scopeNote>
      <rdfs:comment xml:lang="en">Relation indicating that a Thing includes a Document. (epo:Contract &lt;-&gt; epo:Document (+epo:attaches +epo:isAttachedIn)) Relation indicating that a Thing includes a Document. (epo:Tender &lt;-&gt; epo:TenderDocument (+epo:attaches +epo:isAttachedIn)) </rdfs:comment>
      <rdfs:isDefinedBy rdf:resource="http://data.europa.eu/a4g/ontology"/>
   </owl:ObjectProperty>
   <owl:ObjectProperty rdf:about="http://data.europa.eu/a4g/ontology#refersToSignatory">
      <rdfs:label xml:lang="en">Refers to signatory</rdfs:label>
      <skos:prefLabel xml:lang="en">Refers to signatory</skos:prefLabel>
      <rdfs:isDefinedBy rdf:resource="http://data.europa.eu/a4g/ontology"/>
   </owl:ObjectProperty>
   <owl:ObjectProperty rdf:about="http://data.europa.eu/a4g/ontology#hasDuration">
      <rdfs:label xml:lang="en">Has duration</rdfs:label>
      <skos:prefLabel xml:lang="en">Has duration</skos:prefLabel>
      <rdfs:isDefinedBy rdf:resource="http://data.europa.eu/a4g/ontology"/>
   </owl:ObjectProperty>
   <owl:ObjectProperty rdf:about="http://data.europa.eu/a4g/ontology#mentions">
      <rdfs:label xml:lang="en">Mentions</rdfs:label>
      <skos:prefLabel xml:lang="en">Mentions</skos:prefLabel>
      <rdfs:isDefinedBy rdf:resource="http://data.europa.eu/a4g/ontology"/>
   </owl:ObjectProperty>
   <owl:ObjectProperty rdf:about="http://data.europa.eu/a4g/ontology#hasEstimatedDuration">
      <rdfs:label xml:lang="en">Has estimated duration</rdfs:label>
      <skos:prefLabel xml:lang="en">Has estimated duration</skos:prefLabel>
      <rdfs:isDefinedBy rdf:resource="http://data.europa.eu/a4g/ontology"/>
   </owl:ObjectProperty>
   <owl:ObjectProperty rdf:about="http://data.europa.eu/a4g/ontology#hasProcurementValue">
      <rdfs:label xml:lang="en">Has procurement value</rdfs:label>
      <skos:prefLabel xml:lang="en">Has procurement value</skos:prefLabel>
      <skos:definition xml:lang="en">At contract time, this procurement value may be different from the Procurement Value of a Lot or a Procedure that was announced. (epo:Contract -&gt; epo:Value (+epo:hasProcurementValue)) </skos:definition>
      <rdfs:comment xml:lang="en">At contract time, this procurement value may be different from the Procurement Value of a Lot or a Procedure that was announced. (epo:Contract -&gt; epo:Value (+epo:hasProcurementValue)) </rdfs:comment>
      <rdfs:isDefinedBy rdf:resource="http://data.europa.eu/a4g/ontology"/>
   </owl:ObjectProperty>
   <owl:ObjectProperty rdf:about="http://data.europa.eu/a4g/ontology#hasDurationEvaluationPeriod">
      <rdfs:label xml:lang="en">Has duration evaluation period</rdfs:label>
      <skos:prefLabel xml:lang="en">Has duration evaluation period</skos:prefLabel>
      <rdfs:isDefinedBy rdf:resource="http://data.europa.eu/a4g/ontology"/>
   </owl:ObjectProperty>
   <owl:ObjectProperty rdf:about="http://data.europa.eu/a4g/ontology#hasContractPurpose">
      <rdfs:label xml:lang="en">Has contract purpose</rdfs:label>
      <skos:prefLabel xml:lang="en">Has contract purpose</skos:prefLabel>
      <rdfs:isDefinedBy rdf:resource="http://data.europa.eu/a4g/ontology"/>
   </owl:ObjectProperty>
   <owl:ObjectProperty rdf:about="http://data.europa.eu/a4g/ontology#modifies">
      <rdfs:label xml:lang="en">Modifies</rdfs:label>
      <skos:prefLabel xml:lang="en">Modifies</skos:prefLabel>
      <rdfs:isDefinedBy rdf:resource="http://data.europa.eu/a4g/ontology"/>
   </owl:ObjectProperty>
   <owl:ObjectProperty rdf:about="http://data.europa.eu/a4g/ontology#leadsTo">
      <rdfs:label xml:lang="en">Leads to</rdfs:label>
      <skos:prefLabel xml:lang="en">Leads to</skos:prefLabel>
      <rdfs:isDefinedBy rdf:resource="http://data.europa.eu/a4g/ontology"/>
   </owl:ObjectProperty>
   <owl:ObjectProperty rdf:about="http://data.europa.eu/a4g/ontology#concludes">
      <rdfs:label xml:lang="en">Concludes</rdfs:label>
      <skos:prefLabel xml:lang="en">Concludes</skos:prefLabel>
      <rdfs:isDefinedBy rdf:resource="http://data.europa.eu/a4g/ontology"/>
   </owl:ObjectProperty>
   <owl:ObjectProperty rdf:about="http://data.europa.eu/a4g/ontology#isConcludedBy">
      <rdfs:label xml:lang="en">Is concluded by</rdfs:label>
      <skos:prefLabel xml:lang="en">Is concluded by</skos:prefLabel>
      <rdfs:isDefinedBy rdf:resource="http://data.europa.eu/a4g/ontology"/>
   </owl:ObjectProperty>
   <owl:ObjectProperty rdf:about="http://data.europa.eu/a4g/ontology#hasTotalFrameworkValue">
      <rdfs:label xml:lang="en">Has total framework value</rdfs:label>
      <skos:prefLabel xml:lang="en">Has total framework value</skos:prefLabel>
      <skos:definition xml:lang="en">The maximum value which can be spent through all the framework agreements announced in this notice, including options and renewals of contracts.

Additional information:

The value provided is a threshold value that implicity means that it cannot be exceeded however it may not be reached during the execution of a contract.

The Framework Agreements in a CAN are to be traced back and added to provide this value. The path to get the value of an individual Framework Agreement is:

CAN isA Notice,
CAN notifiesAwardResult AwardDecision,
AwardDecision refersTo Lot,
Lot uses Technique, 
FrameworkAgreement isA Technique,
FrameworkAgreement hasAwardedValue ProcurementValue .

WG Approval 03/12/2019

 (epo:ContractAwardNotice -&gt; epo:Value (+epo:hasTotalFrameworkValue)) </skos:definition>
      <rdfs:comment xml:lang="en">The maximum value which can be spent through all the framework agreements announced in this notice, including options and renewals of contracts.

Additional information:

The value provided is a threshold value that implicity means that it cannot be exceeded however it may not be reached during the execution of a contract.

The Framework Agreements in a CAN are to be traced back and added to provide this value. The path to get the value of an individual Framework Agreement is:

CAN isA Notice,
CAN notifiesAwardResult AwardDecision,
AwardDecision refersTo Lot,
Lot uses Technique, 
FrameworkAgreement isA Technique,
FrameworkAgreement hasAwardedValue ProcurementValue .

WG Approval 03/12/2019

 (epo:ContractAwardNotice -&gt; epo:Value (+epo:hasTotalFrameworkValue)) </rdfs:comment>
      <rdfs:isDefinedBy rdf:resource="http://data.europa.eu/a4g/ontology"/>
   </owl:ObjectProperty>
   <owl:ObjectProperty rdf:about="http://data.europa.eu/a4g/ontology#hasTotalValue">
      <rdfs:label xml:lang="en">Has total value</rdfs:label>
      <skos:prefLabel xml:lang="en">Has total value</skos:prefLabel>
      <skos:definition xml:lang="en">The value of all lots awarded for this notice, including options and renewals. 

Additional information:
The values of the individual Lots awarded under a framework agreement and mentioned in this notice are included.

The values of the individual lots announced in a CAN are to be traced back and added to provide this value.

The path to get the value of an individual Lot is:

CAN isA Notice ,
CAN notifiesAwardResult AwardDecision ,
AwardDecision refersTo Lot ,
hasAwardedValue ProcurementValue .

WG Approval 03/12/2019
 (epo:ContractAwardNotice -&gt; epo:Value (+epo:hasTotalValue)) </skos:definition>
      <rdfs:comment xml:lang="en">The value of all lots awarded for this notice, including options and renewals. 

Additional information:
The values of the individual Lots awarded under a framework agreement and mentioned in this notice are included.

The values of the individual lots announced in a CAN are to be traced back and added to provide this value.

The path to get the value of an individual Lot is:

CAN isA Notice ,
CAN notifiesAwardResult AwardDecision ,
AwardDecision refersTo Lot ,
hasAwardedValue ProcurementValue .

WG Approval 03/12/2019
 (epo:ContractAwardNotice -&gt; epo:Value (+epo:hasTotalValue)) </rdfs:comment>
      <rdfs:isDefinedBy rdf:resource="http://data.europa.eu/a4g/ontology"/>
   </owl:ObjectProperty>
   <owl:ObjectProperty rdf:about="http://data.europa.eu/a4g/ontology#isSummarisedBy">
      <rdfs:label xml:lang="en">Is summarised by</rdfs:label>
      <skos:prefLabel xml:lang="en">Is summarised by</skos:prefLabel>
      <rdfs:isDefinedBy rdf:resource="http://data.europa.eu/a4g/ontology"/>
   </owl:ObjectProperty>
   <owl:ObjectProperty rdf:about="http://data.europa.eu/a4g/ontology#summarisesProcedure">
      <rdfs:label xml:lang="en">Summarises procedure</rdfs:label>
      <skos:prefLabel xml:lang="en">Summarises procedure</skos:prefLabel>
      <rdfs:isDefinedBy rdf:resource="http://data.europa.eu/a4g/ontology"/>
   </owl:ObjectProperty>
   <owl:ObjectProperty rdf:about="http://data.europa.eu/a4g/ontology#hasContractModficationJustification">
      <rdfs:label xml:lang="en">Has contract modfication justification</rdfs:label>
      <skos:prefLabel xml:lang="en">Has contract modfication justification</skos:prefLabel>
      <skos:definition xml:lang="en">The codelist to be used is at-voc:modification-justification which is available at https://op.europa.eu/en/web/eu-vocabularies/at-dataset/-/resource/dataset/modification-justification
 (epo:ContractModificationNotice -&gt; at-voc:modification-justification (+epo:hasContractModficationJustification)) </skos:definition>
      <rdfs:comment xml:lang="en">The codelist to be used is at-voc:modification-justification which is available at https://op.europa.eu/en/web/eu-vocabularies/at-dataset/-/resource/dataset/modification-justification
 (epo:ContractModificationNotice -&gt; at-voc:modification-justification (+epo:hasContractModficationJustification)) </rdfs:comment>
      <rdfs:isDefinedBy rdf:resource="http://data.europa.eu/a4g/ontology"/>
   </owl:ObjectProperty>
   <owl:ObjectProperty rdf:about="http://data.europa.eu/a4g/ontology#hasBroadPlaceOfPerformance">
      <rdfs:label xml:lang="en">Has broad place of performance</rdfs:label>
      <skos:prefLabel xml:lang="en">Has broad place of performance</skos:prefLabel>
      <skos:definition xml:lang="en">The codelist to be used is at-voc:other-place-service which is available at https://op.europa.eu/en/web/eu-vocabularies/at-dataset/-/resource/dataset/other-place-service
 (epo:ContractTerm -&gt; at-voc:other-place-service (+epo:hasBroadPlaceOfPerformance)) </skos:definition>
      <rdfs:comment xml:lang="en">The codelist to be used is at-voc:other-place-service which is available at https://op.europa.eu/en/web/eu-vocabularies/at-dataset/-/resource/dataset/other-place-service
 (epo:ContractTerm -&gt; at-voc:other-place-service (+epo:hasBroadPlaceOfPerformance)) </rdfs:comment>
      <rdfs:isDefinedBy rdf:resource="http://data.europa.eu/a4g/ontology"/>
   </owl:ObjectProperty>
   <owl:ObjectProperty rdf:about="http://data.europa.eu/a4g/ontology#hasReservedExecution">
      <rdfs:label xml:lang="en">Has reserved execution</rdfs:label>
      <skos:prefLabel xml:lang="en">Has reserved execution</skos:prefLabel>
      <skos:definition xml:lang="en">The codelist to be used is at-voc:applicability which is available at https://op.europa.eu/web/eu-vocabularies/at-dataset/-/resource/dataset/applicability (epo:ContractTerm -&gt; at-voc:applicability (+epo:hasReservedExecution)) </skos:definition>
      <rdfs:comment xml:lang="en">The codelist to be used is at-voc:applicability which is available at https://op.europa.eu/web/eu-vocabularies/at-dataset/-/resource/dataset/applicability (epo:ContractTerm -&gt; at-voc:applicability (+epo:hasReservedExecution)) </rdfs:comment>
      <rdfs:isDefinedBy rdf:resource="http://data.europa.eu/a4g/ontology"/>
   </owl:ObjectProperty>
   <owl:ObjectProperty rdf:about="http://data.europa.eu/a4g/ontology#isSubTermof">
      <rdfs:label xml:lang="en">Is sub termof</rdfs:label>
      <skos:prefLabel xml:lang="en">Is sub termof</skos:prefLabel>
      <skos:scopeNote xml:lang="en">Relation indication a term is a subterm of another term. (epo:ContractTerm &lt;-&gt; epo:SubcontractTerm (+epo:hasSubTerm +epo:isSubTermof)) </skos:scopeNote>
      <rdfs:comment xml:lang="en">Relation indication a term is a subterm of another term. (epo:ContractTerm &lt;-&gt; epo:SubcontractTerm (+epo:hasSubTerm +epo:isSubTermof)) </rdfs:comment>
      <rdfs:isDefinedBy rdf:resource="http://data.europa.eu/a4g/ontology"/>
   </owl:ObjectProperty>
   <owl:ObjectProperty rdf:about="http://data.europa.eu/a4g/ontology#hasSubTerm">
      <rdfs:label xml:lang="en">Has sub term</rdfs:label>
      <skos:prefLabel xml:lang="en">Has sub term</skos:prefLabel>
      <skos:scopeNote xml:lang="en">Relation indicating a term has a subterm. (epo:ContractTerm &lt;-&gt; epo:SubcontractTerm (+epo:hasSubTerm +epo:isSubTermof)) </skos:scopeNote>
      <rdfs:comment xml:lang="en">Relation indicating a term has a subterm. (epo:ContractTerm &lt;-&gt; epo:SubcontractTerm (+epo:hasSubTerm +epo:isSubTermof)) </rdfs:comment>
      <rdfs:isDefinedBy rdf:resource="http://data.europa.eu/a4g/ontology"/>
   </owl:ObjectProperty>
   <owl:ObjectProperty rdf:about="http://data.europa.eu/a4g/ontology#setsContextFor">
      <rdfs:label xml:lang="en">Sets context for</rdfs:label>
      <skos:prefLabel xml:lang="en">Sets context for</skos:prefLabel>
      <skos:definition xml:lang="en">Identifier of one or more lots within the procedure to which this submission terms refer.

WG Approval 07/03/2019 16:29:39

 (epo:SubmissionTerm &lt;-&gt; epo:Lot (+epo:setsContextFor +epo:isSubjectToTerm)) </skos:definition>
      <rdfs:comment xml:lang="en">Identifier of one or more lots within the procedure to which this submission terms refer.

WG Approval 07/03/2019 16:29:39

 (epo:SubmissionTerm &lt;-&gt; epo:Lot (+epo:setsContextFor +epo:isSubjectToTerm)) </rdfs:comment>
      <skos:scopeNote xml:lang="en">Relation that specifies the lot to which these rules apply. (epo:Lot &lt;-&gt; epo:ContractTerm (+epo:isSubjectToTerm +epo:setsContextFor)) Relation that specifies rules that are applicable to the lot. (epo:Lot &lt;-&gt; epo:DesignContestRegimeTerm (+epo:isSubjectToTerm +epo:setsContextFor)) Relation that specifies the lot to which these rules apply. (epo:FrameworkAgreementTerm &lt;-&gt; epo:Lot (+epo:setsContextFor +epo:isSubjectToTerm)) Relation that specifies the lot to which these rules apply. (epo:Lot &lt;-&gt; epo:MultipleStageProcedureTerm (+epo:isSubjectToTerm +epo:setsContextFor)) Relation that specifies the lot to which these rules apply. (epo:SubmissionTerm &lt;-&gt; epo:Lot (+epo:setsContextFor +epo:isSubjectToTerm)) </skos:scopeNote>
      <rdfs:comment xml:lang="en">Relation that specifies the lot to which these rules apply. (epo:Lot &lt;-&gt; epo:ContractTerm (+epo:isSubjectToTerm +epo:setsContextFor)) Relation that specifies rules that are applicable to the lot. (epo:Lot &lt;-&gt; epo:DesignContestRegimeTerm (+epo:isSubjectToTerm +epo:setsContextFor)) Relation that specifies the lot to which these rules apply. (epo:FrameworkAgreementTerm &lt;-&gt; epo:Lot (+epo:setsContextFor +epo:isSubjectToTerm)) Relation that specifies the lot to which these rules apply. (epo:Lot &lt;-&gt; epo:MultipleStageProcedureTerm (+epo:isSubjectToTerm +epo:setsContextFor)) Relation that specifies the lot to which these rules apply. (epo:SubmissionTerm &lt;-&gt; epo:Lot (+epo:setsContextFor +epo:isSubjectToTerm)) </rdfs:comment>
      <rdfs:isDefinedBy rdf:resource="http://data.europa.eu/a4g/ontology"/>
   </owl:ObjectProperty>
   <owl:ObjectProperty rdf:about="http://data.europa.eu/a4g/ontology#isSubjectToTerm">
      <rdfs:label xml:lang="en">Is subject to term</rdfs:label>
      <skos:prefLabel xml:lang="en">Is subject to term</skos:prefLabel>
      <skos:definition xml:lang="en">Identifier of one or more lots within the procedure to which this submission terms refer.

WG Approval 07/03/2019 16:29:39

 (epo:SubmissionTerm &lt;-&gt; epo:Lot (+epo:setsContextFor +epo:isSubjectToTerm)) </skos:definition>
      <rdfs:comment xml:lang="en">Identifier of one or more lots within the procedure to which this submission terms refer.

WG Approval 07/03/2019 16:29:39

 (epo:SubmissionTerm &lt;-&gt; epo:Lot (+epo:setsContextFor +epo:isSubjectToTerm)) </rdfs:comment>
      <skos:scopeNote xml:lang="en">Relation that specifies rules that are applicable to the lot. (epo:Lot &lt;-&gt; epo:ContractTerm (+epo:isSubjectToTerm +epo:setsContextFor)) Relation that specifies the lot to which these rules apply. (epo:Lot &lt;-&gt; epo:DesignContestRegimeTerm (+epo:isSubjectToTerm +epo:setsContextFor)) Relation that specifies rules that are applicable to the lot. (epo:FrameworkAgreementTerm &lt;-&gt; epo:Lot (+epo:setsContextFor +epo:isSubjectToTerm)) Relation that specifies rules that are applicable to the lot. (epo:Lot &lt;-&gt; epo:MultipleStageProcedureTerm (+epo:isSubjectToTerm +epo:setsContextFor)) Relation that specifies rules that are applicable to the lot. (epo:SubmissionTerm &lt;-&gt; epo:Lot (+epo:setsContextFor +epo:isSubjectToTerm)) </skos:scopeNote>
      <rdfs:comment xml:lang="en">Relation that specifies rules that are applicable to the lot. (epo:Lot &lt;-&gt; epo:ContractTerm (+epo:isSubjectToTerm +epo:setsContextFor)) Relation that specifies the lot to which these rules apply. (epo:Lot &lt;-&gt; epo:DesignContestRegimeTerm (+epo:isSubjectToTerm +epo:setsContextFor)) Relation that specifies rules that are applicable to the lot. (epo:FrameworkAgreementTerm &lt;-&gt; epo:Lot (+epo:setsContextFor +epo:isSubjectToTerm)) Relation that specifies rules that are applicable to the lot. (epo:Lot &lt;-&gt; epo:MultipleStageProcedureTerm (+epo:isSubjectToTerm +epo:setsContextFor)) Relation that specifies rules that are applicable to the lot. (epo:SubmissionTerm &lt;-&gt; epo:Lot (+epo:setsContextFor +epo:isSubjectToTerm)) </rdfs:comment>
      <rdfs:isDefinedBy rdf:resource="http://data.europa.eu/a4g/ontology"/>
   </owl:ObjectProperty>
   <owl:ObjectProperty rdf:about="http://data.europa.eu/a4g/ontology#appliesTo">
      <rdfs:label xml:lang="en">Applies to</rdfs:label>
      <skos:prefLabel xml:lang="en">Applies to</skos:prefLabel>
      <rdfs:isDefinedBy rdf:resource="http://data.europa.eu/a4g/ontology"/>
   </owl:ObjectProperty>
   <owl:ObjectProperty rdf:about="http://data.europa.eu/a4g/ontology#definesPrize">
      <rdfs:label xml:lang="en">Defines prize</rdfs:label>
      <skos:prefLabel xml:lang="en">Defines prize</skos:prefLabel>
      <rdfs:isDefinedBy rdf:resource="http://data.europa.eu/a4g/ontology"/>
   </owl:ObjectProperty>
   <owl:ObjectProperty rdf:about="http://data.europa.eu/a4g/ontology#hasJustificationType">
      <rdfs:label xml:lang="en">Has justification type</rdfs:label>
      <skos:prefLabel xml:lang="en">Has justification type</skos:prefLabel>
      <skos:definition xml:lang="en">The codelist to be used is at-voc:direct-award-justification which is available at https://op.europa.eu/web/eu-vocabularies/at-dataset/-/resource/dataset/direct-award-justification
 (epo:DirectAwardTerm -&gt; at-voc:direct-award-justification (+epo:hasJustificationType)) </skos:definition>
      <rdfs:comment xml:lang="en">The codelist to be used is at-voc:direct-award-justification which is available at https://op.europa.eu/web/eu-vocabularies/at-dataset/-/resource/dataset/direct-award-justification
 (epo:DirectAwardTerm -&gt; at-voc:direct-award-justification (+epo:hasJustificationType)) </rdfs:comment>
      <rdfs:isDefinedBy rdf:resource="http://data.europa.eu/a4g/ontology"/>
   </owl:ObjectProperty>
   <owl:ObjectProperty rdf:about="http://data.europa.eu/a4g/ontology#refersToPreviousProcedureLots">
      <rdfs:label xml:lang="en">Refers to previous procedure lots</rdfs:label>
      <skos:prefLabel xml:lang="en">Refers to previous procedure lots</skos:prefLabel>
      <skos:definition xml:lang="en">Reference to one or more Lots in a previous procedure.

Additional Information:
In the case of Direct Award Terms, this property points to a previous Procedure justifying the use of Direct Award without a prior publication.

WG Approval 22/11/2019 14:33:55 (epo:DirectAwardTerm -&gt; epo:Lot (+epo:refersToPreviousProcedureLots)) </skos:definition>
      <rdfs:comment xml:lang="en">Reference to one or more Lots in a previous procedure.

Additional Information:
In the case of Direct Award Terms, this property points to a previous Procedure justifying the use of Direct Award without a prior publication.

WG Approval 22/11/2019 14:33:55 (epo:DirectAwardTerm -&gt; epo:Lot (+epo:refersToPreviousProcedureLots)) </rdfs:comment>
      <rdfs:isDefinedBy rdf:resource="http://data.europa.eu/a4g/ontology"/>
   </owl:ObjectProperty>
   <owl:ObjectProperty rdf:about="http://data.europa.eu/a4g/ontology#hasNonPublishedElement">
      <rdfs:label xml:lang="en">Has non published element</rdfs:label>
      <skos:prefLabel xml:lang="en">Has non published element</skos:prefLabel>
      <skos:definition xml:lang="en">For example, elements in the Contract Award Notice that are published at a later date. (epo:Document -&gt; epo:PublicationProvision (+epo:hasNonPublishedElement)) </skos:definition>
      <rdfs:comment xml:lang="en">For example, elements in the Contract Award Notice that are published at a later date. (epo:Document -&gt; epo:PublicationProvision (+epo:hasNonPublishedElement)) </rdfs:comment>
      <skos:scopeNote xml:lang="en">Relation indicating that part of a document is not published. (epo:Document -&gt; epo:PublicationProvision (+epo:hasNonPublishedElement)) </skos:scopeNote>
      <rdfs:comment xml:lang="en">Relation indicating that part of a document is not published. (epo:Document -&gt; epo:PublicationProvision (+epo:hasNonPublishedElement)) </rdfs:comment>
      <rdfs:isDefinedBy rdf:resource="http://data.europa.eu/a4g/ontology"/>
   </owl:ObjectProperty>
   <owl:ObjectProperty rdf:about="http://data.europa.eu/a4g/ontology#hasRestrictedCommunicationJustification">
      <rdfs:label xml:lang="en">Has restricted communication justification</rdfs:label>
      <skos:prefLabel xml:lang="en">Has restricted communication justification</skos:prefLabel>
      <skos:definition xml:lang="en">The codelist to be used is at-voc:communication-justification which is available at https://op.europa.eu/web/eu-vocabularies/at-dataset/-/resource/dataset/communication-justification
 (epo:Document -&gt; at-voc:communication-justification (+epo:hasRestrictedCommunicationJustification)) </skos:definition>
      <rdfs:comment xml:lang="en">The codelist to be used is at-voc:communication-justification which is available at https://op.europa.eu/web/eu-vocabularies/at-dataset/-/resource/dataset/communication-justification
 (epo:Document -&gt; at-voc:communication-justification (+epo:hasRestrictedCommunicationJustification)) </rdfs:comment>
      <rdfs:isDefinedBy rdf:resource="http://data.europa.eu/a4g/ontology"/>
   </owl:ObjectProperty>
   <owl:ObjectProperty rdf:about="http://data.europa.eu/a4g/ontology#hasOfficialLanguage">
      <rdfs:label xml:lang="en">Has official language</rdfs:label>
      <skos:prefLabel xml:lang="en">Has official language</skos:prefLabel>
      <skos:definition xml:lang="en">The codelist to be used is at-voc:language which is available at https://op.europa.eu/en/web/eu-vocabularies/at-dataset/-/resource/dataset/language
 (epo:Document -&gt; at-voc:language (+epo:hasOfficialLanguage)) </skos:definition>
      <rdfs:comment xml:lang="en">The codelist to be used is at-voc:language which is available at https://op.europa.eu/en/web/eu-vocabularies/at-dataset/-/resource/dataset/language
 (epo:Document -&gt; at-voc:language (+epo:hasOfficialLanguage)) </rdfs:comment>
      <rdfs:isDefinedBy rdf:resource="http://data.europa.eu/a4g/ontology"/>
   </owl:ObjectProperty>
   <owl:ObjectProperty rdf:about="http://data.europa.eu/a4g/ontology#changeRefersToInstance">
      <rdfs:label xml:lang="en">Change refers to instance</rdfs:label>
      <skos:prefLabel xml:lang="en">Change refers to instance</skos:prefLabel>
      <rdfs:isDefinedBy rdf:resource="http://data.europa.eu/a4g/ontology"/>
   </owl:ObjectProperty>
   <owl:ObjectProperty rdf:about="http://data.europa.eu/a4g/ontology#relatesTo">
      <rdfs:label xml:lang="en">Relates to</rdfs:label>
      <skos:prefLabel xml:lang="en">Relates to</skos:prefLabel>
      <skos:definition xml:lang="en">Associated to. 

Additional information: 

In the case of a Planning form this subproperty notifies is used. 

In the case of Competition form this subproperty announces is used. 

In the case of Result form this subproperty summarises is used.  (epo:Document -&gt; epo:Procedure (+epo:relatesTo)) </skos:definition>
      <rdfs:comment xml:lang="en">Associated to. 

Additional information: 

In the case of a Planning form this subproperty notifies is used. 

In the case of Competition form this subproperty announces is used. 

In the case of Result form this subproperty summarises is used.  (epo:Document -&gt; epo:Procedure (+epo:relatesTo)) </rdfs:comment>
      <rdfs:isDefinedBy rdf:resource="http://data.europa.eu/a4g/ontology"/>
   </owl:ObjectProperty>
   <owl:ObjectProperty rdf:about="http://data.europa.eu/a4g/ontology#hasUnofficialLanguage">
      <rdfs:label xml:lang="en">Has unofficial language</rdfs:label>
      <skos:prefLabel xml:lang="en">Has unofficial language</skos:prefLabel>
      <skos:definition xml:lang="en">The language translation(s) in which the instances of the given concepts are available. These linguistic versions are not an official translation, they are provided only for information.

WG Approval 03/10/2019

The codelist to be used is at-voc:language which is available at https://op.europa.eu/en/web/eu-vocabularies/at-dataset/-/resource/dataset/language
 (epo:Document -&gt; at-voc:language (+epo:hasUnofficialLanguage)) </skos:definition>
      <rdfs:comment xml:lang="en">The language translation(s) in which the instances of the given concepts are available. These linguistic versions are not an official translation, they are provided only for information.

WG Approval 03/10/2019

The codelist to be used is at-voc:language which is available at https://op.europa.eu/en/web/eu-vocabularies/at-dataset/-/resource/dataset/language
 (epo:Document -&gt; at-voc:language (+epo:hasUnofficialLanguage)) </rdfs:comment>
      <rdfs:isDefinedBy rdf:resource="http://data.europa.eu/a4g/ontology"/>
   </owl:ObjectProperty>
   <owl:ObjectProperty rdf:about="http://data.europa.eu/a4g/ontology#includes">
      <rdfs:label xml:lang="en">Includes</rdfs:label>
      <skos:prefLabel xml:lang="en">Includes</skos:prefLabel>
      <rdfs:isDefinedBy rdf:resource="http://data.europa.eu/a4g/ontology"/>
   </owl:ObjectProperty>
   <owl:ObjectProperty rdf:about="http://data.europa.eu/a4g/ontology#refersToPrevious">
      <rdfs:label xml:lang="en">Refers to previous</rdfs:label>
      <skos:prefLabel xml:lang="en">Refers to previous</skos:prefLabel>
      <rdfs:isDefinedBy rdf:resource="http://data.europa.eu/a4g/ontology"/>
   </owl:ObjectProperty>
   <owl:ObjectProperty rdf:about="http://data.europa.eu/a4g/ontology#hasSecurityClearanceTerm">
      <rdfs:label xml:lang="en">Has security clearance term</rdfs:label>
      <skos:prefLabel xml:lang="en">Has security clearance term</skos:prefLabel>
      <skos:scopeNote xml:lang="en">Relation indicating that security clearance is required for access. (epo:SecurityClearanceTerm &lt;-&gt; epo:Document (+epo:describesAccessRestrictionsTo +epo:hasSecurityClearanceTerm)) </skos:scopeNote>
      <rdfs:comment xml:lang="en">Relation indicating that security clearance is required for access. (epo:SecurityClearanceTerm &lt;-&gt; epo:Document (+epo:describesAccessRestrictionsTo +epo:hasSecurityClearanceTerm)) </rdfs:comment>
      <rdfs:isDefinedBy rdf:resource="http://data.europa.eu/a4g/ontology"/>
   </owl:ObjectProperty>
   <owl:ObjectProperty rdf:about="http://data.europa.eu/a4g/ontology#describesAccessRestrictionsTo">
      <rdfs:label xml:lang="en">Describes access restrictions to</rdfs:label>
      <skos:prefLabel xml:lang="en">Describes access restrictions to</skos:prefLabel>
      <skos:scopeNote xml:lang="en">Relation that specifies access rules. (epo:SecurityClearanceTerm &lt;-&gt; epo:Document (+epo:describesAccessRestrictionsTo +epo:hasSecurityClearanceTerm)) </skos:scopeNote>
      <rdfs:comment xml:lang="en">Relation that specifies access rules. (epo:SecurityClearanceTerm &lt;-&gt; epo:Document (+epo:describesAccessRestrictionsTo +epo:hasSecurityClearanceTerm)) </rdfs:comment>
      <rdfs:isDefinedBy rdf:resource="http://data.europa.eu/a4g/ontology"/>
   </owl:ObjectProperty>
   <owl:ObjectProperty rdf:about="http://data.europa.eu/a4g/ontology#hasEAuctionUsage">
      <rdfs:label xml:lang="en">Has e auction usage</rdfs:label>
      <skos:prefLabel xml:lang="en">Has e auction usage</skos:prefLabel>
      <skos:definition xml:lang="en">The codelist to be used is at-voc:usage which is available at https://op.europa.eu/en/web/eu-vocabularies/at-dataset/-/resource/dataset/usage (epo:EAuctionTechnique -&gt; at-voc:usage (+epo:hasEAuctionUsage)) </skos:definition>
      <rdfs:comment xml:lang="en">The codelist to be used is at-voc:usage which is available at https://op.europa.eu/en/web/eu-vocabularies/at-dataset/-/resource/dataset/usage (epo:EAuctionTechnique -&gt; at-voc:usage (+epo:hasEAuctionUsage)) </rdfs:comment>
      <rdfs:isDefinedBy rdf:resource="http://data.europa.eu/a4g/ontology"/>
   </owl:ObjectProperty>
   <owl:ObjectProperty rdf:about="http://data.europa.eu/a4g/ontology#hasEORoleType">
      <rdfs:label xml:lang="en">Has e o role type</rdfs:label>
      <skos:prefLabel xml:lang="en">Has e o role type</skos:prefLabel>
      <rdfs:isDefinedBy rdf:resource="http://data.europa.eu/a4g/ontology"/>
   </owl:ObjectProperty>
   <owl:ObjectProperty rdf:about="http://data.europa.eu/a4g/ontology#specifiesSubcontractors">
      <rdfs:label xml:lang="en">Specifies subcontractors</rdfs:label>
      <skos:prefLabel xml:lang="en">Specifies subcontractors</skos:prefLabel>
      <rdfs:isDefinedBy rdf:resource="http://data.europa.eu/a4g/ontology"/>
   </owl:ObjectProperty>
   <owl:ObjectProperty rdf:about="http://data.europa.eu/a4g/ontology#hasEvaluationGroupType">
      <rdfs:label xml:lang="en">Has evaluation group type</rdfs:label>
      <skos:prefLabel xml:lang="en">Has evaluation group type</skos:prefLabel>
      <rdfs:isDefinedBy rdf:resource="http://data.europa.eu/a4g/ontology"/>
   </owl:ObjectProperty>
   <owl:ObjectProperty rdf:about="http://data.europa.eu/a4g/ontology#isEvaluatedBy">
      <rdfs:label xml:lang="en">Is evaluated by</rdfs:label>
      <skos:prefLabel xml:lang="en">Is evaluated by</skos:prefLabel>
      <skos:scopeNote xml:lang="en">Relation indicating by whom a criterion is evaluated. (epo:EvaluationBoard &lt;-&gt; epo:ExclusionGround (+epo:evaluates +epo:isEvaluatedBy)) </skos:scopeNote>
      <rdfs:comment xml:lang="en">Relation indicating by whom a criterion is evaluated. (epo:EvaluationBoard &lt;-&gt; epo:ExclusionGround (+epo:evaluates +epo:isEvaluatedBy)) </rdfs:comment>
      <rdfs:isDefinedBy rdf:resource="http://data.europa.eu/a4g/ontology"/>
   </owl:ObjectProperty>
   <owl:ObjectProperty rdf:about="http://data.europa.eu/a4g/ontology#isAssignedForEvaluationOf">
      <rdfs:label xml:lang="en">Is assigned for evaluation of</rdfs:label>
      <skos:prefLabel xml:lang="en">Is assigned for evaluation of</skos:prefLabel>
      <rdfs:isDefinedBy rdf:resource="http://data.europa.eu/a4g/ontology"/>
   </owl:ObjectProperty>
   <owl:ObjectProperty rdf:about="http://data.europa.eu/a4g/ontology#evaluates">
      <rdfs:label xml:lang="en">Evaluates</rdfs:label>
      <skos:prefLabel xml:lang="en">Evaluates</skos:prefLabel>
      <skos:scopeNote xml:lang="en">Relation indicating who evaluates a criterion. (epo:EvaluationBoard &lt;-&gt; epo:ExclusionGround (+epo:evaluates +epo:isEvaluatedBy)) </skos:scopeNote>
      <rdfs:comment xml:lang="en">Relation indicating who evaluates a criterion. (epo:EvaluationBoard &lt;-&gt; epo:ExclusionGround (+epo:evaluates +epo:isEvaluatedBy)) </rdfs:comment>
      <rdfs:isDefinedBy rdf:resource="http://data.europa.eu/a4g/ontology"/>
   </owl:ObjectProperty>
   <owl:ObjectProperty rdf:about="http://data.europa.eu/a4g/ontology#hasTenderEvaluationTerm">
      <rdfs:label xml:lang="en">Has tender evaluation term</rdfs:label>
      <skos:prefLabel xml:lang="en">Has tender evaluation term</skos:prefLabel>
      <rdfs:isDefinedBy rdf:resource="http://data.europa.eu/a4g/ontology"/>
   </owl:ObjectProperty>
   <owl:ObjectProperty rdf:about="http://data.europa.eu/a4g/ontology#substantiates">
      <rdfs:label xml:lang="en">Substantiates</rdfs:label>
      <skos:prefLabel xml:lang="en">Substantiates</skos:prefLabel>
      <rdfs:isDefinedBy rdf:resource="http://data.europa.eu/a4g/ontology"/>
   </owl:ObjectProperty>
   <owl:ObjectProperty rdf:about="http://data.europa.eu/a4g/ontology#setsRulesOf">
      <rdfs:label xml:lang="en">Sets rules of</rdfs:label>
      <skos:prefLabel xml:lang="en">Sets rules of</skos:prefLabel>
      <rdfs:isDefinedBy rdf:resource="http://data.europa.eu/a4g/ontology"/>
   </owl:ObjectProperty>
   <owl:ObjectProperty rdf:about="http://data.europa.eu/a4g/ontology#hasRulesSetBy">
      <rdfs:label xml:lang="en">Has rules set by</rdfs:label>
      <skos:prefLabel xml:lang="en">Has rules set by</skos:prefLabel>
      <rdfs:isDefinedBy rdf:resource="http://data.europa.eu/a4g/ontology"/>
   </owl:ObjectProperty>
   <owl:ObjectProperty rdf:about="http://data.europa.eu/a4g/ontology#isSupportedBy">
      <rdfs:label xml:lang="en">Is supported by</rdfs:label>
      <skos:prefLabel xml:lang="en">Is supported by</skos:prefLabel>
      <skos:scopeNote xml:lang="en">Relation indicating that the FrameworkAgreement is supported by the FrameworkAgreementTechnique. (epo:FrameworkAgreementTechnique -&gt; epo:FrameworkAgreement (+epo:isSupportedBy)) </skos:scopeNote>
      <rdfs:comment xml:lang="en">Relation indicating that the FrameworkAgreement is supported by the FrameworkAgreementTechnique. (epo:FrameworkAgreementTechnique -&gt; epo:FrameworkAgreement (+epo:isSupportedBy)) </rdfs:comment>
      <rdfs:isDefinedBy rdf:resource="http://data.europa.eu/a4g/ontology"/>
   </owl:ObjectProperty>
   <owl:ObjectProperty rdf:about="http://data.europa.eu/a4g/ontology#isOrganisedIn">
      <rdfs:label xml:lang="en">Is organised in</rdfs:label>
      <skos:prefLabel xml:lang="en">Is organised in</skos:prefLabel>
      <skos:definition xml:lang="en">

Additional Information
This property allows to obtain the estimated value of both a group of lots used in a Framework Agreement and the estimated value of each individual lot; which helps to compare the difference between the estimated value of the group against the addition of each lot estimated value.

 (epo:FrameworkAgreementTechnique &lt;-&gt; epo:LotGroup (+epo:isOrganisedIn +epo:uses)) </skos:definition>
      <rdfs:comment xml:lang="en">

Additional Information
This property allows to obtain the estimated value of both a group of lots used in a Framework Agreement and the estimated value of each individual lot; which helps to compare the difference between the estimated value of the group against the addition of each lot estimated value.

 (epo:FrameworkAgreementTechnique &lt;-&gt; epo:LotGroup (+epo:isOrganisedIn +epo:uses)) </rdfs:comment>
      <rdfs:isDefinedBy rdf:resource="http://data.europa.eu/a4g/ontology"/>
   </owl:ObjectProperty>
   <owl:ObjectProperty rdf:about="http://data.europa.eu/a4g/ontology#hasFrameworkAgreementType">
      <rdfs:label xml:lang="en">Has framework agreement type</rdfs:label>
      <skos:prefLabel xml:lang="en">Has framework agreement type</skos:prefLabel>
      <skos:definition xml:lang="en">The codelist to be used is at-voc:framework-agreement which is available at https://op.europa.eu/en/web/eu-vocabularies/at-dataset/-/resource/dataset/framework-agreement
 (epo:FrameworkAgreementTerm -&gt; at-voc:framework-agreement (+epo:hasFrameworkAgreementType)) </skos:definition>
      <rdfs:comment xml:lang="en">The codelist to be used is at-voc:framework-agreement which is available at https://op.europa.eu/en/web/eu-vocabularies/at-dataset/-/resource/dataset/framework-agreement
 (epo:FrameworkAgreementTerm -&gt; at-voc:framework-agreement (+epo:hasFrameworkAgreementType)) </rdfs:comment>
      <rdfs:isDefinedBy rdf:resource="http://data.europa.eu/a4g/ontology"/>
   </owl:ObjectProperty>
   <owl:ObjectProperty rdf:about="http://data.europa.eu/a4g/ontology#hasOverallMaximumValue">
      <rdfs:label xml:lang="en">Has overall maximum value</rdfs:label>
      <skos:prefLabel xml:lang="en">Has overall maximum value</skos:prefLabel>
      <skos:definition xml:lang="en">Establishes the maximum value for the Framework Agreement, either for the lots specified in the Framework Agreement Lots or for all the lots of the procedure.

 (epo:FrameworkAgreementTerm -&gt; epo:Value (+epo:hasOverallMaximumValue)) </skos:definition>
      <rdfs:comment xml:lang="en">Establishes the maximum value for the Framework Agreement, either for the lots specified in the Framework Agreement Lots or for all the lots of the procedure.

 (epo:FrameworkAgreementTerm -&gt; epo:Value (+epo:hasOverallMaximumValue)) </rdfs:comment>
      <rdfs:isDefinedBy rdf:resource="http://data.europa.eu/a4g/ontology"/>
   </owl:ObjectProperty>
   <owl:ObjectProperty rdf:about="http://data.europa.eu/a4g/ontology#isFundedWith">
      <rdfs:label xml:lang="en">Is funded with</rdfs:label>
      <skos:prefLabel xml:lang="en">Is funded with</skos:prefLabel>
      <rdfs:isDefinedBy rdf:resource="http://data.europa.eu/a4g/ontology"/>
   </owl:ObjectProperty>
   <owl:ObjectProperty rdf:about="http://data.europa.eu/a4g/ontology#fulfillsRequirement">
      <rdfs:label xml:lang="en">Fulfills requirement</rdfs:label>
      <skos:prefLabel xml:lang="en">Fulfills requirement</skos:prefLabel>
      <skos:definition xml:lang="en">The codelist to be used is at-voc:environmental-impact which is available at https://op.europa.eu/en/web/eu-vocabularies/at-dataset/-/resource/dataset/environmental-impact
 (epo:GreenProcurement -&gt; at-voc:environmental-impact (+epo:fulfillsRequirement)) The codelist to be used is at-voc:innovative-acquisition which is available at https://op.europa.eu/en/web/eu-vocabularies/at-dataset/-/resource/dataset/innovative-acquisition
 (epo:InnovativeProcurement -&gt; at-voc:innovative-acquisition (+epo:fulfillsRequirement)) The codelist to be used is at-voc:social-objective which is available at https://op.europa.eu/en/web/eu-vocabularies/at-dataset/-/resource/dataset/social-objective
 (epo:SocialProcurement -&gt; at-voc:social-objective (+epo:fulfillsRequirement)) </skos:definition>
      <rdfs:comment xml:lang="en">The codelist to be used is at-voc:environmental-impact which is available at https://op.europa.eu/en/web/eu-vocabularies/at-dataset/-/resource/dataset/environmental-impact
 (epo:GreenProcurement -&gt; at-voc:environmental-impact (+epo:fulfillsRequirement)) The codelist to be used is at-voc:innovative-acquisition which is available at https://op.europa.eu/en/web/eu-vocabularies/at-dataset/-/resource/dataset/innovative-acquisition
 (epo:InnovativeProcurement -&gt; at-voc:innovative-acquisition (+epo:fulfillsRequirement)) The codelist to be used is at-voc:social-objective which is available at https://op.europa.eu/en/web/eu-vocabularies/at-dataset/-/resource/dataset/social-objective
 (epo:SocialProcurement -&gt; at-voc:social-objective (+epo:fulfillsRequirement)) </rdfs:comment>
      <rdfs:isDefinedBy rdf:resource="http://data.europa.eu/a4g/ontology"/>
   </owl:ObjectProperty>
   <owl:ObjectProperty rdf:about="http://data.europa.eu/a4g/ontology#hasCountryOfOrigin">
      <rdfs:label xml:lang="en">Has country of origin</rdfs:label>
      <skos:prefLabel xml:lang="en">Has country of origin</skos:prefLabel>
      <skos:definition xml:lang="en">The codelist to be used is at-voc:country which is available at https://op.europa.eu/web/eu-vocabularies/at-dataset/-/resource/dataset/country
 (epo:Item -&gt; at-voc:country (+epo:hasCountryOfOrigin)) </skos:definition>
      <rdfs:comment xml:lang="en">The codelist to be used is at-voc:country which is available at https://op.europa.eu/web/eu-vocabularies/at-dataset/-/resource/dataset/country
 (epo:Item -&gt; at-voc:country (+epo:hasCountryOfOrigin)) </rdfs:comment>
      <rdfs:isDefinedBy rdf:resource="http://data.europa.eu/a4g/ontology"/>
   </owl:ObjectProperty>
   <owl:ObjectProperty rdf:about="http://data.europa.eu/a4g/ontology#groups">
      <rdfs:label xml:lang="en">Groups</rdfs:label>
      <skos:prefLabel xml:lang="en">Groups</skos:prefLabel>
      <rdfs:isDefinedBy rdf:resource="http://data.europa.eu/a4g/ontology"/>
   </owl:ObjectProperty>
   <owl:ObjectProperty rdf:about="http://data.europa.eu/a4g/ontology#isGroupedIn">
      <rdfs:label xml:lang="en">Is grouped in</rdfs:label>
      <skos:prefLabel xml:lang="en">Is grouped in</skos:prefLabel>
      <rdfs:isDefinedBy rdf:resource="http://data.europa.eu/a4g/ontology"/>
   </owl:ObjectProperty>
   <owl:ObjectProperty rdf:about="http://data.europa.eu/a4g/ontology#hasAwardedEstimatedValue">
      <rdfs:label xml:lang="en">Has awarded estimated value</rdfs:label>
      <skos:prefLabel xml:lang="en">Has awarded estimated value</skos:prefLabel>
      <skos:definition xml:lang="en">The estimated value that can be spent as provided by the Award Decision.

&lt;u&gt;Additional Information&lt;/u&gt;:
This property is used for framework agreements and dynamic purchasing systems. 
Different cases of awarded values may refer to a lot, the global value of the procedure, or of a combinatorial value of a group of lots.

WG Approval 12/12/2019

 (epo:Lot -&gt; epo:Value (+epo:hasAwardedEstimatedValue)) </skos:definition>
      <rdfs:comment xml:lang="en">The estimated value that can be spent as provided by the Award Decision.

&lt;u&gt;Additional Information&lt;/u&gt;:
This property is used for framework agreements and dynamic purchasing systems. 
Different cases of awarded values may refer to a lot, the global value of the procedure, or of a combinatorial value of a group of lots.

WG Approval 12/12/2019

 (epo:Lot -&gt; epo:Value (+epo:hasAwardedEstimatedValue)) </rdfs:comment>
      <rdfs:isDefinedBy rdf:resource="http://data.europa.eu/a4g/ontology"/>
   </owl:ObjectProperty>
   <owl:ObjectProperty rdf:about="http://data.europa.eu/a4g/ontology#providesAdditionalInformation">
      <rdfs:label xml:lang="en">Provides additional information</rdfs:label>
      <skos:prefLabel xml:lang="en">Provides additional information</skos:prefLabel>
      <rdfs:isDefinedBy rdf:resource="http://data.europa.eu/a4g/ontology"/>
   </owl:ObjectProperty>
   <owl:ObjectProperty rdf:about="http://data.europa.eu/a4g/ontology#requires">
      <rdfs:label xml:lang="en">Requires</rdfs:label>
      <skos:prefLabel xml:lang="en">Requires</skos:prefLabel>
      <rdfs:isDefinedBy rdf:resource="http://data.europa.eu/a4g/ontology"/>
   </owl:ObjectProperty>
   <owl:ObjectProperty rdf:about="http://data.europa.eu/a4g/ontology#hasEstimatedValue">
      <rdfs:label xml:lang="en">Has estimated value</rdfs:label>
      <skos:prefLabel xml:lang="en">Has estimated value</skos:prefLabel>
      <skos:definition xml:lang="en">A forecast of the value of the procurement before competition.

Additional Information
Different cases of estimated values may refer to a lot, the global value of the procedure, or of a combinatorial value of a group of lots.
The forecast is calculated by the buyer and covers all revenues  whether coming from the buyer or third parties.
See for example recital (19), Article 5 of Directive 2014/24/EU and other articles from the rest of Directives about procurement.

In the case of framework agreements and dynamic purchasing systems this refers to the maximum estimated value.
&lt;b&gt;
&lt;/b&gt;&lt;b&gt;WG Approval 05/12/2019&lt;/b&gt;
 (epo:Lot -&gt; epo:Value (+epo:hasEstimatedValue)) A forecast of the value of the procurement before competition.

Additional Information
Different cases of estimated values may refer to a lot, the global value of the procedure, or of a combinatorial value of a group of lots.
The forecast is calculated by the buyer and covers all revenues  whether coming from the buyer or third parties.
See for example recital (19), Article 5 of Directive 2014/24/EU and other articles from the rest of Directives about procurement.

In the case of lots or groups of lots using framework agreements and dynamic purchasing systems this refers to the maximum estimated value.
&lt;b&gt;
&lt;/b&gt;&lt;b&gt;WG Approval 05/12/2019&lt;/b&gt; (epo:LotGroup -&gt; epo:Value (+epo:hasEstimatedValue)) A forecast of the value of the procurement before competition.

Additional Information
Different cases of estimated values may refer to a lot, the global value of the procedure, or of a combinatorial value of a group of lots.
The forecast is calculated by the buyer and covers all revenues  whether coming from the buyer or third parties.
See for example recital (19), Article 5 of Directive 2014/24/EU and other articles from the rest of Directives about procurement.

In the case of framework agreements and dynamic purchasing systems this refers to the maximum estimated value.
&lt;b&gt;
&lt;/b&gt;&lt;b&gt;WG Approval 05/12/2019&lt;/b&gt;
 (epo:Procedure -&gt; epo:Value (+epo:hasEstimatedValue)) The estimated value of a single subcontract.

WG Approval 01/09/2020

 (epo:Subcontract -&gt; epo:Value (+epo:hasEstimatedValue)) </skos:definition>
      <rdfs:comment xml:lang="en">A forecast of the value of the procurement before competition.

Additional Information
Different cases of estimated values may refer to a lot, the global value of the procedure, or of a combinatorial value of a group of lots.
The forecast is calculated by the buyer and covers all revenues  whether coming from the buyer or third parties.
See for example recital (19), Article 5 of Directive 2014/24/EU and other articles from the rest of Directives about procurement.

In the case of framework agreements and dynamic purchasing systems this refers to the maximum estimated value.
&lt;b&gt;
&lt;/b&gt;&lt;b&gt;WG Approval 05/12/2019&lt;/b&gt;
 (epo:Lot -&gt; epo:Value (+epo:hasEstimatedValue)) A forecast of the value of the procurement before competition.

Additional Information
Different cases of estimated values may refer to a lot, the global value of the procedure, or of a combinatorial value of a group of lots.
The forecast is calculated by the buyer and covers all revenues  whether coming from the buyer or third parties.
See for example recital (19), Article 5 of Directive 2014/24/EU and other articles from the rest of Directives about procurement.

In the case of lots or groups of lots using framework agreements and dynamic purchasing systems this refers to the maximum estimated value.
&lt;b&gt;
&lt;/b&gt;&lt;b&gt;WG Approval 05/12/2019&lt;/b&gt; (epo:LotGroup -&gt; epo:Value (+epo:hasEstimatedValue)) A forecast of the value of the procurement before competition.

Additional Information
Different cases of estimated values may refer to a lot, the global value of the procedure, or of a combinatorial value of a group of lots.
The forecast is calculated by the buyer and covers all revenues  whether coming from the buyer or third parties.
See for example recital (19), Article 5 of Directive 2014/24/EU and other articles from the rest of Directives about procurement.

In the case of framework agreements and dynamic purchasing systems this refers to the maximum estimated value.
&lt;b&gt;
&lt;/b&gt;&lt;b&gt;WG Approval 05/12/2019&lt;/b&gt;
 (epo:Procedure -&gt; epo:Value (+epo:hasEstimatedValue)) The estimated value of a single subcontract.

WG Approval 01/09/2020

 (epo:Subcontract -&gt; epo:Value (+epo:hasEstimatedValue)) </rdfs:comment>
      <rdfs:isDefinedBy rdf:resource="http://data.europa.eu/a4g/ontology"/>
   </owl:ObjectProperty>
   <owl:ObjectProperty rdf:about="http://data.europa.eu/a4g/ontology#isSpecifiedIn">
      <rdfs:label xml:lang="en">Is specified in</rdfs:label>
      <skos:prefLabel xml:lang="en">Is specified in</skos:prefLabel>
      <skos:scopeNote xml:lang="en">Relation indicating that the Lot is referenced in the Procedure.
WG approval 18/05/2021 (epo:Lot -&gt; epo:Procedure (+epo:isSpecifiedIn)) Relation indicating a selection criterion in a given Lot or LotGroup. (epo:SelectionCriterion &lt;-&gt; epo:Lot (+epo:isSpecifiedIn +epo:specifies)) Relation indicating a selection criterion in a given Lot or LotGroup. (epo:SelectionCriterion &lt;-&gt; epo:LotGroup (+epo:isSpecifiedIn +epo:specifies)) </skos:scopeNote>
      <rdfs:comment xml:lang="en">Relation indicating that the Lot is referenced in the Procedure.
WG approval 18/05/2021 (epo:Lot -&gt; epo:Procedure (+epo:isSpecifiedIn)) Relation indicating a selection criterion in a given Lot or LotGroup. (epo:SelectionCriterion &lt;-&gt; epo:Lot (+epo:isSpecifiedIn +epo:specifies)) Relation indicating a selection criterion in a given Lot or LotGroup. (epo:SelectionCriterion &lt;-&gt; epo:LotGroup (+epo:isSpecifiedIn +epo:specifies)) </rdfs:comment>
      <rdfs:isDefinedBy rdf:resource="http://data.europa.eu/a4g/ontology"/>
   </owl:ObjectProperty>
   <owl:ObjectProperty rdf:about="http://data.europa.eu/a4g/ontology#contributesToImplement">
      <rdfs:label xml:lang="en">Contributes to implement</rdfs:label>
      <skos:prefLabel xml:lang="en">Contributes to implement</skos:prefLabel>
      <rdfs:isDefinedBy rdf:resource="http://data.europa.eu/a4g/ontology"/>
   </owl:ObjectProperty>
   <owl:ObjectProperty rdf:about="http://data.europa.eu/a4g/ontology#hasPurpose">
      <rdfs:label xml:lang="en">Has purpose</rdfs:label>
      <skos:prefLabel xml:lang="en">Has purpose</skos:prefLabel>
      <skos:scopeNote xml:lang="en">Relation indicating a contract, procedure, lot or planned procurement part has a puropse. (epo:Lot -&gt; epo:Purpose (+epo:hasPurpose)) </skos:scopeNote>
      <rdfs:comment xml:lang="en">Relation indicating a contract, procedure, lot or planned procurement part has a puropse. (epo:Lot -&gt; epo:Purpose (+epo:hasPurpose)) </rdfs:comment>
      <rdfs:isDefinedBy rdf:resource="http://data.europa.eu/a4g/ontology"/>
   </owl:ObjectProperty>
   <owl:ObjectProperty rdf:about="http://data.europa.eu/a4g/ontology#isAwardedTo">
      <rdfs:label xml:lang="en">Is awarded to</rdfs:label>
      <skos:prefLabel xml:lang="en">Is awarded to</skos:prefLabel>
      <rdfs:isDefinedBy rdf:resource="http://data.europa.eu/a4g/ontology"/>
   </owl:ObjectProperty>
   <owl:ObjectProperty rdf:about="http://data.europa.eu/a4g/ontology#hasReservedProcurement">
      <rdfs:label xml:lang="en">Has reserved procurement</rdfs:label>
      <skos:prefLabel xml:lang="en">Has reserved procurement</skos:prefLabel>
      <skos:definition xml:lang="en">The codelist to be used is at-voc:reserved-procurement which is available at https://op.europa.eu/en/web/eu-vocabularies/at-dataset/-/resource/dataset/reserved-procurement
 (epo:Lot -&gt; at-voc:reserved-procurement (+epo:hasReservedProcurement)) </skos:definition>
      <rdfs:comment xml:lang="en">The codelist to be used is at-voc:reserved-procurement which is available at https://op.europa.eu/en/web/eu-vocabularies/at-dataset/-/resource/dataset/reserved-procurement
 (epo:Lot -&gt; at-voc:reserved-procurement (+epo:hasReservedProcurement)) </rdfs:comment>
      <rdfs:isDefinedBy rdf:resource="http://data.europa.eu/a4g/ontology"/>
   </owl:ObjectProperty>
   <owl:ObjectProperty rdf:about="http://data.europa.eu/a4g/ontology#involvesOverallStrategicProcurement">
      <rdfs:label xml:lang="en">Involves overall strategic procurement</rdfs:label>
      <skos:prefLabel xml:lang="en">Involves overall strategic procurement</skos:prefLabel>
      <rdfs:isDefinedBy rdf:resource="http://data.europa.eu/a4g/ontology"/>
   </owl:ObjectProperty>
   <owl:ObjectProperty rdf:about="http://data.europa.eu/a4g/ontology#isProvidedWithin">
      <rdfs:label xml:lang="en">Is provided within</rdfs:label>
      <skos:prefLabel xml:lang="en">Is provided within</skos:prefLabel>
      <skos:definition xml:lang="en">The codelist to be used is at-voc:requirement-stage which is available at https://op.europa.eu/en/web/eu-vocabularies/at-dataset/-/resource/dataset/requirement-stage (epo:Lot -&gt; at-voc:requirement-stage (+epo:isProvidedWithin)) </skos:definition>
      <rdfs:comment xml:lang="en">The codelist to be used is at-voc:requirement-stage which is available at https://op.europa.eu/en/web/eu-vocabularies/at-dataset/-/resource/dataset/requirement-stage (epo:Lot -&gt; at-voc:requirement-stage (+epo:isProvidedWithin)) </rdfs:comment>
      <rdfs:isDefinedBy rdf:resource="http://data.europa.eu/a4g/ontology"/>
   </owl:ObjectProperty>
   <owl:ObjectProperty rdf:about="http://data.europa.eu/a4g/ontology#hasVariantsPermission">
      <rdfs:label xml:lang="en">Has variants permission</rdfs:label>
      <skos:prefLabel xml:lang="en">Has variants permission</skos:prefLabel>
      <skos:definition xml:lang="en">The codelist to be used is at-voc:permission which is available at https://op.europa.eu/en/web/eu-vocabularies/at-dataset/-/resource/dataset/permission
 (epo:Lot -&gt; at-voc:permission (+epo:hasVariantsPermission)) </skos:definition>
      <rdfs:comment xml:lang="en">The codelist to be used is at-voc:permission which is available at https://op.europa.eu/en/web/eu-vocabularies/at-dataset/-/resource/dataset/permission
 (epo:Lot -&gt; at-voc:permission (+epo:hasVariantsPermission)) </rdfs:comment>
      <rdfs:isDefinedBy rdf:resource="http://data.europa.eu/a4g/ontology"/>
   </owl:ObjectProperty>
   <owl:ObjectProperty rdf:about="http://data.europa.eu/a4g/ontology#hasEstimatedUserConcessionRevenue">
      <rdfs:label xml:lang="en">Has estimated user concession revenue</rdfs:label>
      <skos:prefLabel xml:lang="en">Has estimated user concession revenue</skos:prefLabel>
      <skos:definition xml:lang="en">The estimated revenue coming from the use of the concession.

Additional Information:
Revenues are for example fees and fines. For example, the fees and fines coming from the cars using a motorway. (epo:Lot -&gt; epo:Value (+epo:hasEstimatedUserConcessionRevenue)) </skos:definition>
      <rdfs:comment xml:lang="en">The estimated revenue coming from the use of the concession.

Additional Information:
Revenues are for example fees and fines. For example, the fees and fines coming from the cars using a motorway. (epo:Lot -&gt; epo:Value (+epo:hasEstimatedUserConcessionRevenue)) </rdfs:comment>
      <rdfs:isDefinedBy rdf:resource="http://data.europa.eu/a4g/ontology"/>
   </owl:ObjectProperty>
   <owl:ObjectProperty rdf:about="http://data.europa.eu/a4g/ontology#hasContractDuration">
      <rdfs:label xml:lang="en">Has contract duration</rdfs:label>
      <skos:prefLabel xml:lang="en">Has contract duration</skos:prefLabel>
      <skos:definition xml:lang="en">The estimated date when the contract is to be started.

Additional Information

When the Lot uses a Technique the contract estimated duration applies to the Technique.

 (epo:Lot -&gt; epo:Period (+epo:hasContractDuration)) </skos:definition>
      <rdfs:comment xml:lang="en">The estimated date when the contract is to be started.

Additional Information

When the Lot uses a Technique the contract estimated duration applies to the Technique.

 (epo:Lot -&gt; epo:Period (+epo:hasContractDuration)) </rdfs:comment>
      <rdfs:isDefinedBy rdf:resource="http://data.europa.eu/a4g/ontology"/>
   </owl:ObjectProperty>
   <owl:ObjectProperty rdf:about="http://data.europa.eu/a4g/ontology#hasEstimatedBuyerConcessionRevenue">
      <rdfs:label xml:lang="en">Has estimated buyer concession revenue</rdfs:label>
      <skos:prefLabel xml:lang="en">Has estimated buyer concession revenue</skos:prefLabel>
      <skos:definition xml:lang="en">The expected payments made by the buyer to the economic operator awarded the concession that are not directly related to the use of the concession.

&lt;u&gt;Additional Information:&lt;/u&gt;
For example the public buyer pays a yearly fee to provide a ticketing solution to the public.  The fee the public pays for every ticket sold through the solution is not included in this estimation but in the estimation of the user concession revenue.

WG Approval 07/01/2020 (epo:Lot -&gt; epo:Value (+epo:hasEstimatedBuyerConcessionRevenue)) </skos:definition>
      <rdfs:comment xml:lang="en">The expected payments made by the buyer to the economic operator awarded the concession that are not directly related to the use of the concession.

&lt;u&gt;Additional Information:&lt;/u&gt;
For example the public buyer pays a yearly fee to provide a ticketing solution to the public.  The fee the public pays for every ticket sold through the solution is not included in this estimation but in the estimation of the user concession revenue.

WG Approval 07/01/2020 (epo:Lot -&gt; epo:Value (+epo:hasEstimatedBuyerConcessionRevenue)) </rdfs:comment>
      <rdfs:isDefinedBy rdf:resource="http://data.europa.eu/a4g/ontology"/>
   </owl:ObjectProperty>
   <owl:ObjectProperty rdf:about="http://data.europa.eu/a4g/ontology#isReferredToIn">
      <rdfs:label xml:lang="en">Is referred to in</rdfs:label>
      <skos:prefLabel xml:lang="en">Is referred to in</skos:prefLabel>
      <skos:scopeNote xml:lang="en">Relation indicating the lot is referred to in a Procurement Document.
WG approval 18/05/2021 (epo:Lot -&gt; epo:ProcurementDocument (+epo:isReferredToIn)) </skos:scopeNote>
      <rdfs:comment xml:lang="en">Relation indicating the lot is referred to in a Procurement Document.
WG approval 18/05/2021 (epo:Lot -&gt; epo:ProcurementDocument (+epo:isReferredToIn)) </rdfs:comment>
      <rdfs:isDefinedBy rdf:resource="http://data.europa.eu/a4g/ontology"/>
   </owl:ObjectProperty>
   <owl:ObjectProperty rdf:about="http://data.europa.eu/a4g/ontology#hasAwardedValue">
      <rdfs:label xml:lang="en">Has awarded value</rdfs:label>
      <skos:prefLabel xml:lang="en">Has awarded value</skos:prefLabel>
      <skos:definition xml:lang="en">The value of the procurement provided by the Award Decision.

Additional Information:
Different cases of awarded values may refer to a lot, the global value of the procedure, or of a combinatorial value of a group of lots.

In the case of framework agreements and dynamic purchasing systems this refers to the maximum awarded value.

WG Approval 10/12/2019 (epo:LotGroup -&gt; epo:Value (+epo:hasAwardedValue)) </skos:definition>
      <rdfs:comment xml:lang="en">The value of the procurement provided by the Award Decision.

Additional Information:
Different cases of awarded values may refer to a lot, the global value of the procedure, or of a combinatorial value of a group of lots.

In the case of framework agreements and dynamic purchasing systems this refers to the maximum awarded value.

WG Approval 10/12/2019 (epo:LotGroup -&gt; epo:Value (+epo:hasAwardedValue)) </rdfs:comment>
      <rdfs:isDefinedBy rdf:resource="http://data.europa.eu/a4g/ontology"/>
   </owl:ObjectProperty>
   <owl:ObjectProperty rdf:about="http://data.europa.eu/a4g/ontology#isAppliedBy">
      <rdfs:label xml:lang="en">Is applied by</rdfs:label>
      <skos:prefLabel xml:lang="en">Is applied by</skos:prefLabel>
      <rdfs:isDefinedBy rdf:resource="http://data.europa.eu/a4g/ontology"/>
   </owl:ObjectProperty>
   <owl:ObjectProperty rdf:about="http://data.europa.eu/a4g/ontology#isRelatedTo">
      <rdfs:label xml:lang="en">Is related to</rdfs:label>
      <skos:prefLabel xml:lang="en">Is related to</skos:prefLabel>
      <rdfs:isDefinedBy rdf:resource="http://data.europa.eu/a4g/ontology"/>
   </owl:ObjectProperty>
   <owl:ObjectProperty rdf:about="http://data.europa.eu/a4g/ontology#specifies">
      <rdfs:label xml:lang="en">Specifies</rdfs:label>
      <skos:prefLabel xml:lang="en">Specifies</skos:prefLabel>
      <skos:scopeNote xml:lang="en">Relation that indicates the conditions for selecting economic operators for tendering. (epo:SelectionCriterion &lt;-&gt; epo:Lot (+epo:isSpecifiedIn +epo:specifies)) Relation that indicates the conditions for selecting economic operators for tendering. (epo:SelectionCriterion &lt;-&gt; epo:LotGroup (+epo:isSpecifiedIn +epo:specifies)) </skos:scopeNote>
      <rdfs:comment xml:lang="en">Relation that indicates the conditions for selecting economic operators for tendering. (epo:SelectionCriterion &lt;-&gt; epo:Lot (+epo:isSpecifiedIn +epo:specifies)) Relation that indicates the conditions for selecting economic operators for tendering. (epo:SelectionCriterion &lt;-&gt; epo:LotGroup (+epo:isSpecifiedIn +epo:specifies)) </rdfs:comment>
      <rdfs:isDefinedBy rdf:resource="http://data.europa.eu/a4g/ontology"/>
   </owl:ObjectProperty>
   <owl:ObjectProperty rdf:about="http://data.europa.eu/a4g/ontology#isUsedBy">
      <rdfs:label xml:lang="en">Is used by</rdfs:label>
      <skos:prefLabel xml:lang="en">Is used by</skos:prefLabel>
      <rdfs:isDefinedBy rdf:resource="http://data.europa.eu/a4g/ontology"/>
   </owl:ObjectProperty>
   <owl:ObjectProperty rdf:about="http://data.europa.eu/a4g/ontology#usedForReductionOfCandidates">
      <rdfs:label xml:lang="en">Used for reduction of candidates</rdfs:label>
      <skos:prefLabel xml:lang="en">Used for reduction of candidates</skos:prefLabel>
      <rdfs:isDefinedBy rdf:resource="http://data.europa.eu/a4g/ontology"/>
   </owl:ObjectProperty>
   <owl:ObjectProperty rdf:about="http://data.europa.eu/a4g/ontology#isComponentOf">
      <rdfs:label xml:lang="en">Is component of</rdfs:label>
      <skos:prefLabel xml:lang="en">Is component of</skos:prefLabel>
      <skos:scopeNote xml:lang="en">Relation showing the lot is part of the procedure. (epo:Procedure &lt;-&gt; epo:Lot (+epo:isComposedOf +epo:isComponentOf)) </skos:scopeNote>
      <rdfs:comment xml:lang="en">Relation showing the lot is part of the procedure. (epo:Procedure &lt;-&gt; epo:Lot (+epo:isComposedOf +epo:isComponentOf)) </rdfs:comment>
      <rdfs:isDefinedBy rdf:resource="http://data.europa.eu/a4g/ontology"/>
   </owl:ObjectProperty>
   <owl:ObjectProperty rdf:about="http://data.europa.eu/a4g/ontology#isComposedOf">
      <rdfs:label xml:lang="en">Is composed of</rdfs:label>
      <skos:prefLabel xml:lang="en">Is composed of</skos:prefLabel>
      <skos:scopeNote xml:lang="en">Relation showing a component part of a procedure. (epo:Procedure &lt;-&gt; epo:Lot (+epo:isComposedOf +epo:isComponentOf)) </skos:scopeNote>
      <rdfs:comment xml:lang="en">Relation showing a component part of a procedure. (epo:Procedure &lt;-&gt; epo:Lot (+epo:isComposedOf +epo:isComponentOf)) </rdfs:comment>
      <rdfs:isDefinedBy rdf:resource="http://data.europa.eu/a4g/ontology"/>
   </owl:ObjectProperty>
   <owl:ObjectProperty rdf:about="http://data.europa.eu/a4g/ontology#combineLotsInto">
      <rdfs:label xml:lang="en">Combine lots into</rdfs:label>
      <skos:prefLabel xml:lang="en">Combine lots into</skos:prefLabel>
      <rdfs:isDefinedBy rdf:resource="http://data.europa.eu/a4g/ontology"/>
   </owl:ObjectProperty>
   <owl:ObjectProperty rdf:about="http://data.europa.eu/a4g/ontology#hasTenderLot">
      <rdfs:label xml:lang="en">Has tender lot</rdfs:label>
      <skos:prefLabel xml:lang="en">Has tender lot</skos:prefLabel>
      <skos:scopeNote xml:lang="en">Relation indicating a GroupLot has a TenderLot associated to it. (epo:TenderLot &lt;-&gt; epo:LotGroup (+epo:isSubmittedFor +epo:hasTenderLot)) </skos:scopeNote>
      <rdfs:comment xml:lang="en">Relation indicating a GroupLot has a TenderLot associated to it. (epo:TenderLot &lt;-&gt; epo:LotGroup (+epo:isSubmittedFor +epo:hasTenderLot)) </rdfs:comment>
      <rdfs:isDefinedBy rdf:resource="http://data.europa.eu/a4g/ontology"/>
   </owl:ObjectProperty>
   <owl:ObjectProperty rdf:about="http://data.europa.eu/a4g/ontology#isSubmittedFor">
      <rdfs:label xml:lang="en">Is submitted for</rdfs:label>
      <skos:prefLabel xml:lang="en">Is submitted for</skos:prefLabel>
      <skos:scopeNote xml:lang="en">Relation showing that a TenderLot is sumbitted for a group of lots. (epo:TenderLot &lt;-&gt; epo:LotGroup (+epo:isSubmittedFor +epo:hasTenderLot)) </skos:scopeNote>
      <rdfs:comment xml:lang="en">Relation showing that a TenderLot is sumbitted for a group of lots. (epo:TenderLot &lt;-&gt; epo:LotGroup (+epo:isSubmittedFor +epo:hasTenderLot)) </rdfs:comment>
      <rdfs:isDefinedBy rdf:resource="http://data.europa.eu/a4g/ontology"/>
   </owl:ObjectProperty>
   <owl:ObjectProperty rdf:about="http://data.europa.eu/a4g/ontology#hasNotificationContentType">
      <rdfs:label xml:lang="en">Has notification content type</rdfs:label>
      <skos:prefLabel xml:lang="en">Has notification content type</skos:prefLabel>
      <rdfs:isDefinedBy rdf:resource="http://data.europa.eu/a4g/ontology"/>
   </owl:ObjectProperty>
   <owl:ObjectProperty rdf:about="http://data.europa.eu/a4g/ontology#relatedToNotice">
      <rdfs:label xml:lang="en">Related to notice</rdfs:label>
      <skos:prefLabel xml:lang="en">Related to notice</skos:prefLabel>
      <rdfs:isDefinedBy rdf:resource="http://data.europa.eu/a4g/ontology"/>
   </owl:ObjectProperty>
   <owl:ObjectProperty rdf:about="http://data.europa.eu/a4g/ontology#relatesToNotice">
      <rdfs:label xml:lang="en">Relates to notice</rdfs:label>
      <skos:prefLabel xml:lang="en">Relates to notice</skos:prefLabel>
      <rdfs:isDefinedBy rdf:resource="http://data.europa.eu/a4g/ontology"/>
   </owl:ObjectProperty>
   <owl:ObjectProperty rdf:about="http://data.europa.eu/a4g/ontology#hasDPSScope">
      <rdfs:label xml:lang="en">Has d p s scope</rdfs:label>
      <skos:prefLabel xml:lang="en">Has d p s scope</skos:prefLabel>
      <skos:definition xml:lang="en">The codelist to be used is at-voc:dps-usage which is available at https://op.europa.eu/en/web/eu-vocabularies/at-dataset/-/resource/dataset/dps-usage
 (epo:Notice -&gt; at-voc:dps-usage (+epo:hasDPSScope)) </skos:definition>
      <rdfs:comment xml:lang="en">The codelist to be used is at-voc:dps-usage which is available at https://op.europa.eu/en/web/eu-vocabularies/at-dataset/-/resource/dataset/dps-usage
 (epo:Notice -&gt; at-voc:dps-usage (+epo:hasDPSScope)) </rdfs:comment>
      <rdfs:isDefinedBy rdf:resource="http://data.europa.eu/a4g/ontology"/>
   </owl:ObjectProperty>
   <owl:ObjectProperty rdf:about="http://data.europa.eu/a4g/ontology#hasFormType">
      <rdfs:label xml:lang="en">Has form type</rdfs:label>
      <skos:prefLabel xml:lang="en">Has form type</skos:prefLabel>
      <skos:definition xml:lang="en">The codelist to be used is at-voc:form-type which is available at https://op.europa.eu/en/web/eu-vocabularies/at-dataset/-/resource/dataset/form-type
 (epo:Notice -&gt; at-voc:form-type (+epo:hasFormType)) </skos:definition>
      <rdfs:comment xml:lang="en">The codelist to be used is at-voc:form-type which is available at https://op.europa.eu/en/web/eu-vocabularies/at-dataset/-/resource/dataset/form-type
 (epo:Notice -&gt; at-voc:form-type (+epo:hasFormType)) </rdfs:comment>
      <rdfs:isDefinedBy rdf:resource="http://data.europa.eu/a4g/ontology"/>
   </owl:ObjectProperty>
   <owl:ObjectProperty rdf:about="http://data.europa.eu/a4g/ontology#hasOpeningPlace">
      <rdfs:label xml:lang="en">Has opening place</rdfs:label>
      <skos:prefLabel xml:lang="en">Has opening place</skos:prefLabel>
      <skos:definition xml:lang="en">The place where the tenders will be publicly opened.

WG Approval 10-10-2019 (epo:OpeningTerm -&gt; locn:Address (+epo:hasOpeningPlace)) </skos:definition>
      <rdfs:comment xml:lang="en">The place where the tenders will be publicly opened.

WG Approval 10-10-2019 (epo:OpeningTerm -&gt; locn:Address (+epo:hasOpeningPlace)) </rdfs:comment>
      <rdfs:isDefinedBy rdf:resource="http://data.europa.eu/a4g/ontology"/>
   </owl:ObjectProperty>
   <owl:ObjectProperty rdf:about="http://data.europa.eu/a4g/ontology#hasMember">
      <rdfs:label xml:lang="en">Has member</rdfs:label>
      <skos:prefLabel xml:lang="en">Has member</skos:prefLabel>
      <rdfs:isDefinedBy rdf:resource="http://data.europa.eu/a4g/ontology"/>
   </owl:ObjectProperty>
   <owl:ObjectProperty rdf:about="http://data.europa.eu/a4g/ontology#isMemberOf">
      <rdfs:label xml:lang="en">Is member of</rdfs:label>
      <skos:prefLabel xml:lang="en">Is member of</skos:prefLabel>
      <rdfs:isDefinedBy rdf:resource="http://data.europa.eu/a4g/ontology"/>
   </owl:ObjectProperty>
   <owl:ObjectProperty rdf:about="http://data.europa.eu/a4g/ontology#hasRegisteredAddress">
      <rdfs:label xml:lang="en">Has registered address</rdfs:label>
      <skos:prefLabel xml:lang="en">Has registered address</skos:prefLabel>
      <skos:scopeNote xml:lang="en">The officially registered place of an organisation.

WG Approval 16/11/2021
 (epo:Organisation -&gt; locn:Address (+epo:hasRegisteredAddress)) The officially registered place of an organisation.

WG Approval 16/11/2021 (epo:Person -&gt; locn:Address (+epo:hasRegisteredAddress)) </skos:scopeNote>
      <rdfs:comment xml:lang="en">The officially registered place of an organisation.

WG Approval 16/11/2021
 (epo:Organisation -&gt; locn:Address (+epo:hasRegisteredAddress)) The officially registered place of an organisation.

WG Approval 16/11/2021 (epo:Person -&gt; locn:Address (+epo:hasRegisteredAddress)) </rdfs:comment>
      <rdfs:isDefinedBy rdf:resource="http://data.europa.eu/a4g/ontology"/>
   </owl:ObjectProperty>
   <owl:ObjectProperty rdf:about="http://data.europa.eu/a4g/ontology#hasAddress">
      <rdfs:label xml:lang="en">Has address</rdfs:label>
      <skos:prefLabel xml:lang="en">Has address</skos:prefLabel>
      <skos:scopeNote xml:lang="en">A place where an organisation is situated.

Additional information:
This is not the registered location

WG Approval 16/11/2021

 (epo:Organisation -&gt; locn:Address (+epo:hasAddress)) </skos:scopeNote>
      <rdfs:comment xml:lang="en">A place where an organisation is situated.

Additional information:
This is not the registered location

WG Approval 16/11/2021

 (epo:Organisation -&gt; locn:Address (+epo:hasAddress)) </rdfs:comment>
      <rdfs:isDefinedBy rdf:resource="http://data.europa.eu/a4g/ontology"/>
   </owl:ObjectProperty>
   <owl:ObjectProperty rdf:about="http://data.europa.eu/a4g/ontology#leadOf">
      <rdfs:label xml:lang="en">Lead of</rdfs:label>
      <skos:prefLabel xml:lang="en">Lead of</skos:prefLabel>
      <rdfs:isDefinedBy rdf:resource="http://data.europa.eu/a4g/ontology"/>
   </owl:ObjectProperty>
   <owl:ObjectProperty rdf:about="http://data.europa.eu/a4g/ontology#hasTimePeriods">
      <rdfs:label xml:lang="en">Has time periods</rdfs:label>
      <skos:prefLabel xml:lang="en">Has time periods</skos:prefLabel>
      <skos:definition xml:lang="en">The codelist to be used is at-voc:timeperiods which is available at https://op.europa.eu/en/web/eu-vocabularies/at-dataset/-/resource/dataset/timeperiods
 (epo:Period -&gt; at-voc:timeperiod (+epo:hasTimePeriods)) </skos:definition>
      <rdfs:comment xml:lang="en">The codelist to be used is at-voc:timeperiods which is available at https://op.europa.eu/en/web/eu-vocabularies/at-dataset/-/resource/dataset/timeperiods
 (epo:Period -&gt; at-voc:timeperiod (+epo:hasTimePeriods)) </rdfs:comment>
      <rdfs:isDefinedBy rdf:resource="http://data.europa.eu/a4g/ontology"/>
   </owl:ObjectProperty>
   <owl:ObjectProperty rdf:about="http://data.europa.eu/a4g/ontology#hasValidityPeriod">
      <rdfs:label xml:lang="en">Has validity period</rdfs:label>
      <skos:prefLabel xml:lang="en">Has validity period</skos:prefLabel>
      <rdfs:isDefinedBy rdf:resource="http://data.europa.eu/a4g/ontology"/>
   </owl:ObjectProperty>
   <owl:ObjectProperty rdf:about="http://data.europa.eu/a4g/ontology#hasPlannedPeriod">
      <rdfs:label xml:lang="en">Has planned period</rdfs:label>
      <skos:prefLabel xml:lang="en">Has planned period</skos:prefLabel>
      <rdfs:isDefinedBy rdf:resource="http://data.europa.eu/a4g/ontology"/>
   </owl:ObjectProperty>
   <owl:ObjectProperty rdf:about="http://data.europa.eu/a4g/ontology#hasNationality">
      <rdfs:label xml:lang="en">Has nationality</rdfs:label>
      <skos:prefLabel xml:lang="en">Has nationality</skos:prefLabel>
      <skos:definition xml:lang="en">The codelist to be used is at-voc:country which is available at https://op.europa.eu/web/eu-vocabularies/at-dataset/-/resource/dataset/country
 (epo:Person -&gt; at-voc:country (+epo:hasNationality)) </skos:definition>
      <rdfs:comment xml:lang="en">The codelist to be used is at-voc:country which is available at https://op.europa.eu/web/eu-vocabularies/at-dataset/-/resource/dataset/country
 (epo:Person -&gt; at-voc:country (+epo:hasNationality)) </rdfs:comment>
      <rdfs:isDefinedBy rdf:resource="http://data.europa.eu/a4g/ontology"/>
   </owl:ObjectProperty>
   <owl:ObjectProperty rdf:about="http://data.europa.eu/a4g/ontology#hasCountryOfBirth">
      <rdfs:label xml:lang="en">Has country of birth</rdfs:label>
      <skos:prefLabel xml:lang="en">Has country of birth</skos:prefLabel>
      <rdfs:isDefinedBy rdf:resource="http://data.europa.eu/a4g/ontology"/>
   </owl:ObjectProperty>
   <owl:ObjectProperty rdf:about="http://data.europa.eu/a4g/ontology#hasLegalBasis">
      <rdfs:label xml:lang="en">Has legal basis</rdfs:label>
      <skos:prefLabel xml:lang="en">Has legal basis</skos:prefLabel>
      <skos:definition xml:lang="en">The codelist to be used is at-voc:legal-basis which is available at https://op.europa.eu/en/web/eu-vocabularies/at-dataset/-/resource/dataset/legal-basis
 (epo:PlannedProcurementPart -&gt; at-voc:legal-basis (+epo:hasLegalBasis)) The codelist to be used is at-voc:legal-basis which is available at https://op.europa.eu/en/web/eu-vocabularies/at-dataset/-/resource/dataset/legal-basis
 (epo:Procedure -&gt; at-voc:legal-basis (+epo:hasLegalBasis)) </skos:definition>
      <rdfs:comment xml:lang="en">The codelist to be used is at-voc:legal-basis which is available at https://op.europa.eu/en/web/eu-vocabularies/at-dataset/-/resource/dataset/legal-basis
 (epo:PlannedProcurementPart -&gt; at-voc:legal-basis (+epo:hasLegalBasis)) The codelist to be used is at-voc:legal-basis which is available at https://op.europa.eu/en/web/eu-vocabularies/at-dataset/-/resource/dataset/legal-basis
 (epo:Procedure -&gt; at-voc:legal-basis (+epo:hasLegalBasis)) </rdfs:comment>
      <rdfs:isDefinedBy rdf:resource="http://data.europa.eu/a4g/ontology"/>
   </owl:ObjectProperty>
   <owl:ObjectProperty rdf:about="http://data.europa.eu/a4g/ontology#isForeseenInProjectProcurement">
      <rdfs:label xml:lang="en">Is foreseen in project procurement</rdfs:label>
      <skos:prefLabel xml:lang="en">Is foreseen in project procurement</skos:prefLabel>
      <rdfs:isDefinedBy rdf:resource="http://data.europa.eu/a4g/ontology"/>
   </owl:ObjectProperty>
   <owl:ObjectProperty rdf:about="http://data.europa.eu/a4g/ontology#foreseesPlannedProcurementPart">
      <rdfs:label xml:lang="en">Foresees planned procurement part</rdfs:label>
      <skos:prefLabel xml:lang="en">Foresees planned procurement part</skos:prefLabel>
      <rdfs:isDefinedBy rdf:resource="http://data.europa.eu/a4g/ontology"/>
   </owl:ObjectProperty>
   <owl:ObjectProperty rdf:about="http://data.europa.eu/a4g/ontology#hasProcedureType">
      <rdfs:label xml:lang="en">Has procedure type</rdfs:label>
      <skos:prefLabel xml:lang="en">Has procedure type</skos:prefLabel>
      <skos:definition xml:lang="en">The codelist to be used is at-voc:procurement-procedure-type which is available at https://op.europa.eu/en/web/eu-vocabularies/at-dataset/-/resource/dataset/procurement-procedure-type
 (epo:Procedure -&gt; at-voc:procurement-procedure-type (+epo:hasProcedureType)) </skos:definition>
      <rdfs:comment xml:lang="en">The codelist to be used is at-voc:procurement-procedure-type which is available at https://op.europa.eu/en/web/eu-vocabularies/at-dataset/-/resource/dataset/procurement-procedure-type
 (epo:Procedure -&gt; at-voc:procurement-procedure-type (+epo:hasProcedureType)) </rdfs:comment>
      <rdfs:isDefinedBy rdf:resource="http://data.europa.eu/a4g/ontology"/>
   </owl:ObjectProperty>
   <owl:ObjectProperty rdf:about="http://data.europa.eu/a4g/ontology#hasOverallPurpose">
      <rdfs:label xml:lang="en">Has overall purpose</rdfs:label>
      <skos:prefLabel xml:lang="en">Has overall purpose</skos:prefLabel>
      <rdfs:isDefinedBy rdf:resource="http://data.europa.eu/a4g/ontology"/>
   </owl:ObjectProperty>
   <owl:ObjectProperty rdf:about="http://data.europa.eu/a4g/ontology#hasLegalRegime">
      <rdfs:label xml:lang="en">Has legal regime</rdfs:label>
      <skos:prefLabel xml:lang="en">Has legal regime</skos:prefLabel>
      <rdfs:isDefinedBy rdf:resource="http://data.europa.eu/a4g/ontology"/>
   </owl:ObjectProperty>
   <owl:ObjectProperty rdf:about="http://data.europa.eu/a4g/ontology#accessMarketThrough">
      <rdfs:label xml:lang="en">Access market through</rdfs:label>
      <skos:prefLabel xml:lang="en">Access market through</skos:prefLabel>
      <rdfs:isDefinedBy rdf:resource="http://data.europa.eu/a4g/ontology"/>
   </owl:ObjectProperty>
   <owl:ObjectProperty rdf:about="http://data.europa.eu/a4g/ontology#hasNonPublicationJustification">
      <rdfs:label xml:lang="en">Has non publication justification</rdfs:label>
      <skos:prefLabel xml:lang="en">Has non publication justification</skos:prefLabel>
      <skos:definition xml:lang="en">The codelist to be used is at-voc:non-publication-justification which is available at https://op.europa.eu/en/web/eu-vocabularies/at-dataset/-/resource/dataset/non-publication-justification
 (epo:PublicationProvision -&gt; at-voc:non-publication-justification (+epo:hasNonPublicationJustification)) </skos:definition>
      <rdfs:comment xml:lang="en">The codelist to be used is at-voc:non-publication-justification which is available at https://op.europa.eu/en/web/eu-vocabularies/at-dataset/-/resource/dataset/non-publication-justification
 (epo:PublicationProvision -&gt; at-voc:non-publication-justification (+epo:hasNonPublicationJustification)) </rdfs:comment>
      <rdfs:isDefinedBy rdf:resource="http://data.europa.eu/a4g/ontology"/>
   </owl:ObjectProperty>
   <owl:ObjectProperty rdf:about="http://data.europa.eu/a4g/ontology#isForResourceElement">
      <rdfs:label xml:lang="en">Is for resource element</rdfs:label>
      <skos:prefLabel xml:lang="en">Is for resource element</skos:prefLabel>
      <skos:scopeNote xml:lang="en">Relation indication that the publication provision applies to a given field of a document. (epo:PublicationProvision -&gt; epo:ResourceElement (+epo:isForResourceElement)) </skos:scopeNote>
      <rdfs:comment xml:lang="en">Relation indication that the publication provision applies to a given field of a document. (epo:PublicationProvision -&gt; epo:ResourceElement (+epo:isForResourceElement)) </rdfs:comment>
      <rdfs:isDefinedBy rdf:resource="http://data.europa.eu/a4g/ontology"/>
   </owl:ObjectProperty>
   <owl:ObjectProperty rdf:about="http://data.europa.eu/a4g/ontology#hasMainClassification">
      <rdfs:label xml:lang="en">Has main classification</rdfs:label>
      <skos:prefLabel xml:lang="en">Has main classification</skos:prefLabel>
      <skos:definition xml:lang="en">The codelist to be used is at-voc:cpv which is available at https://op.europa.eu/web/eu-vocabularies/at-dataset/-/resource/dataset/cpv
 (epo:Purpose -&gt; at-voc:cpv (+epo:hasMainClassification)) </skos:definition>
      <rdfs:comment xml:lang="en">The codelist to be used is at-voc:cpv which is available at https://op.europa.eu/web/eu-vocabularies/at-dataset/-/resource/dataset/cpv
 (epo:Purpose -&gt; at-voc:cpv (+epo:hasMainClassification)) </rdfs:comment>
      <rdfs:isDefinedBy rdf:resource="http://data.europa.eu/a4g/ontology"/>
   </owl:ObjectProperty>
   <owl:ObjectProperty rdf:about="http://data.europa.eu/a4g/ontology#hasAdditionalClassification">
      <rdfs:label xml:lang="en">Has additional classification</rdfs:label>
      <skos:prefLabel xml:lang="en">Has additional classification</skos:prefLabel>
      <skos:definition xml:lang="en">The codelist to be used is at-voc:cpv which is available at https://op.europa.eu/web/eu-vocabularies/at-dataset/-/resource/dataset/cpv
 (epo:Purpose -&gt; at-voc:cpv (+epo:hasAdditionalClassification)) </skos:definition>
      <rdfs:comment xml:lang="en">The codelist to be used is at-voc:cpv which is available at https://op.europa.eu/web/eu-vocabularies/at-dataset/-/resource/dataset/cpv
 (epo:Purpose -&gt; at-voc:cpv (+epo:hasAdditionalClassification)) </rdfs:comment>
      <rdfs:isDefinedBy rdf:resource="http://data.europa.eu/a4g/ontology"/>
   </owl:ObjectProperty>
   <owl:ObjectProperty rdf:about="http://data.europa.eu/a4g/ontology#hasOptionsPermission">
      <rdfs:label xml:lang="en">Has options permission</rdfs:label>
      <skos:prefLabel xml:lang="en">Has options permission</skos:prefLabel>
      <skos:definition xml:lang="en">The codelist to be used is at-voc:permission which is available at https://op.europa.eu/en/web/eu-vocabularies/at-dataset/-/resource/dataset/permission
 (epo:Purpose -&gt; at-voc:permission (+epo:hasOptionsPermission)) </skos:definition>
      <rdfs:comment xml:lang="en">The codelist to be used is at-voc:permission which is available at https://op.europa.eu/en/web/eu-vocabularies/at-dataset/-/resource/dataset/permission
 (epo:Purpose -&gt; at-voc:permission (+epo:hasOptionsPermission)) </rdfs:comment>
      <rdfs:isDefinedBy rdf:resource="http://data.europa.eu/a4g/ontology"/>
   </owl:ObjectProperty>
   <owl:ObjectProperty rdf:about="http://data.europa.eu/a4g/ontology#hasContractNatureType">
      <rdfs:label xml:lang="en">Has contract nature type</rdfs:label>
      <skos:prefLabel xml:lang="en">Has contract nature type</skos:prefLabel>
      <skos:definition xml:lang="en">The codelist to be used is at-voc:contract-nature which is available at https://op.europa.eu/web/eu-vocabularies/at-dataset/-/resource/dataset/contract-nature
 (epo:Purpose -&gt; at-voc:contract-nature (+epo:hasContractNatureType)) </skos:definition>
      <rdfs:comment xml:lang="en">The codelist to be used is at-voc:contract-nature which is available at https://op.europa.eu/web/eu-vocabularies/at-dataset/-/resource/dataset/contract-nature
 (epo:Purpose -&gt; at-voc:contract-nature (+epo:hasContractNatureType)) </rdfs:comment>
      <rdfs:isDefinedBy rdf:resource="http://data.europa.eu/a4g/ontology"/>
   </owl:ObjectProperty>
   <owl:ObjectProperty rdf:about="http://data.europa.eu/a4g/ontology#hasAdditionalContractNature">
      <rdfs:label xml:lang="en">Has additional contract nature</rdfs:label>
      <skos:prefLabel xml:lang="en">Has additional contract nature</skos:prefLabel>
      <skos:definition xml:lang="en">The codelist to be used is at-voc:contract-nature which is available at https://op.europa.eu/web/eu-vocabularies/at-dataset/-/resource/dataset/contract-nature
 (epo:Purpose -&gt; at-voc:contract-nature (+epo:hasAdditionalContractNature)) </skos:definition>
      <rdfs:comment xml:lang="en">The codelist to be used is at-voc:contract-nature which is available at https://op.europa.eu/web/eu-vocabularies/at-dataset/-/resource/dataset/contract-nature
 (epo:Purpose -&gt; at-voc:contract-nature (+epo:hasAdditionalContractNature)) </rdfs:comment>
      <rdfs:isDefinedBy rdf:resource="http://data.europa.eu/a4g/ontology"/>
   </owl:ObjectProperty>
   <owl:ObjectProperty rdf:about="http://data.europa.eu/a4g/ontology#hasRegulatoryFrameworkType">
      <rdfs:label xml:lang="en">Has regulatory framework type</rdfs:label>
      <skos:prefLabel xml:lang="en">Has regulatory framework type</skos:prefLabel>
      <rdfs:isDefinedBy rdf:resource="http://data.europa.eu/a4g/ontology"/>
   </owl:ObjectProperty>
   <owl:ObjectProperty rdf:about="http://data.europa.eu/a4g/ontology#describesSecurityClearanceToAddress">
      <rdfs:label xml:lang="en">Describes security clearance to address</rdfs:label>
      <skos:prefLabel xml:lang="en">Describes security clearance to address</skos:prefLabel>
      <skos:scopeNote xml:lang="en">Relation that specifies access rules to a location. (epo:SecurityClearanceTerm -&gt; locn:Address (+epo:describesSecurityClearanceToAddress)) </skos:scopeNote>
      <rdfs:comment xml:lang="en">Relation that specifies access rules to a location. (epo:SecurityClearanceTerm -&gt; locn:Address (+epo:describesSecurityClearanceToAddress)) </rdfs:comment>
      <rdfs:isDefinedBy rdf:resource="http://data.europa.eu/a4g/ontology"/>
   </owl:ObjectProperty>
   <owl:ObjectProperty rdf:about="http://data.europa.eu/a4g/ontology#hasSelectionCriterionType">
      <rdfs:label xml:lang="en">Has selection criterion type</rdfs:label>
      <skos:prefLabel xml:lang="en">Has selection criterion type</skos:prefLabel>
      <skos:definition xml:lang="en">The codelist to be used is at-voc:selection-criterion which is available at https://op.europa.eu/en/web/eu-vocabularies/at-dataset/-/resource/dataset/selection-criterion
 (epo:SelectionCriterion -&gt; at-voc:selection-criterion (+epo:hasSelectionCriterionType)) </skos:definition>
      <rdfs:comment xml:lang="en">The codelist to be used is at-voc:selection-criterion which is available at https://op.europa.eu/en/web/eu-vocabularies/at-dataset/-/resource/dataset/selection-criterion
 (epo:SelectionCriterion -&gt; at-voc:selection-criterion (+epo:hasSelectionCriterionType)) </rdfs:comment>
      <rdfs:isDefinedBy rdf:resource="http://data.europa.eu/a4g/ontology"/>
   </owl:ObjectProperty>
   <owl:ObjectProperty rdf:about="http://data.europa.eu/a4g/ontology#proposesSubcontractor">
      <rdfs:label xml:lang="en">Proposes subcontractor</rdfs:label>
      <skos:prefLabel xml:lang="en">Proposes subcontractor</skos:prefLabel>
      <rdfs:isDefinedBy rdf:resource="http://data.europa.eu/a4g/ontology"/>
   </owl:ObjectProperty>
   <owl:ObjectProperty rdf:about="http://data.europa.eu/a4g/ontology#proposes">
      <rdfs:label xml:lang="en">Proposes</rdfs:label>
      <skos:prefLabel xml:lang="en">Proposes</skos:prefLabel>
      <rdfs:isDefinedBy rdf:resource="http://data.europa.eu/a4g/ontology"/>
   </owl:ObjectProperty>
   <owl:ObjectProperty rdf:about="http://data.europa.eu/a4g/ontology#hasSubcontractingObligation">
      <rdfs:label xml:lang="en">Has subcontracting obligation</rdfs:label>
      <skos:prefLabel xml:lang="en">Has subcontracting obligation</skos:prefLabel>
      <skos:definition xml:lang="en">The codelist to be used is at-voc:subcontracting-obligation which is available at https://op.europa.eu/en/web/eu-vocabularies/at-dataset/-/resource/dataset/subcontracting-obligation
 (epo:SubcontractTerm -&gt; at-voc:subcontracting-obligation (+epo:hasSubcontractingObligation)) </skos:definition>
      <rdfs:comment xml:lang="en">The codelist to be used is at-voc:subcontracting-obligation which is available at https://op.europa.eu/en/web/eu-vocabularies/at-dataset/-/resource/dataset/subcontracting-obligation
 (epo:SubcontractTerm -&gt; at-voc:subcontracting-obligation (+epo:hasSubcontractingObligation)) </rdfs:comment>
      <rdfs:isDefinedBy rdf:resource="http://data.europa.eu/a4g/ontology"/>
   </owl:ObjectProperty>
   <owl:ObjectProperty rdf:about="http://data.europa.eu/a4g/ontology#hasLateSubmissionPermission">
      <rdfs:label xml:lang="en">Has late submission permission</rdfs:label>
      <skos:prefLabel xml:lang="en">Has late submission permission</skos:prefLabel>
      <skos:definition xml:lang="en">The codelist to be used is at-voc:missing-info-submission which is available at https://op.europa.eu/en/web/eu-vocabularies/at-dataset/-/resource/dataset/missing-info-submission
 (epo:SubmissionTerm -&gt; at-voc:missing-info-submission (+epo:hasLateSubmissionPermission)) </skos:definition>
      <rdfs:comment xml:lang="en">The codelist to be used is at-voc:missing-info-submission which is available at https://op.europa.eu/en/web/eu-vocabularies/at-dataset/-/resource/dataset/missing-info-submission
 (epo:SubmissionTerm -&gt; at-voc:missing-info-submission (+epo:hasLateSubmissionPermission)) </rdfs:comment>
      <rdfs:isDefinedBy rdf:resource="http://data.europa.eu/a4g/ontology"/>
   </owl:ObjectProperty>
   <owl:ObjectProperty rdf:about="http://data.europa.eu/a4g/ontology#hasNonElectronicSubmissionJustification">
      <rdfs:label xml:lang="en">Has non electronic submission justification</rdfs:label>
      <skos:prefLabel xml:lang="en">Has non electronic submission justification</skos:prefLabel>
      <skos:definition xml:lang="en">The codelist to be used is at-voc:communication-justification which is available at https://op.europa.eu/web/eu-vocabularies/at-dataset/-/resource/dataset/communication-justification
 (epo:SubmissionTerm -&gt; at-voc:communication-justification (+epo:hasNonElectronicSubmissionJustification)) </skos:definition>
      <rdfs:comment xml:lang="en">The codelist to be used is at-voc:communication-justification which is available at https://op.europa.eu/web/eu-vocabularies/at-dataset/-/resource/dataset/communication-justification
 (epo:SubmissionTerm -&gt; at-voc:communication-justification (+epo:hasNonElectronicSubmissionJustification)) </rdfs:comment>
      <rdfs:isDefinedBy rdf:resource="http://data.europa.eu/a4g/ontology"/>
   </owl:ObjectProperty>
   <owl:ObjectProperty rdf:about="http://data.europa.eu/a4g/ontology#hasESubmissionPermission">
      <rdfs:label xml:lang="en">Has e submission permission</rdfs:label>
      <skos:prefLabel xml:lang="en">Has e submission permission</skos:prefLabel>
      <skos:definition xml:lang="en">The codelist to be used is at-voc:permission which is available at https://op.europa.eu/en/web/eu-vocabularies/at-dataset/-/resource/dataset/permission
 (epo:SubmissionTerm -&gt; at-voc:permission (+epo:hasESubmissionPermission)) </skos:definition>
      <rdfs:comment xml:lang="en">The codelist to be used is at-voc:permission which is available at https://op.europa.eu/en/web/eu-vocabularies/at-dataset/-/resource/dataset/permission
 (epo:SubmissionTerm -&gt; at-voc:permission (+epo:hasESubmissionPermission)) </rdfs:comment>
      <rdfs:isDefinedBy rdf:resource="http://data.europa.eu/a4g/ontology"/>
   </owl:ObjectProperty>
   <owl:ObjectProperty rdf:about="http://data.europa.eu/a4g/ontology#hasTenderSubcontractingInformation">
      <rdfs:label xml:lang="en">Has tender subcontracting information</rdfs:label>
      <skos:prefLabel xml:lang="en">Has tender subcontracting information</skos:prefLabel>
      <skos:definition xml:lang="en">The codelist to be used is at-voc:subcontracting-indication which is available at https://op.europa.eu/en/web/eu-vocabularies/at-dataset/-/resource/dataset/subcontracting-indication
 (epo:SubmissionTerm -&gt; at-voc:subcontracting-indication (+epo:hasTenderSubcontractingInformation)) </skos:definition>
      <rdfs:comment xml:lang="en">The codelist to be used is at-voc:subcontracting-indication which is available at https://op.europa.eu/en/web/eu-vocabularies/at-dataset/-/resource/dataset/subcontracting-indication
 (epo:SubmissionTerm -&gt; at-voc:subcontracting-indication (+epo:hasTenderSubcontractingInformation)) </rdfs:comment>
      <rdfs:isDefinedBy rdf:resource="http://data.europa.eu/a4g/ontology"/>
   </owl:ObjectProperty>
   <owl:ObjectProperty rdf:about="http://data.europa.eu/a4g/ontology#hasECataloguePermission">
      <rdfs:label xml:lang="en">Has e catalogue permission</rdfs:label>
      <skos:prefLabel xml:lang="en">Has e catalogue permission</skos:prefLabel>
      <skos:definition xml:lang="en">The codelist to be used is at-voc:permission which is available at https://op.europa.eu/en/web/eu-vocabularies/at-dataset/-/resource/dataset/permission
 (epo:SubmissionTerm -&gt; at-voc:permission (+epo:hasECataloguePermission)) </skos:definition>
      <rdfs:comment xml:lang="en">The codelist to be used is at-voc:permission which is available at https://op.europa.eu/en/web/eu-vocabularies/at-dataset/-/resource/dataset/permission
 (epo:SubmissionTerm -&gt; at-voc:permission (+epo:hasECataloguePermission)) </rdfs:comment>
      <rdfs:isDefinedBy rdf:resource="http://data.europa.eu/a4g/ontology"/>
   </owl:ObjectProperty>
   <owl:ObjectProperty rdf:about="http://data.europa.eu/a4g/ontology#hasLanguage">
      <rdfs:label xml:lang="en">Has language</rdfs:label>
      <skos:prefLabel xml:lang="en">Has language</skos:prefLabel>
      <skos:definition xml:lang="en">The codelist to be used is at-voc:language which is available at https://op.europa.eu/en/web/eu-vocabularies/at-dataset/-/resource/dataset/language
 (epo:SubmissionTerm -&gt; at-voc:language (+epo:hasLanguage)) </skos:definition>
      <rdfs:comment xml:lang="en">The codelist to be used is at-voc:language which is available at https://op.europa.eu/en/web/eu-vocabularies/at-dataset/-/resource/dataset/language
 (epo:SubmissionTerm -&gt; at-voc:language (+epo:hasLanguage)) </rdfs:comment>
      <rdfs:isDefinedBy rdf:resource="http://data.europa.eu/a4g/ontology"/>
   </owl:ObjectProperty>
   <owl:ObjectProperty rdf:about="http://data.europa.eu/a4g/ontology#includesAccessibilityCriterion">
      <rdfs:label xml:lang="en">Includes accessibility criterion</rdfs:label>
      <skos:prefLabel xml:lang="en">Includes accessibility criterion</skos:prefLabel>
      <skos:definition xml:lang="en">The code list to be used for the predicate includesAccessibilityCriteria  is at:voc:accessibility which is available at 
https://op.europa.eu/web/eu-vocabularies/at-dataset/-/resource/dataset/accessibility (epo:TechnicalSpecification -&gt; at-voc:accessibility (+epo:includesAccessibilityCriterion)) </skos:definition>
      <rdfs:comment xml:lang="en">The code list to be used for the predicate includesAccessibilityCriteria  is at:voc:accessibility which is available at 
https://op.europa.eu/web/eu-vocabularies/at-dataset/-/resource/dataset/accessibility (epo:TechnicalSpecification -&gt; at-voc:accessibility (+epo:includesAccessibilityCriterion)) </rdfs:comment>
      <rdfs:isDefinedBy rdf:resource="http://data.europa.eu/a4g/ontology"/>
   </owl:ObjectProperty>
   <owl:ObjectProperty rdf:about="http://data.europa.eu/a4g/ontology#isIncludedIn">
      <rdfs:label xml:lang="en">Is included in</rdfs:label>
      <skos:prefLabel xml:lang="en">Is included in</skos:prefLabel>
      <rdfs:isDefinedBy rdf:resource="http://data.europa.eu/a4g/ontology"/>
   </owl:ObjectProperty>
   <owl:ObjectProperty rdf:about="http://data.europa.eu/a4g/ontology#withdraws">
      <rdfs:label xml:lang="en">Withdraws</rdfs:label>
      <skos:prefLabel xml:lang="en">Withdraws</skos:prefLabel>
      <rdfs:isDefinedBy rdf:resource="http://data.europa.eu/a4g/ontology"/>
   </owl:ObjectProperty>
   <owl:ObjectProperty rdf:about="http://data.europa.eu/a4g/ontology#isSubmittedBy">
      <rdfs:label xml:lang="en">Is submitted by</rdfs:label>
      <skos:prefLabel xml:lang="en">Is submitted by</skos:prefLabel>
      <skos:scopeNote xml:lang="en">Relation indicating the economic operator who submitted a Tender.
WG approval 18/05/2021 (epo:Tenderer &lt;-&gt; epo:Tender (+epo:submits +epo:isSubmittedBy)) </skos:scopeNote>
      <rdfs:comment xml:lang="en">Relation indicating the economic operator who submitted a Tender.
WG approval 18/05/2021 (epo:Tenderer &lt;-&gt; epo:Tender (+epo:submits +epo:isSubmittedBy)) </rdfs:comment>
      <rdfs:isDefinedBy rdf:resource="http://data.europa.eu/a4g/ontology"/>
   </owl:ObjectProperty>
   <owl:ObjectProperty rdf:about="http://data.europa.eu/a4g/ontology#submits">
      <rdfs:label xml:lang="en">Submits</rdfs:label>
      <skos:prefLabel xml:lang="en">Submits</skos:prefLabel>
      <skos:scopeNote xml:lang="en">Relation indicating the submission of a tender by an economic operator.
WG approval 18/05/2021 (epo:Tenderer &lt;-&gt; epo:Tender (+epo:submits +epo:isSubmittedBy)) </skos:scopeNote>
      <rdfs:comment xml:lang="en">Relation indicating the submission of a tender by an economic operator.
WG approval 18/05/2021 (epo:Tenderer &lt;-&gt; epo:Tender (+epo:submits +epo:isSubmittedBy)) </rdfs:comment>
      <rdfs:isDefinedBy rdf:resource="http://data.europa.eu/a4g/ontology"/>
   </owl:ObjectProperty>
   <owl:ObjectProperty rdf:about="http://data.europa.eu/a4g/ontology#hasFinancialOfferValue">
      <rdfs:label xml:lang="en">Has financial offer value</rdfs:label>
      <skos:prefLabel xml:lang="en">Has financial offer value</skos:prefLabel>
      <skos:definition xml:lang="en">The value offered by the Tenderer for a Lot.

Additional Information:

This value is normally the one awarded for a winning Tender Lot. In case of negotiated procedures the original financial value may be reviewed and the offer updated.
 (epo:TenderLot -&gt; epo:Value (+epo:hasFinancialOfferValue)) </skos:definition>
      <rdfs:comment xml:lang="en">The value offered by the Tenderer for a Lot.

Additional Information:

This value is normally the one awarded for a winning Tender Lot. In case of negotiated procedures the original financial value may be reviewed and the offer updated.
 (epo:TenderLot -&gt; epo:Value (+epo:hasFinancialOfferValue)) </rdfs:comment>
      <rdfs:isDefinedBy rdf:resource="http://data.europa.eu/a4g/ontology"/>
   </owl:ObjectProperty>
   <owl:ObjectProperty rdf:about="http://data.europa.eu/a4g/ontology#isRankedBy">
      <rdfs:label xml:lang="en">Is ranked by</rdfs:label>
      <skos:prefLabel xml:lang="en">Is ranked by</skos:prefLabel>
      <rdfs:isDefinedBy rdf:resource="http://data.europa.eu/a4g/ontology"/>
   </owl:ObjectProperty>
   <owl:ObjectProperty rdf:about="http://data.europa.eu/a4g/ontology#ranks">
      <rdfs:label xml:lang="en">Ranks</rdfs:label>
      <skos:prefLabel xml:lang="en">Ranks</skos:prefLabel>
      <rdfs:isDefinedBy rdf:resource="http://data.europa.eu/a4g/ontology"/>
   </owl:ObjectProperty>
   <owl:ObjectProperty rdf:about="http://data.europa.eu/a4g/ontology#hasCurrency">
      <rdfs:label xml:lang="en">Has currency</rdfs:label>
      <skos:prefLabel xml:lang="en">Has currency</skos:prefLabel>
      <skos:definition xml:lang="en">The codelist to be used is at-voc:currency which is available at https://op.europa.eu/en/web/eu-vocabularies/at-dataset/-/resource/dataset/currency
 (epo:Amount -&gt; at-voc:currency (+epo:hasCurrency)) </skos:definition>
      <rdfs:comment xml:lang="en">The codelist to be used is at-voc:currency which is available at https://op.europa.eu/en/web/eu-vocabularies/at-dataset/-/resource/dataset/currency
 (epo:Amount -&gt; at-voc:currency (+epo:hasCurrency)) </rdfs:comment>
      <rdfs:isDefinedBy rdf:resource="http://data.europa.eu/a4g/ontology"/>
   </owl:ObjectProperty>
   <owl:ObjectProperty rdf:about="http://data.europa.eu/a4g/ontology#hasUnitCode">
      <rdfs:label xml:lang="en">Has unit code</rdfs:label>
      <skos:prefLabel xml:lang="en">Has unit code</skos:prefLabel>
      <skos:definition xml:lang="en">The codelist to be used is at-voc:measurement-unit which is available at https://op.europa.eu/en/web/eu-vocabularies/at-dataset/-/resource/dataset/measurement-unit
 (epo:Measure -&gt; at-voc:measurement-unit (+epo:hasUnitCode)) </skos:definition>
      <rdfs:comment xml:lang="en">The codelist to be used is at-voc:measurement-unit which is available at https://op.europa.eu/en/web/eu-vocabularies/at-dataset/-/resource/dataset/measurement-unit
 (epo:Measure -&gt; at-voc:measurement-unit (+epo:hasUnitCode)) </rdfs:comment>
      <rdfs:isDefinedBy rdf:resource="http://data.europa.eu/a4g/ontology"/>
   </owl:ObjectProperty>
   <owl:ObjectProperty rdf:about="http://data.europa.eu/a4g/ontology#geographicIdentifier">
      <rdfs:label xml:lang="en">Geographic identifier</rdfs:label>
      <skos:prefLabel xml:lang="en">Geographic identifier</skos:prefLabel>
      <rdfs:comment xml:lang="en">A URI that identifies the Location.

Additional Information:
GeoNames.org provides stable, widely recognised identifiers for more than 10 million geographical names that can be used as links to further information. For example, http://sws.geonames.org/593116/ identifies the Lithuanian capital Vilnius. Unfortunately these URIs cannot easily be automatically deduced since the URI scheme uses simple numeric codes. Finding a GeoNames identifier for a Location is almost always a manual process. Where such identifiers are known or can be found, however, it is recommended that they be used.

Where the Location Class is used to identify a country, if the geonames URI is not known, the recommendation is to use DBpedia URIs of the form http://dbpedia.org/resource/ISO_3166-1:XX where XX is the ISO 3166 two character code for the country.

The EU's Publication Office diverges from ISO 3166-1 and uses EL and UK for Greece and the United Kingdom respectively. DBpedia sticks to the ISO codes and so the correct URIs for these countries are:

- http://dbpedia.org/resource/ISO_3166-1:GR
- http://dbpedia.org/resource/ISO_3166-1:GB
even when the geographic name is given as EL or UK.

The use of a URIs has added advantages:

- it can be used by automated systems to look up additional data (linked data);
- a triple store may store only one copy of the URI, whereas if a string is used, a copy of that string is always stored for each and every person in the database. Thus, in large data sets, the saving on memory capacity and the improvement in transmission efficiency can be substantial. (dct:Location) </rdfs:comment>
      <skos:definition xml:lang="en">A URI that identifies the Location.

Additional Information:
GeoNames.org provides stable, widely recognised identifiers for more than 10 million geographical names that can be used as links to further information. For example, http://sws.geonames.org/593116/ identifies the Lithuanian capital Vilnius. Unfortunately these URIs cannot easily be automatically deduced since the URI scheme uses simple numeric codes. Finding a GeoNames identifier for a Location is almost always a manual process. Where such identifiers are known or can be found, however, it is recommended that they be used.

Where the Location Class is used to identify a country, if the geonames URI is not known, the recommendation is to use DBpedia URIs of the form http://dbpedia.org/resource/ISO_3166-1:XX where XX is the ISO 3166 two character code for the country.

The EU's Publication Office diverges from ISO 3166-1 and uses EL and UK for Greece and the United Kingdom respectively. DBpedia sticks to the ISO codes and so the correct URIs for these countries are:

- http://dbpedia.org/resource/ISO_3166-1:GR
- http://dbpedia.org/resource/ISO_3166-1:GB
even when the geographic name is given as EL or UK.

The use of a URIs has added advantages:

- it can be used by automated systems to look up additional data (linked data);
- a triple store may store only one copy of the URI, whereas if a string is used, a copy of that string is always stored for each and every person in the database. Thus, in large data sets, the saving on memory capacity and the improvement in transmission efficiency can be substantial. (dct:Location) </skos:definition>
      <rdfs:isDefinedBy rdf:resource="http://data.europa.eu/a4g/ontology"/>
   </owl:ObjectProperty>
   <owl:DatatypeProperty rdf:about="http://data.europa.eu/a4g/ontology#geographicName">
      <rdfs:label xml:lang="en">Geographic name</rdfs:label>
      <skos:prefLabel xml:lang="en">Geographic name</skos:prefLabel>
      <rdfs:comment xml:lang="en">A geographic name is a proper noun applied to a spatial object.

Additional Information:
The INSPIRE Data Specification on Geographical Names provides a detailed model for describing a 'named place', including methods for providing multiple names in multiple scripts. This is beyond what is necessary for the Core Location Vocabulary but, importantly, the concept of a geographic name used here is consistent.

A geographic name is a proper noun applied to a spatial object. Taking the example used in the INSPIRE document (page 15), the following are all valid geographic names for the Greek capital:

- "Aθnνa"@gr-Grek (the Greek endonym written in the Greek script)
- "Ath&amp;#237;na"@gr-Latn (the standard Romanisation of the endonym)
- "Athens"@en (the English language exonym)
INSPIRE has a detailed (XML-based) method of providing metadata about a geographic name and in XML-data sets that may be the most appropriate method to follow. When using the Core Location Vocabulary in data sets that are not focussed on environmental/geographical data (the use case for INSPIRE), the Code datatype or a simple language identifier may be used to provide such metadata.

The country codes defined in ISO 3166 may be used as geographic names and these are generally preferred over either the long form or short form of a country's name (as they are less error prone). The Publications Office of the European Union recommends the use of ISO 3166-1 codes for countries in all cases except two:

- use 'UK' in preference to the ISO 3166 code GB for the United Kingdom;
- use 'EL' in preference to the ISO 3166 code GR for Greece.
Where a country has changed its name or no longer exists (such as Czechoslovakia, Yugoslavia etc.) use the ISO 3166-3 code. (dct:Location) </rdfs:comment>
      <skos:definition xml:lang="en">A geographic name is a proper noun applied to a spatial object.

Additional Information:
The INSPIRE Data Specification on Geographical Names provides a detailed model for describing a 'named place', including methods for providing multiple names in multiple scripts. This is beyond what is necessary for the Core Location Vocabulary but, importantly, the concept of a geographic name used here is consistent.

A geographic name is a proper noun applied to a spatial object. Taking the example used in the INSPIRE document (page 15), the following are all valid geographic names for the Greek capital:

- "Aθnνa"@gr-Grek (the Greek endonym written in the Greek script)
- "Ath&amp;#237;na"@gr-Latn (the standard Romanisation of the endonym)
- "Athens"@en (the English language exonym)
INSPIRE has a detailed (XML-based) method of providing metadata about a geographic name and in XML-data sets that may be the most appropriate method to follow. When using the Core Location Vocabulary in data sets that are not focussed on environmental/geographical data (the use case for INSPIRE), the Code datatype or a simple language identifier may be used to provide such metadata.

The country codes defined in ISO 3166 may be used as geographic names and these are generally preferred over either the long form or short form of a country's name (as they are less error prone). The Publications Office of the European Union recommends the use of ISO 3166-1 codes for countries in all cases except two:

- use 'UK' in preference to the ISO 3166 code GB for the United Kingdom;
- use 'EL' in preference to the ISO 3166 code GR for Greece.
Where a country has changed its name or no longer exists (such as Czechoslovakia, Yugoslavia etc.) use the ISO 3166-3 code. (dct:Location) </skos:definition>
      <rdfs:isDefinedBy rdf:resource="http://data.europa.eu/a4g/ontology"/>
   </owl:DatatypeProperty>
   <owl:DatatypeProperty rdf:about="http://data.europa.eu/a4g/ontology#hasAdditionalInformationDeadline">
      <rdfs:label xml:lang="en">Has additional information deadline</rdfs:label>
      <skos:prefLabel xml:lang="en">Has additional information deadline</skos:prefLabel>
      <rdfs:comment xml:lang="en">The time limit for requesting further information.

Additional information:

This is generally used to indicate the deadline for Economic Operators to request further information of the procedure before the submission deadline.

WG Approval 09/06/2020
 (epo:AccessTerm) The time limit for requesting further information.

Additional information:

This is generally used to indicate the deadline for Economic Operators to request further information of the procedure before the submission deadline.

WG Approval 09/06/2020
 (epo:ProcedureTerm) </rdfs:comment>
      <skos:definition xml:lang="en">The time limit for requesting further information.

Additional information:

This is generally used to indicate the deadline for Economic Operators to request further information of the procedure before the submission deadline.

WG Approval 09/06/2020
 (epo:AccessTerm) The time limit for requesting further information.

Additional information:

This is generally used to indicate the deadline for Economic Operators to request further information of the procedure before the submission deadline.

WG Approval 09/06/2020
 (epo:ProcedureTerm) </skos:definition>
      <rdfs:isDefinedBy rdf:resource="http://data.europa.eu/a4g/ontology"/>
   </owl:DatatypeProperty>
   <owl:DatatypeProperty rdf:about="http://data.europa.eu/a4g/ontology#hasProcurementDocumentLandingPage">
      <rdfs:label xml:lang="en">Has procurement document landing page</rdfs:label>
      <skos:prefLabel xml:lang="en">Has procurement document landing page</skos:prefLabel>
      <rdfs:comment xml:lang="en">Web page where the procurement documents can be downloaded.

WG Approval 09/03/2021
 (epo:AccessTerm) </rdfs:comment>
      <skos:definition xml:lang="en">Web page where the procurement documents can be downloaded.

WG Approval 09/03/2021
 (epo:AccessTerm) </skos:definition>
      <rdfs:isDefinedBy rdf:resource="http://data.europa.eu/a4g/ontology"/>
   </owl:DatatypeProperty>
   <owl:DatatypeProperty rdf:about="http://data.europa.eu/a4g/ontology#hasSomeProcurementDocumentRestricted">
      <rdfs:label xml:lang="en">Has some procurement document restricted</rdfs:label>
      <skos:prefLabel xml:lang="en">Has some procurement document restricted</skos:prefLabel>
      <rdfs:comment xml:lang="en">The access to certain procurement documents is restricted.

WG Approval 10/10/2019 (epo:AccessTerm) </rdfs:comment>
      <skos:definition xml:lang="en">The access to certain procurement documents is restricted.

WG Approval 10/10/2019 (epo:AccessTerm) </skos:definition>
      <rdfs:isDefinedBy rdf:resource="http://data.europa.eu/a4g/ontology"/>
   </owl:DatatypeProperty>
   <owl:DatatypeProperty rdf:about="http://data.europa.eu/a4g/ontology#hasSomeProcurementDocumentRestrictedJustification">
      <rdfs:label xml:lang="en">Has some procurement document restricted justification</rdfs:label>
      <skos:prefLabel xml:lang="en">Has some procurement document restricted justification</skos:prefLabel>
      <rdfs:comment xml:lang="en">An explanation about the reasons why some procurement documents are restricted.

WG Approval 09/03/2021
 (epo:AccessTerm) </rdfs:comment>
      <skos:definition xml:lang="en">An explanation about the reasons why some procurement documents are restricted.

WG Approval 09/03/2021
 (epo:AccessTerm) </skos:definition>
      <rdfs:isDefinedBy rdf:resource="http://data.europa.eu/a4g/ontology"/>
   </owl:DatatypeProperty>
   <owl:DatatypeProperty rdf:about="http://data.europa.eu/a4g/ontology#hasAlias">
      <rdfs:label xml:lang="en">Has alias</rdfs:label>
      <skos:prefLabel xml:lang="en">Has alias</skos:prefLabel>
      <rdfs:comment xml:lang="en">Acronym or alternative name of the Agent.
WG Approval 25/03/2021 (epo:Agent) </rdfs:comment>
      <skos:definition xml:lang="en">Acronym or alternative name of the Agent.
WG Approval 25/03/2021 (epo:Agent) </skos:definition>
      <rdfs:isDefinedBy rdf:resource="http://data.europa.eu/a4g/ontology"/>
   </owl:DatatypeProperty>
   <owl:ObjectProperty rdf:about="http://data.europa.eu/a4g/ontology#hasID">
      <rdfs:label xml:lang="en">Has i d</rdfs:label>
      <skos:prefLabel xml:lang="en">Has i d</skos:prefLabel>
      <rdfs:comment xml:lang="en">A unique identifier of the instance of the concept.
Additional Information:
For example, in the case of the Procurement Identifier, this could be the European Public Procurement Identifier, and/or any other identifier provided by the buyer, the service provider or any other stakeholder.
WG Approval 12/11/2019 (epo:Agent) A unique identifier of the instance of the concept.
Additional Information:
For example, in the case of the Procurement Identifier, this could be the European Public Procurement Identifier, and/or any other identifier provided by the buyer, the service provider or any other stakeholder.
WG Approval 12/11/2019
 (epo:AwardCriterion) A unique identifier of the instance of the concept.

Additional Information:

For example, in the case of the Procurement Identifier, this could be the European Public Procurement Identifier, and/or any other identifier provided by the buyer, the service provider or any other stakeholder.

WG Approval 12/11/2019
 (epo:Contract) A unique identifier of the instance of the concept.

Additional Information

For example, in the case of the Procurement Identifier, this could be the European Public Procurement Identifier, and/or any other identifier provided by the buyer, the service provider or any other stakeholder.

WG Approval 12/11/2019
 (epo:Document) A unique identifier of the instance of the concept.

Additional Information

For example, in the case of the Procurement Identifier, this could be the European Public Procurement Identifier, and/or any other identifier provided by the buyer, the service provider or any other stakeholder.

WG Approval 12/11/2019 (epo:Fund) A unique identifier of the instance of the concept.

Additional Information

For example, in the case of the Procurement Identifier, this could be the European Public Procurement Identifier, and/or any other identifier provided by the buyer, the service provider or any other stakeholder.

WG Approval 12/11/2019 (epo:Item) A unique identifier of the instance of the concept.

Additional Information

For example, in the case of the Procurement Identifier, this could be the European Public Procurement Identifier, and/or any other identifier provided by the buyer, the service provider or any other stakeholder.

WG Approval 12/11/2019 (epo:Lot) A unique identifier of the instance of the concept.

Additional Information

For example, in the case of the Procurement Identifier, this could be the European Public Procurement Identifier, and/or any other identifier provided by the buyer, the service provider or any other stakeholder.

WG Approval 12/11/2019 (epo:LotGroup) A unique identifier of the instance of the concept.

Additional Information

For example, in the case of the Procurement Identifier, this could be the European Public Procurement Identifier, and/or any other identifier provided by the buyer, the service provider or any other stakeholder.

WG Approval 12/11/2019 (epo:Person) A unique identifier of the instance of the concept.

Additional Information

For example, in the case of the Procurement Identifier, this could be the European Public Procurement Identifier, and/or any other identifier provided by the buyer, the service provider or any other stakeholder.

WG Approval 12/11/2019
 (epo:PlannedProcurementPart) A unique identifier of the instance of the concept.

Additional Information

For example, in the case of the Procurement Identifier, this could be the European Public Procurement Identifier, and/or any other identifier provided by the buyer, the service provider or any other stakeholder.

WG Approval 12/11/2019 (epo:Procedure) A unique identifier of the instance of the concept.

Additional Information

For example, in the case of the Procurement Identifier, this could be the European Public Procurement Identifier, and/or any other identifier provided by the buyer, the service provider or any other stakeholder.

WG Approval 12/11/2019 (epo:ProcurementCriterion) A unique identifier of the instance of the concept.

Additional Information

For example, in the case of the Procurement Identifier, this could be the European Public Procurement Identifier, and/or any other identifier provided by the buyer, the service provider or any other stakeholder.

WG Approval 12/11/2019 (epo:ProjectProcurement) A unique identifier of the instance of the concept.

Additional Information

For example, in the case of the Procurement Identifier, this could be the European Public Procurement Identifier, and/or any other identifier provided by the buyer, the service provider or any other stakeholder.

WG Approval 12/11/2019 (epo:Technique) A unique identifier of the instance of the concept.

Additional Information

For example, in the case of the Procurement Identifier, this could be the European Public Procurement Identifier, and/or any other identifier provided by the buyer, the service provider or any other stakeholder.

WG Approval 12/11/2019
 (epo:Tender) A unique identifier of the instance of the concept.

Additional Information

For example, in the case of the Procurement Identifier, this could be the European Public Procurement Identifier, and/or any other identifier provided by the buyer, the service provider or any other stakeholder.

WG Approval 12/11/2019 (epo:TenderLot) </rdfs:comment>
      <skos:definition xml:lang="en">A unique identifier of the instance of the concept.
Additional Information:
For example, in the case of the Procurement Identifier, this could be the European Public Procurement Identifier, and/or any other identifier provided by the buyer, the service provider or any other stakeholder.
WG Approval 12/11/2019 (epo:Agent) A unique identifier of the instance of the concept.
Additional Information:
For example, in the case of the Procurement Identifier, this could be the European Public Procurement Identifier, and/or any other identifier provided by the buyer, the service provider or any other stakeholder.
WG Approval 12/11/2019
 (epo:AwardCriterion) A unique identifier of the instance of the concept.

Additional Information:

For example, in the case of the Procurement Identifier, this could be the European Public Procurement Identifier, and/or any other identifier provided by the buyer, the service provider or any other stakeholder.

WG Approval 12/11/2019
 (epo:Contract) A unique identifier of the instance of the concept.

Additional Information

For example, in the case of the Procurement Identifier, this could be the European Public Procurement Identifier, and/or any other identifier provided by the buyer, the service provider or any other stakeholder.

WG Approval 12/11/2019
 (epo:Document) A unique identifier of the instance of the concept.

Additional Information

For example, in the case of the Procurement Identifier, this could be the European Public Procurement Identifier, and/or any other identifier provided by the buyer, the service provider or any other stakeholder.

WG Approval 12/11/2019 (epo:Fund) A unique identifier of the instance of the concept.

Additional Information

For example, in the case of the Procurement Identifier, this could be the European Public Procurement Identifier, and/or any other identifier provided by the buyer, the service provider or any other stakeholder.

WG Approval 12/11/2019 (epo:Item) A unique identifier of the instance of the concept.

Additional Information

For example, in the case of the Procurement Identifier, this could be the European Public Procurement Identifier, and/or any other identifier provided by the buyer, the service provider or any other stakeholder.

WG Approval 12/11/2019 (epo:Lot) A unique identifier of the instance of the concept.

Additional Information

For example, in the case of the Procurement Identifier, this could be the European Public Procurement Identifier, and/or any other identifier provided by the buyer, the service provider or any other stakeholder.

WG Approval 12/11/2019 (epo:LotGroup) A unique identifier of the instance of the concept.

Additional Information

For example, in the case of the Procurement Identifier, this could be the European Public Procurement Identifier, and/or any other identifier provided by the buyer, the service provider or any other stakeholder.

WG Approval 12/11/2019 (epo:Person) A unique identifier of the instance of the concept.

Additional Information

For example, in the case of the Procurement Identifier, this could be the European Public Procurement Identifier, and/or any other identifier provided by the buyer, the service provider or any other stakeholder.

WG Approval 12/11/2019
 (epo:PlannedProcurementPart) A unique identifier of the instance of the concept.

Additional Information

For example, in the case of the Procurement Identifier, this could be the European Public Procurement Identifier, and/or any other identifier provided by the buyer, the service provider or any other stakeholder.

WG Approval 12/11/2019 (epo:Procedure) A unique identifier of the instance of the concept.

Additional Information

For example, in the case of the Procurement Identifier, this could be the European Public Procurement Identifier, and/or any other identifier provided by the buyer, the service provider or any other stakeholder.

WG Approval 12/11/2019 (epo:ProcurementCriterion) A unique identifier of the instance of the concept.

Additional Information

For example, in the case of the Procurement Identifier, this could be the European Public Procurement Identifier, and/or any other identifier provided by the buyer, the service provider or any other stakeholder.

WG Approval 12/11/2019 (epo:ProjectProcurement) A unique identifier of the instance of the concept.

Additional Information

For example, in the case of the Procurement Identifier, this could be the European Public Procurement Identifier, and/or any other identifier provided by the buyer, the service provider or any other stakeholder.

WG Approval 12/11/2019 (epo:Technique) A unique identifier of the instance of the concept.

Additional Information

For example, in the case of the Procurement Identifier, this could be the European Public Procurement Identifier, and/or any other identifier provided by the buyer, the service provider or any other stakeholder.

WG Approval 12/11/2019
 (epo:Tender) A unique identifier of the instance of the concept.

Additional Information

For example, in the case of the Procurement Identifier, this could be the European Public Procurement Identifier, and/or any other identifier provided by the buyer, the service provider or any other stakeholder.

WG Approval 12/11/2019 (epo:TenderLot) </skos:definition>
      <rdfs:isDefinedBy rdf:resource="http://data.europa.eu/a4g/ontology"/>
   </owl:ObjectProperty>
   <owl:DatatypeProperty rdf:about="http://data.europa.eu/a4g/ontology#hasAwardCriterionType">
      <rdfs:label xml:lang="en">Has award criterion type</rdfs:label>
      <skos:prefLabel xml:lang="en">Has award criterion type</skos:prefLabel>
      <rdfs:comment xml:lang="en">Category of award criterion. (epo:AwardCriterion) </rdfs:comment>
      <skos:definition xml:lang="en">Category of award criterion. (epo:AwardCriterion) </skos:definition>
      <rdfs:isDefinedBy rdf:resource="http://data.europa.eu/a4g/ontology"/>
   </owl:DatatypeProperty>
   <owl:DatatypeProperty rdf:about="http://data.europa.eu/a4g/ontology#hasDescription">
      <rdfs:label xml:lang="en">Has description</rdfs:label>
      <skos:prefLabel xml:lang="en">Has description</skos:prefLabel>
      <rdfs:comment xml:lang="en">Explanatory text about the instance of the concept.

WG Approval 30/09/2019 (epo:AwardCriterion) Explanatory text about the instance of the concept.

WG Approval 30/09/2019 (epo:Change) Explanatory text about the instance of the concept.

WG Approval 30/09/2019 (epo:Channel) Explanatory text about the instance of the concept.

WG Approval 30/09/2019 (epo:ContactPoint) Explanatory text about the instance of the concept.

WG Approval 30/09/2019
 (epo:Item) Explanatory text about the instance of the concept.

WG Approval 30/09/2019
 (epo:Lot) Explanatory text about the instance of the concept.

WG Approval 30/09/2019
 (epo:LotGroup) Explanatory text about the instance of the concept.

WG Approval 30/09/2019 (epo:Period) Explanatory text about the instance of the concept.

WG Approval 30/09/2019 (epo:PlannedProcurementPart) Explanatory text about the instance of the concept.

WG Approval 30/09/2019 (epo:Procedure) Explanatory text about the instance of the concept.

WG Approval 30/09/2019 (epo:ProcurementCriterion) Explanatory text about the instance of the concept.

WG Approval 30/09/2019 (epo:ProcurementRole) Explanatory text about the instance of the concept.

WG Approval 30/09/2019
 (epo:ProjectProcurement) Explanatory text about the instance of the concept.

WG Approval 30/09/2019 (epo:ResourceElement) Explanatory text about the instance of the concept.

WG Approval 30/09/2019
 (epo:SecurityClearanceTerm) Explanatory text about the instance of the concept.

WG Approval 30/09/2019
 (epo:Subcontract) Explanatory text about the instance of the concept.

WG Approval 30/09/2019 (epo:SubcontractTerm) Explanatory text about the instance of the concept.

WG Approval 30/09/2019 (epo:System) Explanatory text about the instance of the concept.

WG Approval 30/09/2019 (epo:Technique) </rdfs:comment>
      <skos:definition xml:lang="en">Explanatory text about the instance of the concept.

WG Approval 30/09/2019 (epo:AwardCriterion) Explanatory text about the instance of the concept.

WG Approval 30/09/2019 (epo:Change) Explanatory text about the instance of the concept.

WG Approval 30/09/2019 (epo:Channel) Explanatory text about the instance of the concept.

WG Approval 30/09/2019 (epo:ContactPoint) Explanatory text about the instance of the concept.

WG Approval 30/09/2019
 (epo:Item) Explanatory text about the instance of the concept.

WG Approval 30/09/2019
 (epo:Lot) Explanatory text about the instance of the concept.

WG Approval 30/09/2019
 (epo:LotGroup) Explanatory text about the instance of the concept.

WG Approval 30/09/2019 (epo:Period) Explanatory text about the instance of the concept.

WG Approval 30/09/2019 (epo:PlannedProcurementPart) Explanatory text about the instance of the concept.

WG Approval 30/09/2019 (epo:Procedure) Explanatory text about the instance of the concept.

WG Approval 30/09/2019 (epo:ProcurementCriterion) Explanatory text about the instance of the concept.

WG Approval 30/09/2019 (epo:ProcurementRole) Explanatory text about the instance of the concept.

WG Approval 30/09/2019
 (epo:ProjectProcurement) Explanatory text about the instance of the concept.

WG Approval 30/09/2019 (epo:ResourceElement) Explanatory text about the instance of the concept.

WG Approval 30/09/2019
 (epo:SecurityClearanceTerm) Explanatory text about the instance of the concept.

WG Approval 30/09/2019
 (epo:Subcontract) Explanatory text about the instance of the concept.

WG Approval 30/09/2019 (epo:SubcontractTerm) Explanatory text about the instance of the concept.

WG Approval 30/09/2019 (epo:System) Explanatory text about the instance of the concept.

WG Approval 30/09/2019 (epo:Technique) </skos:definition>
      <rdfs:isDefinedBy rdf:resource="http://data.europa.eu/a4g/ontology"/>
   </owl:DatatypeProperty>
   <owl:DatatypeProperty rdf:about="http://data.europa.eu/a4g/ontology#hasFixedValue">
      <rdfs:label xml:lang="en">Has fixed value</rdfs:label>
      <skos:prefLabel xml:lang="en">Has fixed value</skos:prefLabel>
      <rdfs:comment xml:lang="en">No definition. Waiting on CCCEV alignment.
 (epo:AwardCriterion) </rdfs:comment>
      <skos:definition xml:lang="en">No definition. Waiting on CCCEV alignment.
 (epo:AwardCriterion) </skos:definition>
      <rdfs:isDefinedBy rdf:resource="http://data.europa.eu/a4g/ontology"/>
   </owl:DatatypeProperty>
   <owl:DatatypeProperty rdf:about="http://data.europa.eu/a4g/ontology#hasFixedValueType">
      <rdfs:label xml:lang="en">Has fixed value type</rdfs:label>
      <skos:prefLabel xml:lang="en">Has fixed value type</skos:prefLabel>
      <rdfs:comment xml:lang="en">The method to interpret the fixed value as pertaining to a total or unit.

WG Approval 17/09/2019 (epo:AwardCriterion) </rdfs:comment>
      <skos:definition xml:lang="en">The method to interpret the fixed value as pertaining to a total or unit.

WG Approval 17/09/2019 (epo:AwardCriterion) </skos:definition>
      <rdfs:isDefinedBy rdf:resource="http://data.europa.eu/a4g/ontology"/>
   </owl:DatatypeProperty>
   <owl:DatatypeProperty rdf:about="http://data.europa.eu/a4g/ontology#hasFormula">
      <rdfs:label xml:lang="en">Has formula</rdfs:label>
      <skos:prefLabel xml:lang="en">Has formula</skos:prefLabel>
      <rdfs:comment xml:lang="en">No definition. Waiting on CCCEV alignment.
 (epo:AwardCriterion) No definition. Waiting on CCCEV alignment. (epo:SelectionCriterion) </rdfs:comment>
      <skos:definition xml:lang="en">No definition. Waiting on CCCEV alignment.
 (epo:AwardCriterion) No definition. Waiting on CCCEV alignment. (epo:SelectionCriterion) </skos:definition>
      <rdfs:isDefinedBy rdf:resource="http://data.europa.eu/a4g/ontology"/>
   </owl:DatatypeProperty>
   <owl:DatatypeProperty rdf:about="http://data.europa.eu/a4g/ontology#hasThresholdType">
      <rdfs:label xml:lang="en">Has threshold type</rdfs:label>
      <skos:prefLabel xml:lang="en">Has threshold type</skos:prefLabel>
      <rdfs:comment xml:lang="en">The method to interpret the threshold value as minimum or a maximum.

WG Approval 17/09/2019  (epo:AwardCriterion) The type of threshold for a Selection Criterion.

Additional Information

For example, a minimum score or a maximum number of tenders with the highest score passing.
 (epo:SelectionCriterion) </rdfs:comment>
      <skos:definition xml:lang="en">The method to interpret the threshold value as minimum or a maximum.

WG Approval 17/09/2019  (epo:AwardCriterion) The type of threshold for a Selection Criterion.

Additional Information

For example, a minimum score or a maximum number of tenders with the highest score passing.
 (epo:SelectionCriterion) </skos:definition>
      <rdfs:isDefinedBy rdf:resource="http://data.europa.eu/a4g/ontology"/>
   </owl:DatatypeProperty>
   <owl:DatatypeProperty rdf:about="http://data.europa.eu/a4g/ontology#hasThresholdValue">
      <rdfs:label xml:lang="en">Has threshold value</rdfs:label>
      <skos:prefLabel xml:lang="en">Has threshold value</skos:prefLabel>
      <rdfs:comment xml:lang="en">No definition. Waiting on CCCEV alignment. (epo:AwardCriterion) To be reviewed when treating criterion (epo:SelectionCriterion) </rdfs:comment>
      <skos:definition xml:lang="en">No definition. Waiting on CCCEV alignment. (epo:AwardCriterion) To be reviewed when treating criterion (epo:SelectionCriterion) </skos:definition>
      <rdfs:isDefinedBy rdf:resource="http://data.europa.eu/a4g/ontology"/>
   </owl:DatatypeProperty>
   <owl:DatatypeProperty rdf:about="http://data.europa.eu/a4g/ontology#hasWeightValue">
      <rdfs:label xml:lang="en">Has weight value</rdfs:label>
      <skos:prefLabel xml:lang="en">Has weight value</skos:prefLabel>
      <rdfs:comment xml:lang="en">No definition. Waiting on CCCEV alignment.
 (epo:AwardCriterion) No definition. Waiting on CCCEV alignment. (epo:SelectionCriterion) </rdfs:comment>
      <skos:definition xml:lang="en">No definition. Waiting on CCCEV alignment.
 (epo:AwardCriterion) No definition. Waiting on CCCEV alignment. (epo:SelectionCriterion) </skos:definition>
      <rdfs:isDefinedBy rdf:resource="http://data.europa.eu/a4g/ontology"/>
   </owl:DatatypeProperty>
   <owl:DatatypeProperty rdf:about="http://data.europa.eu/a4g/ontology#hasWeightValueType">
      <rdfs:label xml:lang="en">Has weight value type</rdfs:label>
      <skos:prefLabel xml:lang="en">Has weight value type</skos:prefLabel>
      <rdfs:comment xml:lang="en">No definition. Waiting on CCCEV alignment.
 (epo:AwardCriterion) No definition. Waiting on CCCEV alignment. (epo:SelectionCriterion) </rdfs:comment>
      <skos:definition xml:lang="en">No definition. Waiting on CCCEV alignment.
 (epo:AwardCriterion) No definition. Waiting on CCCEV alignment. (epo:SelectionCriterion) </skos:definition>
      <rdfs:isDefinedBy rdf:resource="http://data.europa.eu/a4g/ontology"/>
   </owl:DatatypeProperty>
   <owl:DatatypeProperty rdf:about="http://data.europa.eu/a4g/ontology#hasWeigthingJustification">
      <rdfs:label xml:lang="en">Has weigthing justification</rdfs:label>
      <skos:prefLabel xml:lang="en">Has weigthing justification</skos:prefLabel>
      <rdfs:comment xml:lang="en">No definition. Waiting on CCCEV alignment.
 (epo:AwardCriterion) </rdfs:comment>
      <skos:definition xml:lang="en">No definition. Waiting on CCCEV alignment.
 (epo:AwardCriterion) </skos:definition>
      <rdfs:isDefinedBy rdf:resource="http://data.europa.eu/a4g/ontology"/>
   </owl:DatatypeProperty>
   <owl:DatatypeProperty rdf:about="http://data.europa.eu/a4g/ontology#hasAwardDecisionDate">
      <rdfs:label xml:lang="en">Has award decision date</rdfs:label>
      <skos:prefLabel xml:lang="en">Has award decision date</skos:prefLabel>
      <rdfs:comment xml:lang="en">The official date of the award decision.

WG Approval 09/01/2020 (epo:AwardDecision) </rdfs:comment>
      <skos:definition xml:lang="en">The official date of the award decision.

WG Approval 09/01/2020 (epo:AwardDecision) </skos:definition>
      <rdfs:isDefinedBy rdf:resource="http://data.europa.eu/a4g/ontology"/>
   </owl:DatatypeProperty>
   <owl:DatatypeProperty rdf:about="http://data.europa.eu/a4g/ontology#hasAwardStatus">
      <rdfs:label xml:lang="en">Has award status</rdfs:label>
      <skos:prefLabel xml:lang="en">Has award status</skos:prefLabel>
      <rdfs:comment xml:lang="en">Indicates whether the lot is awarded, not awarded or still open.

 
WG Approval 03/12/2019 (epo:AwardDecision) </rdfs:comment>
      <skos:definition xml:lang="en">Indicates whether the lot is awarded, not awarded or still open.

 
WG Approval 03/12/2019 (epo:AwardDecision) </skos:definition>
      <rdfs:isDefinedBy rdf:resource="http://data.europa.eu/a4g/ontology"/>
   </owl:DatatypeProperty>
   <owl:DatatypeProperty rdf:about="http://data.europa.eu/a4g/ontology#hasJustification">
      <rdfs:label xml:lang="en">Has justification</rdfs:label>
      <skos:prefLabel xml:lang="en">Has justification</skos:prefLabel>
      <rdfs:comment xml:lang="en">An explanation about the reasons for using the concept. 
WG Approval 5/11/2019
 (epo:AwardDecision) An explanation about the reasons for using the concept. 
WG Approval 5/11/2019
 (epo:DirectAwardTerm) </rdfs:comment>
      <skos:definition xml:lang="en">An explanation about the reasons for using the concept. 
WG Approval 5/11/2019
 (epo:AwardDecision) An explanation about the reasons for using the concept. 
WG Approval 5/11/2019
 (epo:DirectAwardTerm) </skos:definition>
      <rdfs:isDefinedBy rdf:resource="http://data.europa.eu/a4g/ontology"/>
   </owl:DatatypeProperty>
   <owl:DatatypeProperty rdf:about="http://data.europa.eu/a4g/ontology#hasNonAwardJustification">
      <rdfs:label xml:lang="en">Has non award justification</rdfs:label>
      <skos:prefLabel xml:lang="en">Has non award justification</skos:prefLabel>
      <rdfs:comment xml:lang="en">On hold; Enumeration. (epo:AwardDecision) </rdfs:comment>
      <skos:definition xml:lang="en">On hold; Enumeration. (epo:AwardDecision) </skos:definition>
      <rdfs:isDefinedBy rdf:resource="http://data.europa.eu/a4g/ontology"/>
   </owl:DatatypeProperty>
   <owl:DatatypeProperty rdf:about="http://data.europa.eu/a4g/ontology#hasListedCompany">
      <rdfs:label xml:lang="en">Has listed company</rdfs:label>
      <skos:prefLabel xml:lang="en">Has listed company</skos:prefLabel>
      <rdfs:comment xml:lang="en">Public companies listed on a stock exchange and subject to disclosure requirements (either by stock exchange
 rules or through law or enforceable means), which impose requirements to ensure adequate transparency of 
beneficial ownership. 

&lt;u&gt;Additional Information:&lt;/u&gt;

In eForms this indicator is used when the nationality of beneficial owner is not provided because the Economic Operator is registered in a regulated market that is subject to disclosure requirements consistent with Union law or subject to equivalent international standards which ensure adequate transparency of ownership information. 

WG Approval 21/11/2019 (epo:Business) </rdfs:comment>
      <skos:definition xml:lang="en">Public companies listed on a stock exchange and subject to disclosure requirements (either by stock exchange
 rules or through law or enforceable means), which impose requirements to ensure adequate transparency of 
beneficial ownership. 

&lt;u&gt;Additional Information:&lt;/u&gt;

In eForms this indicator is used when the nationality of beneficial owner is not provided because the Economic Operator is registered in a regulated market that is subject to disclosure requirements consistent with Union law or subject to equivalent international standards which ensure adequate transparency of ownership information. 

WG Approval 21/11/2019 (epo:Business) </skos:definition>
      <rdfs:isDefinedBy rdf:resource="http://data.europa.eu/a4g/ontology"/>
   </owl:DatatypeProperty>
   <owl:DatatypeProperty rdf:about="http://data.europa.eu/a4g/ontology#hasSize">
      <rdfs:label xml:lang="en">Has size</rdfs:label>
      <skos:prefLabel xml:lang="en">Has size</skos:prefLabel>
      <rdfs:comment xml:lang="en">The category of the business depending on number of employees and turnover.

Additional information:

See Commission Recommendation of 6 May 2003 concerning the definition of micro, small and medium-sized enterprises.

ELI: http://data.europa.eu/eli/reco/2003/361/oj

WG Approval 28/05/2020 (epo:Business) </rdfs:comment>
      <skos:definition xml:lang="en">The category of the business depending on number of employees and turnover.

Additional information:

See Commission Recommendation of 6 May 2003 concerning the definition of micro, small and medium-sized enterprises.

ELI: http://data.europa.eu/eli/reco/2003/361/oj

WG Approval 28/05/2020 (epo:Business) </skos:definition>
      <rdfs:isDefinedBy rdf:resource="http://data.europa.eu/a4g/ontology"/>
   </owl:DatatypeProperty>
   <owl:DatatypeProperty rdf:about="http://data.europa.eu/a4g/ontology#hasActivityDescription">
      <rdfs:label xml:lang="en">Has activity description</rdfs:label>
      <skos:prefLabel xml:lang="en">Has activity description</skos:prefLabel>
      <rdfs:comment xml:lang="en">In the ePO ontology a taxonomy with all activities, based on different classifications (COFOG, UTILITIES, NACE), will be provided. In ePO this field is to be used exclusively to complement the definition attached to the MainActivityCode.

However, in eForms there is the code "other" to cover undefined activities. For mapping to this eForms feature one could also use this property.
 (epo:Buyer) </rdfs:comment>
      <skos:definition xml:lang="en">In the ePO ontology a taxonomy with all activities, based on different classifications (COFOG, UTILITIES, NACE), will be provided. In ePO this field is to be used exclusively to complement the definition attached to the MainActivityCode.

However, in eForms there is the code "other" to cover undefined activities. For mapping to this eForms feature one could also use this property.
 (epo:Buyer) </skos:definition>
      <rdfs:isDefinedBy rdf:resource="http://data.europa.eu/a4g/ontology"/>
   </owl:DatatypeProperty>
   <owl:DatatypeProperty rdf:about="http://data.europa.eu/a4g/ontology#hasBuyerType">
      <rdfs:label xml:lang="en">Has buyer type</rdfs:label>
      <skos:prefLabel xml:lang="en">Has buyer type</skos:prefLabel>
      <rdfs:comment xml:lang="en">A category that indicates the right of an organisation to play the role of a buyer.
Additional Information:
The category also effects the rules that the buyer has to abide to within the public procurement procedure.
WG 07/09/2021 (epo:Buyer) </rdfs:comment>
      <skos:definition xml:lang="en">A category that indicates the right of an organisation to play the role of a buyer.
Additional Information:
The category also effects the rules that the buyer has to abide to within the public procurement procedure.
WG 07/09/2021 (epo:Buyer) </skos:definition>
      <rdfs:isDefinedBy rdf:resource="http://data.europa.eu/a4g/ontology"/>
   </owl:DatatypeProperty>
   <owl:DatatypeProperty rdf:about="http://data.europa.eu/a4g/ontology#hasBuyerTypeDescription">
      <rdfs:label xml:lang="en">Has buyer type description</rdfs:label>
      <skos:prefLabel xml:lang="en">Has buyer type description</skos:prefLabel>
      <rdfs:comment xml:lang="en">Self-explanatory text about the BuyerType.
WG 07/09/2021
 (epo:Buyer) </rdfs:comment>
      <skos:definition xml:lang="en">Self-explanatory text about the BuyerType.
WG 07/09/2021
 (epo:Buyer) </skos:definition>
      <rdfs:isDefinedBy rdf:resource="http://data.europa.eu/a4g/ontology"/>
   </owl:DatatypeProperty>
   <owl:DatatypeProperty rdf:about="http://data.europa.eu/a4g/ontology#hasContractingEntity">
      <rdfs:label xml:lang="en">Has contracting entity</rdfs:label>
      <skos:prefLabel xml:lang="en">Has contracting entity</skos:prefLabel>
      <rdfs:comment xml:lang="en">Role of entities, which:

(a) are contracting authorities or public undertakings and which pursue one of the activities referred to in Articles 8 to 14 of the Directive 2014/25/EU.

(b) when they are not contracting authorities or public undertakings, have as one of their activities any of the activities referred to in Articles 8 to 14, or any combination thereof and operate on the basis of special or exclusive rights granted by a competent authority of a Member State.

Additional Information

The indicator is needed in order to discriminate between those contracts where the Contracting Entity acts as a Contracting Authority undergoing the limits and the rules of Directive 24 and those where it acts as a  Contracting Entity, with certain relaxed constraints.
For example, the Contracting Entities have different thresholds for the application of Directive 24 if compared with Contracting Authorities.

WG Approval 28/04/2020
 (epo:Buyer) </rdfs:comment>
      <skos:definition xml:lang="en">Role of entities, which:

(a) are contracting authorities or public undertakings and which pursue one of the activities referred to in Articles 8 to 14 of the Directive 2014/25/EU.

(b) when they are not contracting authorities or public undertakings, have as one of their activities any of the activities referred to in Articles 8 to 14, or any combination thereof and operate on the basis of special or exclusive rights granted by a competent authority of a Member State.

Additional Information

The indicator is needed in order to discriminate between those contracts where the Contracting Entity acts as a Contracting Authority undergoing the limits and the rules of Directive 24 and those where it acts as a  Contracting Entity, with certain relaxed constraints.
For example, the Contracting Entities have different thresholds for the application of Directive 24 if compared with Contracting Authorities.

WG Approval 28/04/2020
 (epo:Buyer) </skos:definition>
      <rdfs:isDefinedBy rdf:resource="http://data.europa.eu/a4g/ontology"/>
   </owl:DatatypeProperty>
   <owl:DatatypeProperty rdf:about="http://data.europa.eu/a4g/ontology#hasMainActivityType">
      <rdfs:label xml:lang="en">Has main activity type</rdfs:label>
      <skos:prefLabel xml:lang="en">Has main activity type</skos:prefLabel>
      <rdfs:comment xml:lang="en">The principal sectoral area in which an organisation operates.

Additional information

The activities associated with buyers are derived from the top level of the Classification of the functions of the government (COFOG) from the United Nations Statistics Division.

The activities associated with buyer are derived from sectors explicitly falling within the sectoral directive (2014/25/EU Art. 8 - Art. 14).

WG Approval 05/05/2020 (epo:Buyer) </rdfs:comment>
      <skos:definition xml:lang="en">The principal sectoral area in which an organisation operates.

Additional information

The activities associated with buyers are derived from the top level of the Classification of the functions of the government (COFOG) from the United Nations Statistics Division.

The activities associated with buyer are derived from sectors explicitly falling within the sectoral directive (2014/25/EU Art. 8 - Art. 14).

WG Approval 05/05/2020 (epo:Buyer) </skos:definition>
      <rdfs:isDefinedBy rdf:resource="http://data.europa.eu/a4g/ontology"/>
   </owl:DatatypeProperty>
   <owl:DatatypeProperty rdf:about="http://data.europa.eu/a4g/ontology#hasURL">
      <rdfs:label xml:lang="en">Has u r l</rdfs:label>
      <skos:prefLabel xml:lang="en">Has u r l</skos:prefLabel>
      <rdfs:comment xml:lang="en">The identifier of a resource.

Additional Information

For example:

1. The URL of the system from where to access the procurement documents;
2. The URL of the system for the submission of tender documents;
3. The URL of the system from where to download a tool to communicate with the Buyer;
4. The URL of the system used by a Technique to allow Economic Operators to exchange information with the Buyer (e.g. eAuction and DPS Systems)
5. The URL of the system used to exchange information between Buyer and EO for questions and clarifications;

WG Approval 30/09/2019


 (epo:BuyerProfile) The identifier of a resource.

Additional Information

For example:

1. The URL of the system from where to access the procurement documents;
2. The URL of the system for the submission of tender documents;
3. The URL of the system from where to download a tool to communicate with the Buyer;
4. The URL of the system used by a Technique to allow Economic Operators to exchange information with the Buyer (e.g. eAuction and DPS Systems)
5. The URL of the system used to exchange information between Buyer and EO for questions and clarifications;

WG Approval 30/09/2019

 (epo:Channel) The identifier of a resource.

Additional Information

For example:

1. The URL of the system from where to access the procurement documents;
2. The URL of the system for the submission of tender documents;
3. The URL of the system from where to download a tool to communicate with the Buyer;
4. The URL of the system used by a Technique to allow Economic Operators to exchange information with the Buyer (e.g. eAuction and DPS Systems)
5. The URL of the system used to exchange information between Buyer and EO for questions and clarifications;

WG Approval 30/09/2019 (epo:Fund) </rdfs:comment>
      <skos:definition xml:lang="en">The identifier of a resource.

Additional Information

For example:

1. The URL of the system from where to access the procurement documents;
2. The URL of the system for the submission of tender documents;
3. The URL of the system from where to download a tool to communicate with the Buyer;
4. The URL of the system used by a Technique to allow Economic Operators to exchange information with the Buyer (e.g. eAuction and DPS Systems)
5. The URL of the system used to exchange information between Buyer and EO for questions and clarifications;

WG Approval 30/09/2019


 (epo:BuyerProfile) The identifier of a resource.

Additional Information

For example:

1. The URL of the system from where to access the procurement documents;
2. The URL of the system for the submission of tender documents;
3. The URL of the system from where to download a tool to communicate with the Buyer;
4. The URL of the system used by a Technique to allow Economic Operators to exchange information with the Buyer (e.g. eAuction and DPS Systems)
5. The URL of the system used to exchange information between Buyer and EO for questions and clarifications;

WG Approval 30/09/2019

 (epo:Channel) The identifier of a resource.

Additional Information

For example:

1. The URL of the system from where to access the procurement documents;
2. The URL of the system for the submission of tender documents;
3. The URL of the system from where to download a tool to communicate with the Buyer;
4. The URL of the system used by a Technique to allow Economic Operators to exchange information with the Buyer (e.g. eAuction and DPS Systems)
5. The URL of the system used to exchange information between Buyer and EO for questions and clarifications;

WG Approval 30/09/2019 (epo:Fund) </skos:definition>
      <rdfs:isDefinedBy rdf:resource="http://data.europa.eu/a4g/ontology"/>
   </owl:DatatypeProperty>
   <owl:DatatypeProperty rdf:about="http://data.europa.eu/a4g/ontology#hasChangeReason">
      <rdfs:label xml:lang="en">Has change reason</rdfs:label>
      <skos:prefLabel xml:lang="en">Has change reason</skos:prefLabel>
      <rdfs:comment xml:lang="en">The motives for the change.

WG 5/11/2019 (epo:Change) </rdfs:comment>
      <skos:definition xml:lang="en">The motives for the change.

WG 5/11/2019 (epo:Change) </skos:definition>
      <rdfs:isDefinedBy rdf:resource="http://data.europa.eu/a4g/ontology"/>
   </owl:DatatypeProperty>
   <owl:DatatypeProperty rdf:about="http://data.europa.eu/a4g/ontology#hasDateTime">
      <rdfs:label xml:lang="en">Has date time</rdfs:label>
      <skos:prefLabel xml:lang="en">Has date time</skos:prefLabel>
      <rdfs:comment xml:lang="en">The date and time of the change

WG Approval 5/11/2019
 (epo:Change) </rdfs:comment>
      <skos:definition xml:lang="en">The date and time of the change

WG Approval 5/11/2019
 (epo:Change) </skos:definition>
      <rdfs:isDefinedBy rdf:resource="http://data.europa.eu/a4g/ontology"/>
   </owl:DatatypeProperty>
   <owl:DatatypeProperty rdf:about="http://data.europa.eu/a4g/ontology#hasProcurementDocumentChanged">
      <rdfs:label xml:lang="en">Has procurement document changed</rdfs:label>
      <skos:prefLabel xml:lang="en">Has procurement document changed</skos:prefLabel>
      <rdfs:comment xml:lang="en">One or more procurement documents have been changed.

WG Approval 05/11/2019 (epo:Change) </rdfs:comment>
      <skos:definition xml:lang="en">One or more procurement documents have been changed.

WG Approval 05/11/2019 (epo:Change) </skos:definition>
      <rdfs:isDefinedBy rdf:resource="http://data.europa.eu/a4g/ontology"/>
   </owl:DatatypeProperty>
   <owl:DatatypeProperty rdf:about="http://data.europa.eu/a4g/ontology#hasReason">
      <rdfs:label xml:lang="en">Has reason</rdfs:label>
      <skos:prefLabel xml:lang="en">Has reason</skos:prefLabel>
      <rdfs:comment xml:lang="en">Code explaining the change.

WG Approval 5/11/2019 (epo:Change) </rdfs:comment>
      <skos:definition xml:lang="en">Code explaining the change.

WG Approval 5/11/2019 (epo:Change) </skos:definition>
      <rdfs:isDefinedBy rdf:resource="http://data.europa.eu/a4g/ontology"/>
   </owl:DatatypeProperty>
   <owl:DatatypeProperty rdf:about="http://data.europa.eu/a4g/ontology#hasAdditionalInformation">
      <rdfs:label xml:lang="en">Has additional information</rdfs:label>
      <skos:prefLabel xml:lang="en">Has additional information</skos:prefLabel>
      <rdfs:comment xml:lang="en">Supplementary data about the instance of the concept.

Additional Information

For example, information about the Lot not specified elsewhere in the Notice.

WG Approval 15/10/2019
 (epo:Channel) Supplementary data about the instance of the concept.

Additional Information

For example, information about the Lot not specified elsewhere in the Notice.

WG Approval 15/10/2019 (epo:Lot) Supplementary data about the instance of the concept.

Additional Information

For example, information about the Lot not specified elsewhere in the Notice.

WG Approval 15/10/2019

 (epo:PlannedProcurementPart) </rdfs:comment>
      <skos:definition xml:lang="en">Supplementary data about the instance of the concept.

Additional Information

For example, information about the Lot not specified elsewhere in the Notice.

WG Approval 15/10/2019
 (epo:Channel) Supplementary data about the instance of the concept.

Additional Information

For example, information about the Lot not specified elsewhere in the Notice.

WG Approval 15/10/2019 (epo:Lot) Supplementary data about the instance of the concept.

Additional Information

For example, information about the Lot not specified elsewhere in the Notice.

WG Approval 15/10/2019

 (epo:PlannedProcurementPart) </skos:definition>
      <rdfs:isDefinedBy rdf:resource="http://data.europa.eu/a4g/ontology"/>
   </owl:DatatypeProperty>
   <owl:DatatypeProperty rdf:about="http://data.europa.eu/a4g/ontology#hasEndpoint">
      <rdfs:label xml:lang="en">Has endpoint</rdfs:label>
      <skos:prefLabel xml:lang="en">Has endpoint</skos:prefLabel>
      <rdfs:comment xml:lang="en">The value identifying a communication network node, required to gain access to a service.

Additional information

Examples:
https://data.gov.es/sdg?serviceId=diploma-request
mailto:myname@mycompany.com
+33 6090 92 81 80 Ext. 3213

WG Approval 07/05/2020 (epo:Channel) </rdfs:comment>
      <skos:definition xml:lang="en">The value identifying a communication network node, required to gain access to a service.

Additional information

Examples:
https://data.gov.es/sdg?serviceId=diploma-request
mailto:myname@mycompany.com
+33 6090 92 81 80 Ext. 3213

WG Approval 07/05/2020 (epo:Channel) </skos:definition>
      <rdfs:isDefinedBy rdf:resource="http://data.europa.eu/a4g/ontology"/>
   </owl:DatatypeProperty>
   <owl:DatatypeProperty rdf:about="http://data.europa.eu/a4g/ontology#hasName">
      <rdfs:label xml:lang="en">Has name</rdfs:label>
      <skos:prefLabel xml:lang="en">Has name</skos:prefLabel>
      <rdfs:comment xml:lang="en">A short text by which a thing is known or referred to.

WG Approval 16/11/2021 (epo:Channel) A short text by which a thing is known or referred to.

WG Approval 16/11/2021 (epo:Fund) A short text by which a thing is known or referred to.

WG Approval 16/11/2021 (epo:Item) A short text by which a thing is known or referred to. 

WG Approval 16/11/2021 (epo:Organisation) A short text by which a thing is known or referred to.

WG Approval 16/11/2021 (epo:ProcurementCriterion) A short text by which a thing is known or referred to.

WG Approval 16/11/2021 (epo:System) </rdfs:comment>
      <skos:definition xml:lang="en">A short text by which a thing is known or referred to.

WG Approval 16/11/2021 (epo:Channel) A short text by which a thing is known or referred to.

WG Approval 16/11/2021 (epo:Fund) A short text by which a thing is known or referred to.

WG Approval 16/11/2021 (epo:Item) A short text by which a thing is known or referred to. 

WG Approval 16/11/2021 (epo:Organisation) A short text by which a thing is known or referred to.

WG Approval 16/11/2021 (epo:ProcurementCriterion) A short text by which a thing is known or referred to.

WG Approval 16/11/2021 (epo:System) </skos:definition>
      <rdfs:isDefinedBy rdf:resource="http://data.europa.eu/a4g/ontology"/>
   </owl:DatatypeProperty>
   <owl:DatatypeProperty rdf:about="http://data.europa.eu/a4g/ontology#hasEmail">
      <rdfs:label xml:lang="en">Has email</rdfs:label>
      <skos:prefLabel xml:lang="en">Has email</skos:prefLabel>
      <rdfs:comment xml:lang="en">The eMail address used to reach a person or an organisation. (epo:ContactPoint) </rdfs:comment>
      <skos:definition xml:lang="en">The eMail address used to reach a person or an organisation. (epo:ContactPoint) </skos:definition>
      <rdfs:isDefinedBy rdf:resource="http://data.europa.eu/a4g/ontology"/>
   </owl:DatatypeProperty>
   <owl:DatatypeProperty rdf:about="http://data.europa.eu/a4g/ontology#hasFax">
      <rdfs:label xml:lang="en">Has fax</rdfs:label>
      <skos:prefLabel xml:lang="en">Has fax</skos:prefLabel>
      <rdfs:comment xml:lang="en">The fax number used to reach a person or an organisation. (epo:ContactPoint) </rdfs:comment>
      <skos:definition xml:lang="en">The fax number used to reach a person or an organisation. (epo:ContactPoint) </skos:definition>
      <rdfs:isDefinedBy rdf:resource="http://data.europa.eu/a4g/ontology"/>
   </owl:DatatypeProperty>
   <owl:DatatypeProperty rdf:about="http://data.europa.eu/a4g/ontology#hasInternetAddress">
      <rdfs:label xml:lang="en">Has internet address</rdfs:label>
      <skos:prefLabel xml:lang="en">Has internet address</skos:prefLabel>
      <rdfs:comment xml:lang="en">The website of the organisation.
 (epo:ContactPoint) </rdfs:comment>
      <skos:definition xml:lang="en">The website of the organisation.
 (epo:ContactPoint) </skos:definition>
      <rdfs:isDefinedBy rdf:resource="http://data.europa.eu/a4g/ontology"/>
   </owl:DatatypeProperty>
   <owl:DatatypeProperty rdf:about="http://data.europa.eu/a4g/ontology#hasTelephone">
      <rdfs:label xml:lang="en">Has telephone</rdfs:label>
      <skos:prefLabel xml:lang="en">Has telephone</skos:prefLabel>
      <rdfs:comment xml:lang="en">The telephone number used to reach a person or an organisation.
 (epo:ContactPoint) </rdfs:comment>
      <skos:definition xml:lang="en">The telephone number used to reach a person or an organisation.
 (epo:ContactPoint) </skos:definition>
      <rdfs:isDefinedBy rdf:resource="http://data.europa.eu/a4g/ontology"/>
   </owl:DatatypeProperty>
   <owl:DatatypeProperty rdf:about="http://data.europa.eu/a4g/ontology#hasContractConclusionDate">
      <rdfs:label xml:lang="en">Has contract conclusion date</rdfs:label>
      <skos:prefLabel xml:lang="en">Has contract conclusion date</skos:prefLabel>
      <rdfs:comment xml:lang="en">The date the contract was signed by the last signatory party.

&lt;u&gt;Additional Information:&lt;/u&gt;
In exceptional cases contracts may be concluded without signature and therefore another date may be used. The date of contract conclusion is always later than the end of any standstill period.
This concept is not to be confused with the date of completion/end of the contract.

WG Approval 09/01/2020 (epo:Contract) </rdfs:comment>
      <skos:definition xml:lang="en">The date the contract was signed by the last signatory party.

&lt;u&gt;Additional Information:&lt;/u&gt;
In exceptional cases contracts may be concluded without signature and therefore another date may be used. The date of contract conclusion is always later than the end of any standstill period.
This concept is not to be confused with the date of completion/end of the contract.

WG Approval 09/01/2020 (epo:Contract) </skos:definition>
      <rdfs:isDefinedBy rdf:resource="http://data.europa.eu/a4g/ontology"/>
   </owl:DatatypeProperty>
   <owl:DatatypeProperty rdf:about="http://data.europa.eu/a4g/ontology#hasEntryintoForceDate">
      <rdfs:label xml:lang="en">Has entryinto force date</rdfs:label>
      <skos:prefLabel xml:lang="en">Has entryinto force date</skos:prefLabel>
      <rdfs:comment xml:lang="en">The date on which the contract enters into force.

Additional information: 

This is generally the date on which the fulfillment of the contract begins.

WG approval 05/11/2019 (epo:Contract) </rdfs:comment>
      <skos:definition xml:lang="en">The date on which the contract enters into force.

Additional information: 

This is generally the date on which the fulfillment of the contract begins.

WG approval 05/11/2019 (epo:Contract) </skos:definition>
      <rdfs:isDefinedBy rdf:resource="http://data.europa.eu/a4g/ontology"/>
   </owl:DatatypeProperty>
   <owl:DatatypeProperty rdf:about="http://data.europa.eu/a4g/ontology#hasTitle">
      <rdfs:label xml:lang="en">Has title</rdfs:label>
      <skos:prefLabel xml:lang="en">Has title</skos:prefLabel>
      <rdfs:comment xml:lang="en">A short self-descriptive name of the instance of the concept.

Additional Information:

For example, the title of a planned part that may become a procedure or a lot in the future; the title of a contract, etc.

(WG Approval 11-11-2019)
 (epo:Contract) A short self-descriptive name of the instance of the concept.

Additional Information:

For example, the title of a planned part that may become a procedure or a lot in the future; the title of a contract, etc.

(WG Approval 11-11-2019)
 (epo:Lot) A short self-descriptive name of the instance of the concept.

Additional Information:

For example, the title of a planned part that may become a procedure or a lot in the future; the title of a contract, etc.

(WG Approval 11-11-2019)
 (epo:LotGroup) A short self-descriptive name of the instance of the concept.

Additional Information:

For example, the title of a planned part that may become a procedure or a lot in the future; the title of a contract, etc.

(WG Approval 11-11-2019)
 (epo:PlannedProcurementPart) A short self-descriptive name of the instance of the concept.

Additional Information:

For example, the title of a planned part that may become a procedure or a lot in the future; the title of a contract, etc.

(WG Approval 11-11-2019) (epo:Procedure) A short self-descriptive name of the instance of the concept.

Additional Information:

For example, the title of a planned part that may become a procedure or a lot in the future; the title of a contract, etc.

(WG Approval 11-11-2019)
 (epo:ProcurementRole) A short self-descriptive name of the instance of the concept.

Additional Information:

For example, the title of a planned part that may become a procedure or a lot in the future; the title of a contract, etc.

(WG Approval 11-11-2019)
 (epo:ProjectProcurement) </rdfs:comment>
      <skos:definition xml:lang="en">A short self-descriptive name of the instance of the concept.

Additional Information:

For example, the title of a planned part that may become a procedure or a lot in the future; the title of a contract, etc.

(WG Approval 11-11-2019)
 (epo:Contract) A short self-descriptive name of the instance of the concept.

Additional Information:

For example, the title of a planned part that may become a procedure or a lot in the future; the title of a contract, etc.

(WG Approval 11-11-2019)
 (epo:Lot) A short self-descriptive name of the instance of the concept.

Additional Information:

For example, the title of a planned part that may become a procedure or a lot in the future; the title of a contract, etc.

(WG Approval 11-11-2019)
 (epo:LotGroup) A short self-descriptive name of the instance of the concept.

Additional Information:

For example, the title of a planned part that may become a procedure or a lot in the future; the title of a contract, etc.

(WG Approval 11-11-2019)
 (epo:PlannedProcurementPart) A short self-descriptive name of the instance of the concept.

Additional Information:

For example, the title of a planned part that may become a procedure or a lot in the future; the title of a contract, etc.

(WG Approval 11-11-2019) (epo:Procedure) A short self-descriptive name of the instance of the concept.

Additional Information:

For example, the title of a planned part that may become a procedure or a lot in the future; the title of a contract, etc.

(WG Approval 11-11-2019)
 (epo:ProcurementRole) A short self-descriptive name of the instance of the concept.

Additional Information:

For example, the title of a planned part that may become a procedure or a lot in the future; the title of a contract, etc.

(WG Approval 11-11-2019)
 (epo:ProjectProcurement) </skos:definition>
      <rdfs:isDefinedBy rdf:resource="http://data.europa.eu/a4g/ontology"/>
   </owl:DatatypeProperty>
   <owl:DatatypeProperty rdf:about="http://data.europa.eu/a4g/ontology#hasDescriptionOfTheModification">
      <rdfs:label xml:lang="en">Has description of the modification</rdfs:label>
      <skos:prefLabel xml:lang="en">Has description of the modification</skos:prefLabel>
      <rdfs:comment xml:lang="en">An explanatory text about this context. 

 WG Approval 5/11/2019 (epo:ContractModificationNotice) </rdfs:comment>
      <skos:definition xml:lang="en">An explanatory text about this context. 

 WG Approval 5/11/2019 (epo:ContractModificationNotice) </skos:definition>
      <rdfs:isDefinedBy rdf:resource="http://data.europa.eu/a4g/ontology"/>
   </owl:DatatypeProperty>
   <owl:DatatypeProperty rdf:about="http://data.europa.eu/a4g/ontology#hasJustificationOfTheModification">
      <rdfs:label xml:lang="en">Has justification of the modification</rdfs:label>
      <skos:prefLabel xml:lang="en">Has justification of the modification</skos:prefLabel>
      <rdfs:comment xml:lang="en">An explanation about the reasons for using the concept. 

WG Approval 5/11/2019 (epo:ContractModificationNotice) </rdfs:comment>
      <skos:definition xml:lang="en">An explanation about the reasons for using the concept. 

WG Approval 5/11/2019 (epo:ContractModificationNotice) </skos:definition>
      <rdfs:isDefinedBy rdf:resource="http://data.europa.eu/a4g/ontology"/>
   </owl:DatatypeProperty>
   <owl:DatatypeProperty rdf:about="http://data.europa.eu/a4g/ontology#hasModificationReason">
      <rdfs:label xml:lang="en">Has modification reason</rdfs:label>
      <skos:prefLabel xml:lang="en">Has modification reason</skos:prefLabel>
      <rdfs:comment xml:lang="en">Explanation of why a contract was modified.
WG Approval 09/11/2021 (epo:ContractModificationNotice) </rdfs:comment>
      <skos:definition xml:lang="en">Explanation of why a contract was modified.
WG Approval 09/11/2021 (epo:ContractModificationNotice) </skos:definition>
      <rdfs:isDefinedBy rdf:resource="http://data.europa.eu/a4g/ontology"/>
   </owl:DatatypeProperty>
   <owl:DatatypeProperty rdf:about="http://data.europa.eu/a4g/ontology#hasRecurrence">
      <rdfs:label xml:lang="en">Has recurrence</rdfs:label>
      <skos:prefLabel xml:lang="en">Has recurrence</skos:prefLabel>
      <rdfs:comment xml:lang="en">The Procurement being notified is likely to be included in another procedure in the foreseeable future.

Additional Information:

For example, a regularly re-tendered municipal service. This does not include awarding multiple contracts within a single qualification system, framework agreement, or a dynamic purchasing system.

WG Approval 12/05/2020 (epo:ContractNotice) </rdfs:comment>
      <skos:definition xml:lang="en">The Procurement being notified is likely to be included in another procedure in the foreseeable future.

Additional Information:

For example, a regularly re-tendered municipal service. This does not include awarding multiple contracts within a single qualification system, framework agreement, or a dynamic purchasing system.

WG Approval 12/05/2020 (epo:ContractNotice) </skos:definition>
      <rdfs:isDefinedBy rdf:resource="http://data.europa.eu/a4g/ontology"/>
   </owl:DatatypeProperty>
   <owl:DatatypeProperty rdf:about="http://data.europa.eu/a4g/ontology#hasRecurrenceDescription">
      <rdfs:label xml:lang="en">Has recurrence description</rdfs:label>
      <skos:prefLabel xml:lang="en">Has recurrence description</skos:prefLabel>
      <rdfs:comment xml:lang="en">Any additional information about the recurrence of the Procurement.
 
Additional Information:
For example estimated timing of the Procedure.


(WG approval 2019-01-16) (epo:ContractNotice) </rdfs:comment>
      <skos:definition xml:lang="en">Any additional information about the recurrence of the Procurement.
 
Additional Information:
For example estimated timing of the Procedure.


(WG approval 2019-01-16) (epo:ContractNotice) </skos:definition>
      <rdfs:isDefinedBy rdf:resource="http://data.europa.eu/a4g/ontology"/>
   </owl:DatatypeProperty>
   <owl:DatatypeProperty rdf:about="http://data.europa.eu/a4g/ontology#hasBroadPlaceOfPerformance">
      <rdfs:label xml:lang="en">Has broad place of performance</rdfs:label>
      <skos:prefLabel xml:lang="en">Has broad place of performance</skos:prefLabel>
      <rdfs:comment xml:lang="en">Geopolitical zone where the contract can be executed.

Additional Information

Used for setting restrictions that cannot be established with one country code or a geographical zone identifier (like NUTS), because they have a broader scope (geographical, economic, political, other). (epo:ContractTerm) </rdfs:comment>
      <skos:definition xml:lang="en">Geopolitical zone where the contract can be executed.

Additional Information

Used for setting restrictions that cannot be established with one country code or a geographical zone identifier (like NUTS), because they have a broader scope (geographical, economic, political, other). (epo:ContractTerm) </skos:definition>
      <rdfs:isDefinedBy rdf:resource="http://data.europa.eu/a4g/ontology"/>
   </owl:DatatypeProperty>
   <owl:DatatypeProperty rdf:about="http://data.europa.eu/a4g/ontology#hasContractorLegalFormRequirement">
      <rdfs:label xml:lang="en">Has contractor legal form requirement</rdfs:label>
      <skos:prefLabel xml:lang="en">Has contractor legal form requirement</skos:prefLabel>
      <rdfs:comment xml:lang="en">A specific legal entity must be taken up by a tenderer composed of a group of economic operators once it has been awarded a contract.

Additional information: this may be applied in the case of groups (e.g. a consortium) where the requirement is that they have to formalise the relationship of the group members as a legal entity itself once the contract is awarded.

WG Approval 2019-01-29
 (epo:ContractTerm) </rdfs:comment>
      <skos:definition xml:lang="en">A specific legal entity must be taken up by a tenderer composed of a group of economic operators once it has been awarded a contract.

Additional information: this may be applied in the case of groups (e.g. a consortium) where the requirement is that they have to formalise the relationship of the group members as a legal entity itself once the contract is awarded.

WG Approval 2019-01-29
 (epo:ContractTerm) </skos:definition>
      <rdfs:isDefinedBy rdf:resource="http://data.europa.eu/a4g/ontology"/>
   </owl:DatatypeProperty>
   <owl:DatatypeProperty rdf:about="http://data.europa.eu/a4g/ontology#hasContractorLegalFormRequirementDescription">
      <rdfs:label xml:lang="en">Has contractor legal form requirement description</rdfs:label>
      <skos:prefLabel xml:lang="en">Has contractor legal form requirement description</skos:prefLabel>
      <rdfs:comment xml:lang="en">A constraint concerning the legal form that must be adopted by a tenderer composed of a group of economic operators once it has been awarded a contract. (epo:ContractTerm) </rdfs:comment>
      <skos:definition xml:lang="en">A constraint concerning the legal form that must be adopted by a tenderer composed of a group of economic operators once it has been awarded a contract. (epo:ContractTerm) </skos:definition>
      <rdfs:isDefinedBy rdf:resource="http://data.europa.eu/a4g/ontology"/>
   </owl:DatatypeProperty>
   <owl:DatatypeProperty rdf:about="http://data.europa.eu/a4g/ontology#hasEInvoicing">
      <rdfs:label xml:lang="en">Has e invoicing</rdfs:label>
      <skos:prefLabel xml:lang="en">Has e invoicing</skos:prefLabel>
      <rdfs:comment xml:lang="en">Electronic means will be used for invoicing in the post-award process.

WG Approval 12/09/2019
 (epo:ContractTerm) </rdfs:comment>
      <skos:definition xml:lang="en">Electronic means will be used for invoicing in the post-award process.

WG Approval 12/09/2019
 (epo:ContractTerm) </skos:definition>
      <rdfs:isDefinedBy rdf:resource="http://data.europa.eu/a4g/ontology"/>
   </owl:DatatypeProperty>
   <owl:DatatypeProperty rdf:about="http://data.europa.eu/a4g/ontology#hasEOrdering">
      <rdfs:label xml:lang="en">Has e ordering</rdfs:label>
      <skos:prefLabel xml:lang="en">Has e ordering</skos:prefLabel>
      <rdfs:comment xml:lang="en">Electronic means will be used for requesting and purchasing in the post-award process.

WG Approval 12/09/2019

 (epo:ContractTerm) </rdfs:comment>
      <skos:definition xml:lang="en">Electronic means will be used for requesting and purchasing in the post-award process.

WG Approval 12/09/2019

 (epo:ContractTerm) </skos:definition>
      <rdfs:isDefinedBy rdf:resource="http://data.europa.eu/a4g/ontology"/>
   </owl:DatatypeProperty>
   <owl:DatatypeProperty rdf:about="http://data.europa.eu/a4g/ontology#hasEPayment">
      <rdfs:label xml:lang="en">Has e payment</rdfs:label>
      <skos:prefLabel xml:lang="en">Has e payment</skos:prefLabel>
      <rdfs:comment xml:lang="en">Electronic means must be used for paying.
WG Approval 09/11/2021
 (epo:ContractTerm) </rdfs:comment>
      <skos:definition xml:lang="en">Electronic means must be used for paying.
WG Approval 09/11/2021
 (epo:ContractTerm) </skos:definition>
      <rdfs:isDefinedBy rdf:resource="http://data.europa.eu/a4g/ontology"/>
   </owl:DatatypeProperty>
   <owl:DatatypeProperty rdf:about="http://data.europa.eu/a4g/ontology#hasMaximumNumberOfRenewals">
      <rdfs:label xml:lang="en">Has maximum number of renewals</rdfs:label>
      <skos:prefLabel xml:lang="en">Has maximum number of renewals</skos:prefLabel>
      <rdfs:comment xml:lang="en">The maximum number of times the contract can be renewed. 

Additional Information

By renewing, the buyer reserves the right (i.e. not an obligation) to renew the contract (i.e. extend its duration) without a new procurement procedure. 
For example, a contract may be valid for one year and the buyer may keep a possibility to renew it (e.g. once, twice) for another three months, if he is content with the services he received.

PLEASE REVIEW THIS DEFINITION AGAIN WITH THE WORKING GROUP. It was originally taken from eForms.
 (epo:ContractTerm) </rdfs:comment>
      <skos:definition xml:lang="en">The maximum number of times the contract can be renewed. 

Additional Information

By renewing, the buyer reserves the right (i.e. not an obligation) to renew the contract (i.e. extend its duration) without a new procurement procedure. 
For example, a contract may be valid for one year and the buyer may keep a possibility to renew it (e.g. once, twice) for another three months, if he is content with the services he received.

PLEASE REVIEW THIS DEFINITION AGAIN WITH THE WORKING GROUP. It was originally taken from eForms.
 (epo:ContractTerm) </skos:definition>
      <rdfs:isDefinedBy rdf:resource="http://data.europa.eu/a4g/ontology"/>
   </owl:DatatypeProperty>
   <owl:DatatypeProperty rdf:about="http://data.europa.eu/a4g/ontology#hasPaymentArrangement">
      <rdfs:label xml:lang="en">Has payment arrangement</rdfs:label>
      <skos:prefLabel xml:lang="en">Has payment arrangement</skos:prefLabel>
      <rdfs:comment xml:lang="en">Information about financial clauses that will govern some economic aspects of the execution of the contract.

Additional Information: These clauses usually refer to financial and payment provisions.

This type of information should be structured instead of a free text in order to reuse it an ideal world. Unfortunately this is an information that in the real life no one is willing to provide pro-actively.

WG Pending of discussion with eForms (epo:ContractTerm) </rdfs:comment>
      <skos:definition xml:lang="en">Information about financial clauses that will govern some economic aspects of the execution of the contract.

Additional Information: These clauses usually refer to financial and payment provisions.

This type of information should be structured instead of a free text in order to reuse it an ideal world. Unfortunately this is an information that in the real life no one is willing to provide pro-actively.

WG Pending of discussion with eForms (epo:ContractTerm) </skos:definition>
      <rdfs:isDefinedBy rdf:resource="http://data.europa.eu/a4g/ontology"/>
   </owl:DatatypeProperty>
   <owl:DatatypeProperty rdf:about="http://data.europa.eu/a4g/ontology#hasPerformanceConditions">
      <rdfs:label xml:lang="en">Has performance conditions</rdfs:label>
      <skos:prefLabel xml:lang="en">Has performance conditions</skos:prefLabel>
      <rdfs:comment xml:lang="en">The particular conditions and additional information related to the execution of the contract.

Additional Information: 

For example, specific information about the place of performance, intermediary deliverables, compensation for damages, intellectual property rights.

WG approval 15-01-2019 (epo:ContractTerm) </rdfs:comment>
      <skos:definition xml:lang="en">The particular conditions and additional information related to the execution of the contract.

Additional Information: 

For example, specific information about the place of performance, intermediary deliverables, compensation for damages, intellectual property rights.

WG approval 15-01-2019 (epo:ContractTerm) </skos:definition>
      <rdfs:isDefinedBy rdf:resource="http://data.europa.eu/a4g/ontology"/>
   </owl:DatatypeProperty>
   <owl:DatatypeProperty rdf:about="http://data.europa.eu/a4g/ontology#hasPlaceOfPerformanceAdditionalInformation">
      <rdfs:label xml:lang="en">Has place of performance additional information</rdfs:label>
      <skos:prefLabel xml:lang="en">Has place of performance additional information</skos:prefLabel>
      <rdfs:comment xml:lang="en">Further details on the location of the execution of the contract.

WG Approval 30/07/2019 (epo:ContractTerm) </rdfs:comment>
      <skos:definition xml:lang="en">Further details on the location of the execution of the contract.

WG Approval 30/07/2019 (epo:ContractTerm) </skos:definition>
      <rdfs:isDefinedBy rdf:resource="http://data.europa.eu/a4g/ontology"/>
   </owl:DatatypeProperty>
   <owl:DatatypeProperty rdf:about="http://data.europa.eu/a4g/ontology#hasRenewalDescription">
      <rdfs:label xml:lang="en">Has renewal description</rdfs:label>
      <skos:prefLabel xml:lang="en">Has renewal description</skos:prefLabel>
      <rdfs:comment xml:lang="en">Any other information about the renewal(s).

WG approval 16/04/2019  (epo:ContractTerm) </rdfs:comment>
      <skos:definition xml:lang="en">Any other information about the renewal(s).

WG approval 16/04/2019  (epo:ContractTerm) </skos:definition>
      <rdfs:isDefinedBy rdf:resource="http://data.europa.eu/a4g/ontology"/>
   </owl:DatatypeProperty>
   <owl:DatatypeProperty rdf:about="http://data.europa.eu/a4g/ontology#hasRenewalIndicator">
      <rdfs:label xml:lang="en">Has renewal indicator</rdfs:label>
      <skos:prefLabel xml:lang="en">Has renewal indicator</skos:prefLabel>
      <rdfs:comment xml:lang="en">Indicates whether the contract is subject to a renewal clause.
WG Approval 09/11/2021 (epo:ContractTerm) </rdfs:comment>
      <skos:definition xml:lang="en">Indicates whether the contract is subject to a renewal clause.
WG Approval 09/11/2021 (epo:ContractTerm) </skos:definition>
      <rdfs:isDefinedBy rdf:resource="http://data.europa.eu/a4g/ontology"/>
   </owl:DatatypeProperty>
   <owl:DatatypeProperty rdf:about="http://data.europa.eu/a4g/ontology#hasReservedExecution">
      <rdfs:label xml:lang="en">Has reserved execution</rdfs:label>
      <skos:prefLabel xml:lang="en">Has reserved execution</skos:prefLabel>
      <rdfs:comment xml:lang="en">&lt;foreign otherprops="#24292e"&gt;The execution of the contract is restricted to the framework of sheltered employment programmes&lt;/foreign&gt;.

WG Approval 12/09/2019




 (epo:ContractTerm) </rdfs:comment>
      <skos:definition xml:lang="en">&lt;foreign otherprops="#24292e"&gt;The execution of the contract is restricted to the framework of sheltered employment programmes&lt;/foreign&gt;.

WG Approval 12/09/2019




 (epo:ContractTerm) </skos:definition>
      <rdfs:isDefinedBy rdf:resource="http://data.europa.eu/a4g/ontology"/>
   </owl:DatatypeProperty>
   <owl:DatatypeProperty rdf:about="http://data.europa.eu/a4g/ontology#hasFollowupContract">
      <rdfs:label xml:lang="en">Has followup contract</rdfs:label>
      <skos:prefLabel xml:lang="en">Has followup contract</skos:prefLabel>
      <rdfs:comment xml:lang="en">Any subsequent service contract will be awarded to the winner or, in the case of a design contest, winners.

WG Approval 29/08/2019  (epo:DesignContestRegimeTerm) </rdfs:comment>
      <skos:definition xml:lang="en">Any subsequent service contract will be awarded to the winner or, in the case of a design contest, winners.

WG Approval 29/08/2019  (epo:DesignContestRegimeTerm) </skos:definition>
      <rdfs:isDefinedBy rdf:resource="http://data.europa.eu/a4g/ontology"/>
   </owl:DatatypeProperty>
   <owl:DatatypeProperty rdf:about="http://data.europa.eu/a4g/ontology#hasFollowupContractInformation">
      <rdfs:label xml:lang="en">Has followup contract information</rdfs:label>
      <skos:prefLabel xml:lang="en">Has followup contract information</skos:prefLabel>
      <rdfs:comment xml:lang="en">Further information about follow-up contracts, prizes and payments (for example non-monetary prizes, payments given for participation).

WG Approval 03/09/2019 (epo:DesignContestRegimeTerm) </rdfs:comment>
      <skos:definition xml:lang="en">Further information about follow-up contracts, prizes and payments (for example non-monetary prizes, payments given for participation).

WG Approval 03/09/2019 (epo:DesignContestRegimeTerm) </skos:definition>
      <rdfs:isDefinedBy rdf:resource="http://data.europa.eu/a4g/ontology"/>
   </owl:DatatypeProperty>
   <owl:DatatypeProperty rdf:about="http://data.europa.eu/a4g/ontology#hasJuryDecisionBinding">
      <rdfs:label xml:lang="en">Has jury decision binding</rdfs:label>
      <skos:prefLabel xml:lang="en">Has jury decision binding</skos:prefLabel>
      <rdfs:comment xml:lang="en">Indicates whether the procuring entity is bound to apply the decision of the jury. (epo:DesignContestRegimeTerm) </rdfs:comment>
      <skos:definition xml:lang="en">Indicates whether the procuring entity is bound to apply the decision of the jury. (epo:DesignContestRegimeTerm) </skos:definition>
      <rdfs:isDefinedBy rdf:resource="http://data.europa.eu/a4g/ontology"/>
   </owl:DatatypeProperty>
   <owl:DatatypeProperty rdf:about="http://data.europa.eu/a4g/ontology#hasParticipationPayment">
      <rdfs:label xml:lang="en">Has participation payment</rdfs:label>
      <skos:prefLabel xml:lang="en">Has participation payment</skos:prefLabel>
      <rdfs:comment xml:lang="en">Details on payments to participants 
WG Approval 09/11/2021 (epo:DesignContestRegimeTerm) </rdfs:comment>
      <skos:definition xml:lang="en">Details on payments to participants 
WG Approval 09/11/2021 (epo:DesignContestRegimeTerm) </skos:definition>
      <rdfs:isDefinedBy rdf:resource="http://data.europa.eu/a4g/ontology"/>
   </owl:DatatypeProperty>
   <owl:DatatypeProperty rdf:about="http://data.europa.eu/a4g/ontology#hasJustificationType">
      <rdfs:label xml:lang="en">Has justification type</rdfs:label>
      <skos:prefLabel xml:lang="en">Has justification type</skos:prefLabel>
      <rdfs:comment xml:lang="en">List of reasons for using a procedure which allows awarding contracts directly without publishing a notice. 

WG Approval 28/05/2020 (epo:DirectAwardTerm) </rdfs:comment>
      <skos:definition xml:lang="en">List of reasons for using a procedure which allows awarding contracts directly without publishing a notice. 

WG Approval 28/05/2020 (epo:DirectAwardTerm) </skos:definition>
      <rdfs:isDefinedBy rdf:resource="http://data.europa.eu/a4g/ontology"/>
   </owl:DatatypeProperty>
   <owl:DatatypeProperty rdf:about="http://data.europa.eu/a4g/ontology#hasDispatchDate">
      <rdfs:label xml:lang="en">Has dispatch date</rdfs:label>
      <skos:prefLabel xml:lang="en">Has dispatch date</skos:prefLabel>
      <rdfs:comment xml:lang="en">Date of transmission of a record to an organisation.

WG Approval 12/05/2020 (epo:Document) </rdfs:comment>
      <skos:definition xml:lang="en">Date of transmission of a record to an organisation.

WG Approval 12/05/2020 (epo:Document) </skos:definition>
      <rdfs:isDefinedBy rdf:resource="http://data.europa.eu/a4g/ontology"/>
   </owl:DatatypeProperty>
   <owl:DatatypeProperty rdf:about="http://data.europa.eu/a4g/ontology#hasOfficialLanguage">
      <rdfs:label xml:lang="en">Has official language</rdfs:label>
      <skos:prefLabel xml:lang="en">Has official language</skos:prefLabel>
      <rdfs:comment xml:lang="en">The language(s) in which the instances of the given concepts are officially available. These linguistic versions are equally legally valid.

WG Approval 03/10/2019 (epo:Document) </rdfs:comment>
      <skos:definition xml:lang="en">The language(s) in which the instances of the given concepts are officially available. These linguistic versions are equally legally valid.

WG Approval 03/10/2019 (epo:Document) </skos:definition>
      <rdfs:isDefinedBy rdf:resource="http://data.europa.eu/a4g/ontology"/>
   </owl:DatatypeProperty>
   <owl:DatatypeProperty rdf:about="http://data.europa.eu/a4g/ontology#hasReceptionDate">
      <rdfs:label xml:lang="en">Has reception date</rdfs:label>
      <skos:prefLabel xml:lang="en">Has reception date</skos:prefLabel>
      <rdfs:comment xml:lang="en">Notes: Date when a record is acknowledged by an organisation.

WG Approval 12/05/2020 (epo:Document) </rdfs:comment>
      <skos:definition xml:lang="en">Notes: Date when a record is acknowledged by an organisation.

WG Approval 12/05/2020 (epo:Document) </skos:definition>
      <rdfs:isDefinedBy rdf:resource="http://data.europa.eu/a4g/ontology"/>
   </owl:DatatypeProperty>
   <owl:DatatypeProperty rdf:about="http://data.europa.eu/a4g/ontology#hasRestrictedCommunicationJustification">
      <rdfs:label xml:lang="en">Has restricted communication justification</rdfs:label>
      <skos:prefLabel xml:lang="en">Has restricted communication justification</skos:prefLabel>
      <rdfs:comment xml:lang="en">Explanation of why the means of communication have been restricted.
WG Approval 09/11/2021 (epo:Document) </rdfs:comment>
      <skos:definition xml:lang="en">Explanation of why the means of communication have been restricted.
WG Approval 09/11/2021 (epo:Document) </skos:definition>
      <rdfs:isDefinedBy rdf:resource="http://data.europa.eu/a4g/ontology"/>
   </owl:DatatypeProperty>
   <owl:DatatypeProperty rdf:about="http://data.europa.eu/a4g/ontology#hasUnofficialLanguage">
      <rdfs:label xml:lang="en">Has unofficial language</rdfs:label>
      <skos:prefLabel xml:lang="en">Has unofficial language</skos:prefLabel>
      <rdfs:comment xml:lang="en">The language(s) in which the instances of the given concepts are also available in the following languages. These versions are not an official translation, they are provided only for information.

WG Approval 03/10/2019 (epo:Document) </rdfs:comment>
      <skos:definition xml:lang="en">The language(s) in which the instances of the given concepts are also available in the following languages. These versions are not an official translation, they are provided only for information.

WG Approval 03/10/2019 (epo:Document) </skos:definition>
      <rdfs:isDefinedBy rdf:resource="http://data.europa.eu/a4g/ontology"/>
   </owl:DatatypeProperty>
   <owl:ObjectProperty rdf:about="http://data.europa.eu/a4g/ontology#hasUUID">
      <rdfs:label xml:lang="en">Has u u i d</rdfs:label>
      <skos:prefLabel xml:lang="en">Has u u i d</skos:prefLabel>
      <rdfs:comment xml:lang="en">A universally unique identifier for an instance of this document.

WG Approval 12/05/2020 (epo:Document) </rdfs:comment>
      <skos:definition xml:lang="en">A universally unique identifier for an instance of this document.

WG Approval 12/05/2020 (epo:Document) </skos:definition>
      <rdfs:isDefinedBy rdf:resource="http://data.europa.eu/a4g/ontology"/>
   </owl:ObjectProperty>
   <owl:DatatypeProperty rdf:about="http://data.europa.eu/a4g/ontology#hasDPSTermination">
      <rdfs:label xml:lang="en">Has d p s termination</rdfs:label>
      <skos:prefLabel xml:lang="en">Has d p s termination</skos:prefLabel>
      <rdfs:comment xml:lang="en">End of the Dynamic Purchase System (DPS). 

Additional Information: This property can be used in the contract award notice even if no contracts are awarded . 

WG Approval 22/11/2019 (epo:DynamicPurchaseSystemTechnique) </rdfs:comment>
      <skos:definition xml:lang="en">End of the Dynamic Purchase System (DPS). 

Additional Information: This property can be used in the contract award notice even if no contracts are awarded . 

WG Approval 22/11/2019 (epo:DynamicPurchaseSystemTechnique) </skos:definition>
      <rdfs:isDefinedBy rdf:resource="http://data.europa.eu/a4g/ontology"/>
   </owl:DatatypeProperty>
   <owl:DatatypeProperty rdf:about="http://data.europa.eu/a4g/ontology#hasEAuctionUsage">
      <rdfs:label xml:lang="en">Has e auction usage</rdfs:label>
      <skos:prefLabel xml:lang="en">Has e auction usage</skos:prefLabel>
      <rdfs:comment xml:lang="en">Explanation as to whether an eAuction Technique is to be used.
WG Approval 09/11/2021 (epo:EAuctionTechnique) </rdfs:comment>
      <skos:definition xml:lang="en">Explanation as to whether an eAuction Technique is to be used.
WG Approval 09/11/2021 (epo:EAuctionTechnique) </skos:definition>
      <rdfs:isDefinedBy rdf:resource="http://data.europa.eu/a4g/ontology"/>
   </owl:DatatypeProperty>
   <owl:DatatypeProperty rdf:about="http://data.europa.eu/a4g/ontology#hasEORoleType">
      <rdfs:label xml:lang="en">Has e o role type</rdfs:label>
      <skos:prefLabel xml:lang="en">Has e o role type</skos:prefLabel>
      <rdfs:comment xml:lang="en">The role of an economic operator in the tendering process.
WG Approval 09/11/2021 (epo:EconomicOperator) </rdfs:comment>
      <skos:definition xml:lang="en">The role of an economic operator in the tendering process.
WG Approval 09/11/2021 (epo:EconomicOperator) </skos:definition>
      <rdfs:isDefinedBy rdf:resource="http://data.europa.eu/a4g/ontology"/>
   </owl:DatatypeProperty>
   <owl:DatatypeProperty rdf:about="http://data.europa.eu/a4g/ontology#hasEvaluationGroupType">
      <rdfs:label xml:lang="en">Has evaluation group type</rdfs:label>
      <skos:prefLabel xml:lang="en">Has evaluation group type</skos:prefLabel>
      <rdfs:comment xml:lang="en">The collective form taken to evaluate tenders.
WG Approval 09/11/2021 (epo:EvaluationBoard) </rdfs:comment>
      <skos:definition xml:lang="en">The collective form taken to evaluate tenders.
WG Approval 09/11/2021 (epo:EvaluationBoard) </skos:definition>
      <rdfs:isDefinedBy rdf:resource="http://data.europa.eu/a4g/ontology"/>
   </owl:DatatypeProperty>
   <owl:DatatypeProperty rdf:about="http://data.europa.eu/a4g/ontology#hasAwardCriteriaEvaluationFormula">
      <rdfs:label xml:lang="en">Has award criteria evaluation formula</rdfs:label>
      <skos:prefLabel xml:lang="en">Has award criteria evaluation formula</skos:prefLabel>
      <rdfs:comment xml:lang="en">Based on the Award Dimension Type code list

Let's say we have 5 different quality award criteria

QUALITY

1st - e.g. please describe how you'll make this machine (WEIGHT 20%)
2nd - describe the workflow used to manufacture the machine (WEIGHT 25%)
3rd - describe the materials used for each component of the machine (WEIGHT 10%)
4th - describe the quality control measures (WEIGHT 5%)
5th - describe how the manufacturing dead-lines (WEIGHT 40%)

PRICE CRITERIA
(list of criteria related to price)

COST CRITERIA
(list of criteria related to cost)

Overall award criteria Weight 20% Price, 60% Quality, 20% Cost (epo:EvaluationTerm) </rdfs:comment>
      <skos:definition xml:lang="en">Based on the Award Dimension Type code list

Let's say we have 5 different quality award criteria

QUALITY

1st - e.g. please describe how you'll make this machine (WEIGHT 20%)
2nd - describe the workflow used to manufacture the machine (WEIGHT 25%)
3rd - describe the materials used for each component of the machine (WEIGHT 10%)
4th - describe the quality control measures (WEIGHT 5%)
5th - describe how the manufacturing dead-lines (WEIGHT 40%)

PRICE CRITERIA
(list of criteria related to price)

COST CRITERIA
(list of criteria related to cost)

Overall award criteria Weight 20% Price, 60% Quality, 20% Cost (epo:EvaluationTerm) </skos:definition>
      <rdfs:isDefinedBy rdf:resource="http://data.europa.eu/a4g/ontology"/>
   </owl:DatatypeProperty>
   <owl:DatatypeProperty rdf:about="http://data.europa.eu/a4g/ontology#hasOverallCostAwardCriteriaPonderation">
      <rdfs:label xml:lang="en">Has overall cost award criteria ponderation</rdfs:label>
      <skos:prefLabel xml:lang="en">Has overall cost award criteria ponderation</skos:prefLabel>
      <rdfs:comment xml:lang="en">This needs to be reviewed with the AwardCriterion and the AwardDimension (epo:EvaluationTerm) </rdfs:comment>
      <skos:definition xml:lang="en">This needs to be reviewed with the AwardCriterion and the AwardDimension (epo:EvaluationTerm) </skos:definition>
      <rdfs:isDefinedBy rdf:resource="http://data.europa.eu/a4g/ontology"/>
   </owl:DatatypeProperty>
   <owl:DatatypeProperty rdf:about="http://data.europa.eu/a4g/ontology#hasOverallPriceAwardCriteriaPonderation">
      <rdfs:label xml:lang="en">Has overall price award criteria ponderation</rdfs:label>
      <skos:prefLabel xml:lang="en">Has overall price award criteria ponderation</skos:prefLabel>
      <rdfs:comment xml:lang="en">This needs to be reviewed with the AwardCriterion and the AwardDimension (epo:EvaluationTerm) </rdfs:comment>
      <skos:definition xml:lang="en">This needs to be reviewed with the AwardCriterion and the AwardDimension (epo:EvaluationTerm) </skos:definition>
      <rdfs:isDefinedBy rdf:resource="http://data.europa.eu/a4g/ontology"/>
   </owl:DatatypeProperty>
   <owl:DatatypeProperty rdf:about="http://data.europa.eu/a4g/ontology#hasOverallQualityAwardCriteriaPonderation">
      <rdfs:label xml:lang="en">Has overall quality award criteria ponderation</rdfs:label>
      <skos:prefLabel xml:lang="en">Has overall quality award criteria ponderation</skos:prefLabel>
      <rdfs:comment xml:lang="en">This needs to be reviewed with the AwardCriterion and the AwardDimension (epo:EvaluationTerm) </rdfs:comment>
      <skos:definition xml:lang="en">This needs to be reviewed with the AwardCriterion and the AwardDimension (epo:EvaluationTerm) </skos:definition>
      <rdfs:isDefinedBy rdf:resource="http://data.europa.eu/a4g/ontology"/>
   </owl:DatatypeProperty>
   <owl:DatatypeProperty rdf:about="http://data.europa.eu/a4g/ontology#hasPersonalSituationCondition">
      <rdfs:label xml:lang="en">Has personal situation condition</rdfs:label>
      <skos:prefLabel xml:lang="en">Has personal situation condition</skos:prefLabel>
      <rdfs:comment xml:lang="en">This condition is only used in the specific case of the Standard Form 17 (Defence), section III.2 Conditions for participation (epo:ExclusionGround) </rdfs:comment>
      <skos:definition xml:lang="en">This condition is only used in the specific case of the Standard Form 17 (Defence), section III.2 Conditions for participation (epo:ExclusionGround) </skos:definition>
      <rdfs:isDefinedBy rdf:resource="http://data.europa.eu/a4g/ontology"/>
   </owl:DatatypeProperty>
   <owl:DatatypeProperty rdf:about="http://data.europa.eu/a4g/ontology#hasBuyerCoverage">
      <rdfs:label xml:lang="en">Has buyer coverage</rdfs:label>
      <skos:prefLabel xml:lang="en">Has buyer coverage</skos:prefLabel>
      <rdfs:comment xml:lang="en">Buyers that can use the Framework Agreement not mentioned by name.

Additional Information: 
For example,  "all hospitals in the Tuscany region

WG Approval 2019-05-06 (epo:FrameworkAgreementTerm) </rdfs:comment>
      <skos:definition xml:lang="en">Buyers that can use the Framework Agreement not mentioned by name.

Additional Information: 
For example,  "all hospitals in the Tuscany region

WG Approval 2019-05-06 (epo:FrameworkAgreementTerm) </skos:definition>
      <rdfs:isDefinedBy rdf:resource="http://data.europa.eu/a4g/ontology"/>
   </owl:DatatypeProperty>
   <owl:DatatypeProperty rdf:about="http://data.europa.eu/a4g/ontology#hasDurationExtensionJustification">
      <rdfs:label xml:lang="en">Has duration extension justification</rdfs:label>
      <skos:prefLabel xml:lang="en">Has duration extension justification</skos:prefLabel>
      <rdfs:comment xml:lang="en">The justification for exceptional cases when the duration of the framework agreement exceeds the legal limits. 

Additional Information

Four years in the case of the general procurement Directive, seven years in the case of the defence Directive, and eight years in the case of the sectoral Directive.

WG Approval 26/09/2019 (epo:FrameworkAgreementTerm) </rdfs:comment>
      <skos:definition xml:lang="en">The justification for exceptional cases when the duration of the framework agreement exceeds the legal limits. 

Additional Information

Four years in the case of the general procurement Directive, seven years in the case of the defence Directive, and eight years in the case of the sectoral Directive.

WG Approval 26/09/2019 (epo:FrameworkAgreementTerm) </skos:definition>
      <rdfs:isDefinedBy rdf:resource="http://data.europa.eu/a4g/ontology"/>
   </owl:DatatypeProperty>
   <owl:DatatypeProperty rdf:about="http://data.europa.eu/a4g/ontology#hasFrameworkAgreementType">
      <rdfs:label xml:lang="en">Has framework agreement type</rdfs:label>
      <skos:prefLabel xml:lang="en">Has framework agreement type</skos:prefLabel>
      <rdfs:comment xml:lang="en">The form of framework agreement used in a procurement procedure.

Addition information:

A concept to distinguish the different types of framework agreement, which are: 
1. Framework agreement without reopening of competition,
2. Framework agreement with reopening of competition, or 
3. Framework agreement partly without reopening of competition.

WG Approval 19/09/2019 

 (epo:FrameworkAgreementTerm) </rdfs:comment>
      <skos:definition xml:lang="en">The form of framework agreement used in a procurement procedure.

Addition information:

A concept to distinguish the different types of framework agreement, which are: 
1. Framework agreement without reopening of competition,
2. Framework agreement with reopening of competition, or 
3. Framework agreement partly without reopening of competition.

WG Approval 19/09/2019 

 (epo:FrameworkAgreementTerm) </skos:definition>
      <rdfs:isDefinedBy rdf:resource="http://data.europa.eu/a4g/ontology"/>
   </owl:DatatypeProperty>
   <owl:ObjectProperty rdf:about="http://data.europa.eu/a4g/ontology#hasMaximumNumberOfAwardedTenderers">
      <rdfs:label xml:lang="en">Has maximum number of awarded tenderers</rdfs:label>
      <skos:prefLabel xml:lang="en">Has maximum number of awarded tenderers</skos:prefLabel>
      <rdfs:comment xml:lang="en">Maximum number of tenderers who may be awarded a contract within the framework agreement.

Additional Information: the number is a positive integer.

WG Approval 2019-02-05
 (epo:FrameworkAgreementTerm) </rdfs:comment>
      <skos:definition xml:lang="en">Maximum number of tenderers who may be awarded a contract within the framework agreement.

Additional Information: the number is a positive integer.

WG Approval 2019-02-05
 (epo:FrameworkAgreementTerm) </skos:definition>
      <rdfs:isDefinedBy rdf:resource="http://data.europa.eu/a4g/ontology"/>
   </owl:ObjectProperty>
   <owl:DatatypeProperty rdf:about="http://data.europa.eu/a4g/ontology#fulfillsRequirement">
      <rdfs:label xml:lang="en">Fulfills requirement</rdfs:label>
      <skos:prefLabel xml:lang="en">Fulfills requirement</skos:prefLabel>
      <rdfs:comment xml:lang="en">The requirement to which the concept meets.
WG Approval 09/11/2021 (epo:GreenProcurement) The requirement to which the concept meets.
WG Approval 09/11/2021
 (epo:InnovativeProcurement) The requirement to which the concept meets.
WG Approval 09/11/2021 (epo:SocialProcurement) </rdfs:comment>
      <skos:definition xml:lang="en">The requirement to which the concept meets.
WG Approval 09/11/2021 (epo:GreenProcurement) The requirement to which the concept meets.
WG Approval 09/11/2021
 (epo:InnovativeProcurement) The requirement to which the concept meets.
WG Approval 09/11/2021 (epo:SocialProcurement) </skos:definition>
      <rdfs:isDefinedBy rdf:resource="http://data.europa.eu/a4g/ontology"/>
   </owl:DatatypeProperty>
   <owl:DatatypeProperty rdf:about="http://data.europa.eu/a4g/ontology#hasCountryOfOrigin">
      <rdfs:label xml:lang="en">Has country of origin</rdfs:label>
      <skos:prefLabel xml:lang="en">Has country of origin</skos:prefLabel>
      <rdfs:comment xml:lang="en">The source country of the product or service.

&lt;u&gt;Additional Information:&lt;/u&gt;
&lt;u&gt;
&lt;/u&gt;The country of origin can be provided by  the buyer as a requirement or by the tenderer information of the item to be provided.

WG Approval 07/01/2020 (epo:Item) </rdfs:comment>
      <skos:definition xml:lang="en">The source country of the product or service.

&lt;u&gt;Additional Information:&lt;/u&gt;
&lt;u&gt;
&lt;/u&gt;The country of origin can be provided by  the buyer as a requirement or by the tenderer information of the item to be provided.

WG Approval 07/01/2020 (epo:Item) </skos:definition>
      <rdfs:isDefinedBy rdf:resource="http://data.europa.eu/a4g/ontology"/>
   </owl:DatatypeProperty>
   <owl:DatatypeProperty rdf:about="http://data.europa.eu/a4g/ontology#hasAwardDateScheduled">
      <rdfs:label xml:lang="en">Has award date scheduled</rdfs:label>
      <skos:prefLabel xml:lang="en">Has award date scheduled</skos:prefLabel>
      <rdfs:comment xml:lang="en">Planned date for the award decision.
WG Approval 09/11/2021 (epo:Lot) </rdfs:comment>
      <skos:definition xml:lang="en">Planned date for the award decision.
WG Approval 09/11/2021 (epo:Lot) </skos:definition>
      <rdfs:isDefinedBy rdf:resource="http://data.europa.eu/a4g/ontology"/>
   </owl:DatatypeProperty>
   <owl:DatatypeProperty rdf:about="http://data.europa.eu/a4g/ontology#hasEstimatedTenderInvitationDate">
      <rdfs:label xml:lang="en">Has estimated tender invitation date</rdfs:label>
      <skos:prefLabel xml:lang="en">Has estimated tender invitation date</skos:prefLabel>
      <rdfs:comment xml:lang="en">The planned date for the dispatch of the invitations to submit tenders.
WG Approval 09/11/2021 (epo:Lot) The planned date for the dispatch of the invitations to submit tenders.
WG Approval 09/11/2021 (epo:ProcedureTerm) </rdfs:comment>
      <skos:definition xml:lang="en">The planned date for the dispatch of the invitations to submit tenders.
WG Approval 09/11/2021 (epo:Lot) The planned date for the dispatch of the invitations to submit tenders.
WG Approval 09/11/2021 (epo:ProcedureTerm) </skos:definition>
      <rdfs:isDefinedBy rdf:resource="http://data.europa.eu/a4g/ontology"/>
   </owl:DatatypeProperty>
   <owl:DatatypeProperty rdf:about="http://data.europa.eu/a4g/ontology#hasGPAUsage">
      <rdfs:label xml:lang="en">Has g p a usage</rdfs:label>
      <skos:prefLabel xml:lang="en">Has g p a usage</skos:prefLabel>
      <rdfs:comment xml:lang="en">Specifies whether the Agreement on Government Procurement (GPA) applies.

Additional information: 
The GPA aims to establish a multilateral framework of balanced rights and obligations relating to public contracts with a view to achieving the liberalization and expansion of world trade.

WG Approval 15/10/2019

 (epo:Lot) </rdfs:comment>
      <skos:definition xml:lang="en">Specifies whether the Agreement on Government Procurement (GPA) applies.

Additional information: 
The GPA aims to establish a multilateral framework of balanced rights and obligations relating to public contracts with a view to achieving the liberalization and expansion of world trade.

WG Approval 15/10/2019

 (epo:Lot) </skos:definition>
      <rdfs:isDefinedBy rdf:resource="http://data.europa.eu/a4g/ontology"/>
   </owl:DatatypeProperty>
   <owl:DatatypeProperty rdf:about="http://data.europa.eu/a4g/ontology#hasPerformingStaffQualificationInformation">
      <rdfs:label xml:lang="en">Has performing staff qualification information</rdfs:label>
      <skos:prefLabel xml:lang="en">Has performing staff qualification information</skos:prefLabel>
      <rdfs:comment xml:lang="en">Explanation as to if and/or when information of the persons to carry out the contract is to be provided.
WG Approval 09/11/2021 (epo:Lot) </rdfs:comment>
      <skos:definition xml:lang="en">Explanation as to if and/or when information of the persons to carry out the contract is to be provided.
WG Approval 09/11/2021 (epo:Lot) </skos:definition>
      <rdfs:isDefinedBy rdf:resource="http://data.europa.eu/a4g/ontology"/>
   </owl:DatatypeProperty>
   <owl:DatatypeProperty rdf:about="http://data.europa.eu/a4g/ontology#hasReservedProcurement">
      <rdfs:label xml:lang="en">Has reserved procurement</rdfs:label>
      <skos:prefLabel xml:lang="en">Has reserved procurement</skos:prefLabel>
      <rdfs:comment xml:lang="en">Explanation as to whether a procurement may be reserved for the particpation of certain types of organisation.
WG Approval 09/11/2021 (epo:Lot) </rdfs:comment>
      <skos:definition xml:lang="en">Explanation as to whether a procurement may be reserved for the particpation of certain types of organisation.
WG Approval 09/11/2021 (epo:Lot) </skos:definition>
      <rdfs:isDefinedBy rdf:resource="http://data.europa.eu/a4g/ontology"/>
   </owl:DatatypeProperty>
   <owl:DatatypeProperty rdf:about="http://data.europa.eu/a4g/ontology#hasVariantPermission">
      <rdfs:label xml:lang="en">Has variant permission</rdfs:label>
      <skos:prefLabel xml:lang="en">Has variant permission</skos:prefLabel>
      <rdfs:comment xml:lang="en">The obligation or possibility for tenderers to submit variants or not.

Additional Information:

Variants are alternative ways to fulfil the buyer's needs as opposed to solutions indicated in the procurement documents.

eForms: Whether tenderers are required, allowed or forbidden to submit tenders which fulfil the buyer's needs differently than as proposed in the procurement documents. 

Additional Information:

Further conditions for submitting variant tenders are in the procurement documents.
 (epo:Lot) </rdfs:comment>
      <skos:definition xml:lang="en">The obligation or possibility for tenderers to submit variants or not.

Additional Information:

Variants are alternative ways to fulfil the buyer's needs as opposed to solutions indicated in the procurement documents.

eForms: Whether tenderers are required, allowed or forbidden to submit tenders which fulfil the buyer's needs differently than as proposed in the procurement documents. 

Additional Information:

Further conditions for submitting variant tenders are in the procurement documents.
 (epo:Lot) </skos:definition>
      <rdfs:isDefinedBy rdf:resource="http://data.europa.eu/a4g/ontology"/>
   </owl:DatatypeProperty>
   <owl:DatatypeProperty rdf:about="http://data.europa.eu/a4g/ontology#isSMESuitable">
      <rdfs:label xml:lang="en">Is s m e suitable</rdfs:label>
      <skos:prefLabel xml:lang="en">Is s m e suitable</skos:prefLabel>
      <rdfs:comment xml:lang="en">The Lot is suitable for small and medium enterprises (SMEs).

Additional Information

This allows the buyer to make emphasis on the fact that the procedure has been designed having SMEs in mind. This indicator is also to be reflected in the selection criteria.

For example, number of employees and turnover are applicable to the definition of an SME.

WG Approval 15/10/2019 (epo:Lot) The Lot is suitable for small and medium enterprises (SMEs).

Additional Information

This allows the buyer to make emphasis on the fact that the procedure has been designed having SMEs in mind. This indicator is also to be reflected in the selection criteria.

For example, number of employees and turnover are applicable to the definition of an SME.

WG Approval 15/10/2019
 (epo:PlannedProcurementPart) </rdfs:comment>
      <skos:definition xml:lang="en">The Lot is suitable for small and medium enterprises (SMEs).

Additional Information

This allows the buyer to make emphasis on the fact that the procedure has been designed having SMEs in mind. This indicator is also to be reflected in the selection criteria.

For example, number of employees and turnover are applicable to the definition of an SME.

WG Approval 15/10/2019 (epo:Lot) The Lot is suitable for small and medium enterprises (SMEs).

Additional Information

This allows the buyer to make emphasis on the fact that the procedure has been designed having SMEs in mind. This indicator is also to be reflected in the selection criteria.

For example, number of employees and turnover are applicable to the definition of an SME.

WG Approval 15/10/2019
 (epo:PlannedProcurementPart) </skos:definition>
      <rdfs:isDefinedBy rdf:resource="http://data.europa.eu/a4g/ontology"/>
   </owl:DatatypeProperty>
   <owl:DatatypeProperty rdf:about="http://data.europa.eu/a4g/ontology#hasEstimatedInvitationToExpressInterestDate">
      <rdfs:label xml:lang="en">Has estimated invitation to express interest date</rdfs:label>
      <skos:prefLabel xml:lang="en">Has estimated invitation to express interest date</skos:prefLabel>
      <rdfs:comment xml:lang="en">The estimated date of dispatch of the invitations to confirm interest.
 (epo:MultipleStageProcedureTerm) </rdfs:comment>
      <skos:definition xml:lang="en">The estimated date of dispatch of the invitations to confirm interest.
 (epo:MultipleStageProcedureTerm) </skos:definition>
      <rdfs:isDefinedBy rdf:resource="http://data.europa.eu/a4g/ontology"/>
   </owl:DatatypeProperty>
   <owl:DatatypeProperty rdf:about="http://data.europa.eu/a4g/ontology#hasEstimatedInvitationToTenderDate">
      <rdfs:label xml:lang="en">Has estimated invitation to tender date</rdfs:label>
      <skos:prefLabel xml:lang="en">Has estimated invitation to tender date</skos:prefLabel>
      <rdfs:comment xml:lang="en">The estimated date of dispatch of the invitations to submit tenders in two (or more) stage procedures.

WG Approval 01/10/2019 (epo:MultipleStageProcedureTerm) </rdfs:comment>
      <skos:definition xml:lang="en">The estimated date of dispatch of the invitations to submit tenders in two (or more) stage procedures.

WG Approval 01/10/2019 (epo:MultipleStageProcedureTerm) </skos:definition>
      <rdfs:isDefinedBy rdf:resource="http://data.europa.eu/a4g/ontology"/>
   </owl:DatatypeProperty>
   <owl:DatatypeProperty rdf:about="http://data.europa.eu/a4g/ontology#hasMaximumNumberOfCandidates">
      <rdfs:label xml:lang="en">Has maximum number of candidates</rdfs:label>
      <skos:prefLabel xml:lang="en">Has maximum number of candidates</skos:prefLabel>
      <rdfs:comment xml:lang="en">Maximum number of candidates to be invited for the second stage of the procedure.

WG Approval 22/08/2019 (epo:MultipleStageProcedureTerm) </rdfs:comment>
      <skos:definition xml:lang="en">Maximum number of candidates to be invited for the second stage of the procedure.

WG Approval 22/08/2019 (epo:MultipleStageProcedureTerm) </skos:definition>
      <rdfs:isDefinedBy rdf:resource="http://data.europa.eu/a4g/ontology"/>
   </owl:DatatypeProperty>
   <owl:DatatypeProperty rdf:about="http://data.europa.eu/a4g/ontology#hasMinimumNumberOfCandidates">
      <rdfs:label xml:lang="en">Has minimum number of candidates</rdfs:label>
      <skos:prefLabel xml:lang="en">Has minimum number of candidates</skos:prefLabel>
      <rdfs:comment xml:lang="en">Minimum number of candidates to be invited for the second stage of the procedure.

WG Approval 22/08/2019  (epo:MultipleStageProcedureTerm) </rdfs:comment>
      <skos:definition xml:lang="en">Minimum number of candidates to be invited for the second stage of the procedure.

WG Approval 22/08/2019  (epo:MultipleStageProcedureTerm) </skos:definition>
      <rdfs:isDefinedBy rdf:resource="http://data.europa.eu/a4g/ontology"/>
   </owl:DatatypeProperty>
   <owl:DatatypeProperty rdf:about="http://data.europa.eu/a4g/ontology#hasNoNegotiationNecessary">
      <rdfs:label xml:lang="en">Has no negotiation necessary</rdfs:label>
      <skos:prefLabel xml:lang="en">Has no negotiation necessary</skos:prefLabel>
      <rdfs:comment xml:lang="en">The buyer reserves the right to award the contract on the basis of the initial tenders without any further negotiations.

Additional information:
See Article 29(4) of Directive 2014/24/EU. 
 (epo:MultipleStageProcedureTerm) </rdfs:comment>
      <skos:definition xml:lang="en">The buyer reserves the right to award the contract on the basis of the initial tenders without any further negotiations.

Additional information:
See Article 29(4) of Directive 2014/24/EU. 
 (epo:MultipleStageProcedureTerm) </skos:definition>
      <rdfs:isDefinedBy rdf:resource="http://data.europa.eu/a4g/ontology"/>
   </owl:DatatypeProperty>
   <owl:DatatypeProperty rdf:about="http://data.europa.eu/a4g/ontology#hasSuccessiveReduction">
      <rdfs:label xml:lang="en">Has successive reduction</rdfs:label>
      <skos:prefLabel xml:lang="en">Has successive reduction</skos:prefLabel>
      <rdfs:comment xml:lang="en">The number of solutions or tenders will be reduced in iterative evaluations for multiple staged procedures.

Additional information:
This refers to multiple-stage procedures (included two-stage procedures, at least). Open Procedures can be seen as one-stage procedures.
WG Approval 22/08/2019  (epo:MultipleStageProcedureTerm) </rdfs:comment>
      <skos:definition xml:lang="en">The number of solutions or tenders will be reduced in iterative evaluations for multiple staged procedures.

Additional information:
This refers to multiple-stage procedures (included two-stage procedures, at least). Open Procedures can be seen as one-stage procedures.
WG Approval 22/08/2019  (epo:MultipleStageProcedureTerm) </skos:definition>
      <rdfs:isDefinedBy rdf:resource="http://data.europa.eu/a4g/ontology"/>
   </owl:DatatypeProperty>
   <owl:DatatypeProperty rdf:about="http://data.europa.eu/a4g/ontology#hasDPSScope">
      <rdfs:label xml:lang="en">Has d p s scope</rdfs:label>
      <skos:prefLabel xml:lang="en">Has d p s scope</skos:prefLabel>
      <rdfs:comment xml:lang="en">Explanation as to whether a dps is used and by whom.
WG Approval 09/11/2021 (epo:Notice) </rdfs:comment>
      <skos:definition xml:lang="en">Explanation as to whether a dps is used and by whom.
WG Approval 09/11/2021 (epo:Notice) </skos:definition>
      <rdfs:isDefinedBy rdf:resource="http://data.europa.eu/a4g/ontology"/>
   </owl:DatatypeProperty>
   <owl:DatatypeProperty rdf:about="http://data.europa.eu/a4g/ontology#hasFormType">
      <rdfs:label xml:lang="en">Has form type</rdfs:label>
      <skos:prefLabel xml:lang="en">Has form type</skos:prefLabel>
      <rdfs:comment xml:lang="en">A categorisation of the steps in which the Notice is used.

WG Approval 12/05/2020 (epo:Notice) </rdfs:comment>
      <skos:definition xml:lang="en">A categorisation of the steps in which the Notice is used.

WG Approval 12/05/2020 (epo:Notice) </skos:definition>
      <rdfs:isDefinedBy rdf:resource="http://data.europa.eu/a4g/ontology"/>
   </owl:DatatypeProperty>
   <owl:DatatypeProperty rdf:about="http://data.europa.eu/a4g/ontology#hasNotificationContentType">
      <rdfs:label xml:lang="en">Has notification content type</rdfs:label>
      <skos:prefLabel xml:lang="en">Has notification content type</skos:prefLabel>
      <rdfs:comment xml:lang="en">A categorisation of templates for sets of Procurement information to be conveyed in Notices.

WG Approval 12/05/2020 (epo:Notice) </rdfs:comment>
      <skos:definition xml:lang="en">A categorisation of templates for sets of Procurement information to be conveyed in Notices.

WG Approval 12/05/2020 (epo:Notice) </skos:definition>
      <rdfs:isDefinedBy rdf:resource="http://data.europa.eu/a4g/ontology"/>
   </owl:DatatypeProperty>
   <owl:DatatypeProperty rdf:about="http://data.europa.eu/a4g/ontology#hasPreferredPublicationDate">
      <rdfs:label xml:lang="en">Has preferred publication date</rdfs:label>
      <skos:prefLabel xml:lang="en">Has preferred publication date</skos:prefLabel>
      <rdfs:comment xml:lang="en">The date the buyer would like to have the record made publicly available.

WG Approval 12/05/2020 (epo:Notice) </rdfs:comment>
      <skos:definition xml:lang="en">The date the buyer would like to have the record made publicly available.

WG Approval 12/05/2020 (epo:Notice) </skos:definition>
      <rdfs:isDefinedBy rdf:resource="http://data.europa.eu/a4g/ontology"/>
   </owl:DatatypeProperty>
   <owl:DatatypeProperty rdf:about="http://data.europa.eu/a4g/ontology#hasPublicationDate">
      <rdfs:label xml:lang="en">Has publication date</rdfs:label>
      <skos:prefLabel xml:lang="en">Has publication date</skos:prefLabel>
      <rdfs:comment xml:lang="en">The date when a record is made publicly available.

(WG approval 01/06/2018) (epo:Notice) </rdfs:comment>
      <skos:definition xml:lang="en">The date when a record is made publicly available.

(WG approval 01/06/2018) (epo:Notice) </skos:definition>
      <rdfs:isDefinedBy rdf:resource="http://data.europa.eu/a4g/ontology"/>
   </owl:DatatypeProperty>
   <owl:DatatypeProperty rdf:about="http://data.europa.eu/a4g/ontology#hasOpeningDateTime">
      <rdfs:label xml:lang="en">Has opening date time</rdfs:label>
      <skos:prefLabel xml:lang="en">Has opening date time</skos:prefLabel>
      <rdfs:comment xml:lang="en">Date and time for the opening of tenders.

WG Approval 12/03/2019

 (epo:OpeningTerm) </rdfs:comment>
      <skos:definition xml:lang="en">Date and time for the opening of tenders.

WG Approval 12/03/2019

 (epo:OpeningTerm) </skos:definition>
      <rdfs:isDefinedBy rdf:resource="http://data.europa.eu/a4g/ontology"/>
   </owl:DatatypeProperty>
   <owl:DatatypeProperty rdf:about="http://data.europa.eu/a4g/ontology#hasOpeningDescription">
      <rdfs:label xml:lang="en">Has opening description</rdfs:label>
      <skos:prefLabel xml:lang="en">Has opening description</skos:prefLabel>
      <rdfs:comment xml:lang="en">Further information about the opening of tenders. 

Additional Information
For example, who may participate in the opening and whether any authorization is needed.

WG Approval 12/03/2019 (epo:OpeningTerm) </rdfs:comment>
      <skos:definition xml:lang="en">Further information about the opening of tenders. 

Additional Information
For example, who may participate in the opening and whether any authorization is needed.

WG Approval 12/03/2019 (epo:OpeningTerm) </skos:definition>
      <rdfs:isDefinedBy rdf:resource="http://data.europa.eu/a4g/ontology"/>
   </owl:DatatypeProperty>
   <owl:DatatypeProperty rdf:about="http://data.europa.eu/a4g/ontology#hasOpeningURL">
      <rdfs:label xml:lang="en">Has opening u r l</rdfs:label>
      <skos:prefLabel xml:lang="en">Has opening u r l</skos:prefLabel>
      <rdfs:comment xml:lang="en">The identifier of the address of the Opening of Tenders.
WG Approval 09/11/2021 (epo:OpeningTerm) </rdfs:comment>
      <skos:definition xml:lang="en">The identifier of the address of the Opening of Tenders.
WG Approval 09/11/2021 (epo:OpeningTerm) </skos:definition>
      <rdfs:isDefinedBy rdf:resource="http://data.europa.eu/a4g/ontology"/>
   </owl:DatatypeProperty>
   <owl:DatatypeProperty rdf:about="http://data.europa.eu/a4g/ontology#hasLegalFormType">
      <rdfs:label xml:lang="en">Has legal form type</rdfs:label>
      <skos:prefLabel xml:lang="en">Has legal form type</skos:prefLabel>
      <rdfs:comment xml:lang="en">Note that the codelist provided at national level should be used. (epo:Organisation) </rdfs:comment>
      <skos:definition xml:lang="en">Note that the codelist provided at national level should be used. (epo:Organisation) </skos:definition>
      <rdfs:isDefinedBy rdf:resource="http://data.europa.eu/a4g/ontology"/>
   </owl:DatatypeProperty>
   <owl:DatatypeProperty rdf:about="http://data.europa.eu/a4g/ontology#hasLegalName">
      <rdfs:label xml:lang="en">Has legal name</rdfs:label>
      <skos:prefLabel xml:lang="en">Has legal name</skos:prefLabel>
      <rdfs:comment xml:lang="en">The officially registered name of an organisation. 

WG Approval 16/11/2021 (epo:Organisation) </rdfs:comment>
      <skos:definition xml:lang="en">The officially registered name of an organisation. 

WG Approval 16/11/2021 (epo:Organisation) </skos:definition>
      <rdfs:isDefinedBy rdf:resource="http://data.europa.eu/a4g/ontology"/>
   </owl:DatatypeProperty>
   <owl:DatatypeProperty rdf:about="http://data.europa.eu/a4g/ontology#hasGroupType">
      <rdfs:label xml:lang="en">Has group type</rdfs:label>
      <skos:prefLabel xml:lang="en">Has group type</skos:prefLabel>
      <rdfs:comment xml:lang="en">Form of collabaration agreement between organisations.
WG Approval 09/11/2021 (epo:OrganisationGroup) </rdfs:comment>
      <skos:definition xml:lang="en">Form of collabaration agreement between organisations.
WG Approval 09/11/2021 (epo:OrganisationGroup) </skos:definition>
      <rdfs:isDefinedBy rdf:resource="http://data.europa.eu/a4g/ontology"/>
   </owl:DatatypeProperty>
   <owl:ObjectProperty rdf:about="http://data.europa.eu/a4g/ontology#hasDurationMeasure">
      <rdfs:label xml:lang="en">Has duration measure</rdfs:label>
      <skos:prefLabel xml:lang="en">Has duration measure</skos:prefLabel>
      <rdfs:comment xml:lang="en">The duration of this period, expressed as an ISO 8601 code.  (epo:Period) </rdfs:comment>
      <skos:definition xml:lang="en">The duration of this period, expressed as an ISO 8601 code.  (epo:Period) </skos:definition>
      <rdfs:isDefinedBy rdf:resource="http://data.europa.eu/a4g/ontology"/>
   </owl:ObjectProperty>
   <owl:DatatypeProperty rdf:about="http://data.europa.eu/a4g/ontology#hasEndDate">
      <rdfs:label xml:lang="en">Has end date</rdfs:label>
      <skos:prefLabel xml:lang="en">Has end date</skos:prefLabel>
      <rdfs:comment xml:lang="en">The date on which this period ends. (epo:Period) </rdfs:comment>
      <skos:definition xml:lang="en">The date on which this period ends. (epo:Period) </skos:definition>
      <rdfs:isDefinedBy rdf:resource="http://data.europa.eu/a4g/ontology"/>
   </owl:DatatypeProperty>
   <owl:DatatypeProperty rdf:about="http://data.europa.eu/a4g/ontology#hasEndTime">
      <rdfs:label xml:lang="en">Has end time</rdfs:label>
      <skos:prefLabel xml:lang="en">Has end time</skos:prefLabel>
      <rdfs:comment xml:lang="en">The time at which this period ends. (epo:Period) </rdfs:comment>
      <skos:definition xml:lang="en">The time at which this period ends. (epo:Period) </skos:definition>
      <rdfs:isDefinedBy rdf:resource="http://data.europa.eu/a4g/ontology"/>
   </owl:DatatypeProperty>
   <owl:DatatypeProperty rdf:about="http://data.europa.eu/a4g/ontology#hasStartDate">
      <rdfs:label xml:lang="en">Has start date</rdfs:label>
      <skos:prefLabel xml:lang="en">Has start date</skos:prefLabel>
      <rdfs:comment xml:lang="en">The date on which this period begins. (epo:Period) </rdfs:comment>
      <skos:definition xml:lang="en">The date on which this period begins. (epo:Period) </skos:definition>
      <rdfs:isDefinedBy rdf:resource="http://data.europa.eu/a4g/ontology"/>
   </owl:DatatypeProperty>
   <owl:DatatypeProperty rdf:about="http://data.europa.eu/a4g/ontology#hasStartTime">
      <rdfs:label xml:lang="en">Has start time</rdfs:label>
      <skos:prefLabel xml:lang="en">Has start time</skos:prefLabel>
      <rdfs:comment xml:lang="en">The time at which this period begins. (epo:Period) </rdfs:comment>
      <skos:definition xml:lang="en">The time at which this period begins. (epo:Period) </skos:definition>
      <rdfs:isDefinedBy rdf:resource="http://data.europa.eu/a4g/ontology"/>
   </owl:DatatypeProperty>
   <owl:DatatypeProperty rdf:about="http://data.europa.eu/a4g/ontology#hasAlternativeName">
      <rdfs:label xml:lang="en">Has alternative name</rdfs:label>
      <skos:prefLabel xml:lang="en">Has alternative name</skos:prefLabel>
      <rdfs:comment xml:lang="en">Any name by which an individual is known other than their full name.
WG 09/11/2021 (epo:Person) </rdfs:comment>
      <skos:definition xml:lang="en">Any name by which an individual is known other than their full name.
WG 09/11/2021 (epo:Person) </skos:definition>
      <rdfs:isDefinedBy rdf:resource="http://data.europa.eu/a4g/ontology"/>
   </owl:DatatypeProperty>
   <owl:DatatypeProperty rdf:about="http://data.europa.eu/a4g/ontology#hasBirthFamilyName">
      <rdfs:label xml:lang="en">Has birth family name</rdfs:label>
      <skos:prefLabel xml:lang="en">Has birth family name</skos:prefLabel>
      <rdfs:comment xml:lang="en">Family name of the Person given upon their birth
WG Approval 09/11/2021 (epo:Person) </rdfs:comment>
      <skos:definition xml:lang="en">Family name of the Person given upon their birth
WG Approval 09/11/2021 (epo:Person) </skos:definition>
      <rdfs:isDefinedBy rdf:resource="http://data.europa.eu/a4g/ontology"/>
   </owl:DatatypeProperty>
   <owl:DatatypeProperty rdf:about="http://data.europa.eu/a4g/ontology#hasDateOfBirth">
      <rdfs:label xml:lang="en">Has date of birth</rdfs:label>
      <skos:prefLabel xml:lang="en">Has date of birth</skos:prefLabel>
      <rdfs:comment xml:lang="en">The day on which the Person was born.
WG Approval 09/11/2021 (epo:Person) </rdfs:comment>
      <skos:definition xml:lang="en">The day on which the Person was born.
WG Approval 09/11/2021 (epo:Person) </skos:definition>
      <rdfs:isDefinedBy rdf:resource="http://data.europa.eu/a4g/ontology"/>
   </owl:DatatypeProperty>
   <owl:DatatypeProperty rdf:about="http://data.europa.eu/a4g/ontology#hasDateOfDeath">
      <rdfs:label xml:lang="en">Has date of death</rdfs:label>
      <skos:prefLabel xml:lang="en">Has date of death</skos:prefLabel>
      <rdfs:comment xml:lang="en">The day on which the Person died.
WG Approval 09/11/2021 (epo:Person) </rdfs:comment>
      <skos:definition xml:lang="en">The day on which the Person died.
WG Approval 09/11/2021 (epo:Person) </skos:definition>
      <rdfs:isDefinedBy rdf:resource="http://data.europa.eu/a4g/ontology"/>
   </owl:DatatypeProperty>
   <owl:DatatypeProperty rdf:about="http://data.europa.eu/a4g/ontology#hasFamilyName">
      <rdfs:label xml:lang="en">Has family name</rdfs:label>
      <skos:prefLabel xml:lang="en">Has family name</skos:prefLabel>
      <rdfs:comment xml:lang="en">Name usually shared by members of a family.
WG 09/11/2021

 (epo:Person) </rdfs:comment>
      <skos:definition xml:lang="en">Name usually shared by members of a family.
WG 09/11/2021

 (epo:Person) </skos:definition>
      <rdfs:isDefinedBy rdf:resource="http://data.europa.eu/a4g/ontology"/>
   </owl:DatatypeProperty>
   <owl:DatatypeProperty rdf:about="http://data.europa.eu/a4g/ontology#hasFullName">
      <rdfs:label xml:lang="en">Has full name</rdfs:label>
      <skos:prefLabel xml:lang="en">Has full name</skos:prefLabel>
      <rdfs:comment xml:lang="en">The complete name of a person.
WG 09/11/2021 (epo:Person) </rdfs:comment>
      <skos:definition xml:lang="en">The complete name of a person.
WG 09/11/2021 (epo:Person) </skos:definition>
      <rdfs:isDefinedBy rdf:resource="http://data.europa.eu/a4g/ontology"/>
   </owl:DatatypeProperty>
   <owl:DatatypeProperty rdf:about="http://data.europa.eu/a4g/ontology#hasGivenName">
      <rdfs:label xml:lang="en">Has given name</rdfs:label>
      <skos:prefLabel xml:lang="en">Has given name</skos:prefLabel>
      <rdfs:comment xml:lang="en">The denominator(s) that identify an individual within a family.
WG 09/11/2021
 (epo:Person) </rdfs:comment>
      <skos:definition xml:lang="en">The denominator(s) that identify an individual within a family.
WG 09/11/2021
 (epo:Person) </skos:definition>
      <rdfs:isDefinedBy rdf:resource="http://data.europa.eu/a4g/ontology"/>
   </owl:DatatypeProperty>
   <owl:DatatypeProperty rdf:about="http://data.europa.eu/a4g/ontology#hasNationality">
      <rdfs:label xml:lang="en">Has nationality</rdfs:label>
      <skos:prefLabel xml:lang="en">Has nationality</skos:prefLabel>
      <rdfs:isDefinedBy rdf:resource="http://data.europa.eu/a4g/ontology"/>
   </owl:DatatypeProperty>
   <owl:DatatypeProperty rdf:about="http://data.europa.eu/a4g/ontology#hasPatronimicName">
      <rdfs:label xml:lang="en">Has patronimic name</rdfs:label>
      <skos:prefLabel xml:lang="en">Has patronimic name</skos:prefLabel>
      <rdfs:comment xml:lang="en">Name based on the given name of the Person's father.
WG Approval 09/11/2021 (epo:Person) </rdfs:comment>
      <skos:definition xml:lang="en">Name based on the given name of the Person's father.
WG Approval 09/11/2021 (epo:Person) </skos:definition>
      <rdfs:isDefinedBy rdf:resource="http://data.europa.eu/a4g/ontology"/>
   </owl:DatatypeProperty>
   <owl:DatatypeProperty rdf:about="http://data.europa.eu/a4g/ontology#hasLegalBasis">
      <rdfs:label xml:lang="en">Has legal basis</rdfs:label>
      <skos:prefLabel xml:lang="en">Has legal basis</skos:prefLabel>
      <rdfs:comment xml:lang="en">The legal basis under which the procurement procedure takes place.

Additional Information: 
For example European Directives or Regulations, national law

WG 09/11/2021 (epo:PlannedProcurementPart) The legal basis under which the procurement procedure takes place.

Additional Information: 
For example European Directives or Regulations, national law

WG 09/11/2021
 (epo:Procedure) </rdfs:comment>
      <skos:definition xml:lang="en">The legal basis under which the procurement procedure takes place.

Additional Information: 
For example European Directives or Regulations, national law

WG 09/11/2021 (epo:PlannedProcurementPart) The legal basis under which the procurement procedure takes place.

Additional Information: 
For example European Directives or Regulations, national law

WG 09/11/2021
 (epo:Procedure) </skos:definition>
      <rdfs:isDefinedBy rdf:resource="http://data.europa.eu/a4g/ontology"/>
   </owl:DatatypeProperty>
   <owl:DatatypeProperty rdf:about="http://data.europa.eu/a4g/ontology#hasLegalBasisID">
      <rdfs:label xml:lang="en">Has legal basis i d</rdfs:label>
      <skos:prefLabel xml:lang="en">Has legal basis i d</skos:prefLabel>
      <rdfs:comment xml:lang="en">Identifier of the Legal Basis.
WG 09/11/2021 (epo:PlannedProcurementPart) Identifier of the Legal Basis.
WG 09/11/2021
 (epo:Procedure) </rdfs:comment>
      <skos:definition xml:lang="en">Identifier of the Legal Basis.
WG 09/11/2021 (epo:PlannedProcurementPart) Identifier of the Legal Basis.
WG 09/11/2021
 (epo:Procedure) </skos:definition>
      <rdfs:isDefinedBy rdf:resource="http://data.europa.eu/a4g/ontology"/>
   </owl:DatatypeProperty>
   <owl:DatatypeProperty rdf:about="http://data.europa.eu/a4g/ontology#hasEstimatedContractNoticePublicationDate">
      <rdfs:label xml:lang="en">Has estimated contract notice publication date</rdfs:label>
      <skos:prefLabel xml:lang="en">Has estimated contract notice publication date</skos:prefLabel>
      <rdfs:comment xml:lang="en">Foreseen date for publication of Contract Notice. (epo:PriorInformationNotice) </rdfs:comment>
      <skos:definition xml:lang="en">Foreseen date for publication of Contract Notice. (epo:PriorInformationNotice) </skos:definition>
      <rdfs:isDefinedBy rdf:resource="http://data.europa.eu/a4g/ontology"/>
   </owl:DatatypeProperty>
   <owl:DatatypeProperty rdf:about="http://data.europa.eu/a4g/ontology#hasPrizeRank">
      <rdfs:label xml:lang="en">Has prize rank</rdfs:label>
      <skos:prefLabel xml:lang="en">Has prize rank</skos:prefLabel>
      <rdfs:comment xml:lang="en">The position of the prize (e.g. first place, second place) in a design contest list of prizes.

WG Approval 29/08/2019 
 (epo:Prize) </rdfs:comment>
      <skos:definition xml:lang="en">The position of the prize (e.g. first place, second place) in a design contest list of prizes.

WG Approval 29/08/2019 
 (epo:Prize) </skos:definition>
      <rdfs:isDefinedBy rdf:resource="http://data.europa.eu/a4g/ontology"/>
   </owl:DatatypeProperty>
   <owl:ObjectProperty rdf:about="http://data.europa.eu/a4g/ontology#hasPrizeValue">
      <rdfs:label xml:lang="en">Has prize value</rdfs:label>
      <skos:prefLabel xml:lang="en">Has prize value</skos:prefLabel>
      <rdfs:comment xml:lang="en">The monetary value of a prize, if any, for the winner (or runners-up) of the design contest.

WG Approval 29/08/2019 (epo:Prize) </rdfs:comment>
      <skos:definition xml:lang="en">The monetary value of a prize, if any, for the winner (or runners-up) of the design contest.

WG Approval 29/08/2019 (epo:Prize) </skos:definition>
      <rdfs:isDefinedBy rdf:resource="http://data.europa.eu/a4g/ontology"/>
   </owl:ObjectProperty>
   <owl:DatatypeProperty rdf:about="http://data.europa.eu/a4g/ontology#hasAcceleratedProcedureJustification">
      <rdfs:label xml:lang="en">Has accelerated procedure justification</rdfs:label>
      <skos:prefLabel xml:lang="en">Has accelerated procedure justification</skos:prefLabel>
      <rdfs:comment xml:lang="en">The reasons why the procedure is accelerated.

Additional Information:
A procedure is accelerated to cover needs of extraordinary circumstances ie earthquake relief.

WG Approval 09/06/2020

 (epo:Procedure) </rdfs:comment>
      <skos:definition xml:lang="en">The reasons why the procedure is accelerated.

Additional Information:
A procedure is accelerated to cover needs of extraordinary circumstances ie earthquake relief.

WG Approval 09/06/2020

 (epo:Procedure) </skos:definition>
      <rdfs:isDefinedBy rdf:resource="http://data.europa.eu/a4g/ontology"/>
   </owl:DatatypeProperty>
   <owl:DatatypeProperty rdf:about="http://data.europa.eu/a4g/ontology#hasCompetitionTermination">
      <rdfs:label xml:lang="en">Has competition termination</rdfs:label>
      <skos:prefLabel xml:lang="en">Has competition termination</skos:prefLabel>
      <rdfs:comment xml:lang="en">No further contracts will be awarded in this procedure.

Additional Information: 

PIN for Competition needs to be signaled. This field can be used even if no contracts are awarded in the contract award notice. (epo:Procedure) </rdfs:comment>
      <skos:definition xml:lang="en">No further contracts will be awarded in this procedure.

Additional Information: 

PIN for Competition needs to be signaled. This field can be used even if no contracts are awarded in the contract award notice. (epo:Procedure) </skos:definition>
      <rdfs:isDefinedBy rdf:resource="http://data.europa.eu/a4g/ontology"/>
   </owl:DatatypeProperty>
   <owl:DatatypeProperty rdf:about="http://data.europa.eu/a4g/ontology#hasDesignContest">
      <rdfs:label xml:lang="en">Has design contest</rdfs:label>
      <skos:prefLabel xml:lang="en">Has design contest</skos:prefLabel>
      <rdfs:comment xml:lang="en">A competition which enables the buyer to acquire a  plan or design via a jury.

Additional information: 
Design contests have traditionally mostly been used in the fields of town and country planning, architecture and engineering or data processing, other purposes, such as to obtain plans for financial engineering 

The contest may include or not the award of prizes;

WG approval 04-02-2021  (epo:Procedure) </rdfs:comment>
      <skos:definition xml:lang="en">A competition which enables the buyer to acquire a  plan or design via a jury.

Additional information: 
Design contests have traditionally mostly been used in the fields of town and country planning, architecture and engineering or data processing, other purposes, such as to obtain plans for financial engineering 

The contest may include or not the award of prizes;

WG approval 04-02-2021  (epo:Procedure) </skos:definition>
      <rdfs:isDefinedBy rdf:resource="http://data.europa.eu/a4g/ontology"/>
   </owl:DatatypeProperty>
   <owl:DatatypeProperty rdf:about="http://data.europa.eu/a4g/ontology#hasLegalRegime">
      <rdfs:label xml:lang="en">Has legal regime</rdfs:label>
      <skos:prefLabel xml:lang="en">Has legal regime</skos:prefLabel>
      <rdfs:isDefinedBy rdf:resource="http://data.europa.eu/a4g/ontology"/>
   </owl:DatatypeProperty>
   <owl:DatatypeProperty rdf:about="http://data.europa.eu/a4g/ontology#hasLotMinimumSubmission">
      <rdfs:label xml:lang="en">Has lot minimum submission</rdfs:label>
      <skos:prefLabel xml:lang="en">Has lot minimum submission</skos:prefLabel>
      <rdfs:comment xml:lang="en">The minimum number of lots for which one tenderer must submit tenders. 

Additional Information

This can be used to state that a tenderer has to submit the maximum number of lots announced in the contract notice (i.e. in this case the Lot Minimum Submission would equal to the Lot Submission Limit).

 (epo:Procedure) </rdfs:comment>
      <skos:definition xml:lang="en">The minimum number of lots for which one tenderer must submit tenders. 

Additional Information

This can be used to state that a tenderer has to submit the maximum number of lots announced in the contract notice (i.e. in this case the Lot Minimum Submission would equal to the Lot Submission Limit).

 (epo:Procedure) </skos:definition>
      <rdfs:isDefinedBy rdf:resource="http://data.europa.eu/a4g/ontology"/>
   </owl:DatatypeProperty>
   <owl:DatatypeProperty rdf:about="http://data.europa.eu/a4g/ontology#hasLotSubmissionLimit">
      <rdfs:label xml:lang="en">Has lot submission limit</rdfs:label>
      <skos:prefLabel xml:lang="en">Has lot submission limit</skos:prefLabel>
      <rdfs:comment xml:lang="en">The total number of lots for which one tenderer can submit tenders.

(WG approval 12/12/2018)

 (epo:Procedure) </rdfs:comment>
      <skos:definition xml:lang="en">The total number of lots for which one tenderer can submit tenders.

(WG approval 12/12/2018)

 (epo:Procedure) </skos:definition>
      <rdfs:isDefinedBy rdf:resource="http://data.europa.eu/a4g/ontology"/>
   </owl:DatatypeProperty>
   <owl:DatatypeProperty rdf:about="http://data.europa.eu/a4g/ontology#hasMainFeature">
      <rdfs:label xml:lang="en">Has main feature</rdfs:label>
      <skos:prefLabel xml:lang="en">Has main feature</skos:prefLabel>
      <rdfs:comment xml:lang="en">Main features of the procedure and information about where the full rules for the procedure can be found. 

Additional Information

This information should be given when the procedure is not one of those mentioned in the procurement directives. This can be the case for example for concessions, for social and other specific services, and in case of voluntary publication of procurement procedures below the EU procurement thresholds. (epo:Procedure) </rdfs:comment>
      <skos:definition xml:lang="en">Main features of the procedure and information about where the full rules for the procedure can be found. 

Additional Information

This information should be given when the procedure is not one of those mentioned in the procurement directives. This can be the case for example for concessions, for social and other specific services, and in case of voluntary publication of procurement procedures below the EU procurement thresholds. (epo:Procedure) </skos:definition>
      <rdfs:isDefinedBy rdf:resource="http://data.europa.eu/a4g/ontology"/>
   </owl:DatatypeProperty>
   <owl:DatatypeProperty rdf:about="http://data.europa.eu/a4g/ontology#hasMaximumNumberOfLotsToBeAwarded">
      <rdfs:label xml:lang="en">Has maximum number of lots to be awarded</rdfs:label>
      <skos:prefLabel xml:lang="en">Has maximum number of lots to be awarded</skos:prefLabel>
      <rdfs:comment xml:lang="en">The maximum number of lots for which contract(s) can be awarded to one tenderer.

WG Approval 22/08/2019 (epo:Procedure) </rdfs:comment>
      <skos:definition xml:lang="en">The maximum number of lots for which contract(s) can be awarded to one tenderer.

WG Approval 22/08/2019 (epo:Procedure) </skos:definition>
      <rdfs:isDefinedBy rdf:resource="http://data.europa.eu/a4g/ontology"/>
   </owl:DatatypeProperty>
   <owl:DatatypeProperty rdf:about="http://data.europa.eu/a4g/ontology#hasProcedureType">
      <rdfs:label xml:lang="en">Has procedure type</rdfs:label>
      <skos:prefLabel xml:lang="en">Has procedure type</skos:prefLabel>
      <rdfs:comment xml:lang="en">Identification of the Procedure used.

WG Approval 09/06/2020 (epo:Procedure) </rdfs:comment>
      <skos:definition xml:lang="en">Identification of the Procedure used.

WG Approval 09/06/2020 (epo:Procedure) </skos:definition>
      <rdfs:isDefinedBy rdf:resource="http://data.europa.eu/a4g/ontology"/>
   </owl:DatatypeProperty>
   <owl:DatatypeProperty rdf:about="http://data.europa.eu/a4g/ontology#isAccelerated">
      <rdfs:label xml:lang="en">Is accelerated</rdfs:label>
      <skos:prefLabel xml:lang="en">Is accelerated</skos:prefLabel>
      <rdfs:comment xml:lang="en">Statement about  the fact that the procedure will be reduced due to a state of urgency.

Additional Information

This modifies the time limit for the receipt of requests to participate or the receipt of tenders.

WG Approval 20/08/2019
 (epo:Procedure) </rdfs:comment>
      <skos:definition xml:lang="en">Statement about  the fact that the procedure will be reduced due to a state of urgency.

Additional Information

This modifies the time limit for the receipt of requests to participate or the receipt of tenders.

WG Approval 20/08/2019
 (epo:Procedure) </skos:definition>
      <rdfs:isDefinedBy rdf:resource="http://data.europa.eu/a4g/ontology"/>
   </owl:DatatypeProperty>
   <owl:DatatypeProperty rdf:about="http://data.europa.eu/a4g/ontology#hasGroupLotEvaluationMethod">
      <rdfs:label xml:lang="en">Has group lot evaluation method</rdfs:label>
      <skos:prefLabel xml:lang="en">Has group lot evaluation method</skos:prefLabel>
      <rdfs:comment xml:lang="en">Description of how lots and groups of lots are evaluated against one another in the procedure.



 (epo:ProcedureTerm) </rdfs:comment>
      <skos:definition xml:lang="en">Description of how lots and groups of lots are evaluated against one another in the procedure.



 (epo:ProcedureTerm) </skos:definition>
      <rdfs:isDefinedBy rdf:resource="http://data.europa.eu/a4g/ontology"/>
   </owl:DatatypeProperty>
   <owl:DatatypeProperty rdf:about="http://data.europa.eu/a4g/ontology#hasLotAwardLimit">
      <rdfs:label xml:lang="en">Has lot award limit</rdfs:label>
      <skos:prefLabel xml:lang="en">Has lot award limit</skos:prefLabel>
      <rdfs:comment xml:lang="en">The total number of lots for which contract(s) can be awarded to one tenderer.

(WG Approval 12/12/2018) (epo:ProcedureTerm) </rdfs:comment>
      <skos:definition xml:lang="en">The total number of lots for which contract(s) can be awarded to one tenderer.

(WG Approval 12/12/2018) (epo:ProcedureTerm) </skos:definition>
      <rdfs:isDefinedBy rdf:resource="http://data.europa.eu/a4g/ontology"/>
   </owl:DatatypeProperty>
   <owl:DatatypeProperty rdf:about="http://data.europa.eu/a4g/ontology#hasReceiptExpressionsDeadline">
      <rdfs:label xml:lang="en">Has receipt expressions deadline</rdfs:label>
      <skos:prefLabel xml:lang="en">Has receipt expressions deadline</skos:prefLabel>
      <rdfs:comment xml:lang="en">Time limit for receipt of expressions of interest.

Pending of review by the WG

 (epo:ProcedureTerm) </rdfs:comment>
      <skos:definition xml:lang="en">Time limit for receipt of expressions of interest.

Pending of review by the WG

 (epo:ProcedureTerm) </skos:definition>
      <rdfs:isDefinedBy rdf:resource="http://data.europa.eu/a4g/ontology"/>
   </owl:DatatypeProperty>
   <owl:DatatypeProperty rdf:about="http://data.europa.eu/a4g/ontology#hasFreeEAccess">
      <rdfs:label xml:lang="en">Has free e access</rdfs:label>
      <skos:prefLabel xml:lang="en">Has free e access</skos:prefLabel>
      <rdfs:comment xml:lang="en">Indicates whether the procurement documents are electronically available for unrestricted and full direct access, free of charge. (epo:ProcurementDocument) </rdfs:comment>
      <skos:definition xml:lang="en">Indicates whether the procurement documents are electronically available for unrestricted and full direct access, free of charge. (epo:ProcurementDocument) </skos:definition>
      <rdfs:isDefinedBy rdf:resource="http://data.europa.eu/a4g/ontology"/>
   </owl:DatatypeProperty>
   <owl:DatatypeProperty rdf:about="http://data.europa.eu/a4g/ontology#hasAvailabilityDate">
      <rdfs:label xml:lang="en">Has availability date</rdfs:label>
      <skos:prefLabel xml:lang="en">Has availability date</skos:prefLabel>
      <rdfs:comment xml:lang="en">The date at which unpublished data shall be published.

WG Approval 11/06/2020 (epo:PublicationProvision) </rdfs:comment>
      <skos:definition xml:lang="en">The date at which unpublished data shall be published.

WG Approval 11/06/2020 (epo:PublicationProvision) </skos:definition>
      <rdfs:isDefinedBy rdf:resource="http://data.europa.eu/a4g/ontology"/>
   </owl:DatatypeProperty>
   <owl:DatatypeProperty rdf:about="http://data.europa.eu/a4g/ontology#hasNonPublicationJustification">
      <rdfs:label xml:lang="en">Has non publication justification</rdfs:label>
      <skos:prefLabel xml:lang="en">Has non publication justification</skos:prefLabel>
      <rdfs:comment xml:lang="en">The reason why data is not published.

WG Approval 11/06/2020 (epo:PublicationProvision) </rdfs:comment>
      <skos:definition xml:lang="en">The reason why data is not published.

WG Approval 11/06/2020 (epo:PublicationProvision) </skos:definition>
      <rdfs:isDefinedBy rdf:resource="http://data.europa.eu/a4g/ontology"/>
   </owl:DatatypeProperty>
   <owl:DatatypeProperty rdf:about="http://data.europa.eu/a4g/ontology#hasNonPublicationJustificationDescription">
      <rdfs:label xml:lang="en">Has non publication justification description</rdfs:label>
      <skos:prefLabel xml:lang="en">Has non publication justification description</skos:prefLabel>
      <rdfs:comment xml:lang="en">A narrative explanation of why data is not published.

Additional Information:
This element is generally used when the non-publication-justification code chosen is "other".

WG Approval 09/11/2021 (epo:PublicationProvision) </rdfs:comment>
      <skos:definition xml:lang="en">A narrative explanation of why data is not published.

Additional Information:
This element is generally used when the non-publication-justification code chosen is "other".

WG Approval 09/11/2021 (epo:PublicationProvision) </skos:definition>
      <rdfs:isDefinedBy rdf:resource="http://data.europa.eu/a4g/ontology"/>
   </owl:DatatypeProperty>
   <owl:DatatypeProperty rdf:about="http://data.europa.eu/a4g/ontology#hasAdditionalClassification">
      <rdfs:label xml:lang="en">Has additional classification</rdfs:label>
      <skos:prefLabel xml:lang="en">Has additional classification</skos:prefLabel>
      <rdfs:isDefinedBy rdf:resource="http://data.europa.eu/a4g/ontology"/>
   </owl:DatatypeProperty>
   <owl:DatatypeProperty rdf:about="http://data.europa.eu/a4g/ontology#hasAdditionalContractNature">
      <rdfs:label xml:lang="en">Has additional contract nature</rdfs:label>
      <skos:prefLabel xml:lang="en">Has additional contract nature</skos:prefLabel>
      <rdfs:comment xml:lang="en">Additional type of acquisition taken into consideration in the contract.

WG Approval 11/06/2020 (epo:Purpose) </rdfs:comment>
      <skos:definition xml:lang="en">Additional type of acquisition taken into consideration in the contract.

WG Approval 11/06/2020 (epo:Purpose) </skos:definition>
      <rdfs:isDefinedBy rdf:resource="http://data.europa.eu/a4g/ontology"/>
   </owl:DatatypeProperty>
   <owl:DatatypeProperty rdf:about="http://data.europa.eu/a4g/ontology#hasContractNatureType">
      <rdfs:label xml:lang="en">Has contract nature type</rdfs:label>
      <skos:prefLabel xml:lang="en">Has contract nature type</skos:prefLabel>
      <rdfs:comment xml:lang="en">Subject of the acquisition.

WG Approval 11/06/2020
 (epo:Purpose) </rdfs:comment>
      <skos:definition xml:lang="en">Subject of the acquisition.

WG Approval 11/06/2020
 (epo:Purpose) </skos:definition>
      <rdfs:isDefinedBy rdf:resource="http://data.europa.eu/a4g/ontology"/>
   </owl:DatatypeProperty>
   <owl:DatatypeProperty rdf:about="http://data.europa.eu/a4g/ontology#hasMainClassification">
      <rdfs:label xml:lang="en">Has main classification</rdfs:label>
      <skos:prefLabel xml:lang="en">Has main classification</skos:prefLabel>
      <rdfs:isDefinedBy rdf:resource="http://data.europa.eu/a4g/ontology"/>
   </owl:DatatypeProperty>
   <owl:DatatypeProperty rdf:about="http://data.europa.eu/a4g/ontology#hasOptionsDescription">
      <rdfs:label xml:lang="en">Has options description</rdfs:label>
      <skos:prefLabel xml:lang="en">Has options description</skos:prefLabel>
      <rdfs:comment xml:lang="en">The motivation and details about additional purchases that the buyer may undertake while the contract is valid.

WG Approval 09/04/2019  (epo:Purpose) </rdfs:comment>
      <skos:definition xml:lang="en">The motivation and details about additional purchases that the buyer may undertake while the contract is valid.

WG Approval 09/04/2019  (epo:Purpose) </skos:definition>
      <rdfs:isDefinedBy rdf:resource="http://data.europa.eu/a4g/ontology"/>
   </owl:DatatypeProperty>
   <owl:DatatypeProperty rdf:about="http://data.europa.eu/a4g/ontology#hasOptionsPermission">
      <rdfs:label xml:lang="en">Has options permission</rdfs:label>
      <skos:prefLabel xml:lang="en">Has options permission</skos:prefLabel>
      <rdfs:comment xml:lang="en">Explanation as to whether options are allowed or required.
WG 09/11/2021 (epo:Purpose) </rdfs:comment>
      <skos:definition xml:lang="en">Explanation as to whether options are allowed or required.
WG 09/11/2021 (epo:Purpose) </skos:definition>
      <rdfs:isDefinedBy rdf:resource="http://data.europa.eu/a4g/ontology"/>
   </owl:DatatypeProperty>
   <owl:ObjectProperty rdf:about="http://data.europa.eu/a4g/ontology#hasTotalMagnitudeQuantity">
      <rdfs:label xml:lang="en">Has total magnitude quantity</rdfs:label>
      <skos:prefLabel xml:lang="en">Has total magnitude quantity</skos:prefLabel>
      <rdfs:comment xml:lang="en">The number of units required.

Additional Information

The quantity needs to go along with the unit. 


 (epo:Purpose) </rdfs:comment>
      <skos:definition xml:lang="en">The number of units required.

Additional Information

The quantity needs to go along with the unit. 


 (epo:Purpose) </skos:definition>
      <rdfs:isDefinedBy rdf:resource="http://data.europa.eu/a4g/ontology"/>
   </owl:ObjectProperty>
   <owl:DatatypeProperty rdf:about="http://data.europa.eu/a4g/ontology#hasRegulatoryFrameworkType">
      <rdfs:label xml:lang="en">Has regulatory framework type</rdfs:label>
      <skos:prefLabel xml:lang="en">Has regulatory framework type</skos:prefLabel>
      <rdfs:isDefinedBy rdf:resource="http://data.europa.eu/a4g/ontology"/>
   </owl:DatatypeProperty>
   <owl:DatatypeProperty rdf:about="http://data.europa.eu/a4g/ontology#hasElementIRI">
      <rdfs:label xml:lang="en">Has element i r i</rdfs:label>
      <skos:prefLabel xml:lang="en">Has element i r i</skos:prefLabel>
      <rdfs:comment xml:lang="en">The Element may identify any type of elements, including documents, e.g. a Procurement Document that has changed. (epo:ResourceElement) </rdfs:comment>
      <skos:definition xml:lang="en">The Element may identify any type of elements, including documents, e.g. a Procurement Document that has changed. (epo:ResourceElement) </skos:definition>
      <rdfs:isDefinedBy rdf:resource="http://data.europa.eu/a4g/ontology"/>
   </owl:DatatypeProperty>
   <owl:DatatypeProperty rdf:about="http://data.europa.eu/a4g/ontology#hasReviewDeadline">
      <rdfs:label xml:lang="en">Has review deadline</rdfs:label>
      <skos:prefLabel xml:lang="en">Has review deadline</skos:prefLabel>
      <rdfs:comment xml:lang="en">The time limit for review procedures.
WG Approval 09/11/2021
 (epo:ReviewTerm) </rdfs:comment>
      <skos:definition xml:lang="en">The time limit for review procedures.
WG Approval 09/11/2021
 (epo:ReviewTerm) </skos:definition>
      <rdfs:isDefinedBy rdf:resource="http://data.europa.eu/a4g/ontology"/>
   </owl:DatatypeProperty>
   <owl:DatatypeProperty rdf:about="http://data.europa.eu/a4g/ontology#hasReviewDeadlineInformation">
      <rdfs:label xml:lang="en">Has review deadline information</rdfs:label>
      <skos:prefLabel xml:lang="en">Has review deadline information</skos:prefLabel>
      <rdfs:comment xml:lang="en">The description of the time limits for review procedures.

WG Approval 01/10/2019
 (epo:ReviewTerm) </rdfs:comment>
      <skos:definition xml:lang="en">The description of the time limits for review procedures.

WG Approval 01/10/2019
 (epo:ReviewTerm) </skos:definition>
      <rdfs:isDefinedBy rdf:resource="http://data.europa.eu/a4g/ontology"/>
   </owl:DatatypeProperty>
   <owl:DatatypeProperty rdf:about="http://data.europa.eu/a4g/ontology#hasReviewProcedure">
      <rdfs:label xml:lang="en">Has review procedure</rdfs:label>
      <skos:prefLabel xml:lang="en">Has review procedure</skos:prefLabel>
      <rdfs:comment xml:lang="en">The description of the method used to request the verification that the procedure has been carried out correctly.
WG Approval 09/11/2021 (epo:ReviewTerm) </rdfs:comment>
      <skos:definition xml:lang="en">The description of the method used to request the verification that the procedure has been carried out correctly.
WG Approval 09/11/2021 (epo:ReviewTerm) </skos:definition>
      <rdfs:isDefinedBy rdf:resource="http://data.europa.eu/a4g/ontology"/>
   </owl:DatatypeProperty>
   <owl:DatatypeProperty rdf:about="http://data.europa.eu/a4g/ontology#hasDeadline">
      <rdfs:label xml:lang="en">Has deadline</rdfs:label>
      <skos:prefLabel xml:lang="en">Has deadline</skos:prefLabel>
      <rdfs:comment xml:lang="en">The deadline by which the security clearance must be submitted to the buyer.

WG Approval 12/09/2019

 (epo:SecurityClearanceTerm) </rdfs:comment>
      <skos:definition xml:lang="en">The deadline by which the security clearance must be submitted to the buyer.

WG Approval 12/09/2019

 (epo:SecurityClearanceTerm) </skos:definition>
      <rdfs:isDefinedBy rdf:resource="http://data.europa.eu/a4g/ontology"/>
   </owl:DatatypeProperty>
   <owl:DatatypeProperty rdf:about="http://data.europa.eu/a4g/ontology#hasSelectionCriterionType">
      <rdfs:label xml:lang="en">Has selection criterion type</rdfs:label>
      <skos:prefLabel xml:lang="en">Has selection criterion type</skos:prefLabel>
      <rdfs:comment xml:lang="en">The classification of the selection criteria.
WG Approval 09/11/2021 (epo:SelectionCriterion) </rdfs:comment>
      <skos:definition xml:lang="en">The classification of the selection criteria.
WG Approval 09/11/2021 (epo:SelectionCriterion) </skos:definition>
      <rdfs:isDefinedBy rdf:resource="http://data.europa.eu/a4g/ontology"/>
   </owl:DatatypeProperty>
   <owl:DatatypeProperty rdf:about="http://data.europa.eu/a4g/ontology#hasWeightingJustification">
      <rdfs:label xml:lang="en">Has weighting justification</rdfs:label>
      <skos:prefLabel xml:lang="en">Has weighting justification</skos:prefLabel>
      <rdfs:comment xml:lang="en">Explanation about why the actual weighting model is chosen. 

Additional information: 
In eNotification: This property is specifically used to describe why the order of importance is used over another weighting model.
In ESPD: This is used to explain other complex models of weighting for transparency reasons. 

WG Approval 19/09/2019  (epo:SelectionCriterion) </rdfs:comment>
      <skos:definition xml:lang="en">Explanation about why the actual weighting model is chosen. 

Additional information: 
In eNotification: This property is specifically used to describe why the order of importance is used over another weighting model.
In ESPD: This is used to explain other complex models of weighting for transparency reasons. 

WG Approval 19/09/2019  (epo:SelectionCriterion) </skos:definition>
      <rdfs:isDefinedBy rdf:resource="http://data.europa.eu/a4g/ontology"/>
   </owl:DatatypeProperty>
   <owl:DatatypeProperty rdf:about="http://data.europa.eu/a4g/ontology#isUsedForCandidateRestriction">
      <rdfs:label xml:lang="en">Is used for candidate restriction</rdfs:label>
      <skos:prefLabel xml:lang="en">Is used for candidate restriction</skos:prefLabel>
      <rdfs:comment xml:lang="en">To be reviewed when treating criterion (epo:SelectionCriterion) </rdfs:comment>
      <skos:definition xml:lang="en">To be reviewed when treating criterion (epo:SelectionCriterion) </skos:definition>
      <rdfs:isDefinedBy rdf:resource="http://data.europa.eu/a4g/ontology"/>
   </owl:DatatypeProperty>
   <owl:DatatypeProperty rdf:about="http://data.europa.eu/a4g/ontology#hasAbnormallyLowTenderLots">
      <rdfs:label xml:lang="en">Has abnormally low tender lots</rdfs:label>
      <skos:prefLabel xml:lang="en">Has abnormally low tender lots</skos:prefLabel>
      <rdfs:comment xml:lang="en">Tenders received that were found irregular and non-acceptable due to an abnormally low price or cost.

Additional Information
The definition implies that abnormally Low Tender Lots are Inadmissible Tender Lots.

WG Approval 28/07/2020

 (epo:StatisticalInformation) </rdfs:comment>
      <skos:definition xml:lang="en">Tenders received that were found irregular and non-acceptable due to an abnormally low price or cost.

Additional Information
The definition implies that abnormally Low Tender Lots are Inadmissible Tender Lots.

WG Approval 28/07/2020

 (epo:StatisticalInformation) </skos:definition>
      <rdfs:isDefinedBy rdf:resource="http://data.europa.eu/a4g/ontology"/>
   </owl:DatatypeProperty>
   <owl:DatatypeProperty rdf:about="http://data.europa.eu/a4g/ontology#hasCleanVehicles">
      <rdfs:label xml:lang="en">Has clean vehicles</rdfs:label>
      <skos:prefLabel xml:lang="en">Has clean vehicles</skos:prefLabel>
      <rdfs:comment xml:lang="en">The number of all clean vehicles that have either been purchased, leased, rented, hired-purchased or their use has been contractually committed to for the provision of a purchased service.

Additional Information
In the European Union, the legal requirements and scope for the provision of these vehicles or services are covered by Directive 2009/33/EC.

WG Approval 28/07/2020
 (epo:StatisticalInformation) </rdfs:comment>
      <skos:definition xml:lang="en">The number of all clean vehicles that have either been purchased, leased, rented, hired-purchased or their use has been contractually committed to for the provision of a purchased service.

Additional Information
In the European Union, the legal requirements and scope for the provision of these vehicles or services are covered by Directive 2009/33/EC.

WG Approval 28/07/2020
 (epo:StatisticalInformation) </skos:definition>
      <rdfs:isDefinedBy rdf:resource="http://data.europa.eu/a4g/ontology"/>
   </owl:DatatypeProperty>
   <owl:DatatypeProperty rdf:about="http://data.europa.eu/a4g/ontology#hasEEAReceivedTenderLots">
      <rdfs:label xml:lang="en">Has e e a received tender lots</rdfs:label>
      <skos:prefLabel xml:lang="en">Has e e a received tender lots</skos:prefLabel>
      <rdfs:comment xml:lang="en">The amount of tenders received from economic operators in other EEA countries other than the country of the buyer.

WG Approval 12/12/2019 (epo:StatisticalInformation) </rdfs:comment>
      <skos:definition xml:lang="en">The amount of tenders received from economic operators in other EEA countries other than the country of the buyer.

WG Approval 12/12/2019 (epo:StatisticalInformation) </skos:definition>
      <rdfs:isDefinedBy rdf:resource="http://data.europa.eu/a4g/ontology"/>
   </owl:DatatypeProperty>
   <owl:DatatypeProperty rdf:about="http://data.europa.eu/a4g/ontology#hasElectronicTenderLots">
      <rdfs:label xml:lang="en">Has electronic tender lots</rdfs:label>
      <skos:prefLabel xml:lang="en">Has electronic tender lots</skos:prefLabel>
      <rdfs:comment xml:lang="en">Electronic Tender Lots received.

WG Approval 28/07/2020
 (epo:StatisticalInformation) </rdfs:comment>
      <skos:definition xml:lang="en">Electronic Tender Lots received.

WG Approval 28/07/2020
 (epo:StatisticalInformation) </skos:definition>
      <rdfs:isDefinedBy rdf:resource="http://data.europa.eu/a4g/ontology"/>
   </owl:DatatypeProperty>
   <owl:DatatypeProperty rdf:about="http://data.europa.eu/a4g/ontology#hasEstimatedTotalSubcontracts">
      <rdfs:label xml:lang="en">Has estimated total subcontracts</rdfs:label>
      <skos:prefLabel xml:lang="en">Has estimated total subcontracts</skos:prefLabel>
      <rdfs:comment xml:lang="en">The estimated amount of work to be subcontracted in the contract resulting from the lot.
WG Approval 09/11/2021 (epo:StatisticalInformation) </rdfs:comment>
      <skos:definition xml:lang="en">The estimated amount of work to be subcontracted in the contract resulting from the lot.
WG Approval 09/11/2021 (epo:StatisticalInformation) </skos:definition>
      <rdfs:isDefinedBy rdf:resource="http://data.europa.eu/a4g/ontology"/>
   </owl:DatatypeProperty>
   <owl:ObjectProperty rdf:about="http://data.europa.eu/a4g/ontology#hasHighestReceivedTenderLotValues">
      <rdfs:label xml:lang="en">Has highest received tender lot values</rdfs:label>
      <skos:prefLabel xml:lang="en">Has highest received tender lot values</skos:prefLabel>
      <rdfs:comment xml:lang="en">Amount of the Tender with the highest value.

Additional Information
The value must correspond to an admissible tender. For example, tenders compliant with the procurement document requirements, not having an abnormally low price or cost, etc. 


WG Approval 12/12/2019

 (epo:StatisticalInformation) </rdfs:comment>
      <skos:definition xml:lang="en">Amount of the Tender with the highest value.

Additional Information
The value must correspond to an admissible tender. For example, tenders compliant with the procurement document requirements, not having an abnormally low price or cost, etc. 


WG Approval 12/12/2019

 (epo:StatisticalInformation) </skos:definition>
      <rdfs:isDefinedBy rdf:resource="http://data.europa.eu/a4g/ontology"/>
   </owl:ObjectProperty>
   <owl:DatatypeProperty rdf:about="http://data.europa.eu/a4g/ontology#hasInadmissibleTenderLots">
      <rdfs:label xml:lang="en">Has inadmissible tender lots</rdfs:label>
      <skos:prefLabel xml:lang="en">Has inadmissible tender lots</skos:prefLabel>
      <rdfs:comment xml:lang="en">Tenders received that cannot be awarded  due to non-compliance to procurement document requirements or having an abnormally low price or cost.

&lt;u&gt;Additional Information: &lt;/u&gt;
Non-compliance with a Procurement Document requirements include exclusion grounds, selection criteria and submission deadline, etc.

WG Approval 12/12/2019 (epo:StatisticalInformation) </rdfs:comment>
      <skos:definition xml:lang="en">Tenders received that cannot be awarded  due to non-compliance to procurement document requirements or having an abnormally low price or cost.

&lt;u&gt;Additional Information: &lt;/u&gt;
Non-compliance with a Procurement Document requirements include exclusion grounds, selection criteria and submission deadline, etc.

WG Approval 12/12/2019 (epo:StatisticalInformation) </skos:definition>
      <rdfs:isDefinedBy rdf:resource="http://data.europa.eu/a4g/ontology"/>
   </owl:DatatypeProperty>
   <owl:ObjectProperty rdf:about="http://data.europa.eu/a4g/ontology#hasLowestReceivedTenderLotValues">
      <rdfs:label xml:lang="en">Has lowest received tender lot values</rdfs:label>
      <skos:prefLabel xml:lang="en">Has lowest received tender lot values</skos:prefLabel>
      <rdfs:comment xml:lang="en">Amount of the Tender with the lowest value.

Additional Information
The value must correspond to an admissible tender. For example, tenders compliant with the procurement document requirements, not having an abnormally low price or cost, etc. 

WG Approval 12/12/2019
 (epo:StatisticalInformation) </rdfs:comment>
      <skos:definition xml:lang="en">Amount of the Tender with the lowest value.

Additional Information
The value must correspond to an admissible tender. For example, tenders compliant with the procurement document requirements, not having an abnormally low price or cost, etc. 

WG Approval 12/12/2019
 (epo:StatisticalInformation) </skos:definition>
      <rdfs:isDefinedBy rdf:resource="http://data.europa.eu/a4g/ontology"/>
   </owl:ObjectProperty>
   <owl:DatatypeProperty rdf:about="http://data.europa.eu/a4g/ontology#hasMediumTenderPerLots">
      <rdfs:label xml:lang="en">Has medium tender per lots</rdfs:label>
      <skos:prefLabel xml:lang="en">Has medium tender per lots</skos:prefLabel>
      <rdfs:comment xml:lang="en">Tenders from medium-sized enterprise.

&lt;u&gt;Additional Information:&lt;/u&gt;

See Commission Recommendation 2003/361/EC.
 (epo:StatisticalInformation) </rdfs:comment>
      <skos:definition xml:lang="en">Tenders from medium-sized enterprise.

&lt;u&gt;Additional Information:&lt;/u&gt;

See Commission Recommendation 2003/361/EC.
 (epo:StatisticalInformation) </skos:definition>
      <rdfs:isDefinedBy rdf:resource="http://data.europa.eu/a4g/ontology"/>
   </owl:DatatypeProperty>
   <owl:DatatypeProperty rdf:about="http://data.europa.eu/a4g/ontology#hasNumberOfTenderersInvited">
      <rdfs:label xml:lang="en">Has number of tenderers invited</rdfs:label>
      <skos:prefLabel xml:lang="en">Has number of tenderers invited</skos:prefLabel>
      <rdfs:comment xml:lang="en">Number of economic operators invited to tender.

Additional Information
This may be used for single-stage procedures or to indicate the number of candidates invited to tender in multi-stage procedures.

WG Approval 01/12/2020

 (epo:StatisticalInformation) </rdfs:comment>
      <skos:definition xml:lang="en">Number of economic operators invited to tender.

Additional Information
This may be used for single-stage procedures or to indicate the number of candidates invited to tender in multi-stage procedures.

WG Approval 01/12/2020

 (epo:StatisticalInformation) </skos:definition>
      <rdfs:isDefinedBy rdf:resource="http://data.europa.eu/a4g/ontology"/>
   </owl:DatatypeProperty>
   <owl:DatatypeProperty rdf:about="http://data.europa.eu/a4g/ontology#hasReceivedMicroTenderLots">
      <rdfs:label xml:lang="en">Has received micro tender lots</rdfs:label>
      <skos:prefLabel xml:lang="en">Has received micro tender lots</skos:prefLabel>
      <rdfs:comment xml:lang="en">The amount of tenders received from a micro enterprise.

&lt;u&gt;Additional Information:&lt;/u&gt;

See Commission Recommendation 2003/361/EC. (epo:StatisticalInformation) </rdfs:comment>
      <skos:definition xml:lang="en">The amount of tenders received from a micro enterprise.

&lt;u&gt;Additional Information:&lt;/u&gt;

See Commission Recommendation 2003/361/EC. (epo:StatisticalInformation) </skos:definition>
      <rdfs:isDefinedBy rdf:resource="http://data.europa.eu/a4g/ontology"/>
   </owl:DatatypeProperty>
   <owl:DatatypeProperty rdf:about="http://data.europa.eu/a4g/ontology#hasReceivedNONEEATenderLots">
      <rdfs:label xml:lang="en">Has received n o n e e a tender lots</rdfs:label>
      <skos:prefLabel xml:lang="en">Has received n o n e e a tender lots</skos:prefLabel>
      <rdfs:comment xml:lang="en">The amount of tenders received from economic operators in non-EEA countries. 

WG Approval 12/12/2019 15:20:36 (epo:StatisticalInformation) </rdfs:comment>
      <skos:definition xml:lang="en">The amount of tenders received from economic operators in non-EEA countries. 

WG Approval 12/12/2019 15:20:36 (epo:StatisticalInformation) </skos:definition>
      <rdfs:isDefinedBy rdf:resource="http://data.europa.eu/a4g/ontology"/>
   </owl:DatatypeProperty>
   <owl:DatatypeProperty rdf:about="http://data.europa.eu/a4g/ontology#hasReceivedParticipationRequests">
      <rdfs:label xml:lang="en">Has received participation requests</rdfs:label>
      <skos:prefLabel xml:lang="en">Has received participation requests</skos:prefLabel>
      <rdfs:comment xml:lang="en">The amount of applications to participate from economic operators.

WG Approval 12/12/2019 (epo:StatisticalInformation) </rdfs:comment>
      <skos:definition xml:lang="en">The amount of applications to participate from economic operators.

WG Approval 12/12/2019 (epo:StatisticalInformation) </skos:definition>
      <rdfs:isDefinedBy rdf:resource="http://data.europa.eu/a4g/ontology"/>
   </owl:DatatypeProperty>
   <owl:DatatypeProperty rdf:about="http://data.europa.eu/a4g/ontology#hasReceivedReviewRequests">
      <rdfs:label xml:lang="en">Has received review requests</rdfs:label>
      <skos:prefLabel xml:lang="en">Has received review requests</skos:prefLabel>
      <rdfs:comment xml:lang="en">The number of economic operators that requested the buyer to review any of its decisions (e.g. the technical specifications, award decision), as set out in Art. 1(5) of Directive 89/665/EEC and Directive 92/13/EEC.

WG Approval 11/04/2019 (epo:StatisticalInformation) </rdfs:comment>
      <skos:definition xml:lang="en">The number of economic operators that requested the buyer to review any of its decisions (e.g. the technical specifications, award decision), as set out in Art. 1(5) of Directive 89/665/EEC and Directive 92/13/EEC.

WG Approval 11/04/2019 (epo:StatisticalInformation) </skos:definition>
      <rdfs:isDefinedBy rdf:resource="http://data.europa.eu/a4g/ontology"/>
   </owl:DatatypeProperty>
   <owl:DatatypeProperty rdf:about="http://data.europa.eu/a4g/ontology#hasReceivedSmallTenderLots">
      <rdfs:label xml:lang="en">Has received small tender lots</rdfs:label>
      <skos:prefLabel xml:lang="en">Has received small tender lots</skos:prefLabel>
      <rdfs:comment xml:lang="en">Tenders from small enterprise.

&lt;u&gt;Additional Information:&lt;/u&gt;

See Commission Recommendation 2003/361/EC.

 (epo:StatisticalInformation) </rdfs:comment>
      <skos:definition xml:lang="en">Tenders from small enterprise.

&lt;u&gt;Additional Information:&lt;/u&gt;

See Commission Recommendation 2003/361/EC.

 (epo:StatisticalInformation) </skos:definition>
      <rdfs:isDefinedBy rdf:resource="http://data.europa.eu/a4g/ontology"/>
   </owl:DatatypeProperty>
   <owl:DatatypeProperty rdf:about="http://data.europa.eu/a4g/ontology#hasReceivedSMETenderLots">
      <rdfs:label xml:lang="en">Has received s m e tender lots</rdfs:label>
      <skos:prefLabel xml:lang="en">Has received s m e tender lots</skos:prefLabel>
      <rdfs:comment xml:lang="en">The amount of tenders received from micro, small and medium-sized enterprises.

&lt;u&gt;Additional Information:&lt;/u&gt;

See Commission Recommendation 2003/361/EC. 
The ReceivedSMETenderLots is used when the size of the company is not exactly knokn.

WG Approval 05/03/2020
 (epo:StatisticalInformation) </rdfs:comment>
      <skos:definition xml:lang="en">The amount of tenders received from micro, small and medium-sized enterprises.

&lt;u&gt;Additional Information:&lt;/u&gt;

See Commission Recommendation 2003/361/EC. 
The ReceivedSMETenderLots is used when the size of the company is not exactly knokn.

WG Approval 05/03/2020
 (epo:StatisticalInformation) </skos:definition>
      <rdfs:isDefinedBy rdf:resource="http://data.europa.eu/a4g/ontology"/>
   </owl:DatatypeProperty>
   <owl:DatatypeProperty rdf:about="http://data.europa.eu/a4g/ontology#hasReceivedTenderLots">
      <rdfs:label xml:lang="en">Has received tender lots</rdfs:label>
      <skos:prefLabel xml:lang="en">Has received tender lots</skos:prefLabel>
      <rdfs:comment xml:lang="en">The total amount of tenders received.

WG Approval 12/12/2019 (epo:StatisticalInformation) </rdfs:comment>
      <skos:definition xml:lang="en">The total amount of tenders received.

WG Approval 12/12/2019 (epo:StatisticalInformation) </skos:definition>
      <rdfs:isDefinedBy rdf:resource="http://data.europa.eu/a4g/ontology"/>
   </owl:DatatypeProperty>
   <owl:DatatypeProperty rdf:about="http://data.europa.eu/a4g/ontology#hasSubcontractShareSubjectMatter">
      <rdfs:label xml:lang="en">Has subcontract share subject matter</rdfs:label>
      <skos:prefLabel xml:lang="en">Has subcontract share subject matter</skos:prefLabel>
      <rdfs:comment xml:lang="en">Description of the share of the contract that is to be subcontracted. 

Additional infromation:
This can be an aggregate of several subcontracts.

WG Approval 09/11/2021 (epo:StatisticalInformation) </rdfs:comment>
      <skos:definition xml:lang="en">Description of the share of the contract that is to be subcontracted. 

Additional infromation:
This can be an aggregate of several subcontracts.

WG Approval 09/11/2021 (epo:StatisticalInformation) </skos:definition>
      <rdfs:isDefinedBy rdf:resource="http://data.europa.eu/a4g/ontology"/>
   </owl:DatatypeProperty>
   <owl:DatatypeProperty rdf:about="http://data.europa.eu/a4g/ontology#hasTotalVehicles">
      <rdfs:label xml:lang="en">Has total vehicles</rdfs:label>
      <skos:prefLabel xml:lang="en">Has total vehicles</skos:prefLabel>
      <rdfs:comment xml:lang="en">The number of all vehicles (regardless of whether clean or not) that have either been purchased, leased, rented, hired-purchased or their use has been contractually committed to for the provision of a purchased service.

Additional Information

In the European Union, the legal requirements and scope for the provision of these vehicles or services are covered by Directive 2009/33/EC.

WG Approval 28/07/2020
 (epo:StatisticalInformation) </rdfs:comment>
      <skos:definition xml:lang="en">The number of all vehicles (regardless of whether clean or not) that have either been purchased, leased, rented, hired-purchased or their use has been contractually committed to for the provision of a purchased service.

Additional Information

In the European Union, the legal requirements and scope for the provision of these vehicles or services are covered by Directive 2009/33/EC.

WG Approval 28/07/2020
 (epo:StatisticalInformation) </skos:definition>
      <rdfs:isDefinedBy rdf:resource="http://data.europa.eu/a4g/ontology"/>
   </owl:DatatypeProperty>
   <owl:DatatypeProperty rdf:about="http://data.europa.eu/a4g/ontology#hasUnverifiedTenderLots">
      <rdfs:label xml:lang="en">Has unverified tender lots</rdfs:label>
      <skos:prefLabel xml:lang="en">Has unverified tender lots</skos:prefLabel>
      <rdfs:comment xml:lang="en">Offers received for which it has not been verified if they are admissible or inadmissible (e.g. because award criteria have been evaluated for all tenders and admissibility is checked only for the winning tender).

WG Approval 28/07/2020
 (epo:StatisticalInformation) </rdfs:comment>
      <skos:definition xml:lang="en">Offers received for which it has not been verified if they are admissible or inadmissible (e.g. because award criteria have been evaluated for all tenders and admissibility is checked only for the winning tender).

WG Approval 28/07/2020
 (epo:StatisticalInformation) </skos:definition>
      <rdfs:isDefinedBy rdf:resource="http://data.europa.eu/a4g/ontology"/>
   </owl:DatatypeProperty>
   <owl:DatatypeProperty rdf:about="http://data.europa.eu/a4g/ontology#hasZeroEmissionVehicles">
      <rdfs:label xml:lang="en">Has zero emission vehicles</rdfs:label>
      <skos:prefLabel xml:lang="en">Has zero emission vehicles</skos:prefLabel>
      <rdfs:comment xml:lang="en">The number of all zero-emission heavy-duty vehicles that have either been purchased, leased, rented, hired-purchased or their use has been contractually committed to for the provision of a purchased service.

Additional Information

In the European Union, the legal requirements and scope for the provision of these vehicles or services are covered by Directive 2009/33/EC.

WG Approval 28/07/2020
 (epo:StatisticalInformation) </rdfs:comment>
      <skos:definition xml:lang="en">The number of all zero-emission heavy-duty vehicles that have either been purchased, leased, rented, hired-purchased or their use has been contractually committed to for the provision of a purchased service.

Additional Information

In the European Union, the legal requirements and scope for the provision of these vehicles or services are covered by Directive 2009/33/EC.

WG Approval 28/07/2020
 (epo:StatisticalInformation) </skos:definition>
      <rdfs:isDefinedBy rdf:resource="http://data.europa.eu/a4g/ontology"/>
   </owl:DatatypeProperty>
   <owl:DatatypeProperty rdf:about="http://data.europa.eu/a4g/ontology#hasStrategicProcurementDescription">
      <rdfs:label xml:lang="en">Has strategic procurement description</rdfs:label>
      <skos:prefLabel xml:lang="en">Has strategic procurement description</skos:prefLabel>
      <rdfs:comment xml:lang="en">Self-explanatory text about a concept.
 (epo:StrategicProcurement) </rdfs:comment>
      <skos:definition xml:lang="en">Self-explanatory text about a concept.
 (epo:StrategicProcurement) </skos:definition>
      <rdfs:isDefinedBy rdf:resource="http://data.europa.eu/a4g/ontology"/>
   </owl:DatatypeProperty>
   <owl:DatatypeProperty rdf:about="http://data.europa.eu/a4g/ontology#hasEstimatedShare">
      <rdfs:label xml:lang="en">Has estimated share</rdfs:label>
      <skos:prefLabel xml:lang="en">Has estimated share</skos:prefLabel>
      <rdfs:comment xml:lang="en">The estimated proportion foreseen to be subcontracted.

WG Approval 07/01/2020 (epo:Subcontract) </rdfs:comment>
      <skos:definition xml:lang="en">The estimated proportion foreseen to be subcontracted.

WG Approval 07/01/2020 (epo:Subcontract) </skos:definition>
      <rdfs:isDefinedBy rdf:resource="http://data.europa.eu/a4g/ontology"/>
   </owl:DatatypeProperty>
   <owl:DatatypeProperty rdf:about="http://data.europa.eu/a4g/ontology#hasMaximumShare">
      <rdfs:label xml:lang="en">Has maximum share</rdfs:label>
      <skos:prefLabel xml:lang="en">Has maximum share</skos:prefLabel>
      <rdfs:comment xml:lang="en">The maximum proportion of something to be distributed.

Additional Information:
In the case of subcontracting the share may refer to the proportion of works, services or supplies being subcontracted.

WG Approval 17/09/2019 

 (epo:SubcontractTerm) </rdfs:comment>
      <skos:definition xml:lang="en">The maximum proportion of something to be distributed.

Additional Information:
In the case of subcontracting the share may refer to the proportion of works, services or supplies being subcontracted.

WG Approval 17/09/2019 

 (epo:SubcontractTerm) </skos:definition>
      <rdfs:isDefinedBy rdf:resource="http://data.europa.eu/a4g/ontology"/>
   </owl:DatatypeProperty>
   <owl:DatatypeProperty rdf:about="http://data.europa.eu/a4g/ontology#hasMinimumShare">
      <rdfs:label xml:lang="en">Has minimum share</rdfs:label>
      <skos:prefLabel xml:lang="en">Has minimum share</skos:prefLabel>
      <rdfs:comment xml:lang="en">The minimum proportion of something to be distributed.

Additional Information:
In the case of subcontracting the share may refer to the proportion of works, services or supplies being subcontracted.

WG Approval 17/09/2019 (epo:SubcontractTerm) </rdfs:comment>
      <skos:definition xml:lang="en">The minimum proportion of something to be distributed.

Additional Information:
In the case of subcontracting the share may refer to the proportion of works, services or supplies being subcontracted.

WG Approval 17/09/2019 (epo:SubcontractTerm) </skos:definition>
      <rdfs:isDefinedBy rdf:resource="http://data.europa.eu/a4g/ontology"/>
   </owl:DatatypeProperty>
   <owl:DatatypeProperty rdf:about="http://data.europa.eu/a4g/ontology#hasMinimumSubcontractorsProposedObligation">
      <rdfs:label xml:lang="en">Has minimum subcontractors proposed obligation</rdfs:label>
      <skos:prefLabel xml:lang="en">Has minimum subcontractors proposed obligation</skos:prefLabel>
      <rdfs:comment xml:lang="en">The minimum percentage of the contract value that the contractor must subcontract.

Additional information:
This is used for the competitive procedure described in Title III of Directive 2009/81/EC. 

WG Approval 09/11/2021 (epo:SubcontractTerm) </rdfs:comment>
      <skos:definition xml:lang="en">The minimum percentage of the contract value that the contractor must subcontract.

Additional information:
This is used for the competitive procedure described in Title III of Directive 2009/81/EC. 

WG Approval 09/11/2021 (epo:SubcontractTerm) </skos:definition>
      <rdfs:isDefinedBy rdf:resource="http://data.europa.eu/a4g/ontology"/>
   </owl:DatatypeProperty>
   <owl:DatatypeProperty rdf:about="http://data.europa.eu/a4g/ontology#hasSubcontractingInvolved">
      <rdfs:label xml:lang="en">Has subcontracting involved</rdfs:label>
      <skos:prefLabel xml:lang="en">Has subcontracting involved</skos:prefLabel>
      <rdfs:comment xml:lang="en">List of Subcontractors and the subject matter they cover are required.

Additional Information: 
The tenderer will ned to supply this information in the tender.

WG Approval 28/02/2019 (epo:SubcontractTerm) </rdfs:comment>
      <skos:definition xml:lang="en">List of Subcontractors and the subject matter they cover are required.

Additional Information: 
The tenderer will ned to supply this information in the tender.

WG Approval 28/02/2019 (epo:SubcontractTerm) </skos:definition>
      <rdfs:isDefinedBy rdf:resource="http://data.europa.eu/a4g/ontology"/>
   </owl:DatatypeProperty>
   <owl:DatatypeProperty rdf:about="http://data.europa.eu/a4g/ontology#hasSubcontractingObligation">
      <rdfs:label xml:lang="en">Has subcontracting obligation</rdfs:label>
      <skos:prefLabel xml:lang="en">Has subcontracting obligation</skos:prefLabel>
      <rdfs:comment xml:lang="en">The requirement the tender must meet with regard to subcontracting parts of the contract.
WG Approval 09/11/2021 (epo:SubcontractTerm) </rdfs:comment>
      <skos:definition xml:lang="en">The requirement the tender must meet with regard to subcontracting parts of the contract.
WG Approval 09/11/2021 (epo:SubcontractTerm) </skos:definition>
      <rdfs:isDefinedBy rdf:resource="http://data.europa.eu/a4g/ontology"/>
   </owl:DatatypeProperty>
   <owl:DatatypeProperty rdf:about="http://data.europa.eu/a4g/ontology#hasSubcontractorsProposedAboveObligation">
      <rdfs:label xml:lang="en">Has subcontractors proposed above obligation</rdfs:label>
      <skos:prefLabel xml:lang="en">Has subcontractors proposed above obligation</skos:prefLabel>
      <rdfs:comment xml:lang="en">The maximum percentage of the contract value that the contractor must subcontract.

Additional information:
This is used for the competitive procedure described in Title III of Directive 2009/81/EC. 

WG Approval 09/11/2021 (epo:SubcontractTerm) </rdfs:comment>
      <skos:definition xml:lang="en">The maximum percentage of the contract value that the contractor must subcontract.

Additional information:
This is used for the competitive procedure described in Title III of Directive 2009/81/EC. 

WG Approval 09/11/2021 (epo:SubcontractTerm) </skos:definition>
      <rdfs:isDefinedBy rdf:resource="http://data.europa.eu/a4g/ontology"/>
   </owl:DatatypeProperty>
   <owl:DatatypeProperty rdf:about="http://data.europa.eu/a4g/ontology#hasAdvancedElectronicSignatureRequired">
      <rdfs:label xml:lang="en">Has advanced electronic signature required</rdfs:label>
      <skos:prefLabel xml:lang="en">Has advanced electronic signature required</skos:prefLabel>
      <rdfs:comment xml:lang="en">Advanced or qualified electronic signature or seal (as defined in Regulation (EU) No 910/2014) is required.



The submitted information is required to be signed electronically.

Additional Information: 

Signature can be defined as "data in electronic form which is attached to or logically associated with other data in electronic form and which is used by the signatory to sign. 
For more details on the meaning and uses of electronic signature you may consult different authoritative sources, a relevant one being for instance the Regulation (EU) 910/2014 on electronic identification and trust services for electronic transactions in the internal market.

WG Approval 21/07/2020
 (epo:SubmissionTerm) </rdfs:comment>
      <skos:definition xml:lang="en">Advanced or qualified electronic signature or seal (as defined in Regulation (EU) No 910/2014) is required.



The submitted information is required to be signed electronically.

Additional Information: 

Signature can be defined as "data in electronic form which is attached to or logically associated with other data in electronic form and which is used by the signatory to sign. 
For more details on the meaning and uses of electronic signature you may consult different authoritative sources, a relevant one being for instance the Regulation (EU) 910/2014 on electronic identification and trust services for electronic transactions in the internal market.

WG Approval 21/07/2020
 (epo:SubmissionTerm) </skos:definition>
      <rdfs:isDefinedBy rdf:resource="http://data.europa.eu/a4g/ontology"/>
   </owl:DatatypeProperty>
   <owl:DatatypeProperty rdf:about="http://data.europa.eu/a4g/ontology#hasECataloguePermission">
      <rdfs:label xml:lang="en">Has e catalogue permission</rdfs:label>
      <skos:prefLabel xml:lang="en">Has e catalogue permission</skos:prefLabel>
      <rdfs:comment xml:lang="en">The extent to which electronic catalogues may be used in tenders.

WG Approval 03/10/2019 (epo:SubmissionTerm) </rdfs:comment>
      <skos:definition xml:lang="en">The extent to which electronic catalogues may be used in tenders.

WG Approval 03/10/2019 (epo:SubmissionTerm) </skos:definition>
      <rdfs:isDefinedBy rdf:resource="http://data.europa.eu/a4g/ontology"/>
   </owl:DatatypeProperty>
   <owl:DatatypeProperty rdf:about="http://data.europa.eu/a4g/ontology#hasESubmissionPermission">
      <rdfs:label xml:lang="en">Has e submission permission</rdfs:label>
      <skos:prefLabel xml:lang="en">Has e submission permission</skos:prefLabel>
      <rdfs:comment xml:lang="en">The requirements as to what extent electronic submission is allowed.

WG Approval 03/10/2019 (epo:SubmissionTerm) </rdfs:comment>
      <skos:definition xml:lang="en">The requirements as to what extent electronic submission is allowed.

WG Approval 03/10/2019 (epo:SubmissionTerm) </skos:definition>
      <rdfs:isDefinedBy rdf:resource="http://data.europa.eu/a4g/ontology"/>
   </owl:DatatypeProperty>
   <owl:DatatypeProperty rdf:about="http://data.europa.eu/a4g/ontology#hasGuaranteeDescription">
      <rdfs:label xml:lang="en">Has guarantee description</rdfs:label>
      <skos:prefLabel xml:lang="en">Has guarantee description</skos:prefLabel>
      <rdfs:comment xml:lang="en">Information on the financial commitment required from the economic operator. 

Additional Information:
1.  This information may include the amount and the way of delivering of the guarantee
2. The financial commitment may be retained by the buyer in the case the tenderer withdraws the submitted information (i.e. tender, expression of interest and request for participation, but not request for clarifications) before the award of the contract or does not sign the contract.
3. Usual modalities are bonds, cheques, loans, other.

WG Approval 21/07/20
 (epo:SubmissionTerm) </rdfs:comment>
      <skos:definition xml:lang="en">Information on the financial commitment required from the economic operator. 

Additional Information:
1.  This information may include the amount and the way of delivering of the guarantee
2. The financial commitment may be retained by the buyer in the case the tenderer withdraws the submitted information (i.e. tender, expression of interest and request for participation, but not request for clarifications) before the award of the contract or does not sign the contract.
3. Usual modalities are bonds, cheques, loans, other.

WG Approval 21/07/20
 (epo:SubmissionTerm) </skos:definition>
      <rdfs:isDefinedBy rdf:resource="http://data.europa.eu/a4g/ontology"/>
   </owl:DatatypeProperty>
   <owl:DatatypeProperty rdf:about="http://data.europa.eu/a4g/ontology#hasGuaranteeRequired">
      <rdfs:label xml:lang="en">Has guarantee required</rdfs:label>
      <skos:prefLabel xml:lang="en">Has guarantee required</skos:prefLabel>
      <rdfs:comment xml:lang="en">The submitted information must include a financial commitment to be used in case of default.

Additional Information:
See the additional information provided in  the definition of the 'Guarantee Description' element.

WG Approval 21/07/20

 (epo:SubmissionTerm) </rdfs:comment>
      <skos:definition xml:lang="en">The submitted information must include a financial commitment to be used in case of default.

Additional Information:
See the additional information provided in  the definition of the 'Guarantee Description' element.

WG Approval 21/07/20

 (epo:SubmissionTerm) </skos:definition>
      <rdfs:isDefinedBy rdf:resource="http://data.europa.eu/a4g/ontology"/>
   </owl:DatatypeProperty>
   <owl:DatatypeProperty rdf:about="http://data.europa.eu/a4g/ontology#hasLanguage">
      <rdfs:label xml:lang="en">Has language</rdfs:label>
      <skos:prefLabel xml:lang="en">Has language</skos:prefLabel>
      <rdfs:comment xml:lang="en">Language in which the submitted information is to be expressed. 

WG Approval 21/07/2020
 (epo:SubmissionTerm) </rdfs:comment>
      <skos:definition xml:lang="en">Language in which the submitted information is to be expressed. 

WG Approval 21/07/2020
 (epo:SubmissionTerm) </skos:definition>
      <rdfs:isDefinedBy rdf:resource="http://data.europa.eu/a4g/ontology"/>
   </owl:DatatypeProperty>
   <owl:DatatypeProperty rdf:about="http://data.europa.eu/a4g/ontology#hasLateSubmissionInformationDescription">
      <rdfs:label xml:lang="en">Has late submission information description</rdfs:label>
      <skos:prefLabel xml:lang="en">Has late submission information description</skos:prefLabel>
      <rdfs:comment xml:lang="en">A narrative text explaining the content of the economic operator information that can be submitted late.

Additional Information
This does not apply to requests for clarifications.
 (epo:SubmissionTerm) </rdfs:comment>
      <skos:definition xml:lang="en">A narrative text explaining the content of the economic operator information that can be submitted late.

Additional Information
This does not apply to requests for clarifications.
 (epo:SubmissionTerm) </skos:definition>
      <rdfs:isDefinedBy rdf:resource="http://data.europa.eu/a4g/ontology"/>
   </owl:DatatypeProperty>
   <owl:DatatypeProperty rdf:about="http://data.europa.eu/a4g/ontology#hasLateSubmissionPermission">
      <rdfs:label xml:lang="en">Has late submission permission</rdfs:label>
      <skos:prefLabel xml:lang="en">Has late submission permission</skos:prefLabel>
      <rdfs:comment xml:lang="en">Whether economic operator-related information can be supplemented even after the submission deadline.

Additional Information
This is specific to the information on the economic operator and not the actual offer. This does  not apply to the requests for clarification.

WG Approval 21/07/2020 (epo:SubmissionTerm) </rdfs:comment>
      <skos:definition xml:lang="en">Whether economic operator-related information can be supplemented even after the submission deadline.

Additional Information
This is specific to the information on the economic operator and not the actual offer. This does  not apply to the requests for clarification.

WG Approval 21/07/2020 (epo:SubmissionTerm) </skos:definition>
      <rdfs:isDefinedBy rdf:resource="http://data.europa.eu/a4g/ontology"/>
   </owl:DatatypeProperty>
   <owl:DatatypeProperty rdf:about="http://data.europa.eu/a4g/ontology#hasMultipleTenderSubmissionAllowed">
      <rdfs:label xml:lang="en">Has multiple tender submission allowed</rdfs:label>
      <skos:prefLabel xml:lang="en">Has multiple tender submission allowed</skos:prefLabel>
      <rdfs:comment xml:lang="en">Tenderers may submit more than one competing tenders.

WG Approval 10/10/2019

 (epo:SubmissionTerm) </rdfs:comment>
      <skos:definition xml:lang="en">Tenderers may submit more than one competing tenders.

WG Approval 10/10/2019

 (epo:SubmissionTerm) </skos:definition>
      <rdfs:isDefinedBy rdf:resource="http://data.europa.eu/a4g/ontology"/>
   </owl:DatatypeProperty>
   <owl:DatatypeProperty rdf:about="http://data.europa.eu/a4g/ontology#hasNonElectronicSubmissionDescription">
      <rdfs:label xml:lang="en">Has non electronic submission description</rdfs:label>
      <skos:prefLabel xml:lang="en">Has non electronic submission description</skos:prefLabel>
      <rdfs:comment xml:lang="en">Textual explanation of how non-electronic information is to be presented.

WG Approval 21/07/2020

 (epo:SubmissionTerm) </rdfs:comment>
      <skos:definition xml:lang="en">Textual explanation of how non-electronic information is to be presented.

WG Approval 21/07/2020

 (epo:SubmissionTerm) </skos:definition>
      <rdfs:isDefinedBy rdf:resource="http://data.europa.eu/a4g/ontology"/>
   </owl:DatatypeProperty>
   <owl:DatatypeProperty rdf:about="http://data.europa.eu/a4g/ontology#hasNonElectronicSubmissionJustification">
      <rdfs:label xml:lang="en">Has non electronic submission justification</rdfs:label>
      <skos:prefLabel xml:lang="en">Has non electronic submission justification</skos:prefLabel>
      <rdfs:comment xml:lang="en">Reason for not accepting electronic information.

WG Approval 21/07/2020 (epo:SubmissionTerm) </rdfs:comment>
      <skos:definition xml:lang="en">Reason for not accepting electronic information.

WG Approval 21/07/2020 (epo:SubmissionTerm) </skos:definition>
      <rdfs:isDefinedBy rdf:resource="http://data.europa.eu/a4g/ontology"/>
   </owl:DatatypeProperty>
   <owl:DatatypeProperty rdf:about="http://data.europa.eu/a4g/ontology#hasReceiptDeadline">
      <rdfs:label xml:lang="en">Has receipt deadline</rdfs:label>
      <skos:prefLabel xml:lang="en">Has receipt deadline</skos:prefLabel>
      <rdfs:comment xml:lang="en">The time limit for receiving submissions.

Additional Information
This is the  deadline by which the buyer must receive submissions (e.g. tenders, requests to participate, clarifications, etc.) and is not the time at which the information is submitted by the economic operator.

WG Approval 21/07/2020
 (epo:SubmissionTerm) </rdfs:comment>
      <skos:definition xml:lang="en">The time limit for receiving submissions.

Additional Information
This is the  deadline by which the buyer must receive submissions (e.g. tenders, requests to participate, clarifications, etc.) and is not the time at which the information is submitted by the economic operator.

WG Approval 21/07/2020
 (epo:SubmissionTerm) </skos:definition>
      <rdfs:isDefinedBy rdf:resource="http://data.europa.eu/a4g/ontology"/>
   </owl:DatatypeProperty>
   <owl:DatatypeProperty rdf:about="http://data.europa.eu/a4g/ontology#hasTenderSubcontractingInformation">
      <rdfs:label xml:lang="en">Has tender subcontracting information</rdfs:label>
      <skos:prefLabel xml:lang="en">Has tender subcontracting information</skos:prefLabel>
      <rdfs:comment xml:lang="en">The information about subcontracting that must be indicated in the tender.

WG  Approval 10/10/2019 (epo:SubmissionTerm) </rdfs:comment>
      <skos:definition xml:lang="en">The information about subcontracting that must be indicated in the tender.

WG  Approval 10/10/2019 (epo:SubmissionTerm) </skos:definition>
      <rdfs:isDefinedBy rdf:resource="http://data.europa.eu/a4g/ontology"/>
   </owl:DatatypeProperty>
   <owl:DatatypeProperty rdf:about="http://data.europa.eu/a4g/ontology#hasAccessibilityCriterion">
      <rdfs:label xml:lang="en">Has accessibility criterion</rdfs:label>
      <skos:prefLabel xml:lang="en">Has accessibility criterion</skos:prefLabel>
      <rdfs:comment xml:lang="en">Explanation as to whether accessibility Criterion are used or not.
WG Approval 09/11/2021 (epo:TechnicalSpecification) </rdfs:comment>
      <skos:definition xml:lang="en">Explanation as to whether accessibility Criterion are used or not.
WG Approval 09/11/2021 (epo:TechnicalSpecification) </skos:definition>
      <rdfs:isDefinedBy rdf:resource="http://data.europa.eu/a4g/ontology"/>
   </owl:DatatypeProperty>
   <owl:DatatypeProperty rdf:about="http://data.europa.eu/a4g/ontology#hasNonAccessibilityCriterionJustification">
      <rdfs:label xml:lang="en">Has non accessibility criterion justification</rdfs:label>
      <skos:prefLabel xml:lang="en">Has non accessibility criterion justification</skos:prefLabel>
      <rdfs:comment xml:lang="en">Reason for not applying accessibility criteria.

WG Approval 05/03/2019 (epo:TechnicalSpecification) </rdfs:comment>
      <skos:definition xml:lang="en">Reason for not applying accessibility criteria.

WG Approval 05/03/2019 (epo:TechnicalSpecification) </skos:definition>
      <rdfs:isDefinedBy rdf:resource="http://data.europa.eu/a4g/ontology"/>
   </owl:DatatypeProperty>
   <owl:DatatypeProperty rdf:about="http://data.europa.eu/a4g/ontology#hasElectronicSubmission">
      <rdfs:label xml:lang="en">Has electronic submission</rdfs:label>
      <skos:prefLabel xml:lang="en">Has electronic submission</skos:prefLabel>
      <rdfs:comment xml:lang="en">Transmission of tenders is possible by electronic means of communication.  (epo:Tender) </rdfs:comment>
      <skos:definition xml:lang="en">Transmission of tenders is possible by electronic means of communication.  (epo:Tender) </skos:definition>
      <rdfs:isDefinedBy rdf:resource="http://data.europa.eu/a4g/ontology"/>
   </owl:DatatypeProperty>
   <owl:DatatypeProperty rdf:about="http://data.europa.eu/a4g/ontology#hasVariant">
      <rdfs:label xml:lang="en">Has variant</rdfs:label>
      <skos:prefLabel xml:lang="en">Has variant</skos:prefLabel>
      <rdfs:comment xml:lang="en">Alternative solution to fulfil the buyer's needs as opposed to solutions indicated in the procurement documents.

Additional Information:

The permission to offer variants is only allowed if specified in a Contract Notice or a Prior Information Notice that used as a means for calling for a competition.
The buyer lays out minimum requirements in the procurement documents that must be respected by tenderers submitting variants.

WG Approval 29/05/2019

 (epo:TenderLot) </rdfs:comment>
      <skos:definition xml:lang="en">Alternative solution to fulfil the buyer's needs as opposed to solutions indicated in the procurement documents.

Additional Information:

The permission to offer variants is only allowed if specified in a Contract Notice or a Prior Information Notice that used as a means for calling for a competition.
The buyer lays out minimum requirements in the procurement documents that must be respected by tenderers submitting variants.

WG Approval 29/05/2019

 (epo:TenderLot) </skos:definition>
      <rdfs:isDefinedBy rdf:resource="http://data.europa.eu/a4g/ontology"/>
   </owl:DatatypeProperty>
   <owl:DatatypeProperty rdf:about="http://data.europa.eu/a4g/ontology#hasRankingInFirstStage">
      <rdfs:label xml:lang="en">Has ranking in first stage</rdfs:label>
      <skos:prefLabel xml:lang="en">Has ranking in first stage</skos:prefLabel>
      <rdfs:comment xml:lang="en">The rank of the tender at the end of the selection phase of a multi-stage procedure. 

WG Approval 09/11/2021 (epo:TenderLotEvaluationRank) </rdfs:comment>
      <skos:definition xml:lang="en">The rank of the tender at the end of the selection phase of a multi-stage procedure. 

WG Approval 09/11/2021 (epo:TenderLotEvaluationRank) </skos:definition>
      <rdfs:isDefinedBy rdf:resource="http://data.europa.eu/a4g/ontology"/>
   </owl:DatatypeProperty>
   <owl:DatatypeProperty rdf:about="http://data.europa.eu/a4g/ontology#hasTenderLotRank">
      <rdfs:label xml:lang="en">Has tender lot rank</rdfs:label>
      <skos:prefLabel xml:lang="en">Has tender lot rank</skos:prefLabel>
      <rdfs:comment xml:lang="en">If there's no first stage then there is only a final stage.

 (epo:TenderLotEvaluationRank) </rdfs:comment>
      <skos:definition xml:lang="en">If there's no first stage then there is only a final stage.

 (epo:TenderLotEvaluationRank) </skos:definition>
      <rdfs:isDefinedBy rdf:resource="http://data.europa.eu/a4g/ontology"/>
   </owl:DatatypeProperty>
   <owl:DatatypeProperty rdf:about="http://data.europa.eu/a4g/ontology#hasCalculationMethod">
      <rdfs:label xml:lang="en">Has calculation method</rdfs:label>
      <skos:prefLabel xml:lang="en">Has calculation method</skos:prefLabel>
      <rdfs:comment xml:lang="en">Formula for obtaining values.

Additional Information:
The possible values are monetary values, ranking scores, criterion weighting.

WG Approval 25/05/2018 (epo:Value) </rdfs:comment>
      <skos:definition xml:lang="en">Formula for obtaining values.

Additional Information:
The possible values are monetary values, ranking scores, criterion weighting.

WG Approval 25/05/2018 (epo:Value) </skos:definition>
      <rdfs:isDefinedBy rdf:resource="http://data.europa.eu/a4g/ontology"/>
   </owl:DatatypeProperty>
   <owl:ObjectProperty rdf:about="http://data.europa.eu/a4g/ontology#hasMaximumAmount">
      <rdfs:label xml:lang="en">Has maximum amount</rdfs:label>
      <skos:prefLabel xml:lang="en">Has maximum amount</skos:prefLabel>
      <rdfs:comment xml:lang="en">The highest amount which can be spent within a procurement over its whole duration.

WG Approval 11/10/2019 (epo:Value) </rdfs:comment>
      <skos:definition xml:lang="en">The highest amount which can be spent within a procurement over its whole duration.

WG Approval 11/10/2019 (epo:Value) </skos:definition>
      <rdfs:isDefinedBy rdf:resource="http://data.europa.eu/a4g/ontology"/>
   </owl:ObjectProperty>
   <owl:ObjectProperty rdf:about="http://data.europa.eu/a4g/ontology#hasMinimumAmount">
      <rdfs:label xml:lang="en">Has minimum amount</rdfs:label>
      <skos:prefLabel xml:lang="en">Has minimum amount</skos:prefLabel>
      <rdfs:comment xml:lang="en">Post-poned until  discussion on lots values and amounts

WG approval 22/04/2021
 (epo:Value) </rdfs:comment>
      <skos:definition xml:lang="en">Post-poned until  discussion on lots values and amounts

WG approval 22/04/2021
 (epo:Value) </skos:definition>
      <rdfs:isDefinedBy rdf:resource="http://data.europa.eu/a4g/ontology"/>
   </owl:ObjectProperty>
   <owl:ObjectProperty rdf:about="http://data.europa.eu/a4g/ontology#hasOverallAmount">
      <rdfs:label xml:lang="en">Has overall amount</rdfs:label>
      <skos:prefLabel xml:lang="en">Has overall amount</skos:prefLabel>
      <rdfs:comment xml:lang="en">In the case of a procurement procedure it includes options and renewals.
 (epo:Value) </rdfs:comment>
      <skos:definition xml:lang="en">In the case of a procurement procedure it includes options and renewals.
 (epo:Value) </skos:definition>
      <rdfs:isDefinedBy rdf:resource="http://data.europa.eu/a4g/ontology"/>
   </owl:ObjectProperty>
   <owl:DatatypeProperty rdf:about="http://data.europa.eu/a4g/ontology#hasVATIncludedIndicator">
      <rdfs:label xml:lang="en">Has v a t included indicator</rdfs:label>
      <skos:prefLabel xml:lang="en">Has v a t included indicator</skos:prefLabel>
      <rdfs:comment xml:lang="en">Post-poned until  discussion on lots values and amounts

WG approval 22/04/2021
 (epo:Value) </rdfs:comment>
      <skos:definition xml:lang="en">Post-poned until  discussion on lots values and amounts

WG approval 22/04/2021
 (epo:Value) </skos:definition>
      <rdfs:isDefinedBy rdf:resource="http://data.europa.eu/a4g/ontology"/>
   </owl:DatatypeProperty>
   <owl:DatatypeProperty rdf:about="http://data.europa.eu/a4g/ontology#hasVATPercentage">
      <rdfs:label xml:lang="en">Has v a t percentage</rdfs:label>
      <skos:prefLabel xml:lang="en">Has v a t percentage</skos:prefLabel>
      <rdfs:comment xml:lang="en">Post-poned until  discussion on lots values and amounts

WG approval 22/04/2021 (epo:Value) </rdfs:comment>
      <skos:definition xml:lang="en">Post-poned until  discussion on lots values and amounts

WG approval 22/04/2021 (epo:Value) </skos:definition>
      <rdfs:isDefinedBy rdf:resource="http://data.europa.eu/a4g/ontology"/>
   </owl:DatatypeProperty>
   <owl:DatatypeProperty rdf:about="http://data.europa.eu/a4g/ontology#addressArea">
      <rdfs:label xml:lang="en">Address area</rdfs:label>
      <skos:prefLabel xml:lang="en">Address area</skos:prefLabel>
      <rdfs:comment xml:lang="en">The name or names of a geographic area or locality that groups a number of addressable objects for addressing purposes, without being an administrative unit.

Additional Information:
This would typically be part of a city, a neighbourhood or village, e.g. Montmartre. (locn:Address) </rdfs:comment>
      <skos:definition xml:lang="en">The name or names of a geographic area or locality that groups a number of addressable objects for addressing purposes, without being an administrative unit.

Additional Information:
This would typically be part of a city, a neighbourhood or village, e.g. Montmartre. (locn:Address) </skos:definition>
      <rdfs:isDefinedBy rdf:resource="http://data.europa.eu/a4g/ontology"/>
   </owl:DatatypeProperty>
   <owl:ObjectProperty rdf:about="http://data.europa.eu/a4g/ontology#addressID">
      <rdfs:label xml:lang="en">Address i d</rdfs:label>
      <skos:prefLabel xml:lang="en">Address i d</skos:prefLabel>
      <rdfs:comment xml:lang="en">A globally unique identifier for each instance of an Address.

Additional Information:
The concept of adding a globally unique identifier for each instance of an address is a crucial part of the INSPIRE data spec. A number of EU countries have already implemented an ID (a UUID) in their Address Register/gazetteer, among them Denmark. OASIS xAL also includes an address identifier. It is the address Identifier that allows an address to be represented in a format other than INSPIRE whilst remaining conformant to the Core Vocabulary.

The INSPIRE method of representing addresses is very detailed, designed primarily for use in databases of addresses. Whilst data that is published in full conformance with the INSPIRE data structure can be made available using the Location Core Vocabulary the reverse is not true since the Core Vocabulary allows much greater flexibility.

Many datasets that include address data as one piece of information about something else are likely to have that data in simpler formats. These might be tailored to the specific need of the dataset, follow a national norm, or make use of a standard like vCard.

To provide maximum flexibility in the Core Vocabulary, whilst remaining interoperable with INSPIRE Address Guidelines (which EU Member States are obliged to use), the Location Core Vocabulary provides the extra property of full address and makes use of INSPIRE's addressID. (locn:Address) </rdfs:comment>
      <skos:definition xml:lang="en">A globally unique identifier for each instance of an Address.

Additional Information:
The concept of adding a globally unique identifier for each instance of an address is a crucial part of the INSPIRE data spec. A number of EU countries have already implemented an ID (a UUID) in their Address Register/gazetteer, among them Denmark. OASIS xAL also includes an address identifier. It is the address Identifier that allows an address to be represented in a format other than INSPIRE whilst remaining conformant to the Core Vocabulary.

The INSPIRE method of representing addresses is very detailed, designed primarily for use in databases of addresses. Whilst data that is published in full conformance with the INSPIRE data structure can be made available using the Location Core Vocabulary the reverse is not true since the Core Vocabulary allows much greater flexibility.

Many datasets that include address data as one piece of information about something else are likely to have that data in simpler formats. These might be tailored to the specific need of the dataset, follow a national norm, or make use of a standard like vCard.

To provide maximum flexibility in the Core Vocabulary, whilst remaining interoperable with INSPIRE Address Guidelines (which EU Member States are obliged to use), the Location Core Vocabulary provides the extra property of full address and makes use of INSPIRE's addressID. (locn:Address) </skos:definition>
      <rdfs:isDefinedBy rdf:resource="http://data.europa.eu/a4g/ontology"/>
   </owl:ObjectProperty>
   <owl:DatatypeProperty rdf:about="http://data.europa.eu/a4g/ontology#fullAddress">
      <rdfs:label xml:lang="en">Full address</rdfs:label>
      <skos:prefLabel xml:lang="en">Full address</skos:prefLabel>
      <rdfs:comment xml:lang="en">The complete address written as a formatted string.

Additional Information:
Use of this property is recommended as it will not suffer any misunderstandings that might arise through the breaking up of an address into its component parts. This property is analogous to vCard's label property but with two important differences: (1) formatting is not assumed so that, unlike vCard label, it may not be suitable to print this on an address label, (2) vCard's label property has a domain of vCard Address; the fullAddress property has no such restriction. An example of a full address is "Champ de Mars, 5 Avenue Anatole France, 75007 Paris, France". (locn:Address) </rdfs:comment>
      <skos:definition xml:lang="en">The complete address written as a formatted string.

Additional Information:
Use of this property is recommended as it will not suffer any misunderstandings that might arise through the breaking up of an address into its component parts. This property is analogous to vCard's label property but with two important differences: (1) formatting is not assumed so that, unlike vCard label, it may not be suitable to print this on an address label, (2) vCard's label property has a domain of vCard Address; the fullAddress property has no such restriction. An example of a full address is "Champ de Mars, 5 Avenue Anatole France, 75007 Paris, France". (locn:Address) </skos:definition>
      <rdfs:isDefinedBy rdf:resource="http://data.europa.eu/a4g/ontology"/>
   </owl:DatatypeProperty>
   <owl:DatatypeProperty rdf:about="http://data.europa.eu/a4g/ontology#locatorDesignator">
      <rdfs:label xml:lang="en">Locator designator</rdfs:label>
      <skos:prefLabel xml:lang="en">Locator designator</skos:prefLabel>
      <rdfs:comment xml:lang="en">A number or a sequence of characters which allows a user or an application to interpret, parse and format the locator within the relevant scope. A locator may include more locator designators.

Additional Information:
In simpler terms, this is the building number, apartment number, etc. For an address such as "Flat 3, 17 Bridge Street", the locator is "flat 3, 17". (locn:Address) </rdfs:comment>
      <skos:definition xml:lang="en">A number or a sequence of characters which allows a user or an application to interpret, parse and format the locator within the relevant scope. A locator may include more locator designators.

Additional Information:
In simpler terms, this is the building number, apartment number, etc. For an address such as "Flat 3, 17 Bridge Street", the locator is "flat 3, 17". (locn:Address) </skos:definition>
      <rdfs:isDefinedBy rdf:resource="http://data.europa.eu/a4g/ontology"/>
   </owl:DatatypeProperty>
   <owl:DatatypeProperty rdf:about="http://data.europa.eu/a4g/ontology#locatorName">
      <rdfs:label xml:lang="en">Locator name</rdfs:label>
      <skos:prefLabel xml:lang="en">Locator name</skos:prefLabel>
      <rdfs:comment xml:lang="en">Proper noun(s) applied to the real world entity identified by the locator.

Additional Information:
The locator name could be the name of the property or complex, of the building or part of the building, or it could be the name of a room inside a building.

The key difference between a locator and a locator name is that the latter is a proper name and is unlikely to include digits. For example, "Shumann, Berlaymont" is a meeting room within the European Commission headquarters for which locator name is more appropriate than locator. (locn:Address) </rdfs:comment>
      <skos:definition xml:lang="en">Proper noun(s) applied to the real world entity identified by the locator.

Additional Information:
The locator name could be the name of the property or complex, of the building or part of the building, or it could be the name of a room inside a building.

The key difference between a locator and a locator name is that the latter is a proper name and is unlikely to include digits. For example, "Shumann, Berlaymont" is a meeting room within the European Commission headquarters for which locator name is more appropriate than locator. (locn:Address) </skos:definition>
      <rdfs:isDefinedBy rdf:resource="http://data.europa.eu/a4g/ontology"/>
   </owl:DatatypeProperty>
   <owl:DatatypeProperty rdf:about="http://data.europa.eu/a4g/ontology#postCode">
      <rdfs:label xml:lang="en">Post code</rdfs:label>
      <skos:prefLabel xml:lang="en">Post code</skos:prefLabel>
      <rdfs:comment xml:lang="en">The post/zip code of an address. (INSPIRE's definition is "A code created and maintained for postal purposes to identify a subdivision of addresses and postal delivery points.")

Additional Information:
Post codes are common elements in many countries' postal address systems. One of the many post codes of Paris is for example "75000". (locn:Address) </rdfs:comment>
      <skos:definition xml:lang="en">The post/zip code of an address. (INSPIRE's definition is "A code created and maintained for postal purposes to identify a subdivision of addresses and postal delivery points.")

Additional Information:
Post codes are common elements in many countries' postal address systems. One of the many post codes of Paris is for example "75000". (locn:Address) </skos:definition>
      <rdfs:isDefinedBy rdf:resource="http://data.europa.eu/a4g/ontology"/>
   </owl:DatatypeProperty>
   <owl:DatatypeProperty rdf:about="http://data.europa.eu/a4g/ontology#postName">
      <rdfs:label xml:lang="en">Post name</rdfs:label>
      <skos:prefLabel xml:lang="en">Post name</skos:prefLabel>
      <rdfs:comment xml:lang="en">The key postal division of the address, usually the city. (INSPIRE's definition is "One or more names created and maintained for postal purposes to identify a subdivision of addresses and postal delivery points.) For example, "Paris". (locn:Address) </rdfs:comment>
      <skos:definition xml:lang="en">The key postal division of the address, usually the city. (INSPIRE's definition is "One or more names created and maintained for postal purposes to identify a subdivision of addresses and postal delivery points.) For example, "Paris". (locn:Address) </skos:definition>
      <rdfs:isDefinedBy rdf:resource="http://data.europa.eu/a4g/ontology"/>
   </owl:DatatypeProperty>
   <owl:DatatypeProperty rdf:about="http://data.europa.eu/a4g/ontology#thoroughfare">
      <rdfs:label xml:lang="en">Thoroughfare</rdfs:label>
      <skos:prefLabel xml:lang="en">Thoroughfare</skos:prefLabel>
      <rdfs:comment xml:lang="en">An address component that represents the name or names of a passage or way through from one location to another. A thoroughfare is not necessarily a road, it might be a waterway or some other feature.

Additional Information:
For example, "Avenue des Champs-&amp;#201;lys&amp;#233;es". (locn:Address) </rdfs:comment>
      <skos:definition xml:lang="en">An address component that represents the name or names of a passage or way through from one location to another. A thoroughfare is not necessarily a road, it might be a waterway or some other feature.

Additional Information:
For example, "Avenue des Champs-&amp;#201;lys&amp;#233;es". (locn:Address) </skos:definition>
      <rdfs:isDefinedBy rdf:resource="http://data.europa.eu/a4g/ontology"/>
   </owl:DatatypeProperty>
   <owl:DatatypeProperty rdf:about="http://data.europa.eu/a4g/ontology#coordinates">
      <rdfs:label xml:lang="en">Coordinates</rdfs:label>
      <skos:prefLabel xml:lang="en">Coordinates</skos:prefLabel>
      <rdfs:comment xml:lang="en">The coordinate list. (locn:Geometry) </rdfs:comment>
      <skos:definition xml:lang="en">The coordinate list. (locn:Geometry) </skos:definition>
      <rdfs:isDefinedBy rdf:resource="http://data.europa.eu/a4g/ontology"/>
   </owl:DatatypeProperty>
   <owl:DatatypeProperty rdf:about="http://data.europa.eu/a4g/ontology#latitude">
      <rdfs:label xml:lang="en">Latitude</rdfs:label>
      <skos:prefLabel xml:lang="en">Latitude</skos:prefLabel>
      <rdfs:comment xml:lang="en">The latitude. (locn:Geometry) </rdfs:comment>
      <skos:definition xml:lang="en">The latitude. (locn:Geometry) </skos:definition>
      <rdfs:isDefinedBy rdf:resource="http://data.europa.eu/a4g/ontology"/>
   </owl:DatatypeProperty>
   <owl:DatatypeProperty rdf:about="http://data.europa.eu/a4g/ontology#longitude">
      <rdfs:label xml:lang="en">Longitude</rdfs:label>
      <skos:prefLabel xml:lang="en">Longitude</skos:prefLabel>
      <rdfs:comment xml:lang="en">The longitude. (locn:Geometry) </rdfs:comment>
      <skos:definition xml:lang="en">The longitude. (locn:Geometry) </skos:definition>
      <rdfs:isDefinedBy rdf:resource="http://data.europa.eu/a4g/ontology"/>
   </owl:DatatypeProperty>
   <owl:DatatypeProperty rdf:about="http://data.europa.eu/a4g/ontology#hasAmountValue">
      <rdfs:label xml:lang="en">Has amount value</rdfs:label>
      <skos:prefLabel xml:lang="en">Has amount value</skos:prefLabel>
      <rdfs:comment xml:lang="en">The numeric value of the amount, including decimals. (epo:Amount) </rdfs:comment>
      <skos:definition xml:lang="en">The numeric value of the amount, including decimals. (epo:Amount) </skos:definition>
      <rdfs:isDefinedBy rdf:resource="http://data.europa.eu/a4g/ontology"/>
   </owl:DatatypeProperty>
   <owl:DatatypeProperty rdf:about="http://data.europa.eu/a4g/ontology#hasCurrencyCodeListAgencyID">
      <rdfs:label xml:lang="en">Has currency code list agency i d</rdfs:label>
      <skos:prefLabel xml:lang="en">Has currency code list agency i d</skos:prefLabel>
      <rdfs:comment xml:lang="en">Identifier of the agency that maintains the currency code list used.
WG approval 13/04/2021 (epo:Amount) </rdfs:comment>
      <skos:definition xml:lang="en">Identifier of the agency that maintains the currency code list used.
WG approval 13/04/2021 (epo:Amount) </skos:definition>
      <rdfs:isDefinedBy rdf:resource="http://data.europa.eu/a4g/ontology"/>
   </owl:DatatypeProperty>
   <owl:DatatypeProperty rdf:about="http://data.europa.eu/a4g/ontology#hasCurrencyCodeListAgencyName">
      <rdfs:label xml:lang="en">Has currency code list agency name</rdfs:label>
      <skos:prefLabel xml:lang="en">Has currency code list agency name</skos:prefLabel>
      <rdfs:comment xml:lang="en">Name of the agency that maintains the currency code list used.
WG approval 13/04/2021 (epo:Amount) </rdfs:comment>
      <skos:definition xml:lang="en">Name of the agency that maintains the currency code list used.
WG approval 13/04/2021 (epo:Amount) </skos:definition>
      <rdfs:isDefinedBy rdf:resource="http://data.europa.eu/a4g/ontology"/>
   </owl:DatatypeProperty>
   <owl:DatatypeProperty rdf:about="http://data.europa.eu/a4g/ontology#hasCurrencyCodeListID">
      <rdfs:label xml:lang="en">Has currency code list i d</rdfs:label>
      <skos:prefLabel xml:lang="en">Has currency code list i d</skos:prefLabel>
      <rdfs:comment xml:lang="en">Concept scheme URI used for the currency code list.
WG approval 13/04/2021 (epo:Amount) </rdfs:comment>
      <skos:definition xml:lang="en">Concept scheme URI used for the currency code list.
WG approval 13/04/2021 (epo:Amount) </skos:definition>
      <rdfs:isDefinedBy rdf:resource="http://data.europa.eu/a4g/ontology"/>
   </owl:DatatypeProperty>
   <owl:DatatypeProperty rdf:about="http://data.europa.eu/a4g/ontology#hasCurrencyID">
      <rdfs:label xml:lang="en">Has currency i d</rdfs:label>
      <skos:prefLabel xml:lang="en">Has currency i d</skos:prefLabel>
      <rdfs:comment xml:lang="en">The identifier of the currency as in the standard code list used.  (epo:Amount) </rdfs:comment>
      <skos:definition xml:lang="en">The identifier of the currency as in the standard code list used.  (epo:Amount) </skos:definition>
      <rdfs:isDefinedBy rdf:resource="http://data.europa.eu/a4g/ontology"/>
   </owl:DatatypeProperty>
   <owl:DatatypeProperty rdf:about="http://data.europa.eu/a4g/ontology#hasIdentifierValue">
      <rdfs:label xml:lang="en">Has identifier value</rdfs:label>
      <skos:prefLabel xml:lang="en">Has identifier value</skos:prefLabel>
      <rdfs:comment xml:lang="en">The literal identifying an entity, like a person or an object. (epo:Identifier) </rdfs:comment>
      <skos:definition xml:lang="en">The literal identifying an entity, like a person or an object. (epo:Identifier) </skos:definition>
      <rdfs:isDefinedBy rdf:resource="http://data.europa.eu/a4g/ontology"/>
   </owl:DatatypeProperty>
   <owl:DatatypeProperty rdf:about="http://data.europa.eu/a4g/ontology#hasSchemeAgencyID">
      <rdfs:label xml:lang="en">Has scheme agency i d</rdfs:label>
      <skos:prefLabel xml:lang="en">Has scheme agency i d</skos:prefLabel>
      <rdfs:comment xml:lang="en">The identification of the agency that maintains the identification scheme. (epo:Identifier) </rdfs:comment>
      <skos:definition xml:lang="en">The identification of the agency that maintains the identification scheme. (epo:Identifier) </skos:definition>
      <rdfs:isDefinedBy rdf:resource="http://data.europa.eu/a4g/ontology"/>
   </owl:DatatypeProperty>
   <owl:DatatypeProperty rdf:about="http://data.europa.eu/a4g/ontology#hasSchemeAgencyName">
      <rdfs:label xml:lang="en">Has scheme agency name</rdfs:label>
      <skos:prefLabel xml:lang="en">Has scheme agency name</skos:prefLabel>
      <rdfs:comment xml:lang="en">The name of the agency that maintains the identification scheme. (epo:Identifier) </rdfs:comment>
      <skos:definition xml:lang="en">The name of the agency that maintains the identification scheme. (epo:Identifier) </skos:definition>
      <rdfs:isDefinedBy rdf:resource="http://data.europa.eu/a4g/ontology"/>
   </owl:DatatypeProperty>
   <owl:DatatypeProperty rdf:about="http://data.europa.eu/a4g/ontology#hasSchemeDataURI">
      <rdfs:label xml:lang="en">Has scheme data u r i</rdfs:label>
      <skos:prefLabel xml:lang="en">Has scheme data u r i</skos:prefLabel>
      <rdfs:comment xml:lang="en">The Uniform Resource Identifier that identifies where the identification scheme data is located. (epo:Identifier) </rdfs:comment>
      <skos:definition xml:lang="en">The Uniform Resource Identifier that identifies where the identification scheme data is located. (epo:Identifier) </skos:definition>
      <rdfs:isDefinedBy rdf:resource="http://data.europa.eu/a4g/ontology"/>
   </owl:DatatypeProperty>
   <owl:DatatypeProperty rdf:about="http://data.europa.eu/a4g/ontology#hasSchemeID">
      <rdfs:label xml:lang="en">Has scheme i d</rdfs:label>
      <skos:prefLabel xml:lang="en">Has scheme i d</skos:prefLabel>
      <rdfs:comment xml:lang="en">The identification of the identification scheme. (epo:Identifier) </rdfs:comment>
      <skos:definition xml:lang="en">The identification of the identification scheme. (epo:Identifier) </skos:definition>
      <rdfs:isDefinedBy rdf:resource="http://data.europa.eu/a4g/ontology"/>
   </owl:DatatypeProperty>
   <owl:DatatypeProperty rdf:about="http://data.europa.eu/a4g/ontology#hasSchemeName">
      <rdfs:label xml:lang="en">Has scheme name</rdfs:label>
      <skos:prefLabel xml:lang="en">Has scheme name</skos:prefLabel>
      <rdfs:comment xml:lang="en">The name of the identification scheme. (epo:Identifier) </rdfs:comment>
      <skos:definition xml:lang="en">The name of the identification scheme. (epo:Identifier) </skos:definition>
      <rdfs:isDefinedBy rdf:resource="http://data.europa.eu/a4g/ontology"/>
   </owl:DatatypeProperty>
   <owl:DatatypeProperty rdf:about="http://data.europa.eu/a4g/ontology#hasSchemeURI">
      <rdfs:label xml:lang="en">Has scheme u r i</rdfs:label>
      <skos:prefLabel xml:lang="en">Has scheme u r i</skos:prefLabel>
      <rdfs:comment xml:lang="en">The Uniform Resource Identifier that identifies where the identification scheme is located. (epo:Identifier) </rdfs:comment>
      <skos:definition xml:lang="en">The Uniform Resource Identifier that identifies where the identification scheme is located. (epo:Identifier) </skos:definition>
      <rdfs:isDefinedBy rdf:resource="http://data.europa.eu/a4g/ontology"/>
   </owl:DatatypeProperty>
   <owl:DatatypeProperty rdf:about="http://data.europa.eu/a4g/ontology#hasSchemeVersionID">
      <rdfs:label xml:lang="en">Has scheme version i d</rdfs:label>
      <skos:prefLabel xml:lang="en">Has scheme version i d</skos:prefLabel>
      <rdfs:comment xml:lang="en">The version of the identification scheme. (epo:Identifier) </rdfs:comment>
      <skos:definition xml:lang="en">The version of the identification scheme. (epo:Identifier) </skos:definition>
      <rdfs:isDefinedBy rdf:resource="http://data.europa.eu/a4g/ontology"/>
   </owl:DatatypeProperty>
   <owl:DatatypeProperty rdf:about="http://data.europa.eu/a4g/ontology#hasMeasureValue">
      <rdfs:label xml:lang="en">Has measure value</rdfs:label>
      <skos:prefLabel xml:lang="en">Has measure value</skos:prefLabel>
      <rdfs:comment xml:lang="en">The numeric value of the measure, including decimals if needed. (epo:Measure) </rdfs:comment>
      <skos:definition xml:lang="en">The numeric value of the measure, including decimals if needed. (epo:Measure) </skos:definition>
      <rdfs:isDefinedBy rdf:resource="http://data.europa.eu/a4g/ontology"/>
   </owl:DatatypeProperty>
   <owl:DatatypeProperty rdf:about="http://data.europa.eu/a4g/ontology#hasUnitCode">
      <rdfs:label xml:lang="en">Has unit code</rdfs:label>
      <skos:prefLabel xml:lang="en">Has unit code</skos:prefLabel>
      <rdfs:comment xml:lang="en">The type of unit of measure. (epo:Measure) </rdfs:comment>
      <skos:definition xml:lang="en">The type of unit of measure. (epo:Measure) </skos:definition>
      <rdfs:isDefinedBy rdf:resource="http://data.europa.eu/a4g/ontology"/>
   </owl:DatatypeProperty>
   <owl:DatatypeProperty rdf:about="http://data.europa.eu/a4g/ontology#hasUnitCodeListAgencyID">
      <rdfs:label xml:lang="en">Has unit code list agency i d</rdfs:label>
      <skos:prefLabel xml:lang="en">Has unit code list agency i d</skos:prefLabel>
      <rdfs:comment xml:lang="en">The identification of the agency that maintains the quantity unit code list. (epo:Measure) </rdfs:comment>
      <skos:definition xml:lang="en">The identification of the agency that maintains the quantity unit code list. (epo:Measure) </skos:definition>
      <rdfs:isDefinedBy rdf:resource="http://data.europa.eu/a4g/ontology"/>
   </owl:DatatypeProperty>
   <owl:DatatypeProperty rdf:about="http://data.europa.eu/a4g/ontology#hasUnitCodeListAgencyName">
      <rdfs:label xml:lang="en">Has unit code list agency name</rdfs:label>
      <skos:prefLabel xml:lang="en">Has unit code list agency name</skos:prefLabel>
      <rdfs:comment xml:lang="en">The identification of the agency that maintains the quantity unit code list. (epo:Measure) </rdfs:comment>
      <skos:definition xml:lang="en">The identification of the agency that maintains the quantity unit code list. (epo:Measure) </skos:definition>
      <rdfs:isDefinedBy rdf:resource="http://data.europa.eu/a4g/ontology"/>
   </owl:DatatypeProperty>
   <owl:DatatypeProperty rdf:about="http://data.europa.eu/a4g/ontology#hasUnitCodeListID">
      <rdfs:label xml:lang="en">Has unit code list i d</rdfs:label>
      <skos:prefLabel xml:lang="en">Has unit code list i d</skos:prefLabel>
      <rdfs:comment xml:lang="en">The quantity unit code list. (epo:Measure) </rdfs:comment>
      <skos:definition xml:lang="en">The quantity unit code list. (epo:Measure) </skos:definition>
      <rdfs:isDefinedBy rdf:resource="http://data.europa.eu/a4g/ontology"/>
   </owl:DatatypeProperty>
   <owl:DatatypeProperty rdf:about="http://data.europa.eu/a4g/ontology#hasQuantityValue">
      <rdfs:label xml:lang="en">Has quantity value</rdfs:label>
      <skos:prefLabel xml:lang="en">Has quantity value</skos:prefLabel>
      <rdfs:comment xml:lang="en">The numeric value of the quantity, including decimals. (epo:Quantity) </rdfs:comment>
      <skos:definition xml:lang="en">The numeric value of the quantity, including decimals. (epo:Quantity) </skos:definition>
      <rdfs:isDefinedBy rdf:resource="http://data.europa.eu/a4g/ontology"/>
   </owl:DatatypeProperty>
   <owl:DatatypeProperty rdf:about="http://data.europa.eu/a4g/ontology#hasUnitDescription">
      <rdfs:label xml:lang="en">Has unit description</rdfs:label>
      <skos:prefLabel xml:lang="en">Has unit description</skos:prefLabel>
      <rdfs:comment xml:lang="en">A narrative explanation defining the units of items being counted

Additional information: This could be for example individual items or pack or two.

WG Approval 09/11/2021 (epo:Quantity) </rdfs:comment>
      <skos:definition xml:lang="en">A narrative explanation defining the units of items being counted

Additional information: This could be for example individual items or pack or two.

WG Approval 09/11/2021 (epo:Quantity) </skos:definition>
      <rdfs:isDefinedBy rdf:resource="http://data.europa.eu/a4g/ontology"/>
   </owl:DatatypeProperty>
</rdf:RDF>
