<?xml version="1.0" encoding="UTF-8"?>
<rdf:RDF xmlns="http://data.europa.eu/a4g/ontology#"
         xmlns:adms="http://www.w3.org/ns/adms#"
         xmlns:at-voc="http://publications.europa.eu/resource/authority/"
         xmlns:cccev="http://data.europa.eu/m8g/"
         xmlns:core="http://data.europa.eu/m8g/"
         xmlns:cpov="http://data.europa.eu/m8g/"
         xmlns:cpsv="http://data.europa.eu/m8g/"
         xmlns:cpv="http://data.europa.eu/m8g/"
         xmlns:cv="http://data.europa.eu/m8g/"
         xmlns:dc="http://purl.org/dc/elements/1.1/"
         xmlns:dct="http://purl.org/dc/terms/"
         xmlns:dul="http://www.ontologydesignpatterns.org/ont/dul/DUL.owl#"
         xmlns:eli="http://data.europa.eu/eli/ontology#"
         xmlns:epo="http://data.europa.eu/a4g/ontology#"
         xmlns:epo-acc="http://data.europa.eu/a4g/ontology#"
         xmlns:epo-cat="http://data.europa.eu/a4g/ontology#"
         xmlns:epo-con="http://data.europa.eu/a4g/ontology#"
         xmlns:epo-ful="http://data.europa.eu/a4g/ontology#"
         xmlns:epo-not="http://data.europa.eu/a4g/ontology#"
         xmlns:epo-ord="http://data.europa.eu/a4g/ontology#"
         xmlns:epo-sub="http://data.europa.eu/a4g/ontology#"
         xmlns:espd="https://github.com/ESPD/ESPD-EDM/"
         xmlns:foaf="http://xmlns.com/foaf/0.1/"
         xmlns:frbroo="http://iflastandards.info/ns/fr/frbr/frbroo/"
         xmlns:geosparql="http://www.opengis.net/ont/geosparql#"
         xmlns:locn="http://www.w3.org/ns/locn#"
         xmlns:nuts="http://data.europa.eu/nuts/"
         xmlns:org="http://www.w3.org/ns/org#"
         xmlns:owl="http://www.w3.org/2002/07/owl#"
         xmlns:person="http://www.w3.org/ns/person#"
         xmlns:rdf="http://www.w3.org/1999/02/22-rdf-syntax-ns#"
         xmlns:rdfs="http://www.w3.org/2000/01/rdf-schema#"
         xmlns:skos="http://www.w3.org/2004/02/skos/core#"
         xmlns:time="http://www.w3.org/2006/time#"
         xmlns:vann="http://purl.org/vocab/vann/"
         xmlns:xsd="http://www.w3.org/2001/XMLSchema#">
   <owl:Ontology rdf:about="http://data.europa.eu/a4g/ontology#sub">
      <owl:imports rdf:resource="http://xmlns.com/foaf/0.1/"/>
      <owl:imports rdf:resource="http://purl.org/dc/terms/"/>
      <owl:imports rdf:resource="http://www.w3.org/ns/org#"/>
      <owl:imports rdf:resource="http://www.w3.org/2004/02/skos/core"/>
      <owl:imports rdf:resource="http://www.w3.org/2006/time"/>
      <owl:imports rdf:resource="http://www.w3.org/ns/locn"/>
      <owl:imports rdf:resource="http://data.europa.eu/m8g/"/>
      <owl:imports rdf:resource="http://www.w3.org/ns/person"/>
      <owl:imports rdf:resource="http://www.w3.org/ns/adms"/>
      <owl:imports rdf:resource="http://purl.org/vocab/vann/"/>
      <owl:imports rdf:resource="http://data.europa.eu/eli/ontology#"/>
      <owl:imports rdf:resource="http://iflastandards.info/ns/fr/frbr/frbroo/"/>
      <owl:imports rdf:resource="http://data.europa.eu/a4g/ontology#core"/>
      <owl:imports rdf:resource="http://data.europa.eu/a4g/ontology#acc"/>
      <dct:title xml:lang="en">eProcurement Ontology Submission - core</dct:title>
      <rdfs:label xml:lang="en">eProcurement Ontology Submission - core</rdfs:label>
      <dct:description xml:lang="en">The eProcurement Ontology Submission core describes the concepts and properties representing the European Public Procurement Submission domain. The provision of these semantics offers the basis for a common understanding of the domain for all stakeholders ensuring the quality of data exchange and transparency. The ontology restrictions are published in a separate artefact.</dct:description>
      <dct:publisher>http://publications.europa.eu/resource/authority/corporate-body/PUBL</dct:publisher>
      <rdfs:comment>This version is automatically generated from eSubmission.xml on 2024-03-21</rdfs:comment>
      <rdfs:seeAlso rdf:resource="https://github.com/OP-TED/ePO/releases"/>
      <rdfs:seeAlso rdf:resource="https://joinup.ec.europa.eu/collection/eprocurement/solution/eprocurement-ontology/about"/>
      <rdfs:seeAlso rdf:resource="https://op.europa.eu/en/web/eu-vocabularies/e-procurement"/>
      <rdfs:seeAlso rdf:resource="https://docs.ted.europa.eu/home/index.html"/>
      <dct:issued rdf:datatype="http://www.w3.org/2001/XMLSchema#date">2024-03-21</dct:issued>
      <dct:created rdf:datatype="http://www.w3.org/2001/XMLSchema#date">2021-06-01</dct:created>
      <owl:versionInfo>4.2.0</owl:versionInfo>
      <owl:incompatibleWith>3.1.0</owl:incompatibleWith>
      <owl:versionIRI rdf:resource="http://data.europa.eu/a4g/ontology#sub-4.2.0"/>
      <owl:priorVersion>http://data.europa.eu/a4g/ontology#sub-4.0.2</owl:priorVersion>
      <vann:preferredNamespaceUri>http://data.europa.eu/a4g/ontology#</vann:preferredNamespaceUri>
      <vann:preferredNamespacePrefix>epo</vann:preferredNamespacePrefix>
      <dct:license>Â© European Union, 2014. Unless otherwise noted, the reuse of the Ontology is authorised under the European Union Public Licence v1.2 (https://eupl.eu/).</dct:license>
   </owl:Ontology>
   <owl:Class rdf:about="http://data.europa.eu/m8g/SupportedValue"/>
   <rdf:Description rdf:about="http://data.europa.eu/m8g/SupportedValue">
      <skos:prefLabel xml:lang="en">Supported value</skos:prefLabel>
   </rdf:Description>
   <rdf:Description rdf:about="http://data.europa.eu/m8g/SupportedValue">
      <skos:definition xml:lang="en">Value for an Information Concept that is provided by an Evidence. Additional Information: The notion of Supported Value is closely related to actual data exchange between two parties: (a) the Requirement processor, i.e. the Agent setting out Requirements for an objective and processing the supplied Evidences in the context of the Requirements, and (b) the Evidence provider, i.e. the Agent supplying information to an information request expressed as Requirements. The Requirement processor has expressed its expectations (both business as technical) for the information it wants to recieve as an Information Concept. The Evidence provider is able to supply information for that Information Concept, but its native data representation might not be coherent with the expectations set by the Requirement processor. The Supported Value is bridging both. The Evidence provider can either provide a derived value (fact) from its native data representation that complies with the Information Concept expectations. Or it can provide a query in an agreed language between Evidence provider and Requirement processor that allows the Requirement processor to retrieve the value from the native data representation. Implementers are free to choose their language. It is recommended to document the made agreements well.</skos:definition>
   </rdf:Description>
   <owl:Class rdf:about="http://data.europa.eu/a4g/ontology#CertificateInformation"/>
   <rdf:Description rdf:about="http://data.europa.eu/a4g/ontology#CertificateInformation">
      <skos:prefLabel xml:lang="en">Certificate information</skos:prefLabel>
   </rdf:Description>
   <rdf:Description rdf:about="http://data.europa.eu/a4g/ontology#CertificateInformation">
      <skos:definition xml:lang="en">Information about a Certificate. WG approval 12/03/2024</skos:definition>
   </rdf:Description>
   <rdf:Description rdf:about="http://data.europa.eu/a4g/ontology#CertificateInformation">
      <rdfs:isDefinedBy rdf:resource="http://data.europa.eu/a4g/ontology#sub"/>
   </rdf:Description>
   <owl:Class rdf:about="http://data.europa.eu/a4g/ontology#ESPDResponse"/>
   <rdf:Description rdf:about="http://data.europa.eu/a4g/ontology#ESPDResponse">
      <skos:prefLabel xml:lang="en">E s p d response</skos:prefLabel>
   </rdf:Description>
   <rdf:Description rdf:about="http://data.europa.eu/a4g/ontology#ESPDResponse">
      <skos:definition xml:lang="en">A document conveying the fulfilment or not by the economic operator of the Exclusion Grounds and the Selection Criteria set out by the Buyer for a specific Procurement using an European Single Procurement Document (ESPD) Request. WG Approval 05/03/2024</skos:definition>
   </rdf:Description>
   <rdf:Description rdf:about="http://data.europa.eu/a4g/ontology#ESPDResponse">
      <rdfs:isDefinedBy rdf:resource="http://data.europa.eu/a4g/ontology#sub"/>
   </rdf:Description>
   <owl:Class rdf:about="http://data.europa.eu/a4g/ontology#LegalRepresentative"/>
   <rdf:Description rdf:about="http://data.europa.eu/a4g/ontology#LegalRepresentative">
      <skos:prefLabel xml:lang="en">Legal representative</skos:prefLabel>
   </rdf:Description>
   <rdf:Description rdf:about="http://data.europa.eu/a4g/ontology#LegalRepresentative">
      <skos:definition xml:lang="en">The Role of an Agent that can represent an Organization. WG approval 05/03/2024</skos:definition>
   </rdf:Description>
   <rdf:Description rdf:about="http://data.europa.eu/a4g/ontology#LegalRepresentative">
      <rdfs:isDefinedBy rdf:resource="http://data.europa.eu/a4g/ontology#sub"/>
   </rdf:Description>
   <owl:Class rdf:about="http://data.europa.eu/a4g/ontology#Mandate"/>
   <rdf:Description rdf:about="http://data.europa.eu/a4g/ontology#Mandate">
      <skos:prefLabel xml:lang="en">Mandate</skos:prefLabel>
   </rdf:Description>
   <rdf:Description rdf:about="http://data.europa.eu/a4g/ontology#Mandate">
      <skos:definition xml:lang="en">An authorization to act as a representative of an Organization. WG approval 05/03/2024</skos:definition>
   </rdf:Description>
   <rdf:Description rdf:about="http://data.europa.eu/a4g/ontology#Mandate">
      <rdfs:isDefinedBy rdf:resource="http://data.europa.eu/a4g/ontology#sub"/>
   </rdf:Description>
   <owl:Class rdf:about="http://data.europa.eu/a4g/ontology#NationalPreQualificationData"/>
   <rdf:Description rdf:about="http://data.europa.eu/a4g/ontology#NationalPreQualificationData">
      <skos:prefLabel xml:lang="en">National pre qualification data</skos:prefLabel>
   </rdf:Description>
   <rdf:Description rdf:about="http://data.europa.eu/a4g/ontology#NationalPreQualificationData">
      <skos:definition xml:lang="en">Data that describe the distinctive features or characteristics that qualify an economic operator to take part in a tendering process. WG approval 05/03/2024</skos:definition>
   </rdf:Description>
   <rdf:Description rdf:about="http://data.europa.eu/a4g/ontology#NationalPreQualificationData">
      <rdfs:isDefinedBy rdf:resource="http://data.europa.eu/a4g/ontology#sub"/>
   </rdf:Description>
   <owl:Class rdf:about="http://data.europa.eu/a4g/ontology#PowerOfAttorney"/>
   <rdf:Description rdf:about="http://data.europa.eu/a4g/ontology#PowerOfAttorney">
      <skos:prefLabel xml:lang="en">Power of attorney</skos:prefLabel>
   </rdf:Description>
   <rdf:Description rdf:about="http://data.europa.eu/a4g/ontology#PowerOfAttorney">
      <skos:definition xml:lang="en">A legal document that grants someone the authority to make decisions on behalf of an Organization. WG approval 05/03/2024</skos:definition>
   </rdf:Description>
   <rdf:Description rdf:about="http://data.europa.eu/a4g/ontology#PowerOfAttorney">
      <rdfs:isDefinedBy rdf:resource="http://data.europa.eu/a4g/ontology#sub"/>
   </rdf:Description>
   <owl:Class rdf:about="http://data.europa.eu/a4g/ontology#Response"/>
   <rdf:Description rdf:about="http://data.europa.eu/a4g/ontology#Response">
      <skos:prefLabel xml:lang="en">Response</skos:prefLabel>
   </rdf:Description>
   <rdf:Description rdf:about="http://data.europa.eu/a4g/ontology#Response">
      <skos:definition xml:lang="en">An answer given to a question that is part of an ESPD Request. WG approval 12/03/2024</skos:definition>
   </rdf:Description>
   <rdf:Description rdf:about="http://data.europa.eu/a4g/ontology#Response">
      <rdfs:isDefinedBy rdf:resource="http://data.europa.eu/a4g/ontology#sub"/>
   </rdf:Description>
   <rdfs:Datatype rdf:about="http://www.w3.org/1999/02/22-rdf-syntax-ns#PlainLiteral"/>
   <rdf:Description rdf:about="http://www.w3.org/1999/02/22-rdf-syntax-ns#PlainLiteral">
      <skos:prefLabel xml:lang="en">Plain literal</skos:prefLabel>
   </rdf:Description>
   <rdfs:Datatype rdf:about="http://www.w3.org/2001/XMLSchema#anyURI"/>
   <rdf:Description rdf:about="http://www.w3.org/2001/XMLSchema#anyURI">
      <skos:prefLabel xml:lang="en">Any u r i</skos:prefLabel>
   </rdf:Description>
   <rdfs:Datatype rdf:about="http://www.w3.org/2001/XMLSchema#boolean"/>
   <rdf:Description rdf:about="http://www.w3.org/2001/XMLSchema#boolean">
      <skos:prefLabel xml:lang="en">Boolean</skos:prefLabel>
   </rdf:Description>
   <rdfs:Datatype rdf:about="http://www.w3.org/2001/XMLSchema#date"/>
   <rdf:Description rdf:about="http://www.w3.org/2001/XMLSchema#date">
      <skos:prefLabel xml:lang="en">Date</skos:prefLabel>
   </rdf:Description>
   <rdfs:Datatype rdf:about="http://www.w3.org/2001/XMLSchema#dateTime"/>
   <rdf:Description rdf:about="http://www.w3.org/2001/XMLSchema#dateTime">
      <skos:prefLabel xml:lang="en">Date time</skos:prefLabel>
   </rdf:Description>
   <rdfs:Datatype rdf:about="http://www.w3.org/2001/XMLSchema#decimal"/>
   <rdf:Description rdf:about="http://www.w3.org/2001/XMLSchema#decimal">
      <skos:prefLabel xml:lang="en">Decimal</skos:prefLabel>
   </rdf:Description>
   <rdfs:Datatype rdf:about="http://www.w3.org/2001/XMLSchema#integer"/>
   <rdf:Description rdf:about="http://www.w3.org/2001/XMLSchema#integer">
      <skos:prefLabel xml:lang="en">Integer</skos:prefLabel>
   </rdf:Description>
   <owl:Class rdf:about="http://data.europa.eu/a4g/ontology#CertificateInformation">
      <rdfs:subClassOf rdf:resource="http://data.europa.eu/a4g/ontology#ContextDescription"/>
   </owl:Class>
   <owl:Class rdf:about="http://data.europa.eu/a4g/ontology#ESPDResponse">
      <rdfs:subClassOf rdf:resource="http://data.europa.eu/a4g/ontology#Document"/>
   </owl:Class>
   <owl:Class rdf:about="http://data.europa.eu/a4g/ontology#Mandate">
      <rdfs:subClassOf rdf:resource="http://data.europa.eu/a4g/ontology#Document"/>
   </owl:Class>
   <owl:Class rdf:about="http://data.europa.eu/a4g/ontology#PowerOfAttorney">
      <rdfs:subClassOf rdf:resource="http://data.europa.eu/a4g/ontology#Document"/>
   </owl:Class>
   <owl:Class rdf:about="http://data.europa.eu/a4g/ontology#LegalRepresentative">
      <rdfs:subClassOf rdf:resource="http://data.europa.eu/a4g/ontology#AuxiliaryParty"/>
   </owl:Class>
   <owl:ObjectProperty rdf:about="http://data.europa.eu/m8g/providesValueFor"/>
   <rdf:Description rdf:about="http://data.europa.eu/m8g/providesValueFor">
      <skos:prefLabel xml:lang="en">Provides value for</skos:prefLabel>
   </rdf:Description>
   <rdf:Description rdf:about="http://data.europa.eu/m8g/providesValueFor">
      <skos:definition xml:lang="en">Information Concept for which the Supported Value provides a value. (cccev:SupportedValue -&gt; cccev:InformationConcept (+cccev:providesValueFor))</skos:definition>
   </rdf:Description>
   <owl:ObjectProperty rdf:about="http://data.europa.eu/m8g/supportsValue"/>
   <rdf:Description rdf:about="http://data.europa.eu/m8g/supportsValue">
      <skos:prefLabel xml:lang="en">Supports value</skos:prefLabel>
   </rdf:Description>
   <rdf:Description rdf:about="http://data.europa.eu/m8g/supportsValue">
      <skos:definition xml:lang="en">Supported Value that the Evidence contains. (epo-sub:Response -&gt; cccev:SupportedValue (+cccev:supportsValue)) Supported Value that the Evidence contains. (cccev:Evidence -&gt; cccev:SupportedValue (+cccev:supportsValue))</skos:definition>
   </rdf:Description>
   <owl:ObjectProperty rdf:about="http://data.europa.eu/a4g/ontology#summarisesInformationAboutCertificate"/>
   <rdf:Description rdf:about="http://data.europa.eu/a4g/ontology#summarisesInformationAboutCertificate">
      <skos:prefLabel xml:lang="en">Summarises information about certificate</skos:prefLabel>
   </rdf:Description>
   <rdf:Description rdf:about="http://data.europa.eu/a4g/ontology#summarisesInformationAboutCertificate">
      <skos:definition xml:lang="en">Relation indicating the Certificate that the information refers to. WG approval 12/03/2024 (epo-sub:CertificateInformation -&gt; epo:Certificate (+epo-sub:summarisesInformationAboutCertificate))</skos:definition>
   </rdf:Description>
   <rdf:Description rdf:about="http://data.europa.eu/a4g/ontology#summarisesInformationAboutCertificate">
      <rdfs:isDefinedBy rdf:resource="http://data.europa.eu/a4g/ontology#sub"/>
   </rdf:Description>
   <owl:ObjectProperty rdf:about="http://data.europa.eu/a4g/ontology#relatesToESPDRequest"/>
   <rdf:Description rdf:about="http://data.europa.eu/a4g/ontology#relatesToESPDRequest">
      <skos:prefLabel xml:lang="en">Relates to e s p d request</skos:prefLabel>
   </rdf:Description>
   <rdf:Description rdf:about="http://data.europa.eu/a4g/ontology#relatesToESPDRequest">
      <skos:definition xml:lang="en">Is about an European Single Procurement Document (ESPD) Request. WG approval 05/03/2024 (epo-sub:ESPDResponse -&gt; epo-acc:ESPDRequest (+epo-sub:relatesToESPDRequest))</skos:definition>
   </rdf:Description>
   <rdf:Description rdf:about="http://data.europa.eu/a4g/ontology#relatesToESPDRequest">
      <rdfs:isDefinedBy rdf:resource="http://data.europa.eu/a4g/ontology#sub"/>
   </rdf:Description>
   <owl:ObjectProperty rdf:about="http://data.europa.eu/a4g/ontology#answersExclusionGround"/>
   <rdf:Description rdf:about="http://data.europa.eu/a4g/ontology#answersExclusionGround">
      <skos:prefLabel xml:lang="en">Answers exclusion ground</skos:prefLabel>
   </rdf:Description>
   <rdf:Description rdf:about="http://data.europa.eu/a4g/ontology#answersExclusionGround">
      <rdfs:isDefinedBy rdf:resource="http://data.europa.eu/a4g/ontology#sub"/>
   </rdf:Description>
   <owl:ObjectProperty rdf:about="http://data.europa.eu/a4g/ontology#specifiesResponse"/>
   <rdf:Description rdf:about="http://data.europa.eu/a4g/ontology#specifiesResponse">
      <skos:prefLabel xml:lang="en">Specifies response</skos:prefLabel>
   </rdf:Description>
   <rdf:Description rdf:about="http://data.europa.eu/a4g/ontology#specifiesResponse">
      <skos:definition xml:lang="en">Relation indicating that an ESPD Response contains a Response. WG approval 12/03/2024 (epo-sub:ESPDResponse -&gt; epo-sub:Response (+epo-sub:specifiesResponse))</skos:definition>
   </rdf:Description>
   <rdf:Description rdf:about="http://data.europa.eu/a4g/ontology#specifiesResponse">
      <rdfs:isDefinedBy rdf:resource="http://data.europa.eu/a4g/ontology#sub"/>
   </rdf:Description>
   <owl:ObjectProperty rdf:about="http://data.europa.eu/a4g/ontology#refersToOtherESPDResponse"/>
   <rdf:Description rdf:about="http://data.europa.eu/a4g/ontology#refersToOtherESPDResponse">
      <skos:prefLabel xml:lang="en">Refers to other e s p d response</skos:prefLabel>
   </rdf:Description>
   <rdf:Description rdf:about="http://data.europa.eu/a4g/ontology#refersToOtherESPDResponse">
      <skos:definition xml:lang="en">Reference to other European Single Procurement Document (ESPD) Response. WG approval 05/03/2024 (epo-sub:ESPDResponse -&gt; epo-sub:ESPDResponse (+epo-sub:refersToOtherESPDResponse))</skos:definition>
   </rdf:Description>
   <rdf:Description rdf:about="http://data.europa.eu/a4g/ontology#refersToOtherESPDResponse">
      <rdfs:isDefinedBy rdf:resource="http://data.europa.eu/a4g/ontology#sub"/>
   </rdf:Description>
   <owl:ObjectProperty rdf:about="http://data.europa.eu/a4g/ontology#providesInformationOn"/>
   <rdf:Description rdf:about="http://data.europa.eu/a4g/ontology#providesInformationOn">
      <skos:prefLabel xml:lang="en">Provides information on</skos:prefLabel>
   </rdf:Description>
   <rdf:Description rdf:about="http://data.europa.eu/a4g/ontology#providesInformationOn">
      <skos:definition xml:lang="en">Offers information about an instance of a concept. WG approval 05/03/2024 (epo-sub:ESPDResponse -&gt; org:Organization (+epo-sub:providesInformationOn))</skos:definition>
   </rdf:Description>
   <rdf:Description rdf:about="http://data.europa.eu/a4g/ontology#providesInformationOn">
      <rdfs:isDefinedBy rdf:resource="http://data.europa.eu/a4g/ontology#sub"/>
   </rdf:Description>
   <owl:ObjectProperty rdf:about="http://data.europa.eu/a4g/ontology#answersSelectionCriteria"/>
   <rdf:Description rdf:about="http://data.europa.eu/a4g/ontology#answersSelectionCriteria">
      <skos:prefLabel xml:lang="en">Answers selection criteria</skos:prefLabel>
   </rdf:Description>
   <rdf:Description rdf:about="http://data.europa.eu/a4g/ontology#answersSelectionCriteria">
      <rdfs:isDefinedBy rdf:resource="http://data.europa.eu/a4g/ontology#sub"/>
   </rdf:Description>
   <owl:ObjectProperty rdf:about="http://data.europa.eu/a4g/ontology#isSupportedBy"/>
   <rdf:Description rdf:about="http://data.europa.eu/a4g/ontology#isSupportedBy">
      <skos:prefLabel xml:lang="en">Is supported by</skos:prefLabel>
   </rdf:Description>
   <rdf:Description rdf:about="http://data.europa.eu/a4g/ontology#isSupportedBy">
      <rdfs:isDefinedBy rdf:resource="http://data.europa.eu/a4g/ontology#sub"/>
   </rdf:Description>
   <owl:ObjectProperty rdf:about="http://data.europa.eu/a4g/ontology#hasPowerOfAttorney"/>
   <rdf:Description rdf:about="http://data.europa.eu/a4g/ontology#hasPowerOfAttorney">
      <skos:prefLabel xml:lang="en">Has power of attorney</skos:prefLabel>
   </rdf:Description>
   <rdf:Description rdf:about="http://data.europa.eu/a4g/ontology#hasPowerOfAttorney">
      <skos:definition xml:lang="en">Relation indicating that a Legal Representative has a Power of Attorney. WG approval 12/03/2024 (epo-sub:LegalRepresentative -&gt; epo-sub:PowerOfAttorney (+epo-sub:hasPowerOfAttorney))</skos:definition>
   </rdf:Description>
   <rdf:Description rdf:about="http://data.europa.eu/a4g/ontology#hasPowerOfAttorney">
      <rdfs:isDefinedBy rdf:resource="http://data.europa.eu/a4g/ontology#sub"/>
   </rdf:Description>
   <owl:ObjectProperty rdf:about="http://data.europa.eu/a4g/ontology#actsOnBehalfOf"/>
   <rdf:Description rdf:about="http://data.europa.eu/a4g/ontology#actsOnBehalfOf">
      <skos:prefLabel xml:lang="en">Acts on behalf of</skos:prefLabel>
   </rdf:Description>
   <rdf:Description rdf:about="http://data.europa.eu/a4g/ontology#actsOnBehalfOf">
      <rdfs:isDefinedBy rdf:resource="http://data.europa.eu/a4g/ontology#sub"/>
   </rdf:Description>
   <owl:ObjectProperty rdf:about="http://data.europa.eu/a4g/ontology#hasMandate"/>
   <rdf:Description rdf:about="http://data.europa.eu/a4g/ontology#hasMandate">
      <skos:prefLabel xml:lang="en">Has mandate</skos:prefLabel>
   </rdf:Description>
   <rdf:Description rdf:about="http://data.europa.eu/a4g/ontology#hasMandate">
      <skos:definition xml:lang="en">Relation indicating that a Legal Representative has a Mandate. WG approval 12/03/2024 (epo-sub:LegalRepresentative -&gt; epo-sub:Mandate (+epo-sub:hasMandate))</skos:definition>
   </rdf:Description>
   <rdf:Description rdf:about="http://data.europa.eu/a4g/ontology#hasMandate">
      <rdfs:isDefinedBy rdf:resource="http://data.europa.eu/a4g/ontology#sub"/>
   </rdf:Description>
   <owl:ObjectProperty rdf:about="http://data.europa.eu/a4g/ontology#providesOrganisationPreQualificationListingIdentifier"/>
   <rdf:Description rdf:about="http://data.europa.eu/a4g/ontology#providesOrganisationPreQualificationListingIdentifier">
      <skos:prefLabel xml:lang="en">Provides organisation pre qualification listing identifier</skos:prefLabel>
   </rdf:Description>
   <rdf:Description rdf:about="http://data.europa.eu/a4g/ontology#providesOrganisationPreQualificationListingIdentifier">
      <skos:definition xml:lang="en">The identifier assigned to an economic operator in a national pre-qualification system or official list. WG approval 05/03/2024 (epo-sub:NationalPreQualificationData -&gt; adms:Identifier (+epo-sub:providesOrganisationPreQualificationListingIdentifier))</skos:definition>
   </rdf:Description>
   <rdf:Description rdf:about="http://data.europa.eu/a4g/ontology#providesOrganisationPreQualificationListingIdentifier">
      <rdfs:isDefinedBy rdf:resource="http://data.europa.eu/a4g/ontology#sub"/>
   </rdf:Description>
   <owl:ObjectProperty rdf:about="http://data.europa.eu/a4g/ontology#providesOrganisationEmployeeQuantity"/>
   <rdf:Description rdf:about="http://data.europa.eu/a4g/ontology#providesOrganisationEmployeeQuantity">
      <skos:prefLabel xml:lang="en">Provides organisation employee quantity</skos:prefLabel>
   </rdf:Description>
   <rdf:Description rdf:about="http://data.europa.eu/a4g/ontology#providesOrganisationEmployeeQuantity">
      <skos:definition xml:lang="en">The number of people hired by the Organization. WG approval 05/03/2024 (epo-sub:NationalPreQualificationData -&gt; epo:Quantity (+epo-sub:providesOrganisationEmployeeQuantity))</skos:definition>
   </rdf:Description>
   <rdf:Description rdf:about="http://data.europa.eu/a4g/ontology#providesOrganisationEmployeeQuantity">
      <rdfs:isDefinedBy rdf:resource="http://data.europa.eu/a4g/ontology#sub"/>
   </rdf:Description>
   <owl:ObjectProperty rdf:about="http://data.europa.eu/a4g/ontology#providesOrganisationFinancialCapability"/>
   <rdf:Description rdf:about="http://data.europa.eu/a4g/ontology#providesOrganisationFinancialCapability">
      <skos:prefLabel xml:lang="en">Provides organisation financial capability</skos:prefLabel>
   </rdf:Description>
   <rdf:Description rdf:about="http://data.europa.eu/a4g/ontology#providesOrganisationFinancialCapability">
      <skos:definition xml:lang="en">A monetary amount representing the financial capability of the Organization. Additional information: Used to represent the general Turnover of the Organization (for statistical purposes). WG approval 05/03/2024 (epo-sub:NationalPreQualificationData -&gt; epo:MonetaryValue (+epo-sub:providesOrganisationFinancialCapability))</skos:definition>
   </rdf:Description>
   <rdf:Description rdf:about="http://data.europa.eu/a4g/ontology#providesOrganisationFinancialCapability">
      <rdfs:isDefinedBy rdf:resource="http://data.europa.eu/a4g/ontology#sub"/>
   </rdf:Description>
   <owl:ObjectProperty rdf:about="http://data.europa.eu/a4g/ontology#concernsOrganisation"/>
   <rdf:Description rdf:about="http://data.europa.eu/a4g/ontology#concernsOrganisation">
      <skos:prefLabel xml:lang="en">Concerns organisation</skos:prefLabel>
   </rdf:Description>
   <rdf:Description rdf:about="http://data.europa.eu/a4g/ontology#concernsOrganisation">
      <skos:definition xml:lang="en">Relates to Organization. WG approval 05/03/2024 (epo-sub:NationalPreQualificationData -&gt; org:Organization (+epo-sub:concernsOrganisation))</skos:definition>
   </rdf:Description>
   <rdf:Description rdf:about="http://data.europa.eu/a4g/ontology#concernsOrganisation">
      <rdfs:isDefinedBy rdf:resource="http://data.europa.eu/a4g/ontology#sub"/>
   </rdf:Description>
   <owl:ObjectProperty rdf:about="http://data.europa.eu/m8g/confidentialityLevelType"/>
   <rdf:Description rdf:about="http://data.europa.eu/m8g/confidentialityLevelType">
      <skos:prefLabel xml:lang="en">Confidentiality level type</skos:prefLabel>
   </rdf:Description>
   <rdf:Description rdf:about="http://data.europa.eu/m8g/confidentialityLevelType">
      <skos:definition xml:lang="en">Security classification assigned to an Evidence e.g. classified, sensitive, public. Additional Information: Classifications should be defined by an organisation/country as an outcome of a security assessment. (epo-sub:Response -&gt; at-voc:access-rights (+cccev:confidentialityLevelType))</skos:definition>
   </rdf:Description>
   <owl:ObjectProperty rdf:about="http://data.europa.eu/a4g/ontology#answersQuestion"/>
   <rdf:Description rdf:about="http://data.europa.eu/a4g/ontology#answersQuestion">
      <skos:prefLabel xml:lang="en">Answers question</skos:prefLabel>
   </rdf:Description>
   <rdf:Description rdf:about="http://data.europa.eu/a4g/ontology#answersQuestion">
      <skos:definition xml:lang="en">Relation indicating that the Response replies to a question. WG approval 12/03/2024 (epo-sub:Response -&gt; cccev:InformationRequirement (+epo-sub:answersQuestion))</skos:definition>
   </rdf:Description>
   <rdf:Description rdf:about="http://data.europa.eu/a4g/ontology#answersQuestion">
      <rdfs:isDefinedBy rdf:resource="http://data.europa.eu/a4g/ontology#sub"/>
   </rdf:Description>
   <owl:ObjectProperty rdf:about="http://data.europa.eu/a4g/ontology#isReinforcedBy"/>
   <rdf:Description rdf:about="http://data.europa.eu/a4g/ontology#isReinforcedBy">
      <skos:prefLabel xml:lang="en">Is reinforced by</skos:prefLabel>
   </rdf:Description>
   <rdf:Description rdf:about="http://data.europa.eu/a4g/ontology#isReinforcedBy">
      <skos:definition xml:lang="en">Relation indicating an Evidence that supports the Response. WG approval 12/03/2024 (epo-sub:Response -&gt; cccev:Evidence (+epo-sub:isReinforcedBy))</skos:definition>
   </rdf:Description>
   <rdf:Description rdf:about="http://data.europa.eu/a4g/ontology#isReinforcedBy">
      <rdfs:isDefinedBy rdf:resource="http://data.europa.eu/a4g/ontology#sub"/>
   </rdf:Description>
   <owl:ObjectProperty rdf:about="http://data.europa.eu/a4g/ontology#refersToApplicablePeriod"/>
   <rdf:Description rdf:about="http://data.europa.eu/a4g/ontology#refersToApplicablePeriod">
      <skos:prefLabel xml:lang="en">Refers to applicable period</skos:prefLabel>
   </rdf:Description>
   <rdf:Description rdf:about="http://data.europa.eu/a4g/ontology#refersToApplicablePeriod">
      <skos:definition xml:lang="en">Relation indicating the period to which the Response shall apply. WG approval 12/03/2024 (epo-sub:Response -&gt; epo:Period (+epo-sub:refersToApplicablePeriod))</skos:definition>
   </rdf:Description>
   <rdf:Description rdf:about="http://data.europa.eu/a4g/ontology#refersToApplicablePeriod">
      <rdfs:isDefinedBy rdf:resource="http://data.europa.eu/a4g/ontology#sub"/>
   </rdf:Description>
   <owl:DatatypeProperty rdf:about="http://data.europa.eu/m8g/value"/>
   <rdf:Description rdf:about="http://data.europa.eu/m8g/value">
      <skos:prefLabel xml:lang="en">Value</skos:prefLabel>
   </rdf:Description>
   <rdf:Description rdf:about="http://data.europa.eu/m8g/value">
      <skos:definition xml:lang="en">Value for the Information Concept that the Evidence supports. (cccev:SupportedValue)</skos:definition>
   </rdf:Description>
   <owl:DatatypeProperty rdf:about="http://data.europa.eu/a4g/ontology#coversAllSelectionCriteria"/>
   <rdf:Description rdf:about="http://data.europa.eu/a4g/ontology#coversAllSelectionCriteria">
      <skos:prefLabel xml:lang="en">Covers all selection criteria</skos:prefLabel>
   </rdf:Description>
   <rdf:Description rdf:about="http://data.europa.eu/a4g/ontology#coversAllSelectionCriteria">
      <skos:definition xml:lang="en">Indicator that the Certificate proves whether the Organization fulfils all Selection Criteria. WG approval 12/03/2024 (epo-sub:CertificateInformation)</skos:definition>
   </rdf:Description>
   <rdf:Description rdf:about="http://data.europa.eu/a4g/ontology#coversAllSelectionCriteria">
      <rdfs:isDefinedBy rdf:resource="http://data.europa.eu/a4g/ontology#sub"/>
   </rdf:Description>
   <owl:DatatypeProperty rdf:about="http://purl.org/dc/terms/description"/>
   <rdf:Description rdf:about="http://purl.org/dc/terms/description">
      <skos:prefLabel xml:lang="en">Description</skos:prefLabel>
   </rdf:Description>
   <rdf:Description rdf:about="http://purl.org/dc/terms/description">
      <skos:definition xml:lang="en">An account of the resource. Additional Information: Description may include but is not limited to: an abstract, a table of contents, a graphical representation, or a free-text account of the resource. WG Approval 30/05/2023 (epo-sub:CertificateInformation)</skos:definition>
   </rdf:Description>
   <owl:DatatypeProperty rdf:about="http://data.europa.eu/a4g/ontology#providesOrganisationCompletedTaskDescription"/>
   <rdf:Description rdf:about="http://data.europa.eu/a4g/ontology#providesOrganisationCompletedTaskDescription">
      <skos:prefLabel xml:lang="en">Provides organisation completed task description</skos:prefLabel>
   </rdf:Description>
   <rdf:Description rdf:about="http://data.europa.eu/a4g/ontology#providesOrganisationCompletedTaskDescription">
      <skos:definition xml:lang="en">Text describing the works, supplies or services executed, delivered or performed in a procurement project that can be used as an evidence for the classification of the Organization. WG approval 05/03/2024 (epo-sub:NationalPreQualificationData)</skos:definition>
   </rdf:Description>
   <rdf:Description rdf:about="http://data.europa.eu/a4g/ontology#providesOrganisationCompletedTaskDescription">
      <rdfs:isDefinedBy rdf:resource="http://data.europa.eu/a4g/ontology#sub"/>
   </rdf:Description>
</rdf:RDF>
