@prefix : <http://data.europa.eu/a4g/ontology#> .
@prefix cccev: <http://data.europa.eu/m8g/> .
@prefix dcterms: <http://purl.org/dc/terms/> .
@prefix eli: <http://data.europa.eu/eli/ontology#> .
@prefix foaf: <http://xmlns.com/foaf/0.1/> .
@prefix frbroo: <http://iflastandards.info/ns/fr/frbr/frbroo/> .
@prefix org: <http://www.w3.org/ns/org#> .
@prefix owl: <http://www.w3.org/2002/07/owl#> .
@prefix rdf: <http://www.w3.org/1999/02/22-rdf-syntax-ns#> .
@prefix rdfs: <http://www.w3.org/2000/01/rdf-schema#> .
@prefix skos: <http://www.w3.org/2004/02/skos/core#> .
@prefix vann: <http://purl.org/vocab/vann/> .
@prefix xsd: <http://www.w3.org/2001/XMLSchema#> .

:CertificateInformation a owl:Class ;
    rdfs:isDefinedBy :sub ;
    rdfs:subClassOf :ContextDescription ;
    skos:definition "Information about a Certificate. WG approval 12/03/2024"@en ;
    skos:prefLabel "Certificate information"@en .

:ESPD a owl:Class ;
    rdfs:isDefinedBy :sub ;
    rdfs:subClassOf :Document ;
    skos:definition "A document conveying the fulfilment or not by the economic operator of the Exclusion Grounds and the Selection Criteria set out by the Buyer for a specific Procurement using an European Single Procurement Document (ESPD) Request. WG Approval 05/03/2024"@en ;
    skos:prefLabel "E s p d"@en .

:LegalRepresentative a owl:Class ;
    rdfs:isDefinedBy :sub ;
    rdfs:subClassOf :AuxiliaryParty ;
    skos:definition "The Role of an Agent that can represent an Organization. WG approval 05/03/2024"@en ;
    skos:prefLabel "Legal representative"@en .

:Mandate a owl:Class ;
    rdfs:isDefinedBy :sub ;
    rdfs:subClassOf :Document ;
    skos:definition "An authorization to act as a representative of an Organization. WG approval 05/03/2024"@en ;
    skos:prefLabel "Mandate"@en .

:NationalPreQualificationData a owl:Class ;
    rdfs:isDefinedBy :sub ;
    skos:definition "Data that describe the distinctive features or characteristics that qualify an economic operator to take part in a tendering process. WG approval 05/03/2024"@en ;
    skos:prefLabel "National pre qualification data"@en .

:PowerOfAttorney a owl:Class ;
    rdfs:isDefinedBy :sub ;
    rdfs:subClassOf :Document ;
    skos:definition "A legal document that grants someone the authority to make decisions on behalf of an Organization. WG approval 05/03/2024"@en ;
    skos:prefLabel "Power of attorney"@en .

:Response a owl:Class ;
    rdfs:isDefinedBy :sub ;
    skos:definition "An answer given to a question that is part of an ESPD Request. WG approval 12/03/2024"@en ;
    skos:prefLabel "Response"@en .

:actsOnBehalfOf a owl:ObjectProperty ;
    rdfs:isDefinedBy :sub ;
    skos:prefLabel "Acts on behalf of"@en .

:answersQuestion a owl:ObjectProperty ;
    rdfs:isDefinedBy :sub ;
    skos:definition "Relation indicating that the Response replies to a question. WG approval 12/03/2024 (epo-sub:Response -> cccev:InformationRequirement (+epo-sub:answersQuestion))"@en ;
    skos:prefLabel "Answers question"@en .

:concernsOrganisation a owl:ObjectProperty ;
    rdfs:isDefinedBy :sub ;
    skos:definition "Relates to Organization. WG approval 05/03/2024 (epo-sub:NationalPreQualificationData -> org:Organization (+epo-sub:concernsOrganisation))"@en ;
    skos:prefLabel "Concerns organisation"@en .

:coversAllSelectionCriteria a owl:DatatypeProperty ;
    rdfs:isDefinedBy :sub ;
    skos:definition "Indicator that the Certificate proves whether the Organization fulfils all Selection Criteria. WG approval 12/03/2024 (epo-sub:CertificateInformation)"@en ;
    skos:prefLabel "Covers all selection criteria"@en .

:hasMandate a owl:ObjectProperty ;
    rdfs:isDefinedBy :sub ;
    skos:definition "Relation indicating that a Legal Representative has a Mandate. WG approval 12/03/2024 (epo-sub:LegalRepresentative -> epo-sub:Mandate (+epo-sub:hasMandate))"@en ;
    skos:prefLabel "Has mandate"@en .

:hasPowerOfAttorney a owl:ObjectProperty ;
    rdfs:isDefinedBy :sub ;
    skos:definition "Relation indicating that a Legal Representative has a Power of Attorney. WG approval 12/03/2024 (epo-sub:LegalRepresentative -> epo-sub:PowerOfAttorney (+epo-sub:hasPowerOfAttorney))"@en ;
    skos:prefLabel "Has power of attorney"@en .

:isReinforcedBy a owl:ObjectProperty ;
    rdfs:isDefinedBy :sub ;
    skos:definition "Relation indicating an Evidence that supports the Response. WG approval 12/03/2024 (epo-sub:Response -> cccev:Evidence (+epo-sub:isReinforcedBy))"@en ;
    skos:prefLabel "Is reinforced by"@en .

:isSupportedBy a owl:ObjectProperty ;
    rdfs:isDefinedBy :sub ;
    skos:prefLabel "Is supported by"@en .

:providesInformationOn a owl:ObjectProperty ;
    rdfs:isDefinedBy :sub ;
    skos:definition "Offers information about an instance of a concept. WG approval 05/03/2024 (epo-sub:ESPD -> org:Organization (+epo-sub:providesInformationOn))"@en ;
    skos:prefLabel "Provides information on"@en .

:providesOrganisationCompletedTaskDescription a owl:DatatypeProperty ;
    rdfs:isDefinedBy :sub ;
    skos:definition "Text describing the works, supplies or services executed, delivered or performed in a procurement project that can be used as an evidence for the classification of the Organization. WG approval 05/03/2024 (epo-sub:NationalPreQualificationData)"@en ;
    skos:prefLabel "Provides organisation completed task description"@en .

:providesOrganisationEmployeeQuantity a owl:ObjectProperty ;
    rdfs:isDefinedBy :sub ;
    skos:definition "The number of people hired by the Organization. WG approval 05/03/2024 (epo-sub:NationalPreQualificationData -> epo:Quantity (+epo-sub:providesOrganisationEmployeeQuantity))"@en ;
    skos:prefLabel "Provides organisation employee quantity"@en .

:providesOrganisationFinancialCapability a owl:ObjectProperty ;
    rdfs:isDefinedBy :sub ;
    skos:definition "A monetary amount representing the financial capability of the Organization. Additional information: Used to represent the general Turnover of the Organization (for statistical purposes). WG approval 05/03/2024 (epo-sub:NationalPreQualificationData -> epo:MonetaryValue (+epo-sub:providesOrganisationFinancialCapability))"@en ;
    skos:prefLabel "Provides organisation financial capability"@en .

:providesOrganisationPreQualificationListingIdentifier a owl:ObjectProperty ;
    rdfs:isDefinedBy :sub ;
    skos:definition "The identifier assigned to an economic operator in a national pre-qualification system or official list. WG approval 05/03/2024 (epo-sub:NationalPreQualificationData -> adms:Identifier (+epo-sub:providesOrganisationPreQualificationListingIdentifier))"@en ;
    skos:prefLabel "Provides organisation pre qualification listing identifier"@en .

:refersToApplicablePeriod a owl:ObjectProperty ;
    rdfs:isDefinedBy :sub ;
    skos:definition "Relation indicating the period to which the Response shall apply. WG approval 12/03/2024 (epo-sub:Response -> epo:Period (+epo-sub:refersToApplicablePeriod))"@en ;
    skos:prefLabel "Refers to applicable period"@en .

:refersToOtherESPDResponse a owl:ObjectProperty ;
    rdfs:isDefinedBy :sub ;
    skos:definition "Reference to other European Single Procurement Document (ESPD) Response. WG approval 05/03/2024 (epo-sub:ESPD -> epo-sub:ESPD (+epo-sub:refersToOtherESPDResponse))"@en ;
    skos:prefLabel "Refers to other e s p d response"@en .

:relatesToESPDRequest a owl:ObjectProperty ;
    rdfs:isDefinedBy :sub ;
    skos:definition "Is about an European Single Procurement Document (ESPD) Request. WG approval 05/03/2024 (epo-sub:ESPD -> epo-acc:ESPDRequest (+epo-sub:relatesToESPDRequest))"@en ;
    skos:prefLabel "Relates to e s p d request"@en .

:specifiesResponse a owl:ObjectProperty ;
    rdfs:isDefinedBy :sub ;
    skos:definition "Relation indicating that an ESPD Response contains a Response. WG approval 12/03/2024 (epo-sub:ESPD -> epo-sub:Response (+epo-sub:specifiesResponse))"@en ;
    skos:prefLabel "Specifies response"@en .

:summarisesInformationAboutCertificate a owl:ObjectProperty ;
    rdfs:isDefinedBy :sub ;
    skos:definition "Relation indicating the Certificate that the information refers to. WG approval 12/03/2024 (epo-sub:CertificateInformation -> epo:Certificate (+epo-sub:summarisesInformationAboutCertificate))"@en ;
    skos:prefLabel "Summarises information about certificate"@en .

cccev:SupportedValue a owl:Class ;
    skos:definition "Value for an Information Concept that is provided by an Evidence. Additional Information: The notion of Supported Value is closely related to actual data exchange between two parties: (a) the Requirement processor, i.e. the Agent setting out Requirements for an objective and processing the supplied Evidences in the context of the Requirements, and (b) the Evidence provider, i.e. the Agent supplying information to an information request expressed as Requirements. The Requirement processor has expressed its expectations (both business as technical) for the information it wants to recieve as an Information Concept. The Evidence provider is able to supply information for that Information Concept, but its native data representation might not be coherent with the expectations set by the Requirement processor. The Supported Value is bridging both. The Evidence provider can either provide a derived value (fact) from its native data representation that complies with the Information Concept expectations. Or it can provide a query in an agreed language between Evidence provider and Requirement processor that allows the Requirement processor to retrieve the value from the native data representation. Implementers are free to choose their language. It is recommended to document the made agreements well."@en ;
    skos:prefLabel "Supported value"@en .

cccev:confidentialityLevelType a owl:ObjectProperty ;
    skos:definition "Security classification assigned to an Evidence e.g. classified, sensitive, public. Additional Information: Classifications should be defined by an organisation/country as an outcome of a security assessment. (epo-sub:Response -> at-voc:access-rights (+cccev:confidentialityLevelType))"@en ;
    skos:prefLabel "Confidentiality level type"@en .

cccev:providesValueFor a owl:ObjectProperty ;
    skos:definition "Information Concept for which the Supported Value provides a value. (cccev:SupportedValue -> cccev:InformationConcept (+cccev:providesValueFor))"@en ;
    skos:prefLabel "Provides value for"@en .

cccev:supportsValue a owl:ObjectProperty ;
    skos:definition "Supported Value that the Evidence contains. (epo-sub:Response -> cccev:SupportedValue (+cccev:supportsValue)) Supported Value that the Evidence contains. (cccev:Evidence -> cccev:SupportedValue (+cccev:supportsValue))"@en ;
    skos:prefLabel "Supports value"@en .

cccev:value a owl:DatatypeProperty ;
    skos:definition "Value for the Information Concept that the Evidence supports. (cccev:SupportedValue)"@en ;
    skos:prefLabel "Value"@en .

dcterms:description a owl:DatatypeProperty ;
    skos:definition "An account of the resource. Additional Information: Description may include but is not limited to: an abstract, a table of contents, a graphical representation, or a free-text account of the resource. WG Approval 30/05/2023 (epo-sub:CertificateInformation)"@en ;
    skos:prefLabel "Description"@en .

rdf:PlainLiteral a rdfs:Datatype ;
    skos:prefLabel "Plain literal"@en .

xsd:anyURI a rdfs:Datatype ;
    skos:prefLabel "Any u r i"@en .

xsd:boolean a rdfs:Datatype ;
    skos:prefLabel "Boolean"@en .

xsd:date a rdfs:Datatype ;
    skos:prefLabel "Date"@en .

xsd:dateTime a rdfs:Datatype ;
    skos:prefLabel "Date time"@en .

xsd:decimal a rdfs:Datatype ;
    skos:prefLabel "Decimal"@en .

xsd:integer a rdfs:Datatype ;
    skos:prefLabel "Integer"@en .

:sub a owl:Ontology ;
    rdfs:label "eProcurement Ontology Submission - core"@en ;
    dcterms:created "2021-06-01"^^xsd:date ;
    dcterms:description "The eProcurement Ontology Submission core describes the concepts and properties representing the European Public Procurement Submission domain. The provision of these semantics offers the basis for a common understanding of the domain for all stakeholders ensuring the quality of data exchange and transparency. The ontology restrictions are published in a separate artefact."@en ;
    dcterms:issued "2024-07-23"^^xsd:date ;
    dcterms:license "© European Union, 2014. Unless otherwise noted, the reuse of the Ontology is authorised under the European Union Public Licence v1.2 (https://eupl.eu/)." ;
    dcterms:publisher "http://publications.europa.eu/resource/authority/corporate-body/PUBL" ;
    dcterms:title "eProcurement Ontology Submission - core"@en ;
    vann:preferredNamespacePrefix "epo" ;
    vann:preferredNamespaceUri "http://data.europa.eu/a4g/ontology#" ;
    rdfs:comment "This version is automatically generated from eSubmission.xml on 2024-07-23" ;
    rdfs:seeAlso <https://docs.ted.europa.eu/home/index.html>,
        <https://github.com/OP-TED/ePO/releases>,
        <https://joinup.ec.europa.eu/collection/eprocurement/solution/eprocurement-ontology/about>,
        <https://op.europa.eu/en/web/eu-vocabularies/e-procurement> ;
    owl:imports :acc,
        :core,
        eli:,
        cccev:,
        frbroo:,
        dcterms:,
        vann:,
        <http://www.w3.org/2004/02/skos/core>,
        <http://www.w3.org/2006/time>,
        <http://www.w3.org/ns/adms>,
        <http://www.w3.org/ns/locn>,
        org:,
        <http://www.w3.org/ns/person>,
        foaf: ;
    owl:incompatibleWith "3.1.0" ;
    owl:priorVersion "http://data.europa.eu/a4g/ontology#sub-4.1.0" ;
    owl:versionIRI :sub-4.2.0 ;
    owl:versionInfo "4.2.0" .

