<?xml version="1.0" encoding="UTF-8"?>
<rdf:RDF xmlns="http://data.europa.eu/a4g/ontology#"
         xmlns:adms="http://www.w3.org/ns/adms#"
         xmlns:at-voc="http://publications.europa.eu/resource/authority/"
         xmlns:at-voc-new="http://publications.europa.eu/resource/authority/new/"
         xmlns:cccev="http://data.europa.eu/m8g/"
         xmlns:core="http://data.europa.eu/m8g/"
         xmlns:cpov="http://data.europa.eu/m8g/"
         xmlns:cpsv="http://data.europa.eu/m8g/"
         xmlns:cpv="http://data.europa.eu/m8g/"
         xmlns:cv="http://data.europa.eu/m8g/"
         xmlns:dc="http://purl.org/dc/elements/1.1/"
         xmlns:dct="http://purl.org/dc/terms/"
         xmlns:dul="http://www.ontologydesignpatterns.org/ont/dul/DUL.owl#"
         xmlns:eli="http://data.europa.eu/eli/ontology#"
         xmlns:epo="http://data.europa.eu/a4g/ontology#"
         xmlns:epo-acc="http://data.europa.eu/a4g/ontology#"
         xmlns:epo-cat="http://data.europa.eu/a4g/ontology#"
         xmlns:epo-con="http://data.europa.eu/a4g/ontology#"
         xmlns:epo-ful="http://data.europa.eu/a4g/ontology#"
         xmlns:epo-inv="http://data.europa.eu/a4g/ontology#"
         xmlns:epo-not="http://data.europa.eu/a4g/ontology#"
         xmlns:epo-ord="http://data.europa.eu/a4g/ontology#"
         xmlns:epo-sub="http://data.europa.eu/a4g/ontology#"
         xmlns:espd="https://github.com/ESPD/ESPD-EDM/"
         xmlns:foaf="http://xmlns.com/foaf/0.1/"
         xmlns:frbroo="http://iflastandards.info/ns/fr/frbr/frbroo/"
         xmlns:geosparql="http://www.opengis.net/ont/geosparql#"
         xmlns:locn="http://www.w3.org/ns/locn#"
         xmlns:nuts="http://data.europa.eu/nuts/"
         xmlns:org="http://www.w3.org/ns/org#"
         xmlns:owl="http://www.w3.org/2002/07/owl#"
         xmlns:person="http://www.w3.org/ns/person#"
         xmlns:rdf="http://www.w3.org/1999/02/22-rdf-syntax-ns#"
         xmlns:rdfs="http://www.w3.org/2000/01/rdf-schema#"
         xmlns:skos="http://www.w3.org/2004/02/skos/core#"
         xmlns:time="http://www.w3.org/2006/time#"
         xmlns:vann="http://purl.org/vocab/vann/"
         xmlns:xsd="http://www.w3.org/2001/XMLSchema#">
   <owl:Ontology rdf:about="http://data.europa.eu/a4g/ontology#ful">
      <owl:imports rdf:resource="http://xmlns.com/foaf/0.1/"/>
      <owl:imports rdf:resource="http://purl.org/dc/terms/"/>
      <owl:imports rdf:resource="http://www.w3.org/ns/org#"/>
      <owl:imports rdf:resource="http://www.w3.org/2004/02/skos/core"/>
      <owl:imports rdf:resource="http://data.europa.eu/a4g/ontology#core"/>
      <owl:imports rdf:resource="http://data.europa.eu/a4g/ontology#cat"/>
      <owl:imports rdf:resource="http://data.europa.eu/a4g/ontology#ord"/>
      <owl:imports rdf:resource="http://www.w3.org/2006/time"/>
      <owl:imports rdf:resource="http://www.w3.org/ns/locn"/>
      <owl:imports rdf:resource="http://data.europa.eu/m8g/"/>
      <owl:imports rdf:resource="http://data.europa.eu/m8g/"/>
      <owl:imports rdf:resource="http://data.europa.eu/m8g/"/>
      <owl:imports rdf:resource="http://data.europa.eu/m8g/"/>
      <owl:imports rdf:resource="http://data.europa.eu/m8g/"/>
      <owl:imports rdf:resource="http://data.europa.eu/m8g/"/>
      <owl:imports rdf:resource="http://www.w3.org/ns/person"/>
      <owl:imports rdf:resource="http://www.w3.org/ns/adms"/>
      <owl:imports rdf:resource="http://purl.org/vocab/vann/"/>
      <owl:imports rdf:resource="http://data.europa.eu/eli/ontology#"/>
      <owl:imports rdf:resource="http://iflastandards.info/ns/fr/frbr/frbroo/"/>
      <dct:title xml:lang="en">eProcurement Ontology Fulfilment - core</dct:title>
      <rdfs:label xml:lang="en">eProcurement Ontology Fulfilment - core</rdfs:label>
      <dct:description xml:lang="en">The eProcurement Ontology Fulfilment core describes the concepts and properties representing the European Public Procurement Fulfilment domain. The provision of these semantics offers the basis for a common understanding of the domain for all stakeholders ensuring the quality of data exchange and transparency. The ontology restrictions are published in a separate artefact.</dct:description>
      <dct:publisher>http://publications.europa.eu/resource/authority/corporate-body/PUBL</dct:publisher>
      <rdfs:comment>This version is automatically generated from eFulfilment.xml on 2024-07-23</rdfs:comment>
      <rdfs:seeAlso rdf:resource="https://github.com/OP-TED/ePO/releases"/>
      <rdfs:seeAlso rdf:resource="https://joinup.ec.europa.eu/collection/eprocurement/solution/eprocurement-ontology/about"/>
      <rdfs:seeAlso rdf:resource="https://op.europa.eu/en/web/eu-vocabularies/e-procurement"/>
      <rdfs:seeAlso rdf:resource="https://docs.ted.europa.eu/home/index.html"/>
      <dct:issued rdf:datatype="http://www.w3.org/2001/XMLSchema#date">2024-07-23</dct:issued>
      <dct:created rdf:datatype="http://www.w3.org/2001/XMLSchema#date">2021-06-01</dct:created>
      <owl:versionInfo>4.2.0</owl:versionInfo>
      <owl:incompatibleWith>3.1.0</owl:incompatibleWith>
      <owl:versionIRI rdf:resource="http://data.europa.eu/a4g/ontology#ful-4.2.0"/>
      <owl:priorVersion>http://data.europa.eu/a4g/ontology#ful-4.1.0</owl:priorVersion>
      <vann:preferredNamespaceUri>http://data.europa.eu/a4g/ontology#</vann:preferredNamespaceUri>
      <vann:preferredNamespacePrefix>epo</vann:preferredNamespacePrefix>
      <dct:license>Â© European Union, 2014. Unless otherwise noted, the reuse of the Ontology is authorised under the European Union Public Licence v1.2 (https://eupl.eu/).</dct:license>
   </owl:Ontology>
   <owl:Class rdf:about="http://data.europa.eu/a4g/ontology#TemperatureSpecification"/>
   <rdf:Description rdf:about="http://data.europa.eu/a4g/ontology#TemperatureSpecification">
      <skos:prefLabel xml:lang="en">Temperature specification</skos:prefLabel>
   </rdf:Description>
   <rdf:Description rdf:about="http://data.europa.eu/a4g/ontology#TemperatureSpecification">
      <skos:definition xml:lang="en">Description of the temperature requirements during shipment. WG approval 21/05/2024</skos:definition>
   </rdf:Description>
   <rdf:Description rdf:about="http://data.europa.eu/a4g/ontology#TemperatureSpecification">
      <rdfs:isDefinedBy rdf:resource="http://data.europa.eu/a4g/ontology#ful"/>
   </rdf:Description>
   <owl:Class rdf:about="http://data.europa.eu/a4g/ontology#AbstractContainer"/>
   <rdf:Description rdf:about="http://data.europa.eu/a4g/ontology#AbstractContainer">
      <skos:prefLabel xml:lang="en">Abstract container</skos:prefLabel>
   </rdf:Description>
   <rdf:Description rdf:about="http://data.europa.eu/a4g/ontology#AbstractContainer">
      <skos:definition xml:lang="en">Gathering class for Packages and Transport Handling Units. WG approval 14/05/2024</skos:definition>
   </rdf:Description>
   <rdf:Description rdf:about="http://data.europa.eu/a4g/ontology#AbstractContainer">
      <rdfs:isDefinedBy rdf:resource="http://data.europa.eu/a4g/ontology#ful"/>
   </rdf:Description>
   <owl:Class rdf:about="http://data.europa.eu/a4g/ontology#TransportMeansOperator"/>
   <rdf:Description rdf:about="http://data.europa.eu/a4g/ontology#TransportMeansOperator">
      <skos:prefLabel xml:lang="en">Transport means operator</skos:prefLabel>
   </rdf:Description>
   <rdf:Description rdf:about="http://data.europa.eu/a4g/ontology#TransportMeansOperator">
      <skos:definition xml:lang="en">The Role of an Agent who is responsible for controlling the Transport Means. WG approval 21/05/2024</skos:definition>
   </rdf:Description>
   <rdf:Description rdf:about="http://data.europa.eu/a4g/ontology#TransportMeansOperator">
      <rdfs:isDefinedBy rdf:resource="http://data.europa.eu/a4g/ontology#ful"/>
   </rdf:Description>
   <owl:Class rdf:about="http://data.europa.eu/a4g/ontology#GoodsItem"/>
   <rdf:Description rdf:about="http://data.europa.eu/a4g/ontology#GoodsItem">
      <skos:prefLabel xml:lang="en">Goods item</skos:prefLabel>
   </rdf:Description>
   <rdf:Description rdf:about="http://data.europa.eu/a4g/ontology#GoodsItem">
      <skos:definition xml:lang="en">An Item including its initial packaging during transportation. Additional information: For example, the Item being bought is the computer. The weight of the computer is X. The weight of the Goods Item is the weight of the computer plus the weight of the initial packaging. During transportation you have for example trace ID which is applied to the GoodsItem, rather than on the Item itself. The declared statistical value can only apply once you have a GoodsItem. WG approval 30/03/2023</skos:definition>
   </rdf:Description>
   <rdf:Description rdf:about="http://data.europa.eu/a4g/ontology#GoodsItem">
      <rdfs:isDefinedBy rdf:resource="http://data.europa.eu/a4g/ontology#ful"/>
   </rdf:Description>
   <owl:Class rdf:about="http://data.europa.eu/a4g/ontology#ShipmentAgreement"/>
   <rdf:Description rdf:about="http://data.europa.eu/a4g/ontology#ShipmentAgreement">
      <skos:prefLabel xml:lang="en">Shipment agreement</skos:prefLabel>
   </rdf:Description>
   <rdf:Description rdf:about="http://data.europa.eu/a4g/ontology#ShipmentAgreement">
      <skos:definition xml:lang="en">The commercial agreement between the Buyer and the Seller. Additional Information: The Shipment Agreement describes the items being shipped. WG approval 21/05/2024</skos:definition>
   </rdf:Description>
   <rdf:Description rdf:about="http://data.europa.eu/a4g/ontology#ShipmentAgreement">
      <rdfs:isDefinedBy rdf:resource="http://data.europa.eu/a4g/ontology#ful"/>
   </rdf:Description>
   <owl:Class rdf:about="http://data.europa.eu/a4g/ontology#TransportEquipmentSeal"/>
   <rdf:Description rdf:about="http://data.europa.eu/a4g/ontology#TransportEquipmentSeal">
      <skos:prefLabel xml:lang="en">Transport equipment seal</skos:prefLabel>
   </rdf:Description>
   <rdf:Description rdf:about="http://data.europa.eu/a4g/ontology#TransportEquipmentSeal">
      <skos:definition xml:lang="en">Means used to ensure that the Transport Equipment is not tampered during transportation. WG approval 21/05/2025</skos:definition>
   </rdf:Description>
   <rdf:Description rdf:about="http://data.europa.eu/a4g/ontology#TransportEquipmentSeal">
      <rdfs:isDefinedBy rdf:resource="http://data.europa.eu/a4g/ontology#ful"/>
   </rdf:Description>
   <owl:Class rdf:about="http://data.europa.eu/a4g/ontology#TransportMeans"/>
   <rdf:Description rdf:about="http://data.europa.eu/a4g/ontology#TransportMeans">
      <skos:prefLabel xml:lang="en">Transport means</skos:prefLabel>
   </rdf:Description>
   <rdf:Description rdf:about="http://data.europa.eu/a4g/ontology#TransportMeans">
      <skos:definition xml:lang="en">Description of a particular vehicle or vessel used for the conveyance of goods or persons. WG approval 21/05/2024</skos:definition>
   </rdf:Description>
   <rdf:Description rdf:about="http://data.europa.eu/a4g/ontology#TransportMeans">
      <rdfs:isDefinedBy rdf:resource="http://data.europa.eu/a4g/ontology#ful"/>
   </rdf:Description>
   <owl:Class rdf:about="http://data.europa.eu/a4g/ontology#ShipmentStage"/>
   <rdf:Description rdf:about="http://data.europa.eu/a4g/ontology#ShipmentStage">
      <skos:prefLabel xml:lang="en">Shipment stage</skos:prefLabel>
   </rdf:Description>
   <rdf:Description rdf:about="http://data.europa.eu/a4g/ontology#ShipmentStage">
      <skos:definition xml:lang="en">Part of the itinerary of a shipment. Additional information: In the context of fulfilment only the last part of the itinerary is taken into consideration. WG approval 21/05/2024</skos:definition>
   </rdf:Description>
   <rdf:Description rdf:about="http://data.europa.eu/a4g/ontology#ShipmentStage">
      <rdfs:isDefinedBy rdf:resource="http://data.europa.eu/a4g/ontology#ful"/>
   </rdf:Description>
   <owl:Class rdf:about="http://data.europa.eu/a4g/ontology#Package"/>
   <rdf:Description rdf:about="http://data.europa.eu/a4g/ontology#Package">
      <skos:prefLabel xml:lang="en">Package</skos:prefLabel>
   </rdf:Description>
   <rdf:Description rdf:about="http://data.europa.eu/a4g/ontology#Package">
      <skos:definition xml:lang="en">Container used for transportation. WG approval 14/05/2024</skos:definition>
   </rdf:Description>
   <rdf:Description rdf:about="http://data.europa.eu/a4g/ontology#Package">
      <rdfs:isDefinedBy rdf:resource="http://data.europa.eu/a4g/ontology#ful"/>
   </rdf:Description>
   <owl:Class rdf:about="http://data.europa.eu/a4g/ontology#TransportEquipment"/>
   <rdf:Description rdf:about="http://data.europa.eu/a4g/ontology#TransportEquipment">
      <skos:prefLabel xml:lang="en">Transport equipment</skos:prefLabel>
   </rdf:Description>
   <rdf:Description rdf:about="http://data.europa.eu/a4g/ontology#TransportEquipment">
      <skos:definition xml:lang="en">Description of the apparatus used during transportation. Additional information: The equipment may be a container, a trailer, means of assistance to load or unload the Goods Items. WG approval 21/05/2024</skos:definition>
   </rdf:Description>
   <rdf:Description rdf:about="http://data.europa.eu/a4g/ontology#TransportEquipment">
      <rdfs:isDefinedBy rdf:resource="http://data.europa.eu/a4g/ontology#ful"/>
   </rdf:Description>
   <owl:Class rdf:about="http://data.europa.eu/a4g/ontology#Notifier"/>
   <rdf:Description rdf:about="http://data.europa.eu/a4g/ontology#Notifier">
      <skos:prefLabel xml:lang="en">Notifier</skos:prefLabel>
   </rdf:Description>
   <rdf:Description rdf:about="http://data.europa.eu/a4g/ontology#Notifier">
      <skos:definition xml:lang="en">This class was wrongly named and has been replaced by epo-ful:NotificationReceiver. It will be removed in the next major release.</skos:definition>
   </rdf:Description>
   <rdf:Description rdf:about="http://data.europa.eu/a4g/ontology#Notifier">
      <rdfs:isDefinedBy rdf:resource="http://data.europa.eu/a4g/ontology#ful"/>
   </rdf:Description>
   <owl:Class rdf:about="http://data.europa.eu/a4g/ontology#FreightForwarder"/>
   <rdf:Description rdf:about="http://data.europa.eu/a4g/ontology#FreightForwarder">
      <skos:prefLabel xml:lang="en">Freight forwarder</skos:prefLabel>
   </rdf:Description>
   <rdf:Description rdf:about="http://data.europa.eu/a4g/ontology#FreightForwarder">
      <skos:definition xml:lang="en">The Role of an Agent who organise the logistic operations need for a fulfilment. WG approval 21/05/2024</skos:definition>
   </rdf:Description>
   <rdf:Description rdf:about="http://data.europa.eu/a4g/ontology#FreightForwarder">
      <rdfs:isDefinedBy rdf:resource="http://data.europa.eu/a4g/ontology#ful"/>
   </rdf:Description>
   <owl:Class rdf:about="http://data.europa.eu/a4g/ontology#Consignment"/>
   <rdf:Description rdf:about="http://data.europa.eu/a4g/ontology#Consignment">
      <skos:prefLabel xml:lang="en">Consignment</skos:prefLabel>
   </rdf:Description>
   <rdf:Description rdf:about="http://data.europa.eu/a4g/ontology#Consignment">
      <skos:definition xml:lang="en">A batch of goods destined for or delivered to someone. Additional information: Consignment is a Transport Agreement between the Despatcher and the Consignee as to who and how the goods are despatched and received. WG approval 14/05/2024</skos:definition>
   </rdf:Description>
   <rdf:Description rdf:about="http://data.europa.eu/a4g/ontology#Consignment">
      <rdfs:isDefinedBy rdf:resource="http://data.europa.eu/a4g/ontology#ful"/>
   </rdf:Description>
   <owl:Class rdf:about="http://data.europa.eu/a4g/ontology#NotificationReceiver"/>
   <rdf:Description rdf:about="http://data.europa.eu/a4g/ontology#NotificationReceiver">
      <skos:prefLabel xml:lang="en">Notification receiver</skos:prefLabel>
   </rdf:Description>
   <rdf:Description rdf:about="http://data.europa.eu/a4g/ontology#NotificationReceiver">
      <skos:definition xml:lang="en">The Role of an Agent that is informed about the arrival of a Shipment at a destination. Additional information: This could be for example customs and excise. WG approval 21/05/2024</skos:definition>
   </rdf:Description>
   <rdf:Description rdf:about="http://data.europa.eu/a4g/ontology#NotificationReceiver">
      <rdfs:isDefinedBy rdf:resource="http://data.europa.eu/a4g/ontology#ful"/>
   </rdf:Description>
   <owl:Class rdf:about="http://data.europa.eu/a4g/ontology#DespatchLine"/>
   <rdf:Description rdf:about="http://data.europa.eu/a4g/ontology#DespatchLine">
      <skos:prefLabel xml:lang="en">Despatch line</skos:prefLabel>
   </rdf:Description>
   <rdf:Description rdf:about="http://data.europa.eu/a4g/ontology#DespatchLine">
      <skos:definition xml:lang="en">Details concerning the fulfilment of an Order Line. WG approval 21/05/2024</skos:definition>
   </rdf:Description>
   <rdf:Description rdf:about="http://data.europa.eu/a4g/ontology#DespatchLine">
      <rdfs:isDefinedBy rdf:resource="http://data.europa.eu/a4g/ontology#ful"/>
   </rdf:Description>
   <owl:Class rdf:about="http://data.europa.eu/a4g/ontology#TransportHandlingUnit"/>
   <rdf:Description rdf:about="http://data.europa.eu/a4g/ontology#TransportHandlingUnit">
      <skos:prefLabel xml:lang="en">Transport handling unit</skos:prefLabel>
   </rdf:Description>
   <rdf:Description rdf:about="http://data.europa.eu/a4g/ontology#TransportHandlingUnit">
      <skos:definition xml:lang="en">The outermost Package that the Carrier is handling. WG approval 14/05/2024</skos:definition>
   </rdf:Description>
   <rdf:Description rdf:about="http://data.europa.eu/a4g/ontology#TransportHandlingUnit">
      <rdfs:isDefinedBy rdf:resource="http://data.europa.eu/a4g/ontology#ful"/>
   </rdf:Description>
   <owl:Class rdf:about="http://data.europa.eu/a4g/ontology#ShipmentInformation"/>
   <rdf:Description rdf:about="http://data.europa.eu/a4g/ontology#ShipmentInformation">
      <skos:prefLabel xml:lang="en">Shipment information</skos:prefLabel>
   </rdf:Description>
   <rdf:Description rdf:about="http://data.europa.eu/a4g/ontology#ShipmentInformation">
      <skos:definition xml:lang="en">Information about the transportation of an identifiable collection of Goods Items from the Despatcher to the Consignee. WG approval 21/05/2024</skos:definition>
   </rdf:Description>
   <rdf:Description rdf:about="http://data.europa.eu/a4g/ontology#ShipmentInformation">
      <rdfs:isDefinedBy rdf:resource="http://data.europa.eu/a4g/ontology#ful"/>
   </rdf:Description>
   <owl:Class rdf:about="http://data.europa.eu/a4g/ontology#Despatcher"/>
   <rdf:Description rdf:about="http://data.europa.eu/a4g/ontology#Despatcher">
      <skos:prefLabel xml:lang="en">Despatcher</skos:prefLabel>
   </rdf:Description>
   <rdf:Description rdf:about="http://data.europa.eu/a4g/ontology#Despatcher">
      <skos:definition xml:lang="en">The Role of an Agent who sends the goods or notifies of the service or works execution. Additional Information: The Role is carried out by the Supplier or on behalf of the Supplier. This Role is often referred to as the Despatch Party, Consignor or Deliverer. WG approval 02/07/2024</skos:definition>
   </rdf:Description>
   <rdf:Description rdf:about="http://data.europa.eu/a4g/ontology#Despatcher">
      <rdfs:isDefinedBy rdf:resource="http://data.europa.eu/a4g/ontology#ful"/>
   </rdf:Description>
   <owl:Class rdf:about="http://data.europa.eu/a4g/ontology#DespatchAdvice"/>
   <rdf:Description rdf:about="http://data.europa.eu/a4g/ontology#DespatchAdvice">
      <skos:prefLabel xml:lang="en">Despatch advice</skos:prefLabel>
   </rdf:Description>
   <rdf:Description rdf:about="http://data.europa.eu/a4g/ontology#DespatchAdvice">
      <skos:definition xml:lang="en">A document notifying the sending of goods or the execution of works or services. WG approval 14/05/2024</skos:definition>
   </rdf:Description>
   <rdf:Description rdf:about="http://data.europa.eu/a4g/ontology#DespatchAdvice">
      <rdfs:isDefinedBy rdf:resource="http://data.europa.eu/a4g/ontology#ful"/>
   </rdf:Description>
   <owl:Class rdf:about="http://data.europa.eu/a4g/ontology#Carrier"/>
   <rdf:Description rdf:about="http://data.europa.eu/a4g/ontology#Carrier">
      <skos:prefLabel xml:lang="en">Carrier</skos:prefLabel>
   </rdf:Description>
   <rdf:Description rdf:about="http://data.europa.eu/a4g/ontology#Carrier">
      <skos:definition xml:lang="en">The Role of an Agent who handles the physical Delivery/Transportation of the (Despatched) Shipment. Additional Information: This Role is often referred to as the deliverer. WG approval 14/05/2024</skos:definition>
   </rdf:Description>
   <rdf:Description rdf:about="http://data.europa.eu/a4g/ontology#Carrier">
      <rdfs:isDefinedBy rdf:resource="http://data.europa.eu/a4g/ontology#ful"/>
   </rdf:Description>
   <owl:Class rdf:about="http://data.europa.eu/a4g/ontology#ReceiptAdvice"/>
   <rdf:Description rdf:about="http://data.europa.eu/a4g/ontology#ReceiptAdvice">
      <skos:prefLabel xml:lang="en">Receipt advice</skos:prefLabel>
   </rdf:Description>
   <rdf:Description rdf:about="http://data.europa.eu/a4g/ontology#ReceiptAdvice">
      <rdfs:isDefinedBy rdf:resource="http://data.europa.eu/a4g/ontology#ful"/>
   </rdf:Description>
   <owl:Class rdf:about="http://data.europa.eu/a4g/ontology#ReceiptAdviceLine"/>
   <rdf:Description rdf:about="http://data.europa.eu/a4g/ontology#ReceiptAdviceLine">
      <skos:prefLabel xml:lang="en">Receipt advice line</skos:prefLabel>
   </rdf:Description>
   <rdf:Description rdf:about="http://data.europa.eu/a4g/ontology#ReceiptAdviceLine">
      <rdfs:isDefinedBy rdf:resource="http://data.europa.eu/a4g/ontology#ful"/>
   </rdf:Description>
   <rdfs:Datatype rdf:about="http://www.w3.org/1999/02/22-rdf-syntax-ns#PlainLiteral"/>
   <rdf:Description rdf:about="http://www.w3.org/1999/02/22-rdf-syntax-ns#PlainLiteral">
      <skos:prefLabel xml:lang="en">Plain literal</skos:prefLabel>
   </rdf:Description>
   <rdfs:Datatype rdf:about="http://www.w3.org/2001/XMLSchema#anyURI"/>
   <rdf:Description rdf:about="http://www.w3.org/2001/XMLSchema#anyURI">
      <skos:prefLabel xml:lang="en">Any u r i</skos:prefLabel>
   </rdf:Description>
   <rdfs:Datatype rdf:about="http://www.w3.org/2001/XMLSchema#boolean"/>
   <rdf:Description rdf:about="http://www.w3.org/2001/XMLSchema#boolean">
      <skos:prefLabel xml:lang="en">Boolean</skos:prefLabel>
   </rdf:Description>
   <rdfs:Datatype rdf:about="http://www.w3.org/2001/XMLSchema#date"/>
   <rdf:Description rdf:about="http://www.w3.org/2001/XMLSchema#date">
      <skos:prefLabel xml:lang="en">Date</skos:prefLabel>
   </rdf:Description>
   <rdfs:Datatype rdf:about="http://www.w3.org/2001/XMLSchema#dateTime"/>
   <rdf:Description rdf:about="http://www.w3.org/2001/XMLSchema#dateTime">
      <skos:prefLabel xml:lang="en">Date time</skos:prefLabel>
   </rdf:Description>
   <rdfs:Datatype rdf:about="http://www.w3.org/2001/XMLSchema#decimal"/>
   <rdf:Description rdf:about="http://www.w3.org/2001/XMLSchema#decimal">
      <skos:prefLabel xml:lang="en">Decimal</skos:prefLabel>
   </rdf:Description>
   <rdfs:Datatype rdf:about="http://www.w3.org/2001/XMLSchema#integer"/>
   <rdf:Description rdf:about="http://www.w3.org/2001/XMLSchema#integer">
      <skos:prefLabel xml:lang="en">Integer</skos:prefLabel>
   </rdf:Description>
   <rdf:Description rdf:about="http://data.europa.eu/a4g/ontology#hasCarrierConsignmentID">
      <skos:editorialNote xml:lang="en">to be removed from future ePO version</skos:editorialNote>
   </rdf:Description>
   <rdf:Description rdf:about="http://data.europa.eu/a4g/ontology#hasFreightForwarderConsignmentID">
      <skos:editorialNote xml:lang="en">to be removed from future ePO version</skos:editorialNote>
   </rdf:Description>
   <rdf:Description rdf:about="http://data.europa.eu/a4g/ontology#Consignment">
      <skos:editorialNote xml:lang="en">to remove epo-ful:hasVehicleDescription</skos:editorialNote>
   </rdf:Description>
   <rdf:Description rdf:about="http://data.europa.eu/a4g/ontology#hasConsignmentFreeOnBoardValue">
      <skos:editorialNote xml:lang="en">to be removed in a future ePO version</skos:editorialNote>
   </rdf:Description>
   <rdf:Description rdf:about="http://data.europa.eu/a4g/ontology#hasConsignmentInvoiceValue">
      <skos:editorialNote xml:lang="en">to be removed in a future ePO version</skos:editorialNote>
   </rdf:Description>
   <rdf:Description rdf:about="http://data.europa.eu/a4g/ontology#hasFreightAllowanceCharge">
      <skos:editorialNote xml:lang="en">to be removed in a future ePO version</skos:editorialNote>
   </rdf:Description>
   <rdf:Description rdf:about="http://data.europa.eu/a4g/ontology#specifiesShipment">
      <skos:editorialNote xml:lang="en">proposal to be removed in the future ePO version</skos:editorialNote>
   </rdf:Description>
   <rdf:Description rdf:about="http://data.europa.eu/a4g/ontology#specifiesTransportHandlingUnits">
      <skos:editorialNote xml:lang="en">proposal to be removed in the future ePO version</skos:editorialNote>
   </rdf:Description>
   <rdf:Description rdf:about="http://data.europa.eu/a4g/ontology#specifiesShipment">
      <skos:editorialNote xml:lang="en">proposal to be removed in the future ePO version</skos:editorialNote>
   </rdf:Description>
   <rdf:Description rdf:about="http://data.europa.eu/a4g/ontology#specifiesTransportHandlingUnits">
      <skos:editorialNote xml:lang="en">proposal to be removed in the future ePO version</skos:editorialNote>
   </rdf:Description>
   <rdf:Description rdf:about="http://data.europa.eu/a4g/ontology#transportsItemFrom">
      <skos:editorialNote xml:lang="en">proposal to be removed in the future ePO version</skos:editorialNote>
   </rdf:Description>
   <rdf:Description rdf:about="http://data.europa.eu/a4g/ontology#TransportHandlingUnit">
      <skos:editorialNote xml:lang="en">we should re-use epo-ord:hasShippingMark instead of epo-ful:hasShippingMark.</skos:editorialNote>
   </rdf:Description>
   <rdf:Description rdf:about="http://data.europa.eu/a4g/ontology#hasConsignmentDeclaredStatisticsValue">
      <skos:editorialNote xml:lang="en">to be removed in a future ePO version and to re-use epo-ful:hasDeclaredStatisticalValue instead.</skos:editorialNote>
   </rdf:Description>
   <rdf:Description rdf:about="http://data.europa.eu/a4g/ontology#hasChargeableWeight">
      <skos:editorialNote xml:lang="en">to be removed from future ePO version</skos:editorialNote>
   </rdf:Description>
   <rdf:Description rdf:about="http://data.europa.eu/a4g/ontology#hasLoadingLength">
      <skos:editorialNote xml:lang="en">to be removed from future ePO version</skos:editorialNote>
   </rdf:Description>
   <rdf:Description rdf:about="http://data.europa.eu/a4g/ontology#Notifier">
      <skos:editorialNote xml:lang="en">This class was wrongly named and has been replaced by epo-ful:NotificationReceiver. It will be removed in the next major release.</skos:editorialNote>
   </rdf:Description>
   <rdf:Description rdf:about="http://data.europa.eu/a4g/ontology#TransportEquipment">
      <skos:editorialNote xml:lang="en">isReturnable attribute should be removed in a future release.</skos:editorialNote>
   </rdf:Description>
   <rdf:Description rdf:about="http://data.europa.eu/a4g/ontology#hasVehicleSegmentID">
      <skos:editorialNote xml:lang="en">used for rail car identifier.</skos:editorialNote>
   </rdf:Description>
   <owl:Class rdf:about="http://data.europa.eu/a4g/ontology#Package">
      <rdfs:subClassOf rdf:resource="http://data.europa.eu/a4g/ontology#AbstractContainer"/>
   </owl:Class>
   <owl:Class rdf:about="http://data.europa.eu/a4g/ontology#TransportMeansOperator">
      <rdfs:subClassOf rdf:resource="http://data.europa.eu/a4g/ontology#AuxiliaryParty"/>
   </owl:Class>
   <owl:Class rdf:about="http://data.europa.eu/a4g/ontology#Notifier">
      <rdfs:subClassOf rdf:resource="http://data.europa.eu/a4g/ontology#AuxiliaryParty"/>
   </owl:Class>
   <owl:Class rdf:about="http://data.europa.eu/a4g/ontology#FreightForwarder">
      <rdfs:subClassOf rdf:resource="http://data.europa.eu/a4g/ontology#AuxiliaryParty"/>
   </owl:Class>
   <owl:Class rdf:about="http://data.europa.eu/a4g/ontology#NotificationReceiver">
      <rdfs:subClassOf rdf:resource="http://data.europa.eu/a4g/ontology#AuxiliaryParty"/>
   </owl:Class>
   <owl:Class rdf:about="http://data.europa.eu/a4g/ontology#Carrier">
      <rdfs:subClassOf rdf:resource="http://data.europa.eu/a4g/ontology#AuxiliaryParty"/>
   </owl:Class>
   <owl:Class rdf:about="http://data.europa.eu/a4g/ontology#TransportHandlingUnit">
      <rdfs:subClassOf rdf:resource="http://data.europa.eu/a4g/ontology#Package"/>
   </owl:Class>
   <owl:Class rdf:about="http://data.europa.eu/a4g/ontology#DespatchLine">
      <rdfs:subClassOf rdf:resource="http://data.europa.eu/a4g/ontology#Line"/>
   </owl:Class>
   <owl:Class rdf:about="http://data.europa.eu/a4g/ontology#ReceiptAdviceLine">
      <rdfs:subClassOf rdf:resource="http://data.europa.eu/a4g/ontology#Line"/>
   </owl:Class>
   <owl:Class rdf:about="http://data.europa.eu/a4g/ontology#ShipmentInformation">
      <rdfs:subClassOf rdf:resource="http://data.europa.eu/a4g/ontology#InformationHub"/>
   </owl:Class>
   <owl:Class rdf:about="http://data.europa.eu/a4g/ontology#Despatcher">
      <rdfs:subClassOf rdf:resource="http://data.europa.eu/a4g/ontology#OfferingParty"/>
   </owl:Class>
   <owl:Class rdf:about="http://data.europa.eu/a4g/ontology#DespatchAdvice">
      <rdfs:subClassOf rdf:resource="http://data.europa.eu/a4g/ontology#PostAwardDocument"/>
   </owl:Class>
   <owl:Class rdf:about="http://data.europa.eu/a4g/ontology#ReceiptAdvice">
      <rdfs:subClassOf rdf:resource="http://data.europa.eu/a4g/ontology#PostAwardDocument"/>
   </owl:Class>
   <owl:ObjectProperty rdf:about="http://data.europa.eu/a4g/ontology#hasMaximumTemperature"/>
   <rdf:Description rdf:about="http://data.europa.eu/a4g/ontology#hasMaximumTemperature">
      <skos:prefLabel xml:lang="en">Has maximum temperature</skos:prefLabel>
   </rdf:Description>
   <rdf:Description rdf:about="http://data.europa.eu/a4g/ontology#hasMaximumTemperature">
      <skos:definition xml:lang="en">The highest tolerated temperature. WG approval 18/06/2024 (epo-ful:TemperatureSpecification -&gt; epo:Quantity (+epo-ful:hasMaximumTemperature))</skos:definition>
   </rdf:Description>
   <rdf:Description rdf:about="http://data.europa.eu/a4g/ontology#hasMaximumTemperature">
      <rdfs:isDefinedBy rdf:resource="http://data.europa.eu/a4g/ontology#ful"/>
   </rdf:Description>
   <owl:ObjectProperty rdf:about="http://data.europa.eu/a4g/ontology#hasMinimumTemperature"/>
   <rdf:Description rdf:about="http://data.europa.eu/a4g/ontology#hasMinimumTemperature">
      <skos:prefLabel xml:lang="en">Has minimum temperature</skos:prefLabel>
   </rdf:Description>
   <rdf:Description rdf:about="http://data.europa.eu/a4g/ontology#hasMinimumTemperature">
      <skos:definition xml:lang="en">The lowest tolerated temperature. WG approval 18/06/2024 (epo-ful:TemperatureSpecification -&gt; epo:Quantity (+epo-ful:hasMinimumTemperature))</skos:definition>
   </rdf:Description>
   <rdf:Description rdf:about="http://data.europa.eu/a4g/ontology#hasMinimumTemperature">
      <rdfs:isDefinedBy rdf:resource="http://data.europa.eu/a4g/ontology#ful"/>
   </rdf:Description>
   <owl:ObjectProperty rdf:about="http://data.europa.eu/a4g/ontology#hasTemperatureSpecification"/>
   <rdf:Description rdf:about="http://data.europa.eu/a4g/ontology#hasTemperatureSpecification">
      <skos:prefLabel xml:lang="en">Has temperature specification</skos:prefLabel>
   </rdf:Description>
   <rdf:Description rdf:about="http://data.europa.eu/a4g/ontology#hasTemperatureSpecification">
      <skos:definition xml:lang="en">Relation indicating the Temperature Specification for the instance of the concept. WG approval 25/06/2024 (epo-ful:AbstractContainer -&gt; epo-ful:TemperatureSpecification (+epo-ful:hasTemperatureSpecification))</skos:definition>
   </rdf:Description>
   <rdf:Description rdf:about="http://data.europa.eu/a4g/ontology#hasTemperatureSpecification">
      <rdfs:isDefinedBy rdf:resource="http://data.europa.eu/a4g/ontology#ful"/>
   </rdf:Description>
   <owl:ObjectProperty rdf:about="http://data.europa.eu/a4g/ontology#hasGrossWeight"/>
   <rdf:Description rdf:about="http://data.europa.eu/a4g/ontology#hasGrossWeight">
      <skos:prefLabel xml:lang="en">Has gross weight</skos:prefLabel>
   </rdf:Description>
   <rdf:Description rdf:about="http://data.europa.eu/a4g/ontology#hasGrossWeight">
      <skos:definition xml:lang="en">The total mass of goods including the packaging. WG approval 18/06/2024 (epo-ful:AbstractContainer -&gt; epo:Quantity (+epo-ful:hasGrossWeight)) The total mass of goods including the packaging. WG approval 18/06/2024 (epo-ful:Consignment -&gt; epo:Quantity (+epo-ful:hasGrossWeight))</skos:definition>
   </rdf:Description>
   <rdf:Description rdf:about="http://data.europa.eu/a4g/ontology#hasGrossWeight">
      <rdfs:isDefinedBy rdf:resource="http://data.europa.eu/a4g/ontology#ful"/>
   </rdf:Description>
   <owl:ObjectProperty rdf:about="http://data.europa.eu/a4g/ontology#hasNetWeight"/>
   <rdf:Description rdf:about="http://data.europa.eu/a4g/ontology#hasNetWeight">
      <skos:prefLabel xml:lang="en">Has net weight</skos:prefLabel>
   </rdf:Description>
   <rdf:Description rdf:about="http://data.europa.eu/a4g/ontology#hasNetWeight">
      <skos:definition xml:lang="en">The total mass of goods without the packaging. WG approval 18/06/2024 (epo-ful:AbstractContainer -&gt; epo:Quantity (+epo-ful:hasNetWeight)) The total mass of goods without the packaging. WG approval 18/06/2024 (epo-ful:Consignment -&gt; epo:Quantity (+epo-ful:hasNetWeight))</skos:definition>
   </rdf:Description>
   <rdf:Description rdf:about="http://data.europa.eu/a4g/ontology#hasNetWeight">
      <rdfs:isDefinedBy rdf:resource="http://data.europa.eu/a4g/ontology#ful"/>
   </rdf:Description>
   <owl:ObjectProperty rdf:about="http://data.europa.eu/a4g/ontology#hasLength"/>
   <rdf:Description rdf:about="http://data.europa.eu/a4g/ontology#hasLength">
      <skos:prefLabel xml:lang="en">Has length</skos:prefLabel>
   </rdf:Description>
   <rdf:Description rdf:about="http://data.europa.eu/a4g/ontology#hasLength">
      <skos:definition xml:lang="en">The horizontal measurement. Additional Information: The length is the longer side between the length and the width. WG approval 18/06/2024 (epo-ful:AbstractContainer -&gt; epo:Quantity (+epo-ful:hasLength))</skos:definition>
   </rdf:Description>
   <rdf:Description rdf:about="http://data.europa.eu/a4g/ontology#hasLength">
      <rdfs:isDefinedBy rdf:resource="http://data.europa.eu/a4g/ontology#ful"/>
   </rdf:Description>
   <owl:ObjectProperty rdf:about="http://data.europa.eu/a4g/ontology#hasGrossVolume"/>
   <rdf:Description rdf:about="http://data.europa.eu/a4g/ontology#hasGrossVolume">
      <skos:prefLabel xml:lang="en">Has gross volume</skos:prefLabel>
   </rdf:Description>
   <rdf:Description rdf:about="http://data.europa.eu/a4g/ontology#hasGrossVolume">
      <skos:definition xml:lang="en">The amount of space that is required including the packaging. WG approval 18/06/2024 (epo-ful:AbstractContainer -&gt; epo:Quantity (+epo-ful:hasGrossVolume)) The amount of space that is required including the packaging. WG approval 18/06/2024 (epo-ful:Consignment -&gt; epo:Quantity (+epo-ful:hasGrossVolume))</skos:definition>
   </rdf:Description>
   <rdf:Description rdf:about="http://data.europa.eu/a4g/ontology#hasGrossVolume">
      <rdfs:isDefinedBy rdf:resource="http://data.europa.eu/a4g/ontology#ful"/>
   </rdf:Description>
   <owl:ObjectProperty rdf:about="http://data.europa.eu/a4g/ontology#hasWidth"/>
   <rdf:Description rdf:about="http://data.europa.eu/a4g/ontology#hasWidth">
      <skos:prefLabel xml:lang="en">Has width</skos:prefLabel>
   </rdf:Description>
   <rdf:Description rdf:about="http://data.europa.eu/a4g/ontology#hasWidth">
      <skos:definition xml:lang="en">The measurement of the depth. Additional Information: The width is the shorter side between the length and the width. WG approval 18/06/2024 (epo-ful:AbstractContainer -&gt; epo:Quantity (+epo-ful:hasWidth))</skos:definition>
   </rdf:Description>
   <rdf:Description rdf:about="http://data.europa.eu/a4g/ontology#hasWidth">
      <rdfs:isDefinedBy rdf:resource="http://data.europa.eu/a4g/ontology#ful"/>
   </rdf:Description>
   <owl:ObjectProperty rdf:about="http://data.europa.eu/a4g/ontology#hasHeight"/>
   <rdf:Description rdf:about="http://data.europa.eu/a4g/ontology#hasHeight">
      <skos:prefLabel xml:lang="en">Has height</skos:prefLabel>
   </rdf:Description>
   <rdf:Description rdf:about="http://data.europa.eu/a4g/ontology#hasHeight">
      <skos:definition xml:lang="en">The vertical measurement. WG approval 18/06/2024 (epo-ful:AbstractContainer -&gt; epo:Quantity (+epo-ful:hasHeight))</skos:definition>
   </rdf:Description>
   <rdf:Description rdf:about="http://data.europa.eu/a4g/ontology#hasHeight">
      <rdfs:isDefinedBy rdf:resource="http://data.europa.eu/a4g/ontology#ful"/>
   </rdf:Description>
   <owl:ObjectProperty rdf:about="http://data.europa.eu/a4g/ontology#hasTotalGoodsItemQuantity"/>
   <rdf:Description rdf:about="http://data.europa.eu/a4g/ontology#hasTotalGoodsItemQuantity">
      <skos:prefLabel xml:lang="en">Has total goods item quantity</skos:prefLabel>
   </rdf:Description>
   <rdf:Description rdf:about="http://data.europa.eu/a4g/ontology#hasTotalGoodsItemQuantity">
      <skos:definition xml:lang="en">Relation indicating the number of the Goods Items. WG approval 25/06/2024 (epo-ful:AbstractContainer -&gt; epo:Quantity (+epo-ful:hasTotalGoodsItemQuantity)) Relation indicating the number of the Goods Items. WG approval 25/06/2024 (epo-ful:Consignment -&gt; epo:Quantity (+epo-ful:hasTotalGoodsItemQuantity))</skos:definition>
   </rdf:Description>
   <rdf:Description rdf:about="http://data.europa.eu/a4g/ontology#hasTotalGoodsItemQuantity">
      <rdfs:isDefinedBy rdf:resource="http://data.europa.eu/a4g/ontology#ful"/>
   </rdf:Description>
   <owl:ObjectProperty rdf:about="http://www.w3.org/ns/adms#identifier"/>
   <rdf:Description rdf:about="http://www.w3.org/ns/adms#identifier">
      <skos:prefLabel xml:lang="en">Identifier</skos:prefLabel>
   </rdf:Description>
   <rdf:Description rdf:about="http://www.w3.org/ns/adms#identifier">
      <skos:definition xml:lang="en">Links a resource to an adms:Identifier class. (epo-ful:AbstractContainer -&gt; adms:Identifier (+adms:identifier)) Links a resource to an adms:Identifier class. (epo-ful:Consignment -&gt; adms:Identifier (+adms:identifier)) Links a resource to an adms:Identifier class. (epo-ful:ShipmentInformation -&gt; adms:Identifier (+adms:identifier))</skos:definition>
   </rdf:Description>
   <owl:ObjectProperty rdf:about="http://data.europa.eu/a4g/ontology#hasNetVolume"/>
   <rdf:Description rdf:about="http://data.europa.eu/a4g/ontology#hasNetVolume">
      <skos:prefLabel xml:lang="en">Has net volume</skos:prefLabel>
   </rdf:Description>
   <rdf:Description rdf:about="http://data.europa.eu/a4g/ontology#hasNetVolume">
      <skos:definition xml:lang="en">The amount of space that is required without the packaging. WG approval 18/06/2024 (epo-ful:AbstractContainer -&gt; epo:Quantity (+epo-ful:hasNetVolume))</skos:definition>
   </rdf:Description>
   <rdf:Description rdf:about="http://data.europa.eu/a4g/ontology#hasNetVolume">
      <rdfs:isDefinedBy rdf:resource="http://data.europa.eu/a4g/ontology#ful"/>
   </rdf:Description>
   <owl:ObjectProperty rdf:about="http://data.europa.eu/a4g/ontology#playedBy"/>
   <rdf:Description rdf:about="http://data.europa.eu/a4g/ontology#playedBy">
      <skos:prefLabel xml:lang="en">Played by</skos:prefLabel>
   </rdf:Description>
   <rdf:Description rdf:about="http://data.europa.eu/a4g/ontology#playedBy">
      <rdfs:isDefinedBy rdf:resource="http://data.europa.eu/a4g/ontology#ful"/>
   </rdf:Description>
   <owl:ObjectProperty rdf:about="http://data.europa.eu/a4g/ontology#hasDriverPerson"/>
   <rdf:Description rdf:about="http://data.europa.eu/a4g/ontology#hasDriverPerson">
      <skos:prefLabel xml:lang="en">Has driver person</skos:prefLabel>
   </rdf:Description>
   <rdf:Description rdf:about="http://data.europa.eu/a4g/ontology#hasDriverPerson">
      <skos:definition xml:lang="en">Relation indicating the operator of the Transport Means. WG approval 02/07/2024 (epo-ful:TransportMeans -&gt; epo-ful:TransportMeansOperator (+epo:hasDriverPerson))</skos:definition>
   </rdf:Description>
   <rdf:Description rdf:about="http://data.europa.eu/a4g/ontology#hasDriverPerson">
      <rdfs:isDefinedBy rdf:resource="http://data.europa.eu/a4g/ontology#ful"/>
   </rdf:Description>
   <owl:ObjectProperty rdf:about="http://data.europa.eu/a4g/ontology#hasTraceID"/>
   <rdf:Description rdf:about="http://data.europa.eu/a4g/ontology#hasTraceID">
      <skos:prefLabel xml:lang="en">Has trace i d</skos:prefLabel>
   </rdf:Description>
   <rdf:Description rdf:about="http://data.europa.eu/a4g/ontology#hasTraceID">
      <skos:definition xml:lang="en">The identifier used for tracking the Goods Item. Additional information: An example is the EPC number used in RFID. WG approval 21/09/2023 (epo-ful:GoodsItem -&gt; adms:Identifier (+epo-ful:hasTraceID))</skos:definition>
   </rdf:Description>
   <rdf:Description rdf:about="http://data.europa.eu/a4g/ontology#hasTraceID">
      <rdfs:isDefinedBy rdf:resource="http://data.europa.eu/a4g/ontology#ful"/>
   </rdf:Description>
   <owl:ObjectProperty rdf:about="http://data.europa.eu/a4g/ontology#hasDeclaredStatisticalValue"/>
   <rdf:Description rdf:about="http://data.europa.eu/a4g/ontology#hasDeclaredStatisticalValue">
      <skos:prefLabel xml:lang="en">Has declared statistical value</skos:prefLabel>
   </rdf:Description>
   <rdf:Description rdf:about="http://data.europa.eu/a4g/ontology#hasDeclaredStatisticalValue">
      <skos:definition xml:lang="en">The Monetary Value declared for statistical purposes. WG approval 10/06/2024 (epo-ful:Consignment -&gt; epo:MonetaryValue (+epo-ful:hasDeclaredStatisticalValue))</skos:definition>
   </rdf:Description>
   <rdf:Description rdf:about="http://data.europa.eu/a4g/ontology#hasDeclaredStatisticalValue">
      <rdfs:isDefinedBy rdf:resource="http://data.europa.eu/a4g/ontology#ful"/>
   </rdf:Description>
   <owl:ObjectProperty rdf:about="http://data.europa.eu/a4g/ontology#refersToDespatchLine"/>
   <rdf:Description rdf:about="http://data.europa.eu/a4g/ontology#refersToDespatchLine">
      <skos:prefLabel xml:lang="en">Refers to despatch line</skos:prefLabel>
   </rdf:Description>
   <rdf:Description rdf:about="http://data.europa.eu/a4g/ontology#refersToDespatchLine">
      <skos:definition xml:lang="en">Reference to a Despatch Line. WG approval 25/06/2024 (epo-ful:GoodsItem -&gt; epo-ful:DespatchLine (+epo-ful:refersToDespatchLine))</skos:definition>
   </rdf:Description>
   <rdf:Description rdf:about="http://data.europa.eu/a4g/ontology#refersToDespatchLine">
      <rdfs:isDefinedBy rdf:resource="http://data.europa.eu/a4g/ontology#ful"/>
   </rdf:Description>
   <owl:ObjectProperty rdf:about="http://data.europa.eu/a4g/ontology#containsGoodsItem"/>
   <rdf:Description rdf:about="http://data.europa.eu/a4g/ontology#containsGoodsItem">
      <skos:prefLabel xml:lang="en">Contains goods item</skos:prefLabel>
   </rdf:Description>
   <rdf:Description rdf:about="http://data.europa.eu/a4g/ontology#containsGoodsItem">
      <skos:definition xml:lang="en">Includes Goods Item. WG approval 10/06/2024 (epo-ful:Package -&gt; epo-ful:GoodsItem (+epo-ful:containsGoodsItem))</skos:definition>
   </rdf:Description>
   <rdf:Description rdf:about="http://data.europa.eu/a4g/ontology#containsGoodsItem">
      <rdfs:isDefinedBy rdf:resource="http://data.europa.eu/a4g/ontology#ful"/>
   </rdf:Description>
   <owl:ObjectProperty rdf:about="http://data.europa.eu/a4g/ontology#agreedBySeller"/>
   <rdf:Description rdf:about="http://data.europa.eu/a4g/ontology#agreedBySeller">
      <skos:prefLabel xml:lang="en">Agreed by seller</skos:prefLabel>
   </rdf:Description>
   <rdf:Description rdf:about="http://data.europa.eu/a4g/ontology#agreedBySeller">
      <skos:definition xml:lang="en">Accepted by Seller. WG approval 10/06/2024 (epo-ful:ShipmentAgreement -&gt; epo-ord:Seller (+epo-ful:agreedBySeller))</skos:definition>
   </rdf:Description>
   <rdf:Description rdf:about="http://data.europa.eu/a4g/ontology#agreedBySeller">
      <rdfs:isDefinedBy rdf:resource="http://data.europa.eu/a4g/ontology#ful"/>
   </rdf:Description>
   <owl:ObjectProperty rdf:about="http://data.europa.eu/a4g/ontology#agreedByBuyer"/>
   <rdf:Description rdf:about="http://data.europa.eu/a4g/ontology#agreedByBuyer">
      <skos:prefLabel xml:lang="en">Agreed by buyer</skos:prefLabel>
   </rdf:Description>
   <rdf:Description rdf:about="http://data.europa.eu/a4g/ontology#agreedByBuyer">
      <skos:definition xml:lang="en">Accepted by Buyer. WG approval 10/06/2024 (epo-ful:ShipmentAgreement -&gt; epo:Buyer (+epo-ful:agreedByBuyer))</skos:definition>
   </rdf:Description>
   <rdf:Description rdf:about="http://data.europa.eu/a4g/ontology#agreedByBuyer">
      <rdfs:isDefinedBy rdf:resource="http://data.europa.eu/a4g/ontology#ful"/>
   </rdf:Description>
   <owl:ObjectProperty rdf:about="http://data.europa.eu/a4g/ontology#refersToShipmentAgreement"/>
   <rdf:Description rdf:about="http://data.europa.eu/a4g/ontology#refersToShipmentAgreement">
      <skos:prefLabel xml:lang="en">Refers to shipment agreement</skos:prefLabel>
   </rdf:Description>
   <rdf:Description rdf:about="http://data.europa.eu/a4g/ontology#refersToShipmentAgreement">
      <skos:definition xml:lang="en">Reference to a Shipment Agreement. WG approval 25/06/2024 (epo-ful:DespatchAdvice -&gt; epo-ful:ShipmentAgreement (+epo-ful:refersToShipmentAgreement))</skos:definition>
   </rdf:Description>
   <rdf:Description rdf:about="http://data.europa.eu/a4g/ontology#refersToShipmentAgreement">
      <rdfs:isDefinedBy rdf:resource="http://data.europa.eu/a4g/ontology#ful"/>
   </rdf:Description>
   <owl:ObjectProperty rdf:about="http://data.europa.eu/a4g/ontology#hasTransportEquipmentSeal"/>
   <rdf:Description rdf:about="http://data.europa.eu/a4g/ontology#hasTransportEquipmentSeal">
      <skos:prefLabel xml:lang="en">Has transport equipment seal</skos:prefLabel>
   </rdf:Description>
   <rdf:Description rdf:about="http://data.europa.eu/a4g/ontology#hasTransportEquipmentSeal">
      <skos:definition xml:lang="en">Relation indicating that the instance of the concept has a Transport Equipment Seal. WG approval 25/06/2024 (epo-ful:TransportEquipment -&gt; epo-ful:TransportEquipmentSeal (+epo-ful:hasTransportEquipmentSeal))</skos:definition>
   </rdf:Description>
   <rdf:Description rdf:about="http://data.europa.eu/a4g/ontology#hasTransportEquipmentSeal">
      <rdfs:isDefinedBy rdf:resource="http://data.europa.eu/a4g/ontology#ful"/>
   </rdf:Description>
   <owl:ObjectProperty rdf:about="http://data.europa.eu/a4g/ontology#hasTransportMeansType"/>
   <rdf:Description rdf:about="http://data.europa.eu/a4g/ontology#hasTransportMeansType">
      <skos:prefLabel xml:lang="en">Has transport means type</skos:prefLabel>
   </rdf:Description>
   <rdf:Description rdf:about="http://data.europa.eu/a4g/ontology#hasTransportMeansType">
      <skos:definition xml:lang="en">The kind of Transport Means. WG approval 25/06/2024 (epo-ful:TransportMeans -&gt; at-voc-new:transport-means-type (+epo-ful:hasTransportMeansType))</skos:definition>
   </rdf:Description>
   <rdf:Description rdf:about="http://data.europa.eu/a4g/ontology#hasTransportMeansType">
      <rdfs:isDefinedBy rdf:resource="http://data.europa.eu/a4g/ontology#ful"/>
   </rdf:Description>
   <owl:ObjectProperty rdf:about="http://data.europa.eu/a4g/ontology#hasTransportMode"/>
   <rdf:Description rdf:about="http://data.europa.eu/a4g/ontology#hasTransportMode">
      <skos:prefLabel xml:lang="en">Has transport mode</skos:prefLabel>
   </rdf:Description>
   <rdf:Description rdf:about="http://data.europa.eu/a4g/ontology#hasTransportMode">
      <skos:definition xml:lang="en">The type of the transport used. WG approval 25/06/2024 (epo-ful:TransportMeans -&gt; at-voc-new:transport-mode (+epo-ful:hasTransportMode))</skos:definition>
   </rdf:Description>
   <rdf:Description rdf:about="http://data.europa.eu/a4g/ontology#hasTransportMode">
      <rdfs:isDefinedBy rdf:resource="http://data.europa.eu/a4g/ontology#ful"/>
   </rdf:Description>
   <owl:ObjectProperty rdf:about="http://data.europa.eu/a4g/ontology#hasVehicleSegmentID"/>
   <rdf:Description rdf:about="http://data.europa.eu/a4g/ontology#hasVehicleSegmentID">
      <skos:prefLabel xml:lang="en">Has vehicle segment i d</skos:prefLabel>
   </rdf:Description>
   <rdf:Description rdf:about="http://data.europa.eu/a4g/ontology#hasVehicleSegmentID">
      <skos:definition xml:lang="en">The identifier of a part of the Transport Means. WG approval 25/06/2024 (epo-ful:TransportMeans -&gt; adms:Identifier (+epo-ful:hasVehicleSegmentID))</skos:definition>
   </rdf:Description>
   <rdf:Description rdf:about="http://data.europa.eu/a4g/ontology#hasVehicleSegmentID">
      <rdfs:isDefinedBy rdf:resource="http://data.europa.eu/a4g/ontology#ful"/>
   </rdf:Description>
   <owl:ObjectProperty rdf:about="http://data.europa.eu/a4g/ontology#hasVehicleID"/>
   <rdf:Description rdf:about="http://data.europa.eu/a4g/ontology#hasVehicleID">
      <skos:prefLabel xml:lang="en">Has vehicle i d</skos:prefLabel>
   </rdf:Description>
   <rdf:Description rdf:about="http://data.europa.eu/a4g/ontology#hasVehicleID">
      <skos:definition xml:lang="en">The identifier of the Transport Means. WG approval 25/06/2024 (epo-ful:TransportMeans -&gt; adms:Identifier (+epo-ful:hasVehicleID))</skos:definition>
   </rdf:Description>
   <rdf:Description rdf:about="http://data.europa.eu/a4g/ontology#hasVehicleID">
      <rdfs:isDefinedBy rdf:resource="http://data.europa.eu/a4g/ontology#ful"/>
   </rdf:Description>
   <owl:ObjectProperty rdf:about="http://data.europa.eu/a4g/ontology#usesTransportMeans"/>
   <rdf:Description rdf:about="http://data.europa.eu/a4g/ontology#usesTransportMeans">
      <skos:prefLabel xml:lang="en">Uses transport means</skos:prefLabel>
   </rdf:Description>
   <rdf:Description rdf:about="http://data.europa.eu/a4g/ontology#usesTransportMeans">
      <skos:definition xml:lang="en">Relation indicating that a Shipment Stage utilises a Transport Means. WG approval 02/07/2024 (epo-ful:ShipmentStage -&gt; epo-ful:TransportMeans (+epo-ful:usesTransportMeans))</skos:definition>
   </rdf:Description>
   <rdf:Description rdf:about="http://data.europa.eu/a4g/ontology#usesTransportMeans">
      <rdfs:isDefinedBy rdf:resource="http://data.europa.eu/a4g/ontology#ful"/>
   </rdf:Description>
   <owl:ObjectProperty rdf:about="http://data.europa.eu/a4g/ontology#hasDepartureShipmentInformation"/>
   <rdf:Description rdf:about="http://data.europa.eu/a4g/ontology#hasDepartureShipmentInformation">
      <skos:prefLabel xml:lang="en">Has departure shipment information</skos:prefLabel>
   </rdf:Description>
   <rdf:Description rdf:about="http://data.europa.eu/a4g/ontology#hasDepartureShipmentInformation">
      <skos:definition xml:lang="en">Shipment Information about the place the Consignment is leaving from in a given Shipment Stage. WG approval 18/06/2024 (epo-ful:ShipmentStage -&gt; epo-ful:ShipmentInformation (+epo-ful:hasDepartureShipmentInformation))</skos:definition>
   </rdf:Description>
   <rdf:Description rdf:about="http://data.europa.eu/a4g/ontology#hasDepartureShipmentInformation">
      <rdfs:isDefinedBy rdf:resource="http://data.europa.eu/a4g/ontology#ful"/>
   </rdf:Description>
   <owl:ObjectProperty rdf:about="http://data.europa.eu/a4g/ontology#hasArrivalShipmentInformation"/>
   <rdf:Description rdf:about="http://data.europa.eu/a4g/ontology#hasArrivalShipmentInformation">
      <skos:prefLabel xml:lang="en">Has arrival shipment information</skos:prefLabel>
   </rdf:Description>
   <rdf:Description rdf:about="http://data.europa.eu/a4g/ontology#hasArrivalShipmentInformation">
      <skos:definition xml:lang="en">Shipment Information about the destination of the Consignment for a given Shipment Stage. WG approval 18/06/2024 (epo-ful:ShipmentStage -&gt; epo-ful:ShipmentInformation (+epo:hasArrivalShipmentInformation))</skos:definition>
   </rdf:Description>
   <rdf:Description rdf:about="http://data.europa.eu/a4g/ontology#hasArrivalShipmentInformation">
      <rdfs:isDefinedBy rdf:resource="http://data.europa.eu/a4g/ontology#ful"/>
   </rdf:Description>
   <owl:ObjectProperty rdf:about="http://data.europa.eu/a4g/ontology#specifiesCarrier"/>
   <rdf:Description rdf:about="http://data.europa.eu/a4g/ontology#specifiesCarrier">
      <skos:prefLabel xml:lang="en">Specifies carrier</skos:prefLabel>
   </rdf:Description>
   <rdf:Description rdf:about="http://data.europa.eu/a4g/ontology#specifiesCarrier">
      <skos:definition xml:lang="en">Relation indicating that the instance of the concept involves the Carrier. WG approval 25/06/2024 (epo-ful:ShipmentStage -&gt; epo-ful:Carrier (+epo:specifiesCarrier))</skos:definition>
   </rdf:Description>
   <rdf:Description rdf:about="http://data.europa.eu/a4g/ontology#specifiesCarrier">
      <rdfs:isDefinedBy rdf:resource="http://data.europa.eu/a4g/ontology#ful"/>
   </rdf:Description>
   <owl:ObjectProperty rdf:about="http://data.europa.eu/a4g/ontology#hasPreCarriageShipmentStage"/>
   <rdf:Description rdf:about="http://data.europa.eu/a4g/ontology#hasPreCarriageShipmentStage">
      <skos:prefLabel xml:lang="en">Has pre carriage shipment stage</skos:prefLabel>
   </rdf:Description>
   <rdf:Description rdf:about="http://data.europa.eu/a4g/ontology#hasPreCarriageShipmentStage">
      <skos:definition xml:lang="en">Any Shipment Stage between the Despatcher and the departure point of the main carriage in a transport chain. WG approval 18/06/2024 (epo-ful:Consignment -&gt; epo-ful:ShipmentStage (+epo-ful:hasPreCarriageShipmentStage))</skos:definition>
   </rdf:Description>
   <rdf:Description rdf:about="http://data.europa.eu/a4g/ontology#hasPreCarriageShipmentStage">
      <rdfs:isDefinedBy rdf:resource="http://data.europa.eu/a4g/ontology#ful"/>
   </rdf:Description>
   <owl:ObjectProperty rdf:about="http://data.europa.eu/a4g/ontology#hasOnCarriageShipmentStage"/>
   <rdf:Description rdf:about="http://data.europa.eu/a4g/ontology#hasOnCarriageShipmentStage">
      <skos:prefLabel xml:lang="en">Has on carriage shipment stage</skos:prefLabel>
   </rdf:Description>
   <rdf:Description rdf:about="http://data.europa.eu/a4g/ontology#hasOnCarriageShipmentStage">
      <skos:definition xml:lang="en">Any Shipment Stage between the main carriage arrival point and the ultimate receiver in a transport chain. WG approval 18/06/2024 (epo-ful:Consignment -&gt; epo-ful:ShipmentStage (+epo-ful:hasOnCarriageShipmentStage))</skos:definition>
   </rdf:Description>
   <rdf:Description rdf:about="http://data.europa.eu/a4g/ontology#hasOnCarriageShipmentStage">
      <rdfs:isDefinedBy rdf:resource="http://data.europa.eu/a4g/ontology#ful"/>
   </rdf:Description>
   <owl:ObjectProperty rdf:about="http://data.europa.eu/a4g/ontology#hasMainCarriageShipmentStage"/>
   <rdf:Description rdf:about="http://data.europa.eu/a4g/ontology#hasMainCarriageShipmentStage">
      <skos:prefLabel xml:lang="en">Has main carriage shipment stage</skos:prefLabel>
   </rdf:Description>
   <rdf:Description rdf:about="http://data.europa.eu/a4g/ontology#hasMainCarriageShipmentStage">
      <skos:definition xml:lang="en">The Shipment Stage for the longest distance covered in a transport chain. WG approval 18/06/2024 (epo-ful:Consignment -&gt; epo-ful:ShipmentStage (+epo-ful:hasMainCarriageShipmentStage))</skos:definition>
   </rdf:Description>
   <rdf:Description rdf:about="http://data.europa.eu/a4g/ontology#hasMainCarriageShipmentStage">
      <rdfs:isDefinedBy rdf:resource="http://data.europa.eu/a4g/ontology#ful"/>
   </rdf:Description>
   <owl:ObjectProperty rdf:about="http://data.europa.eu/a4g/ontology#hasPackagingType"/>
   <rdf:Description rdf:about="http://data.europa.eu/a4g/ontology#hasPackagingType">
      <skos:prefLabel xml:lang="en">Has packaging type</skos:prefLabel>
   </rdf:Description>
   <rdf:Description rdf:about="http://data.europa.eu/a4g/ontology#hasPackagingType">
      <skos:definition xml:lang="en">The kind of Package. WG approval 25/06/2024 (epo-ful:Package -&gt; at-voc-new:packaging-type (+epo-ful:hasPackagingType))</skos:definition>
   </rdf:Description>
   <rdf:Description rdf:about="http://data.europa.eu/a4g/ontology#hasPackagingType">
      <rdfs:isDefinedBy rdf:resource="http://data.europa.eu/a4g/ontology#ful"/>
   </rdf:Description>
   <owl:ObjectProperty rdf:about="http://data.europa.eu/a4g/ontology#containsPackage"/>
   <rdf:Description rdf:about="http://data.europa.eu/a4g/ontology#containsPackage">
      <skos:prefLabel xml:lang="en">Contains package</skos:prefLabel>
   </rdf:Description>
   <rdf:Description rdf:about="http://data.europa.eu/a4g/ontology#containsPackage">
      <skos:definition xml:lang="en">Includes Package. WG approval 10/06/2024 (epo-ful:Package -&gt; epo-ful:Package (+epo-ful:containsPackage))</skos:definition>
   </rdf:Description>
   <rdf:Description rdf:about="http://data.europa.eu/a4g/ontology#containsPackage">
      <rdfs:isDefinedBy rdf:resource="http://data.europa.eu/a4g/ontology#ful"/>
   </rdf:Description>
   <owl:ObjectProperty rdf:about="http://data.europa.eu/a4g/ontology#foreseesPackage"/>
   <rdf:Description rdf:about="http://data.europa.eu/a4g/ontology#foreseesPackage">
      <skos:prefLabel xml:lang="en">Foresees package</skos:prefLabel>
   </rdf:Description>
   <rdf:Description rdf:about="http://data.europa.eu/a4g/ontology#foreseesPackage">
      <rdfs:isDefinedBy rdf:resource="http://data.europa.eu/a4g/ontology#ful"/>
   </rdf:Description>
   <owl:ObjectProperty rdf:about="http://data.europa.eu/a4g/ontology#hasTransportEquipmentType"/>
   <rdf:Description rdf:about="http://data.europa.eu/a4g/ontology#hasTransportEquipmentType">
      <skos:prefLabel xml:lang="en">Has transport equipment type</skos:prefLabel>
   </rdf:Description>
   <rdf:Description rdf:about="http://data.europa.eu/a4g/ontology#hasTransportEquipmentType">
      <skos:definition xml:lang="en">The kind of Transport Equipment. WG approval 25/06/2024 (epo-ful:TransportEquipment -&gt; at-voc-new:transport-equipment-type (+epo-ful:hasTransportEquipmentType))</skos:definition>
   </rdf:Description>
   <rdf:Description rdf:about="http://data.europa.eu/a4g/ontology#hasTransportEquipmentType">
      <rdfs:isDefinedBy rdf:resource="http://data.europa.eu/a4g/ontology#ful"/>
   </rdf:Description>
   <owl:ObjectProperty rdf:about="http://data.europa.eu/a4g/ontology#hasSizeType"/>
   <rdf:Description rdf:about="http://data.europa.eu/a4g/ontology#hasSizeType">
      <skos:prefLabel xml:lang="en">Has size type</skos:prefLabel>
   </rdf:Description>
   <rdf:Description rdf:about="http://data.europa.eu/a4g/ontology#hasSizeType">
      <skos:definition xml:lang="en">An extension classification specifying the measurement of the Transport Equipment. Additional Information: This codelist should be used only in the case of a container. WG approval 25/06/2024 (epo-ful:TransportEquipment -&gt; at-voc-new:size-type (+epo-ful:hasSizeType))</skos:definition>
   </rdf:Description>
   <rdf:Description rdf:about="http://data.europa.eu/a4g/ontology#hasSizeType">
      <rdfs:isDefinedBy rdf:resource="http://data.europa.eu/a4g/ontology#ful"/>
   </rdf:Description>
   <owl:ObjectProperty rdf:about="http://data.europa.eu/a4g/ontology#usesTransportEquipment"/>
   <rdf:Description rdf:about="http://data.europa.eu/a4g/ontology#usesTransportEquipment">
      <skos:prefLabel xml:lang="en">Uses transport equipment</skos:prefLabel>
   </rdf:Description>
   <rdf:Description rdf:about="http://data.europa.eu/a4g/ontology#usesTransportEquipment">
      <skos:definition xml:lang="en">Relation indicating that a Transport Handling Unit utilises a Transport Equipment. WG approval 02/07/2024 (epo-ful:TransportHandlingUnit -&gt; epo-ful:TransportEquipment (+epo-ful:usesTransportEquipment))</skos:definition>
   </rdf:Description>
   <rdf:Description rdf:about="http://data.europa.eu/a4g/ontology#usesTransportEquipment">
      <rdfs:isDefinedBy rdf:resource="http://data.europa.eu/a4g/ontology#ful"/>
   </rdf:Description>
   <owl:ObjectProperty rdf:about="http://data.europa.eu/a4g/ontology#specifiesNotifier"/>
   <rdf:Description rdf:about="http://data.europa.eu/a4g/ontology#specifiesNotifier">
      <skos:prefLabel xml:lang="en">Specifies notifier</skos:prefLabel>
   </rdf:Description>
   <rdf:Description rdf:about="http://data.europa.eu/a4g/ontology#specifiesNotifier">
      <rdfs:isDefinedBy rdf:resource="http://data.europa.eu/a4g/ontology#ful"/>
   </rdf:Description>
   <owl:ObjectProperty rdf:about="http://data.europa.eu/a4g/ontology#specifiesFreightForwarder"/>
   <rdf:Description rdf:about="http://data.europa.eu/a4g/ontology#specifiesFreightForwarder">
      <skos:prefLabel xml:lang="en">Specifies freight forwarder</skos:prefLabel>
   </rdf:Description>
   <rdf:Description rdf:about="http://data.europa.eu/a4g/ontology#specifiesFreightForwarder">
      <skos:definition xml:lang="en">Relation indicating that the instance of the concept involves the Freight Forwarder. WG approval 25/06/2024 (epo-ful:Consignment -&gt; epo-ful:FreightForwarder (+epo:specifiesFreightForwarder))</skos:definition>
   </rdf:Description>
   <rdf:Description rdf:about="http://data.europa.eu/a4g/ontology#specifiesFreightForwarder">
      <rdfs:isDefinedBy rdf:resource="http://data.europa.eu/a4g/ontology#ful"/>
   </rdf:Description>
   <owl:ObjectProperty rdf:about="http://data.europa.eu/a4g/ontology#hasFreightAllowanceCharge"/>
   <rdf:Description rdf:about="http://data.europa.eu/a4g/ontology#hasFreightAllowanceCharge">
      <skos:prefLabel xml:lang="en">Has freight allowance charge</skos:prefLabel>
   </rdf:Description>
   <rdf:Description rdf:about="http://data.europa.eu/a4g/ontology#hasFreightAllowanceCharge">
      <rdfs:isDefinedBy rdf:resource="http://data.europa.eu/a4g/ontology#ful"/>
   </rdf:Description>
   <owl:ObjectProperty rdf:about="http://data.europa.eu/a4g/ontology#hasConsignmentInvoiceValue"/>
   <rdf:Description rdf:about="http://data.europa.eu/a4g/ontology#hasConsignmentInvoiceValue">
      <skos:prefLabel xml:lang="en">Has consignment invoice value</skos:prefLabel>
   </rdf:Description>
   <rdf:Description rdf:about="http://data.europa.eu/a4g/ontology#hasConsignmentInvoiceValue">
      <skos:definition xml:lang="en">Declared amount of the Consignment. Additional Information: This is a logistics information needed for logistics, security measures, customs check, etc. WG approval 18/06/2024 (epo-ful:Consignment -&gt; epo:MonetaryValue (+epo-ful:hasConsignmentInvoiceValue))</skos:definition>
   </rdf:Description>
   <rdf:Description rdf:about="http://data.europa.eu/a4g/ontology#hasConsignmentInvoiceValue">
      <rdfs:isDefinedBy rdf:resource="http://data.europa.eu/a4g/ontology#ful"/>
   </rdf:Description>
   <owl:ObjectProperty rdf:about="http://data.europa.eu/a4g/ontology#hasDespatcherConsignmentID"/>
   <rdf:Description rdf:about="http://data.europa.eu/a4g/ontology#hasDespatcherConsignmentID">
      <skos:prefLabel xml:lang="en">Has despatcher consignment i d</skos:prefLabel>
   </rdf:Description>
   <rdf:Description rdf:about="http://data.europa.eu/a4g/ontology#hasDespatcherConsignmentID">
      <skos:definition xml:lang="en">The identifier of the the Consignment given by the Despatcher. WG approval 10/06/2024 (epo-ful:Consignment -&gt; adms:Identifier (+epo-ful:hasDespatcherConsignmentID))</skos:definition>
   </rdf:Description>
   <rdf:Description rdf:about="http://data.europa.eu/a4g/ontology#hasDespatcherConsignmentID">
      <rdfs:isDefinedBy rdf:resource="http://data.europa.eu/a4g/ontology#ful"/>
   </rdf:Description>
   <owl:ObjectProperty rdf:about="http://data.europa.eu/a4g/ontology#hasChargeableWeight"/>
   <rdf:Description rdf:about="http://data.europa.eu/a4g/ontology#hasChargeableWeight">
      <skos:prefLabel xml:lang="en">Has chargeable weight</skos:prefLabel>
   </rdf:Description>
   <rdf:Description rdf:about="http://data.europa.eu/a4g/ontology#hasChargeableWeight">
      <skos:definition xml:lang="en">The (epo-ful:Consignment -&gt; epo:Quantity (+epo-ful:hasChargeableWeight))</skos:definition>
   </rdf:Description>
   <rdf:Description rdf:about="http://data.europa.eu/a4g/ontology#hasChargeableWeight">
      <rdfs:isDefinedBy rdf:resource="http://data.europa.eu/a4g/ontology#ful"/>
   </rdf:Description>
   <owl:ObjectProperty rdf:about="http://data.europa.eu/a4g/ontology#hasConsignmentFreeOnBoardValue"/>
   <rdf:Description rdf:about="http://data.europa.eu/a4g/ontology#hasConsignmentFreeOnBoardValue">
      <skos:prefLabel xml:lang="en">Has consignment free on board value</skos:prefLabel>
   </rdf:Description>
   <rdf:Description rdf:about="http://data.europa.eu/a4g/ontology#hasConsignmentFreeOnBoardValue">
      <skos:definition xml:lang="en">The Monetary Value of the Consignment when there is a transfer of liability for goods, damaged or destroyed, during shipping. at the exporter's customs frontier. (epo-ful:Consignment -&gt; epo:MonetaryValue (+epo-ful:hasConsignmentFreeOnBoardValue))</skos:definition>
   </rdf:Description>
   <rdf:Description rdf:about="http://data.europa.eu/a4g/ontology#hasConsignmentFreeOnBoardValue">
      <rdfs:isDefinedBy rdf:resource="http://data.europa.eu/a4g/ontology#ful"/>
   </rdf:Description>
   <owl:ObjectProperty rdf:about="http://data.europa.eu/a4g/ontology#hasConsignmentDeclaredStatisticsValue"/>
   <rdf:Description rdf:about="http://data.europa.eu/a4g/ontology#hasConsignmentDeclaredStatisticsValue">
      <skos:prefLabel xml:lang="en">Has consignment declared statistics value</skos:prefLabel>
   </rdf:Description>
   <rdf:Description rdf:about="http://data.europa.eu/a4g/ontology#hasConsignmentDeclaredStatisticsValue">
      <rdfs:isDefinedBy rdf:resource="http://data.europa.eu/a4g/ontology#ful"/>
   </rdf:Description>
   <owl:ObjectProperty rdf:about="http://data.europa.eu/a4g/ontology#hasTransportHandlingUnitQuantity"/>
   <rdf:Description rdf:about="http://data.europa.eu/a4g/ontology#hasTransportHandlingUnitQuantity">
      <skos:prefLabel xml:lang="en">Has transport handling unit quantity</skos:prefLabel>
   </rdf:Description>
   <rdf:Description rdf:about="http://data.europa.eu/a4g/ontology#hasTransportHandlingUnitQuantity">
      <skos:definition xml:lang="en">Relation indicating the number of the Transport Handling Unit. WG approval 25/06/2024 (epo-ful:Consignment -&gt; epo:Quantity (+epo-ful:hasTransportHandlingUnitQuantity))</skos:definition>
   </rdf:Description>
   <rdf:Description rdf:about="http://data.europa.eu/a4g/ontology#hasTransportHandlingUnitQuantity">
      <rdfs:isDefinedBy rdf:resource="http://data.europa.eu/a4g/ontology#ful"/>
   </rdf:Description>
   <owl:ObjectProperty rdf:about="http://data.europa.eu/a4g/ontology#hasFreightCharge"/>
   <rdf:Description rdf:about="http://data.europa.eu/a4g/ontology#hasFreightCharge">
      <skos:prefLabel xml:lang="en">Has freight charge</skos:prefLabel>
   </rdf:Description>
   <rdf:Description rdf:about="http://data.europa.eu/a4g/ontology#hasFreightCharge">
      <skos:definition xml:lang="en">The total cost for moving the goods. WG approval 18/06/2024 (epo-ful:Consignment -&gt; epo-cat:ChargeInformation (+epo-ful:hasFreightCharge))</skos:definition>
   </rdf:Description>
   <rdf:Description rdf:about="http://data.europa.eu/a4g/ontology#hasFreightCharge">
      <rdfs:isDefinedBy rdf:resource="http://data.europa.eu/a4g/ontology#ful"/>
   </rdf:Description>
   <owl:ObjectProperty rdf:about="http://data.europa.eu/a4g/ontology#hasLoadingMeter"/>
   <rdf:Description rdf:about="http://data.europa.eu/a4g/ontology#hasLoadingMeter">
      <skos:prefLabel xml:lang="en">Has loading meter</skos:prefLabel>
   </rdf:Description>
   <rdf:Description rdf:about="http://data.europa.eu/a4g/ontology#hasLoadingMeter">
      <skos:definition xml:lang="en">The area of the Consignment in meters divided by the width of the truck, which is considered to be 2.4 meters. WG approval 18/06/2024 (epo-ful:Consignment -&gt; epo:Quantity (+epo-ful:hasLoadingMeter))</skos:definition>
   </rdf:Description>
   <rdf:Description rdf:about="http://data.europa.eu/a4g/ontology#hasLoadingMeter">
      <rdfs:isDefinedBy rdf:resource="http://data.europa.eu/a4g/ontology#ful"/>
   </rdf:Description>
   <owl:ObjectProperty rdf:about="http://data.europa.eu/a4g/ontology#hasLoadingLength"/>
   <rdf:Description rdf:about="http://data.europa.eu/a4g/ontology#hasLoadingLength">
      <skos:prefLabel xml:lang="en">Has loading length</skos:prefLabel>
   </rdf:Description>
   <rdf:Description rdf:about="http://data.europa.eu/a4g/ontology#hasLoadingLength">
      <skos:definition xml:lang="en">The length (epo-ful:Consignment -&gt; epo:Quantity (+epo-ful:hasLoadingLength))</skos:definition>
   </rdf:Description>
   <rdf:Description rdf:about="http://data.europa.eu/a4g/ontology#hasLoadingLength">
      <rdfs:isDefinedBy rdf:resource="http://data.europa.eu/a4g/ontology#ful"/>
   </rdf:Description>
   <owl:ObjectProperty rdf:about="http://data.europa.eu/a4g/ontology#hasHandlingInstructionCode"/>
   <rdf:Description rdf:about="http://data.europa.eu/a4g/ontology#hasHandlingInstructionCode">
      <skos:prefLabel xml:lang="en">Has handling instruction code</skos:prefLabel>
   </rdf:Description>
   <rdf:Description rdf:about="http://data.europa.eu/a4g/ontology#hasHandlingInstructionCode">
      <skos:definition xml:lang="en">Instruction on how to handle the Goods Items during transportation, expressed as a code. WG approval 18/06/2024 (epo-ful:Consignment -&gt; at-voc-new:handling-instruction (+epo-ful:hasHandlingInstructionCode)) Instruction on how to handle the Goods Items during transportation, expressed as a code. WG approval 18/06/2024 (epo-ful:TransportHandlingUnit -&gt; at-voc-new:handling-instruction (+epo-ful:hasHandlingInstructionCode))</skos:definition>
   </rdf:Description>
   <rdf:Description rdf:about="http://data.europa.eu/a4g/ontology#hasHandlingInstructionCode">
      <rdfs:isDefinedBy rdf:resource="http://data.europa.eu/a4g/ontology#ful"/>
   </rdf:Description>
   <owl:ObjectProperty rdf:about="http://data.europa.eu/a4g/ontology#hasFreightForwarderConsignmentID"/>
   <rdf:Description rdf:about="http://data.europa.eu/a4g/ontology#hasFreightForwarderConsignmentID">
      <skos:prefLabel xml:lang="en">Has freight forwarder consignment i d</skos:prefLabel>
   </rdf:Description>
   <rdf:Description rdf:about="http://data.europa.eu/a4g/ontology#hasFreightForwarderConsignmentID">
      <skos:definition xml:lang="en">The identifier of the the Consignment given by the Freight Forwarder. WG approval 10/06/2024 (epo-ful:Consignment -&gt; adms:Identifier (+epo-ful:hasFreightForwarderConsignmentID))</skos:definition>
   </rdf:Description>
   <rdf:Description rdf:about="http://data.europa.eu/a4g/ontology#hasFreightForwarderConsignmentID">
      <rdfs:isDefinedBy rdf:resource="http://data.europa.eu/a4g/ontology#ful"/>
   </rdf:Description>
   <owl:ObjectProperty rdf:about="http://data.europa.eu/a4g/ontology#hasCarrierConsignmentID"/>
   <rdf:Description rdf:about="http://data.europa.eu/a4g/ontology#hasCarrierConsignmentID">
      <skos:prefLabel xml:lang="en">Has carrier consignment i d</skos:prefLabel>
   </rdf:Description>
   <rdf:Description rdf:about="http://data.europa.eu/a4g/ontology#hasCarrierConsignmentID">
      <skos:definition xml:lang="en">The identifier of the the Consignment given by the Carrier. WG approval 10/06/2024 (epo-ful:Consignment -&gt; adms:Identifier (+epo-ful:hasCarrierConsignmentID))</skos:definition>
   </rdf:Description>
   <rdf:Description rdf:about="http://data.europa.eu/a4g/ontology#hasCarrierConsignmentID">
      <rdfs:isDefinedBy rdf:resource="http://data.europa.eu/a4g/ontology#ful"/>
   </rdf:Description>
   <owl:ObjectProperty rdf:about="http://data.europa.eu/a4g/ontology#containsTransportHandlingUnit"/>
   <rdf:Description rdf:about="http://data.europa.eu/a4g/ontology#containsTransportHandlingUnit">
      <skos:prefLabel xml:lang="en">Contains transport handling unit</skos:prefLabel>
   </rdf:Description>
   <rdf:Description rdf:about="http://data.europa.eu/a4g/ontology#containsTransportHandlingUnit">
      <skos:definition xml:lang="en">Includes Transport Handling Unit. WG approval 10/06/2024 (epo-ful:Consignment -&gt; epo-ful:TransportHandlingUnit (+epo-ful:containsTransportHandlingUnit))</skos:definition>
   </rdf:Description>
   <rdf:Description rdf:about="http://data.europa.eu/a4g/ontology#containsTransportHandlingUnit">
      <rdfs:isDefinedBy rdf:resource="http://data.europa.eu/a4g/ontology#ful"/>
   </rdf:Description>
   <owl:ObjectProperty rdf:about="http://data.europa.eu/a4g/ontology#specifiesNotificationReceiver"/>
   <rdf:Description rdf:about="http://data.europa.eu/a4g/ontology#specifiesNotificationReceiver">
      <skos:prefLabel xml:lang="en">Specifies notification receiver</skos:prefLabel>
   </rdf:Description>
   <rdf:Description rdf:about="http://data.europa.eu/a4g/ontology#specifiesNotificationReceiver">
      <skos:definition xml:lang="en">c (epo-ful:Consignment -&gt; epo-ful:NotificationReceiver (+epo:specifiesNotificationReceiver))</skos:definition>
   </rdf:Description>
   <rdf:Description rdf:about="http://data.europa.eu/a4g/ontology#specifiesNotificationReceiver">
      <rdfs:isDefinedBy rdf:resource="http://data.europa.eu/a4g/ontology#ful"/>
   </rdf:Description>
   <owl:ObjectProperty rdf:about="http://data.europa.eu/a4g/ontology#hasConsigneeConsignmentID"/>
   <rdf:Description rdf:about="http://data.europa.eu/a4g/ontology#hasConsigneeConsignmentID">
      <skos:prefLabel xml:lang="en">Has consignee consignment i d</skos:prefLabel>
   </rdf:Description>
   <rdf:Description rdf:about="http://data.europa.eu/a4g/ontology#hasConsigneeConsignmentID">
      <skos:definition xml:lang="en">The identifier of the the Consignment given by the Consignee. WG approval 10/06/2024 (epo-ful:Consignment -&gt; adms:Identifier (+epo-ful:hasConsigneeConsignmentID))</skos:definition>
   </rdf:Description>
   <rdf:Description rdf:about="http://data.europa.eu/a4g/ontology#hasConsigneeConsignmentID">
      <rdfs:isDefinedBy rdf:resource="http://data.europa.eu/a4g/ontology#ful"/>
   </rdf:Description>
   <owl:ObjectProperty rdf:about="http://data.europa.eu/a4g/ontology#hasRequestedPickUpInformation"/>
   <rdf:Description rdf:about="http://data.europa.eu/a4g/ontology#hasRequestedPickUpInformation">
      <skos:prefLabel xml:lang="en">Has requested pick up information</skos:prefLabel>
   </rdf:Description>
   <rdf:Description rdf:about="http://data.europa.eu/a4g/ontology#hasRequestedPickUpInformation">
      <skos:definition xml:lang="en">Information about the requested despatch of the Goods Items. WG approval 25/06/2024 (epo-ful:Consignment -&gt; epo-ful:ShipmentInformation (+epo-ful:hasRequestedPickUpInformation))</skos:definition>
   </rdf:Description>
   <rdf:Description rdf:about="http://data.europa.eu/a4g/ontology#hasRequestedPickUpInformation">
      <rdfs:isDefinedBy rdf:resource="http://data.europa.eu/a4g/ontology#ful"/>
   </rdf:Description>
   <owl:ObjectProperty rdf:about="http://data.europa.eu/a4g/ontology#refersToConsignment"/>
   <rdf:Description rdf:about="http://data.europa.eu/a4g/ontology#refersToConsignment">
      <skos:prefLabel xml:lang="en">Refers to consignment</skos:prefLabel>
   </rdf:Description>
   <rdf:Description rdf:about="http://data.europa.eu/a4g/ontology#refersToConsignment">
      <skos:definition xml:lang="en">Reference to a Consignment. WG approval 25/06/2024 (epo-ful:DespatchAdvice -&gt; epo-ful:Consignment (+epo-ful:refersToConsignment))</skos:definition>
   </rdf:Description>
   <rdf:Description rdf:about="http://data.europa.eu/a4g/ontology#refersToConsignment">
      <rdfs:isDefinedBy rdf:resource="http://data.europa.eu/a4g/ontology#ful"/>
   </rdf:Description>
   <owl:ObjectProperty rdf:about="http://data.europa.eu/a4g/ontology#hasDespatchedQuantity"/>
   <rdf:Description rdf:about="http://data.europa.eu/a4g/ontology#hasDespatchedQuantity">
      <skos:prefLabel xml:lang="en">Has despatched quantity</skos:prefLabel>
   </rdf:Description>
   <rdf:Description rdf:about="http://data.europa.eu/a4g/ontology#hasDespatchedQuantity">
      <skos:definition xml:lang="en">The Quantity that has been sent. WG approval 18/06/2024 (epo-ful:DespatchLine -&gt; epo:Quantity (+epo-ful:hasDespatchedQuantity))</skos:definition>
   </rdf:Description>
   <rdf:Description rdf:about="http://data.europa.eu/a4g/ontology#hasDespatchedQuantity">
      <rdfs:isDefinedBy rdf:resource="http://data.europa.eu/a4g/ontology#ful"/>
   </rdf:Description>
   <owl:ObjectProperty rdf:about="http://data.europa.eu/a4g/ontology#hasAssociatedDocument"/>
   <rdf:Description rdf:about="http://data.europa.eu/a4g/ontology#hasAssociatedDocument">
      <skos:prefLabel xml:lang="en">Has associated document</skos:prefLabel>
   </rdf:Description>
   <rdf:Description rdf:about="http://data.europa.eu/a4g/ontology#hasAssociatedDocument">
      <skos:definition xml:lang="en">Is related to a Document. WG approval 06/10/2024 (epo-ful:DespatchLine -&gt; epo:Document (+epo-ful:hasAssociatedDocument)) Is related to a Document. WG approval 06/10/2024 (epo-ful:DespatchAdvice -&gt; epo:Document (+epo-ful:hasAssociatedDocument))</skos:definition>
   </rdf:Description>
   <rdf:Description rdf:about="http://data.europa.eu/a4g/ontology#hasAssociatedDocument">
      <rdfs:isDefinedBy rdf:resource="http://data.europa.eu/a4g/ontology#ful"/>
   </rdf:Description>
   <owl:ObjectProperty rdf:about="http://data.europa.eu/a4g/ontology#hasOutstandingQuantity"/>
   <rdf:Description rdf:about="http://data.europa.eu/a4g/ontology#hasOutstandingQuantity">
      <skos:prefLabel xml:lang="en">Has outstanding quantity</skos:prefLabel>
   </rdf:Description>
   <rdf:Description rdf:about="http://data.europa.eu/a4g/ontology#hasOutstandingQuantity">
      <skos:definition xml:lang="en">The Quantity of non-despatched Goods Items. WG approval 05/06/2024 (epo-ful:DespatchLine -&gt; epo:Quantity (+epo-ful:hasOutstandingQuantity))</skos:definition>
   </rdf:Description>
   <rdf:Description rdf:about="http://data.europa.eu/a4g/ontology#hasOutstandingQuantity">
      <rdfs:isDefinedBy rdf:resource="http://data.europa.eu/a4g/ontology#ful"/>
   </rdf:Description>
   <owl:ObjectProperty rdf:about="http://data.europa.eu/a4g/ontology#refersToOrderLine"/>
   <rdf:Description rdf:about="http://data.europa.eu/a4g/ontology#refersToOrderLine">
      <skos:prefLabel xml:lang="en">Refers to order line</skos:prefLabel>
   </rdf:Description>
   <rdf:Description rdf:about="http://data.europa.eu/a4g/ontology#refersToOrderLine">
      <skos:definition xml:lang="en">Reference to an Order Line. WG approval 25/06/2024 (epo-ful:DespatchLine -&gt; epo-ord:OrderLine (+epo-ful:refersToOrderLine))</skos:definition>
   </rdf:Description>
   <rdf:Description rdf:about="http://data.europa.eu/a4g/ontology#refersToOrderLine">
      <rdfs:isDefinedBy rdf:resource="http://data.europa.eu/a4g/ontology#ful"/>
   </rdf:Description>
   <owl:ObjectProperty rdf:about="http://data.europa.eu/a4g/ontology#comprisesDespatchLine"/>
   <rdf:Description rdf:about="http://data.europa.eu/a4g/ontology#comprisesDespatchLine">
      <skos:prefLabel xml:lang="en">Comprises despatch line</skos:prefLabel>
   </rdf:Description>
   <rdf:Description rdf:about="http://data.europa.eu/a4g/ontology#comprisesDespatchLine">
      <skos:definition xml:lang="en">Incorporates Despatch Line. WG approval 10/06/2024 (epo-ful:DespatchAdvice -&gt; epo-ful:DespatchLine (+epo-ful:comprisesDespatchLine))</skos:definition>
   </rdf:Description>
   <rdf:Description rdf:about="http://data.europa.eu/a4g/ontology#comprisesDespatchLine">
      <rdfs:isDefinedBy rdf:resource="http://data.europa.eu/a4g/ontology#ful"/>
   </rdf:Description>
   <owl:ObjectProperty rdf:about="http://data.europa.eu/a4g/ontology#isSubmittedForDespatchLine"/>
   <rdf:Description rdf:about="http://data.europa.eu/a4g/ontology#isSubmittedForDespatchLine">
      <skos:prefLabel xml:lang="en">Is submitted for despatch line</skos:prefLabel>
   </rdf:Description>
   <rdf:Description rdf:about="http://data.europa.eu/a4g/ontology#isSubmittedForDespatchLine">
      <rdfs:isDefinedBy rdf:resource="http://data.europa.eu/a4g/ontology#ful"/>
   </rdf:Description>
   <owl:ObjectProperty rdf:about="http://data.europa.eu/a4g/ontology#transportsItemFrom"/>
   <rdf:Description rdf:about="http://data.europa.eu/a4g/ontology#transportsItemFrom">
      <skos:prefLabel xml:lang="en">Transports item from</skos:prefLabel>
   </rdf:Description>
   <rdf:Description rdf:about="http://data.europa.eu/a4g/ontology#transportsItemFrom">
      <rdfs:isDefinedBy rdf:resource="http://data.europa.eu/a4g/ontology#ful"/>
   </rdf:Description>
   <owl:ObjectProperty rdf:about="http://data.europa.eu/a4g/ontology#isSpecificToDespatchLine"/>
   <rdf:Description rdf:about="http://data.europa.eu/a4g/ontology#isSpecificToDespatchLine">
      <skos:prefLabel xml:lang="en">Is specific to despatch line</skos:prefLabel>
   </rdf:Description>
   <rdf:Description rdf:about="http://data.europa.eu/a4g/ontology#isSpecificToDespatchLine">
      <skos:definition xml:lang="en">Information that is particular to a Despatch Line. WG approval 25/06/2024 (epo-ful:ShipmentInformation -&gt; epo-ful:DespatchLine (+epo-ful:isSpecificToDespatchLine))</skos:definition>
   </rdf:Description>
   <rdf:Description rdf:about="http://data.europa.eu/a4g/ontology#isSpecificToDespatchLine">
      <rdfs:isDefinedBy rdf:resource="http://data.europa.eu/a4g/ontology#ful"/>
   </rdf:Description>
   <owl:ObjectProperty rdf:about="http://data.europa.eu/a4g/ontology#specifiesTransportHandlingUnits"/>
   <rdf:Description rdf:about="http://data.europa.eu/a4g/ontology#specifiesTransportHandlingUnits">
      <skos:prefLabel xml:lang="en">Specifies transport handling units</skos:prefLabel>
   </rdf:Description>
   <rdf:Description rdf:about="http://data.europa.eu/a4g/ontology#specifiesTransportHandlingUnits">
      <skos:definition xml:lang="en">Relation indicating the use of a Transport Handling Unit. WG approval 25/06/2024 (epo-ful:DespatchAdvice -&gt; epo-ful:TransportHandlingUnit (+epo-ful:specifiesTransportHandlingUnits))</skos:definition>
   </rdf:Description>
   <rdf:Description rdf:about="http://data.europa.eu/a4g/ontology#specifiesTransportHandlingUnits">
      <rdfs:isDefinedBy rdf:resource="http://data.europa.eu/a4g/ontology#ful"/>
   </rdf:Description>
   <owl:ObjectProperty rdf:about="http://data.europa.eu/a4g/ontology#hasEstimatedDeliveryPeriod"/>
   <rdf:Description rdf:about="http://data.europa.eu/a4g/ontology#hasEstimatedDeliveryPeriod">
      <skos:prefLabel xml:lang="en">Has estimated delivery period</skos:prefLabel>
   </rdf:Description>
   <rdf:Description rdf:about="http://data.europa.eu/a4g/ontology#hasEstimatedDeliveryPeriod">
      <skos:definition xml:lang="en">The forecasted time period given by the Despatcher to provide the goods and services. WG approval 18/06/2024 (epo-ful:ShipmentInformation -&gt; epo:Period (+epo-ful:hasEstimatedDeliveryPeriod))</skos:definition>
   </rdf:Description>
   <rdf:Description rdf:about="http://data.europa.eu/a4g/ontology#hasEstimatedDeliveryPeriod">
      <rdfs:isDefinedBy rdf:resource="http://data.europa.eu/a4g/ontology#ful"/>
   </rdf:Description>
   <owl:ObjectProperty rdf:about="http://data.europa.eu/a4g/ontology#hasDespatchPeriod"/>
   <rdf:Description rdf:about="http://data.europa.eu/a4g/ontology#hasDespatchPeriod">
      <skos:prefLabel xml:lang="en">Has despatch period</skos:prefLabel>
   </rdf:Description>
   <rdf:Description rdf:about="http://data.europa.eu/a4g/ontology#hasDespatchPeriod">
      <skos:definition xml:lang="en">The time period when the Despatcher picks-up the Goods Items to be delivered. WG approval 16/07/2024 (epo-ful:ShipmentInformation -&gt; epo:Period (+epo-ful:hasDespatchPeriod))</skos:definition>
   </rdf:Description>
   <rdf:Description rdf:about="http://data.europa.eu/a4g/ontology#hasDespatchPeriod">
      <rdfs:isDefinedBy rdf:resource="http://data.europa.eu/a4g/ontology#ful"/>
   </rdf:Description>
   <owl:ObjectProperty rdf:about="http://data.europa.eu/a4g/ontology#refersToDeliveryInformation"/>
   <rdf:Description rdf:about="http://data.europa.eu/a4g/ontology#refersToDeliveryInformation">
      <skos:prefLabel xml:lang="en">Refers to delivery information</skos:prefLabel>
   </rdf:Description>
   <rdf:Description rdf:about="http://data.europa.eu/a4g/ontology#refersToDeliveryInformation">
      <skos:definition xml:lang="en">Reference to a Delivery Information. WG approval 25/06/2024 (epo-ful:ShipmentInformation -&gt; epo-ord:DeliveryInformation (+epo-ful:refersToDeliveryInformation))</skos:definition>
   </rdf:Description>
   <rdf:Description rdf:about="http://data.europa.eu/a4g/ontology#refersToDeliveryInformation">
      <rdfs:isDefinedBy rdf:resource="http://data.europa.eu/a4g/ontology#ful"/>
   </rdf:Description>
   <owl:ObjectProperty rdf:about="http://data.europa.eu/a4g/ontology#specifiesPlaceOfDespatch"/>
   <rdf:Description rdf:about="http://data.europa.eu/a4g/ontology#specifiesPlaceOfDespatch">
      <skos:prefLabel xml:lang="en">Specifies place of despatch</skos:prefLabel>
   </rdf:Description>
   <rdf:Description rdf:about="http://data.europa.eu/a4g/ontology#specifiesPlaceOfDespatch">
      <skos:definition xml:lang="en">Relation indicating the Location of the Despatch of the Goods Items to be delivered. WG approval 25/06/2024 (epo-ful:ShipmentInformation -&gt; dct:Location (+epo-ful:specifiesPlaceOfDespatch))</skos:definition>
   </rdf:Description>
   <rdf:Description rdf:about="http://data.europa.eu/a4g/ontology#specifiesPlaceOfDespatch">
      <rdfs:isDefinedBy rdf:resource="http://data.europa.eu/a4g/ontology#ful"/>
   </rdf:Description>
   <owl:ObjectProperty rdf:about="http://data.europa.eu/a4g/ontology#specifiesShipment"/>
   <rdf:Description rdf:about="http://data.europa.eu/a4g/ontology#specifiesShipment">
      <skos:prefLabel xml:lang="en">Specifies shipment</skos:prefLabel>
   </rdf:Description>
   <rdf:Description rdf:about="http://data.europa.eu/a4g/ontology#specifiesShipment">
      <rdfs:isDefinedBy rdf:resource="http://data.europa.eu/a4g/ontology#ful"/>
   </rdf:Description>
   <owl:ObjectProperty rdf:about="http://data.europa.eu/a4g/ontology#isSubmittedForShipment"/>
   <rdf:Description rdf:about="http://data.europa.eu/a4g/ontology#isSubmittedForShipment">
      <skos:prefLabel xml:lang="en">Is submitted for shipment</skos:prefLabel>
   </rdf:Description>
   <rdf:Description rdf:about="http://data.europa.eu/a4g/ontology#isSubmittedForShipment">
      <rdfs:isDefinedBy rdf:resource="http://data.europa.eu/a4g/ontology#ful"/>
   </rdf:Description>
   <owl:ObjectProperty rdf:about="http://data.europa.eu/a4g/ontology#specifiesDespatcher"/>
   <rdf:Description rdf:about="http://data.europa.eu/a4g/ontology#specifiesDespatcher">
      <skos:prefLabel xml:lang="en">Specifies despatcher</skos:prefLabel>
   </rdf:Description>
   <rdf:Description rdf:about="http://data.europa.eu/a4g/ontology#specifiesDespatcher">
      <skos:definition xml:lang="en">Relation indicating that the instance of the concept involves the Despatcher. WG approval 25/06/2024 (epo-ful:DespatchAdvice -&gt; epo-ful:Despatcher (+epo-ful:specifiesDespatcher))</skos:definition>
   </rdf:Description>
   <rdf:Description rdf:about="http://data.europa.eu/a4g/ontology#specifiesDespatcher">
      <rdfs:isDefinedBy rdf:resource="http://data.europa.eu/a4g/ontology#ful"/>
   </rdf:Description>
   <owl:ObjectProperty rdf:about="http://data.europa.eu/a4g/ontology#specifiesDespatcher"/>
   <rdf:Description rdf:about="http://data.europa.eu/a4g/ontology#specifiesDespatcher">
      <skos:prefLabel xml:lang="en">Specifies despatcher</skos:prefLabel>
   </rdf:Description>
   <rdf:Description rdf:about="http://data.europa.eu/a4g/ontology#specifiesDespatcher">
      <skos:definition xml:lang="en">Relation indicating that the instance of the concept involves the Despatcher. WG approval 25/06/2024 (epo-ord:Order -&gt; epo-ful:Despatcher (+epo:specifiesDespatcher))</skos:definition>
   </rdf:Description>
   <rdf:Description rdf:about="http://data.europa.eu/a4g/ontology#specifiesDespatcher">
      <rdfs:isDefinedBy rdf:resource="http://data.europa.eu/a4g/ontology#ful"/>
   </rdf:Description>
   <owl:ObjectProperty rdf:about="http://data.europa.eu/a4g/ontology#refersToOrder"/>
   <rdf:Description rdf:about="http://data.europa.eu/a4g/ontology#refersToOrder">
      <skos:prefLabel xml:lang="en">Refers to order</skos:prefLabel>
   </rdf:Description>
   <rdf:Description rdf:about="http://data.europa.eu/a4g/ontology#refersToOrder">
      <skos:definition xml:lang="en">Reference to an Order. WG approval 25/06/2024 (epo-ful:DespatchAdvice -&gt; epo-ord:Order (+epo-ful:refersToOrder))</skos:definition>
   </rdf:Description>
   <rdf:Description rdf:about="http://data.europa.eu/a4g/ontology#refersToOrder">
      <rdfs:isDefinedBy rdf:resource="http://data.europa.eu/a4g/ontology#ful"/>
   </rdf:Description>
   <owl:ObjectProperty rdf:about="http://data.europa.eu/a4g/ontology#hasDespatchAdviceType"/>
   <rdf:Description rdf:about="http://data.europa.eu/a4g/ontology#hasDespatchAdviceType">
      <skos:prefLabel xml:lang="en">Has despatch advice type</skos:prefLabel>
   </rdf:Description>
   <rdf:Description rdf:about="http://data.europa.eu/a4g/ontology#hasDespatchAdviceType">
      <skos:definition xml:lang="en">Classification of a Despatch Advice. WG approval 18/06/2024 (epo-ful:DespatchAdvice -&gt; at-voc-new:despatch-advice-type (+epo-ful:hasDespatchAdviceType))</skos:definition>
   </rdf:Description>
   <rdf:Description rdf:about="http://data.europa.eu/a4g/ontology#hasDespatchAdviceType">
      <rdfs:isDefinedBy rdf:resource="http://data.europa.eu/a4g/ontology#ful"/>
   </rdf:Description>
   <owl:ObjectProperty rdf:about="http://data.europa.eu/a4g/ontology#specifiesConsignee"/>
   <rdf:Description rdf:about="http://data.europa.eu/a4g/ontology#specifiesConsignee">
      <skos:prefLabel xml:lang="en">Specifies consignee</skos:prefLabel>
   </rdf:Description>
   <rdf:Description rdf:about="http://data.europa.eu/a4g/ontology#specifiesConsignee">
      <skos:definition xml:lang="en">Relation indicating that the instance of the concept involves the Consignee. WG approval 25/06/2024 (epo-ful:DespatchAdvice -&gt; epo-ord:Consignee (+epo-ful:specifiesConsignee))</skos:definition>
   </rdf:Description>
   <rdf:Description rdf:about="http://data.europa.eu/a4g/ontology#specifiesConsignee">
      <rdfs:isDefinedBy rdf:resource="http://data.europa.eu/a4g/ontology#ful"/>
   </rdf:Description>
   <owl:ObjectProperty rdf:about="http://data.europa.eu/a4g/ontology#specifiesOriginator"/>
   <rdf:Description rdf:about="http://data.europa.eu/a4g/ontology#specifiesOriginator">
      <skos:prefLabel xml:lang="en">Specifies originator</skos:prefLabel>
   </rdf:Description>
   <rdf:Description rdf:about="http://data.europa.eu/a4g/ontology#specifiesOriginator">
      <skos:definition xml:lang="en">Relation indicating that the instance of the concept involves the Originator. WG approval 25/06/2024 (epo-ful:DespatchAdvice -&gt; epo-ord:Originator (+epo-ful:specifiesOriginator))</skos:definition>
   </rdf:Description>
   <rdf:Description rdf:about="http://data.europa.eu/a4g/ontology#specifiesOriginator">
      <rdfs:isDefinedBy rdf:resource="http://data.europa.eu/a4g/ontology#ful"/>
   </rdf:Description>
   <owl:ObjectProperty rdf:about="http://data.europa.eu/a4g/ontology#isSubmittedForDespatchAdvice"/>
   <rdf:Description rdf:about="http://data.europa.eu/a4g/ontology#isSubmittedForDespatchAdvice">
      <skos:prefLabel xml:lang="en">Is submitted for despatch advice</skos:prefLabel>
   </rdf:Description>
   <rdf:Description rdf:about="http://data.europa.eu/a4g/ontology#isSubmittedForDespatchAdvice">
      <skos:definition xml:lang="en">Additional information: In PEPPOL (https://test-docs.peppol.eu/logistics/qa/codelist/ReceiptAdviceTypeCode/) this predicate is used for option D - Response to the Advanced Despatch Advice document. (epo-ful:ReceiptAdvice -&gt; epo-ful:DespatchAdvice (+epo-ful:isSubmittedForDespatchAdvice))</skos:definition>
   </rdf:Description>
   <rdf:Description rdf:about="http://data.europa.eu/a4g/ontology#isSubmittedForDespatchAdvice">
      <rdfs:isDefinedBy rdf:resource="http://data.europa.eu/a4g/ontology#ful"/>
   </rdf:Description>
   <owl:ObjectProperty rdf:about="http://data.europa.eu/a4g/ontology#refersToDespatchAdvice"/>
   <rdf:Description rdf:about="http://data.europa.eu/a4g/ontology#refersToDespatchAdvice">
      <skos:prefLabel xml:lang="en">Refers to despatch advice</skos:prefLabel>
   </rdf:Description>
   <rdf:Description rdf:about="http://data.europa.eu/a4g/ontology#refersToDespatchAdvice">
      <rdfs:isDefinedBy rdf:resource="http://data.europa.eu/a4g/ontology#ful"/>
   </rdf:Description>
   <owl:ObjectProperty rdf:about="http://data.europa.eu/a4g/ontology#hasAllowanceChargeReason"/>
   <rdf:Description rdf:about="http://data.europa.eu/a4g/ontology#hasAllowanceChargeReason">
      <skos:prefLabel xml:lang="en">Has allowance charge reason</skos:prefLabel>
   </rdf:Description>
   <rdf:Description rdf:about="http://data.europa.eu/a4g/ontology#hasAllowanceChargeReason">
      <skos:definition xml:lang="en">The justification for using the Allowance or the Charge. WG approval 10/06/2024 (epo-ord:AllowanceChargeInformation -&gt; at-voc-new:allowance-charge-reason (+epo-ful:hasAllowanceChargeReason))</skos:definition>
   </rdf:Description>
   <rdf:Description rdf:about="http://data.europa.eu/a4g/ontology#hasAllowanceChargeReason">
      <rdfs:isDefinedBy rdf:resource="http://data.europa.eu/a4g/ontology#ful"/>
   </rdf:Description>
   <owl:ObjectProperty rdf:about="http://data.europa.eu/a4g/ontology#hasDocumentStatus"/>
   <rdf:Description rdf:about="http://data.europa.eu/a4g/ontology#hasDocumentStatus">
      <skos:prefLabel xml:lang="en">Has document status</skos:prefLabel>
   </rdf:Description>
   <rdf:Description rdf:about="http://data.europa.eu/a4g/ontology#hasDocumentStatus">
      <skos:definition xml:lang="en">https://test-docs.peppol.eu/logistics/transport-execution/codelist/DocumentStatusCode/ (epo-cat:PostAwardDocument -&gt; at-voc-new:document-status (+epo:hasDocumentStatus))</skos:definition>
   </rdf:Description>
   <rdf:Description rdf:about="http://data.europa.eu/a4g/ontology#hasDocumentStatus">
      <rdfs:isDefinedBy rdf:resource="http://data.europa.eu/a4g/ontology#ful"/>
   </rdf:Description>
   <owl:ObjectProperty rdf:about="http://data.europa.eu/a4g/ontology#specifiesBuyer"/>
   <rdf:Description rdf:about="http://data.europa.eu/a4g/ontology#specifiesBuyer">
      <skos:prefLabel xml:lang="en">Specifies buyer</skos:prefLabel>
   </rdf:Description>
   <rdf:Description rdf:about="http://data.europa.eu/a4g/ontology#specifiesBuyer">
      <rdfs:isDefinedBy rdf:resource="http://data.europa.eu/a4g/ontology#ful"/>
   </rdf:Description>
   <owl:ObjectProperty rdf:about="http://data.europa.eu/a4g/ontology#specifiesSeller"/>
   <rdf:Description rdf:about="http://data.europa.eu/a4g/ontology#specifiesSeller">
      <skos:prefLabel xml:lang="en">Specifies seller</skos:prefLabel>
   </rdf:Description>
   <rdf:Description rdf:about="http://data.europa.eu/a4g/ontology#specifiesSeller">
      <rdfs:isDefinedBy rdf:resource="http://data.europa.eu/a4g/ontology#ful"/>
   </rdf:Description>
   <owl:ObjectProperty rdf:about="http://data.europa.eu/a4g/ontology#comprisesReceiptAdviceLine"/>
   <rdf:Description rdf:about="http://data.europa.eu/a4g/ontology#comprisesReceiptAdviceLine">
      <skos:prefLabel xml:lang="en">Comprises receipt advice line</skos:prefLabel>
   </rdf:Description>
   <rdf:Description rdf:about="http://data.europa.eu/a4g/ontology#comprisesReceiptAdviceLine">
      <rdfs:isDefinedBy rdf:resource="http://data.europa.eu/a4g/ontology#ful"/>
   </rdf:Description>
   <owl:ObjectProperty rdf:about="http://data.europa.eu/a4g/ontology#refersToReceiptAdvice"/>
   <rdf:Description rdf:about="http://data.europa.eu/a4g/ontology#refersToReceiptAdvice">
      <skos:prefLabel xml:lang="en">Refers to receipt advice</skos:prefLabel>
   </rdf:Description>
   <rdf:Description rdf:about="http://data.europa.eu/a4g/ontology#refersToReceiptAdvice">
      <rdfs:isDefinedBy rdf:resource="http://data.europa.eu/a4g/ontology#ful"/>
   </rdf:Description>
   <owl:ObjectProperty rdf:about="http://data.europa.eu/a4g/ontology#hasOversupplyQuantity"/>
   <rdf:Description rdf:about="http://data.europa.eu/a4g/ontology#hasOversupplyQuantity">
      <skos:prefLabel xml:lang="en">Has oversupply quantity</skos:prefLabel>
   </rdf:Description>
   <rdf:Description rdf:about="http://data.europa.eu/a4g/ontology#hasOversupplyQuantity">
      <rdfs:isDefinedBy rdf:resource="http://data.europa.eu/a4g/ontology#ful"/>
   </rdf:Description>
   <owl:ObjectProperty rdf:about="http://data.europa.eu/a4g/ontology#hasReceivedQuantity"/>
   <rdf:Description rdf:about="http://data.europa.eu/a4g/ontology#hasReceivedQuantity">
      <skos:prefLabel xml:lang="en">Has received quantity</skos:prefLabel>
   </rdf:Description>
   <rdf:Description rdf:about="http://data.europa.eu/a4g/ontology#hasReceivedQuantity">
      <rdfs:isDefinedBy rdf:resource="http://data.europa.eu/a4g/ontology#ful"/>
   </rdf:Description>
   <owl:ObjectProperty rdf:about="http://data.europa.eu/a4g/ontology#hasShortageAction"/>
   <rdf:Description rdf:about="http://data.europa.eu/a4g/ontology#hasShortageAction">
      <skos:prefLabel xml:lang="en">Has shortage action</skos:prefLabel>
   </rdf:Description>
   <rdf:Description rdf:about="http://data.europa.eu/a4g/ontology#hasShortageAction">
      <rdfs:isDefinedBy rdf:resource="http://data.europa.eu/a4g/ontology#ful"/>
   </rdf:Description>
   <owl:ObjectProperty rdf:about="http://data.europa.eu/a4g/ontology#hasShortQuantity"/>
   <rdf:Description rdf:about="http://data.europa.eu/a4g/ontology#hasShortQuantity">
      <skos:prefLabel xml:lang="en">Has short quantity</skos:prefLabel>
   </rdf:Description>
   <rdf:Description rdf:about="http://data.europa.eu/a4g/ontology#hasShortQuantity">
      <rdfs:isDefinedBy rdf:resource="http://data.europa.eu/a4g/ontology#ful"/>
   </rdf:Description>
   <owl:ObjectProperty rdf:about="http://data.europa.eu/a4g/ontology#hasRejectReason"/>
   <rdf:Description rdf:about="http://data.europa.eu/a4g/ontology#hasRejectReason">
      <skos:prefLabel xml:lang="en">Has reject reason</skos:prefLabel>
   </rdf:Description>
   <rdf:Description rdf:about="http://data.europa.eu/a4g/ontology#hasRejectReason">
      <rdfs:isDefinedBy rdf:resource="http://data.europa.eu/a4g/ontology#ful"/>
   </rdf:Description>
   <owl:ObjectProperty rdf:about="http://data.europa.eu/a4g/ontology#hasRejectedQuantity"/>
   <rdf:Description rdf:about="http://data.europa.eu/a4g/ontology#hasRejectedQuantity">
      <skos:prefLabel xml:lang="en">Has rejected quantity</skos:prefLabel>
   </rdf:Description>
   <rdf:Description rdf:about="http://data.europa.eu/a4g/ontology#hasRejectedQuantity">
      <rdfs:isDefinedBy rdf:resource="http://data.europa.eu/a4g/ontology#ful"/>
   </rdf:Description>
   <owl:ObjectProperty rdf:about="http://data.europa.eu/a4g/ontology#RejectionAction"/>
   <rdf:Description rdf:about="http://data.europa.eu/a4g/ontology#RejectionAction">
      <skos:prefLabel xml:lang="en">Rejection action</skos:prefLabel>
   </rdf:Description>
   <rdf:Description rdf:about="http://data.europa.eu/a4g/ontology#RejectionAction">
      <rdfs:isDefinedBy rdf:resource="http://data.europa.eu/a4g/ontology#ful"/>
   </rdf:Description>
   <owl:DatatypeProperty rdf:about="http://purl.org/dc/terms/description"/>
   <rdf:Description rdf:about="http://purl.org/dc/terms/description">
      <skos:prefLabel xml:lang="en">Description</skos:prefLabel>
   </rdf:Description>
   <rdf:Description rdf:about="http://purl.org/dc/terms/description">
      <skos:definition xml:lang="en">An account of the resource. Additional Information: Description may include but is not limited to: an abstract, a table of contents, a graphical representation, or a free-text account of the resource. WG Approval 30/05/2023 (epo-ful:TemperatureSpecification) An account of the resource. Additional Information: Description may include but is not limited to: an abstract, a table of contents, a graphical representation, or a free-text account of the resource. WG Approval 30/05/2023 (epo-ful:TransportEquipment) An account of the resource. Additional Information: Description may include but is not limited to: an abstract, a table of contents, a graphical representation, or a free-text account of the resource. WG Approval 30/05/2023 (epo-ful:ShipmentInformation)</skos:definition>
   </rdf:Description>
   <owl:DatatypeProperty rdf:about="http://data.europa.eu/a4g/ontology#isReturnableMaterial"/>
   <rdf:Description rdf:about="http://data.europa.eu/a4g/ontology#isReturnableMaterial">
      <skos:prefLabel xml:lang="en">Is returnable material</skos:prefLabel>
   </rdf:Description>
   <rdf:Description rdf:about="http://data.europa.eu/a4g/ontology#isReturnableMaterial">
      <skos:definition xml:lang="en">Indicates whether the container or part of the container is to be sent back. WG approval 21/05/2024 (epo-ful:AbstractContainer)</skos:definition>
   </rdf:Description>
   <rdf:Description rdf:about="http://data.europa.eu/a4g/ontology#isReturnableMaterial">
      <rdfs:isDefinedBy rdf:resource="http://data.europa.eu/a4g/ontology#ful"/>
   </rdf:Description>
   <owl:DatatypeProperty rdf:about="http://data.europa.eu/a4g/ontology#isHazardousRisk"/>
   <rdf:Description rdf:about="http://data.europa.eu/a4g/ontology#isHazardousRisk">
      <skos:prefLabel xml:lang="en">Is hazardous risk</skos:prefLabel>
   </rdf:Description>
   <rdf:Description rdf:about="http://data.europa.eu/a4g/ontology#isHazardousRisk">
      <skos:definition xml:lang="en">Indicates whether some of the contained Goods Items are hazardous. WG approval 21/05/2024 (epo-ful:AbstractContainer) Pending confirmation on whether this attribute should be removed in the next major release because is covered at the level of Consignment. (epo-ful:ShipmentStage) Indicates whether some of the contained Goods Items are hazardous. WG approval 21/05/2024 (epo-ful:Consignment)</skos:definition>
   </rdf:Description>
   <rdf:Description rdf:about="http://data.europa.eu/a4g/ontology#isHazardousRisk">
      <rdfs:isDefinedBy rdf:resource="http://data.europa.eu/a4g/ontology#ful"/>
   </rdf:Description>
   <owl:DatatypeProperty rdf:about="http://data.europa.eu/a4g/ontology#hasPackagingTypeDescription"/>
   <rdf:Description rdf:about="http://data.europa.eu/a4g/ontology#hasPackagingTypeDescription">
      <skos:prefLabel xml:lang="en">Has packaging type description</skos:prefLabel>
   </rdf:Description>
   <rdf:Description rdf:about="http://data.europa.eu/a4g/ontology#hasPackagingTypeDescription">
      <skos:definition xml:lang="en">Explanatory text about how the Goods Item is packed. WG approval 05/06/2024 (epo-ful:Package)</skos:definition>
   </rdf:Description>
   <rdf:Description rdf:about="http://data.europa.eu/a4g/ontology#hasPackagingTypeDescription">
      <rdfs:isDefinedBy rdf:resource="http://data.europa.eu/a4g/ontology#ful"/>
   </rdf:Description>
   <owl:DatatypeProperty rdf:about="http://data.europa.eu/a4g/ontology#isReturnable"/>
   <rdf:Description rdf:about="http://data.europa.eu/a4g/ontology#isReturnable">
      <skos:prefLabel xml:lang="en">Is returnable</skos:prefLabel>
   </rdf:Description>
   <rdf:Description rdf:about="http://data.europa.eu/a4g/ontology#isReturnable">
      <rdfs:isDefinedBy rdf:resource="http://data.europa.eu/a4g/ontology#ful"/>
   </rdf:Description>
   <owl:DatatypeProperty rdf:about="http://data.europa.eu/a4g/ontology#isRefrigerated"/>
   <rdf:Description rdf:about="http://data.europa.eu/a4g/ontology#isRefrigerated">
      <skos:prefLabel xml:lang="en">Is refrigerated</skos:prefLabel>
   </rdf:Description>
   <rdf:Description rdf:about="http://data.europa.eu/a4g/ontology#isRefrigerated">
      <skos:definition xml:lang="en">Indicates whether the instance of the concept includes refrigeration. Additional Information: The instance of the concept can be, for example, Transport Equipment. WG approval 05/06/2024 (epo-ful:TransportEquipment)</skos:definition>
   </rdf:Description>
   <rdf:Description rdf:about="http://data.europa.eu/a4g/ontology#isRefrigerated">
      <rdfs:isDefinedBy rdf:resource="http://data.europa.eu/a4g/ontology#ful"/>
   </rdf:Description>
   <owl:DatatypeProperty rdf:about="http://data.europa.eu/a4g/ontology#isPowerIndicated"/>
   <rdf:Description rdf:about="http://data.europa.eu/a4g/ontology#isPowerIndicated">
      <skos:prefLabel xml:lang="en">Is power indicated</skos:prefLabel>
   </rdf:Description>
   <rdf:Description rdf:about="http://data.europa.eu/a4g/ontology#isPowerIndicated">
      <skos:definition xml:lang="en">Indicates whether the instance of the concept can supply electrical energy. Additional Information: The instance of the concept can be, for example, Transport Equipment. WG approval 05/06/2024 (epo-ful:TransportEquipment)</skos:definition>
   </rdf:Description>
   <rdf:Description rdf:about="http://data.europa.eu/a4g/ontology#isPowerIndicated">
      <rdfs:isDefinedBy rdf:resource="http://data.europa.eu/a4g/ontology#ful"/>
   </rdf:Description>
   <owl:DatatypeProperty rdf:about="http://data.europa.eu/a4g/ontology#hasVehicleDescription"/>
   <rdf:Description rdf:about="http://data.europa.eu/a4g/ontology#hasVehicleDescription">
      <skos:prefLabel xml:lang="en">Has vehicle description</skos:prefLabel>
   </rdf:Description>
   <rdf:Description rdf:about="http://data.europa.eu/a4g/ontology#hasVehicleDescription">
      <skos:definition xml:lang="en">(epo-ful:Consignment)</skos:definition>
   </rdf:Description>
   <rdf:Description rdf:about="http://data.europa.eu/a4g/ontology#hasVehicleDescription">
      <rdfs:isDefinedBy rdf:resource="http://data.europa.eu/a4g/ontology#ful"/>
   </rdf:Description>
   <owl:DatatypeProperty rdf:about="http://data.europa.eu/a4g/ontology#hasHandlingInstruction"/>
   <rdf:Description rdf:about="http://data.europa.eu/a4g/ontology#hasHandlingInstruction">
      <skos:prefLabel xml:lang="en">Has handling instruction</skos:prefLabel>
   </rdf:Description>
   <rdf:Description rdf:about="http://data.europa.eu/a4g/ontology#hasHandlingInstruction">
      <skos:definition xml:lang="en">Instruction on how to handle the Goods Items during transportation. WG approval 05/06/2024 (epo-ful:Consignment) Instruction on how to handle the Goods Items during transportation. WG approval 05/06/2024 (epo-ful:TransportHandlingUnit)</skos:definition>
   </rdf:Description>
   <rdf:Description rdf:about="http://data.europa.eu/a4g/ontology#hasHandlingInstruction">
      <rdfs:isDefinedBy rdf:resource="http://data.europa.eu/a4g/ontology#ful"/>
   </rdf:Description>
   <owl:DatatypeProperty rdf:about="http://data.europa.eu/a4g/ontology#hasCarrierServiceInstruction"/>
   <rdf:Description rdf:about="http://data.europa.eu/a4g/ontology#hasCarrierServiceInstruction">
      <skos:prefLabel xml:lang="en">Has carrier service instruction</skos:prefLabel>
   </rdf:Description>
   <rdf:Description rdf:about="http://data.europa.eu/a4g/ontology#hasCarrierServiceInstruction">
      <skos:definition xml:lang="en">This attribute should be removed in the next major release. (epo-ful:Consignment)</skos:definition>
   </rdf:Description>
   <rdf:Description rdf:about="http://data.europa.eu/a4g/ontology#hasCarrierServiceInstruction">
      <rdfs:isDefinedBy rdf:resource="http://data.europa.eu/a4g/ontology#ful"/>
   </rdf:Description>
   <owl:DatatypeProperty rdf:about="http://data.europa.eu/a4g/ontology#hasSpecialInstruction"/>
   <rdf:Description rdf:about="http://data.europa.eu/a4g/ontology#hasSpecialInstruction">
      <skos:prefLabel xml:lang="en">Has special instruction</skos:prefLabel>
   </rdf:Description>
   <rdf:Description rdf:about="http://data.europa.eu/a4g/ontology#hasSpecialInstruction">
      <skos:definition xml:lang="en">This attribute should be removed in the next major release. (epo-ful:Consignment)</skos:definition>
   </rdf:Description>
   <rdf:Description rdf:about="http://data.europa.eu/a4g/ontology#hasSpecialInstruction">
      <rdfs:isDefinedBy rdf:resource="http://data.europa.eu/a4g/ontology#ful"/>
   </rdf:Description>
   <owl:DatatypeProperty rdf:about="http://data.europa.eu/a4g/ontology#hasDeliveryInstruction"/>
   <rdf:Description rdf:about="http://data.europa.eu/a4g/ontology#hasDeliveryInstruction">
      <skos:prefLabel xml:lang="en">Has delivery instruction</skos:prefLabel>
   </rdf:Description>
   <rdf:Description rdf:about="http://data.europa.eu/a4g/ontology#hasDeliveryInstruction">
      <skos:definition xml:lang="en">This attribute should be removed in the next major release. (epo-ful:Consignment)</skos:definition>
   </rdf:Description>
   <rdf:Description rdf:about="http://data.europa.eu/a4g/ontology#hasDeliveryInstruction">
      <rdfs:isDefinedBy rdf:resource="http://data.europa.eu/a4g/ontology#ful"/>
   </rdf:Description>
   <owl:DatatypeProperty rdf:about="http://data.europa.eu/a4g/ontology#hasSpecialServiceInstruction"/>
   <rdf:Description rdf:about="http://data.europa.eu/a4g/ontology#hasSpecialServiceInstruction">
      <skos:prefLabel xml:lang="en">Has special service instruction</skos:prefLabel>
   </rdf:Description>
   <rdf:Description rdf:about="http://data.europa.eu/a4g/ontology#hasSpecialServiceInstruction">
      <skos:definition xml:lang="en">Description about special services needed for loading or unloading the Goods Items. WG approval 21/05/2024 (epo-ful:Consignment)</skos:definition>
   </rdf:Description>
   <rdf:Description rdf:about="http://data.europa.eu/a4g/ontology#hasSpecialServiceInstruction">
      <rdfs:isDefinedBy rdf:resource="http://data.europa.eu/a4g/ontology#ful"/>
   </rdf:Description>
   <owl:DatatypeProperty rdf:about="http://data.europa.eu/a4g/ontology#hasOutstandingQuantityReason"/>
   <rdf:Description rdf:about="http://data.europa.eu/a4g/ontology#hasOutstandingQuantityReason">
      <skos:prefLabel xml:lang="en">Has outstanding quantity reason</skos:prefLabel>
   </rdf:Description>
   <rdf:Description rdf:about="http://data.europa.eu/a4g/ontology#hasOutstandingQuantityReason">
      <skos:definition xml:lang="en">Explanation of the outstanding quantity still to be despatched. WG approval 05/06/2024 (epo-ful:DespatchLine)</skos:definition>
   </rdf:Description>
   <rdf:Description rdf:about="http://data.europa.eu/a4g/ontology#hasOutstandingQuantityReason">
      <rdfs:isDefinedBy rdf:resource="http://data.europa.eu/a4g/ontology#ful"/>
   </rdf:Description>
   <owl:DatatypeProperty rdf:about="http://data.europa.eu/a4g/ontology#hasShippingMark"/>
   <rdf:Description rdf:about="http://data.europa.eu/a4g/ontology#hasShippingMark">
      <skos:prefLabel xml:lang="en">Has shipping mark</skos:prefLabel>
   </rdf:Description>
   <rdf:Description rdf:about="http://data.europa.eu/a4g/ontology#hasShippingMark">
      <skos:definition xml:lang="en">A text that the buyer requests to be printed on the packing labels. WG approval 05/06/2024 (epo-ful:TransportHandlingUnit)</skos:definition>
   </rdf:Description>
   <rdf:Description rdf:about="http://data.europa.eu/a4g/ontology#hasShippingMark">
      <rdfs:isDefinedBy rdf:resource="http://data.europa.eu/a4g/ontology#ful"/>
   </rdf:Description>
   <owl:DatatypeProperty rdf:about="http://data.europa.eu/a4g/ontology#despatchDate"/>
   <rdf:Description rdf:about="http://data.europa.eu/a4g/ontology#despatchDate">
      <skos:prefLabel xml:lang="en">Despatch date</skos:prefLabel>
   </rdf:Description>
   <rdf:Description rdf:about="http://data.europa.eu/a4g/ontology#despatchDate">
      <skos:definition xml:lang="en">The date of sending of goods or the execution of works or services. WG approval 05/06/2024 (epo-ful:ShipmentInformation)</skos:definition>
   </rdf:Description>
   <rdf:Description rdf:about="http://data.europa.eu/a4g/ontology#despatchDate">
      <rdfs:isDefinedBy rdf:resource="http://data.europa.eu/a4g/ontology#ful"/>
   </rdf:Description>
</rdf:RDF>
