<?xml version="1.0" encoding="utf-8"?>
<rdf:RDF xmlns:a4g="http://data.europa.eu/a4g/ontology#" xmlns:a4g_shape="http://data.europa.eu/a4g/data-shape#" xmlns:adms="http://www.w3.org/ns/adms#" xmlns:at="http://publications.europa.eu/ontology/authority/" xmlns:atold="http://publications.europa.eu/resource/authority/" xmlns:cpov="http://data.europa.eu/m8g/" xmlns:dcterms="http://purl.org/dc/terms/" xmlns:eli="http://data.europa.eu/eli/ontology#" xmlns:foaf="http://xmlns.com/foaf/0.1/" xmlns:locn="http://www.w3.org/ns/locn#" xmlns:org="http://www.w3.org/ns/org#" xmlns:owl="http://www.w3.org/2002/07/owl#" xmlns:person="http://www.w3.org/ns/person#" xmlns:r2rml="http://www.w3.org/ns/r2rml#" xmlns:rdf="http://www.w3.org/1999/02/22-rdf-syntax-ns#" xmlns:rdfs="http://www.w3.org/2000/01/rdf-schema#" xmlns:rml="http://semweb.mmlab.be/ns/rml#" xmlns:schema="http://schema.org/" xmlns:sfrml="http://data.europa.eu/a4g/mapping/sf-rml/" xmlns:sh="http://www.w3.org/ns/shacl#" xmlns:skos="http://www.w3.org/2004/02/skos/core#" xmlns:time="http://www.w3.org/2006/time#" xmlns:vann="http://purl.org/vocab/vann/" xmlns:xsd="http://www.w3.org/2001/XMLSchema#">
  <rdf:Description rdf:about="http://data.europa.eu/a4g/ontology#Carrier">
    <rdf:type rdf:resource="http://www.w3.org/2002/07/owl#Class"/>
  </rdf:Description>
  <rdf:Description rdf:about="http://data.europa.eu/a4g/ontology#Carrier">
    <rdfs:isDefinedBy rdf:resource="http://data.europa.eu/a4g/ontology#ful"/>
  </rdf:Description>
  <rdf:Description rdf:about="http://data.europa.eu/a4g/ontology#Carrier">
    <rdfs:subClassOf rdf:resource="http://data.europa.eu/a4g/ontology#AuxiliaryParty"/>
  </rdf:Description>
  <rdf:Description rdf:about="http://data.europa.eu/a4g/ontology#Carrier">
    <skos:definition xml:lang="en">The Role of an Agent who handles the physical Delivery/Transportation of the (Despatched) Shipment. Additional Information: This Role is often referred to as the deliverer.</skos:definition>
  </rdf:Description>
  <rdf:Description rdf:about="http://data.europa.eu/a4g/ontology#Carrier">
    <skos:prefLabel xml:lang="en">Carrier</skos:prefLabel>
  </rdf:Description>
  <rdf:Description rdf:about="http://data.europa.eu/a4g/ontology#ful">
    <rdf:type rdf:resource="http://www.w3.org/2002/07/owl#Ontology"/>
  </rdf:Description>
  <rdf:Description rdf:about="http://data.europa.eu/a4g/ontology#ful">
    <dcterms:description xml:lang="en">The eProcurement Ontology Fulfilment core describes the concepts and properties representing the European Public Procurement Fulfilment domain. The provision of these semantics offers the basis for a common understanding of the domain for all stakeholders ensuring the quality of data exchange and transparency. The ontology restrictions are published in a separate artefact.</dcterms:description>
  </rdf:Description>
  <rdf:Description rdf:about="http://data.europa.eu/a4g/ontology#ful">
    <rdfs:label xml:lang="en">eProcurement Ontology Fulfilment - core</rdfs:label>
  </rdf:Description>
  <rdf:Description rdf:about="http://data.europa.eu/a4g/ontology#ful">
    <dcterms:created rdf:datatype="http://www.w3.org/2001/XMLSchema#date">2021-06-01</dcterms:created>
  </rdf:Description>
  <rdf:Description rdf:about="http://data.europa.eu/a4g/ontology#ful">
    <dcterms:issued rdf:datatype="http://www.w3.org/2001/XMLSchema#date">2024-11-12</dcterms:issued>
  </rdf:Description>
  <rdf:Description rdf:about="http://data.europa.eu/a4g/ontology#ful">
    <dcterms:license>Â© European Union, 2014. Unless otherwise noted, the reuse of the Ontology is authorised under the European Union Public Licence v1.2 (https://eupl.eu/).</dcterms:license>
  </rdf:Description>
  <rdf:Description rdf:about="http://data.europa.eu/a4g/ontology#ful">
    <dcterms:publisher>http://publications.europa.eu/resource/authority/corporate-body/PUBL</dcterms:publisher>
  </rdf:Description>
  <rdf:Description rdf:about="http://data.europa.eu/a4g/ontology#ful">
    <dcterms:title xml:lang="en">eProcurement Ontology Fulfilment - core</dcterms:title>
  </rdf:Description>
  <rdf:Description rdf:about="http://data.europa.eu/a4g/ontology#ful">
    <vann:preferredNamespacePrefix>epo</vann:preferredNamespacePrefix>
  </rdf:Description>
  <rdf:Description rdf:about="http://data.europa.eu/a4g/ontology#ful">
    <vann:preferredNamespaceUri>http://data.europa.eu/a4g/ontology#</vann:preferredNamespaceUri>
  </rdf:Description>
  <rdf:Description rdf:about="http://data.europa.eu/a4g/ontology#ful">
    <rdfs:comment>This version is automatically generated from eFulfilment.xml on 2024-11-12</rdfs:comment>
  </rdf:Description>
  <rdf:Description rdf:about="http://data.europa.eu/a4g/ontology#ful">
    <rdfs:seeAlso rdf:resource="https://docs.ted.europa.eu/home/index.html"/>
  </rdf:Description>
  <rdf:Description rdf:about="http://data.europa.eu/a4g/ontology#ful">
    <rdfs:seeAlso rdf:resource="https://github.com/OP-TED/ePO/releases"/>
  </rdf:Description>
  <rdf:Description rdf:about="http://data.europa.eu/a4g/ontology#ful">
    <rdfs:seeAlso rdf:resource="https://joinup.ec.europa.eu/collection/eprocurement/solution/eprocurement-ontology/about"/>
  </rdf:Description>
  <rdf:Description rdf:about="http://data.europa.eu/a4g/ontology#ful">
    <rdfs:seeAlso rdf:resource="https://op.europa.eu/en/web/eu-vocabularies/e-procurement"/>
  </rdf:Description>
  <rdf:Description rdf:about="http://data.europa.eu/a4g/ontology#ful">
    <owl:imports rdf:resource="http://data.europa.eu/a4g/ontology#cat"/>
  </rdf:Description>
  <rdf:Description rdf:about="http://data.europa.eu/a4g/ontology#ful">
    <owl:imports rdf:resource="http://data.europa.eu/a4g/ontology#core"/>
  </rdf:Description>
  <rdf:Description rdf:about="http://data.europa.eu/a4g/ontology#ful">
    <owl:imports rdf:resource="http://data.europa.eu/a4g/ontology#ord"/>
  </rdf:Description>
  <rdf:Description rdf:about="http://data.europa.eu/a4g/ontology#ful">
    <owl:imports rdf:resource="http://data.europa.eu/eli/ontology#"/>
  </rdf:Description>
  <rdf:Description rdf:about="http://data.europa.eu/a4g/ontology#ful">
    <owl:imports rdf:resource="http://data.europa.eu/m8g/"/>
  </rdf:Description>
  <rdf:Description rdf:about="http://data.europa.eu/a4g/ontology#ful">
    <owl:imports rdf:resource="http://iflastandards.info/ns/fr/frbr/frbroo/"/>
  </rdf:Description>
  <rdf:Description rdf:about="http://data.europa.eu/a4g/ontology#ful">
    <owl:imports rdf:resource="http://purl.org/dc/terms/"/>
  </rdf:Description>
  <rdf:Description rdf:about="http://data.europa.eu/a4g/ontology#ful">
    <owl:imports rdf:resource="http://purl.org/vocab/vann/"/>
  </rdf:Description>
  <rdf:Description rdf:about="http://data.europa.eu/a4g/ontology#ful">
    <owl:imports rdf:resource="http://www.w3.org/2004/02/skos/core"/>
  </rdf:Description>
  <rdf:Description rdf:about="http://data.europa.eu/a4g/ontology#ful">
    <owl:imports rdf:resource="http://www.w3.org/2006/time"/>
  </rdf:Description>
  <rdf:Description rdf:about="http://data.europa.eu/a4g/ontology#ful">
    <owl:imports rdf:resource="http://www.w3.org/ns/adms"/>
  </rdf:Description>
  <rdf:Description rdf:about="http://data.europa.eu/a4g/ontology#ful">
    <owl:imports rdf:resource="http://www.w3.org/ns/locn"/>
  </rdf:Description>
  <rdf:Description rdf:about="http://data.europa.eu/a4g/ontology#ful">
    <owl:imports rdf:resource="http://www.w3.org/ns/org#"/>
  </rdf:Description>
  <rdf:Description rdf:about="http://data.europa.eu/a4g/ontology#ful">
    <owl:imports rdf:resource="http://www.w3.org/ns/person"/>
  </rdf:Description>
  <rdf:Description rdf:about="http://data.europa.eu/a4g/ontology#ful">
    <owl:imports rdf:resource="http://xmlns.com/foaf/0.1/"/>
  </rdf:Description>
  <rdf:Description rdf:about="http://data.europa.eu/a4g/ontology#ful">
    <owl:incompatibleWith>3.1.0</owl:incompatibleWith>
  </rdf:Description>
  <rdf:Description rdf:about="http://data.europa.eu/a4g/ontology#ful">
    <owl:priorVersion>http://data.europa.eu/a4g/ontology#ful-4.1.1</owl:priorVersion>
  </rdf:Description>
  <rdf:Description rdf:about="http://data.europa.eu/a4g/ontology#ful">
    <owl:versionIRI rdf:resource="http://data.europa.eu/a4g/ontology#ful-4.2.0"/>
  </rdf:Description>
  <rdf:Description rdf:about="http://data.europa.eu/a4g/ontology#ful">
    <owl:versionInfo>4.2.0</owl:versionInfo>
  </rdf:Description>
  <rdf:Description rdf:about="http://data.europa.eu/a4g/ontology#Consignment">
    <rdf:type rdf:resource="http://www.w3.org/2002/07/owl#Class"/>
  </rdf:Description>
  <rdf:Description rdf:about="http://data.europa.eu/a4g/ontology#Consignment">
    <rdfs:isDefinedBy rdf:resource="http://data.europa.eu/a4g/ontology#ful"/>
  </rdf:Description>
  <rdf:Description rdf:about="http://data.europa.eu/a4g/ontology#Consignment">
    <skos:definition xml:lang="en">A batch of goods destined for or delivered to someone. Additional information: Consignment is a Transport Agreement between the Despatcher and the Consignee as to who and how the goods are despatched and received.</skos:definition>
  </rdf:Description>
  <rdf:Description rdf:about="http://data.europa.eu/a4g/ontology#Consignment">
    <skos:prefLabel xml:lang="en">Consignment</skos:prefLabel>
  </rdf:Description>
  <rdf:Description rdf:about="http://data.europa.eu/a4g/ontology#DespatchAdvice">
    <rdf:type rdf:resource="http://www.w3.org/2002/07/owl#Class"/>
  </rdf:Description>
  <rdf:Description rdf:about="http://data.europa.eu/a4g/ontology#DespatchAdvice">
    <rdfs:isDefinedBy rdf:resource="http://data.europa.eu/a4g/ontology#ful"/>
  </rdf:Description>
  <rdf:Description rdf:about="http://data.europa.eu/a4g/ontology#DespatchAdvice">
    <rdfs:subClassOf rdf:resource="http://data.europa.eu/a4g/ontology#PostAwardDocument"/>
  </rdf:Description>
  <rdf:Description rdf:about="http://data.europa.eu/a4g/ontology#DespatchAdvice">
    <skos:definition xml:lang="en">A document notifying the sending of goods or the execution of works or services.</skos:definition>
  </rdf:Description>
  <rdf:Description rdf:about="http://data.europa.eu/a4g/ontology#DespatchAdvice">
    <skos:prefLabel xml:lang="en">Despatch advice</skos:prefLabel>
  </rdf:Description>
  <rdf:Description rdf:about="http://data.europa.eu/a4g/ontology#DespatchLine">
    <rdf:type rdf:resource="http://www.w3.org/2002/07/owl#Class"/>
  </rdf:Description>
  <rdf:Description rdf:about="http://data.europa.eu/a4g/ontology#DespatchLine">
    <rdfs:isDefinedBy rdf:resource="http://data.europa.eu/a4g/ontology#ful"/>
  </rdf:Description>
  <rdf:Description rdf:about="http://data.europa.eu/a4g/ontology#DespatchLine">
    <rdfs:subClassOf rdf:resource="http://data.europa.eu/a4g/ontology#Line"/>
  </rdf:Description>
  <rdf:Description rdf:about="http://data.europa.eu/a4g/ontology#DespatchLine">
    <skos:definition xml:lang="en">Details concerning the fulfilment of an Order Line.</skos:definition>
  </rdf:Description>
  <rdf:Description rdf:about="http://data.europa.eu/a4g/ontology#DespatchLine">
    <skos:prefLabel xml:lang="en">Despatch line</skos:prefLabel>
  </rdf:Description>
  <rdf:Description rdf:about="http://data.europa.eu/a4g/ontology#Despatcher">
    <rdf:type rdf:resource="http://www.w3.org/2002/07/owl#Class"/>
  </rdf:Description>
  <rdf:Description rdf:about="http://data.europa.eu/a4g/ontology#Despatcher">
    <rdfs:isDefinedBy rdf:resource="http://data.europa.eu/a4g/ontology#ful"/>
  </rdf:Description>
  <rdf:Description rdf:about="http://data.europa.eu/a4g/ontology#Despatcher">
    <rdfs:subClassOf rdf:resource="http://data.europa.eu/a4g/ontology#OfferingParty"/>
  </rdf:Description>
  <rdf:Description rdf:about="http://data.europa.eu/a4g/ontology#Despatcher">
    <skos:definition xml:lang="en">The Role of an Agent who sends the goods or notifies of the service or works execution. Additional Information: The Role is carried out by the Supplier or on behalf of the Supplier. This Role is often referred to as the Despatch Party, Consignor or Deliverer.</skos:definition>
  </rdf:Description>
  <rdf:Description rdf:about="http://data.europa.eu/a4g/ontology#Despatcher">
    <skos:prefLabel xml:lang="en">Despatcher</skos:prefLabel>
  </rdf:Description>
  <rdf:Description rdf:about="http://data.europa.eu/a4g/ontology#FreightForwarder">
    <rdf:type rdf:resource="http://www.w3.org/2002/07/owl#Class"/>
  </rdf:Description>
  <rdf:Description rdf:about="http://data.europa.eu/a4g/ontology#FreightForwarder">
    <rdfs:isDefinedBy rdf:resource="http://data.europa.eu/a4g/ontology#ful"/>
  </rdf:Description>
  <rdf:Description rdf:about="http://data.europa.eu/a4g/ontology#FreightForwarder">
    <rdfs:subClassOf rdf:resource="http://data.europa.eu/a4g/ontology#AuxiliaryParty"/>
  </rdf:Description>
  <rdf:Description rdf:about="http://data.europa.eu/a4g/ontology#FreightForwarder">
    <skos:definition xml:lang="en">The Role of an Agent who organise the logistic operations need for a fulfilment.</skos:definition>
  </rdf:Description>
  <rdf:Description rdf:about="http://data.europa.eu/a4g/ontology#FreightForwarder">
    <skos:prefLabel xml:lang="en">Freight forwarder</skos:prefLabel>
  </rdf:Description>
  <rdf:Description rdf:about="http://data.europa.eu/a4g/ontology#GoodsItem">
    <rdf:type rdf:resource="http://www.w3.org/2002/07/owl#Class"/>
  </rdf:Description>
  <rdf:Description rdf:about="http://data.europa.eu/a4g/ontology#GoodsItem">
    <rdfs:isDefinedBy rdf:resource="http://data.europa.eu/a4g/ontology#ful"/>
  </rdf:Description>
  <rdf:Description rdf:about="http://data.europa.eu/a4g/ontology#GoodsItem">
    <skos:definition xml:lang="en">An Item including its initial packaging during transportation. Additional information: For example, the Item being bought is the computer. The weight of the computer is X. The weight of the Goods Item is the weight of the computer plus the weight of the initial packaging. During transportation you have for example trace ID which is applied to the GoodsItem, rather than on the Item itself. The declared statistical value can only apply once you have a GoodsItem.</skos:definition>
  </rdf:Description>
  <rdf:Description rdf:about="http://data.europa.eu/a4g/ontology#GoodsItem">
    <skos:prefLabel xml:lang="en">Goods item</skos:prefLabel>
  </rdf:Description>
  <rdf:Description rdf:about="http://data.europa.eu/a4g/ontology#NotificationReceiver">
    <rdf:type rdf:resource="http://www.w3.org/2002/07/owl#Class"/>
  </rdf:Description>
  <rdf:Description rdf:about="http://data.europa.eu/a4g/ontology#NotificationReceiver">
    <rdfs:isDefinedBy rdf:resource="http://data.europa.eu/a4g/ontology#ful"/>
  </rdf:Description>
  <rdf:Description rdf:about="http://data.europa.eu/a4g/ontology#NotificationReceiver">
    <rdfs:subClassOf rdf:resource="http://data.europa.eu/a4g/ontology#AuxiliaryParty"/>
  </rdf:Description>
  <rdf:Description rdf:about="http://data.europa.eu/a4g/ontology#NotificationReceiver">
    <skos:definition xml:lang="en">The Role of an Agent that is informed about the arrival of a Shipment at a destination. Additional information: This could be for example customs and excise.</skos:definition>
  </rdf:Description>
  <rdf:Description rdf:about="http://data.europa.eu/a4g/ontology#NotificationReceiver">
    <skos:prefLabel xml:lang="en">Notification receiver</skos:prefLabel>
  </rdf:Description>
  <rdf:Description rdf:about="http://data.europa.eu/a4g/ontology#Notifier">
    <rdf:type rdf:resource="http://www.w3.org/2002/07/owl#Class"/>
  </rdf:Description>
  <rdf:Description rdf:about="http://data.europa.eu/a4g/ontology#Notifier">
    <rdfs:isDefinedBy rdf:resource="http://data.europa.eu/a4g/ontology#ful"/>
  </rdf:Description>
  <rdf:Description rdf:about="http://data.europa.eu/a4g/ontology#Notifier">
    <rdfs:subClassOf rdf:resource="http://data.europa.eu/a4g/ontology#AuxiliaryParty"/>
  </rdf:Description>
  <rdf:Description rdf:about="http://data.europa.eu/a4g/ontology#Notifier">
    <skos:definition xml:lang="en">This class was wrongly named and has been replaced by epo-ful:NotificationReceiver. It will be removed in the next major release.</skos:definition>
  </rdf:Description>
  <rdf:Description rdf:about="http://data.europa.eu/a4g/ontology#Notifier">
    <skos:prefLabel xml:lang="en">Notifier</skos:prefLabel>
  </rdf:Description>
  <rdf:Description rdf:about="http://data.europa.eu/a4g/ontology#ReceiptAdvice">
    <rdf:type rdf:resource="http://www.w3.org/2002/07/owl#Class"/>
  </rdf:Description>
  <rdf:Description rdf:about="http://data.europa.eu/a4g/ontology#ReceiptAdvice">
    <rdfs:isDefinedBy rdf:resource="http://data.europa.eu/a4g/ontology#ful"/>
  </rdf:Description>
  <rdf:Description rdf:about="http://data.europa.eu/a4g/ontology#ReceiptAdvice">
    <rdfs:subClassOf rdf:resource="http://data.europa.eu/a4g/ontology#PostAwardDocument"/>
  </rdf:Description>
  <rdf:Description rdf:about="http://data.europa.eu/a4g/ontology#ReceiptAdvice">
    <skos:prefLabel xml:lang="en">Receipt advice</skos:prefLabel>
  </rdf:Description>
  <rdf:Description rdf:about="http://data.europa.eu/a4g/ontology#ReceiptAdviceLine">
    <rdf:type rdf:resource="http://www.w3.org/2002/07/owl#Class"/>
  </rdf:Description>
  <rdf:Description rdf:about="http://data.europa.eu/a4g/ontology#ReceiptAdviceLine">
    <rdfs:isDefinedBy rdf:resource="http://data.europa.eu/a4g/ontology#ful"/>
  </rdf:Description>
  <rdf:Description rdf:about="http://data.europa.eu/a4g/ontology#ReceiptAdviceLine">
    <rdfs:subClassOf rdf:resource="http://data.europa.eu/a4g/ontology#Line"/>
  </rdf:Description>
  <rdf:Description rdf:about="http://data.europa.eu/a4g/ontology#ReceiptAdviceLine">
    <skos:prefLabel xml:lang="en">Receipt advice line</skos:prefLabel>
  </rdf:Description>
  <rdf:Description rdf:about="http://data.europa.eu/a4g/ontology#RejectionAction">
    <rdf:type rdf:resource="http://www.w3.org/2002/07/owl#ObjectProperty"/>
  </rdf:Description>
  <rdf:Description rdf:about="http://data.europa.eu/a4g/ontology#RejectionAction">
    <rdfs:isDefinedBy rdf:resource="http://data.europa.eu/a4g/ontology#ful"/>
  </rdf:Description>
  <rdf:Description rdf:about="http://data.europa.eu/a4g/ontology#RejectionAction">
    <skos:prefLabel xml:lang="en">Rejection action</skos:prefLabel>
  </rdf:Description>
  <rdf:Description rdf:about="http://data.europa.eu/a4g/ontology#ShipmentAgreement">
    <rdf:type rdf:resource="http://www.w3.org/2002/07/owl#Class"/>
  </rdf:Description>
  <rdf:Description rdf:about="http://data.europa.eu/a4g/ontology#ShipmentAgreement">
    <rdfs:isDefinedBy rdf:resource="http://data.europa.eu/a4g/ontology#ful"/>
  </rdf:Description>
  <rdf:Description rdf:about="http://data.europa.eu/a4g/ontology#ShipmentAgreement">
    <skos:definition xml:lang="en">The commercial agreement between the Buyer and the Seller. Additional Information: The Shipment Agreement describes the items being shipped.</skos:definition>
  </rdf:Description>
  <rdf:Description rdf:about="http://data.europa.eu/a4g/ontology#ShipmentAgreement">
    <skos:prefLabel xml:lang="en">Shipment agreement</skos:prefLabel>
  </rdf:Description>
  <rdf:Description rdf:about="http://data.europa.eu/a4g/ontology#ShipmentInformation">
    <rdf:type rdf:resource="http://www.w3.org/2002/07/owl#Class"/>
  </rdf:Description>
  <rdf:Description rdf:about="http://data.europa.eu/a4g/ontology#ShipmentInformation">
    <rdfs:isDefinedBy rdf:resource="http://data.europa.eu/a4g/ontology#ful"/>
  </rdf:Description>
  <rdf:Description rdf:about="http://data.europa.eu/a4g/ontology#ShipmentInformation">
    <rdfs:subClassOf rdf:resource="http://data.europa.eu/a4g/ontology#InformationHub"/>
  </rdf:Description>
  <rdf:Description rdf:about="http://data.europa.eu/a4g/ontology#ShipmentInformation">
    <skos:definition xml:lang="en">Information about the transportation of an identifiable collection of Goods Items from the Despatcher to the Consignee.</skos:definition>
  </rdf:Description>
  <rdf:Description rdf:about="http://data.europa.eu/a4g/ontology#ShipmentInformation">
    <skos:prefLabel xml:lang="en">Shipment information</skos:prefLabel>
  </rdf:Description>
  <rdf:Description rdf:about="http://data.europa.eu/a4g/ontology#ShipmentStage">
    <rdf:type rdf:resource="http://www.w3.org/2002/07/owl#Class"/>
  </rdf:Description>
  <rdf:Description rdf:about="http://data.europa.eu/a4g/ontology#ShipmentStage">
    <rdfs:isDefinedBy rdf:resource="http://data.europa.eu/a4g/ontology#ful"/>
  </rdf:Description>
  <rdf:Description rdf:about="http://data.europa.eu/a4g/ontology#ShipmentStage">
    <skos:definition xml:lang="en">Part of the itinerary of a shipment. Additional information: In the context of fulfilment only the last part of the itinerary is taken into consideration.</skos:definition>
  </rdf:Description>
  <rdf:Description rdf:about="http://data.europa.eu/a4g/ontology#ShipmentStage">
    <skos:prefLabel xml:lang="en">Shipment stage</skos:prefLabel>
  </rdf:Description>
  <rdf:Description rdf:about="http://data.europa.eu/a4g/ontology#TemperatureSpecification">
    <rdf:type rdf:resource="http://www.w3.org/2002/07/owl#Class"/>
  </rdf:Description>
  <rdf:Description rdf:about="http://data.europa.eu/a4g/ontology#TemperatureSpecification">
    <rdfs:isDefinedBy rdf:resource="http://data.europa.eu/a4g/ontology#ful"/>
  </rdf:Description>
  <rdf:Description rdf:about="http://data.europa.eu/a4g/ontology#TemperatureSpecification">
    <skos:definition xml:lang="en">Description of the temperature requirements during shipment.</skos:definition>
  </rdf:Description>
  <rdf:Description rdf:about="http://data.europa.eu/a4g/ontology#TemperatureSpecification">
    <skos:prefLabel xml:lang="en">Temperature specification</skos:prefLabel>
  </rdf:Description>
  <rdf:Description rdf:about="http://data.europa.eu/a4g/ontology#TransportEquipment">
    <rdf:type rdf:resource="http://www.w3.org/2002/07/owl#Class"/>
  </rdf:Description>
  <rdf:Description rdf:about="http://data.europa.eu/a4g/ontology#TransportEquipment">
    <rdfs:isDefinedBy rdf:resource="http://data.europa.eu/a4g/ontology#ful"/>
  </rdf:Description>
  <rdf:Description rdf:about="http://data.europa.eu/a4g/ontology#TransportEquipment">
    <skos:definition xml:lang="en">Description of the apparatus used during transportation. Additional information: The equipment may be a container, a trailer, means of assistance to load or unload the Goods Items.</skos:definition>
  </rdf:Description>
  <rdf:Description rdf:about="http://data.europa.eu/a4g/ontology#TransportEquipment">
    <skos:prefLabel xml:lang="en">Transport equipment</skos:prefLabel>
  </rdf:Description>
  <rdf:Description rdf:about="http://data.europa.eu/a4g/ontology#TransportEquipmentSeal">
    <rdf:type rdf:resource="http://www.w3.org/2002/07/owl#Class"/>
  </rdf:Description>
  <rdf:Description rdf:about="http://data.europa.eu/a4g/ontology#TransportEquipmentSeal">
    <rdfs:isDefinedBy rdf:resource="http://data.europa.eu/a4g/ontology#ful"/>
  </rdf:Description>
  <rdf:Description rdf:about="http://data.europa.eu/a4g/ontology#TransportEquipmentSeal">
    <skos:definition xml:lang="en">Means used to ensure that the Transport Equipment is not tampered during transportation.</skos:definition>
  </rdf:Description>
  <rdf:Description rdf:about="http://data.europa.eu/a4g/ontology#TransportEquipmentSeal">
    <skos:prefLabel xml:lang="en">Transport equipment seal</skos:prefLabel>
  </rdf:Description>
  <rdf:Description rdf:about="http://data.europa.eu/a4g/ontology#TransportHandlingUnit">
    <rdf:type rdf:resource="http://www.w3.org/2002/07/owl#Class"/>
  </rdf:Description>
  <rdf:Description rdf:about="http://data.europa.eu/a4g/ontology#TransportHandlingUnit">
    <rdfs:isDefinedBy rdf:resource="http://data.europa.eu/a4g/ontology#ful"/>
  </rdf:Description>
  <rdf:Description rdf:about="http://data.europa.eu/a4g/ontology#TransportHandlingUnit">
    <rdfs:subClassOf rdf:resource="http://data.europa.eu/a4g/ontology#Package"/>
  </rdf:Description>
  <rdf:Description rdf:about="http://data.europa.eu/a4g/ontology#TransportHandlingUnit">
    <skos:definition xml:lang="en">The outermost Package that the Carrier is handling.</skos:definition>
  </rdf:Description>
  <rdf:Description rdf:about="http://data.europa.eu/a4g/ontology#TransportHandlingUnit">
    <skos:prefLabel xml:lang="en">Transport handling unit</skos:prefLabel>
  </rdf:Description>
  <rdf:Description rdf:about="http://data.europa.eu/a4g/ontology#Package">
    <rdf:type rdf:resource="http://www.w3.org/2002/07/owl#Class"/>
  </rdf:Description>
  <rdf:Description rdf:about="http://data.europa.eu/a4g/ontology#Package">
    <rdfs:isDefinedBy rdf:resource="http://data.europa.eu/a4g/ontology#ful"/>
  </rdf:Description>
  <rdf:Description rdf:about="http://data.europa.eu/a4g/ontology#Package">
    <rdfs:subClassOf rdf:resource="http://data.europa.eu/a4g/ontology#AbstractContainer"/>
  </rdf:Description>
  <rdf:Description rdf:about="http://data.europa.eu/a4g/ontology#Package">
    <skos:definition xml:lang="en">Container used for transportation.</skos:definition>
  </rdf:Description>
  <rdf:Description rdf:about="http://data.europa.eu/a4g/ontology#Package">
    <skos:prefLabel xml:lang="en">Package</skos:prefLabel>
  </rdf:Description>
  <rdf:Description rdf:about="http://data.europa.eu/a4g/ontology#AbstractContainer">
    <rdf:type rdf:resource="http://www.w3.org/2002/07/owl#Class"/>
  </rdf:Description>
  <rdf:Description rdf:about="http://data.europa.eu/a4g/ontology#AbstractContainer">
    <rdfs:isDefinedBy rdf:resource="http://data.europa.eu/a4g/ontology#ful"/>
  </rdf:Description>
  <rdf:Description rdf:about="http://data.europa.eu/a4g/ontology#AbstractContainer">
    <skos:definition xml:lang="en">Gathering class for Packages and Transport Handling Units.</skos:definition>
  </rdf:Description>
  <rdf:Description rdf:about="http://data.europa.eu/a4g/ontology#AbstractContainer">
    <skos:prefLabel xml:lang="en">Abstract container</skos:prefLabel>
  </rdf:Description>
  <rdf:Description rdf:about="http://data.europa.eu/a4g/ontology#TransportMeans">
    <rdf:type rdf:resource="http://www.w3.org/2002/07/owl#Class"/>
  </rdf:Description>
  <rdf:Description rdf:about="http://data.europa.eu/a4g/ontology#TransportMeans">
    <rdfs:isDefinedBy rdf:resource="http://data.europa.eu/a4g/ontology#ful"/>
  </rdf:Description>
  <rdf:Description rdf:about="http://data.europa.eu/a4g/ontology#TransportMeans">
    <skos:definition xml:lang="en">Description of a particular vehicle or vessel used for the conveyance of goods or persons.</skos:definition>
  </rdf:Description>
  <rdf:Description rdf:about="http://data.europa.eu/a4g/ontology#TransportMeans">
    <skos:prefLabel xml:lang="en">Transport means</skos:prefLabel>
  </rdf:Description>
  <rdf:Description rdf:about="http://data.europa.eu/a4g/ontology#TransportMeansOperator">
    <rdf:type rdf:resource="http://www.w3.org/2002/07/owl#Class"/>
  </rdf:Description>
  <rdf:Description rdf:about="http://data.europa.eu/a4g/ontology#TransportMeansOperator">
    <rdfs:isDefinedBy rdf:resource="http://data.europa.eu/a4g/ontology#ful"/>
  </rdf:Description>
  <rdf:Description rdf:about="http://data.europa.eu/a4g/ontology#TransportMeansOperator">
    <rdfs:subClassOf rdf:resource="http://data.europa.eu/a4g/ontology#AuxiliaryParty"/>
  </rdf:Description>
  <rdf:Description rdf:about="http://data.europa.eu/a4g/ontology#TransportMeansOperator">
    <skos:definition xml:lang="en">The Role of an Agent who is responsible for controlling the Transport Means.</skos:definition>
  </rdf:Description>
  <rdf:Description rdf:about="http://data.europa.eu/a4g/ontology#TransportMeansOperator">
    <skos:prefLabel xml:lang="en">Transport means operator</skos:prefLabel>
  </rdf:Description>
  <rdf:Description rdf:about="http://data.europa.eu/a4g/ontology#agreedByBuyer">
    <rdf:type rdf:resource="http://www.w3.org/2002/07/owl#ObjectProperty"/>
  </rdf:Description>
  <rdf:Description rdf:about="http://data.europa.eu/a4g/ontology#agreedByBuyer">
    <rdfs:isDefinedBy rdf:resource="http://data.europa.eu/a4g/ontology#ful"/>
  </rdf:Description>
  <rdf:Description rdf:about="http://data.europa.eu/a4g/ontology#agreedByBuyer">
    <skos:definition xml:lang="en">Accepted by Buyer. (epo-ful:ShipmentAgreement -&gt; epo:Buyer (+epo-ful:agreedByBuyer))</skos:definition>
  </rdf:Description>
  <rdf:Description rdf:about="http://data.europa.eu/a4g/ontology#agreedByBuyer">
    <skos:prefLabel xml:lang="en">Agreed by buyer</skos:prefLabel>
  </rdf:Description>
  <rdf:Description rdf:about="http://data.europa.eu/a4g/ontology#agreedByBuyer">
    <skos:historyNote xml:lang="en">WG Approval 10/06/2024</skos:historyNote>
  </rdf:Description>
  <rdf:Description rdf:about="http://data.europa.eu/a4g/ontology#agreedBySeller">
    <rdf:type rdf:resource="http://www.w3.org/2002/07/owl#ObjectProperty"/>
  </rdf:Description>
  <rdf:Description rdf:about="http://data.europa.eu/a4g/ontology#agreedBySeller">
    <rdfs:isDefinedBy rdf:resource="http://data.europa.eu/a4g/ontology#ful"/>
  </rdf:Description>
  <rdf:Description rdf:about="http://data.europa.eu/a4g/ontology#agreedBySeller">
    <skos:definition xml:lang="en">Accepted by Seller. (epo-ful:ShipmentAgreement -&gt; epo-ord:Seller (+epo-ful:agreedBySeller))</skos:definition>
  </rdf:Description>
  <rdf:Description rdf:about="http://data.europa.eu/a4g/ontology#agreedBySeller">
    <skos:prefLabel xml:lang="en">Agreed by seller</skos:prefLabel>
  </rdf:Description>
  <rdf:Description rdf:about="http://data.europa.eu/a4g/ontology#agreedBySeller">
    <skos:historyNote xml:lang="en">WG Approval 10/06/2024</skos:historyNote>
  </rdf:Description>
  <rdf:Description rdf:about="http://data.europa.eu/a4g/ontology#comprisesDespatchLine">
    <rdf:type rdf:resource="http://www.w3.org/2002/07/owl#ObjectProperty"/>
  </rdf:Description>
  <rdf:Description rdf:about="http://data.europa.eu/a4g/ontology#comprisesDespatchLine">
    <rdfs:isDefinedBy rdf:resource="http://data.europa.eu/a4g/ontology#ful"/>
  </rdf:Description>
  <rdf:Description rdf:about="http://data.europa.eu/a4g/ontology#comprisesDespatchLine">
    <skos:definition xml:lang="en">Incorporates Despatch Line. (epo-ful:DespatchAdvice -&gt; epo-ful:DespatchLine (+epo-ful:comprisesDespatchLine))</skos:definition>
  </rdf:Description>
  <rdf:Description rdf:about="http://data.europa.eu/a4g/ontology#comprisesDespatchLine">
    <skos:prefLabel xml:lang="en">Comprises despatch line</skos:prefLabel>
  </rdf:Description>
  <rdf:Description rdf:about="http://data.europa.eu/a4g/ontology#comprisesDespatchLine">
    <skos:historyNote xml:lang="en">WG Approval 10/06/2024</skos:historyNote>
  </rdf:Description>
  <rdf:Description rdf:about="http://data.europa.eu/a4g/ontology#comprisesReceiptAdviceLine">
    <rdf:type rdf:resource="http://www.w3.org/2002/07/owl#ObjectProperty"/>
  </rdf:Description>
  <rdf:Description rdf:about="http://data.europa.eu/a4g/ontology#comprisesReceiptAdviceLine">
    <rdfs:isDefinedBy rdf:resource="http://data.europa.eu/a4g/ontology#ful"/>
  </rdf:Description>
  <rdf:Description rdf:about="http://data.europa.eu/a4g/ontology#comprisesReceiptAdviceLine">
    <skos:prefLabel xml:lang="en">Comprises receipt advice line</skos:prefLabel>
  </rdf:Description>
  <rdf:Description rdf:about="http://data.europa.eu/a4g/ontology#containsGoodsItem">
    <rdf:type rdf:resource="http://www.w3.org/2002/07/owl#ObjectProperty"/>
  </rdf:Description>
  <rdf:Description rdf:about="http://data.europa.eu/a4g/ontology#containsGoodsItem">
    <rdfs:isDefinedBy rdf:resource="http://data.europa.eu/a4g/ontology#ful"/>
  </rdf:Description>
  <rdf:Description rdf:about="http://data.europa.eu/a4g/ontology#containsGoodsItem">
    <skos:definition xml:lang="en">Includes Goods Item. (epo-ful:Package -&gt; epo-ful:GoodsItem (+epo-ful:containsGoodsItem))</skos:definition>
  </rdf:Description>
  <rdf:Description rdf:about="http://data.europa.eu/a4g/ontology#containsGoodsItem">
    <skos:prefLabel xml:lang="en">Contains goods item</skos:prefLabel>
  </rdf:Description>
  <rdf:Description rdf:about="http://data.europa.eu/a4g/ontology#containsGoodsItem">
    <skos:historyNote xml:lang="en">WG Approval 10/06/2024</skos:historyNote>
  </rdf:Description>
  <rdf:Description rdf:about="http://data.europa.eu/a4g/ontology#containsPackage">
    <rdf:type rdf:resource="http://www.w3.org/2002/07/owl#ObjectProperty"/>
  </rdf:Description>
  <rdf:Description rdf:about="http://data.europa.eu/a4g/ontology#containsPackage">
    <rdfs:isDefinedBy rdf:resource="http://data.europa.eu/a4g/ontology#ful"/>
  </rdf:Description>
  <rdf:Description rdf:about="http://data.europa.eu/a4g/ontology#containsPackage">
    <skos:definition xml:lang="en">Includes Package. (epo-ful:Package -&gt; epo-ful:Package (+epo-ful:containsPackage))</skos:definition>
  </rdf:Description>
  <rdf:Description rdf:about="http://data.europa.eu/a4g/ontology#containsPackage">
    <skos:prefLabel xml:lang="en">Contains package</skos:prefLabel>
  </rdf:Description>
  <rdf:Description rdf:about="http://data.europa.eu/a4g/ontology#containsPackage">
    <skos:historyNote xml:lang="en">WG Approval 10/06/2024</skos:historyNote>
  </rdf:Description>
  <rdf:Description rdf:about="http://data.europa.eu/a4g/ontology#containsTransportHandlingUnit">
    <rdf:type rdf:resource="http://www.w3.org/2002/07/owl#ObjectProperty"/>
  </rdf:Description>
  <rdf:Description rdf:about="http://data.europa.eu/a4g/ontology#containsTransportHandlingUnit">
    <rdfs:isDefinedBy rdf:resource="http://data.europa.eu/a4g/ontology#ful"/>
  </rdf:Description>
  <rdf:Description rdf:about="http://data.europa.eu/a4g/ontology#containsTransportHandlingUnit">
    <skos:definition xml:lang="en">Includes Transport Handling Unit. (epo-ful:Consignment -&gt; epo-ful:TransportHandlingUnit (+epo-ful:containsTransportHandlingUnit))</skos:definition>
  </rdf:Description>
  <rdf:Description rdf:about="http://data.europa.eu/a4g/ontology#containsTransportHandlingUnit">
    <skos:prefLabel xml:lang="en">Contains transport handling unit</skos:prefLabel>
  </rdf:Description>
  <rdf:Description rdf:about="http://data.europa.eu/a4g/ontology#containsTransportHandlingUnit">
    <skos:historyNote xml:lang="en">WG Approval 10/06/2024</skos:historyNote>
  </rdf:Description>
  <rdf:Description rdf:about="http://data.europa.eu/a4g/ontology#despatchDate">
    <rdf:type rdf:resource="http://www.w3.org/2002/07/owl#DatatypeProperty"/>
  </rdf:Description>
  <rdf:Description rdf:about="http://data.europa.eu/a4g/ontology#despatchDate">
    <rdfs:isDefinedBy rdf:resource="http://data.europa.eu/a4g/ontology#ful"/>
  </rdf:Description>
  <rdf:Description rdf:about="http://data.europa.eu/a4g/ontology#despatchDate">
    <skos:definition xml:lang="en">The date of sending of goods or the execution of works or services. (epo-ful:ShipmentInformation)</skos:definition>
  </rdf:Description>
  <rdf:Description rdf:about="http://data.europa.eu/a4g/ontology#despatchDate">
    <skos:prefLabel xml:lang="en">Despatch date</skos:prefLabel>
  </rdf:Description>
  <rdf:Description rdf:about="http://data.europa.eu/a4g/ontology#despatchDate">
    <skos:historyNote xml:lang="en">WG Approval 05/06/2024</skos:historyNote>
  </rdf:Description>
  <rdf:Description rdf:about="http://data.europa.eu/a4g/ontology#foreseesPackage">
    <rdf:type rdf:resource="http://www.w3.org/2002/07/owl#ObjectProperty"/>
  </rdf:Description>
  <rdf:Description rdf:about="http://data.europa.eu/a4g/ontology#foreseesPackage">
    <rdfs:isDefinedBy rdf:resource="http://data.europa.eu/a4g/ontology#ful"/>
  </rdf:Description>
  <rdf:Description rdf:about="http://data.europa.eu/a4g/ontology#foreseesPackage">
    <skos:prefLabel xml:lang="en">Foresees package</skos:prefLabel>
  </rdf:Description>
  <rdf:Description rdf:about="http://data.europa.eu/a4g/ontology#hasAllowanceChargeReason">
    <rdf:type rdf:resource="http://www.w3.org/2002/07/owl#ObjectProperty"/>
  </rdf:Description>
  <rdf:Description rdf:about="http://data.europa.eu/a4g/ontology#hasAllowanceChargeReason">
    <rdfs:isDefinedBy rdf:resource="http://data.europa.eu/a4g/ontology#ful"/>
  </rdf:Description>
  <rdf:Description rdf:about="http://data.europa.eu/a4g/ontology#hasAllowanceChargeReason">
    <skos:definition xml:lang="en">The justification for using the Allowance or the Charge. (epo-ord:AllowanceChargeInformation -&gt; at-voc-new:allowance-charge-reason (+epo-ful:hasAllowanceChargeReason))</skos:definition>
  </rdf:Description>
  <rdf:Description rdf:about="http://data.europa.eu/a4g/ontology#hasAllowanceChargeReason">
    <skos:prefLabel xml:lang="en">Has allowance charge reason</skos:prefLabel>
  </rdf:Description>
  <rdf:Description rdf:about="http://data.europa.eu/a4g/ontology#hasArrivalShipmentInformation">
    <rdf:type rdf:resource="http://www.w3.org/2002/07/owl#ObjectProperty"/>
  </rdf:Description>
  <rdf:Description rdf:about="http://data.europa.eu/a4g/ontology#hasArrivalShipmentInformation">
    <rdfs:isDefinedBy rdf:resource="http://data.europa.eu/a4g/ontology#ful"/>
  </rdf:Description>
  <rdf:Description rdf:about="http://data.europa.eu/a4g/ontology#hasArrivalShipmentInformation">
    <skos:definition xml:lang="en">Shipment Information about the destination of the Consignment for a given Shipment Stage. (epo-ful:ShipmentStage -&gt; epo-ful:ShipmentInformation (+epo:hasArrivalShipmentInformation))</skos:definition>
  </rdf:Description>
  <rdf:Description rdf:about="http://data.europa.eu/a4g/ontology#hasArrivalShipmentInformation">
    <skos:prefLabel xml:lang="en">Has arrival shipment information</skos:prefLabel>
  </rdf:Description>
  <rdf:Description rdf:about="http://data.europa.eu/a4g/ontology#hasArrivalShipmentInformation">
    <skos:historyNote xml:lang="en">WG Approval 18/06/2024</skos:historyNote>
  </rdf:Description>
  <rdf:Description rdf:about="http://data.europa.eu/a4g/ontology#hasAssociatedDocument">
    <rdf:type rdf:resource="http://www.w3.org/2002/07/owl#ObjectProperty"/>
  </rdf:Description>
  <rdf:Description rdf:about="http://data.europa.eu/a4g/ontology#hasAssociatedDocument">
    <rdfs:isDefinedBy rdf:resource="http://data.europa.eu/a4g/ontology#ful"/>
  </rdf:Description>
  <rdf:Description rdf:about="http://data.europa.eu/a4g/ontology#hasAssociatedDocument">
    <skos:definition xml:lang="en">Is related to a Document. (epo-ful:DespatchLine -&gt; epo:Document (+epo-ful:hasAssociatedDocument)) Is related to a Document. (epo-ful:DespatchAdvice -&gt; epo:Document (+epo-ful:hasAssociatedDocument))</skos:definition>
  </rdf:Description>
  <rdf:Description rdf:about="http://data.europa.eu/a4g/ontology#hasAssociatedDocument">
    <skos:prefLabel xml:lang="en">Has associated document</skos:prefLabel>
  </rdf:Description>
  <rdf:Description rdf:about="http://data.europa.eu/a4g/ontology#hasAssociatedDocument">
    <skos:historyNote xml:lang="en">WG Approval 06/10/2024</skos:historyNote>
  </rdf:Description>
  <rdf:Description rdf:about="http://data.europa.eu/a4g/ontology#hasCarrierConsignmentID">
    <rdf:type rdf:resource="http://www.w3.org/2002/07/owl#ObjectProperty"/>
  </rdf:Description>
  <rdf:Description rdf:about="http://data.europa.eu/a4g/ontology#hasCarrierConsignmentID">
    <rdfs:isDefinedBy rdf:resource="http://data.europa.eu/a4g/ontology#ful"/>
  </rdf:Description>
  <rdf:Description rdf:about="http://data.europa.eu/a4g/ontology#hasCarrierConsignmentID">
    <skos:definition xml:lang="en">The identifier of the the Consignment given by the Carrier. (epo-ful:Consignment -&gt; adms:Identifier (+epo-ful:hasCarrierConsignmentID))</skos:definition>
  </rdf:Description>
  <rdf:Description rdf:about="http://data.europa.eu/a4g/ontology#hasCarrierConsignmentID">
    <skos:prefLabel xml:lang="en">Has carrier consignment i d</skos:prefLabel>
  </rdf:Description>
  <rdf:Description rdf:about="http://data.europa.eu/a4g/ontology#hasCarrierConsignmentID">
    <skos:historyNote xml:lang="en">WG Approval 10/06/2024</skos:historyNote>
  </rdf:Description>
  <rdf:Description rdf:about="http://data.europa.eu/a4g/ontology#hasCarrierServiceInstruction">
    <rdf:type rdf:resource="http://www.w3.org/2002/07/owl#DatatypeProperty"/>
  </rdf:Description>
  <rdf:Description rdf:about="http://data.europa.eu/a4g/ontology#hasCarrierServiceInstruction">
    <rdfs:isDefinedBy rdf:resource="http://data.europa.eu/a4g/ontology#ful"/>
  </rdf:Description>
  <rdf:Description rdf:about="http://data.europa.eu/a4g/ontology#hasCarrierServiceInstruction">
    <skos:definition xml:lang="en">This attribute should be removed in the next major release. (epo-ful:Consignment)</skos:definition>
  </rdf:Description>
  <rdf:Description rdf:about="http://data.europa.eu/a4g/ontology#hasCarrierServiceInstruction">
    <skos:prefLabel xml:lang="en">Has carrier service instruction</skos:prefLabel>
  </rdf:Description>
  <rdf:Description rdf:about="http://data.europa.eu/a4g/ontology#hasChargeableWeight">
    <rdf:type rdf:resource="http://www.w3.org/2002/07/owl#ObjectProperty"/>
  </rdf:Description>
  <rdf:Description rdf:about="http://data.europa.eu/a4g/ontology#hasChargeableWeight">
    <rdfs:isDefinedBy rdf:resource="http://data.europa.eu/a4g/ontology#ful"/>
  </rdf:Description>
  <rdf:Description rdf:about="http://data.europa.eu/a4g/ontology#hasChargeableWeight">
    <skos:definition xml:lang="en">The (epo-ful:Consignment -&gt; epo:Quantity (+epo-ful:hasChargeableWeight))</skos:definition>
  </rdf:Description>
  <rdf:Description rdf:about="http://data.europa.eu/a4g/ontology#hasChargeableWeight">
    <skos:prefLabel xml:lang="en">Has chargeable weight</skos:prefLabel>
  </rdf:Description>
  <rdf:Description rdf:about="http://data.europa.eu/a4g/ontology#hasConsigneeConsignmentID">
    <rdf:type rdf:resource="http://www.w3.org/2002/07/owl#ObjectProperty"/>
  </rdf:Description>
  <rdf:Description rdf:about="http://data.europa.eu/a4g/ontology#hasConsigneeConsignmentID">
    <rdfs:isDefinedBy rdf:resource="http://data.europa.eu/a4g/ontology#ful"/>
  </rdf:Description>
  <rdf:Description rdf:about="http://data.europa.eu/a4g/ontology#hasConsigneeConsignmentID">
    <skos:definition xml:lang="en">The identifier of the the Consignment given by the Consignee. (epo-ful:Consignment -&gt; adms:Identifier (+epo-ful:hasConsigneeConsignmentID))</skos:definition>
  </rdf:Description>
  <rdf:Description rdf:about="http://data.europa.eu/a4g/ontology#hasConsigneeConsignmentID">
    <skos:prefLabel xml:lang="en">Has consignee consignment i d</skos:prefLabel>
  </rdf:Description>
  <rdf:Description rdf:about="http://data.europa.eu/a4g/ontology#hasConsigneeConsignmentID">
    <skos:historyNote xml:lang="en">WG Approval 10/06/2024</skos:historyNote>
  </rdf:Description>
  <rdf:Description rdf:about="http://data.europa.eu/a4g/ontology#hasConsignmentDeclaredStatisticsValue">
    <rdf:type rdf:resource="http://www.w3.org/2002/07/owl#ObjectProperty"/>
  </rdf:Description>
  <rdf:Description rdf:about="http://data.europa.eu/a4g/ontology#hasConsignmentDeclaredStatisticsValue">
    <rdfs:isDefinedBy rdf:resource="http://data.europa.eu/a4g/ontology#ful"/>
  </rdf:Description>
  <rdf:Description rdf:about="http://data.europa.eu/a4g/ontology#hasConsignmentDeclaredStatisticsValue">
    <skos:prefLabel xml:lang="en">Has consignment declared statistics value</skos:prefLabel>
  </rdf:Description>
  <rdf:Description rdf:about="http://data.europa.eu/a4g/ontology#hasConsignmentFreeOnBoardValue">
    <rdf:type rdf:resource="http://www.w3.org/2002/07/owl#ObjectProperty"/>
  </rdf:Description>
  <rdf:Description rdf:about="http://data.europa.eu/a4g/ontology#hasConsignmentFreeOnBoardValue">
    <rdfs:isDefinedBy rdf:resource="http://data.europa.eu/a4g/ontology#ful"/>
  </rdf:Description>
  <rdf:Description rdf:about="http://data.europa.eu/a4g/ontology#hasConsignmentFreeOnBoardValue">
    <skos:definition xml:lang="en">The Monetary Value of the Consignment when there is a transfer of liability for goods, damaged or destroyed, during shipping. at the exporter's customs frontier. (epo-ful:Consignment -&gt; epo:MonetaryValue (+epo-ful:hasConsignmentFreeOnBoardValue))</skos:definition>
  </rdf:Description>
  <rdf:Description rdf:about="http://data.europa.eu/a4g/ontology#hasConsignmentFreeOnBoardValue">
    <skos:prefLabel xml:lang="en">Has consignment free on board value</skos:prefLabel>
  </rdf:Description>
  <rdf:Description rdf:about="http://data.europa.eu/a4g/ontology#hasConsignmentInvoiceValue">
    <rdf:type rdf:resource="http://www.w3.org/2002/07/owl#ObjectProperty"/>
  </rdf:Description>
  <rdf:Description rdf:about="http://data.europa.eu/a4g/ontology#hasConsignmentInvoiceValue">
    <rdfs:isDefinedBy rdf:resource="http://data.europa.eu/a4g/ontology#ful"/>
  </rdf:Description>
  <rdf:Description rdf:about="http://data.europa.eu/a4g/ontology#hasConsignmentInvoiceValue">
    <skos:definition xml:lang="en">Declared amount of the Consignment. Additional Information: This is a logistics information needed for logistics, security measures, customs check, etc. (epo-ful:Consignment -&gt; epo:MonetaryValue (+epo-ful:hasConsignmentInvoiceValue))</skos:definition>
  </rdf:Description>
  <rdf:Description rdf:about="http://data.europa.eu/a4g/ontology#hasConsignmentInvoiceValue">
    <skos:prefLabel xml:lang="en">Has consignment invoice value</skos:prefLabel>
  </rdf:Description>
  <rdf:Description rdf:about="http://data.europa.eu/a4g/ontology#hasConsignmentInvoiceValue">
    <skos:historyNote xml:lang="en">WG Approval 18/06/2024</skos:historyNote>
  </rdf:Description>
  <rdf:Description rdf:about="http://data.europa.eu/a4g/ontology#hasDeclaredStatisticalValue">
    <rdf:type rdf:resource="http://www.w3.org/2002/07/owl#ObjectProperty"/>
  </rdf:Description>
  <rdf:Description rdf:about="http://data.europa.eu/a4g/ontology#hasDeclaredStatisticalValue">
    <rdfs:isDefinedBy rdf:resource="http://data.europa.eu/a4g/ontology#ful"/>
  </rdf:Description>
  <rdf:Description rdf:about="http://data.europa.eu/a4g/ontology#hasDeclaredStatisticalValue">
    <skos:definition xml:lang="en">The Monetary Value declared for statistical purposes. (epo-ful:Consignment -&gt; epo:MonetaryValue (+epo-ful:hasDeclaredStatisticalValue))</skos:definition>
  </rdf:Description>
  <rdf:Description rdf:about="http://data.europa.eu/a4g/ontology#hasDeclaredStatisticalValue">
    <skos:prefLabel xml:lang="en">Has declared statistical value</skos:prefLabel>
  </rdf:Description>
  <rdf:Description rdf:about="http://data.europa.eu/a4g/ontology#hasDeclaredStatisticalValue">
    <skos:historyNote xml:lang="en">WG Approval 10/06/2024</skos:historyNote>
  </rdf:Description>
  <rdf:Description rdf:about="http://data.europa.eu/a4g/ontology#hasDeliveryInstruction">
    <rdf:type rdf:resource="http://www.w3.org/2002/07/owl#DatatypeProperty"/>
  </rdf:Description>
  <rdf:Description rdf:about="http://data.europa.eu/a4g/ontology#hasDeliveryInstruction">
    <rdfs:isDefinedBy rdf:resource="http://data.europa.eu/a4g/ontology#ful"/>
  </rdf:Description>
  <rdf:Description rdf:about="http://data.europa.eu/a4g/ontology#hasDeliveryInstruction">
    <skos:definition xml:lang="en">This attribute should be removed in the next major release. (epo-ful:Consignment)</skos:definition>
  </rdf:Description>
  <rdf:Description rdf:about="http://data.europa.eu/a4g/ontology#hasDeliveryInstruction">
    <skos:prefLabel xml:lang="en">Has delivery instruction</skos:prefLabel>
  </rdf:Description>
  <rdf:Description rdf:about="http://data.europa.eu/a4g/ontology#hasDepartureShipmentInformation">
    <rdf:type rdf:resource="http://www.w3.org/2002/07/owl#ObjectProperty"/>
  </rdf:Description>
  <rdf:Description rdf:about="http://data.europa.eu/a4g/ontology#hasDepartureShipmentInformation">
    <rdfs:isDefinedBy rdf:resource="http://data.europa.eu/a4g/ontology#ful"/>
  </rdf:Description>
  <rdf:Description rdf:about="http://data.europa.eu/a4g/ontology#hasDepartureShipmentInformation">
    <skos:definition xml:lang="en">Shipment Information about the place the Consignment is leaving from in a given Shipment Stage. (epo-ful:ShipmentStage -&gt; epo-ful:ShipmentInformation (+epo-ful:hasDepartureShipmentInformation))</skos:definition>
  </rdf:Description>
  <rdf:Description rdf:about="http://data.europa.eu/a4g/ontology#hasDepartureShipmentInformation">
    <skos:prefLabel xml:lang="en">Has departure shipment information</skos:prefLabel>
  </rdf:Description>
  <rdf:Description rdf:about="http://data.europa.eu/a4g/ontology#hasDepartureShipmentInformation">
    <skos:historyNote xml:lang="en">WG Approval 18/06/2024</skos:historyNote>
  </rdf:Description>
  <rdf:Description rdf:about="http://data.europa.eu/a4g/ontology#hasDespatchAdviceType">
    <rdf:type rdf:resource="http://www.w3.org/2002/07/owl#ObjectProperty"/>
  </rdf:Description>
  <rdf:Description rdf:about="http://data.europa.eu/a4g/ontology#hasDespatchAdviceType">
    <rdfs:isDefinedBy rdf:resource="http://data.europa.eu/a4g/ontology#ful"/>
  </rdf:Description>
  <rdf:Description rdf:about="http://data.europa.eu/a4g/ontology#hasDespatchAdviceType">
    <skos:definition xml:lang="en">Classification of a Despatch Advice. (epo-ful:DespatchAdvice -&gt; at-voc-new:despatch-advice-type (+epo-ful:hasDespatchAdviceType))</skos:definition>
  </rdf:Description>
  <rdf:Description rdf:about="http://data.europa.eu/a4g/ontology#hasDespatchAdviceType">
    <skos:prefLabel xml:lang="en">Has despatch advice type</skos:prefLabel>
  </rdf:Description>
  <rdf:Description rdf:about="http://data.europa.eu/a4g/ontology#hasDespatchPeriod">
    <rdf:type rdf:resource="http://www.w3.org/2002/07/owl#ObjectProperty"/>
  </rdf:Description>
  <rdf:Description rdf:about="http://data.europa.eu/a4g/ontology#hasDespatchPeriod">
    <rdfs:isDefinedBy rdf:resource="http://data.europa.eu/a4g/ontology#ful"/>
  </rdf:Description>
  <rdf:Description rdf:about="http://data.europa.eu/a4g/ontology#hasDespatchPeriod">
    <skos:definition xml:lang="en">The time period when the Despatcher picks-up the Goods Items to be delivered. (epo-ful:ShipmentInformation -&gt; epo:Period (+epo-ful:hasDespatchPeriod))</skos:definition>
  </rdf:Description>
  <rdf:Description rdf:about="http://data.europa.eu/a4g/ontology#hasDespatchPeriod">
    <skos:prefLabel xml:lang="en">Has despatch period</skos:prefLabel>
  </rdf:Description>
  <rdf:Description rdf:about="http://data.europa.eu/a4g/ontology#hasDespatchPeriod">
    <skos:historyNote xml:lang="en">WG Approval 16/07/2024</skos:historyNote>
  </rdf:Description>
  <rdf:Description rdf:about="http://data.europa.eu/a4g/ontology#hasDespatchedQuantity">
    <rdf:type rdf:resource="http://www.w3.org/2002/07/owl#ObjectProperty"/>
  </rdf:Description>
  <rdf:Description rdf:about="http://data.europa.eu/a4g/ontology#hasDespatchedQuantity">
    <rdfs:isDefinedBy rdf:resource="http://data.europa.eu/a4g/ontology#ful"/>
  </rdf:Description>
  <rdf:Description rdf:about="http://data.europa.eu/a4g/ontology#hasDespatchedQuantity">
    <skos:definition xml:lang="en">The Quantity that has been sent. (epo-ful:DespatchLine -&gt; epo:Quantity (+epo-ful:hasDespatchedQuantity))</skos:definition>
  </rdf:Description>
  <rdf:Description rdf:about="http://data.europa.eu/a4g/ontology#hasDespatchedQuantity">
    <skos:prefLabel xml:lang="en">Has despatched quantity</skos:prefLabel>
  </rdf:Description>
  <rdf:Description rdf:about="http://data.europa.eu/a4g/ontology#hasDespatchedQuantity">
    <skos:historyNote xml:lang="en">WG Approval 18/06/2024</skos:historyNote>
  </rdf:Description>
  <rdf:Description rdf:about="http://data.europa.eu/a4g/ontology#hasDespatcherConsignmentID">
    <rdf:type rdf:resource="http://www.w3.org/2002/07/owl#ObjectProperty"/>
  </rdf:Description>
  <rdf:Description rdf:about="http://data.europa.eu/a4g/ontology#hasDespatcherConsignmentID">
    <rdfs:isDefinedBy rdf:resource="http://data.europa.eu/a4g/ontology#ful"/>
  </rdf:Description>
  <rdf:Description rdf:about="http://data.europa.eu/a4g/ontology#hasDespatcherConsignmentID">
    <skos:definition xml:lang="en">The identifier of the the Consignment given by the Despatcher. (epo-ful:Consignment -&gt; adms:Identifier (+epo-ful:hasDespatcherConsignmentID))</skos:definition>
  </rdf:Description>
  <rdf:Description rdf:about="http://data.europa.eu/a4g/ontology#hasDespatcherConsignmentID">
    <skos:prefLabel xml:lang="en">Has despatcher consignment i d</skos:prefLabel>
  </rdf:Description>
  <rdf:Description rdf:about="http://data.europa.eu/a4g/ontology#hasDespatcherConsignmentID">
    <skos:historyNote xml:lang="en">WG Approval 10/06/2024</skos:historyNote>
  </rdf:Description>
  <rdf:Description rdf:about="http://data.europa.eu/a4g/ontology#hasDocumentStatus">
    <rdf:type rdf:resource="http://www.w3.org/2002/07/owl#ObjectProperty"/>
  </rdf:Description>
  <rdf:Description rdf:about="http://data.europa.eu/a4g/ontology#hasDocumentStatus">
    <rdfs:isDefinedBy rdf:resource="http://data.europa.eu/a4g/ontology#ful"/>
  </rdf:Description>
  <rdf:Description rdf:about="http://data.europa.eu/a4g/ontology#hasDocumentStatus">
    <skos:definition xml:lang="en">https://test-docs.peppol.eu/logistics/transport-execution/codelist/DocumentStatusCode/ (epo-cat:PostAwardDocument -&gt; at-voc-new:document-status (+epo:hasDocumentStatus))</skos:definition>
  </rdf:Description>
  <rdf:Description rdf:about="http://data.europa.eu/a4g/ontology#hasDocumentStatus">
    <skos:prefLabel xml:lang="en">Has document status</skos:prefLabel>
  </rdf:Description>
  <rdf:Description rdf:about="http://data.europa.eu/a4g/ontology#hasDriverPerson">
    <rdf:type rdf:resource="http://www.w3.org/2002/07/owl#ObjectProperty"/>
  </rdf:Description>
  <rdf:Description rdf:about="http://data.europa.eu/a4g/ontology#hasDriverPerson">
    <rdfs:isDefinedBy rdf:resource="http://data.europa.eu/a4g/ontology#ful"/>
  </rdf:Description>
  <rdf:Description rdf:about="http://data.europa.eu/a4g/ontology#hasDriverPerson">
    <skos:definition xml:lang="en">Relation indicating the operator of the Transport Means. (epo-ful:TransportMeans -&gt; epo-ful:TransportMeansOperator (+epo:hasDriverPerson))</skos:definition>
  </rdf:Description>
  <rdf:Description rdf:about="http://data.europa.eu/a4g/ontology#hasDriverPerson">
    <skos:prefLabel xml:lang="en">Has driver person</skos:prefLabel>
  </rdf:Description>
  <rdf:Description rdf:about="http://data.europa.eu/a4g/ontology#hasDriverPerson">
    <skos:historyNote xml:lang="en">WG Approval 02/07/2024</skos:historyNote>
  </rdf:Description>
  <rdf:Description rdf:about="http://data.europa.eu/a4g/ontology#hasEstimatedDeliveryPeriod">
    <rdf:type rdf:resource="http://www.w3.org/2002/07/owl#ObjectProperty"/>
  </rdf:Description>
  <rdf:Description rdf:about="http://data.europa.eu/a4g/ontology#hasEstimatedDeliveryPeriod">
    <rdfs:isDefinedBy rdf:resource="http://data.europa.eu/a4g/ontology#ful"/>
  </rdf:Description>
  <rdf:Description rdf:about="http://data.europa.eu/a4g/ontology#hasEstimatedDeliveryPeriod">
    <skos:definition xml:lang="en">The forecasted time period given by the Despatcher to provide the goods and services. (epo-ful:ShipmentInformation -&gt; epo:Period (+epo-ful:hasEstimatedDeliveryPeriod))</skos:definition>
  </rdf:Description>
  <rdf:Description rdf:about="http://data.europa.eu/a4g/ontology#hasEstimatedDeliveryPeriod">
    <skos:prefLabel xml:lang="en">Has estimated delivery period</skos:prefLabel>
  </rdf:Description>
  <rdf:Description rdf:about="http://data.europa.eu/a4g/ontology#hasEstimatedDeliveryPeriod">
    <skos:historyNote xml:lang="en">WG Approval 18/06/2024</skos:historyNote>
  </rdf:Description>
  <rdf:Description rdf:about="http://data.europa.eu/a4g/ontology#hasFreightAllowanceCharge">
    <rdf:type rdf:resource="http://www.w3.org/2002/07/owl#ObjectProperty"/>
  </rdf:Description>
  <rdf:Description rdf:about="http://data.europa.eu/a4g/ontology#hasFreightAllowanceCharge">
    <rdfs:isDefinedBy rdf:resource="http://data.europa.eu/a4g/ontology#ful"/>
  </rdf:Description>
  <rdf:Description rdf:about="http://data.europa.eu/a4g/ontology#hasFreightAllowanceCharge">
    <skos:prefLabel xml:lang="en">Has freight allowance charge</skos:prefLabel>
  </rdf:Description>
  <rdf:Description rdf:about="http://data.europa.eu/a4g/ontology#hasFreightCharge">
    <rdf:type rdf:resource="http://www.w3.org/2002/07/owl#ObjectProperty"/>
  </rdf:Description>
  <rdf:Description rdf:about="http://data.europa.eu/a4g/ontology#hasFreightCharge">
    <rdfs:isDefinedBy rdf:resource="http://data.europa.eu/a4g/ontology#ful"/>
  </rdf:Description>
  <rdf:Description rdf:about="http://data.europa.eu/a4g/ontology#hasFreightCharge">
    <skos:definition xml:lang="en">The total cost for moving the goods. (epo-ful:Consignment -&gt; epo-cat:ChargeInformation (+epo-ful:hasFreightCharge))</skos:definition>
  </rdf:Description>
  <rdf:Description rdf:about="http://data.europa.eu/a4g/ontology#hasFreightCharge">
    <skos:prefLabel xml:lang="en">Has freight charge</skos:prefLabel>
  </rdf:Description>
  <rdf:Description rdf:about="http://data.europa.eu/a4g/ontology#hasFreightCharge">
    <skos:historyNote xml:lang="en">WG Approval 18/06/2024</skos:historyNote>
  </rdf:Description>
  <rdf:Description rdf:about="http://data.europa.eu/a4g/ontology#hasFreightForwarderConsignmentID">
    <rdf:type rdf:resource="http://www.w3.org/2002/07/owl#ObjectProperty"/>
  </rdf:Description>
  <rdf:Description rdf:about="http://data.europa.eu/a4g/ontology#hasFreightForwarderConsignmentID">
    <rdfs:isDefinedBy rdf:resource="http://data.europa.eu/a4g/ontology#ful"/>
  </rdf:Description>
  <rdf:Description rdf:about="http://data.europa.eu/a4g/ontology#hasFreightForwarderConsignmentID">
    <skos:definition xml:lang="en">The identifier of the the Consignment given by the Freight Forwarder. (epo-ful:Consignment -&gt; adms:Identifier (+epo-ful:hasFreightForwarderConsignmentID))</skos:definition>
  </rdf:Description>
  <rdf:Description rdf:about="http://data.europa.eu/a4g/ontology#hasFreightForwarderConsignmentID">
    <skos:prefLabel xml:lang="en">Has freight forwarder consignment i d</skos:prefLabel>
  </rdf:Description>
  <rdf:Description rdf:about="http://data.europa.eu/a4g/ontology#hasFreightForwarderConsignmentID">
    <skos:historyNote xml:lang="en">WG Approval 10/06/2024</skos:historyNote>
  </rdf:Description>
  <rdf:Description rdf:about="http://data.europa.eu/a4g/ontology#hasGrossVolume">
    <rdf:type rdf:resource="http://www.w3.org/2002/07/owl#ObjectProperty"/>
  </rdf:Description>
  <rdf:Description rdf:about="http://data.europa.eu/a4g/ontology#hasGrossVolume">
    <rdfs:isDefinedBy rdf:resource="http://data.europa.eu/a4g/ontology#ful"/>
  </rdf:Description>
  <rdf:Description rdf:about="http://data.europa.eu/a4g/ontology#hasGrossVolume">
    <skos:definition xml:lang="en">The amount of space that is required including the packaging. (epo-ful:AbstractContainer -&gt; epo:Quantity (+epo-ful:hasGrossVolume)) The amount of space that is required including the packaging. (epo-ful:Consignment -&gt; epo:Quantity (+epo-ful:hasGrossVolume))</skos:definition>
  </rdf:Description>
  <rdf:Description rdf:about="http://data.europa.eu/a4g/ontology#hasGrossVolume">
    <skos:prefLabel xml:lang="en">Has gross volume</skos:prefLabel>
  </rdf:Description>
  <rdf:Description rdf:about="http://data.europa.eu/a4g/ontology#hasGrossVolume">
    <skos:historyNote xml:lang="en">WG Approval 18/06/2024</skos:historyNote>
  </rdf:Description>
  <rdf:Description rdf:about="http://data.europa.eu/a4g/ontology#hasGrossWeight">
    <rdf:type rdf:resource="http://www.w3.org/2002/07/owl#ObjectProperty"/>
  </rdf:Description>
  <rdf:Description rdf:about="http://data.europa.eu/a4g/ontology#hasGrossWeight">
    <rdfs:isDefinedBy rdf:resource="http://data.europa.eu/a4g/ontology#ful"/>
  </rdf:Description>
  <rdf:Description rdf:about="http://data.europa.eu/a4g/ontology#hasGrossWeight">
    <skos:definition xml:lang="en">The total mass of goods including the packaging. (epo-ful:AbstractContainer -&gt; epo:Quantity (+epo-ful:hasGrossWeight)) The total mass of goods including the packaging. (epo-ful:Consignment -&gt; epo:Quantity (+epo-ful:hasGrossWeight))</skos:definition>
  </rdf:Description>
  <rdf:Description rdf:about="http://data.europa.eu/a4g/ontology#hasGrossWeight">
    <skos:prefLabel xml:lang="en">Has gross weight</skos:prefLabel>
  </rdf:Description>
  <rdf:Description rdf:about="http://data.europa.eu/a4g/ontology#hasGrossWeight">
    <skos:historyNote xml:lang="en">WG Approval 18/06/2024</skos:historyNote>
  </rdf:Description>
  <rdf:Description rdf:about="http://data.europa.eu/a4g/ontology#hasHandlingInstruction">
    <rdf:type rdf:resource="http://www.w3.org/2002/07/owl#DatatypeProperty"/>
  </rdf:Description>
  <rdf:Description rdf:about="http://data.europa.eu/a4g/ontology#hasHandlingInstruction">
    <rdfs:isDefinedBy rdf:resource="http://data.europa.eu/a4g/ontology#ful"/>
  </rdf:Description>
  <rdf:Description rdf:about="http://data.europa.eu/a4g/ontology#hasHandlingInstruction">
    <skos:definition xml:lang="en">Instruction on how to handle the Goods Items during transportation. (epo-ful:Consignment) Instruction on how to handle the Goods Items during transportation. (epo-ful:TransportHandlingUnit)</skos:definition>
  </rdf:Description>
  <rdf:Description rdf:about="http://data.europa.eu/a4g/ontology#hasHandlingInstruction">
    <skos:prefLabel xml:lang="en">Has handling instruction</skos:prefLabel>
  </rdf:Description>
  <rdf:Description rdf:about="http://data.europa.eu/a4g/ontology#hasHandlingInstruction">
    <skos:historyNote xml:lang="en">WG Approval 05/06/2024</skos:historyNote>
  </rdf:Description>
  <rdf:Description rdf:about="http://data.europa.eu/a4g/ontology#hasHandlingInstructionCode">
    <rdf:type rdf:resource="http://www.w3.org/2002/07/owl#ObjectProperty"/>
  </rdf:Description>
  <rdf:Description rdf:about="http://data.europa.eu/a4g/ontology#hasHandlingInstructionCode">
    <rdfs:isDefinedBy rdf:resource="http://data.europa.eu/a4g/ontology#ful"/>
  </rdf:Description>
  <rdf:Description rdf:about="http://data.europa.eu/a4g/ontology#hasHandlingInstructionCode">
    <skos:definition xml:lang="en">Instruction on how to handle the Goods Items during transportation, expressed as a code. (epo-ful:Consignment -&gt; at-voc-new:handling-instruction (+epo-ful:hasHandlingInstructionCode)) Instruction on how to handle the Goods Items during transportation, expressed as a code. (epo-ful:TransportHandlingUnit -&gt; at-voc-new:handling-instruction (+epo-ful:hasHandlingInstructionCode))</skos:definition>
  </rdf:Description>
  <rdf:Description rdf:about="http://data.europa.eu/a4g/ontology#hasHandlingInstructionCode">
    <skos:prefLabel xml:lang="en">Has handling instruction code</skos:prefLabel>
  </rdf:Description>
  <rdf:Description rdf:about="http://data.europa.eu/a4g/ontology#hasHeight">
    <rdf:type rdf:resource="http://www.w3.org/2002/07/owl#ObjectProperty"/>
  </rdf:Description>
  <rdf:Description rdf:about="http://data.europa.eu/a4g/ontology#hasHeight">
    <rdfs:isDefinedBy rdf:resource="http://data.europa.eu/a4g/ontology#ful"/>
  </rdf:Description>
  <rdf:Description rdf:about="http://data.europa.eu/a4g/ontology#hasHeight">
    <skos:definition xml:lang="en">The vertical measurement. (epo-ful:AbstractContainer -&gt; epo:Quantity (+epo-ful:hasHeight))</skos:definition>
  </rdf:Description>
  <rdf:Description rdf:about="http://data.europa.eu/a4g/ontology#hasHeight">
    <skos:prefLabel xml:lang="en">Has height</skos:prefLabel>
  </rdf:Description>
  <rdf:Description rdf:about="http://data.europa.eu/a4g/ontology#hasHeight">
    <skos:historyNote xml:lang="en">WG Approval 18/06/2024</skos:historyNote>
  </rdf:Description>
  <rdf:Description rdf:about="http://data.europa.eu/a4g/ontology#hasLength">
    <rdf:type rdf:resource="http://www.w3.org/2002/07/owl#ObjectProperty"/>
  </rdf:Description>
  <rdf:Description rdf:about="http://data.europa.eu/a4g/ontology#hasLength">
    <rdfs:isDefinedBy rdf:resource="http://data.europa.eu/a4g/ontology#ful"/>
  </rdf:Description>
  <rdf:Description rdf:about="http://data.europa.eu/a4g/ontology#hasLength">
    <skos:definition xml:lang="en">The horizontal measurement. Additional Information: The length is the longer side between the length and the width. (epo-ful:AbstractContainer -&gt; epo:Quantity (+epo-ful:hasLength))</skos:definition>
  </rdf:Description>
  <rdf:Description rdf:about="http://data.europa.eu/a4g/ontology#hasLength">
    <skos:prefLabel xml:lang="en">Has length</skos:prefLabel>
  </rdf:Description>
  <rdf:Description rdf:about="http://data.europa.eu/a4g/ontology#hasLength">
    <skos:historyNote xml:lang="en">WG Approval 18/06/2024</skos:historyNote>
  </rdf:Description>
  <rdf:Description rdf:about="http://data.europa.eu/a4g/ontology#hasLoadingLength">
    <rdf:type rdf:resource="http://www.w3.org/2002/07/owl#ObjectProperty"/>
  </rdf:Description>
  <rdf:Description rdf:about="http://data.europa.eu/a4g/ontology#hasLoadingLength">
    <rdfs:isDefinedBy rdf:resource="http://data.europa.eu/a4g/ontology#ful"/>
  </rdf:Description>
  <rdf:Description rdf:about="http://data.europa.eu/a4g/ontology#hasLoadingLength">
    <skos:definition xml:lang="en">The length (epo-ful:Consignment -&gt; epo:Quantity (+epo-ful:hasLoadingLength))</skos:definition>
  </rdf:Description>
  <rdf:Description rdf:about="http://data.europa.eu/a4g/ontology#hasLoadingLength">
    <skos:prefLabel xml:lang="en">Has loading length</skos:prefLabel>
  </rdf:Description>
  <rdf:Description rdf:about="http://data.europa.eu/a4g/ontology#hasLoadingMeter">
    <rdf:type rdf:resource="http://www.w3.org/2002/07/owl#ObjectProperty"/>
  </rdf:Description>
  <rdf:Description rdf:about="http://data.europa.eu/a4g/ontology#hasLoadingMeter">
    <rdfs:isDefinedBy rdf:resource="http://data.europa.eu/a4g/ontology#ful"/>
  </rdf:Description>
  <rdf:Description rdf:about="http://data.europa.eu/a4g/ontology#hasLoadingMeter">
    <skos:definition xml:lang="en">The area of the Consignment in meters divided by the width of the truck, which is considered to be 2.4 meters. (epo-ful:Consignment -&gt; epo:Quantity (+epo-ful:hasLoadingMeter))</skos:definition>
  </rdf:Description>
  <rdf:Description rdf:about="http://data.europa.eu/a4g/ontology#hasLoadingMeter">
    <skos:prefLabel xml:lang="en">Has loading meter</skos:prefLabel>
  </rdf:Description>
  <rdf:Description rdf:about="http://data.europa.eu/a4g/ontology#hasLoadingMeter">
    <skos:historyNote xml:lang="en">WG Approval 18/06/2024</skos:historyNote>
  </rdf:Description>
  <rdf:Description rdf:about="http://data.europa.eu/a4g/ontology#hasMainCarriageShipmentStage">
    <rdf:type rdf:resource="http://www.w3.org/2002/07/owl#ObjectProperty"/>
  </rdf:Description>
  <rdf:Description rdf:about="http://data.europa.eu/a4g/ontology#hasMainCarriageShipmentStage">
    <rdfs:isDefinedBy rdf:resource="http://data.europa.eu/a4g/ontology#ful"/>
  </rdf:Description>
  <rdf:Description rdf:about="http://data.europa.eu/a4g/ontology#hasMainCarriageShipmentStage">
    <skos:definition xml:lang="en">The Shipment Stage for the longest distance covered in a transport chain. (epo-ful:Consignment -&gt; epo-ful:ShipmentStage (+epo-ful:hasMainCarriageShipmentStage))</skos:definition>
  </rdf:Description>
  <rdf:Description rdf:about="http://data.europa.eu/a4g/ontology#hasMainCarriageShipmentStage">
    <skos:prefLabel xml:lang="en">Has main carriage shipment stage</skos:prefLabel>
  </rdf:Description>
  <rdf:Description rdf:about="http://data.europa.eu/a4g/ontology#hasMainCarriageShipmentStage">
    <skos:historyNote xml:lang="en">WG Approval 18/06/2024</skos:historyNote>
  </rdf:Description>
  <rdf:Description rdf:about="http://data.europa.eu/a4g/ontology#hasMaximumTemperature">
    <rdf:type rdf:resource="http://www.w3.org/2002/07/owl#ObjectProperty"/>
  </rdf:Description>
  <rdf:Description rdf:about="http://data.europa.eu/a4g/ontology#hasMaximumTemperature">
    <rdfs:isDefinedBy rdf:resource="http://data.europa.eu/a4g/ontology#ful"/>
  </rdf:Description>
  <rdf:Description rdf:about="http://data.europa.eu/a4g/ontology#hasMaximumTemperature">
    <skos:definition xml:lang="en">The highest tolerated temperature. (epo-ful:TemperatureSpecification -&gt; epo:Quantity (+epo-ful:hasMaximumTemperature))</skos:definition>
  </rdf:Description>
  <rdf:Description rdf:about="http://data.europa.eu/a4g/ontology#hasMaximumTemperature">
    <skos:prefLabel xml:lang="en">Has maximum temperature</skos:prefLabel>
  </rdf:Description>
  <rdf:Description rdf:about="http://data.europa.eu/a4g/ontology#hasMaximumTemperature">
    <skos:historyNote xml:lang="en">WG Approval 18/06/2024</skos:historyNote>
  </rdf:Description>
  <rdf:Description rdf:about="http://data.europa.eu/a4g/ontology#hasMinimumTemperature">
    <rdf:type rdf:resource="http://www.w3.org/2002/07/owl#ObjectProperty"/>
  </rdf:Description>
  <rdf:Description rdf:about="http://data.europa.eu/a4g/ontology#hasMinimumTemperature">
    <rdfs:isDefinedBy rdf:resource="http://data.europa.eu/a4g/ontology#ful"/>
  </rdf:Description>
  <rdf:Description rdf:about="http://data.europa.eu/a4g/ontology#hasMinimumTemperature">
    <skos:definition xml:lang="en">The lowest tolerated temperature. (epo-ful:TemperatureSpecification -&gt; epo:Quantity (+epo-ful:hasMinimumTemperature))</skos:definition>
  </rdf:Description>
  <rdf:Description rdf:about="http://data.europa.eu/a4g/ontology#hasMinimumTemperature">
    <skos:prefLabel xml:lang="en">Has minimum temperature</skos:prefLabel>
  </rdf:Description>
  <rdf:Description rdf:about="http://data.europa.eu/a4g/ontology#hasMinimumTemperature">
    <skos:historyNote xml:lang="en">WG Approval 18/06/2024</skos:historyNote>
  </rdf:Description>
  <rdf:Description rdf:about="http://data.europa.eu/a4g/ontology#hasNetVolume">
    <rdf:type rdf:resource="http://www.w3.org/2002/07/owl#ObjectProperty"/>
  </rdf:Description>
  <rdf:Description rdf:about="http://data.europa.eu/a4g/ontology#hasNetVolume">
    <rdfs:isDefinedBy rdf:resource="http://data.europa.eu/a4g/ontology#ful"/>
  </rdf:Description>
  <rdf:Description rdf:about="http://data.europa.eu/a4g/ontology#hasNetVolume">
    <skos:definition xml:lang="en">The amount of space that is required without the packaging. (epo-ful:AbstractContainer -&gt; epo:Quantity (+epo-ful:hasNetVolume))</skos:definition>
  </rdf:Description>
  <rdf:Description rdf:about="http://data.europa.eu/a4g/ontology#hasNetVolume">
    <skos:prefLabel xml:lang="en">Has net volume</skos:prefLabel>
  </rdf:Description>
  <rdf:Description rdf:about="http://data.europa.eu/a4g/ontology#hasNetVolume">
    <skos:historyNote xml:lang="en">WG Approval 18/06/2024</skos:historyNote>
  </rdf:Description>
  <rdf:Description rdf:about="http://data.europa.eu/a4g/ontology#hasNetWeight">
    <rdf:type rdf:resource="http://www.w3.org/2002/07/owl#ObjectProperty"/>
  </rdf:Description>
  <rdf:Description rdf:about="http://data.europa.eu/a4g/ontology#hasNetWeight">
    <rdfs:isDefinedBy rdf:resource="http://data.europa.eu/a4g/ontology#ful"/>
  </rdf:Description>
  <rdf:Description rdf:about="http://data.europa.eu/a4g/ontology#hasNetWeight">
    <skos:definition xml:lang="en">The total mass of goods without the packaging. (epo-ful:AbstractContainer -&gt; epo:Quantity (+epo-ful:hasNetWeight)) The total mass of goods without the packaging. (epo-ful:Consignment -&gt; epo:Quantity (+epo-ful:hasNetWeight))</skos:definition>
  </rdf:Description>
  <rdf:Description rdf:about="http://data.europa.eu/a4g/ontology#hasNetWeight">
    <skos:prefLabel xml:lang="en">Has net weight</skos:prefLabel>
  </rdf:Description>
  <rdf:Description rdf:about="http://data.europa.eu/a4g/ontology#hasNetWeight">
    <skos:historyNote xml:lang="en">WG Approval 18/06/2024</skos:historyNote>
  </rdf:Description>
  <rdf:Description rdf:about="http://data.europa.eu/a4g/ontology#hasOnCarriageShipmentStage">
    <rdf:type rdf:resource="http://www.w3.org/2002/07/owl#ObjectProperty"/>
  </rdf:Description>
  <rdf:Description rdf:about="http://data.europa.eu/a4g/ontology#hasOnCarriageShipmentStage">
    <rdfs:isDefinedBy rdf:resource="http://data.europa.eu/a4g/ontology#ful"/>
  </rdf:Description>
  <rdf:Description rdf:about="http://data.europa.eu/a4g/ontology#hasOnCarriageShipmentStage">
    <skos:definition xml:lang="en">Any Shipment Stage between the main carriage arrival point and the ultimate receiver in a transport chain. (epo-ful:Consignment -&gt; epo-ful:ShipmentStage (+epo-ful:hasOnCarriageShipmentStage))</skos:definition>
  </rdf:Description>
  <rdf:Description rdf:about="http://data.europa.eu/a4g/ontology#hasOnCarriageShipmentStage">
    <skos:prefLabel xml:lang="en">Has on carriage shipment stage</skos:prefLabel>
  </rdf:Description>
  <rdf:Description rdf:about="http://data.europa.eu/a4g/ontology#hasOnCarriageShipmentStage">
    <skos:historyNote xml:lang="en">WG Approval 18/06/2024</skos:historyNote>
  </rdf:Description>
  <rdf:Description rdf:about="http://data.europa.eu/a4g/ontology#hasOutstandingQuantity">
    <rdf:type rdf:resource="http://www.w3.org/2002/07/owl#ObjectProperty"/>
  </rdf:Description>
  <rdf:Description rdf:about="http://data.europa.eu/a4g/ontology#hasOutstandingQuantity">
    <rdfs:isDefinedBy rdf:resource="http://data.europa.eu/a4g/ontology#ful"/>
  </rdf:Description>
  <rdf:Description rdf:about="http://data.europa.eu/a4g/ontology#hasOutstandingQuantity">
    <skos:definition xml:lang="en">The Quantity of non-despatched Goods Items. (epo-ful:DespatchLine -&gt; epo:Quantity (+epo-ful:hasOutstandingQuantity))</skos:definition>
  </rdf:Description>
  <rdf:Description rdf:about="http://data.europa.eu/a4g/ontology#hasOutstandingQuantity">
    <skos:prefLabel xml:lang="en">Has outstanding quantity</skos:prefLabel>
  </rdf:Description>
  <rdf:Description rdf:about="http://data.europa.eu/a4g/ontology#hasOutstandingQuantity">
    <skos:historyNote xml:lang="en">WG Approval 05/06/2024</skos:historyNote>
  </rdf:Description>
  <rdf:Description rdf:about="http://data.europa.eu/a4g/ontology#hasOutstandingQuantityReason">
    <rdf:type rdf:resource="http://www.w3.org/2002/07/owl#DatatypeProperty"/>
  </rdf:Description>
  <rdf:Description rdf:about="http://data.europa.eu/a4g/ontology#hasOutstandingQuantityReason">
    <rdfs:isDefinedBy rdf:resource="http://data.europa.eu/a4g/ontology#ful"/>
  </rdf:Description>
  <rdf:Description rdf:about="http://data.europa.eu/a4g/ontology#hasOutstandingQuantityReason">
    <skos:definition xml:lang="en">Explanation of the outstanding quantity still to be despatched. (epo-ful:DespatchLine)</skos:definition>
  </rdf:Description>
  <rdf:Description rdf:about="http://data.europa.eu/a4g/ontology#hasOutstandingQuantityReason">
    <skos:prefLabel xml:lang="en">Has outstanding quantity reason</skos:prefLabel>
  </rdf:Description>
  <rdf:Description rdf:about="http://data.europa.eu/a4g/ontology#hasOutstandingQuantityReason">
    <skos:historyNote xml:lang="en">WG Approval 05/06/2024</skos:historyNote>
  </rdf:Description>
  <rdf:Description rdf:about="http://data.europa.eu/a4g/ontology#hasOversupplyQuantity">
    <rdf:type rdf:resource="http://www.w3.org/2002/07/owl#ObjectProperty"/>
  </rdf:Description>
  <rdf:Description rdf:about="http://data.europa.eu/a4g/ontology#hasOversupplyQuantity">
    <rdfs:isDefinedBy rdf:resource="http://data.europa.eu/a4g/ontology#ful"/>
  </rdf:Description>
  <rdf:Description rdf:about="http://data.europa.eu/a4g/ontology#hasOversupplyQuantity">
    <skos:prefLabel xml:lang="en">Has oversupply quantity</skos:prefLabel>
  </rdf:Description>
  <rdf:Description rdf:about="http://data.europa.eu/a4g/ontology#hasPackagingType">
    <rdf:type rdf:resource="http://www.w3.org/2002/07/owl#ObjectProperty"/>
  </rdf:Description>
  <rdf:Description rdf:about="http://data.europa.eu/a4g/ontology#hasPackagingType">
    <rdfs:isDefinedBy rdf:resource="http://data.europa.eu/a4g/ontology#ful"/>
  </rdf:Description>
  <rdf:Description rdf:about="http://data.europa.eu/a4g/ontology#hasPackagingType">
    <skos:definition xml:lang="en">The kind of Package. (epo-ful:Package -&gt; at-voc-new:packaging-type (+epo-ful:hasPackagingType))</skos:definition>
  </rdf:Description>
  <rdf:Description rdf:about="http://data.europa.eu/a4g/ontology#hasPackagingType">
    <skos:prefLabel xml:lang="en">Has packaging type</skos:prefLabel>
  </rdf:Description>
  <rdf:Description rdf:about="http://data.europa.eu/a4g/ontology#hasPackagingTypeDescription">
    <rdf:type rdf:resource="http://www.w3.org/2002/07/owl#DatatypeProperty"/>
  </rdf:Description>
  <rdf:Description rdf:about="http://data.europa.eu/a4g/ontology#hasPackagingTypeDescription">
    <rdfs:isDefinedBy rdf:resource="http://data.europa.eu/a4g/ontology#ful"/>
  </rdf:Description>
  <rdf:Description rdf:about="http://data.europa.eu/a4g/ontology#hasPackagingTypeDescription">
    <skos:definition xml:lang="en">Explanatory text about how the Goods Item is packed. (epo-ful:Package)</skos:definition>
  </rdf:Description>
  <rdf:Description rdf:about="http://data.europa.eu/a4g/ontology#hasPackagingTypeDescription">
    <skos:prefLabel xml:lang="en">Has packaging type description</skos:prefLabel>
  </rdf:Description>
  <rdf:Description rdf:about="http://data.europa.eu/a4g/ontology#hasPackagingTypeDescription">
    <skos:historyNote xml:lang="en">WG Approval 05/06/2024</skos:historyNote>
  </rdf:Description>
  <rdf:Description rdf:about="http://data.europa.eu/a4g/ontology#hasPreCarriageShipmentStage">
    <rdf:type rdf:resource="http://www.w3.org/2002/07/owl#ObjectProperty"/>
  </rdf:Description>
  <rdf:Description rdf:about="http://data.europa.eu/a4g/ontology#hasPreCarriageShipmentStage">
    <rdfs:isDefinedBy rdf:resource="http://data.europa.eu/a4g/ontology#ful"/>
  </rdf:Description>
  <rdf:Description rdf:about="http://data.europa.eu/a4g/ontology#hasPreCarriageShipmentStage">
    <skos:definition xml:lang="en">Any Shipment Stage between the Despatcher and the departure point of the main carriage in a transport chain. (epo-ful:Consignment -&gt; epo-ful:ShipmentStage (+epo-ful:hasPreCarriageShipmentStage))</skos:definition>
  </rdf:Description>
  <rdf:Description rdf:about="http://data.europa.eu/a4g/ontology#hasPreCarriageShipmentStage">
    <skos:prefLabel xml:lang="en">Has pre carriage shipment stage</skos:prefLabel>
  </rdf:Description>
  <rdf:Description rdf:about="http://data.europa.eu/a4g/ontology#hasPreCarriageShipmentStage">
    <skos:historyNote xml:lang="en">WG Approval 18/06/2024</skos:historyNote>
  </rdf:Description>
  <rdf:Description rdf:about="http://data.europa.eu/a4g/ontology#hasReceivedQuantity">
    <rdf:type rdf:resource="http://www.w3.org/2002/07/owl#ObjectProperty"/>
  </rdf:Description>
  <rdf:Description rdf:about="http://data.europa.eu/a4g/ontology#hasReceivedQuantity">
    <rdfs:isDefinedBy rdf:resource="http://data.europa.eu/a4g/ontology#ful"/>
  </rdf:Description>
  <rdf:Description rdf:about="http://data.europa.eu/a4g/ontology#hasReceivedQuantity">
    <skos:prefLabel xml:lang="en">Has received quantity</skos:prefLabel>
  </rdf:Description>
  <rdf:Description rdf:about="http://data.europa.eu/a4g/ontology#hasRejectReason">
    <rdf:type rdf:resource="http://www.w3.org/2002/07/owl#ObjectProperty"/>
  </rdf:Description>
  <rdf:Description rdf:about="http://data.europa.eu/a4g/ontology#hasRejectReason">
    <rdfs:isDefinedBy rdf:resource="http://data.europa.eu/a4g/ontology#ful"/>
  </rdf:Description>
  <rdf:Description rdf:about="http://data.europa.eu/a4g/ontology#hasRejectReason">
    <skos:prefLabel xml:lang="en">Has reject reason</skos:prefLabel>
  </rdf:Description>
  <rdf:Description rdf:about="http://data.europa.eu/a4g/ontology#hasRejectedQuantity">
    <rdf:type rdf:resource="http://www.w3.org/2002/07/owl#ObjectProperty"/>
  </rdf:Description>
  <rdf:Description rdf:about="http://data.europa.eu/a4g/ontology#hasRejectedQuantity">
    <rdfs:isDefinedBy rdf:resource="http://data.europa.eu/a4g/ontology#ful"/>
  </rdf:Description>
  <rdf:Description rdf:about="http://data.europa.eu/a4g/ontology#hasRejectedQuantity">
    <skos:prefLabel xml:lang="en">Has rejected quantity</skos:prefLabel>
  </rdf:Description>
  <rdf:Description rdf:about="http://data.europa.eu/a4g/ontology#hasRequestedPickUpInformation">
    <rdf:type rdf:resource="http://www.w3.org/2002/07/owl#ObjectProperty"/>
  </rdf:Description>
  <rdf:Description rdf:about="http://data.europa.eu/a4g/ontology#hasRequestedPickUpInformation">
    <rdfs:isDefinedBy rdf:resource="http://data.europa.eu/a4g/ontology#ful"/>
  </rdf:Description>
  <rdf:Description rdf:about="http://data.europa.eu/a4g/ontology#hasRequestedPickUpInformation">
    <skos:definition xml:lang="en">Information about the requested despatch of the Goods Items. (epo-ful:Consignment -&gt; epo-ful:ShipmentInformation (+epo-ful:hasRequestedPickUpInformation))</skos:definition>
  </rdf:Description>
  <rdf:Description rdf:about="http://data.europa.eu/a4g/ontology#hasRequestedPickUpInformation">
    <skos:prefLabel xml:lang="en">Has requested pick up information</skos:prefLabel>
  </rdf:Description>
  <rdf:Description rdf:about="http://data.europa.eu/a4g/ontology#hasRequestedPickUpInformation">
    <skos:historyNote xml:lang="en">WG Approval 25/06/2024</skos:historyNote>
  </rdf:Description>
  <rdf:Description rdf:about="http://data.europa.eu/a4g/ontology#hasShippingMark">
    <rdf:type rdf:resource="http://www.w3.org/2002/07/owl#DatatypeProperty"/>
  </rdf:Description>
  <rdf:Description rdf:about="http://data.europa.eu/a4g/ontology#hasShippingMark">
    <rdfs:isDefinedBy rdf:resource="http://data.europa.eu/a4g/ontology#ful"/>
  </rdf:Description>
  <rdf:Description rdf:about="http://data.europa.eu/a4g/ontology#hasShippingMark">
    <skos:definition xml:lang="en">A text that the buyer requests to be printed on the packing labels. (epo-ful:TransportHandlingUnit)</skos:definition>
  </rdf:Description>
  <rdf:Description rdf:about="http://data.europa.eu/a4g/ontology#hasShippingMark">
    <skos:prefLabel xml:lang="en">Has shipping mark</skos:prefLabel>
  </rdf:Description>
  <rdf:Description rdf:about="http://data.europa.eu/a4g/ontology#hasShippingMark">
    <skos:historyNote xml:lang="en">WG Approval 05/06/2024</skos:historyNote>
  </rdf:Description>
  <rdf:Description rdf:about="http://data.europa.eu/a4g/ontology#hasShortQuantity">
    <rdf:type rdf:resource="http://www.w3.org/2002/07/owl#ObjectProperty"/>
  </rdf:Description>
  <rdf:Description rdf:about="http://data.europa.eu/a4g/ontology#hasShortQuantity">
    <rdfs:isDefinedBy rdf:resource="http://data.europa.eu/a4g/ontology#ful"/>
  </rdf:Description>
  <rdf:Description rdf:about="http://data.europa.eu/a4g/ontology#hasShortQuantity">
    <skos:prefLabel xml:lang="en">Has short quantity</skos:prefLabel>
  </rdf:Description>
  <rdf:Description rdf:about="http://data.europa.eu/a4g/ontology#hasShortageAction">
    <rdf:type rdf:resource="http://www.w3.org/2002/07/owl#ObjectProperty"/>
  </rdf:Description>
  <rdf:Description rdf:about="http://data.europa.eu/a4g/ontology#hasShortageAction">
    <rdfs:isDefinedBy rdf:resource="http://data.europa.eu/a4g/ontology#ful"/>
  </rdf:Description>
  <rdf:Description rdf:about="http://data.europa.eu/a4g/ontology#hasShortageAction">
    <skos:prefLabel xml:lang="en">Has shortage action</skos:prefLabel>
  </rdf:Description>
  <rdf:Description rdf:about="http://data.europa.eu/a4g/ontology#hasSizeType">
    <rdf:type rdf:resource="http://www.w3.org/2002/07/owl#ObjectProperty"/>
  </rdf:Description>
  <rdf:Description rdf:about="http://data.europa.eu/a4g/ontology#hasSizeType">
    <rdfs:isDefinedBy rdf:resource="http://data.europa.eu/a4g/ontology#ful"/>
  </rdf:Description>
  <rdf:Description rdf:about="http://data.europa.eu/a4g/ontology#hasSizeType">
    <skos:definition xml:lang="en">An extension classification specifying the measurement of the Transport Equipment. Additional Information: This codelist should be used only in the case of a container. (epo-ful:TransportEquipment -&gt; at-voc-new:size-type (+epo-ful:hasSizeType))</skos:definition>
  </rdf:Description>
  <rdf:Description rdf:about="http://data.europa.eu/a4g/ontology#hasSizeType">
    <skos:prefLabel xml:lang="en">Has size type</skos:prefLabel>
  </rdf:Description>
  <rdf:Description rdf:about="http://data.europa.eu/a4g/ontology#hasSpecialInstruction">
    <rdf:type rdf:resource="http://www.w3.org/2002/07/owl#DatatypeProperty"/>
  </rdf:Description>
  <rdf:Description rdf:about="http://data.europa.eu/a4g/ontology#hasSpecialInstruction">
    <rdfs:isDefinedBy rdf:resource="http://data.europa.eu/a4g/ontology#ful"/>
  </rdf:Description>
  <rdf:Description rdf:about="http://data.europa.eu/a4g/ontology#hasSpecialInstruction">
    <skos:definition xml:lang="en">This attribute should be removed in the next major release. (epo-ful:Consignment)</skos:definition>
  </rdf:Description>
  <rdf:Description rdf:about="http://data.europa.eu/a4g/ontology#hasSpecialInstruction">
    <skos:prefLabel xml:lang="en">Has special instruction</skos:prefLabel>
  </rdf:Description>
  <rdf:Description rdf:about="http://data.europa.eu/a4g/ontology#hasSpecialServiceInstruction">
    <rdf:type rdf:resource="http://www.w3.org/2002/07/owl#DatatypeProperty"/>
  </rdf:Description>
  <rdf:Description rdf:about="http://data.europa.eu/a4g/ontology#hasSpecialServiceInstruction">
    <rdfs:isDefinedBy rdf:resource="http://data.europa.eu/a4g/ontology#ful"/>
  </rdf:Description>
  <rdf:Description rdf:about="http://data.europa.eu/a4g/ontology#hasSpecialServiceInstruction">
    <skos:definition xml:lang="en">Description about special services needed for loading or unloading the Goods Items. (epo-ful:Consignment)</skos:definition>
  </rdf:Description>
  <rdf:Description rdf:about="http://data.europa.eu/a4g/ontology#hasSpecialServiceInstruction">
    <skos:prefLabel xml:lang="en">Has special service instruction</skos:prefLabel>
  </rdf:Description>
  <rdf:Description rdf:about="http://data.europa.eu/a4g/ontology#hasSpecialServiceInstruction">
    <skos:historyNote xml:lang="en">WG Approval 21/05/2024</skos:historyNote>
  </rdf:Description>
  <rdf:Description rdf:about="http://data.europa.eu/a4g/ontology#hasTemperatureSpecification">
    <rdf:type rdf:resource="http://www.w3.org/2002/07/owl#ObjectProperty"/>
  </rdf:Description>
  <rdf:Description rdf:about="http://data.europa.eu/a4g/ontology#hasTemperatureSpecification">
    <rdfs:isDefinedBy rdf:resource="http://data.europa.eu/a4g/ontology#ful"/>
  </rdf:Description>
  <rdf:Description rdf:about="http://data.europa.eu/a4g/ontology#hasTemperatureSpecification">
    <skos:definition xml:lang="en">Relation indicating the Temperature Specification for the instance of the concept. (epo-ful:AbstractContainer -&gt; epo-ful:TemperatureSpecification (+epo-ful:hasTemperatureSpecification))</skos:definition>
  </rdf:Description>
  <rdf:Description rdf:about="http://data.europa.eu/a4g/ontology#hasTemperatureSpecification">
    <skos:prefLabel xml:lang="en">Has temperature specification</skos:prefLabel>
  </rdf:Description>
  <rdf:Description rdf:about="http://data.europa.eu/a4g/ontology#hasTemperatureSpecification">
    <skos:historyNote xml:lang="en">WG Approval 25/06/2024</skos:historyNote>
  </rdf:Description>
  <rdf:Description rdf:about="http://data.europa.eu/a4g/ontology#hasTotalGoodsItemQuantity">
    <rdf:type rdf:resource="http://www.w3.org/2002/07/owl#ObjectProperty"/>
  </rdf:Description>
  <rdf:Description rdf:about="http://data.europa.eu/a4g/ontology#hasTotalGoodsItemQuantity">
    <rdfs:isDefinedBy rdf:resource="http://data.europa.eu/a4g/ontology#ful"/>
  </rdf:Description>
  <rdf:Description rdf:about="http://data.europa.eu/a4g/ontology#hasTotalGoodsItemQuantity">
    <skos:definition xml:lang="en">Relation indicating the number of the Goods Items. (epo-ful:AbstractContainer -&gt; epo:Quantity (+epo-ful:hasTotalGoodsItemQuantity)) Relation indicating the number of the Goods Items. (epo-ful:Consignment -&gt; epo:Quantity (+epo-ful:hasTotalGoodsItemQuantity))</skos:definition>
  </rdf:Description>
  <rdf:Description rdf:about="http://data.europa.eu/a4g/ontology#hasTotalGoodsItemQuantity">
    <skos:prefLabel xml:lang="en">Has total goods item quantity</skos:prefLabel>
  </rdf:Description>
  <rdf:Description rdf:about="http://data.europa.eu/a4g/ontology#hasTotalGoodsItemQuantity">
    <skos:historyNote xml:lang="en">WG Approval 25/06/2024</skos:historyNote>
  </rdf:Description>
  <rdf:Description rdf:about="http://data.europa.eu/a4g/ontology#hasTraceID">
    <rdf:type rdf:resource="http://www.w3.org/2002/07/owl#ObjectProperty"/>
  </rdf:Description>
  <rdf:Description rdf:about="http://data.europa.eu/a4g/ontology#hasTraceID">
    <rdfs:isDefinedBy rdf:resource="http://data.europa.eu/a4g/ontology#ful"/>
  </rdf:Description>
  <rdf:Description rdf:about="http://data.europa.eu/a4g/ontology#hasTraceID">
    <skos:definition xml:lang="en">The identifier used for tracking the Goods Item. Additional information: An example is the EPC number used in RFID. (epo-ful:GoodsItem -&gt; adms:Identifier (+epo-ful:hasTraceID))</skos:definition>
  </rdf:Description>
  <rdf:Description rdf:about="http://data.europa.eu/a4g/ontology#hasTraceID">
    <skos:prefLabel xml:lang="en">Has trace i d</skos:prefLabel>
  </rdf:Description>
  <rdf:Description rdf:about="http://data.europa.eu/a4g/ontology#hasTraceID">
    <skos:historyNote xml:lang="en">WG Approval 21/09/2023</skos:historyNote>
  </rdf:Description>
  <rdf:Description rdf:about="http://data.europa.eu/a4g/ontology#hasTransportEquipmentSeal">
    <rdf:type rdf:resource="http://www.w3.org/2002/07/owl#ObjectProperty"/>
  </rdf:Description>
  <rdf:Description rdf:about="http://data.europa.eu/a4g/ontology#hasTransportEquipmentSeal">
    <rdfs:isDefinedBy rdf:resource="http://data.europa.eu/a4g/ontology#ful"/>
  </rdf:Description>
  <rdf:Description rdf:about="http://data.europa.eu/a4g/ontology#hasTransportEquipmentSeal">
    <skos:definition xml:lang="en">Relation indicating that the instance of the concept has a Transport Equipment Seal. (epo-ful:TransportEquipment -&gt; epo-ful:TransportEquipmentSeal (+epo-ful:hasTransportEquipmentSeal))</skos:definition>
  </rdf:Description>
  <rdf:Description rdf:about="http://data.europa.eu/a4g/ontology#hasTransportEquipmentSeal">
    <skos:prefLabel xml:lang="en">Has transport equipment seal</skos:prefLabel>
  </rdf:Description>
  <rdf:Description rdf:about="http://data.europa.eu/a4g/ontology#hasTransportEquipmentSeal">
    <skos:historyNote xml:lang="en">WG Approval 25/06/2024</skos:historyNote>
  </rdf:Description>
  <rdf:Description rdf:about="http://data.europa.eu/a4g/ontology#hasTransportEquipmentType">
    <rdf:type rdf:resource="http://www.w3.org/2002/07/owl#ObjectProperty"/>
  </rdf:Description>
  <rdf:Description rdf:about="http://data.europa.eu/a4g/ontology#hasTransportEquipmentType">
    <rdfs:isDefinedBy rdf:resource="http://data.europa.eu/a4g/ontology#ful"/>
  </rdf:Description>
  <rdf:Description rdf:about="http://data.europa.eu/a4g/ontology#hasTransportEquipmentType">
    <skos:definition xml:lang="en">The kind of Transport Equipment. (epo-ful:TransportEquipment -&gt; at-voc-new:transport-equipment-type (+epo-ful:hasTransportEquipmentType))</skos:definition>
  </rdf:Description>
  <rdf:Description rdf:about="http://data.europa.eu/a4g/ontology#hasTransportEquipmentType">
    <skos:prefLabel xml:lang="en">Has transport equipment type</skos:prefLabel>
  </rdf:Description>
  <rdf:Description rdf:about="http://data.europa.eu/a4g/ontology#hasTransportHandlingUnitQuantity">
    <rdf:type rdf:resource="http://www.w3.org/2002/07/owl#ObjectProperty"/>
  </rdf:Description>
  <rdf:Description rdf:about="http://data.europa.eu/a4g/ontology#hasTransportHandlingUnitQuantity">
    <rdfs:isDefinedBy rdf:resource="http://data.europa.eu/a4g/ontology#ful"/>
  </rdf:Description>
  <rdf:Description rdf:about="http://data.europa.eu/a4g/ontology#hasTransportHandlingUnitQuantity">
    <skos:definition xml:lang="en">Relation indicating the number of the Transport Handling Unit. (epo-ful:Consignment -&gt; epo:Quantity (+epo-ful:hasTransportHandlingUnitQuantity))</skos:definition>
  </rdf:Description>
  <rdf:Description rdf:about="http://data.europa.eu/a4g/ontology#hasTransportHandlingUnitQuantity">
    <skos:prefLabel xml:lang="en">Has transport handling unit quantity</skos:prefLabel>
  </rdf:Description>
  <rdf:Description rdf:about="http://data.europa.eu/a4g/ontology#hasTransportHandlingUnitQuantity">
    <skos:historyNote xml:lang="en">WG Approval 25/06/2024</skos:historyNote>
  </rdf:Description>
  <rdf:Description rdf:about="http://data.europa.eu/a4g/ontology#hasTransportMeansType">
    <rdf:type rdf:resource="http://www.w3.org/2002/07/owl#ObjectProperty"/>
  </rdf:Description>
  <rdf:Description rdf:about="http://data.europa.eu/a4g/ontology#hasTransportMeansType">
    <rdfs:isDefinedBy rdf:resource="http://data.europa.eu/a4g/ontology#ful"/>
  </rdf:Description>
  <rdf:Description rdf:about="http://data.europa.eu/a4g/ontology#hasTransportMeansType">
    <skos:definition xml:lang="en">The kind of Transport Means. (epo-ful:TransportMeans -&gt; at-voc-new:transport-means-type (+epo-ful:hasTransportMeansType))</skos:definition>
  </rdf:Description>
  <rdf:Description rdf:about="http://data.europa.eu/a4g/ontology#hasTransportMeansType">
    <skos:prefLabel xml:lang="en">Has transport means type</skos:prefLabel>
  </rdf:Description>
  <rdf:Description rdf:about="http://data.europa.eu/a4g/ontology#hasTransportMode">
    <rdf:type rdf:resource="http://www.w3.org/2002/07/owl#ObjectProperty"/>
  </rdf:Description>
  <rdf:Description rdf:about="http://data.europa.eu/a4g/ontology#hasTransportMode">
    <rdfs:isDefinedBy rdf:resource="http://data.europa.eu/a4g/ontology#ful"/>
  </rdf:Description>
  <rdf:Description rdf:about="http://data.europa.eu/a4g/ontology#hasTransportMode">
    <skos:definition xml:lang="en">The type of the transport used. (epo-ful:TransportMeans -&gt; at-voc-new:transport-mode (+epo-ful:hasTransportMode))</skos:definition>
  </rdf:Description>
  <rdf:Description rdf:about="http://data.europa.eu/a4g/ontology#hasTransportMode">
    <skos:prefLabel xml:lang="en">Has transport mode</skos:prefLabel>
  </rdf:Description>
  <rdf:Description rdf:about="http://data.europa.eu/a4g/ontology#hasVehicleDescription">
    <rdf:type rdf:resource="http://www.w3.org/2002/07/owl#DatatypeProperty"/>
  </rdf:Description>
  <rdf:Description rdf:about="http://data.europa.eu/a4g/ontology#hasVehicleDescription">
    <rdfs:isDefinedBy rdf:resource="http://data.europa.eu/a4g/ontology#ful"/>
  </rdf:Description>
  <rdf:Description rdf:about="http://data.europa.eu/a4g/ontology#hasVehicleDescription">
    <skos:definition xml:lang="en">(epo-ful:Consignment)</skos:definition>
  </rdf:Description>
  <rdf:Description rdf:about="http://data.europa.eu/a4g/ontology#hasVehicleDescription">
    <skos:prefLabel xml:lang="en">Has vehicle description</skos:prefLabel>
  </rdf:Description>
  <rdf:Description rdf:about="http://data.europa.eu/a4g/ontology#hasVehicleID">
    <rdf:type rdf:resource="http://www.w3.org/2002/07/owl#ObjectProperty"/>
  </rdf:Description>
  <rdf:Description rdf:about="http://data.europa.eu/a4g/ontology#hasVehicleID">
    <rdfs:isDefinedBy rdf:resource="http://data.europa.eu/a4g/ontology#ful"/>
  </rdf:Description>
  <rdf:Description rdf:about="http://data.europa.eu/a4g/ontology#hasVehicleID">
    <skos:definition xml:lang="en">The identifier of the Transport Means. (epo-ful:TransportMeans -&gt; adms:Identifier (+epo-ful:hasVehicleID))</skos:definition>
  </rdf:Description>
  <rdf:Description rdf:about="http://data.europa.eu/a4g/ontology#hasVehicleID">
    <skos:prefLabel xml:lang="en">Has vehicle i d</skos:prefLabel>
  </rdf:Description>
  <rdf:Description rdf:about="http://data.europa.eu/a4g/ontology#hasVehicleID">
    <skos:historyNote xml:lang="en">WG Approval 25/06/2024</skos:historyNote>
  </rdf:Description>
  <rdf:Description rdf:about="http://data.europa.eu/a4g/ontology#hasVehicleSegmentID">
    <rdf:type rdf:resource="http://www.w3.org/2002/07/owl#ObjectProperty"/>
  </rdf:Description>
  <rdf:Description rdf:about="http://data.europa.eu/a4g/ontology#hasVehicleSegmentID">
    <rdfs:isDefinedBy rdf:resource="http://data.europa.eu/a4g/ontology#ful"/>
  </rdf:Description>
  <rdf:Description rdf:about="http://data.europa.eu/a4g/ontology#hasVehicleSegmentID">
    <skos:definition xml:lang="en">The identifier of a part of the Transport Means. (epo-ful:TransportMeans -&gt; adms:Identifier (+epo-ful:hasVehicleSegmentID))</skos:definition>
  </rdf:Description>
  <rdf:Description rdf:about="http://data.europa.eu/a4g/ontology#hasVehicleSegmentID">
    <skos:prefLabel xml:lang="en">Has vehicle segment i d</skos:prefLabel>
  </rdf:Description>
  <rdf:Description rdf:about="http://data.europa.eu/a4g/ontology#hasVehicleSegmentID">
    <skos:historyNote xml:lang="en">WG Approval 25/06/2024</skos:historyNote>
  </rdf:Description>
  <rdf:Description rdf:about="http://data.europa.eu/a4g/ontology#hasWidth">
    <rdf:type rdf:resource="http://www.w3.org/2002/07/owl#ObjectProperty"/>
  </rdf:Description>
  <rdf:Description rdf:about="http://data.europa.eu/a4g/ontology#hasWidth">
    <rdfs:isDefinedBy rdf:resource="http://data.europa.eu/a4g/ontology#ful"/>
  </rdf:Description>
  <rdf:Description rdf:about="http://data.europa.eu/a4g/ontology#hasWidth">
    <skos:definition xml:lang="en">The measurement of the depth. Additional Information: The width is the shorter side between the length and the width. (epo-ful:AbstractContainer -&gt; epo:Quantity (+epo-ful:hasWidth))</skos:definition>
  </rdf:Description>
  <rdf:Description rdf:about="http://data.europa.eu/a4g/ontology#hasWidth">
    <skos:prefLabel xml:lang="en">Has width</skos:prefLabel>
  </rdf:Description>
  <rdf:Description rdf:about="http://data.europa.eu/a4g/ontology#hasWidth">
    <skos:historyNote xml:lang="en">WG Approval 18/06/2024</skos:historyNote>
  </rdf:Description>
  <rdf:Description rdf:about="http://data.europa.eu/a4g/ontology#isHazardousRisk">
    <rdf:type rdf:resource="http://www.w3.org/2002/07/owl#DatatypeProperty"/>
  </rdf:Description>
  <rdf:Description rdf:about="http://data.europa.eu/a4g/ontology#isHazardousRisk">
    <rdfs:isDefinedBy rdf:resource="http://data.europa.eu/a4g/ontology#ful"/>
  </rdf:Description>
  <rdf:Description rdf:about="http://data.europa.eu/a4g/ontology#isHazardousRisk">
    <skos:definition xml:lang="en">Indicates whether some of the contained Goods Items are hazardous. (epo-ful:AbstractContainer) Pending confirmation on whether this attribute should be removed in the next major release because is covered at the level of Consignment. (epo-ful:ShipmentStage) Indicates whether some of the contained Goods Items are hazardous. (epo-ful:Consignment)</skos:definition>
  </rdf:Description>
  <rdf:Description rdf:about="http://data.europa.eu/a4g/ontology#isHazardousRisk">
    <skos:prefLabel xml:lang="en">Is hazardous risk</skos:prefLabel>
  </rdf:Description>
  <rdf:Description rdf:about="http://data.europa.eu/a4g/ontology#isHazardousRisk">
    <skos:historyNote xml:lang="en">WG Approval 21/05/2024</skos:historyNote>
  </rdf:Description>
  <rdf:Description rdf:about="http://data.europa.eu/a4g/ontology#isPowerIndicated">
    <rdf:type rdf:resource="http://www.w3.org/2002/07/owl#DatatypeProperty"/>
  </rdf:Description>
  <rdf:Description rdf:about="http://data.europa.eu/a4g/ontology#isPowerIndicated">
    <rdfs:isDefinedBy rdf:resource="http://data.europa.eu/a4g/ontology#ful"/>
  </rdf:Description>
  <rdf:Description rdf:about="http://data.europa.eu/a4g/ontology#isPowerIndicated">
    <skos:definition xml:lang="en">Indicates whether the instance of the concept can supply electrical energy. Additional Information: The instance of the concept can be, for example, Transport Equipment. (epo-ful:TransportEquipment)</skos:definition>
  </rdf:Description>
  <rdf:Description rdf:about="http://data.europa.eu/a4g/ontology#isPowerIndicated">
    <skos:prefLabel xml:lang="en">Is power indicated</skos:prefLabel>
  </rdf:Description>
  <rdf:Description rdf:about="http://data.europa.eu/a4g/ontology#isPowerIndicated">
    <skos:historyNote xml:lang="en">WG Approval 05/06/2024</skos:historyNote>
  </rdf:Description>
  <rdf:Description rdf:about="http://data.europa.eu/a4g/ontology#isRefrigerated">
    <rdf:type rdf:resource="http://www.w3.org/2002/07/owl#DatatypeProperty"/>
  </rdf:Description>
  <rdf:Description rdf:about="http://data.europa.eu/a4g/ontology#isRefrigerated">
    <rdfs:isDefinedBy rdf:resource="http://data.europa.eu/a4g/ontology#ful"/>
  </rdf:Description>
  <rdf:Description rdf:about="http://data.europa.eu/a4g/ontology#isRefrigerated">
    <skos:definition xml:lang="en">Indicates whether the instance of the concept includes refrigeration. Additional Information: The instance of the concept can be, for example, Transport Equipment. (epo-ful:TransportEquipment)</skos:definition>
  </rdf:Description>
  <rdf:Description rdf:about="http://data.europa.eu/a4g/ontology#isRefrigerated">
    <skos:prefLabel xml:lang="en">Is refrigerated</skos:prefLabel>
  </rdf:Description>
  <rdf:Description rdf:about="http://data.europa.eu/a4g/ontology#isRefrigerated">
    <skos:historyNote xml:lang="en">WG Approval 05/06/2024</skos:historyNote>
  </rdf:Description>
  <rdf:Description rdf:about="http://data.europa.eu/a4g/ontology#isReturnable">
    <rdf:type rdf:resource="http://www.w3.org/2002/07/owl#DatatypeProperty"/>
  </rdf:Description>
  <rdf:Description rdf:about="http://data.europa.eu/a4g/ontology#isReturnable">
    <rdfs:isDefinedBy rdf:resource="http://data.europa.eu/a4g/ontology#ful"/>
  </rdf:Description>
  <rdf:Description rdf:about="http://data.europa.eu/a4g/ontology#isReturnable">
    <skos:prefLabel xml:lang="en">Is returnable</skos:prefLabel>
  </rdf:Description>
  <rdf:Description rdf:about="http://data.europa.eu/a4g/ontology#isReturnableMaterial">
    <rdf:type rdf:resource="http://www.w3.org/2002/07/owl#DatatypeProperty"/>
  </rdf:Description>
  <rdf:Description rdf:about="http://data.europa.eu/a4g/ontology#isReturnableMaterial">
    <rdfs:isDefinedBy rdf:resource="http://data.europa.eu/a4g/ontology#ful"/>
  </rdf:Description>
  <rdf:Description rdf:about="http://data.europa.eu/a4g/ontology#isReturnableMaterial">
    <skos:definition xml:lang="en">Indicates whether the container or part of the container is to be sent back. (epo-ful:AbstractContainer)</skos:definition>
  </rdf:Description>
  <rdf:Description rdf:about="http://data.europa.eu/a4g/ontology#isReturnableMaterial">
    <skos:prefLabel xml:lang="en">Is returnable material</skos:prefLabel>
  </rdf:Description>
  <rdf:Description rdf:about="http://data.europa.eu/a4g/ontology#isReturnableMaterial">
    <skos:historyNote xml:lang="en">WG Approval 21/05/2024</skos:historyNote>
  </rdf:Description>
  <rdf:Description rdf:about="http://data.europa.eu/a4g/ontology#isSpecificToDespatchLine">
    <rdf:type rdf:resource="http://www.w3.org/2002/07/owl#ObjectProperty"/>
  </rdf:Description>
  <rdf:Description rdf:about="http://data.europa.eu/a4g/ontology#isSpecificToDespatchLine">
    <rdfs:isDefinedBy rdf:resource="http://data.europa.eu/a4g/ontology#ful"/>
  </rdf:Description>
  <rdf:Description rdf:about="http://data.europa.eu/a4g/ontology#isSpecificToDespatchLine">
    <skos:definition xml:lang="en">Information that is particular to a Despatch Line. (epo-ful:ShipmentInformation -&gt; epo-ful:DespatchLine (+epo-ful:isSpecificToDespatchLine))</skos:definition>
  </rdf:Description>
  <rdf:Description rdf:about="http://data.europa.eu/a4g/ontology#isSpecificToDespatchLine">
    <skos:prefLabel xml:lang="en">Is specific to despatch line</skos:prefLabel>
  </rdf:Description>
  <rdf:Description rdf:about="http://data.europa.eu/a4g/ontology#isSpecificToDespatchLine">
    <skos:historyNote xml:lang="en">WG Approval 25/06/2024</skos:historyNote>
  </rdf:Description>
  <rdf:Description rdf:about="http://data.europa.eu/a4g/ontology#isSubmittedForDespatchAdvice">
    <rdf:type rdf:resource="http://www.w3.org/2002/07/owl#ObjectProperty"/>
  </rdf:Description>
  <rdf:Description rdf:about="http://data.europa.eu/a4g/ontology#isSubmittedForDespatchAdvice">
    <rdfs:isDefinedBy rdf:resource="http://data.europa.eu/a4g/ontology#ful"/>
  </rdf:Description>
  <rdf:Description rdf:about="http://data.europa.eu/a4g/ontology#isSubmittedForDespatchAdvice">
    <skos:definition xml:lang="en">Additional information: In PEPPOL (https://test-docs.peppol.eu/logistics/qa/codelist/ReceiptAdviceTypeCode/) this predicate is used for option D - Response to the Advanced Despatch Advice document. (epo-ful:ReceiptAdvice -&gt; epo-ful:DespatchAdvice (+epo-ful:isSubmittedForDespatchAdvice))</skos:definition>
  </rdf:Description>
  <rdf:Description rdf:about="http://data.europa.eu/a4g/ontology#isSubmittedForDespatchAdvice">
    <skos:prefLabel xml:lang="en">Is submitted for despatch advice</skos:prefLabel>
  </rdf:Description>
  <rdf:Description rdf:about="http://data.europa.eu/a4g/ontology#isSubmittedForDespatchLine">
    <rdf:type rdf:resource="http://www.w3.org/2002/07/owl#ObjectProperty"/>
  </rdf:Description>
  <rdf:Description rdf:about="http://data.europa.eu/a4g/ontology#isSubmittedForDespatchLine">
    <rdfs:isDefinedBy rdf:resource="http://data.europa.eu/a4g/ontology#ful"/>
  </rdf:Description>
  <rdf:Description rdf:about="http://data.europa.eu/a4g/ontology#isSubmittedForDespatchLine">
    <skos:prefLabel xml:lang="en">Is submitted for despatch line</skos:prefLabel>
  </rdf:Description>
  <rdf:Description rdf:about="http://data.europa.eu/a4g/ontology#isSubmittedForShipment">
    <rdf:type rdf:resource="http://www.w3.org/2002/07/owl#ObjectProperty"/>
  </rdf:Description>
  <rdf:Description rdf:about="http://data.europa.eu/a4g/ontology#isSubmittedForShipment">
    <rdfs:isDefinedBy rdf:resource="http://data.europa.eu/a4g/ontology#ful"/>
  </rdf:Description>
  <rdf:Description rdf:about="http://data.europa.eu/a4g/ontology#isSubmittedForShipment">
    <skos:prefLabel xml:lang="en">Is submitted for shipment</skos:prefLabel>
  </rdf:Description>
  <rdf:Description rdf:about="http://data.europa.eu/a4g/ontology#playedBy">
    <rdf:type rdf:resource="http://www.w3.org/2002/07/owl#ObjectProperty"/>
  </rdf:Description>
  <rdf:Description rdf:about="http://data.europa.eu/a4g/ontology#playedBy">
    <rdfs:isDefinedBy rdf:resource="http://data.europa.eu/a4g/ontology#ful"/>
  </rdf:Description>
  <rdf:Description rdf:about="http://data.europa.eu/a4g/ontology#playedBy">
    <skos:prefLabel xml:lang="en">Played by</skos:prefLabel>
  </rdf:Description>
  <rdf:Description rdf:about="http://data.europa.eu/a4g/ontology#refersToConsignment">
    <rdf:type rdf:resource="http://www.w3.org/2002/07/owl#ObjectProperty"/>
  </rdf:Description>
  <rdf:Description rdf:about="http://data.europa.eu/a4g/ontology#refersToConsignment">
    <rdfs:isDefinedBy rdf:resource="http://data.europa.eu/a4g/ontology#ful"/>
  </rdf:Description>
  <rdf:Description rdf:about="http://data.europa.eu/a4g/ontology#refersToConsignment">
    <skos:definition xml:lang="en">Reference to a Consignment. (epo-ful:DespatchAdvice -&gt; epo-ful:Consignment (+epo-ful:refersToConsignment))</skos:definition>
  </rdf:Description>
  <rdf:Description rdf:about="http://data.europa.eu/a4g/ontology#refersToConsignment">
    <skos:prefLabel xml:lang="en">Refers to consignment</skos:prefLabel>
  </rdf:Description>
  <rdf:Description rdf:about="http://data.europa.eu/a4g/ontology#refersToConsignment">
    <skos:historyNote xml:lang="en">WG Approval 25/06/2024</skos:historyNote>
  </rdf:Description>
  <rdf:Description rdf:about="http://data.europa.eu/a4g/ontology#refersToDeliveryInformation">
    <rdf:type rdf:resource="http://www.w3.org/2002/07/owl#ObjectProperty"/>
  </rdf:Description>
  <rdf:Description rdf:about="http://data.europa.eu/a4g/ontology#refersToDeliveryInformation">
    <rdfs:isDefinedBy rdf:resource="http://data.europa.eu/a4g/ontology#ful"/>
  </rdf:Description>
  <rdf:Description rdf:about="http://data.europa.eu/a4g/ontology#refersToDeliveryInformation">
    <skos:definition xml:lang="en">Reference to a Delivery Information. (epo-ful:ShipmentInformation -&gt; epo-ord:DeliveryInformation (+epo-ful:refersToDeliveryInformation))</skos:definition>
  </rdf:Description>
  <rdf:Description rdf:about="http://data.europa.eu/a4g/ontology#refersToDeliveryInformation">
    <skos:prefLabel xml:lang="en">Refers to delivery information</skos:prefLabel>
  </rdf:Description>
  <rdf:Description rdf:about="http://data.europa.eu/a4g/ontology#refersToDeliveryInformation">
    <skos:historyNote xml:lang="en">WG Approval 25/06/2024</skos:historyNote>
  </rdf:Description>
  <rdf:Description rdf:about="http://data.europa.eu/a4g/ontology#refersToDespatchAdvice">
    <rdf:type rdf:resource="http://www.w3.org/2002/07/owl#ObjectProperty"/>
  </rdf:Description>
  <rdf:Description rdf:about="http://data.europa.eu/a4g/ontology#refersToDespatchAdvice">
    <rdfs:isDefinedBy rdf:resource="http://data.europa.eu/a4g/ontology#ful"/>
  </rdf:Description>
  <rdf:Description rdf:about="http://data.europa.eu/a4g/ontology#refersToDespatchAdvice">
    <skos:prefLabel xml:lang="en">Refers to despatch advice</skos:prefLabel>
  </rdf:Description>
  <rdf:Description rdf:about="http://data.europa.eu/a4g/ontology#refersToDespatchLine">
    <rdf:type rdf:resource="http://www.w3.org/2002/07/owl#ObjectProperty"/>
  </rdf:Description>
  <rdf:Description rdf:about="http://data.europa.eu/a4g/ontology#refersToDespatchLine">
    <rdfs:isDefinedBy rdf:resource="http://data.europa.eu/a4g/ontology#ful"/>
  </rdf:Description>
  <rdf:Description rdf:about="http://data.europa.eu/a4g/ontology#refersToDespatchLine">
    <skos:definition xml:lang="en">Reference to a Despatch Line. (epo-ful:GoodsItem -&gt; epo-ful:DespatchLine (+epo-ful:refersToDespatchLine))</skos:definition>
  </rdf:Description>
  <rdf:Description rdf:about="http://data.europa.eu/a4g/ontology#refersToDespatchLine">
    <skos:prefLabel xml:lang="en">Refers to despatch line</skos:prefLabel>
  </rdf:Description>
  <rdf:Description rdf:about="http://data.europa.eu/a4g/ontology#refersToDespatchLine">
    <skos:historyNote xml:lang="en">WG Approval 25/06/2024</skos:historyNote>
  </rdf:Description>
  <rdf:Description rdf:about="http://data.europa.eu/a4g/ontology#refersToOrder">
    <rdf:type rdf:resource="http://www.w3.org/2002/07/owl#ObjectProperty"/>
  </rdf:Description>
  <rdf:Description rdf:about="http://data.europa.eu/a4g/ontology#refersToOrder">
    <rdfs:isDefinedBy rdf:resource="http://data.europa.eu/a4g/ontology#ful"/>
  </rdf:Description>
  <rdf:Description rdf:about="http://data.europa.eu/a4g/ontology#refersToOrder">
    <skos:definition xml:lang="en">Reference to an Order. (epo-ful:DespatchAdvice -&gt; epo-ord:Order (+epo-ful:refersToOrder))</skos:definition>
  </rdf:Description>
  <rdf:Description rdf:about="http://data.europa.eu/a4g/ontology#refersToOrder">
    <skos:prefLabel xml:lang="en">Refers to order</skos:prefLabel>
  </rdf:Description>
  <rdf:Description rdf:about="http://data.europa.eu/a4g/ontology#refersToOrder">
    <skos:historyNote xml:lang="en">WG Approval 25/06/2024</skos:historyNote>
  </rdf:Description>
  <rdf:Description rdf:about="http://data.europa.eu/a4g/ontology#refersToOrderLine">
    <rdf:type rdf:resource="http://www.w3.org/2002/07/owl#ObjectProperty"/>
  </rdf:Description>
  <rdf:Description rdf:about="http://data.europa.eu/a4g/ontology#refersToOrderLine">
    <rdfs:isDefinedBy rdf:resource="http://data.europa.eu/a4g/ontology#ful"/>
  </rdf:Description>
  <rdf:Description rdf:about="http://data.europa.eu/a4g/ontology#refersToOrderLine">
    <skos:definition xml:lang="en">Reference to an Order Line. (epo-ful:DespatchLine -&gt; epo-ord:OrderLine (+epo-ful:refersToOrderLine))</skos:definition>
  </rdf:Description>
  <rdf:Description rdf:about="http://data.europa.eu/a4g/ontology#refersToOrderLine">
    <skos:prefLabel xml:lang="en">Refers to order line</skos:prefLabel>
  </rdf:Description>
  <rdf:Description rdf:about="http://data.europa.eu/a4g/ontology#refersToOrderLine">
    <skos:historyNote xml:lang="en">WG Approval 25/06/2024</skos:historyNote>
  </rdf:Description>
  <rdf:Description rdf:about="http://data.europa.eu/a4g/ontology#refersToReceiptAdvice">
    <rdf:type rdf:resource="http://www.w3.org/2002/07/owl#ObjectProperty"/>
  </rdf:Description>
  <rdf:Description rdf:about="http://data.europa.eu/a4g/ontology#refersToReceiptAdvice">
    <rdfs:isDefinedBy rdf:resource="http://data.europa.eu/a4g/ontology#ful"/>
  </rdf:Description>
  <rdf:Description rdf:about="http://data.europa.eu/a4g/ontology#refersToReceiptAdvice">
    <skos:prefLabel xml:lang="en">Refers to receipt advice</skos:prefLabel>
  </rdf:Description>
  <rdf:Description rdf:about="http://data.europa.eu/a4g/ontology#refersToShipmentAgreement">
    <rdf:type rdf:resource="http://www.w3.org/2002/07/owl#ObjectProperty"/>
  </rdf:Description>
  <rdf:Description rdf:about="http://data.europa.eu/a4g/ontology#refersToShipmentAgreement">
    <rdfs:isDefinedBy rdf:resource="http://data.europa.eu/a4g/ontology#ful"/>
  </rdf:Description>
  <rdf:Description rdf:about="http://data.europa.eu/a4g/ontology#refersToShipmentAgreement">
    <skos:definition xml:lang="en">Reference to a Shipment Agreement. (epo-ful:DespatchAdvice -&gt; epo-ful:ShipmentAgreement (+epo-ful:refersToShipmentAgreement))</skos:definition>
  </rdf:Description>
  <rdf:Description rdf:about="http://data.europa.eu/a4g/ontology#refersToShipmentAgreement">
    <skos:prefLabel xml:lang="en">Refers to shipment agreement</skos:prefLabel>
  </rdf:Description>
  <rdf:Description rdf:about="http://data.europa.eu/a4g/ontology#refersToShipmentAgreement">
    <skos:historyNote xml:lang="en">WG Approval 25/06/2024</skos:historyNote>
  </rdf:Description>
  <rdf:Description rdf:about="http://data.europa.eu/a4g/ontology#specifiesBuyer">
    <rdf:type rdf:resource="http://www.w3.org/2002/07/owl#ObjectProperty"/>
  </rdf:Description>
  <rdf:Description rdf:about="http://data.europa.eu/a4g/ontology#specifiesBuyer">
    <rdfs:isDefinedBy rdf:resource="http://data.europa.eu/a4g/ontology#ful"/>
  </rdf:Description>
  <rdf:Description rdf:about="http://data.europa.eu/a4g/ontology#specifiesBuyer">
    <skos:prefLabel xml:lang="en">Specifies buyer</skos:prefLabel>
  </rdf:Description>
  <rdf:Description rdf:about="http://data.europa.eu/a4g/ontology#specifiesCarrier">
    <rdf:type rdf:resource="http://www.w3.org/2002/07/owl#ObjectProperty"/>
  </rdf:Description>
  <rdf:Description rdf:about="http://data.europa.eu/a4g/ontology#specifiesCarrier">
    <rdfs:isDefinedBy rdf:resource="http://data.europa.eu/a4g/ontology#ful"/>
  </rdf:Description>
  <rdf:Description rdf:about="http://data.europa.eu/a4g/ontology#specifiesCarrier">
    <skos:definition xml:lang="en">Relation indicating that the instance of the concept involves the Carrier. (epo-ful:ShipmentStage -&gt; epo-ful:Carrier (+epo:specifiesCarrier))</skos:definition>
  </rdf:Description>
  <rdf:Description rdf:about="http://data.europa.eu/a4g/ontology#specifiesCarrier">
    <skos:prefLabel xml:lang="en">Specifies carrier</skos:prefLabel>
  </rdf:Description>
  <rdf:Description rdf:about="http://data.europa.eu/a4g/ontology#specifiesCarrier">
    <skos:historyNote xml:lang="en">WG Approval 25/06/2024</skos:historyNote>
  </rdf:Description>
  <rdf:Description rdf:about="http://data.europa.eu/a4g/ontology#specifiesConsignee">
    <rdf:type rdf:resource="http://www.w3.org/2002/07/owl#ObjectProperty"/>
  </rdf:Description>
  <rdf:Description rdf:about="http://data.europa.eu/a4g/ontology#specifiesConsignee">
    <rdfs:isDefinedBy rdf:resource="http://data.europa.eu/a4g/ontology#ful"/>
  </rdf:Description>
  <rdf:Description rdf:about="http://data.europa.eu/a4g/ontology#specifiesConsignee">
    <skos:definition xml:lang="en">Relation indicating that the instance of the concept involves the Consignee. (epo-ful:DespatchAdvice -&gt; epo-ord:Consignee (+epo-ful:specifiesConsignee))</skos:definition>
  </rdf:Description>
  <rdf:Description rdf:about="http://data.europa.eu/a4g/ontology#specifiesConsignee">
    <skos:prefLabel xml:lang="en">Specifies consignee</skos:prefLabel>
  </rdf:Description>
  <rdf:Description rdf:about="http://data.europa.eu/a4g/ontology#specifiesConsignee">
    <skos:historyNote xml:lang="en">WG Approval 25/06/2024</skos:historyNote>
  </rdf:Description>
  <rdf:Description rdf:about="http://data.europa.eu/a4g/ontology#specifiesDespatcher">
    <rdf:type rdf:resource="http://www.w3.org/2002/07/owl#ObjectProperty"/>
  </rdf:Description>
  <rdf:Description rdf:about="http://data.europa.eu/a4g/ontology#specifiesDespatcher">
    <rdfs:isDefinedBy rdf:resource="http://data.europa.eu/a4g/ontology#ful"/>
  </rdf:Description>
  <rdf:Description rdf:about="http://data.europa.eu/a4g/ontology#specifiesDespatcher">
    <skos:definition xml:lang="en">Relation indicating that the instance of the concept involves the Despatcher. (epo-ful:DespatchAdvice -&gt; epo-ful:Despatcher (+epo-ful:specifiesDespatcher))</skos:definition>
  </rdf:Description>
  <rdf:Description rdf:about="http://data.europa.eu/a4g/ontology#specifiesDespatcher">
    <skos:definition xml:lang="en">Relation indicating that the instance of the concept involves the Despatcher. (epo-ord:Order -&gt; epo-ful:Despatcher (+epo:specifiesDespatcher))</skos:definition>
  </rdf:Description>
  <rdf:Description rdf:about="http://data.europa.eu/a4g/ontology#specifiesDespatcher">
    <skos:prefLabel xml:lang="en">Specifies despatcher</skos:prefLabel>
  </rdf:Description>
  <rdf:Description rdf:about="http://data.europa.eu/a4g/ontology#specifiesDespatcher">
    <skos:historyNote xml:lang="en">WG Approval 25/06/2024</skos:historyNote>
  </rdf:Description>
  <rdf:Description rdf:about="http://data.europa.eu/a4g/ontology#specifiesFreightForwarder">
    <rdf:type rdf:resource="http://www.w3.org/2002/07/owl#ObjectProperty"/>
  </rdf:Description>
  <rdf:Description rdf:about="http://data.europa.eu/a4g/ontology#specifiesFreightForwarder">
    <rdfs:isDefinedBy rdf:resource="http://data.europa.eu/a4g/ontology#ful"/>
  </rdf:Description>
  <rdf:Description rdf:about="http://data.europa.eu/a4g/ontology#specifiesFreightForwarder">
    <skos:definition xml:lang="en">Relation indicating that the instance of the concept involves the Freight Forwarder. (epo-ful:Consignment -&gt; epo-ful:FreightForwarder (+epo:specifiesFreightForwarder))</skos:definition>
  </rdf:Description>
  <rdf:Description rdf:about="http://data.europa.eu/a4g/ontology#specifiesFreightForwarder">
    <skos:prefLabel xml:lang="en">Specifies freight forwarder</skos:prefLabel>
  </rdf:Description>
  <rdf:Description rdf:about="http://data.europa.eu/a4g/ontology#specifiesFreightForwarder">
    <skos:historyNote xml:lang="en">WG Approval 25/06/2024</skos:historyNote>
  </rdf:Description>
  <rdf:Description rdf:about="http://data.europa.eu/a4g/ontology#specifiesNotificationReceiver">
    <rdf:type rdf:resource="http://www.w3.org/2002/07/owl#ObjectProperty"/>
  </rdf:Description>
  <rdf:Description rdf:about="http://data.europa.eu/a4g/ontology#specifiesNotificationReceiver">
    <rdfs:isDefinedBy rdf:resource="http://data.europa.eu/a4g/ontology#ful"/>
  </rdf:Description>
  <rdf:Description rdf:about="http://data.europa.eu/a4g/ontology#specifiesNotificationReceiver">
    <skos:definition xml:lang="en">c (epo-ful:Consignment -&gt; epo-ful:NotificationReceiver (+epo:specifiesNotificationReceiver))</skos:definition>
  </rdf:Description>
  <rdf:Description rdf:about="http://data.europa.eu/a4g/ontology#specifiesNotificationReceiver">
    <skos:prefLabel xml:lang="en">Specifies notification receiver</skos:prefLabel>
  </rdf:Description>
  <rdf:Description rdf:about="http://data.europa.eu/a4g/ontology#specifiesNotifier">
    <rdf:type rdf:resource="http://www.w3.org/2002/07/owl#ObjectProperty"/>
  </rdf:Description>
  <rdf:Description rdf:about="http://data.europa.eu/a4g/ontology#specifiesNotifier">
    <rdfs:isDefinedBy rdf:resource="http://data.europa.eu/a4g/ontology#ful"/>
  </rdf:Description>
  <rdf:Description rdf:about="http://data.europa.eu/a4g/ontology#specifiesNotifier">
    <skos:prefLabel xml:lang="en">Specifies notifier</skos:prefLabel>
  </rdf:Description>
  <rdf:Description rdf:about="http://data.europa.eu/a4g/ontology#specifiesOriginator">
    <rdf:type rdf:resource="http://www.w3.org/2002/07/owl#ObjectProperty"/>
  </rdf:Description>
  <rdf:Description rdf:about="http://data.europa.eu/a4g/ontology#specifiesOriginator">
    <rdfs:isDefinedBy rdf:resource="http://data.europa.eu/a4g/ontology#ful"/>
  </rdf:Description>
  <rdf:Description rdf:about="http://data.europa.eu/a4g/ontology#specifiesOriginator">
    <skos:definition xml:lang="en">Relation indicating that the instance of the concept involves the Originator. (epo-ful:DespatchAdvice -&gt; epo-ord:Originator (+epo-ful:specifiesOriginator))</skos:definition>
  </rdf:Description>
  <rdf:Description rdf:about="http://data.europa.eu/a4g/ontology#specifiesOriginator">
    <skos:prefLabel xml:lang="en">Specifies originator</skos:prefLabel>
  </rdf:Description>
  <rdf:Description rdf:about="http://data.europa.eu/a4g/ontology#specifiesOriginator">
    <skos:historyNote xml:lang="en">WG Approval 25/06/2024</skos:historyNote>
  </rdf:Description>
  <rdf:Description rdf:about="http://data.europa.eu/a4g/ontology#specifiesPlaceOfDespatch">
    <rdf:type rdf:resource="http://www.w3.org/2002/07/owl#ObjectProperty"/>
  </rdf:Description>
  <rdf:Description rdf:about="http://data.europa.eu/a4g/ontology#specifiesPlaceOfDespatch">
    <rdfs:isDefinedBy rdf:resource="http://data.europa.eu/a4g/ontology#ful"/>
  </rdf:Description>
  <rdf:Description rdf:about="http://data.europa.eu/a4g/ontology#specifiesPlaceOfDespatch">
    <skos:definition xml:lang="en">Relation indicating the Location of the Despatch of the Goods Items to be delivered. (epo-ful:ShipmentInformation -&gt; dct:Location (+epo-ful:specifiesPlaceOfDespatch))</skos:definition>
  </rdf:Description>
  <rdf:Description rdf:about="http://data.europa.eu/a4g/ontology#specifiesPlaceOfDespatch">
    <skos:prefLabel xml:lang="en">Specifies place of despatch</skos:prefLabel>
  </rdf:Description>
  <rdf:Description rdf:about="http://data.europa.eu/a4g/ontology#specifiesPlaceOfDespatch">
    <skos:historyNote xml:lang="en">WG Approval 25/06/2024</skos:historyNote>
  </rdf:Description>
  <rdf:Description rdf:about="http://data.europa.eu/a4g/ontology#specifiesSeller">
    <rdf:type rdf:resource="http://www.w3.org/2002/07/owl#ObjectProperty"/>
  </rdf:Description>
  <rdf:Description rdf:about="http://data.europa.eu/a4g/ontology#specifiesSeller">
    <rdfs:isDefinedBy rdf:resource="http://data.europa.eu/a4g/ontology#ful"/>
  </rdf:Description>
  <rdf:Description rdf:about="http://data.europa.eu/a4g/ontology#specifiesSeller">
    <skos:prefLabel xml:lang="en">Specifies seller</skos:prefLabel>
  </rdf:Description>
  <rdf:Description rdf:about="http://data.europa.eu/a4g/ontology#specifiesShipment">
    <rdf:type rdf:resource="http://www.w3.org/2002/07/owl#ObjectProperty"/>
  </rdf:Description>
  <rdf:Description rdf:about="http://data.europa.eu/a4g/ontology#specifiesShipment">
    <rdfs:isDefinedBy rdf:resource="http://data.europa.eu/a4g/ontology#ful"/>
  </rdf:Description>
  <rdf:Description rdf:about="http://data.europa.eu/a4g/ontology#specifiesShipment">
    <skos:prefLabel xml:lang="en">Specifies shipment</skos:prefLabel>
  </rdf:Description>
  <rdf:Description rdf:about="http://data.europa.eu/a4g/ontology#specifiesTransportHandlingUnits">
    <rdf:type rdf:resource="http://www.w3.org/2002/07/owl#ObjectProperty"/>
  </rdf:Description>
  <rdf:Description rdf:about="http://data.europa.eu/a4g/ontology#specifiesTransportHandlingUnits">
    <rdfs:isDefinedBy rdf:resource="http://data.europa.eu/a4g/ontology#ful"/>
  </rdf:Description>
  <rdf:Description rdf:about="http://data.europa.eu/a4g/ontology#specifiesTransportHandlingUnits">
    <skos:definition xml:lang="en">Relation indicating the use of a Transport Handling Unit. (epo-ful:DespatchAdvice -&gt; epo-ful:TransportHandlingUnit (+epo-ful:specifiesTransportHandlingUnits))</skos:definition>
  </rdf:Description>
  <rdf:Description rdf:about="http://data.europa.eu/a4g/ontology#specifiesTransportHandlingUnits">
    <skos:prefLabel xml:lang="en">Specifies transport handling units</skos:prefLabel>
  </rdf:Description>
  <rdf:Description rdf:about="http://data.europa.eu/a4g/ontology#specifiesTransportHandlingUnits">
    <skos:historyNote xml:lang="en">WG Approval 25/06/2024</skos:historyNote>
  </rdf:Description>
  <rdf:Description rdf:about="http://data.europa.eu/a4g/ontology#transportsItemFrom">
    <rdf:type rdf:resource="http://www.w3.org/2002/07/owl#ObjectProperty"/>
  </rdf:Description>
  <rdf:Description rdf:about="http://data.europa.eu/a4g/ontology#transportsItemFrom">
    <rdfs:isDefinedBy rdf:resource="http://data.europa.eu/a4g/ontology#ful"/>
  </rdf:Description>
  <rdf:Description rdf:about="http://data.europa.eu/a4g/ontology#transportsItemFrom">
    <skos:prefLabel xml:lang="en">Transports item from</skos:prefLabel>
  </rdf:Description>
  <rdf:Description rdf:about="http://data.europa.eu/a4g/ontology#usesTransportEquipment">
    <rdf:type rdf:resource="http://www.w3.org/2002/07/owl#ObjectProperty"/>
  </rdf:Description>
  <rdf:Description rdf:about="http://data.europa.eu/a4g/ontology#usesTransportEquipment">
    <rdfs:isDefinedBy rdf:resource="http://data.europa.eu/a4g/ontology#ful"/>
  </rdf:Description>
  <rdf:Description rdf:about="http://data.europa.eu/a4g/ontology#usesTransportEquipment">
    <skos:definition xml:lang="en">Relation indicating that a Transport Handling Unit utilises a Transport Equipment. (epo-ful:TransportHandlingUnit -&gt; epo-ful:TransportEquipment (+epo-ful:usesTransportEquipment))</skos:definition>
  </rdf:Description>
  <rdf:Description rdf:about="http://data.europa.eu/a4g/ontology#usesTransportEquipment">
    <skos:prefLabel xml:lang="en">Uses transport equipment</skos:prefLabel>
  </rdf:Description>
  <rdf:Description rdf:about="http://data.europa.eu/a4g/ontology#usesTransportEquipment">
    <skos:historyNote xml:lang="en">WG Approval 02/07/2024</skos:historyNote>
  </rdf:Description>
  <rdf:Description rdf:about="http://data.europa.eu/a4g/ontology#usesTransportMeans">
    <rdf:type rdf:resource="http://www.w3.org/2002/07/owl#ObjectProperty"/>
  </rdf:Description>
  <rdf:Description rdf:about="http://data.europa.eu/a4g/ontology#usesTransportMeans">
    <rdfs:isDefinedBy rdf:resource="http://data.europa.eu/a4g/ontology#ful"/>
  </rdf:Description>
  <rdf:Description rdf:about="http://data.europa.eu/a4g/ontology#usesTransportMeans">
    <skos:definition xml:lang="en">Relation indicating that a Shipment Stage utilises a Transport Means. (epo-ful:ShipmentStage -&gt; epo-ful:TransportMeans (+epo-ful:usesTransportMeans))</skos:definition>
  </rdf:Description>
  <rdf:Description rdf:about="http://data.europa.eu/a4g/ontology#usesTransportMeans">
    <skos:prefLabel xml:lang="en">Uses transport means</skos:prefLabel>
  </rdf:Description>
  <rdf:Description rdf:about="http://data.europa.eu/a4g/ontology#usesTransportMeans">
    <skos:historyNote xml:lang="en">WG Approval 02/07/2024</skos:historyNote>
  </rdf:Description>
</rdf:RDF>
