@prefix : <http://data.europa.eu/a4g/ontology#> .
@prefix cc: <http://creativecommons.org/ns#> .
@prefix dc: <http://purl.org/dc/elements/1.1/> .
@prefix dcterms: <http://purl.org/dc/terms/> .
@prefix foaf: <http://xmlns.com/foaf/0.1/> .
@prefix owl: <http://www.w3.org/2002/07/owl#> .
@prefix rdf: <http://www.w3.org/1999/02/22-rdf-syntax-ns#> .
@prefix rdfs: <http://www.w3.org/2000/01/rdf-schema#> .
@prefix schema: <https://schema.org/> .
@prefix skos: <http://www.w3.org/2004/02/skos/core#> .
@prefix vann: <http://purl.org/vocab/vann/> .
@prefix xsd: <http://www.w3.org/2001/XMLSchema#> .

:Batch a owl:Class ;
    rdfs:label "Batch"@en ;
    rdfs:comment """A production Lot in which the Item instances were produced. 

WG Acceptance 10/03/2022
"""@en ;
    rdfs:isDefinedBy <http://data.europa.eu/a4g/ontology> ;
    skos:definition """A production Lot in which the Item instances were produced. 

WG Acceptance 10/03/2022
"""@en ;
    skos:prefLabel "Batch"@en .

:Brand a owl:Class ;
    rdfs:label "Brand"@en ;
    rdfs:comment """Name given by an organisation to its product or service, or range of products or services. 

Additional information:
Brand name allows economic operators to distinctively describe an item in their eCatalogue. This may be different from the "item name".

WG acceptance 10/03/2022
"""@en ;
    rdfs:isDefinedBy <http://data.europa.eu/a4g/ontology> ;
    skos:definition """Name given by an organisation to its product or service, or range of products or services. 

Additional information:
Brand name allows economic operators to distinctively describe an item in their eCatalogue. This may be different from the "item name".

WG acceptance 10/03/2022
"""@en ;
    skos:prefLabel "Brand"@en .

:CatalogueFragment a owl:Class ;
    rdfs:label "Catalogue fragment"@en ;
    rdfs:comment """A part of the Catalogue.

Additional Information:
The Catalogue fragment generally represents a difference between two Catalogue versions, but there may be other use cases."""@en ;
    rdfs:isDefinedBy <http://data.europa.eu/a4g/ontology> ;
    rdfs:subClassOf :Catalogue ;
    skos:definition """A part of the Catalogue.

Additional Information:
The Catalogue fragment generally represents a difference between two Catalogue versions, but there may be other use cases."""@en ;
    skos:prefLabel "Catalogue fragment"@en .

:CatalogueLine a owl:Class ;
    rdfs:label "Catalogue line"@en ;
    rdfs:comment """Aggregated information about the Terms and specifications for procuring an Item.


Details about an Item, like Prices, packaging, discounts, special promotions, etc.


TC 440:

Detailed information of an Item, Price and its composition in a Catalogue.

Composition: e.g. information referring to its description, how to order it, what it is made of, properties, delivery conditions, etc.





"""@en ;
    rdfs:isDefinedBy <http://data.europa.eu/a4g/ontology> ;
    rdfs:subClassOf :Line ;
    skos:definition """Aggregated information about the Terms and specifications for procuring an Item.


Details about an Item, like Prices, packaging, discounts, special promotions, etc.


TC 440:

Detailed information of an Item, Price and its composition in a Catalogue.

Composition: e.g. information referring to its description, how to order it, what it is made of, properties, delivery conditions, etc.





"""@en ;
    skos:prefLabel "Catalogue line"@en .

:Certificate a owl:Class ;
    rdfs:label "Certificate"@en ;
    rdfs:comment """Proof of conformance of the instance of the concept to a defined set of criteria. 

Additional Information:
Certificates provide assurance of credibility, trust, and transparency in the procurement process. 

WG approval 16/05/2023
"""@en ;
    rdfs:isDefinedBy <http://data.europa.eu/a4g/ontology> ;
    skos:definition """Proof of conformance of the instance of the concept to a defined set of criteria. 

Additional Information:
Certificates provide assurance of credibility, trust, and transparency in the procurement process. 

WG approval 16/05/2023
"""@en ;
    skos:prefLabel "Certificate"@en .

:CertificationLabel a owl:Class ;
    rdfs:label "Certification label"@en ;
    rdfs:comment """Concept that stands for a set of norms, expectations, standards and policies.

Additional Information:
Such standards may relate to social, ethical and quality etc.

WG approval 26/07/2022
"""@en ;
    rdfs:isDefinedBy <http://data.europa.eu/a4g/ontology> ;
    skos:definition """Concept that stands for a set of norms, expectations, standards and policies.

Additional Information:
Such standards may relate to social, ethical and quality etc.

WG approval 26/07/2022
"""@en ;
    skos:prefLabel "Certification label"@en .

:Certifier a owl:Class ;
    rdfs:label "Certifier"@en ;
    rdfs:comment """The role of an agent who issues a certificate. 

Additional Information:
The certifier is responsible for verifying and confirming the conformance of the instance of the concept to a defined set of criteria.

WG approval 16/05/2023"""@en ;
    rdfs:isDefinedBy <http://data.europa.eu/a4g/ontology> ;
    skos:definition """The role of an agent who issues a certificate. 

Additional Information:
The certifier is responsible for verifying and confirming the conformance of the instance of the concept to a defined set of criteria.

WG approval 16/05/2023"""@en ;
    skos:prefLabel "Certifier"@en .

:ChargeInformation a owl:Class ;
    rdfs:label "Charge information"@en ;
    rdfs:comment """Information about tax, fee or duty imposed.

Additional Information:
Charge category indicates the nature of the tax/duty/fee, for example VAT, CAR, etc.
Charge category modifier may be used in case different levels, exemptions or other modifications apply.
The charge can be fixed or relative to the price.

WG approval 16/05/2023"""@en ;
    rdfs:isDefinedBy <http://data.europa.eu/a4g/ontology> ;
    skos:definition """Information about tax, fee or duty imposed.

Additional Information:
Charge category indicates the nature of the tax/duty/fee, for example VAT, CAR, etc.
Charge category modifier may be used in case different levels, exemptions or other modifications apply.
The charge can be fixed or relative to the price.

WG approval 16/05/2023"""@en ;
    skos:prefLabel "Charge information"@en .

:InformationHub a owl:Class ;
    rdfs:label "Information hub"@en ;
    rdfs:comment """Grouping of data that may be associated to various concepts.

Additional Information:
For example, AllowanceChargeInformation may be associated to the Order or the Catalogue (either at the Line level or at the Document level), amongst others.

WG approval 16/05/2023"""@en ;
    rdfs:isDefinedBy <http://data.europa.eu/a4g/ontology> ;
    skos:definition """Grouping of data that may be associated to various concepts.

Additional Information:
For example, AllowanceChargeInformation may be associated to the Order or the Catalogue (either at the Line level or at the Document level), amongst others.

WG approval 16/05/2023"""@en ;
    skos:prefLabel "Information hub"@en .

:Item a owl:Class ;
    rdfs:label "Item"@en ;
    rdfs:comment """A product, work, service or any combination of them.

Additional Information:
An Item can be an atomic Thing or a composition of things that together are seen as a unit, e.g. a tetrabrik of milk or an indivisible package of six tetrabriks.

No distinction is provided between services, goods and works to leave room for innovation.

WG approval 30/06/2022"""@en ;
    rdfs:isDefinedBy <http://data.europa.eu/a4g/ontology> ;
    skos:definition """A product, work, service or any combination of them.

Additional Information:
An Item can be an atomic Thing or a composition of things that together are seen as a unit, e.g. a tetrabrik of milk or an indivisible package of six tetrabriks.

No distinction is provided between services, goods and works to leave room for innovation.

WG approval 30/06/2022"""@en ;
    skos:prefLabel "Item"@en .

:ItemModel a owl:Class ;
    rdfs:label "Item model"@en ;
    rdfs:comment """A specific design or version of a product or service.

Additional information:
This class is meant as a reusable reference to the model name rather than as a set of specifications of an Item of this particular model. 

WG acceptance 10/03/2022

"""@en ;
    rdfs:isDefinedBy <http://data.europa.eu/a4g/ontology> ;
    skos:definition """A specific design or version of a product or service.

Additional information:
This class is meant as a reusable reference to the model name rather than as a set of specifications of an Item of this particular model. 

WG acceptance 10/03/2022

"""@en ;
    skos:prefLabel "Item model"@en .

:ItemProperty a owl:Class ;
    rdfs:label "Item property"@en ;
    rdfs:comment """Construct meant to represent the association between an attribute defined in an external classification scheme and the value ascribed to it.

WG approval 26/07/2022"""@en ;
    rdfs:isDefinedBy <http://data.europa.eu/a4g/ontology> ;
    skos:definition """Construct meant to represent the association between an attribute defined in an external classification scheme and the value ascribed to it.

WG approval 26/07/2022"""@en ;
    skos:prefLabel "Item property"@en .

:Manufacturer a owl:Class ;
    rdfs:label "Manufacturer"@en ;
    rdfs:comment """The Producer of goods or provider of services. 

Additional Information:
Also, known as Supplier and Manufacturer.

We do not care who provides these service or products we care with whom Business is done.

PEPPOL - Invoice:
The Supplier is the Legal Person or Organisation who provides a product and/or service.

PEPPOL - Order: The supplier is the legal person or organisation who provides a product or service.
Examples of supplier roles: seller, despatch party, creditor, economic operator.

"""@en ;
    rdfs:isDefinedBy <http://data.europa.eu/a4g/ontology> ;
    skos:definition """The Producer of goods or provider of services. 

Additional Information:
Also, known as Supplier and Manufacturer.

We do not care who provides these service or products we care with whom Business is done.

PEPPOL - Invoice:
The Supplier is the Legal Person or Organisation who provides a product and/or service.

PEPPOL - Order: The supplier is the legal person or organisation who provides a product or service.
Examples of supplier roles: seller, despatch party, creditor, economic operator.

"""@en ;
    skos:prefLabel "Manufacturer"@en .

:Price a owl:Class ;
    rdfs:label "Price"@en ;
    rdfs:comment """Amount of money required or given in exchange for Items.

Additional information:
The Price excludes any charges (such as taxes, duties and fees) and discounts.

WG approval 26/07/2022"""@en ;
    rdfs:isDefinedBy <http://data.europa.eu/a4g/ontology> ;
    skos:definition """Amount of money required or given in exchange for Items.

Additional information:
The Price excludes any charges (such as taxes, duties and fees) and discounts.

WG approval 26/07/2022"""@en ;
    skos:prefLabel "Price"@en .

:ProductSpecification a owl:Class ;
    rdfs:label "Product specification"@en ;
    rdfs:comment """Document providing information about an Item. 

WG approval 07/04/2022

"""@en ;
    rdfs:isDefinedBy <http://data.europa.eu/a4g/ontology> ;
    skos:definition """Document providing information about an Item. 

WG approval 07/04/2022

"""@en ;
    skos:prefLabel "Product specification"@en .

:attestedByLabel a owl:ObjectProperty ;
    rdfs:label "Attested by label"@en ;
    rdfs:comment """Relation indicating which label the certificate is about. 

WG approval 28/07/2022 (epo-cat:Certificate -> epo-cat:CertificationLabel (+epo-cat:attestedByLabel)) """@en ;
    rdfs:isDefinedBy <http://data.europa.eu/a4g/ontology> ;
    skos:definition """Relation indicating which label the certificate is about. 

WG approval 28/07/2022 (epo-cat:Certificate -> epo-cat:CertificationLabel (+epo-cat:attestedByLabel)) """@en ;
    skos:prefLabel "Attested by label"@en .

:comprisesCatalogueLine a owl:ObjectProperty ;
    rdfs:label "Comprises catalogue line"@en ;
    rdfs:isDefinedBy <http://data.europa.eu/a4g/ontology> ;
    skos:prefLabel "Comprises catalogue line"@en .

:describesItem a owl:ObjectProperty ;
    rdfs:label "Describes item"@en ;
    rdfs:isDefinedBy <http://data.europa.eu/a4g/ontology> ;
    skos:prefLabel "Describes item"@en .

:hasAccessoryItem a owl:ObjectProperty ;
    rdfs:label "Has accessory item"@en ;
    rdfs:comment """An additional item that can enhance the original item. 

WG Approval: 19/05/2022
 (epo-cat:Item -> epo-cat:Item (+epo-cat:hasAccessoryItem)) """@en,
        """An item that can be added to another item to enhance it.

WG Approval: 30/06/2022 (epo-cat:Item -> epo-cat:Item (+epo-cat:hasAccessoryItem)) """@en ;
    rdfs:isDefinedBy <http://data.europa.eu/a4g/ontology> ;
    skos:definition """An item that can be added to another item to enhance it.

WG Approval: 30/06/2022 (epo-cat:Item -> epo-cat:Item (+epo-cat:hasAccessoryItem)) """@en ;
    skos:prefLabel "Has accessory item"@en ;
    skos:scopeNote """An additional item that can enhance the original item. 

WG Approval: 19/05/2022
 (epo-cat:Item -> epo-cat:Item (+epo-cat:hasAccessoryItem)) """@en .

:hasActivityCode a owl:ObjectProperty ;
    rdfs:label "Has activity code"@en ;
    rdfs:comment """Code that defines how the line should be applied to an existing eCatalogue.
 (epo-cat:CatalogueFragment -> at-voc-new:activity-code (+epo-cat:hasActivityCode)) """@en ;
    rdfs:isDefinedBy <http://data.europa.eu/a4g/ontology> ;
    skos:definition """Code that defines how the line should be applied to an existing eCatalogue.
 (epo-cat:CatalogueFragment -> at-voc-new:activity-code (+epo-cat:hasActivityCode)) """@en ;
    skos:prefLabel "Has activity code"@en .

:hasAttributeType a rdf:Property ;
    rdfs:label "Has attribute type"@en ;
    rdfs:comment """The property defined in a classification scheme. 

Additional Information:
For example, the following two properties are defined in the ECLASS classification of goods and services: (0173-1#02-AAA026#007) drilling diameter: drilling diameter, (0173-1#02-AAA030#007) flange diameter: flange diameter .


WG approval 28/07/2022 (epo-cat:ItemProperty) """@en ;
    rdfs:isDefinedBy <http://data.europa.eu/a4g/ontology> ;
    skos:definition """The property defined in a classification scheme. 

Additional Information:
For example, the following two properties are defined in the ECLASS classification of goods and services: (0173-1#02-AAA026#007) drilling diameter: drilling diameter, (0173-1#02-AAA030#007) flange diameter: flange diameter .


WG approval 28/07/2022 (epo-cat:ItemProperty) """@en ;
    skos:prefLabel "Has attribute type"@en .

:hasBaseQuantity a owl:ObjectProperty ;
    rdfs:label "Has base quantity"@en ;
    rdfs:comment "The quantity at which the net monetary value applies. (epo-cat:Price -> epo:Quantity (+epo-cat:hasBaseQuantity)) "@en ;
    rdfs:isDefinedBy <http://data.europa.eu/a4g/ontology> ;
    skos:definition "The quantity at which the net monetary value applies. (epo-cat:Price -> epo:Quantity (+epo-cat:hasBaseQuantity)) "@en ;
    skos:prefLabel "Has base quantity"@en .

:hasBatchID a owl:ObjectProperty ;
    rdfs:label "Has batch i d"@en ;
    rdfs:comment """The identifier assigned to a specific batch of the produced Item.
WG Approval 16/05/2023
 (epo-cat:Batch -> adms:Identifier (+epo:hasBatchID)) """@en ;
    rdfs:isDefinedBy <http://data.europa.eu/a4g/ontology> ;
    skos:definition """The identifier assigned to a specific batch of the produced Item.
WG Approval 16/05/2023
 (epo-cat:Batch -> adms:Identifier (+epo:hasBatchID)) """@en ;
    skos:prefLabel "Has batch i d"@en .

:hasBestBeforeDate a owl:DatatypeProperty ;
    rdfs:label "Has best before date"@en ;
    rdfs:comment """The day until which the quality of the item will remain optimal.

WG approval 10/03/2021 (epo-cat:Batch) """@en ;
    rdfs:isDefinedBy <http://data.europa.eu/a4g/ontology> ;
    skos:definition """The day until which the quality of the item will remain optimal.

WG approval 10/03/2021 (epo-cat:Batch) """@en ;
    skos:prefLabel "Has best before date"@en .

:hasBrand a owl:ObjectProperty ;
    rdfs:label "Has brand"@en ;
    rdfs:isDefinedBy <http://data.europa.eu/a4g/ontology> ;
    skos:prefLabel "Has brand"@en .

:hasBuyerItemID a owl:ObjectProperty ;
    rdfs:label "Has buyer item i d"@en ;
    rdfs:comment """This refers to the identifier for the specific instance of the produced concept.
WG Approval 16/05/2023
 (epo-cat:Item -> adms:Identifier (+epo:hasBuyerItemID)) """@en ;
    rdfs:isDefinedBy <http://data.europa.eu/a4g/ontology> ;
    skos:definition """This refers to the identifier for the specific instance of the produced concept.
WG Approval 16/05/2023
 (epo-cat:Item -> adms:Identifier (+epo:hasBuyerItemID)) """@en ;
    skos:prefLabel "Has buyer item i d"@en .

:hasCatalogueLineValidity a owl:ObjectProperty ;
    rdfs:label "Has catalogue line validity"@en ;
    rdfs:isDefinedBy <http://data.europa.eu/a4g/ontology> ;
    skos:prefLabel "Has catalogue line validity"@en .

:hasCertification a owl:ObjectProperty ;
    rdfs:label "Has certification"@en ;
    rdfs:comment """Relation to the proof of conformance.

WG approval 30/05/2023 (foaf:Person -> epo-cat:Certificate (+epo:hasCertification)) Relation to the proof of conformance.

WG approval 30/05/2023 (epo-cat:Item -> epo-cat:Certificate (+epo:hasCertification)) Relation to the proof of conformance.

WG approval 30/05/2023 (org:Organization -> epo-cat:Certificate (+epo:hasCertification)) """@en ;
    rdfs:isDefinedBy <http://data.europa.eu/a4g/ontology> ;
    skos:definition """Relation to the proof of conformance.

WG approval 30/05/2023 (foaf:Person -> epo-cat:Certificate (+epo:hasCertification)) Relation to the proof of conformance.

WG approval 30/05/2023 (epo-cat:Item -> epo-cat:Certificate (+epo:hasCertification)) Relation to the proof of conformance.

WG approval 30/05/2023 (org:Organization -> epo-cat:Certificate (+epo:hasCertification)) """@en ;
    skos:prefLabel "Has certification"@en .

:hasCertificationNumber a rdf:Property ;
    rdfs:label "Has certification number"@en ;
    rdfs:comment """The unique identifier of the certificate.

WG approval 26/07/2022 (epo-cat:Certificate) """@en ;
    rdfs:isDefinedBy <http://data.europa.eu/a4g/ontology> ;
    skos:definition """The unique identifier of the certificate.

WG approval 26/07/2022 (epo-cat:Certificate) """@en ;
    skos:prefLabel "Has certification number"@en .

:hasChargeInformation a owl:ObjectProperty ;
    rdfs:label "Has charge information"@en ;
    rdfs:isDefinedBy <http://data.europa.eu/a4g/ontology> ;
    skos:prefLabel "Has charge information"@en .

:hasClassificationScheme a rdf:Property ;
    rdfs:label "Has classification scheme"@en ;
    rdfs:comment """The classification scheme where a property is defined. 

Additional Information:
For example, the following two properties are defined in the ECLASS classification of goods and services: (0173-1#02-AAA026#007) drilling diameter: drilling diameter, (0173-1#02-AAA030#007) flange diameter: flange diameter .

WG approval 28/07/2022
 (epo-cat:ItemProperty) """@en ;
    rdfs:isDefinedBy <http://data.europa.eu/a4g/ontology> ;
    skos:definition """The classification scheme where a property is defined. 

Additional Information:
For example, the following two properties are defined in the ECLASS classification of goods and services: (0173-1#02-AAA026#007) drilling diameter: drilling diameter, (0173-1#02-AAA030#007) flange diameter: flange diameter .

WG approval 28/07/2022
 (epo-cat:ItemProperty) """@en ;
    skos:prefLabel "Has classification scheme"@en .

:hasComplementaryItem a owl:ObjectProperty ;
    rdfs:label "Has complementary item"@en ;
    rdfs:comment """An item that if used with another item provides mutual enhancements to both of them.

Additional information:
For example, gin and tonic; or smart-phone and smart-watch.

WG Approval: 19/05/2022

 (epo-cat:Item -> epo-cat:Item (+epo-cat:hasComplementaryItem)) """@en ;
    rdfs:isDefinedBy <http://data.europa.eu/a4g/ontology> ;
    skos:definition """An item that if used with another item provides mutual enhancements to both of them.

Additional information:
For example, gin and tonic; or smart-phone and smart-watch.

WG Approval: 19/05/2022

 (epo-cat:Item -> epo-cat:Item (+epo-cat:hasComplementaryItem)) """@en ;
    skos:prefLabel "Has complementary item"@en .

:hasCountryOfOrigin a owl:ObjectProperty ;
    rdfs:label "Has country of origin"@en ;
    rdfs:comment """The source country of the product or service.

Additional Information:

The country of origin can be provided by  the buyer as a requirement or by the tenderer information of the item to be provided.

WG Approval 07/01/2020
 (epo-cat:Item -> at-voc:country (+epo-cat:hasCountryOfOrigin)) """@en ;
    rdfs:isDefinedBy <http://data.europa.eu/a4g/ontology> ;
    skos:prefLabel "Has country of origin"@en ;
    skos:scopeNote """The source country of the product or service.

Additional Information:

The country of origin can be provided by  the buyer as a requirement or by the tenderer information of the item to be provided.

WG Approval 07/01/2020
 (epo-cat:Item -> at-voc:country (+epo-cat:hasCountryOfOrigin)) """@en .

:hasDeliveryClassification a owl:ObjectProperty ;
    rdfs:label "Has delivery classification"@en ;
    rdfs:isDefinedBy <http://data.europa.eu/a4g/ontology> ;
    skos:prefLabel "Has delivery classification"@en .

:hasDeliveryLocation a owl:ObjectProperty ;
    rdfs:label "Has delivery location"@en ;
    rdfs:comment """Location delivery area where the Item can be ordered to the given price.
 (epo-cat:Price -> dct:Location (+epo-cat:hasDeliveryLocation)) """@en ;
    rdfs:isDefinedBy <http://data.europa.eu/a4g/ontology> ;
    skos:prefLabel "Has delivery location"@en ;
    skos:scopeNote """Location delivery area where the Item can be ordered to the given price.
 (epo-cat:Price -> dct:Location (+epo-cat:hasDeliveryLocation)) """@en .

:hasDimensionDescription a rdf:Property ;
    rdfs:label "Has dimension description"@en ;
    rdfs:comment "Textual description of the item's dimensions. (epo-cat:Item) "@en ;
    rdfs:isDefinedBy <http://data.europa.eu/a4g/ontology> ;
    skos:definition "Textual description of the item's dimensions. (epo-cat:Item) "@en ;
    skos:prefLabel "Has dimension description"@en .

:hasDocumentType a owl:ObjectProperty ;
    rdfs:label "Has document type"@en ;
    rdfs:isDefinedBy <http://data.europa.eu/a4g/ontology> ;
    skos:prefLabel "Has document type"@en .

:hasExpectedDeliveryTime a owl:ObjectProperty ;
    rdfs:label "Has expected delivery time"@en ;
    rdfs:comment """
 (epo-cat:Price -> epo:Duration (+epo-cat:hasExpectedDeliveryTime)) """@en,
        """The expected amount of time between the order and delivery of an item. 

WG approval 26/07/2022 (epo-cat:Price -> epo:Duration (+epo-cat:hasExpectedDeliveryTime)) """@en ;
    rdfs:isDefinedBy <http://data.europa.eu/a4g/ontology> ;
    skos:definition """The expected amount of time between the order and delivery of an item. 

WG approval 26/07/2022 (epo-cat:Price -> epo:Duration (+epo-cat:hasExpectedDeliveryTime)) """@en ;
    skos:prefLabel "Has expected delivery time"@en ;
    skos:scopeNote """
 (epo-cat:Price -> epo:Duration (+epo-cat:hasExpectedDeliveryTime)) """@en .

:hasExpiryDate a owl:DatatypeProperty ;
    rdfs:label "Has expiry date"@en ;
    rdfs:comment """The last day until which the item can be used.

WG approval 10/03/2021
 (epo-cat:Batch) """@en ;
    rdfs:isDefinedBy <http://data.europa.eu/a4g/ontology> ;
    skos:definition """The last day until which the item can be used.

WG approval 10/03/2021
 (epo-cat:Batch) """@en ;
    skos:prefLabel "Has expiry date"@en .

:hasExternalSpecification a owl:ObjectProperty ;
    rdfs:label "Has external specification"@en ;
    rdfs:comment """URI reference to external item information or specifications, e.g. web address.
 (epo-cat:Item -> epo:Document (+epo-cat:hasExternalSpecification)) """@en ;
    rdfs:isDefinedBy <http://data.europa.eu/a4g/ontology> ;
    skos:definition """URI reference to external item information or specifications, e.g. web address.
 (epo-cat:Item -> epo:Document (+epo-cat:hasExternalSpecification)) """@en ;
    skos:prefLabel "Has external specification"@en .

:hasFactor a owl:DatatypeProperty ;
    rdfs:label "Has factor"@en ;
    rdfs:comment "The number or the fraction of a related item.  (epo-cat:ItemRelation) "@en ;
    rdfs:isDefinedBy <http://data.europa.eu/a4g/ontology> ;
    skos:definition "The number or the fraction of a related item.  (epo-cat:ItemRelation) "@en ;
    skos:prefLabel "Has factor"@en .

:hasFreightAllowanceCharge a owl:ObjectProperty ;
    rdfs:label "Has freight allowance charge"@en ;
    rdfs:isDefinedBy <http://data.europa.eu/a4g/ontology> ;
    skos:prefLabel "Has freight allowance charge"@en .

:hasHazardousClass a rdf:Property ;
    rdfs:label "Has hazardous class"@en ;
    rdfs:comment "Specification of the hazardous nature of an item according to a classification schema. Provides detail of the classification and nature of a hazardous item. (epo-cat:Item) "@en ;
    rdfs:isDefinedBy <http://data.europa.eu/a4g/ontology> ;
    skos:definition "Specification of the hazardous nature of an item according to a classification schema. Provides detail of the classification and nature of a hazardous item. (epo-cat:Item) "@en ;
    skos:prefLabel "Has hazardous class"@en .

:hasHazardousItemUNDGCode a owl:ObjectProperty ;
    rdfs:label "Has hazardous item u n d g code"@en ;
    rdfs:comment """Specification of the hazardous nature of an item according to the UNDG classification schema. Provides detail of the classification and nature of a hazardous item.
 (epo-cat:Item -> at-voc-new:dangerous-goods-list (+epo-cat:hasHazardousItemUNDGCode)) """@en ;
    rdfs:isDefinedBy <http://data.europa.eu/a4g/ontology> ;
    skos:prefLabel "Has hazardous item u n d g code"@en ;
    skos:scopeNote """Specification of the hazardous nature of an item according to the UNDG classification schema. Provides detail of the classification and nature of a hazardous item.
 (epo-cat:Item -> at-voc-new:dangerous-goods-list (+epo-cat:hasHazardousItemUNDGCode)) """@en .

:hasItemClassification a owl:ObjectProperty ;
    rdfs:label "Has item classification"@en ;
    rdfs:comment """A classification of this item according to a specific system for classifying products or services.

Additional information: 
Examples of classification schemes are: CPV, UNSPC, eCl@ss, GPC, ...

WG acceptance 10/03/2022 (epo-cat:Item -> at-voc-new:item-classification (+epo-cat:hasItemClassification)) """@en ;
    rdfs:isDefinedBy <http://data.europa.eu/a4g/ontology> ;
    skos:definition """A classification of this item according to a specific system for classifying products or services.

Additional information: 
Examples of classification schemes are: CPV, UNSPC, eCl@ss, GPC, ...

WG acceptance 10/03/2022 (epo-cat:Item -> at-voc-new:item-classification (+epo-cat:hasItemClassification)) """@en ;
    skos:prefLabel "Has item classification"@en .

:hasItemStandardID a owl:ObjectProperty ;
    rdfs:label "Has item standard i d"@en ;
    rdfs:comment """The identifier for the instance of the concept based on a standard scheme.

Additional information: 
For example the GTIN scheme (Global Trade Item Number). 

WG Approval 24/02/2022
 (epo-cat:Item -> adms:Identifier (+epo:hasItemStandardID)) """@en ;
    rdfs:isDefinedBy <http://data.europa.eu/a4g/ontology> ;
    skos:definition """The identifier for the instance of the concept based on a standard scheme.

Additional information: 
For example the GTIN scheme (Global Trade Item Number). 

WG Approval 24/02/2022
 (epo-cat:Item -> adms:Identifier (+epo:hasItemStandardID)) """@en ;
    skos:prefLabel "Has item standard i d"@en .

:hasKeyword a rdf:Property ;
    rdfs:label "Has keyword"@en ;
    rdfs:comment """List of words (e.g, synonyms) to make the item searchable. 

WG Approval 7/04/2022
 (epo-cat:Item) """@en ;
    rdfs:isDefinedBy <http://data.europa.eu/a4g/ontology> ;
    skos:definition """List of words (e.g, synonyms) to make the item searchable. 

WG Approval 7/04/2022
 (epo-cat:Item) """@en ;
    skos:prefLabel "Has keyword"@en .

:hasLabelType a owl:ObjectProperty ;
    rdfs:label "Has label type"@en ;
    rdfs:comment "The label type such environmental, quality, social etc. (epo-cat:CertificationLabel -> at-voc-new:certification-label-type (+epo-cat:hasLabelType)) "@en ;
    rdfs:isDefinedBy <http://data.europa.eu/a4g/ontology> ;
    skos:prefLabel "Has label type"@en ;
    skos:scopeNote "The label type such environmental, quality, social etc. (epo-cat:CertificationLabel -> at-voc-new:certification-label-type (+epo-cat:hasLabelType)) "@en .

:hasLiteralValue a rdf:Property ;
    rdfs:label "Has literal value"@en ;
    rdfs:comment """Simple value of the property, which is defined in a classification scheme.

Additional Information:
For example, the (0173-1#02-AAV139#001) coating 1 of an optical material has value of "silver". 

This simple literal value is for the cases when the property value does not have units, in which case the qualifiedValue shall be used. 

WG approval 28/07/2022


 (epo-cat:ItemProperty) """@en ;
    rdfs:isDefinedBy <http://data.europa.eu/a4g/ontology> ;
    skos:definition """Simple value of the property, which is defined in a classification scheme.

Additional Information:
For example, the (0173-1#02-AAV139#001) coating 1 of an optical material has value of "silver". 

This simple literal value is for the cases when the property value does not have units, in which case the qualifiedValue shall be used. 

WG approval 28/07/2022


 (epo-cat:ItemProperty) """@en ;
    skos:prefLabel "Has literal value"@en .

:hasManufactureDate a owl:DatatypeProperty ;
    rdfs:label "Has manufacture date"@en ;
    rdfs:comment """The day of production.
 (epo-cat:Batch) """@en ;
    rdfs:isDefinedBy <http://data.europa.eu/a4g/ontology> ;
    skos:definition """The day of production.
 (epo-cat:Batch) """@en ;
    skos:prefLabel "Has manufacture date"@en .

:hasManufacturer a owl:ObjectProperty ;
    rdfs:label "Has manufacturer"@en ;
    rdfs:comment "The product maker or service provider. (epo-cat:Item -> epo-cat:Manufacturer (+epo-cat:hasManufacturer)) "@en ;
    rdfs:isDefinedBy <http://data.europa.eu/a4g/ontology> ;
    skos:prefLabel "Has manufacturer"@en ;
    skos:scopeNote "The product maker or service provider. (epo-cat:Item -> epo-cat:Manufacturer (+epo-cat:hasManufacturer)) "@en .

:hasManufacturerID a owl:ObjectProperty ;
    rdfs:label "Has manufacturer i d"@en ;
    rdfs:comment """The manufacturer's identifier for the item.
 (epo-cat:Manufacturer -> adms:Identifier (+epo:hasManufacturerID)) """@en ;
    rdfs:isDefinedBy <http://data.europa.eu/a4g/ontology> ;
    skos:definition """The manufacturer's identifier for the item.
 (epo-cat:Manufacturer -> adms:Identifier (+epo:hasManufacturerID)) """@en ;
    skos:prefLabel "Has manufacturer i d"@en .

:hasManufacturerItemID a owl:ObjectProperty ;
    rdfs:label "Has manufacturer item i d"@en ;
    rdfs:comment """This refers to the general identifier for the concept as defined by the manufacturer.


WG Approval 16/05/2023

 (epo-cat:Item -> adms:Identifier (+epo:hasManufacturerItemID)) """@en ;
    rdfs:isDefinedBy <http://data.europa.eu/a4g/ontology> ;
    skos:definition """This refers to the general identifier for the concept as defined by the manufacturer.


WG Approval 16/05/2023

 (epo-cat:Item -> adms:Identifier (+epo:hasManufacturerItemID)) """@en ;
    skos:prefLabel "Has manufacturer item i d"@en .

:hasMaximumOrderQuantity a owl:ObjectProperty ;
    rdfs:label "Has maximum order quantity"@en ;
    rdfs:comment """The maximum number of orderable units that can be ordered according to details provided in the catalogue line, such as price.
 (epo-cat:CatalogueLine -> epo:Quantity (+epo-cat:hasMaximumOrderQuantity)) """@en ;
    rdfs:isDefinedBy <http://data.europa.eu/a4g/ontology> ;
    skos:definition """The maximum number of orderable units that can be ordered according to details provided in the catalogue line, such as price.
 (epo-cat:CatalogueLine -> epo:Quantity (+epo-cat:hasMaximumOrderQuantity)) """@en ;
    skos:prefLabel "Has maximum order quantity"@en .

:hasMinimumQuantityGuaranteedForDelivery a owl:ObjectProperty ;
    rdfs:label "Has minimum quantity guaranteed for delivery"@en ;
    rdfs:comment """The minimum quantity of an item that is guaranteed by the seller to be delivered.

 (epo-cat:CatalogueLine -> epo:Quantity (+epo-cat:hasMinimumQuantityGuaranteedForDelivery)) """@en ;
    rdfs:isDefinedBy <http://data.europa.eu/a4g/ontology> ;
    skos:definition """The minimum quantity of an item that is guaranteed by the seller to be delivered.

 (epo-cat:CatalogueLine -> epo:Quantity (+epo-cat:hasMinimumQuantityGuaranteedForDelivery)) """@en ;
    skos:prefLabel "Has minimum quantity guaranteed for delivery"@en .

:hasModel a owl:ObjectProperty ;
    rdfs:label "Has model"@en ;
    rdfs:isDefinedBy <http://data.europa.eu/a4g/ontology> ;
    skos:prefLabel "Has model"@en .

:hasNetMonetaryValue a owl:ObjectProperty ;
    rdfs:label "Has net monetary value"@en ;
    rdfs:comment "The price amount of an Item exclusive of taxes and after substracting price discounts.  (epo-cat:Price -> epo:MonetaryValue (+epo-cat:hasNetMonetaryValue)) "@en ;
    rdfs:isDefinedBy <http://data.europa.eu/a4g/ontology> ;
    skos:prefLabel "Has net monetary value"@en ;
    skos:scopeNote "The price amount of an Item exclusive of taxes and after substracting price discounts.  (epo-cat:Price -> epo:MonetaryValue (+epo-cat:hasNetMonetaryValue)) "@en .

:hasNetQuantity a owl:ObjectProperty ;
    rdfs:label "Has net quantity"@en ;
    rdfs:comment """The net quantity of the item that is contained in each consumable unit, excluding any packaging materials.
 (epo-cat:Item -> epo:Quantity (+epo-cat:hasNetQuantity)) """@en ;
    rdfs:isDefinedBy <http://data.europa.eu/a4g/ontology> ;
    skos:definition """The net quantity of the item that is contained in each consumable unit, excluding any packaging materials.
 (epo-cat:Item -> epo:Quantity (+epo-cat:hasNetQuantity)) """@en ;
    skos:prefLabel "Has net quantity"@en .

:hasOrderabableUnitFactorRate a owl:ObjectProperty ;
    rdfs:label "Has orderabable unit factor rate"@en ;
    rdfs:comment """The factor by which the base unit of the price can be converted to orderable unit.

Additional information:
This is needed when the base price is provided different than the orderable unit. For example, when selling paper, the price may be set per page, but the  orderable unit is a package of 500 pieces. Therefore the price needs to be converted to the orderable unit. 

 (epo-cat:Price -> epo:Quantity (+epo-cat:hasOrderabableUnitFactorRate)) """@en ;
    rdfs:isDefinedBy <http://data.europa.eu/a4g/ontology> ;
    skos:prefLabel "Has orderabable unit factor rate"@en ;
    skos:scopeNote """The factor by which the base unit of the price can be converted to orderable unit.

Additional information:
This is needed when the base price is provided different than the orderable unit. For example, when selling paper, the price may be set per page, but the  orderable unit is a package of 500 pieces. Therefore the price needs to be converted to the orderable unit. 

 (epo-cat:Price -> epo:Quantity (+epo-cat:hasOrderabableUnitFactorRate)) """@en .

:hasOrderableQuantityIncrement a owl:DatatypeProperty ;
    rdfs:label "Has orderable quantity increment"@en ;
    rdfs:comment "Orderable quantity increment: The increment of Orderable units that can be ordered. (epo-cat:CatalogueLine) "@en ;
    rdfs:isDefinedBy <http://data.europa.eu/a4g/ontology> ;
    skos:definition "Orderable quantity increment: The increment of Orderable units that can be ordered. (epo-cat:CatalogueLine) "@en ;
    skos:prefLabel "Has orderable quantity increment"@en .

:hasOrderableUnit a owl:ObjectProperty ;
    rdfs:label "Has orderable unit"@en ;
    rdfs:comment "The unit in which the item described in this catalogue line can be ordered. (epo-cat:CatalogueLine -> at-voc-new:orderable-unit (+epo-cat:hasOrderableUnit)) "@en ;
    rdfs:isDefinedBy <http://data.europa.eu/a4g/ontology> ;
    skos:definition "The unit in which the item described in this catalogue line can be ordered. (epo-cat:CatalogueLine -> at-voc-new:orderable-unit (+epo-cat:hasOrderableUnit)) "@en ;
    skos:prefLabel "Has orderable unit"@en .

:hasOrderableUnitFactorRate a owl:DatatypeProperty ;
    rdfs:label "Has orderable unit factor rate"@en ;
    rdfs:comment "The factor by which the Item net price of an unit of an item can be converted to the orderable unit. (epo-cat:CatalogueLine) "@en ;
    rdfs:isDefinedBy <http://data.europa.eu/a4g/ontology> ;
    skos:definition "The factor by which the Item net price of an unit of an item can be converted to the orderable unit. (epo-cat:CatalogueLine) "@en ;
    skos:prefLabel "Has orderable unit factor rate"@en .

:hasPart a owl:ObjectProperty ;
    rdfs:label "Has part"@en ;
    rdfs:comment """A related resource that is included either physically or logically in the described resource.

Additional Information: 
In the eCatalogue context, when this relation is used between two items, the resource in the definition refers to Items, i.e. one item is part of another item.

WG Approval: 30/06/2022
 (epo-cat:Item -> epo-cat:Item (+dct:hasPart)) """@en ;
    rdfs:isDefinedBy <http://data.europa.eu/a4g/ontology> ;
    skos:definition """A related resource that is included either physically or logically in the described resource.

Additional Information: 
In the eCatalogue context, when this relation is used between two items, the resource in the definition refers to Items, i.e. one item is part of another item.

WG Approval: 30/06/2022
 (epo-cat:Item -> epo-cat:Item (+dct:hasPart)) """@en ;
    skos:prefLabel "Has part"@en .

:hasPrice a owl:ObjectProperty ;
    rdfs:label "Has price"@en ;
    rdfs:isDefinedBy <http://data.europa.eu/a4g/ontology> ;
    skos:prefLabel "Has price"@en .

:hasPriceDiscountInformation a owl:ObjectProperty ;
    rdfs:label "Has price discount information"@en ;
    rdfs:isDefinedBy <http://data.europa.eu/a4g/ontology> ;
    skos:prefLabel "Has price discount information"@en .

:hasPriceSurchargeInformation a owl:ObjectProperty ;
    rdfs:label "Has price surcharge information"@en ;
    rdfs:isDefinedBy <http://data.europa.eu/a4g/ontology> ;
    skos:prefLabel "Has price surcharge information"@en .

:hasPriceType a owl:ObjectProperty ;
    rdfs:label "Has price type"@en ;
    rdfs:isDefinedBy <http://data.europa.eu/a4g/ontology> ;
    skos:prefLabel "Has price type"@en .

:hasPriceValidity a owl:ObjectProperty ;
    rdfs:label "Has price validity"@en ;
    rdfs:comment """The period of time when the Item can be ordered to the given price.
 (epo-cat:Price -> epo:Period (+epo-cat:hasPriceValidity)) """@en ;
    rdfs:isDefinedBy <http://data.europa.eu/a4g/ontology> ;
    skos:prefLabel "Has price validity"@en ;
    skos:scopeNote """The period of time when the Item can be ordered to the given price.
 (epo-cat:Price -> epo:Period (+epo-cat:hasPriceValidity)) """@en .

:hasQualifiedItemRelation a owl:ObjectProperty ;
    rdfs:label "Has qualified item relation"@en ;
    rdfs:isDefinedBy <http://data.europa.eu/a4g/ontology> ;
    skos:prefLabel "Has qualified item relation"@en .

:hasQualifiedValue a owl:ObjectProperty ;
    rdfs:label "Has qualified value"@en ;
    rdfs:comment """Qualified value of the property, which is defined in a classification scheme.

Additional Information:
For example, the (0173-1#02-AAA026#007) drilling diameter of an item has value of 12 inches. 

WG approval 28/07/2022 (epo-cat:ItemProperty -> epo:Quantity (+epo-cat:hasQualifiedValue)) """@en ;
    rdfs:isDefinedBy <http://data.europa.eu/a4g/ontology> ;
    skos:definition """Qualified value of the property, which is defined in a classification scheme.

Additional Information:
For example, the (0173-1#02-AAA026#007) drilling diameter of an item has value of 12 inches. 

WG approval 28/07/2022 (epo-cat:ItemProperty -> epo:Quantity (+epo-cat:hasQualifiedValue)) """@en ;
    skos:prefLabel "Has qualified value"@en .

:hasQuantityThreshold a owl:ObjectProperty ;
    rdfs:label "Has quantity threshold"@en ;
    rdfs:comment "The minimum quantity of the item that can be ordered to the given net monetary value. (epo-cat:Price -> epo:Quantity (+epo-cat:hasQuantityThreshold)) "@en ;
    rdfs:isDefinedBy <http://data.europa.eu/a4g/ontology> ;
    skos:prefLabel "Has quantity threshold"@en ;
    skos:scopeNote "The minimum quantity of the item that can be ordered to the given net monetary value. (epo-cat:Price -> epo:Quantity (+epo-cat:hasQuantityThreshold)) "@en .

:hasReferenceURI a owl:DatatypeProperty ;
    rdfs:label "Has reference u r i"@en ;
    rdfs:comment """A reference to where the label specification (norms, expectations, standards and policies) can be found.

WG approval 26/07/2022 (epo-cat:CertificationLabel) """@en ;
    rdfs:isDefinedBy <http://data.europa.eu/a4g/ontology> ;
    skos:definition """A reference to where the label specification (norms, expectations, standards and policies) can be found.

WG approval 26/07/2022 (epo-cat:CertificationLabel) """@en ;
    skos:prefLabel "Has reference u r i"@en .

:hasSellerItemID a owl:ObjectProperty ;
    rdfs:label "Has seller item i d"@en ;
    rdfs:comment """ The general identifier for the concept as defined by the seller.

WG Approval 16/05/2023
 (epo-cat:Item -> adms:Identifier (+epo:hasSellerItemID)) """@en ;
    rdfs:isDefinedBy <http://data.europa.eu/a4g/ontology> ;
    skos:definition """ The general identifier for the concept as defined by the seller.

WG Approval 16/05/2023
 (epo-cat:Item -> adms:Identifier (+epo:hasSellerItemID)) """@en ;
    skos:prefLabel "Has seller item i d"@en .

:hasSerialID a owl:ObjectProperty ;
    rdfs:label "Has serial i d"@en ;
    rdfs:comment """The identifier assigned to the specific instance of the produced concept.
WG Approval 16/05/2023
 (epo-cat:Item -> adms:Identifier (+epo:hasSerialID)) """@en ;
    rdfs:isDefinedBy <http://data.europa.eu/a4g/ontology> ;
    skos:definition """The identifier assigned to the specific instance of the produced concept.
WG Approval 16/05/2023
 (epo-cat:Item -> adms:Identifier (+epo:hasSerialID)) """@en ;
    skos:prefLabel "Has serial i d"@en .

:hasSpecificPaymentArrangement a rdf:Property ;
    rdfs:label "Has specific payment arrangement"@en ;
    rdfs:comment """Information about payment conditions applied to all items in the catalogue.

Additional information:
This property may need to be used together with the payment arrangements provided in the ContractTerms, where such terms exists.

WG approval 30/06/2022

 (epo-cat:Catalogue) """@en ;
    rdfs:isDefinedBy <http://data.europa.eu/a4g/ontology> ;
    skos:definition """Information about payment conditions applied to all items in the catalogue.

Additional information:
This property may need to be used together with the payment arrangements provided in the ContractTerms, where such terms exists.

WG approval 30/06/2022

 (epo-cat:Catalogue) """@en ;
    skos:prefLabel "Has specific payment arrangement"@en .

:hasSpecification a owl:ObjectProperty ;
    rdfs:label "Has specification"@en ;
    rdfs:isDefinedBy <http://data.europa.eu/a4g/ontology> ;
    skos:prefLabel "Has specification"@en .

:hasStandardisedUnitPrice a owl:ObjectProperty ;
    rdfs:label "Has standardised unit price"@en ;
    rdfs:comment """The item price based on a standardised unit.

Additional Information:
The unit must be indicated in the Quantity, with a quantity value of 1. (epo-cat:CatalogueLine -> epo-cat:Price (+epo-cat:hasStandardisedUnitPrice)) """@en ;
    rdfs:isDefinedBy <http://data.europa.eu/a4g/ontology> ;
    skos:definition """The item price based on a standardised unit.

Additional Information:
The unit must be indicated in the Quantity, with a quantity value of 1. (epo-cat:CatalogueLine -> epo-cat:Price (+epo-cat:hasStandardisedUnitPrice)) """@en ;
    skos:prefLabel "Has standardised unit price"@en .

:hasTaxCategory a owl:ObjectProperty ;
    rdfs:label "Has tax category"@en ;
    rdfs:isDefinedBy <http://data.europa.eu/a4g/ontology> ;
    skos:prefLabel "Has tax category"@en .

:hasTaxInformation a owl:ObjectProperty ;
    rdfs:label "Has tax information"@en ;
    rdfs:isDefinedBy <http://data.europa.eu/a4g/ontology> ;
    skos:prefLabel "Has tax information"@en .

:hasTaxScheme a owl:ObjectProperty ;
    rdfs:label "Has tax scheme"@en ;
    rdfs:isDefinedBy <http://data.europa.eu/a4g/ontology> ;
    skos:prefLabel "Has tax scheme"@en .

:hasTransactionConditions a rdf:Property ;
    rdfs:label "Has transaction conditions"@en ;
    rdfs:comment "Textual description of the specific transaction conditions (purchasing, sales, payment) for an item. (epo-cat:CatalogueLine) "@en ;
    rdfs:isDefinedBy <http://data.europa.eu/a4g/ontology> ;
    skos:definition "Textual description of the specific transaction conditions (purchasing, sales, payment) for an item. (epo-cat:CatalogueLine) "@en ;
    skos:prefLabel "Has transaction conditions"@en .

:hasTransactionConditionsCode a owl:ObjectProperty ;
    rdfs:label "Has transaction conditions code"@en ;
    rdfs:comment """Coded description of the specific transaction conditions (purchasing, sales, payment) for an item.
 (epo-cat:CatalogueLine -> at-voc-new:transaction-conditions (+epo-cat:hasTransactionConditionsCode)) """@en ;
    rdfs:isDefinedBy <http://data.europa.eu/a4g/ontology> ;
    skos:definition """Coded description of the specific transaction conditions (purchasing, sales, payment) for an item.
 (epo-cat:CatalogueLine -> at-voc-new:transaction-conditions (+epo-cat:hasTransactionConditionsCode)) """@en ;
    skos:prefLabel "Has transaction conditions code"@en .

:hasURL a owl:DatatypeProperty ;
    rdfs:label "Has u r l"@en ;
    rdfs:comment """The identifier of a resource.

Additional Information

For example:

1. The URL of the system from where to access the procurement documents;
2. The URL of the system for the submission of tender documents;
3. The URL of the system from where to download a tool to communicate with the Buyer;
4. The URL of the system used by a Technique to allow Economic Operators to exchange information with the Buyer (e.g. eAuction and DPS Systems)
5. The URL of the system used to exchange information between Buyer and EO for questions and clarifications;

WG Approval 30/09/2019
 (epo-cat:Certificate) """@en ;
    rdfs:isDefinedBy <http://data.europa.eu/a4g/ontology> ;
    skos:definition """The identifier of a resource.

Additional Information

For example:

1. The URL of the system from where to access the procurement documents;
2. The URL of the system for the submission of tender documents;
3. The URL of the system from where to download a tool to communicate with the Buyer;
4. The URL of the system used by a Technique to allow Economic Operators to exchange information with the Buyer (e.g. eAuction and DPS Systems)
5. The URL of the system used to exchange information between Buyer and EO for questions and clarifications;

WG Approval 30/09/2019
 (epo-cat:Certificate) """@en ;
    skos:prefLabel "Has u r l"@en .

:hasVATCategory a owl:ObjectProperty ;
    rdfs:label "Has v a t category"@en ;
    rdfs:comment """Value-added tax category of the item.
 (epo-ord:TaxInformation -> at-voc-new:vat-category (+epo-cat:hasVATCategory)) """@en ;
    rdfs:isDefinedBy <http://data.europa.eu/a4g/ontology> ;
    skos:definition """Value-added tax category of the item.
 (epo-ord:TaxInformation -> at-voc-new:vat-category (+epo-cat:hasVATCategory)) """@en ;
    skos:prefLabel "Has v a t category"@en .

:hasValidityPeriod a owl:ObjectProperty ;
    rdfs:label "Has validity period"@en ;
    rdfs:comment """The relation indicating until when a given instance of a concept is applicable.

WG approval 30/05/2023 (epo-cat:Certificate -> epo:Period (+epo:hasValidityPeriod)) """@en ;
    rdfs:isDefinedBy <http://data.europa.eu/a4g/ontology> ;
    skos:definition """The relation indicating until when a given instance of a concept is applicable.

WG approval 30/05/2023 (epo-cat:Certificate -> epo:Period (+epo:hasValidityPeriod)) """@en ;
    skos:prefLabel "Has validity period"@en .

:hasWarrantyInformation a rdf:Property ;
    rdfs:label "Has warranty information"@en ;
    rdfs:comment "Warranty information that applies to the catalogue line item. (epo-cat:CatalogueLine) "@en ;
    rdfs:isDefinedBy <http://data.europa.eu/a4g/ontology> ;
    skos:definition "Warranty information that applies to the catalogue line item. (epo-cat:CatalogueLine) "@en ;
    skos:prefLabel "Has warranty information"@en .

:identifier a owl:ObjectProperty ;
    rdfs:label "Identifier"@en ;
    rdfs:comment "Links a resource to an adms:Identifier class. (epo-cat:Line -> adms:Identifier (+adms:identifier)) "@en ;
    rdfs:isDefinedBy <http://data.europa.eu/a4g/ontology> ;
    skos:definition "Links a resource to an adms:Identifier class. (epo-cat:Line -> adms:Identifier (+adms:identifier)) "@en ;
    skos:prefLabel "Identifier"@en .

:isContractedItem a owl:DatatypeProperty ;
    rdfs:label "Is contracted item"@en ;
    rdfs:comment "Indicator if the item is offered in accordance to an existing contract. (epo-cat:CatalogueLine) "@en ;
    rdfs:isDefinedBy <http://data.europa.eu/a4g/ontology> ;
    skos:definition "Indicator if the item is offered in accordance to an existing contract. (epo-cat:CatalogueLine) "@en ;
    skos:prefLabel "Is contracted item"@en .

:isInStock a owl:DatatypeProperty ;
    rdfs:label "Is in stock"@en ;
    rdfs:comment "Indicator whether an item is in the supplier's stock. If not in stock the supplier has to order the item. (epo-cat:Item) "@en ;
    rdfs:isDefinedBy <http://data.europa.eu/a4g/ontology> ;
    skos:definition "Indicator whether an item is in the supplier's stock. If not in stock the supplier has to order the item. (epo-cat:Item) "@en ;
    skos:prefLabel "Is in stock"@en .

:isOrderable a owl:DatatypeProperty ;
    rdfs:label "Is orderable"@en ;
    rdfs:comment "Indicator, if the item is orderable or not, e.g. because it is temporarily out of stock. (epo-cat:CatalogueLine) "@en ;
    rdfs:isDefinedBy <http://data.europa.eu/a4g/ontology> ;
    skos:definition "Indicator, if the item is orderable or not, e.g. because it is temporarily out of stock. (epo-cat:CatalogueLine) "@en ;
    skos:prefLabel "Is orderable"@en .

:isProductionOf a owl:ObjectProperty ;
    rdfs:label "Is production of"@en ;
    rdfs:isDefinedBy <http://data.europa.eu/a4g/ontology> ;
    skos:prefLabel "Is production of"@en .

:isRelatedToItem a owl:ObjectProperty ;
    rdfs:label "Is related to item"@en ;
    rdfs:isDefinedBy <http://data.europa.eu/a4g/ontology> ;
    skos:prefLabel "Is related to item"@en .

:isReplacedBy a owl:ObjectProperty ;
    rdfs:label "Is replaced by"@en ;
    rdfs:comment """A related resource that is supplanted, displaced, or superseded by the described resource.

Additional Information: 
In the eCatalogue context, when this relation is used between two items, the resource in the definition refers to Items, i.e. one item replaces another item. 

WG Approval: 30/06/2022
 (epo-cat:Item <-> epo-cat:Item (+dct:isReplacedBy +dct:replaces)) """@en ;
    rdfs:isDefinedBy <http://data.europa.eu/a4g/ontology> ;
    skos:definition """A related resource that is supplanted, displaced, or superseded by the described resource.

Additional Information: 
In the eCatalogue context, when this relation is used between two items, the resource in the definition refers to Items, i.e. one item replaces another item. 

WG Approval: 30/06/2022
 (epo-cat:Item <-> epo-cat:Item (+dct:isReplacedBy +dct:replaces)) """@en ;
    skos:prefLabel "Is replaced by"@en .

:isSpecificToLine a owl:ObjectProperty ;
    rdfs:label "Is specific to line"@en ;
    rdfs:isDefinedBy <http://data.europa.eu/a4g/ontology> ;
    skos:prefLabel "Is specific to line"@en .

:isSpecificToOrderLine a owl:ObjectProperty ;
    rdfs:label "Is specific to order line"@en ;
    rdfs:comment """Information that is particular to one or multiple Order Lines.
 (epo-cat:ChargeInformation -> epo-ord:OrderLine (+epo-ord:isSpecificToOrderLine)) """@en ;
    rdfs:isDefinedBy <http://data.europa.eu/a4g/ontology> ;
    skos:definition """Information that is particular to one or multiple Order Lines.
 (epo-cat:ChargeInformation -> epo-ord:OrderLine (+epo-ord:isSpecificToOrderLine)) """@en ;
    skos:prefLabel "Is specific to order line"@en .

:isSubordinatedToContract a owl:ObjectProperty ;
    rdfs:label "Is subordinated to contract"@en ;
    rdfs:isDefinedBy <http://data.europa.eu/a4g/ontology> ;
    skos:prefLabel "Is subordinated to contract"@en .

:issuedByCertifier a owl:ObjectProperty ;
    rdfs:label "Issued by certifier"@en ;
    rdfs:comment """Relation indicating the Certifier responsible for providing the ItemCertificate.

Additional Information:
Certifier is a role played by an organisation.

WG approval 26/07/2022 (epo-cat:Certificate -> epo-cat:Certifier (+epo-cat:issuedByCertifier)) """@en ;
    rdfs:isDefinedBy <http://data.europa.eu/a4g/ontology> ;
    skos:definition """Relation indicating the Certifier responsible for providing the ItemCertificate.

Additional Information:
Certifier is a role played by an organisation.

WG approval 26/07/2022 (epo-cat:Certificate -> epo-cat:Certifier (+epo-cat:issuedByCertifier)) """@en ;
    skos:prefLabel "Issued by certifier"@en .

:refersToCatalogue a owl:ObjectProperty ;
    rdfs:label "Refers to catalogue"@en ;
    rdfs:comment """
Additional information:
If an order refers to multiple catalogues then all these catalogues ideally are subordinated to the same contract. 
Some countries however may allow multiple contracts per order (i.e Italy).  (epo-ord:Order -> epo-cat:Catalogue (+epo-ord:refersToCatalogue)) """@en ;
    rdfs:isDefinedBy <http://data.europa.eu/a4g/ontology> ;
    skos:definition """
Additional information:
If an order refers to multiple catalogues then all these catalogues ideally are subordinated to the same contract. 
Some countries however may allow multiple contracts per order (i.e Italy).  (epo-ord:Order -> epo-cat:Catalogue (+epo-ord:refersToCatalogue)) """@en ;
    skos:prefLabel "Refers to catalogue"@en .

:refersToCatalogueLine a owl:ObjectProperty ;
    rdfs:label "Refers to catalogue line"@en ;
    rdfs:comment """
Additional Information:
The reference to the catalogue line is for information only, to trace the source of the information provided in the order line.  (epo-ord:OrderLine -> epo-cat:CatalogueLine (+epo-ord:refersToCatalogueLine)) """@en ;
    rdfs:isDefinedBy <http://data.europa.eu/a4g/ontology> ;
    skos:definition """
Additional Information:
The reference to the catalogue line is for information only, to trace the source of the information provided in the order line.  (epo-ord:OrderLine -> epo-cat:CatalogueLine (+epo-ord:refersToCatalogueLine)) """@en ;
    skos:prefLabel "Refers to catalogue line"@en .

:replaces a owl:ObjectProperty ;
    rdfs:label "Replaces"@en ;
    rdfs:comment """A related resource that is supplanted, displaced, or superseded by the described resource.

Additional Information: 
In the eCatalogue context, when this relation is used between two items, the resource in the definition refers to Items, i.e. one item replaces another item. 

WG Approval: 30/06/2022
 (epo-cat:Item <-> epo-cat:Item (+dct:isReplacedBy +dct:replaces)) """@en,
        """A related resource that is supplanted, displaced, or superseded by the described resource.
 (epo-cat:Item <-> epo-cat:Item (+dct:isReplacedBy +dct:replaces)) """@en ;
    rdfs:isDefinedBy <http://data.europa.eu/a4g/ontology> ;
    skos:definition """A related resource that is supplanted, displaced, or superseded by the described resource.

Additional Information: 
In the eCatalogue context, when this relation is used between two items, the resource in the definition refers to Items, i.e. one item replaces another item. 

WG Approval: 30/06/2022
 (epo-cat:Item <-> epo-cat:Item (+dct:isReplacedBy +dct:replaces)) """@en ;
    skos:prefLabel "Replaces"@en ;
    skos:scopeNote """A related resource that is supplanted, displaced, or superseded by the described resource.
 (epo-cat:Item <-> epo-cat:Item (+dct:isReplacedBy +dct:replaces)) """@en .

:requires a owl:ObjectProperty ;
    rdfs:label "Requires"@en ;
    rdfs:comment """A related resource that is required by the described resource to support its function, delivery, or coherence.

Additional Information:
In the eCatalogue context, when this relation is used between two items, the resource in the definition refers to Items, i.e. one Item requires another Item. 

WG Approval: 30/06/2022
 (epo-cat:Item -> epo-cat:Item (+dct:requires)) """@en ;
    rdfs:isDefinedBy <http://data.europa.eu/a4g/ontology> ;
    skos:definition """A related resource that is required by the described resource to support its function, delivery, or coherence.

Additional Information:
In the eCatalogue context, when this relation is used between two items, the resource in the definition refers to Items, i.e. one Item requires another Item. 

WG Approval: 30/06/2022
 (epo-cat:Item -> epo-cat:Item (+dct:requires)) """@en ;
    skos:prefLabel "Requires"@en .

:specifiesBuyer a owl:ObjectProperty ;
    rdfs:label "Specifies buyer"@en ;
    rdfs:isDefinedBy <http://data.europa.eu/a4g/ontology> ;
    skos:prefLabel "Specifies buyer"@en .

:specifiesCatalogueProvider a owl:ObjectProperty ;
    rdfs:label "Specifies catalogue provider"@en ;
    rdfs:isDefinedBy <http://data.europa.eu/a4g/ontology> ;
    skos:prefLabel "Specifies catalogue provider"@en .

:specifiesCatalogueReceiver a owl:ObjectProperty ;
    rdfs:label "Specifies catalogue receiver"@en ;
    rdfs:isDefinedBy <http://data.europa.eu/a4g/ontology> ;
    skos:prefLabel "Specifies catalogue receiver"@en .

:specifiesChargeInformation a owl:ObjectProperty ;
    rdfs:label "Specifies charge information"@en ;
    rdfs:isDefinedBy <http://data.europa.eu/a4g/ontology> ;
    skos:prefLabel "Specifies charge information"@en .

:specifiesItem a owl:ObjectProperty ;
    rdfs:label "Specifies item"@en ;
    rdfs:isDefinedBy <http://data.europa.eu/a4g/ontology> ;
    skos:prefLabel "Specifies item"@en .

:specifiesSeller a owl:ObjectProperty ;
    rdfs:label "Specifies seller"@en ;
    rdfs:isDefinedBy <http://data.europa.eu/a4g/ontology> ;
    skos:prefLabel "Specifies seller"@en .

:updatesCatalogue a owl:ObjectProperty ;
    rdfs:label "Updates catalogue"@en ;
    rdfs:comment "Relation indicating (epo-cat:CatalogueFragment -> epo-cat:Catalogue (+epo-cat:updatesCatalogue)) "@en ;
    rdfs:isDefinedBy <http://data.europa.eu/a4g/ontology> ;
    skos:definition "Relation indicating (epo-cat:CatalogueFragment -> epo-cat:Catalogue (+epo-cat:updatesCatalogue)) "@en ;
    skos:prefLabel "Updates catalogue"@en .

dcterms:description a rdf:Property ;
    rdfs:label "Description"@en ;
    rdfs:comment """An account of the resource.

Additional Information:
Description may include but is not limited to: an abstract, a table of contents, a graphical representation, or a free-text account of the resource.

WG Approval 30/05/2023 (epo-cat:Item) An account of the resource.

Additional Information:
Description may include but is not limited to: an abstract, a table of contents, a graphical representation, or a free-text account of the resource.

WG Approval 30/05/2023 (epo-cat:Line) """@en ;
    skos:definition """An account of the resource.

Additional Information:
Description may include but is not limited to: an abstract, a table of contents, a graphical representation, or a free-text account of the resource.

WG Approval 30/05/2023 (epo-cat:Item) An account of the resource.

Additional Information:
Description may include but is not limited to: an abstract, a table of contents, a graphical representation, or a free-text account of the resource.

WG Approval 30/05/2023 (epo-cat:Line) """@en ;
    skos:prefLabel "Description"@en .

dcterms:title a rdf:Property ;
    rdfs:label "Title"@en ;
    rdfs:comment """A name given to the resource.

WG approval 30/05/2023 (epo-cat:ItemModel) A name given to the resource.

WG approval 30/05/2023
 (epo-cat:Brand) A name given to the resource.

WG approval 30/05/2023 (epo-cat:Item) """@en ;
    skos:definition """A name given to the resource.

WG approval 30/05/2023 (epo-cat:ItemModel) A name given to the resource.

WG approval 30/05/2023
 (epo-cat:Brand) A name given to the resource.

WG approval 30/05/2023 (epo-cat:Item) """@en ;
    skos:prefLabel "Title"@en .

rdf:PlainLiteral a rdfs:Datatype ;
    rdfs:label "Plain literal"@en ;
    skos:prefLabel "Plain literal"@en .

xsd:AnyURI a rdfs:Datatype ;
    rdfs:label "Any u r i"@en ;
    skos:prefLabel "Any u r i"@en .

xsd:Boolean a rdfs:Datatype ;
    rdfs:label "Boolean"@en ;
    skos:prefLabel "Boolean"@en .

xsd:Date a rdfs:Datatype ;
    rdfs:label "Date"@en ;
    skos:prefLabel "Date"@en .

xsd:DateTime a rdfs:Datatype ;
    rdfs:label "Date time"@en ;
    skos:prefLabel "Date time"@en .

xsd:Decimal a rdfs:Datatype ;
    rdfs:label "Decimal"@en ;
    skos:prefLabel "Decimal"@en .

xsd:Integer a rdfs:Datatype ;
    rdfs:label "Integer"@en ;
    skos:prefLabel "Integer"@en .

:Catalogue a owl:Class ;
    rdfs:label "Catalogue"@en ;
    rdfs:comment """A Document describing a set of Items offered for purchase that can be processed in an electronic way.
"""@en ;
    rdfs:isDefinedBy <http://data.europa.eu/a4g/ontology> ;
    skos:definition """A Document describing a set of Items offered for purchase that can be processed in an electronic way.
"""@en ;
    skos:prefLabel "Catalogue"@en .

:Line a owl:Class ;
    rdfs:label "Line"@en ;
    rdfs:isDefinedBy <http://data.europa.eu/a4g/ontology> ;
    skos:prefLabel "Line"@en .

:ItemAccessoryRelation a owl:Class ;
    rdfs:label "Item accessory relation"@en ;
    rdfs:comment """Combination of two Items where the former enhances the latter.

WG Approval: 30/06/2022
"""@en ;
    rdfs:isDefinedBy <http://data.europa.eu/a4g/ontology> ;
    rdfs:subClassOf :ItemRelation ;
    owl:disjointWith :ItemComplementaryRelation,
        :ItemComposition,
        :ItemReplacement,
        :ItemRequirement ;
    skos:definition """Combination of two Items where the former enhances the latter.

WG Approval: 30/06/2022
"""@en ;
    skos:prefLabel "Item accessory relation"@en .

:ItemComplementaryRelation a owl:Class ;
    rdfs:label "Item complementary relation"@en ;
    rdfs:comment """Combination of two Items which mutually enhance one another.

WG Approval: 30/06/2022

"""@en ;
    rdfs:isDefinedBy <http://data.europa.eu/a4g/ontology> ;
    rdfs:subClassOf :ItemRelation ;
    owl:disjointWith :ItemAccessoryRelation,
        :ItemComposition,
        :ItemReplacement,
        :ItemRequirement ;
    skos:definition """Combination of two Items which mutually enhance one another.

WG Approval: 30/06/2022

"""@en ;
    skos:prefLabel "Item complementary relation"@en .

:ItemComposition a owl:Class ;
    rdfs:label "Item composition"@en ;
    rdfs:comment """Inclusion of an Item into in the described Item.

Additional Information:
The Item is provided with its components, however, the component Items may also be provided separately. 
For example, a bicycle has wheels as components, but they may be provided as spare parts as well. 
This relation is useful to describe different package levels of an item or hierarchies of Items.

WG Approval: 19/05/2022


"""@en ;
    rdfs:isDefinedBy <http://data.europa.eu/a4g/ontology> ;
    rdfs:subClassOf :ItemRelation ;
    owl:disjointWith :ItemAccessoryRelation,
        :ItemComplementaryRelation,
        :ItemReplacement,
        :ItemRequirement ;
    skos:definition """Inclusion of an Item into in the described Item.

Additional Information:
The Item is provided with its components, however, the component Items may also be provided separately. 
For example, a bicycle has wheels as components, but they may be provided as spare parts as well. 
This relation is useful to describe different package levels of an item or hierarchies of Items.

WG Approval: 19/05/2022


"""@en ;
    skos:prefLabel "Item composition"@en .

:ItemReplacement a owl:Class ;
    rdfs:label "Item replacement"@en ;
    rdfs:comment """Supplantment, displacement or suspension of an Item by the described Item.

WG Approval: 30/06/2022
"""@en ;
    rdfs:isDefinedBy <http://data.europa.eu/a4g/ontology> ;
    rdfs:subClassOf :ItemRelation ;
    owl:disjointWith :ItemAccessoryRelation,
        :ItemComplementaryRelation,
        :ItemComposition,
        :ItemRequirement ;
    skos:definition """Supplantment, displacement or suspension of an Item by the described Item.

WG Approval: 30/06/2022
"""@en ;
    skos:prefLabel "Item replacement"@en .

:ItemRequirement a owl:Class ;
    rdfs:label "Item requirement"@en ;
    rdfs:comment """Necessity of an Item by the described item. 

Additional Information:
The described item is provided without other items that are required for proper functionality.

For example, a printer cannot be used without ink cartridge; or a Server cannot be used without its installation. 

WG Approval: 19/05/2022

"""@en ;
    rdfs:isDefinedBy <http://data.europa.eu/a4g/ontology> ;
    rdfs:subClassOf :ItemRelation ;
    owl:disjointWith :ItemAccessoryRelation,
        :ItemComplementaryRelation,
        :ItemComposition,
        :ItemReplacement ;
    skos:definition """Necessity of an Item by the described item. 

Additional Information:
The described item is provided without other items that are required for proper functionality.

For example, a printer cannot be used without ink cartridge; or a Server cannot be used without its installation. 

WG Approval: 19/05/2022

"""@en ;
    skos:prefLabel "Item requirement"@en .

:ItemRelation a owl:Class ;
    rdfs:label "Item relation"@en ;
    rdfs:comment """Connection between two Items.

WG Approval: 30/06/2022
"""@en ;
    rdfs:isDefinedBy <http://data.europa.eu/a4g/ontology> ;
    skos:definition """Connection between two Items.

WG Approval: 30/06/2022
"""@en ;
    skos:prefLabel "Item relation"@en .

<http://data.europa.eu/a4g/ontology> a owl:Ontology ;
    rdfs:label "eProcurement Ontology - eCatalogue"@en ;
    cc:attributionName "PublicationsOffice of the European Union" ;
    cc:attributionURL <http://publications.europa.eu/resource/authority/corporate-body/PUBL> ;
    dc:contributor [ a foaf:Person ;
            foaf:name "Natalie" ;
            foaf:surname "Muric" ;
            schema:affiliation [ foaf:name "Publications Office of the European Union" ] ],
        [ a foaf:Person ;
            foaf:name "Andreea" ;
            foaf:surname "Pasare" ;
            schema:affiliation [ foaf:name "Meaningfy" ;
                    foaf:page <http://meaningfy.ws> ] ],
        [ a foaf:Person ;
            foaf:homepage <http://costezki.ro> ;
            foaf:name "Eugeniu" ;
            foaf:surname "Costetchi" ;
            schema:affiliation [ foaf:name "Meaningfy" ;
                    foaf:page <http://meaningfy.ws> ] ] ;
    dc:rights "This ontology is licenced under CC BY-SA 4.0 - http://creativecommons.org/licenses/by-sa/4.0/" ;
    dcterms:creator [ a foaf:Person ;
            foaf:name "eProcurement Ontology Working Group" ] ;
    dcterms:date "2023-06-22"^^xsd:date ;
    dcterms:description """
        This module provides the definitions for the eCatalogue of eProcurement ontology.
        Procurement data has been identified as data with a high-reuse potential.
        Given the increasing importance of data standards for eProcurement, a number of initiatives
        driven by the public sector, the industry and academia have been kick-started in recent years.
        Some have grown organically, while others are the result of standardisation work.
        The vocabularies and the semantics that they are introducing, the phases of public procurement that they are covering,
        and the technologies that they are using all differ. These differences hamper data interoperability and thus its reuse by them or by the wider public.
        This creates the need for a common data standard for publishing procurement data, hence allowing data
        from different sources to be easily accessed and linked, and consequently reused.
    """@en ;
    dcterms:license <http://creativecommons.org/licenses/by-sa/4.0/> ;
    dcterms:title "eProcurement Ontology - eCatalogue"@en ;
    vann:preferredNamespacePrefix "epo" ;
    vann:preferredNamespaceUri "http://data.europa.eu/a4g/ontology#" ;
    rdfs:comment "This version is automatically generated from eCatalogue_CM.xml on 2023-06-22" ;
    rdfs:seeAlso <https://github.com/eprocurementontology/eprocurementontology>,
        <https://joinup.ec.europa.eu/collection/eprocurement/solution/eprocurement-ontology/about>,
        <https://op.europa.eu/en/web/eu-vocabularies/e-procurement> ;
    owl:imports dcterms:,
        <http://www.w3.org/2004/02/skos/core> ;
    owl:incompatibleWith "2.x.x" ;
    owl:versionIRI :eCatalogue_CM.xml-2023-06-22 ;
    owl:versionInfo "3.1.0" .

