<?xml version="1.0" encoding="UTF-8"?>
<rdf:RDF xmlns="http://data.europa.eu/a4g/ontology#"
         xmlns:cc="http://creativecommons.org/ns#"
         xmlns:dc="http://www.omg.org/spec/UML/20131001/UMLDC"
         xmlns:dct="http://purl.org/dc/terms/"
         xmlns:epo="http://data.europa.eu/a4g/ontology#"
         xmlns:epor="http://data.europa.eu/a4g/rule#"
         xmlns:epos="http://data.europa.eu/a4g/shape#"
         xmlns:foaf="http://xmlns.com/foaf/0.1/"
         xmlns:org="http://www.w3.org/ns/org#"
         xmlns:owl="http://www.w3.org/2002/07/owl#"
         xmlns:rdf="http://www.w3.org/1999/02/22-rdf-syntax-ns#"
         xmlns:rdfs="http://www.w3.org/2000/01/rdf-schema#"
         xmlns:skos="http://www.w3.org/2004/02/skos/core#"
         xmlns:vann="http://purl.org/vocab/vann/"
         xml:base="http://data.europa.eu/a4g/ontology">
   <owl:Ontology rdf:about="http://data.europa.eu/a4g/ontology">
            <!-- Imports -->
            <owl:imports rdf:resource="http://purl.org/dc/terms/"/>
            <owl:imports rdf:resource="http://www.w3.org/2004/02/skos/core"/>

            <!-- Descriptive metadata -->
            <dct:title xml:lang="en">eProcurement core ontology</dct:title>
            <dct:date rdf:datatype="http://www.w3.org/2001/XMLSchema#date">2022-09-23</dct:date>
            <owl:versionInfo>3.0.1</owl:versionInfo>
            <owl:versionIRI rdf:resource="http://data.europa.eu/a4g/ontology#version-3.0.1"/>
            <owl:incompatibleWith>2.x.x</owl:incompatibleWith>
            <dct:description xml:lang="en">This module provides the definitions for the core eProcurement ontology.

        Procurement data has been identified as data with a
        high-reuse potential. Given the increasing importance of data standards for
        eProcurement, a number of initiatives driven by the public sector, the industry and
        academia have been kick-started in recent years. Some have grown organically, while
        others are the result of standardisation work. The vocabularies and the semantics that
        they are introducing, the phases of public procurement that they are covering, and the
        technologies that they are using all differ. These differences hamper data
        interoperability and thus its reuse by them or by the wider public. This creates the
        need for a common data standard for publishing procurement data, hence allowing data
        from different sources to be easily accessed and linked, and consequently
        reused.</dct:description>
            <vann:preferredNamespacePrefix>epo</vann:preferredNamespacePrefix>
            <vann:preferredNamespaceUri>http://data.europa.eu/a4g/ontology#</vann:preferredNamespaceUri>
            <rdfs:comment>eProcurement core ontology version generated automatically from ePO_CM.xml on 23/09/2022</rdfs:comment>
            <rdfs:seeAlso rdf:resource="https://op.europa.eu/en/web/eu-vocabularies/e-procurement"/>
            <rdfs:seeAlso rdf:resource="https://joinup.ec.europa.eu/collection/eprocurement/solution/eprocurement-ontology"/>
            <rdfs:seeAlso rdf:resource="https://docs.ted.europa.eu/EPO/dev/index.html"/>
            <dct:license rdf:resource="http://creativecommons.org/licenses/by-sa/4.0/"/>
            <dc:rights>This ontology is licenced under CC BY-SA 4.0 - http://creativecommons.org/licenses/by-sa/4.0/</dc:rights>
            <cc:attributionName>Publications Office of the European Union</cc:attributionName>
            <cc:attributionURL rdf:resource="http://publications.europa.eu/resource/authority/corporate-body/PUBL"/>

            <dc:contributor>
                  <foaf:Person>
                        <foaf:name>Eugeniu</foaf:name>
                        <foaf:surname>Costetchi</foaf:surname>
                        <foaf:homepage rdf:resource="http://costezki.ro"/>
                        <schema:affiliation rdf:parseType="Resource">
                              <foaf:name>Meaningfy</foaf:name>
                              <foaf:page rdf:resource="http://meaningfy.ws"/>
                        </schema:affiliation>
                  </foaf:Person>
            </dc:contributor>

            <dc:contributor>
                  <foaf:Person>
                        <foaf:name>Andreea</foaf:name>
                        <foaf:surname>Pasare</foaf:surname>
                        <schema:affiliation rdf:parseType="Resource">
                              <foaf:name>Meaningfy</foaf:name>
                              <foaf:page rdf:resource="http://meaningfy.ws"/>
                        </schema:affiliation>
                  </foaf:Person>
            </dc:contributor>

            <dc:contributor>
                  <foaf:Person>
                        <foaf:name>Natalie</foaf:name>
                        <foaf:surname>Muric</foaf:surname>
                        <schema:affiliation rdf:parseType="Resource">
                              <foaf:name>Publications Office of the European Union</foaf:name>
                        </schema:affiliation>
                  </foaf:Person>
            </dc:contributor>

            <dct:creator>
                  <foaf:Person>
                        <foaf:name>eProcurement Ontology Working Group</foaf:name>
                  </foaf:Person>
            </dct:creator>

      </owl:Ontology>
   <owl:Class rdf:about="http://data.europa.eu/a4g/ontology#Brand">
      <rdfs:label xml:lang="en">Brand</rdfs:label>
      <skos:prefLabel xml:lang="en">Brand</skos:prefLabel>
      <rdfs:comment xml:lang="en">Name given by an organisation to its product or service, or range of products or services. 

Additional information:
Brand name allows economic operators to distinctively describe an item in their eCatalogue. This may be different from the "item name".

WG acceptance 10/03/2022
</rdfs:comment>
      <skos:definition xml:lang="en">Name given by an organisation to its product or service, or range of products or services. 

Additional information:
Brand name allows economic operators to distinctively describe an item in their eCatalogue. This may be different from the "item name".

WG acceptance 10/03/2022
</skos:definition>
      <rdfs:isDefinedBy rdf:resource="http://data.europa.eu/a4g/ontology"/>
   </owl:Class>
   <owl:Class rdf:about="http://data.europa.eu/a4g/ontology#CatalogueDocument">
      <rdfs:label xml:lang="en">Catalogue document</rdfs:label>
      <skos:prefLabel xml:lang="en">Catalogue document</skos:prefLabel>
      <rdfs:comment xml:lang="en">A document containing a catalogue.

Additional Information:
A complete catalogue is provided in such a document.</rdfs:comment>
      <skos:definition xml:lang="en">A document containing a catalogue.

Additional Information:
A complete catalogue is provided in such a document.</skos:definition>
      <rdfs:isDefinedBy rdf:resource="http://data.europa.eu/a4g/ontology"/>
   </owl:Class>
   <owl:Class rdf:about="http://data.europa.eu/a4g/ontology#CatalogueFragment">
      <rdfs:label xml:lang="en">Catalogue fragment</rdfs:label>
      <skos:prefLabel xml:lang="en">Catalogue fragment</skos:prefLabel>
      <rdfs:comment xml:lang="en">A part of the catalogue.

Additional Information:
The catalogue fragment generally represents a difference between two catalogue versions, but there may be other use cases.</rdfs:comment>
      <skos:definition xml:lang="en">A part of the catalogue.

Additional Information:
The catalogue fragment generally represents a difference between two catalogue versions, but there may be other use cases.</skos:definition>
      <rdfs:isDefinedBy rdf:resource="http://data.europa.eu/a4g/ontology"/>
   </owl:Class>
   <owl:Class rdf:about="http://data.europa.eu/a4g/ontology#CatalogueUpdateDocument">
      <rdfs:label xml:lang="en">Catalogue update document</rdfs:label>
      <skos:prefLabel xml:lang="en">Catalogue update document</skos:prefLabel>
      <rdfs:comment xml:lang="en">A document containing only a fragment of a catalogue expected to alter an existing complete catalogue evolving it to its subsequent version.

Additional Information:
One or more catalogue fragments can be provided in such a document. Each fragment has its own update/alteration action.
</rdfs:comment>
      <skos:definition xml:lang="en">A document containing only a fragment of a catalogue expected to alter an existing complete catalogue evolving it to its subsequent version.

Additional Information:
One or more catalogue fragments can be provided in such a document. Each fragment has its own update/alteration action.
</skos:definition>
      <rdfs:isDefinedBy rdf:resource="http://data.europa.eu/a4g/ontology"/>
   </owl:Class>
   <owl:Class rdf:about="http://data.europa.eu/a4g/ontology#CertificationLabel">
      <rdfs:label xml:lang="en">Certification label</rdfs:label>
      <skos:prefLabel xml:lang="en">Certification label</skos:prefLabel>
      <rdfs:comment xml:lang="en">Concept that stands for a set of norms, expectations, standards and policies.

Additional Information:
Such standards may relate to social, ethical and quality etc.

WG approval 26/07/2022
</rdfs:comment>
      <skos:definition xml:lang="en">Concept that stands for a set of norms, expectations, standards and policies.

Additional Information:
Such standards may relate to social, ethical and quality etc.

WG approval 26/07/2022
</skos:definition>
      <rdfs:isDefinedBy rdf:resource="http://data.europa.eu/a4g/ontology"/>
   </owl:Class>
   <owl:Class rdf:about="http://data.europa.eu/a4g/ontology#Certifier">
      <rdfs:label xml:lang="en">Certifier</rdfs:label>
      <skos:prefLabel xml:lang="en">Certifier</skos:prefLabel>
      <rdfs:comment xml:lang="en">A role of an agent that assesses the conformance of an Item to a set of requirements and grants the certificate as a proof of conformance.

WG approval 26/07/2022</rdfs:comment>
      <skos:definition xml:lang="en">A role of an agent that assesses the conformance of an Item to a set of requirements and grants the certificate as a proof of conformance.

WG approval 26/07/2022</skos:definition>
      <rdfs:isDefinedBy rdf:resource="http://data.europa.eu/a4g/ontology"/>
   </owl:Class>
   <owl:Class rdf:about="http://data.europa.eu/a4g/ontology#ChargeInformation">
      <rdfs:label xml:lang="en">Charge information</rdfs:label>
      <skos:prefLabel xml:lang="en">Charge information</skos:prefLabel>
      <rdfs:comment xml:lang="en">A tax, fee or duty imposed on the item.

Additional Information:
Charge category indicates the nature of the tax/duty/fee, for example VAT, CAR, etc.
Charge category modifier may be used in case different levels, exemptions or other modifications apply.
The charge can be fixed or relative to the price.</rdfs:comment>
      <skos:definition xml:lang="en">A tax, fee or duty imposed on the item.

Additional Information:
Charge category indicates the nature of the tax/duty/fee, for example VAT, CAR, etc.
Charge category modifier may be used in case different levels, exemptions or other modifications apply.
The charge can be fixed or relative to the price.</skos:definition>
      <rdfs:isDefinedBy rdf:resource="http://data.europa.eu/a4g/ontology"/>
   </owl:Class>
   <owl:Class rdf:about="http://data.europa.eu/a4g/ontology#ItemAccessoryRelation">
      <rdfs:label xml:lang="en">Item accessory relation</rdfs:label>
      <skos:prefLabel xml:lang="en">Item accessory relation</skos:prefLabel>
      <rdfs:comment xml:lang="en">Combination of two items where the former enhances the latter.

WG Approval: 30/06/2022
</rdfs:comment>
      <skos:definition xml:lang="en">Combination of two items where the former enhances the latter.

WG Approval: 30/06/2022
</skos:definition>
      <rdfs:isDefinedBy rdf:resource="http://data.europa.eu/a4g/ontology"/>
   </owl:Class>
   <owl:Class rdf:about="http://data.europa.eu/a4g/ontology#ItemCertificate">
      <rdfs:label xml:lang="en">Item certificate</rdfs:label>
      <skos:prefLabel xml:lang="en">Item certificate</skos:prefLabel>
      <rdfs:comment xml:lang="en">Proof that an item is conformant.</rdfs:comment>
      <skos:definition xml:lang="en">Proof that an item is conformant.</skos:definition>
      <rdfs:isDefinedBy rdf:resource="http://data.europa.eu/a4g/ontology"/>
   </owl:Class>
   <owl:Class rdf:about="http://data.europa.eu/a4g/ontology#ItemComplementaryRelation">
      <rdfs:label xml:lang="en">Item complementary relation</rdfs:label>
      <skos:prefLabel xml:lang="en">Item complementary relation</skos:prefLabel>
      <rdfs:comment xml:lang="en">Combination of two items which mutually enhance one another.

WG Approval: 30/06/2022

</rdfs:comment>
      <skos:definition xml:lang="en">Combination of two items which mutually enhance one another.

WG Approval: 30/06/2022

</skos:definition>
      <rdfs:isDefinedBy rdf:resource="http://data.europa.eu/a4g/ontology"/>
   </owl:Class>
   <owl:Class rdf:about="http://data.europa.eu/a4g/ontology#ItemComposition">
      <rdfs:label xml:lang="en">Item composition</rdfs:label>
      <skos:prefLabel xml:lang="en">Item composition</skos:prefLabel>
      <rdfs:comment xml:lang="en">Inclusion of an Item into in the described Item.

Additional Information:
The item is provided with its components, however, the component items may also be provided separately. 
For example, a bicycle has wheels as components, but they may be provided as spare parts as well. 
This relation is useful to describe different package levels of an item or hierarchies of items.

WG Approval: 19/05/2022


</rdfs:comment>
      <skos:definition xml:lang="en">Inclusion of an Item into in the described Item.

Additional Information:
The item is provided with its components, however, the component items may also be provided separately. 
For example, a bicycle has wheels as components, but they may be provided as spare parts as well. 
This relation is useful to describe different package levels of an item or hierarchies of items.

WG Approval: 19/05/2022


</skos:definition>
      <rdfs:isDefinedBy rdf:resource="http://data.europa.eu/a4g/ontology"/>
   </owl:Class>
   <owl:Class rdf:about="http://data.europa.eu/a4g/ontology#ItemDescription">
      <rdfs:label xml:lang="en">Item description</rdfs:label>
      <skos:prefLabel xml:lang="en">Item description</skos:prefLabel>
      <rdfs:comment xml:lang="en">Construct meant to represent the association between an attribute defined in an external classification scheme and the value ascribed to it.

WG approval 26/07/2022</rdfs:comment>
      <skos:definition xml:lang="en">Construct meant to represent the association between an attribute defined in an external classification scheme and the value ascribed to it.

WG approval 26/07/2022</skos:definition>
      <rdfs:isDefinedBy rdf:resource="http://data.europa.eu/a4g/ontology"/>
   </owl:Class>
   <owl:Class rdf:about="http://data.europa.eu/a4g/ontology#ItemModel">
      <rdfs:label xml:lang="en">Item model</rdfs:label>
      <skos:prefLabel xml:lang="en">Item model</skos:prefLabel>
      <rdfs:comment xml:lang="en">A specific design or version of a product or service.

Additional information:
This class is meant as a reusable reference to the model name rather than as a set of specifications of an item of this particular model. 

WG acceptance 10/03/2022

</rdfs:comment>
      <skos:definition xml:lang="en">A specific design or version of a product or service.

Additional information:
This class is meant as a reusable reference to the model name rather than as a set of specifications of an item of this particular model. 

WG acceptance 10/03/2022

</skos:definition>
      <rdfs:isDefinedBy rdf:resource="http://data.europa.eu/a4g/ontology"/>
   </owl:Class>
   <owl:Class rdf:about="http://data.europa.eu/a4g/ontology#ItemRelation">
      <rdfs:label xml:lang="en">Item relation</rdfs:label>
      <skos:prefLabel xml:lang="en">Item relation</skos:prefLabel>
      <rdfs:comment xml:lang="en">Connection between two items.

WG Approval: 30/06/2022
</rdfs:comment>
      <skos:definition xml:lang="en">Connection between two items.

WG Approval: 30/06/2022
</skos:definition>
      <rdfs:isDefinedBy rdf:resource="http://data.europa.eu/a4g/ontology"/>
   </owl:Class>
   <owl:Class rdf:about="http://data.europa.eu/a4g/ontology#ItemReplacement">
      <rdfs:label xml:lang="en">Item replacement</rdfs:label>
      <skos:prefLabel xml:lang="en">Item replacement</skos:prefLabel>
      <rdfs:comment xml:lang="en">Supplantment, displacement or suspension of an Item by the described Item.

WG Approval: 30/06/2022
</rdfs:comment>
      <skos:definition xml:lang="en">Supplantment, displacement or suspension of an Item by the described Item.

WG Approval: 30/06/2022
</skos:definition>
      <rdfs:isDefinedBy rdf:resource="http://data.europa.eu/a4g/ontology"/>
   </owl:Class>
   <owl:Class rdf:about="http://data.europa.eu/a4g/ontology#ItemRequirement">
      <rdfs:label xml:lang="en">Item requirement</rdfs:label>
      <skos:prefLabel xml:lang="en">Item requirement</skos:prefLabel>
      <rdfs:comment xml:lang="en">Necessity of an item by the described item. 

Additional Information:
The described item is provided without other items that are required for proper functionality.

For example, a printer cannot be used without ink cartridge; or a Server cannot be used without its installation. 

WG Approval: 19/05/2022

</rdfs:comment>
      <skos:definition xml:lang="en">Necessity of an item by the described item. 

Additional Information:
The described item is provided without other items that are required for proper functionality.

For example, a printer cannot be used without ink cartridge; or a Server cannot be used without its installation. 

WG Approval: 19/05/2022

</skos:definition>
      <rdfs:isDefinedBy rdf:resource="http://data.europa.eu/a4g/ontology"/>
   </owl:Class>
   <owl:Class rdf:about="http://data.europa.eu/a4g/ontology#Price">
      <rdfs:label xml:lang="en">Price</rdfs:label>
      <skos:prefLabel xml:lang="en">Price</skos:prefLabel>
      <rdfs:comment xml:lang="en">Amount of money required or given in exchange for items.

Additional information:
The price excludes any charges (such as taxes, duties and fees) and discounts.

WG approval 26/07/2022</rdfs:comment>
      <skos:definition xml:lang="en">Amount of money required or given in exchange for items.

Additional information:
The price excludes any charges (such as taxes, duties and fees) and discounts.

WG approval 26/07/2022</skos:definition>
      <rdfs:isDefinedBy rdf:resource="http://data.europa.eu/a4g/ontology"/>
   </owl:Class>
   <owl:Class rdf:about="http://data.europa.eu/a4g/ontology#ProductSpecification">
      <rdfs:label xml:lang="en">Product specification</rdfs:label>
      <skos:prefLabel xml:lang="en">Product specification</skos:prefLabel>
      <rdfs:comment xml:lang="en">Document providing information about an Item. 

WG approval 07/04/2022

</rdfs:comment>
      <skos:definition xml:lang="en">Document providing information about an Item. 

WG approval 07/04/2022

</skos:definition>
      <rdfs:isDefinedBy rdf:resource="http://data.europa.eu/a4g/ontology"/>
   </owl:Class>
   <owl:Class rdf:about="http://data.europa.eu/a4g/ontology#Manufacturer">
      <rdfs:label xml:lang="en">Manufacturer</rdfs:label>
      <skos:prefLabel xml:lang="en">Manufacturer</skos:prefLabel>
      <rdfs:comment xml:lang="en">The producer of goods or provider of services. 

Additional Information:
Also, known as Supplier and Manufacturer.

We do not care who provides these service or products we care with whom business is done.

PEPPOL - Invoice:
The supplier is the legal person or organization who provides a product and/or service.

PEPPOL - Order: The supplier is the legal person or organization who provides a product or service.
Examples of supplier roles: seller, despatch party, creditor, economic operator.

</rdfs:comment>
      <skos:definition xml:lang="en">The producer of goods or provider of services. 

Additional Information:
Also, known as Supplier and Manufacturer.

We do not care who provides these service or products we care with whom business is done.

PEPPOL - Invoice:
The supplier is the legal person or organization who provides a product and/or service.

PEPPOL - Order: The supplier is the legal person or organization who provides a product or service.
Examples of supplier roles: seller, despatch party, creditor, economic operator.

</skos:definition>
      <rdfs:isDefinedBy rdf:resource="http://data.europa.eu/a4g/ontology"/>
   </owl:Class>
   <owl:Class rdf:about="http://data.europa.eu/a4g/ontology#Catalogue">
      <rdfs:label xml:lang="en">Catalogue</rdfs:label>
      <skos:prefLabel xml:lang="en">Catalogue</skos:prefLabel>
      <rdfs:comment xml:lang="en">A describing a set of items offered for purchase that can be processed in an electronic way.
</rdfs:comment>
      <skos:definition xml:lang="en">A describing a set of items offered for purchase that can be processed in an electronic way.
</skos:definition>
      <rdfs:isDefinedBy rdf:resource="http://data.europa.eu/a4g/ontology"/>
   </owl:Class>
   <owl:Class rdf:about="http://data.europa.eu/a4g/ontology#CatalogueLine">
      <rdfs:label xml:lang="en">Catalogue line</rdfs:label>
      <skos:prefLabel xml:lang="en">Catalogue line</skos:prefLabel>
      <rdfs:comment xml:lang="en">Aggregated information about the terms and specifications for procuring an item.


Details about an item, like prices, packaging, discounts, special promotions, etc.


TC 440:

Detailed information of an item, price and its composition in a Catalogue.

Composition: e.g. information referring to its description, how to order it, what it is made of, properties, delivery conditions, etc.





</rdfs:comment>
      <skos:definition xml:lang="en">Aggregated information about the terms and specifications for procuring an item.


Details about an item, like prices, packaging, discounts, special promotions, etc.


TC 440:

Detailed information of an item, price and its composition in a Catalogue.

Composition: e.g. information referring to its description, how to order it, what it is made of, properties, delivery conditions, etc.





</skos:definition>
      <rdfs:isDefinedBy rdf:resource="http://data.europa.eu/a4g/ontology"/>
   </owl:Class>
   <owl:Class rdf:about="http://data.europa.eu/a4g/ontology#Batch">
      <rdfs:label xml:lang="en">Batch</rdfs:label>
      <skos:prefLabel xml:lang="en">Batch</skos:prefLabel>
      <rdfs:comment xml:lang="en">A production lot in which the item instances were produced. 

WG Acceptance 10/03/2022
</rdfs:comment>
      <skos:definition xml:lang="en">A production lot in which the item instances were produced. 

WG Acceptance 10/03/2022
</skos:definition>
      <rdfs:isDefinedBy rdf:resource="http://data.europa.eu/a4g/ontology"/>
   </owl:Class>
   <owl:Class rdf:about="http://data.europa.eu/a4g/ontology#Item">
      <rdfs:label xml:lang="en">Item</rdfs:label>
      <skos:prefLabel xml:lang="en">Item</skos:prefLabel>
      <rdfs:comment xml:lang="en">A product, work, service or any combination of them.

Additional Information:
An item can be an atomic thing or a composition of things that together are seen as a unit, e.g. a tetrabrik of milk or an indivisible package of six tetrabriks.

No distinction is provided between services, goods and works to leave room for innovation.

WG approval 30/06/2022</rdfs:comment>
      <skos:definition xml:lang="en">A product, work, service or any combination of them.

Additional Information:
An item can be an atomic thing or a composition of things that together are seen as a unit, e.g. a tetrabrik of milk or an indivisible package of six tetrabriks.

No distinction is provided between services, goods and works to leave room for innovation.

WG approval 30/06/2022</skos:definition>
      <rdfs:isDefinedBy rdf:resource="http://data.europa.eu/a4g/ontology"/>
   </owl:Class>
   <rdfs:Datatype rdf:about="http://www.w3.org/2000/01/rdf-schema#Literal">
      <rdfs:label xml:lang="en">Literal</rdfs:label>
      <skos:prefLabel xml:lang="en">Literal</skos:prefLabel>
   </rdfs:Datatype>
   <rdfs:Datatype rdf:about="http://www.w3.org/2001/XMLSchema#AnyURI">
      <rdfs:label xml:lang="en">Any u r i</rdfs:label>
      <skos:prefLabel xml:lang="en">Any u r i</skos:prefLabel>
   </rdfs:Datatype>
   <rdfs:Datatype rdf:about="http://www.w3.org/2001/XMLSchema#Boolean">
      <rdfs:label xml:lang="en">Boolean</rdfs:label>
      <skos:prefLabel xml:lang="en">Boolean</skos:prefLabel>
   </rdfs:Datatype>
   <rdfs:Datatype rdf:about="http://www.w3.org/2001/XMLSchema#Date">
      <rdfs:label xml:lang="en">Date</rdfs:label>
      <skos:prefLabel xml:lang="en">Date</skos:prefLabel>
   </rdfs:Datatype>
   <rdfs:Datatype rdf:about="http://www.w3.org/2001/XMLSchema#DateTime">
      <rdfs:label xml:lang="en">Date time</rdfs:label>
      <skos:prefLabel xml:lang="en">Date time</skos:prefLabel>
   </rdfs:Datatype>
   <rdfs:Datatype rdf:about="http://www.w3.org/2001/XMLSchema#Decimal">
      <rdfs:label xml:lang="en">Decimal</rdfs:label>
      <skos:prefLabel xml:lang="en">Decimal</skos:prefLabel>
   </rdfs:Datatype>
   <rdfs:Datatype rdf:about="http://www.w3.org/2001/XMLSchema#Integer">
      <rdfs:label xml:lang="en">Integer</rdfs:label>
      <skos:prefLabel xml:lang="en">Integer</skos:prefLabel>
   </rdfs:Datatype>
   <owl:Class rdf:about="http://data.europa.eu/a4g/ontology#CatalogueFragment">
      <rdfs:subClassOf rdf:resource="http://data.europa.eu/a4g/ontology#Catalogue"/>
   </owl:Class>
   <owl:Class rdf:about="http://data.europa.eu/a4g/ontology#ItemAccessoryRelation">
      <rdfs:subClassOf rdf:resource="http://data.europa.eu/a4g/ontology#ItemRelation"/>
   </owl:Class>
   <rdf:Description rdf:about="http://data.europa.eu/a4g/ontology#ItemAccessoryRelation">
      <owl:disjointWith rdf:resource="http://data.europa.eu/a4g/ontology#ItemComplementaryRelation"/>
   </rdf:Description>
   <rdf:Description rdf:about="http://data.europa.eu/a4g/ontology#ItemAccessoryRelation">
      <owl:disjointWith rdf:resource="http://data.europa.eu/a4g/ontology#ItemComposition"/>
   </rdf:Description>
   <rdf:Description rdf:about="http://data.europa.eu/a4g/ontology#ItemAccessoryRelation">
      <owl:disjointWith rdf:resource="http://data.europa.eu/a4g/ontology#ItemReplacement"/>
   </rdf:Description>
   <rdf:Description rdf:about="http://data.europa.eu/a4g/ontology#ItemAccessoryRelation">
      <owl:disjointWith rdf:resource="http://data.europa.eu/a4g/ontology#ItemRequirement"/>
   </rdf:Description>
   <owl:Class rdf:about="http://data.europa.eu/a4g/ontology#ItemComplementaryRelation">
      <rdfs:subClassOf rdf:resource="http://data.europa.eu/a4g/ontology#ItemRelation"/>
   </owl:Class>
   <rdf:Description rdf:about="http://data.europa.eu/a4g/ontology#ItemComplementaryRelation">
      <owl:disjointWith rdf:resource="http://data.europa.eu/a4g/ontology#ItemAccessoryRelation"/>
   </rdf:Description>
   <rdf:Description rdf:about="http://data.europa.eu/a4g/ontology#ItemComplementaryRelation">
      <owl:disjointWith rdf:resource="http://data.europa.eu/a4g/ontology#ItemComposition"/>
   </rdf:Description>
   <rdf:Description rdf:about="http://data.europa.eu/a4g/ontology#ItemComplementaryRelation">
      <owl:disjointWith rdf:resource="http://data.europa.eu/a4g/ontology#ItemReplacement"/>
   </rdf:Description>
   <rdf:Description rdf:about="http://data.europa.eu/a4g/ontology#ItemComplementaryRelation">
      <owl:disjointWith rdf:resource="http://data.europa.eu/a4g/ontology#ItemRequirement"/>
   </rdf:Description>
   <owl:Class rdf:about="http://data.europa.eu/a4g/ontology#ItemComposition">
      <rdfs:subClassOf rdf:resource="http://data.europa.eu/a4g/ontology#ItemRelation"/>
   </owl:Class>
   <rdf:Description rdf:about="http://data.europa.eu/a4g/ontology#ItemComposition">
      <owl:disjointWith rdf:resource="http://data.europa.eu/a4g/ontology#ItemAccessoryRelation"/>
   </rdf:Description>
   <rdf:Description rdf:about="http://data.europa.eu/a4g/ontology#ItemComposition">
      <owl:disjointWith rdf:resource="http://data.europa.eu/a4g/ontology#ItemComplementaryRelation"/>
   </rdf:Description>
   <rdf:Description rdf:about="http://data.europa.eu/a4g/ontology#ItemComposition">
      <owl:disjointWith rdf:resource="http://data.europa.eu/a4g/ontology#ItemReplacement"/>
   </rdf:Description>
   <rdf:Description rdf:about="http://data.europa.eu/a4g/ontology#ItemComposition">
      <owl:disjointWith rdf:resource="http://data.europa.eu/a4g/ontology#ItemRequirement"/>
   </rdf:Description>
   <owl:Class rdf:about="http://data.europa.eu/a4g/ontology#ItemReplacement">
      <rdfs:subClassOf rdf:resource="http://data.europa.eu/a4g/ontology#ItemRelation"/>
   </owl:Class>
   <rdf:Description rdf:about="http://data.europa.eu/a4g/ontology#ItemReplacement">
      <owl:disjointWith rdf:resource="http://data.europa.eu/a4g/ontology#ItemAccessoryRelation"/>
   </rdf:Description>
   <rdf:Description rdf:about="http://data.europa.eu/a4g/ontology#ItemReplacement">
      <owl:disjointWith rdf:resource="http://data.europa.eu/a4g/ontology#ItemComplementaryRelation"/>
   </rdf:Description>
   <rdf:Description rdf:about="http://data.europa.eu/a4g/ontology#ItemReplacement">
      <owl:disjointWith rdf:resource="http://data.europa.eu/a4g/ontology#ItemComposition"/>
   </rdf:Description>
   <rdf:Description rdf:about="http://data.europa.eu/a4g/ontology#ItemReplacement">
      <owl:disjointWith rdf:resource="http://data.europa.eu/a4g/ontology#ItemRequirement"/>
   </rdf:Description>
   <owl:Class rdf:about="http://data.europa.eu/a4g/ontology#ItemRequirement">
      <rdfs:subClassOf rdf:resource="http://data.europa.eu/a4g/ontology#ItemRelation"/>
   </owl:Class>
   <rdf:Description rdf:about="http://data.europa.eu/a4g/ontology#ItemRequirement">
      <owl:disjointWith rdf:resource="http://data.europa.eu/a4g/ontology#ItemAccessoryRelation"/>
   </rdf:Description>
   <rdf:Description rdf:about="http://data.europa.eu/a4g/ontology#ItemRequirement">
      <owl:disjointWith rdf:resource="http://data.europa.eu/a4g/ontology#ItemComplementaryRelation"/>
   </rdf:Description>
   <rdf:Description rdf:about="http://data.europa.eu/a4g/ontology#ItemRequirement">
      <owl:disjointWith rdf:resource="http://data.europa.eu/a4g/ontology#ItemComposition"/>
   </rdf:Description>
   <rdf:Description rdf:about="http://data.europa.eu/a4g/ontology#ItemRequirement">
      <owl:disjointWith rdf:resource="http://data.europa.eu/a4g/ontology#ItemReplacement"/>
   </rdf:Description>
   <owl:ObjectProperty rdf:about="http://data.europa.eu/a4g/ontology#hasBrand">
      <rdfs:label xml:lang="en">Has brand</rdfs:label>
      <skos:prefLabel xml:lang="en">Has brand</skos:prefLabel>
      <rdfs:isDefinedBy rdf:resource="http://data.europa.eu/a4g/ontology"/>
   </owl:ObjectProperty>
   <owl:ObjectProperty rdf:about="http://data.europa.eu/a4g/ontology#instantiatesCatalogue">
      <rdfs:label xml:lang="en">Instantiates catalogue</rdfs:label>
      <skos:prefLabel xml:lang="en">Instantiates catalogue</skos:prefLabel>
      <rdfs:isDefinedBy rdf:resource="http://data.europa.eu/a4g/ontology"/>
   </owl:ObjectProperty>
   <owl:ObjectProperty rdf:about="http://data.europa.eu/a4g/ontology#updatesCatalogue">
      <rdfs:label xml:lang="en">Updates catalogue</rdfs:label>
      <skos:prefLabel xml:lang="en">Updates catalogue</skos:prefLabel>
      <skos:definition xml:lang="en">Relation indicating (epo-cat:CatalogueFragment -&gt; epo-cat:Catalogue (+epo-cat:updatesCatalogue)) </skos:definition>
      <rdfs:comment xml:lang="en">Relation indicating (epo-cat:CatalogueFragment -&gt; epo-cat:Catalogue (+epo-cat:updatesCatalogue)) </rdfs:comment>
      <rdfs:isDefinedBy rdf:resource="http://data.europa.eu/a4g/ontology"/>
   </owl:ObjectProperty>
   <owl:ObjectProperty rdf:about="http://data.europa.eu/a4g/ontology#hasActivityCode">
      <rdfs:label xml:lang="en">Has activity code</rdfs:label>
      <skos:prefLabel xml:lang="en">Has activity code</skos:prefLabel>
      <skos:definition xml:lang="en">Code that defines how the line should be applied to an existing eCatalogue.
 (epo-cat:CatalogueFragment -&gt; epo-cat:activity-code (+epo-cat:hasActivityCode)) </skos:definition>
      <rdfs:comment xml:lang="en">Code that defines how the line should be applied to an existing eCatalogue.
 (epo-cat:CatalogueFragment -&gt; epo-cat:activity-code (+epo-cat:hasActivityCode)) </rdfs:comment>
      <rdfs:isDefinedBy rdf:resource="http://data.europa.eu/a4g/ontology"/>
   </owl:ObjectProperty>
   <owl:ObjectProperty rdf:about="http://data.europa.eu/a4g/ontology#announcesCatalogueFragment">
      <rdfs:label xml:lang="en">Announces catalogue fragment</rdfs:label>
      <skos:prefLabel xml:lang="en">Announces catalogue fragment</skos:prefLabel>
      <rdfs:isDefinedBy rdf:resource="http://data.europa.eu/a4g/ontology"/>
   </owl:ObjectProperty>
   <owl:ObjectProperty rdf:about="http://data.europa.eu/a4g/ontology#hasLabelType">
      <rdfs:label xml:lang="en">Has label type</rdfs:label>
      <skos:prefLabel xml:lang="en">Has label type</skos:prefLabel>
      <skos:scopeNote xml:lang="en">The label type such environmental, quality, social etc. (epo-cat:CertificationLabel -&gt; at-voc-new:certification-label-type (+epo-cat:hasLabelType)) </skos:scopeNote>
      <rdfs:comment xml:lang="en">The label type such environmental, quality, social etc. (epo-cat:CertificationLabel -&gt; at-voc-new:certification-label-type (+epo-cat:hasLabelType)) </rdfs:comment>
      <rdfs:isDefinedBy rdf:resource="http://data.europa.eu/a4g/ontology"/>
   </owl:ObjectProperty>
   <owl:ObjectProperty rdf:about="http://data.europa.eu/a4g/ontology#attestedByLabel">
      <rdfs:label xml:lang="en">Attested by label</rdfs:label>
      <skos:prefLabel xml:lang="en">Attested by label</skos:prefLabel>
      <skos:definition xml:lang="en">Relation indicating which label the certificate is about. 

WG approval 28/07/2022 (epo-cat:ItemCertificate -&gt; epo-cat:CertificationLabel (+epo-cat:attestedByLabel)) </skos:definition>
      <rdfs:comment xml:lang="en">Relation indicating which label the certificate is about. 

WG approval 28/07/2022 (epo-cat:ItemCertificate -&gt; epo-cat:CertificationLabel (+epo-cat:attestedByLabel)) </rdfs:comment>
      <rdfs:isDefinedBy rdf:resource="http://data.europa.eu/a4g/ontology"/>
   </owl:ObjectProperty>
   <owl:ObjectProperty rdf:about="http://data.europa.eu/a4g/ontology#issuedByCertifier">
      <rdfs:label xml:lang="en">Issued by certifier</rdfs:label>
      <skos:prefLabel xml:lang="en">Issued by certifier</skos:prefLabel>
      <skos:definition xml:lang="en">Relation indicating the Certifier responsible for providing the ItemCertificate.

Additional Information:
Certifier is a role played by an organisation.

WG approval 26/07/2022 (epo-cat:ItemCertificate -&gt; epo-cat:Certifier (+epo-cat:issuedByCertifier)) </skos:definition>
      <rdfs:comment xml:lang="en">Relation indicating the Certifier responsible for providing the ItemCertificate.

Additional Information:
Certifier is a role played by an organisation.

WG approval 26/07/2022 (epo-cat:ItemCertificate -&gt; epo-cat:Certifier (+epo-cat:issuedByCertifier)) </rdfs:comment>
      <rdfs:isDefinedBy rdf:resource="http://data.europa.eu/a4g/ontology"/>
   </owl:ObjectProperty>
   <owl:ObjectProperty rdf:about="http://data.europa.eu/a4g/ontology#hasChargeCategory">
      <rdfs:label xml:lang="en">Has charge category</rdfs:label>
      <skos:prefLabel xml:lang="en">Has charge category</skos:prefLabel>
      <rdfs:isDefinedBy rdf:resource="http://data.europa.eu/a4g/ontology"/>
   </owl:ObjectProperty>
   <owl:ObjectProperty rdf:about="http://data.europa.eu/a4g/ontology#hasChargeCategoryModifier">
      <rdfs:label xml:lang="en">Has charge category modifier</rdfs:label>
      <skos:prefLabel xml:lang="en">Has charge category modifier</skos:prefLabel>
      <rdfs:isDefinedBy rdf:resource="http://data.europa.eu/a4g/ontology"/>
   </owl:ObjectProperty>
   <owl:ObjectProperty rdf:about="http://data.europa.eu/a4g/ontology#hasChargeInformation">
      <rdfs:label xml:lang="en">Has charge information</rdfs:label>
      <skos:prefLabel xml:lang="en">Has charge information</skos:prefLabel>
      <rdfs:isDefinedBy rdf:resource="http://data.europa.eu/a4g/ontology"/>
   </owl:ObjectProperty>
   <owl:ObjectProperty rdf:about="http://data.europa.eu/a4g/ontology#hasValidityPeriod">
      <rdfs:label xml:lang="en">Has validity period</rdfs:label>
      <skos:prefLabel xml:lang="en">Has validity period</skos:prefLabel>
      <skos:definition xml:lang="en">The property indicating when the ItemCertificate is in force.

WG approval 26/07/2022 (epo-cat:ItemCertificate -&gt; epo:Period (+epo:hasValidityPeriod)) </skos:definition>
      <rdfs:comment xml:lang="en">The property indicating when the ItemCertificate is in force.

WG approval 26/07/2022 (epo-cat:ItemCertificate -&gt; epo:Period (+epo:hasValidityPeriod)) </rdfs:comment>
      <rdfs:isDefinedBy rdf:resource="http://data.europa.eu/a4g/ontology"/>
   </owl:ObjectProperty>
   <owl:ObjectProperty rdf:about="http://data.europa.eu/a4g/ontology#hasCertification">
      <rdfs:label xml:lang="en">Has certification</rdfs:label>
      <skos:prefLabel xml:lang="en">Has certification</skos:prefLabel>
      <skos:definition xml:lang="en">The property providing the proof of conformance.

WG approval 26/07/2022 (epo-cat:Item -&gt; epo-cat:ItemCertificate (+epo-cat:hasCertification)) </skos:definition>
      <rdfs:comment xml:lang="en">The property providing the proof of conformance.

WG approval 26/07/2022 (epo-cat:Item -&gt; epo-cat:ItemCertificate (+epo-cat:hasCertification)) </rdfs:comment>
      <rdfs:isDefinedBy rdf:resource="http://data.europa.eu/a4g/ontology"/>
   </owl:ObjectProperty>
   <owl:ObjectProperty rdf:about="http://data.europa.eu/a4g/ontology#describesItem">
      <rdfs:label xml:lang="en">Describes item</rdfs:label>
      <skos:prefLabel xml:lang="en">Describes item</skos:prefLabel>
      <rdfs:isDefinedBy rdf:resource="http://data.europa.eu/a4g/ontology"/>
   </owl:ObjectProperty>
   <owl:ObjectProperty rdf:about="http://data.europa.eu/a4g/ontology#hasQualifiedValue">
      <rdfs:label xml:lang="en">Has qualified value</rdfs:label>
      <skos:prefLabel xml:lang="en">Has qualified value</skos:prefLabel>
      <skos:definition xml:lang="en">Qualified value of the property, which is defined in a classification scheme.

Additional Information:
For example, the (0173-1#02-AAA026#007) drilling diameter of an item has value of 12 inches. 

WG approval 28/07/2022 (epo-cat:ItemDescription -&gt; epo:Quantity (+epo-cat:hasQualifiedValue)) </skos:definition>
      <rdfs:comment xml:lang="en">Qualified value of the property, which is defined in a classification scheme.

Additional Information:
For example, the (0173-1#02-AAA026#007) drilling diameter of an item has value of 12 inches. 

WG approval 28/07/2022 (epo-cat:ItemDescription -&gt; epo:Quantity (+epo-cat:hasQualifiedValue)) </rdfs:comment>
      <rdfs:isDefinedBy rdf:resource="http://data.europa.eu/a4g/ontology"/>
   </owl:ObjectProperty>
   <owl:ObjectProperty rdf:about="http://data.europa.eu/a4g/ontology#hasModel">
      <rdfs:label xml:lang="en">Has model</rdfs:label>
      <skos:prefLabel xml:lang="en">Has model</skos:prefLabel>
      <rdfs:isDefinedBy rdf:resource="http://data.europa.eu/a4g/ontology"/>
   </owl:ObjectProperty>
   <owl:ObjectProperty rdf:about="http://data.europa.eu/a4g/ontology#isRelatedToItem">
      <rdfs:label xml:lang="en">Is related to item</rdfs:label>
      <skos:prefLabel xml:lang="en">Is related to item</skos:prefLabel>
      <rdfs:isDefinedBy rdf:resource="http://data.europa.eu/a4g/ontology"/>
   </owl:ObjectProperty>
   <owl:ObjectProperty rdf:about="http://data.europa.eu/a4g/ontology#hasQualifiedItemRelation">
      <rdfs:label xml:lang="en">Has qualified item relation</rdfs:label>
      <skos:prefLabel xml:lang="en">Has qualified item relation</skos:prefLabel>
      <rdfs:isDefinedBy rdf:resource="http://data.europa.eu/a4g/ontology"/>
   </owl:ObjectProperty>
   <owl:ObjectProperty rdf:about="http://data.europa.eu/a4g/ontology#hasQuantityThreshold">
      <rdfs:label xml:lang="en">Has quantity threshold</rdfs:label>
      <skos:prefLabel xml:lang="en">Has quantity threshold</skos:prefLabel>
      <skos:scopeNote xml:lang="en">The minimum quantity of the item that can be ordered to the given net monetary value. (epo-cat:Price -&gt; epo:Quantity (+epo-cat:hasQuantityThreshold)) </skos:scopeNote>
      <rdfs:comment xml:lang="en">The minimum quantity of the item that can be ordered to the given net monetary value. (epo-cat:Price -&gt; epo:Quantity (+epo-cat:hasQuantityThreshold)) </rdfs:comment>
      <rdfs:isDefinedBy rdf:resource="http://data.europa.eu/a4g/ontology"/>
   </owl:ObjectProperty>
   <owl:ObjectProperty rdf:about="http://data.europa.eu/a4g/ontology#hasExpectedDeliveryTime">
      <rdfs:label xml:lang="en">Has expected delivery time</rdfs:label>
      <skos:prefLabel xml:lang="en">Has expected delivery time</skos:prefLabel>
      <skos:definition xml:lang="en">The expected amount of time between the order and delivery of an item. 

WG approval 26/07/2022 (epo-cat:Price -&gt; epo:Duration (+epo-cat:hasExpectedDeliveryTime)) </skos:definition>
      <rdfs:comment xml:lang="en">The expected amount of time between the order and delivery of an item. 

WG approval 26/07/2022 (epo-cat:Price -&gt; epo:Duration (+epo-cat:hasExpectedDeliveryTime)) </rdfs:comment>
      <skos:scopeNote xml:lang="en">
 (epo-cat:Price -&gt; epo:Duration (+epo-cat:hasExpectedDeliveryTime)) </skos:scopeNote>
      <rdfs:comment xml:lang="en">
 (epo-cat:Price -&gt; epo:Duration (+epo-cat:hasExpectedDeliveryTime)) </rdfs:comment>
      <rdfs:isDefinedBy rdf:resource="http://data.europa.eu/a4g/ontology"/>
   </owl:ObjectProperty>
   <owl:ObjectProperty rdf:about="http://data.europa.eu/a4g/ontology#hasPriceValidity">
      <rdfs:label xml:lang="en">Has price validity</rdfs:label>
      <skos:prefLabel xml:lang="en">Has price validity</skos:prefLabel>
      <skos:scopeNote xml:lang="en">The period of time when the Item can be ordered to the given price.
 (epo-cat:Price -&gt; epo:Period (+epo-cat:hasPriceValidity)) </skos:scopeNote>
      <rdfs:comment xml:lang="en">The period of time when the Item can be ordered to the given price.
 (epo-cat:Price -&gt; epo:Period (+epo-cat:hasPriceValidity)) </rdfs:comment>
      <rdfs:isDefinedBy rdf:resource="http://data.europa.eu/a4g/ontology"/>
   </owl:ObjectProperty>
   <owl:ObjectProperty rdf:about="http://data.europa.eu/a4g/ontology#hasNetMonetaryValue">
      <rdfs:label xml:lang="en">Has net monetary value</rdfs:label>
      <skos:prefLabel xml:lang="en">Has net monetary value</skos:prefLabel>
      <skos:scopeNote xml:lang="en">The price amount of an Item exclusive of taxes and after substracting price discounts.  (epo-cat:Price -&gt; epo:MonetaryValue (+epo-cat:hasNetMonetaryValue)) </skos:scopeNote>
      <rdfs:comment xml:lang="en">The price amount of an Item exclusive of taxes and after substracting price discounts.  (epo-cat:Price -&gt; epo:MonetaryValue (+epo-cat:hasNetMonetaryValue)) </rdfs:comment>
      <rdfs:isDefinedBy rdf:resource="http://data.europa.eu/a4g/ontology"/>
   </owl:ObjectProperty>
   <owl:ObjectProperty rdf:about="http://data.europa.eu/a4g/ontology#hasBaseQuantity">
      <rdfs:label xml:lang="en">Has base quantity</rdfs:label>
      <skos:prefLabel xml:lang="en">Has base quantity</skos:prefLabel>
      <skos:definition xml:lang="en">The quantity at which the net monetary value applies. (epo-cat:Price -&gt; epo:Quantity (+epo-cat:hasBaseQuantity)) </skos:definition>
      <rdfs:comment xml:lang="en">The quantity at which the net monetary value applies. (epo-cat:Price -&gt; epo:Quantity (+epo-cat:hasBaseQuantity)) </rdfs:comment>
      <rdfs:isDefinedBy rdf:resource="http://data.europa.eu/a4g/ontology"/>
   </owl:ObjectProperty>
   <owl:ObjectProperty rdf:about="http://data.europa.eu/a4g/ontology#hasOrderabableUnitFactorRate">
      <rdfs:label xml:lang="en">Has orderabable unit factor rate</rdfs:label>
      <skos:prefLabel xml:lang="en">Has orderabable unit factor rate</skos:prefLabel>
      <skos:scopeNote xml:lang="en">The factor by which the base unit of the price can be converted to orderable unit.

Additional information:
This is needed when the base price is provided different than the orderable unit. For example, when selling paper, the price may be set per page, but the  orderable unit is a package of 500 pieces. Therefore the price needs to be converted to the orderable unit. 

 (epo-cat:Price -&gt; epo:Quantity (+epo-cat:hasOrderabableUnitFactorRate)) </skos:scopeNote>
      <rdfs:comment xml:lang="en">The factor by which the base unit of the price can be converted to orderable unit.

Additional information:
This is needed when the base price is provided different than the orderable unit. For example, when selling paper, the price may be set per page, but the  orderable unit is a package of 500 pieces. Therefore the price needs to be converted to the orderable unit. 

 (epo-cat:Price -&gt; epo:Quantity (+epo-cat:hasOrderabableUnitFactorRate)) </rdfs:comment>
      <rdfs:isDefinedBy rdf:resource="http://data.europa.eu/a4g/ontology"/>
   </owl:ObjectProperty>
   <owl:ObjectProperty rdf:about="http://data.europa.eu/a4g/ontology#hasDeliveryLocation">
      <rdfs:label xml:lang="en">Has delivery location</rdfs:label>
      <skos:prefLabel xml:lang="en">Has delivery location</skos:prefLabel>
      <skos:scopeNote xml:lang="en">Location delivery area where the Item can be ordered to the given price.
 (epo-cat:Price -&gt; dct:Location (+epo-cat:hasDeliveryLocation)) </skos:scopeNote>
      <rdfs:comment xml:lang="en">Location delivery area where the Item can be ordered to the given price.
 (epo-cat:Price -&gt; dct:Location (+epo-cat:hasDeliveryLocation)) </rdfs:comment>
      <rdfs:isDefinedBy rdf:resource="http://data.europa.eu/a4g/ontology"/>
   </owl:ObjectProperty>
   <owl:ObjectProperty rdf:about="http://data.europa.eu/a4g/ontology#hasPrice">
      <rdfs:label xml:lang="en">Has price</rdfs:label>
      <skos:prefLabel xml:lang="en">Has price</skos:prefLabel>
      <rdfs:isDefinedBy rdf:resource="http://data.europa.eu/a4g/ontology"/>
   </owl:ObjectProperty>
   <owl:ObjectProperty rdf:about="http://data.europa.eu/a4g/ontology#hasStandardisedUnitPrice">
      <rdfs:label xml:lang="en">Has standardised unit price</rdfs:label>
      <skos:prefLabel xml:lang="en">Has standardised unit price</skos:prefLabel>
      <skos:definition xml:lang="en">The item price based on a standardised unit.

Additional Information:
The unit must be indicated in the Quantity, with a quantity value of 1. (epo-cat:CatalogueLine -&gt; epo-cat:Price (+epo-cat:hasStandardisedUnitPrice)) </skos:definition>
      <rdfs:comment xml:lang="en">The item price based on a standardised unit.

Additional Information:
The unit must be indicated in the Quantity, with a quantity value of 1. (epo-cat:CatalogueLine -&gt; epo-cat:Price (+epo-cat:hasStandardisedUnitPrice)) </rdfs:comment>
      <rdfs:isDefinedBy rdf:resource="http://data.europa.eu/a4g/ontology"/>
   </owl:ObjectProperty>
   <owl:ObjectProperty rdf:about="http://data.europa.eu/a4g/ontology#hasSpecification">
      <rdfs:label xml:lang="en">Has specification</rdfs:label>
      <skos:prefLabel xml:lang="en">Has specification</skos:prefLabel>
      <rdfs:isDefinedBy rdf:resource="http://data.europa.eu/a4g/ontology"/>
   </owl:ObjectProperty>
   <owl:ObjectProperty rdf:about="http://data.europa.eu/a4g/ontology#hasManufacturerID">
      <rdfs:label xml:lang="en">Has manufacturer i d</rdfs:label>
      <skos:prefLabel xml:lang="en">Has manufacturer i d</skos:prefLabel>
      <skos:definition xml:lang="en">The manufacturer's identifier for the item.
 (epo-cat:Manufacturer -&gt; epo:Identifier (+epo:hasManufacturerID)) </skos:definition>
      <rdfs:comment xml:lang="en">The manufacturer's identifier for the item.
 (epo-cat:Manufacturer -&gt; epo:Identifier (+epo:hasManufacturerID)) </rdfs:comment>
      <rdfs:isDefinedBy rdf:resource="http://data.europa.eu/a4g/ontology"/>
   </owl:ObjectProperty>
   <owl:ObjectProperty rdf:about="http://data.europa.eu/a4g/ontology#hasContractor">
      <rdfs:label xml:lang="en">Has contractor</rdfs:label>
      <skos:prefLabel xml:lang="en">Has contractor</skos:prefLabel>
      <rdfs:isDefinedBy rdf:resource="http://data.europa.eu/a4g/ontology"/>
   </owl:ObjectProperty>
   <owl:ObjectProperty rdf:about="http://data.europa.eu/a4g/ontology#hasManufacturer">
      <rdfs:label xml:lang="en">Has manufacturer</rdfs:label>
      <skos:prefLabel xml:lang="en">Has manufacturer</skos:prefLabel>
      <skos:scopeNote xml:lang="en">The product maker or service provider. (epo-cat:Item -&gt; epo-cat:Manufacturer (+epo-cat:hasManufacturer)) </skos:scopeNote>
      <rdfs:comment xml:lang="en">The product maker or service provider. (epo-cat:Item -&gt; epo-cat:Manufacturer (+epo-cat:hasManufacturer)) </rdfs:comment>
      <rdfs:isDefinedBy rdf:resource="http://data.europa.eu/a4g/ontology"/>
   </owl:ObjectProperty>
   <owl:ObjectProperty rdf:about="http://data.europa.eu/a4g/ontology#isProvidedByCatalogueProvider">
      <rdfs:label xml:lang="en">Is provided by catalogue provider</rdfs:label>
      <skos:prefLabel xml:lang="en">Is provided by catalogue provider</skos:prefLabel>
      <rdfs:isDefinedBy rdf:resource="http://data.europa.eu/a4g/ontology"/>
   </owl:ObjectProperty>
   <owl:ObjectProperty rdf:about="http://data.europa.eu/a4g/ontology#comprisesCatalogueLine">
      <rdfs:label xml:lang="en">Comprises catalogue line</rdfs:label>
      <skos:prefLabel xml:lang="en">Comprises catalogue line</skos:prefLabel>
      <rdfs:isDefinedBy rdf:resource="http://data.europa.eu/a4g/ontology"/>
   </owl:ObjectProperty>
   <owl:ObjectProperty rdf:about="http://data.europa.eu/a4g/ontology#isSubordinatedToContract">
      <rdfs:label xml:lang="en">Is subordinated to contract</rdfs:label>
      <skos:prefLabel xml:lang="en">Is subordinated to contract</skos:prefLabel>
      <rdfs:isDefinedBy rdf:resource="http://data.europa.eu/a4g/ontology"/>
   </owl:ObjectProperty>
   <owl:ObjectProperty rdf:about="http://data.europa.eu/a4g/ontology#hasID">
      <rdfs:label xml:lang="en">Has i d</rdfs:label>
      <skos:prefLabel xml:lang="en">Has i d</skos:prefLabel>
      <skos:definition xml:lang="en">A unique identifier of the instance of the concept.

Additional Information

For example, in the case of the Procurement Identifier, this could be the European Public Procurement Identifier, and/or any other identifier provided by the buyer, the service provider or any other stakeholder.

WG Approval 12/11/2019
 (epo-cat:CatalogueLine -&gt; epo:Identifier (+epo:hasID)) A unique identifier of the instance of the concept.

Additional Information

For example, in the case of the Procurement Identifier, this could be the European Public Procurement Identifier, and/or any other identifier provided by the buyer, the service provider or any other stakeholder.

WG Approval 12/11/2019 (epo-cat:Batch -&gt; epo:Identifier (+epo:hasID)) </skos:definition>
      <rdfs:comment xml:lang="en">A unique identifier of the instance of the concept.

Additional Information

For example, in the case of the Procurement Identifier, this could be the European Public Procurement Identifier, and/or any other identifier provided by the buyer, the service provider or any other stakeholder.

WG Approval 12/11/2019
 (epo-cat:CatalogueLine -&gt; epo:Identifier (+epo:hasID)) A unique identifier of the instance of the concept.

Additional Information

For example, in the case of the Procurement Identifier, this could be the European Public Procurement Identifier, and/or any other identifier provided by the buyer, the service provider or any other stakeholder.

WG Approval 12/11/2019 (epo-cat:Batch -&gt; epo:Identifier (+epo:hasID)) </rdfs:comment>
      <rdfs:isDefinedBy rdf:resource="http://data.europa.eu/a4g/ontology"/>
   </owl:ObjectProperty>
   <owl:ObjectProperty rdf:about="http://data.europa.eu/a4g/ontology#specifiesItem">
      <rdfs:label xml:lang="en">Specifies item</rdfs:label>
      <skos:prefLabel xml:lang="en">Specifies item</skos:prefLabel>
      <rdfs:isDefinedBy rdf:resource="http://data.europa.eu/a4g/ontology"/>
   </owl:ObjectProperty>
   <owl:ObjectProperty rdf:about="http://data.europa.eu/a4g/ontology#hasTransactionConditionsCode">
      <rdfs:label xml:lang="en">Has transaction conditions code</rdfs:label>
      <skos:prefLabel xml:lang="en">Has transaction conditions code</skos:prefLabel>
      <skos:definition xml:lang="en">Coded description of the specific transaction conditions (purchasing, sales, payment) for an item.
 (epo-cat:CatalogueLine -&gt; epo-cat:transaction-conditions (+epo-cat:hasTransactionConditionsCode)) </skos:definition>
      <rdfs:comment xml:lang="en">Coded description of the specific transaction conditions (purchasing, sales, payment) for an item.
 (epo-cat:CatalogueLine -&gt; epo-cat:transaction-conditions (+epo-cat:hasTransactionConditionsCode)) </rdfs:comment>
      <rdfs:isDefinedBy rdf:resource="http://data.europa.eu/a4g/ontology"/>
   </owl:ObjectProperty>
   <owl:ObjectProperty rdf:about="http://data.europa.eu/a4g/ontology#hasOrderableUnit">
      <rdfs:label xml:lang="en">Has orderable unit</rdfs:label>
      <skos:prefLabel xml:lang="en">Has orderable unit</skos:prefLabel>
      <skos:definition xml:lang="en">The unit in which the item described in this catalogue line can be ordered. (epo-cat:CatalogueLine -&gt; epo-cat:orderable-unit (+epo-cat:hasOrderableUnit)) </skos:definition>
      <rdfs:comment xml:lang="en">The unit in which the item described in this catalogue line can be ordered. (epo-cat:CatalogueLine -&gt; epo-cat:orderable-unit (+epo-cat:hasOrderableUnit)) </rdfs:comment>
      <rdfs:isDefinedBy rdf:resource="http://data.europa.eu/a4g/ontology"/>
   </owl:ObjectProperty>
   <owl:ObjectProperty rdf:about="http://data.europa.eu/a4g/ontology#hasCatalogueLineValidity">
      <rdfs:label xml:lang="en">Has catalogue line validity</rdfs:label>
      <skos:prefLabel xml:lang="en">Has catalogue line validity</skos:prefLabel>
      <rdfs:isDefinedBy rdf:resource="http://data.europa.eu/a4g/ontology"/>
   </owl:ObjectProperty>
   <owl:ObjectProperty rdf:about="http://data.europa.eu/a4g/ontology#hasMinimumQuantityGuaranteedForDelivery">
      <rdfs:label xml:lang="en">Has minimum quantity guaranteed for delivery</rdfs:label>
      <skos:prefLabel xml:lang="en">Has minimum quantity guaranteed for delivery</skos:prefLabel>
      <skos:definition xml:lang="en">The minimum quantity of an item that is guaranteed by the seller to be delivered.

 (epo-cat:CatalogueLine -&gt; epo:Quantity (+epo-cat:hasMinimumQuantityGuaranteedForDelivery)) </skos:definition>
      <rdfs:comment xml:lang="en">The minimum quantity of an item that is guaranteed by the seller to be delivered.

 (epo-cat:CatalogueLine -&gt; epo:Quantity (+epo-cat:hasMinimumQuantityGuaranteedForDelivery)) </rdfs:comment>
      <rdfs:isDefinedBy rdf:resource="http://data.europa.eu/a4g/ontology"/>
   </owl:ObjectProperty>
   <owl:ObjectProperty rdf:about="http://data.europa.eu/a4g/ontology#hasMaximumOrderQuantity">
      <rdfs:label xml:lang="en">Has maximum order quantity</rdfs:label>
      <skos:prefLabel xml:lang="en">Has maximum order quantity</skos:prefLabel>
      <skos:definition xml:lang="en">The maximum number of orderable units that can be ordered according to details provided in the catalogue line, such as price.
 (epo-cat:CatalogueLine -&gt; epo:Quantity (+epo-cat:hasMaximumOrderQuantity)) </skos:definition>
      <rdfs:comment xml:lang="en">The maximum number of orderable units that can be ordered according to details provided in the catalogue line, such as price.
 (epo-cat:CatalogueLine -&gt; epo:Quantity (+epo-cat:hasMaximumOrderQuantity)) </rdfs:comment>
      <rdfs:isDefinedBy rdf:resource="http://data.europa.eu/a4g/ontology"/>
   </owl:ObjectProperty>
   <owl:ObjectProperty rdf:about="http://data.europa.eu/a4g/ontology#isProductionOf">
      <rdfs:label xml:lang="en">Is production of</rdfs:label>
      <skos:prefLabel xml:lang="en">Is production of</skos:prefLabel>
      <rdfs:isDefinedBy rdf:resource="http://data.europa.eu/a4g/ontology"/>
   </owl:ObjectProperty>
   <owl:ObjectProperty rdf:about="http://data.europa.eu/a4g/ontology#hasCountryOfOrigin">
      <rdfs:label xml:lang="en">Has country of origin</rdfs:label>
      <skos:prefLabel xml:lang="en">Has country of origin</skos:prefLabel>
      <skos:scopeNote xml:lang="en">The source country of the product or service.

Additional Information:

The country of origin can be provided by  the buyer as a requirement or by the tenderer information of the item to be provided.

WG Approval 07/01/2020
 (epo-cat:Item -&gt; at-voc:country (+epo-cat:hasCountryOfOrigin)) </skos:scopeNote>
      <rdfs:comment xml:lang="en">The source country of the product or service.

Additional Information:

The country of origin can be provided by  the buyer as a requirement or by the tenderer information of the item to be provided.

WG Approval 07/01/2020
 (epo-cat:Item -&gt; at-voc:country (+epo-cat:hasCountryOfOrigin)) </rdfs:comment>
      <rdfs:isDefinedBy rdf:resource="http://data.europa.eu/a4g/ontology"/>
   </owl:ObjectProperty>
   <owl:ObjectProperty rdf:about="http://data.europa.eu/a4g/ontology#requires">
      <rdfs:label xml:lang="en">Requires</rdfs:label>
      <skos:prefLabel xml:lang="en">Requires</skos:prefLabel>
      <skos:definition xml:lang="en">A related resource that is required by the described resource to support its function, delivery, or coherence.

Additional Information:
In the eCatalogue context, when this relation is used between two items, the resource in the definition refers to Items, i.e. one Item requires another Item. 

WG Approval: 30/06/2022
 (epo-cat:Item -&gt; epo-cat:Item (+dct:requires)) </skos:definition>
      <rdfs:comment xml:lang="en">A related resource that is required by the described resource to support its function, delivery, or coherence.

Additional Information:
In the eCatalogue context, when this relation is used between two items, the resource in the definition refers to Items, i.e. one Item requires another Item. 

WG Approval: 30/06/2022
 (epo-cat:Item -&gt; epo-cat:Item (+dct:requires)) </rdfs:comment>
      <rdfs:isDefinedBy rdf:resource="http://data.europa.eu/a4g/ontology"/>
   </owl:ObjectProperty>
   <owl:ObjectProperty rdf:about="http://data.europa.eu/a4g/ontology#hasItemStandardID">
      <rdfs:label xml:lang="en">Has item standard i d</rdfs:label>
      <skos:prefLabel xml:lang="en">Has item standard i d</skos:prefLabel>
      <skos:definition xml:lang="en">The identifier for the instance of the concept based on a standard scheme.

Additional information: 
For example the GTIN scheme (Global Trade Item Number). 

WG Approval 24/02/2022
 (epo-cat:Item -&gt; epo:Identifier (+epo:hasItemStandardID)) </skos:definition>
      <rdfs:comment xml:lang="en">The identifier for the instance of the concept based on a standard scheme.

Additional information: 
For example the GTIN scheme (Global Trade Item Number). 

WG Approval 24/02/2022
 (epo-cat:Item -&gt; epo:Identifier (+epo:hasItemStandardID)) </rdfs:comment>
      <rdfs:isDefinedBy rdf:resource="http://data.europa.eu/a4g/ontology"/>
   </owl:ObjectProperty>
   <owl:ObjectProperty rdf:about="http://data.europa.eu/a4g/ontology#hasNetQuantity">
      <rdfs:label xml:lang="en">Has net quantity</rdfs:label>
      <skos:prefLabel xml:lang="en">Has net quantity</skos:prefLabel>
      <skos:definition xml:lang="en">The net quantity of the item that is contained in each consumable unit, excluding any packaging materials.
 (epo-cat:Item -&gt; epo:Quantity (+epo-cat:hasNetQuantity)) </skos:definition>
      <rdfs:comment xml:lang="en">The net quantity of the item that is contained in each consumable unit, excluding any packaging materials.
 (epo-cat:Item -&gt; epo:Quantity (+epo-cat:hasNetQuantity)) </rdfs:comment>
      <rdfs:isDefinedBy rdf:resource="http://data.europa.eu/a4g/ontology"/>
   </owl:ObjectProperty>
   <owl:ObjectProperty rdf:about="http://data.europa.eu/a4g/ontology#hasPart">
      <rdfs:label xml:lang="en">Has part</rdfs:label>
      <skos:prefLabel xml:lang="en">Has part</skos:prefLabel>
      <skos:definition xml:lang="en">A related resource that is included either physically or logically in the described resource.

Additional Information: 
In the eCatalogue context, when this relation is used between two items, the resource in the definition refers to Items, i.e. one item is part of another item.

WG Approval: 30/06/2022
 (epo-cat:Item -&gt; epo-cat:Item (+dct:hasPart)) </skos:definition>
      <rdfs:comment xml:lang="en">A related resource that is included either physically or logically in the described resource.

Additional Information: 
In the eCatalogue context, when this relation is used between two items, the resource in the definition refers to Items, i.e. one item is part of another item.

WG Approval: 30/06/2022
 (epo-cat:Item -&gt; epo-cat:Item (+dct:hasPart)) </rdfs:comment>
      <rdfs:isDefinedBy rdf:resource="http://data.europa.eu/a4g/ontology"/>
   </owl:ObjectProperty>
   <owl:ObjectProperty rdf:about="http://data.europa.eu/a4g/ontology#hasAccessoryItem">
      <rdfs:label xml:lang="en">Has accessory item</rdfs:label>
      <skos:prefLabel xml:lang="en">Has accessory item</skos:prefLabel>
      <skos:definition xml:lang="en">An item that can be added to another item to enhance it.

WG Approval: 30/06/2022 (epo-cat:Item -&gt; epo-cat:Item (+epo-cat:hasAccessoryItem)) </skos:definition>
      <rdfs:comment xml:lang="en">An item that can be added to another item to enhance it.

WG Approval: 30/06/2022 (epo-cat:Item -&gt; epo-cat:Item (+epo-cat:hasAccessoryItem)) </rdfs:comment>
      <skos:scopeNote xml:lang="en">An additional item that can enhance the original item. 

WG Approval: 19/05/2022
 (epo-cat:Item -&gt; epo-cat:Item (+epo-cat:hasAccessoryItem)) </skos:scopeNote>
      <rdfs:comment xml:lang="en">An additional item that can enhance the original item. 

WG Approval: 19/05/2022
 (epo-cat:Item -&gt; epo-cat:Item (+epo-cat:hasAccessoryItem)) </rdfs:comment>
      <rdfs:isDefinedBy rdf:resource="http://data.europa.eu/a4g/ontology"/>
   </owl:ObjectProperty>
   <owl:ObjectProperty rdf:about="http://data.europa.eu/a4g/ontology#hasItemClassification">
      <rdfs:label xml:lang="en">Has item classification</rdfs:label>
      <skos:prefLabel xml:lang="en">Has item classification</skos:prefLabel>
      <skos:scopeNote xml:lang="en">A classification of this item according to a specific system for classifying products or services.

Additional information: 
Examples of classification schemes are: CPV, UNSPC, eCl@ss, GPC, ...

WG acceptance 10/03/2022 (epo-cat:Item -&gt; at-voc-new:unspc (+epo-cat:hasItemClassification)) </skos:scopeNote>
      <rdfs:comment xml:lang="en">A classification of this item according to a specific system for classifying products or services.

Additional information: 
Examples of classification schemes are: CPV, UNSPC, eCl@ss, GPC, ...

WG acceptance 10/03/2022 (epo-cat:Item -&gt; at-voc-new:unspc (+epo-cat:hasItemClassification)) </rdfs:comment>
      <rdfs:isDefinedBy rdf:resource="http://data.europa.eu/a4g/ontology"/>
   </owl:ObjectProperty>
   <owl:ObjectProperty rdf:about="http://data.europa.eu/a4g/ontology#hasCatalogueItemID">
      <rdfs:label xml:lang="en">Has catalogue item i d</rdfs:label>
      <skos:prefLabel xml:lang="en">Has catalogue item i d</skos:prefLabel>
      <skos:definition xml:lang="en">The identifier for the instance of the concept as defined in the catalogue.

WG Approval 24/02/2022
 (epo-cat:Item -&gt; epo:Identifier (+epo:hasCatalogueItemID)) </skos:definition>
      <rdfs:comment xml:lang="en">The identifier for the instance of the concept as defined in the catalogue.

WG Approval 24/02/2022
 (epo-cat:Item -&gt; epo:Identifier (+epo:hasCatalogueItemID)) </rdfs:comment>
      <rdfs:isDefinedBy rdf:resource="http://data.europa.eu/a4g/ontology"/>
   </owl:ObjectProperty>
   <owl:ObjectProperty rdf:about="http://data.europa.eu/a4g/ontology#hasHazardousItemUNDGCode">
      <rdfs:label xml:lang="en">Has hazardous item u n d g code</rdfs:label>
      <skos:prefLabel xml:lang="en">Has hazardous item u n d g code</skos:prefLabel>
      <skos:scopeNote xml:lang="en">Specification of the hazardous nature of an item according to the UNDG classification schema. Provides detail of the classification and nature of a hazardous item.
 (epo-cat:Item -&gt; at-voc-new:dangerous-goods-list (+epo-cat:hasHazardousItemUNDGCode)) </skos:scopeNote>
      <rdfs:comment xml:lang="en">Specification of the hazardous nature of an item according to the UNDG classification schema. Provides detail of the classification and nature of a hazardous item.
 (epo-cat:Item -&gt; at-voc-new:dangerous-goods-list (+epo-cat:hasHazardousItemUNDGCode)) </rdfs:comment>
      <rdfs:isDefinedBy rdf:resource="http://data.europa.eu/a4g/ontology"/>
   </owl:ObjectProperty>
   <owl:ObjectProperty rdf:about="http://data.europa.eu/a4g/ontology#hasComplementaryItem">
      <rdfs:label xml:lang="en">Has complementary item</rdfs:label>
      <skos:prefLabel xml:lang="en">Has complementary item</skos:prefLabel>
      <skos:definition xml:lang="en">An item that if used with another item provides mutual enhancements to both of them.

Additional information:
For example, gin and tonic; or smart-phone and smart-watch.

WG Approval: 19/05/2022

 (epo-cat:Item -&gt; epo-cat:Item (+epo-cat:hasComplementaryItem)) </skos:definition>
      <rdfs:comment xml:lang="en">An item that if used with another item provides mutual enhancements to both of them.

Additional information:
For example, gin and tonic; or smart-phone and smart-watch.

WG Approval: 19/05/2022

 (epo-cat:Item -&gt; epo-cat:Item (+epo-cat:hasComplementaryItem)) </rdfs:comment>
      <rdfs:isDefinedBy rdf:resource="http://data.europa.eu/a4g/ontology"/>
   </owl:ObjectProperty>
   <owl:ObjectProperty rdf:about="http://data.europa.eu/a4g/ontology#replaces">
      <rdfs:label xml:lang="en">Replaces</rdfs:label>
      <skos:prefLabel xml:lang="en">Replaces</skos:prefLabel>
      <skos:definition xml:lang="en">A related resource that is supplanted, displaced, or superseded by the described resource.

Additional Information: 
In the eCatalogue context, when this relation is used between two items, the resource in the definition refers to Items, i.e. one item replaces another item. 

WG Approval: 30/06/2022
 (epo-cat:Item &lt;-&gt; epo-cat:Item (+dct:isReplaceBy +dct:replaces)) </skos:definition>
      <rdfs:comment xml:lang="en">A related resource that is supplanted, displaced, or superseded by the described resource.

Additional Information: 
In the eCatalogue context, when this relation is used between two items, the resource in the definition refers to Items, i.e. one item replaces another item. 

WG Approval: 30/06/2022
 (epo-cat:Item &lt;-&gt; epo-cat:Item (+dct:isReplaceBy +dct:replaces)) </rdfs:comment>
      <skos:scopeNote xml:lang="en">A related resource that is supplanted, displaced, or superseded by the described resource.
 (epo-cat:Item &lt;-&gt; epo-cat:Item (+dct:isReplaceBy +dct:replaces)) </skos:scopeNote>
      <rdfs:comment xml:lang="en">A related resource that is supplanted, displaced, or superseded by the described resource.
 (epo-cat:Item &lt;-&gt; epo-cat:Item (+dct:isReplaceBy +dct:replaces)) </rdfs:comment>
      <rdfs:isDefinedBy rdf:resource="http://data.europa.eu/a4g/ontology"/>
   </owl:ObjectProperty>
   <owl:ObjectProperty rdf:about="http://data.europa.eu/a4g/ontology#isReplaceBy">
      <rdfs:label xml:lang="en">Is replace by</rdfs:label>
      <skos:prefLabel xml:lang="en">Is replace by</skos:prefLabel>
      <skos:definition xml:lang="en">A related resource that is supplanted, displaced, or superseded by the described resource.

Additional Information: 
In the eCatalogue context, when this relation is used between two items, the resource in the definition refers to Items, i.e. one item replaces another item. 

WG Approval: 30/06/2022
 (epo-cat:Item &lt;-&gt; epo-cat:Item (+dct:isReplaceBy +dct:replaces)) </skos:definition>
      <rdfs:comment xml:lang="en">A related resource that is supplanted, displaced, or superseded by the described resource.

Additional Information: 
In the eCatalogue context, when this relation is used between two items, the resource in the definition refers to Items, i.e. one item replaces another item. 

WG Approval: 30/06/2022
 (epo-cat:Item &lt;-&gt; epo-cat:Item (+dct:isReplaceBy +dct:replaces)) </rdfs:comment>
      <skos:scopeNote xml:lang="en">A related resource that supplants, displaces, or supersedes the described resource.

Additional Information:
WG Approval: 19/05/2022 (epo-cat:Item &lt;-&gt; epo-cat:Item (+dct:isReplaceBy +dct:replaces)) </skos:scopeNote>
      <rdfs:comment xml:lang="en">A related resource that supplants, displaces, or supersedes the described resource.

Additional Information:
WG Approval: 19/05/2022 (epo-cat:Item &lt;-&gt; epo-cat:Item (+dct:isReplaceBy +dct:replaces)) </rdfs:comment>
      <rdfs:isDefinedBy rdf:resource="http://data.europa.eu/a4g/ontology"/>
   </owl:ObjectProperty>
   <owl:ObjectProperty rdf:about="http://data.europa.eu/a4g/ontology#hasVATCategoryCode">
      <rdfs:label xml:lang="en">Has v a t category code</rdfs:label>
      <skos:prefLabel xml:lang="en">Has v a t category code</skos:prefLabel>
      <skos:scopeNote xml:lang="en">Value-added tax category of the item.
 (epo-cat:Item -&gt; epo-cat:vat-category (+epo-cat:hasVATCategoryCode)) </skos:scopeNote>
      <rdfs:comment xml:lang="en">Value-added tax category of the item.
 (epo-cat:Item -&gt; epo-cat:vat-category (+epo-cat:hasVATCategoryCode)) </rdfs:comment>
      <rdfs:isDefinedBy rdf:resource="http://data.europa.eu/a4g/ontology"/>
   </owl:ObjectProperty>
   <owl:ObjectProperty rdf:about="http://data.europa.eu/a4g/ontology#hasManufacturerItemID">
      <rdfs:label xml:lang="en">Has manufacturer item i d</rdfs:label>
      <skos:prefLabel xml:lang="en">Has manufacturer item i d</skos:prefLabel>
      <skos:definition xml:lang="en">The identifier for the instance of the concept as defined by the manufacturer.

WG Approval 24/02/2022
 (epo-cat:Item -&gt; epo:Identifier (+epo:hasManufacturerItemID)) </skos:definition>
      <rdfs:comment xml:lang="en">The identifier for the instance of the concept as defined by the manufacturer.

WG Approval 24/02/2022
 (epo-cat:Item -&gt; epo:Identifier (+epo:hasManufacturerItemID)) </rdfs:comment>
      <rdfs:isDefinedBy rdf:resource="http://data.europa.eu/a4g/ontology"/>
   </owl:ObjectProperty>
   <owl:ObjectProperty rdf:about="http://data.europa.eu/a4g/ontology#hasDeliveryClassification">
      <rdfs:label xml:lang="en">Has delivery classification</rdfs:label>
      <skos:prefLabel xml:lang="en">Has delivery classification</skos:prefLabel>
      <rdfs:isDefinedBy rdf:resource="http://data.europa.eu/a4g/ontology"/>
   </owl:ObjectProperty>
   <owl:DatatypeProperty rdf:about="http://data.europa.eu/a4g/ontology#hasName">
      <rdfs:label xml:lang="en">Has name</rdfs:label>
      <skos:prefLabel xml:lang="en">Has name</skos:prefLabel>
      <rdfs:comment xml:lang="en">A short text by which a thing is known or referred to.

WG Approval 16/11/2021
 (epo-cat:Brand) A short text by which a thing is known or referred to.

WG Approval 16/11/2021
 (epo-cat:CatalogueDocument) A short text by which a thing is known or referred to.

WG Approval 16/11/2021 (epo-cat:ItemModel) A short text by which a thing is known or referred to.

WG Approval 16/11/2021 (epo-cat:Item) </rdfs:comment>
      <skos:definition xml:lang="en">A short text by which a thing is known or referred to.

WG Approval 16/11/2021
 (epo-cat:Brand) A short text by which a thing is known or referred to.

WG Approval 16/11/2021
 (epo-cat:CatalogueDocument) A short text by which a thing is known or referred to.

WG Approval 16/11/2021 (epo-cat:ItemModel) A short text by which a thing is known or referred to.

WG Approval 16/11/2021 (epo-cat:Item) </skos:definition>
      <rdfs:isDefinedBy rdf:resource="http://data.europa.eu/a4g/ontology"/>
   </owl:DatatypeProperty>
   <owl:DatatypeProperty rdf:about="http://data.europa.eu/a4g/ontology#hasSourceCatalogueVersion">
      <rdfs:label xml:lang="en">Has source catalogue version</rdfs:label>
      <skos:prefLabel xml:lang="en">Has source catalogue version</skos:prefLabel>
      <rdfs:comment xml:lang="en">The version of the catalogue to be updated.

Additional Information:
For example, if we start with source version 005 and add a fragment to it we will end up with a target version number 006. (epo-cat:CatalogueUpdateDocument) </rdfs:comment>
      <skos:definition xml:lang="en">The version of the catalogue to be updated.

Additional Information:
For example, if we start with source version 005 and add a fragment to it we will end up with a target version number 006. (epo-cat:CatalogueUpdateDocument) </skos:definition>
      <rdfs:isDefinedBy rdf:resource="http://data.europa.eu/a4g/ontology"/>
   </owl:DatatypeProperty>
   <owl:DatatypeProperty rdf:about="http://data.europa.eu/a4g/ontology#hasTargetCatalogueVersion">
      <rdfs:label xml:lang="en">Has target catalogue version</rdfs:label>
      <skos:prefLabel xml:lang="en">Has target catalogue version</skos:prefLabel>
      <rdfs:comment xml:lang="en">The version of the catalogue after the update is applied.

Additional Information:
For example, if we start with source version 005 and add a fragment to it we will end up with a target version number 006.
 (epo-cat:CatalogueUpdateDocument) </rdfs:comment>
      <skos:definition xml:lang="en">The version of the catalogue after the update is applied.

Additional Information:
For example, if we start with source version 005 and add a fragment to it we will end up with a target version number 006.
 (epo-cat:CatalogueUpdateDocument) </skos:definition>
      <rdfs:isDefinedBy rdf:resource="http://data.europa.eu/a4g/ontology"/>
   </owl:DatatypeProperty>
   <owl:DatatypeProperty rdf:about="http://data.europa.eu/a4g/ontology#hasReferenceURI">
      <rdfs:label xml:lang="en">Has reference u r i</rdfs:label>
      <skos:prefLabel xml:lang="en">Has reference u r i</skos:prefLabel>
      <rdfs:comment xml:lang="en">A reference to where the label specification (norms, expectations, standards and policies) can be found.

WG approval 26/07/2022 (epo-cat:CertificationLabel) </rdfs:comment>
      <skos:definition xml:lang="en">A reference to where the label specification (norms, expectations, standards and policies) can be found.

WG approval 26/07/2022 (epo-cat:CertificationLabel) </skos:definition>
      <rdfs:isDefinedBy rdf:resource="http://data.europa.eu/a4g/ontology"/>
   </owl:DatatypeProperty>
   <owl:DatatypeProperty rdf:about="http://data.europa.eu/a4g/ontology#hasCertificationNumber">
      <rdfs:label xml:lang="en">Has certification number</rdfs:label>
      <skos:prefLabel xml:lang="en">Has certification number</skos:prefLabel>
      <rdfs:comment xml:lang="en">The unique identifier of the certificate.

WG approval 26/07/2022 (epo-cat:ItemCertificate) </rdfs:comment>
      <skos:definition xml:lang="en">The unique identifier of the certificate.

WG approval 26/07/2022 (epo-cat:ItemCertificate) </skos:definition>
      <rdfs:isDefinedBy rdf:resource="http://data.europa.eu/a4g/ontology"/>
   </owl:DatatypeProperty>
   <owl:DatatypeProperty rdf:about="http://data.europa.eu/a4g/ontology#hasURL">
      <rdfs:label xml:lang="en">Has u r l</rdfs:label>
      <skos:prefLabel xml:lang="en">Has u r l</skos:prefLabel>
      <rdfs:comment xml:lang="en">The identifier of a resource.

Additional Information

For example:

1. The URL of the system from where to access the procurement documents;
2. The URL of the system for the submission of tender documents;
3. The URL of the system from where to download a tool to communicate with the Buyer;
4. The URL of the system used by a Technique to allow Economic Operators to exchange information with the Buyer (e.g. eAuction and DPS Systems)
5. The URL of the system used to exchange information between Buyer and EO for questions and clarifications;

WG Approval 30/09/2019
 (epo-cat:ItemCertificate) </rdfs:comment>
      <skos:definition xml:lang="en">The identifier of a resource.

Additional Information

For example:

1. The URL of the system from where to access the procurement documents;
2. The URL of the system for the submission of tender documents;
3. The URL of the system from where to download a tool to communicate with the Buyer;
4. The URL of the system used by a Technique to allow Economic Operators to exchange information with the Buyer (e.g. eAuction and DPS Systems)
5. The URL of the system used to exchange information between Buyer and EO for questions and clarifications;

WG Approval 30/09/2019
 (epo-cat:ItemCertificate) </skos:definition>
      <rdfs:isDefinedBy rdf:resource="http://data.europa.eu/a4g/ontology"/>
   </owl:DatatypeProperty>
   <owl:DatatypeProperty rdf:about="http://data.europa.eu/a4g/ontology#hasAttributeType">
      <rdfs:label xml:lang="en">Has attribute type</rdfs:label>
      <skos:prefLabel xml:lang="en">Has attribute type</skos:prefLabel>
      <rdfs:comment xml:lang="en">The property defined in a classification scheme. 

Additional Information:
For example, the following two properties are defined in the ECLASS classification of goods and services: (0173-1#02-AAA026#007) drilling diameter: drilling diameter, (0173-1#02-AAA030#007) flange diameter: flange diameter .


WG approval 28/07/2022 (epo-cat:ItemDescription) </rdfs:comment>
      <skos:definition xml:lang="en">The property defined in a classification scheme. 

Additional Information:
For example, the following two properties are defined in the ECLASS classification of goods and services: (0173-1#02-AAA026#007) drilling diameter: drilling diameter, (0173-1#02-AAA030#007) flange diameter: flange diameter .


WG approval 28/07/2022 (epo-cat:ItemDescription) </skos:definition>
      <rdfs:isDefinedBy rdf:resource="http://data.europa.eu/a4g/ontology"/>
   </owl:DatatypeProperty>
   <owl:DatatypeProperty rdf:about="http://data.europa.eu/a4g/ontology#hasClassificationScheme">
      <rdfs:label xml:lang="en">Has classification scheme</rdfs:label>
      <skos:prefLabel xml:lang="en">Has classification scheme</skos:prefLabel>
      <rdfs:comment xml:lang="en">The classification scheme where a property is defined. 

Additional Information:
For example, the following two properties are defined in the ECLASS classification of goods and services: (0173-1#02-AAA026#007) drilling diameter: drilling diameter, (0173-1#02-AAA030#007) flange diameter: flange diameter .

WG approval 28/07/2022
 (epo-cat:ItemDescription) </rdfs:comment>
      <skos:definition xml:lang="en">The classification scheme where a property is defined. 

Additional Information:
For example, the following two properties are defined in the ECLASS classification of goods and services: (0173-1#02-AAA026#007) drilling diameter: drilling diameter, (0173-1#02-AAA030#007) flange diameter: flange diameter .

WG approval 28/07/2022
 (epo-cat:ItemDescription) </skos:definition>
      <rdfs:isDefinedBy rdf:resource="http://data.europa.eu/a4g/ontology"/>
   </owl:DatatypeProperty>
   <owl:DatatypeProperty rdf:about="http://data.europa.eu/a4g/ontology#hasLiteralValue">
      <rdfs:label xml:lang="en">Has literal value</rdfs:label>
      <skos:prefLabel xml:lang="en">Has literal value</skos:prefLabel>
      <rdfs:comment xml:lang="en">Simple value of the property, which is defined in a classification scheme.

Additional Information:
For example, the (0173-1#02-AAV139#001) coating 1 of an optical material has value of "silver". 

This simple literal value is for the cases when the property value does not have units, in which case the qualifiedValue shall be used. 

WG approval 28/07/2022


 (epo-cat:ItemDescription) </rdfs:comment>
      <skos:definition xml:lang="en">Simple value of the property, which is defined in a classification scheme.

Additional Information:
For example, the (0173-1#02-AAV139#001) coating 1 of an optical material has value of "silver". 

This simple literal value is for the cases when the property value does not have units, in which case the qualifiedValue shall be used. 

WG approval 28/07/2022


 (epo-cat:ItemDescription) </skos:definition>
      <rdfs:isDefinedBy rdf:resource="http://data.europa.eu/a4g/ontology"/>
   </owl:DatatypeProperty>
   <owl:DatatypeProperty rdf:about="http://data.europa.eu/a4g/ontology#hasFactor">
      <rdfs:label xml:lang="en">Has factor</rdfs:label>
      <skos:prefLabel xml:lang="en">Has factor</skos:prefLabel>
      <rdfs:comment xml:lang="en">The number or the fraction of a related item.  (epo-cat:ItemRelation) </rdfs:comment>
      <skos:definition xml:lang="en">The number or the fraction of a related item.  (epo-cat:ItemRelation) </skos:definition>
      <rdfs:isDefinedBy rdf:resource="http://data.europa.eu/a4g/ontology"/>
   </owl:DatatypeProperty>
   <owl:DatatypeProperty rdf:about="http://data.europa.eu/a4g/ontology#hasSpecificPaymentArrangement">
      <rdfs:label xml:lang="en">Has specific payment arrangement</rdfs:label>
      <skos:prefLabel xml:lang="en">Has specific payment arrangement</skos:prefLabel>
      <rdfs:comment xml:lang="en">Information about payment conditions applied to all items in the catalogue.

Additional information:
This property may need to be used together with the payment arrangements provided in the ContractTerms, where such terms exists.

WG approval 30/06/2022

 (epo-cat:Catalogue) </rdfs:comment>
      <skos:definition xml:lang="en">Information about payment conditions applied to all items in the catalogue.

Additional information:
This property may need to be used together with the payment arrangements provided in the ContractTerms, where such terms exists.

WG approval 30/06/2022

 (epo-cat:Catalogue) </skos:definition>
      <rdfs:isDefinedBy rdf:resource="http://data.europa.eu/a4g/ontology"/>
   </owl:DatatypeProperty>
   <owl:DatatypeProperty rdf:about="http://data.europa.eu/a4g/ontology#isOrderable">
      <rdfs:label xml:lang="en">Is orderable</rdfs:label>
      <skos:prefLabel xml:lang="en">Is orderable</skos:prefLabel>
      <rdfs:comment xml:lang="en">Indicator, if the item is orderable or not, e.g. because it is temporarily out of stock. (epo-cat:CatalogueLine) </rdfs:comment>
      <skos:definition xml:lang="en">Indicator, if the item is orderable or not, e.g. because it is temporarily out of stock. (epo-cat:CatalogueLine) </skos:definition>
      <rdfs:isDefinedBy rdf:resource="http://data.europa.eu/a4g/ontology"/>
   </owl:DatatypeProperty>
   <owl:DatatypeProperty rdf:about="http://data.europa.eu/a4g/ontology#hasOrderableUnitFactorRate">
      <rdfs:label xml:lang="en">Has orderable unit factor rate</rdfs:label>
      <skos:prefLabel xml:lang="en">Has orderable unit factor rate</skos:prefLabel>
      <rdfs:comment xml:lang="en">The factor by which the Item net price of an unit of an item can be converted to the orderable unit. (epo-cat:CatalogueLine) </rdfs:comment>
      <skos:definition xml:lang="en">The factor by which the Item net price of an unit of an item can be converted to the orderable unit. (epo-cat:CatalogueLine) </skos:definition>
      <rdfs:isDefinedBy rdf:resource="http://data.europa.eu/a4g/ontology"/>
   </owl:DatatypeProperty>
   <owl:DatatypeProperty rdf:about="http://data.europa.eu/a4g/ontology#hasOrderableQuantityIncrement">
      <rdfs:label xml:lang="en">Has orderable quantity increment</rdfs:label>
      <skos:prefLabel xml:lang="en">Has orderable quantity increment</skos:prefLabel>
      <rdfs:comment xml:lang="en">Orderable quantity increment: The increment of Orderable units that can be ordered. (epo-cat:CatalogueLine) </rdfs:comment>
      <skos:definition xml:lang="en">Orderable quantity increment: The increment of Orderable units that can be ordered. (epo-cat:CatalogueLine) </skos:definition>
      <rdfs:isDefinedBy rdf:resource="http://data.europa.eu/a4g/ontology"/>
   </owl:DatatypeProperty>
   <owl:DatatypeProperty rdf:about="http://data.europa.eu/a4g/ontology#hasWarrantyInformation">
      <rdfs:label xml:lang="en">Has warranty information</rdfs:label>
      <skos:prefLabel xml:lang="en">Has warranty information</skos:prefLabel>
      <rdfs:comment xml:lang="en">Warranty information that applies to the catalogue line item. (epo-cat:CatalogueLine) </rdfs:comment>
      <skos:definition xml:lang="en">Warranty information that applies to the catalogue line item. (epo-cat:CatalogueLine) </skos:definition>
      <rdfs:isDefinedBy rdf:resource="http://data.europa.eu/a4g/ontology"/>
   </owl:DatatypeProperty>
   <owl:DatatypeProperty rdf:about="http://data.europa.eu/a4g/ontology#isContractedItem">
      <rdfs:label xml:lang="en">Is contracted item</rdfs:label>
      <skos:prefLabel xml:lang="en">Is contracted item</skos:prefLabel>
      <rdfs:comment xml:lang="en">Indicator if the item is offered in accordance to an existing contract. (epo-cat:CatalogueLine) </rdfs:comment>
      <skos:definition xml:lang="en">Indicator if the item is offered in accordance to an existing contract. (epo-cat:CatalogueLine) </skos:definition>
      <rdfs:isDefinedBy rdf:resource="http://data.europa.eu/a4g/ontology"/>
   </owl:DatatypeProperty>
   <owl:DatatypeProperty rdf:about="http://data.europa.eu/a4g/ontology#hasTransactionConditions">
      <rdfs:label xml:lang="en">Has transaction conditions</rdfs:label>
      <skos:prefLabel xml:lang="en">Has transaction conditions</skos:prefLabel>
      <rdfs:comment xml:lang="en">Textual description of the specific transaction conditions (purchasing, sales, payment) for an item. (epo-cat:CatalogueLine) </rdfs:comment>
      <skos:definition xml:lang="en">Textual description of the specific transaction conditions (purchasing, sales, payment) for an item. (epo-cat:CatalogueLine) </skos:definition>
      <rdfs:isDefinedBy rdf:resource="http://data.europa.eu/a4g/ontology"/>
   </owl:DatatypeProperty>
   <owl:DatatypeProperty rdf:about="http://data.europa.eu/a4g/ontology#hasBestBeforeDate">
      <rdfs:label xml:lang="en">Has best before date</rdfs:label>
      <skos:prefLabel xml:lang="en">Has best before date</skos:prefLabel>
      <rdfs:comment xml:lang="en">The day until which the quality of the item will remain optimal.

WG approval 10/03/2021 (epo-cat:Batch) </rdfs:comment>
      <skos:definition xml:lang="en">The day until which the quality of the item will remain optimal.

WG approval 10/03/2021 (epo-cat:Batch) </skos:definition>
      <rdfs:isDefinedBy rdf:resource="http://data.europa.eu/a4g/ontology"/>
   </owl:DatatypeProperty>
   <owl:DatatypeProperty rdf:about="http://data.europa.eu/a4g/ontology#hasExpiryDate">
      <rdfs:label xml:lang="en">Has expiry date</rdfs:label>
      <skos:prefLabel xml:lang="en">Has expiry date</skos:prefLabel>
      <rdfs:comment xml:lang="en">The last day until which the item can be used.

WG approval 10/03/2021
 (epo-cat:Batch) </rdfs:comment>
      <skos:definition xml:lang="en">The last day until which the item can be used.

WG approval 10/03/2021
 (epo-cat:Batch) </skos:definition>
      <rdfs:isDefinedBy rdf:resource="http://data.europa.eu/a4g/ontology"/>
   </owl:DatatypeProperty>
   <owl:DatatypeProperty rdf:about="http://data.europa.eu/a4g/ontology#hasDescription">
      <rdfs:label xml:lang="en">Has description</rdfs:label>
      <skos:prefLabel xml:lang="en">Has description</skos:prefLabel>
      <rdfs:comment xml:lang="en">Explanatory text about the instance of the concept.

WG Approval 30/09/2019 (epo-cat:Item) </rdfs:comment>
      <skos:definition xml:lang="en">Explanatory text about the instance of the concept.

WG Approval 30/09/2019 (epo-cat:Item) </skos:definition>
      <rdfs:isDefinedBy rdf:resource="http://data.europa.eu/a4g/ontology"/>
   </owl:DatatypeProperty>
   <owl:DatatypeProperty rdf:about="http://data.europa.eu/a4g/ontology#hasDimensionDescription">
      <rdfs:label xml:lang="en">Has dimension description</rdfs:label>
      <skos:prefLabel xml:lang="en">Has dimension description</skos:prefLabel>
      <rdfs:comment xml:lang="en">Textual description of the item's dimensions. (epo-cat:Item) </rdfs:comment>
      <skos:definition xml:lang="en">Textual description of the item's dimensions. (epo-cat:Item) </skos:definition>
      <rdfs:isDefinedBy rdf:resource="http://data.europa.eu/a4g/ontology"/>
   </owl:DatatypeProperty>
   <owl:DatatypeProperty rdf:about="http://data.europa.eu/a4g/ontology#hasExternalSpecification">
      <rdfs:label xml:lang="en">Has external specification</rdfs:label>
      <skos:prefLabel xml:lang="en">Has external specification</skos:prefLabel>
      <rdfs:comment xml:lang="en">URI reference to external item information or specifications, e.g. web address.

 (epo-cat:Item) </rdfs:comment>
      <skos:definition xml:lang="en">URI reference to external item information or specifications, e.g. web address.

 (epo-cat:Item) </skos:definition>
      <rdfs:isDefinedBy rdf:resource="http://data.europa.eu/a4g/ontology"/>
   </owl:DatatypeProperty>
   <owl:DatatypeProperty rdf:about="http://data.europa.eu/a4g/ontology#hasHazardousClass">
      <rdfs:label xml:lang="en">Has hazardous class</rdfs:label>
      <skos:prefLabel xml:lang="en">Has hazardous class</skos:prefLabel>
      <rdfs:comment xml:lang="en">Specification of the hazardous nature of an item according to a classification schema. Provides detail of the classification and nature of a hazardous item. (epo-cat:Item) </rdfs:comment>
      <skos:definition xml:lang="en">Specification of the hazardous nature of an item according to a classification schema. Provides detail of the classification and nature of a hazardous item. (epo-cat:Item) </skos:definition>
      <rdfs:isDefinedBy rdf:resource="http://data.europa.eu/a4g/ontology"/>
   </owl:DatatypeProperty>
   <owl:DatatypeProperty rdf:about="http://data.europa.eu/a4g/ontology#hasVATRate">
      <rdfs:label xml:lang="en">Has v a t rate</rdfs:label>
      <skos:prefLabel xml:lang="en">Has v a t rate</skos:prefLabel>
      <rdfs:comment xml:lang="en">Percentage of value-added tax of the item. (epo-cat:Item) </rdfs:comment>
      <skos:definition xml:lang="en">Percentage of value-added tax of the item. (epo-cat:Item) </skos:definition>
      <rdfs:isDefinedBy rdf:resource="http://data.europa.eu/a4g/ontology"/>
   </owl:DatatypeProperty>
   <owl:DatatypeProperty rdf:about="http://data.europa.eu/a4g/ontology#isInStock">
      <rdfs:label xml:lang="en">Is in stock</rdfs:label>
      <skos:prefLabel xml:lang="en">Is in stock</skos:prefLabel>
      <rdfs:comment xml:lang="en">Indicator whether an item is in the supplier's stock. If not in stock the supplier has to order the item. (epo-cat:Item) </rdfs:comment>
      <skos:definition xml:lang="en">Indicator whether an item is in the supplier's stock. If not in stock the supplier has to order the item. (epo-cat:Item) </skos:definition>
      <rdfs:isDefinedBy rdf:resource="http://data.europa.eu/a4g/ontology"/>
   </owl:DatatypeProperty>
   <owl:DatatypeProperty rdf:about="http://data.europa.eu/a4g/ontology#hasKeyword">
      <rdfs:label xml:lang="en">Has keyword</rdfs:label>
      <skos:prefLabel xml:lang="en">Has keyword</skos:prefLabel>
      <rdfs:comment xml:lang="en">List of words (e.g, synonyms) to make the item searchable. 

WG Approval 7/04/2022
 (epo-cat:Item) </rdfs:comment>
      <skos:definition xml:lang="en">List of words (e.g, synonyms) to make the item searchable. 

WG Approval 7/04/2022
 (epo-cat:Item) </skos:definition>
      <rdfs:isDefinedBy rdf:resource="http://data.europa.eu/a4g/ontology"/>
   </owl:DatatypeProperty>
</rdf:RDF>
